@base          <https://mmisw.org/ont/~draven/BarbaraNanning> .
@prefix :      <https://mmisw.org/ont/~draven/BarbaraNanning/> .
@prefix owl:   <http://www.w3.org/2002/07/owl#> .
@prefix rdf:   <http://www.w3.org/1999/02/22-rdf-syntax-ns#> .
@prefix xsd:   <http://www.w3.org/2001/XMLSchema#> .
@prefix rdfs:  <http://www.w3.org/2000/01/rdf-schema#> .
@prefix j.1:   <http://www.semanticweb.org/ontologies/Daan/2020/BarbaraNanning#Examining_Quality_(Final_Result)> .
@prefix j.0:   <http://www.semanticweb.org/ontologies/Daan/2020/BarbaraNanning#Examining_Quality_(Result)> .
@prefix j.3:   <http://www.semanticweb.org/ontologies/Daan/2020/BarbaraNanning#Examining_Quality_(Check_for_Irregularities_in_the_Glass)> .
@prefix j.2:   <http://www.semanticweb.org/ontologies/Daan/2020/BarbaraNanning#Examining_Quality_(Shape/Form)> .

:ARTWORK_75_PreparingGlass
        a                 :Preparing_Glass , owl:NamedIndividual ;
        rdfs:comment      "Instance of an activity which is part of the creation process of ARTWORK_75."@en ;
        rdfs:label        "ARTWORK_75_Preparing Glass"@en ;
        :Followed-By      :ARTWORK_75_SetupAndTestingOfTheMetalMold ;
        :Has-Duration     <http://www.semanticweb.org/ontologies/Daan/2020/BarbaraNanning#2018> ;
        :Involves         :BarbaraNanning , <http://www.semanticweb.org/ontologies/Daan/2020/BarbaraNanning#RadekKoten(CZ)> ;
        :Located-In       :CzechRepublic ;
        :Part-Of          :Creation_Artwork_75 ;
        :Requires-Use-Of  :Marver , :BlowingPipe , :Garage , :Pontis , :GloryHole ;
        :Starts           :Creation_Artwork_75 .

:Creation_Artwork_36  a  owl:NamedIndividual , :Creation_Event ;
        rdfs:comment    "Creation event for Artwork_36 by Barbara Nanning."@en ;
        rdfs:label      "Creation_Artwork_36"@en ;
        :Consists-Of    :ARTWORK_36_Packing_5 , :ARTWORK_36_TransportingColouredCanes , :ARTWORK_36_Sandblasting , :ARTWORK_36_ExaminingTheQualityOfTheGlass_2 , :ARTWORK_36_PreparingGlass , :ARTWORK_36_PreparingGlass_2 , :ARTWORK_36_Resting , :ARTWORK_36_FusingSheets , :ARTWORK_36_Modeling , :ARTWORK_36_Polishing , :ARTWORK_36_TackfusingColouredCanes , :ARTWORK_36_Photographing , :ARTWORK_36_TransportingColouredCanes_2 , <http://www.semanticweb.org/ontologies/Daan/2020/BarbaraNanning#ARTWORK_36_ExaminingQuality(CheckForIrregularitiesInTheGlass)_2> , :ARTWORK_36_CuttingSheets , :ARTWORK_36_Packing_4 , <http://www.semanticweb.org/ontologies/Daan/2020/BarbaraNanning#ARTWORK_36_ExaminingQuality(Result)_2> , <http://www.semanticweb.org/ontologies/Daan/2020/BarbaraNanning#ARTWORK_36_ExaminingQuality(FinalResult)_2> , :ARTWORK_36_Sensing_4 , :ARTWORK_36_ExaminingTheQualityOfTheGlass , :ARTWORK_36_Resting_2 , :ARTWORK_36_SetupAndTestingOfTheMetalMold , :ARTWORK_36_DecidingColourPalette_2 , :ARTWORK_36_Ordening , :ARTWORK_36_Cooling_2 , :ARTWORK_36_Documenting , :ARTWORK_36_Sawing , :ARTWORK_36_Documenting_2 , :ARTWORK_36_Cooling , :ARTWORK_36_Photographing_2 , :ARTWORK_36_Grinding , :ARTWORK_36_Packing_7 , :ARTWORK_36_Sawing_2 , :ARTWORK_36_FlatFusingSheetsWithARTWORK36PeacockToOnePanel , :ARTWORK_36_FillingKilnsWithMetalBowl_2 , :ARTWORK_36_TransportingMetalBowlWithCanes , :ARTWORK_36_Signing_2 , :ARTWORK_36_PreparingForBlowing , :ARTWORK_36_Transporting_4 , <http://www.semanticweb.org/ontologies/Daan/2020/BarbaraNanning#ARTWORK_36_ExaminingQuality(Result)> , :ARTWORK_36_ProducingColouredCanes , <http://www.semanticweb.org/ontologies/Daan/2020/BarbaraNanning#ARTWORK_36_ExaminingQuality(FinalResult)> , :ARTWORK_36_HeatingMetalMold , :ARTWORK_36_PickingUpColouredCanesPattern , :ARTWORK_36_SlumpingPanel , :ARTWORK_36_Transporting , :ARTWORK_36_DecidingColourPaletteAndPatterns_2 , :ARTWORK_36_Packing , :ARTWORK_36_Packing_3 , :ARTWORK_36_Grinding_2 , :ARTWORK_36_ApplyingMassivePieceOfClearGlass , :ARTWORK_36_Sensing_3 , <http://www.semanticweb.org/ontologies/Daan/2020/BarbaraNanning#ARTWORK_36_ExaminingQuality(CheckForIrregularitiesInTheGlass)> , :ARTWORK_36_DecidingColourPalette , :ARTWORK_36_ApplyingClearGlassBell , :ARTWORK_36_MakingPatternsWithColouredCanesInTheMetalBowl , :ARTWORK_36_Transporting_6 , :ARTWORK_36_Packing_6 , :ARTWORK_36_FillingKilnsWithMetalBowl , :ARTWORK_36_Polishing_2 , :ARTWORK_36_Transporting_3 , :ARTWORK_36_MeasuringAndBoxesMaking_2 , :ARTWORK_36_DecidingColourPaletteAndPatterns , :ARTWORK_36_TransportingMonochromeRods , :ARTWORK_36_CuttingAndPolishingCastedMonochromeSheetsToSmallRods , :ARTWORK_36_Transporting_2 , :ARTWORK_36_PreparingForBlowing_2 , :ARTWORK_36_CuttingAndPolishingColouredCanes , :ARTWORK_36_Glassblowing , :ARTWORK_36_Packing_2 , :ARTWORK_36_MeasuringAndBoxesMaking , :ARTWORK_36_Modeling_2 , :ARTWORK_36_FlatFusingFinishedArtwork , :ARTWORK_36_Sensing_2 , :ARTWORK_36_Casting , :ARTWORK_36_Packing_8 , :ARTWORK_36_PickingUpColouredPanel , <http://www.semanticweb.org/ontologies/Daan/2020/BarbaraNanning#ARTWORK_36_ExaminingQuality(Shape/Form)> , <http://www.semanticweb.org/ontologies/Daan/2020/BarbaraNanning#ARTWORK_36_ExaminingQuality(Shape/Form)_2> , :ARTWORK_36_OrdeningFlatSheets , :ARTWORK_36_TransportingMetalBowlWithPanel , :ARTWORK_36_Sensing , :ARTWORK_36_Signing , :ARTWORK_36_Transporting_5 , :ARTWORK_36_CuttingMonochromeSheets ;
        :Created        :Artwork_36 ;
        :Finishes-With  :ARTWORK_36_Documenting_2 ;
        :Starts-With    :ARTWORK_36_DecidingColourPaletteAndPatterns .

:ARTWORK_76_Transporting_2
        a              owl:NamedIndividual , :Transporting ;
        rdfs:comment   "Instance of an activity which is part of the creation process of ARTWORK_76."@en ;
        rdfs:label     "ARTWORK_76_Transporting_2"@en ;
        :Followed-By   :ARTWORK_76_Sandblasting ;
        :Follows       :ARTWORK_76_Packing_2 ;
        :Has-Duration  <http://www.semanticweb.org/ontologies/Daan/2020/BarbaraNanning#2018> ;
        :Involves      :AlešZvěřina , :BarbaraNanning ;
        :Located-In    :CzechRepublic ;
        :Part-Of       :Creation_Artwork_76 .

<http://data.beeldengeluid.nl/gtaa/34528>
        a           owl:NamedIndividual ;
        owl:sameAs  :Germany .

:ARTWORK_36_TackfusingColouredCanes
        a                 :Tackfusing_Coloured_Canes , owl:NamedIndividual ;
        rdfs:comment      "Instance of an activity which is part of the creation process of ARTWORK_36."@en ;
        rdfs:label        "ARTWORK_36_Tackfusing Coloured Canes"@en ;
        :Followed-By      :ARTWORK_36_TransportingMetalBowlWithCanes ;
        :Follows          :ARTWORK_36_MakingPatternsWithColouredCanesInTheMetalBowl ;
        :Has-Duration     <http://www.semanticweb.org/ontologies/Daan/2020/BarbaraNanning#2015> ;
        :Involves         :BarbaraNanning ;
        :Located-In       :Amsterdam ;
        :Part-Of          :Creation_Artwork_36 ;
        :Requires-Use-Of  :FusingKiln .

:Artwork  a              owl:Class ;
        rdfs:comment     "An artwork is an artistic work created by an artist (e.g. paintings)."@en ;
        rdfs:label       "Artwork"@en ;
        rdfs:subClassOf  :Thing .

:Created  a            owl:ObjectProperty ;
        rdfs:comment   "Created is a property of a thing connecting the thing with a Creation Event."@en ;
        rdfs:domain    :Creation_Event ;
        rdfs:label     "Created"@en ;
        rdfs:range     :Thing ;
        owl:inverseOf  :Created-By .

:ARTWORK_18_64_Packing_3
        a              owl:NamedIndividual , :Packing ;
        rdfs:comment   "Instance of an activity which is part of the creation process of ARTWORK_18_64."@en ;
        rdfs:label     "ARTWORK_18_64_Packing_3"@en ;
        :Followed-By   :ARTWORK_18_64_Documenting ;
        :Follows       :ARTWORK_18_64_Photographing ;
        :Has-Duration  <http://www.semanticweb.org/ontologies/Daan/2020/BarbaraNanning#2015> ;
        :Involves      :BarbaraNanning ;
        :Located-In    :Amsterdam ;
        :Part-Of       :Creation_Artwork_18_64 .

<http://www.cidoc-crm.org/cidoc-crm/E78_Collection>
        a                    owl:Class ;
        owl:equivalentClass  :Collection .

<http://vocab.getty.edu/aat/300025976>
        a                    owl:Class ;
        owl:equivalentClass  :Collection .

:ARTWORK_80_Packing_3
        a              owl:NamedIndividual , :Packing ;
        rdfs:comment   "Instance of an activity which is part of the creation process of ARTWORK_80."@en ;
        rdfs:label     "ARTWORK_80_Packing_3"@en ;
        :Followed-By   :ARTWORK_80_Transporting_3 ;
        :Follows       :ARTWORK_80_Signing ;
        :Has-Duration  <http://www.semanticweb.org/ontologies/Daan/2020/BarbaraNanning#2018> ;
        :Involves      :BarbaraNanning , :VáçlavNovák_Doksy_CzechRepublic , :AlešZvěřina ;
        :Located-In    :CzechRepublic ;
        :Part-Of       :Creation_Artwork_80 .

<http://www.wikidata.org/entity/Q2004>
        a       owl:NamedIndividual .

:ARTWORK_77_Modeling  a   owl:NamedIndividual , :Modeling ;
        rdfs:comment      "Instance of an activity which is part of the creation process of ARTWORK_77."@en ;
        rdfs:label        "ARTWORK_77_Modeling"@en ;
        :Followed-By      <http://www.semanticweb.org/ontologies/Daan/2020/BarbaraNanning#ARTWORK_77_ExaminingQuality(Shape/Form)> ;
        :Follows          :ARTWORK_77_Sensing ;
        :Has-Duration     <http://www.semanticweb.org/ontologies/Daan/2020/BarbaraNanning#2018> ;
        :Involves         <http://www.semanticweb.org/ontologies/Daan/2020/BarbaraNanning#LukasHavlas(CZ)> , :AssistantOfBarbara , <http://www.semanticweb.org/ontologies/Daan/2020/BarbaraNanning#JiriMoravec(CZ)> , <http://www.semanticweb.org/ontologies/Daan/2020/BarbaraNanning#Tom%C3%A1%C5%A1Moravec(CZ)> , :BarbaraNanning , <http://www.semanticweb.org/ontologies/Daan/2020/BarbaraNanning#RadekKoten(CZ)> ;
        :Located-In       :CzechRepublic ;
        :Part-Of          :Creation_Artwork_77 ;
        :Requires-Use-Of  :PropaneTorch , :InterchangeableMetalMoldSetup , :BlowingPipe , :AirCompressor , :Gloves .

:ARTWORK_36_Transporting_6
        a              :Transporting , owl:NamedIndividual ;
        rdfs:comment   "Instance of an activity which is part of the creation process of ARTWORK_36."@en ;
        rdfs:label     "ARTWORK_36_Transporting_6"@en ;
        :Followed-By   :ARTWORK_36_Photographing_2 ;
        :Follows       :ARTWORK_36_Packing_7 ;
        :Has-Duration  <http://www.semanticweb.org/ontologies/Daan/2020/BarbaraNanning#2019> ;
        :Involves      :BarbaraNanning , :AlešZvěřina ;
        :Located-In    :Amsterdam ;
        :Part-Of       :Creation_Artwork_36 .

<http://www.wikidata.org/entity/Q30>
        a       owl:NamedIndividual .

<http://vocab.getty.edu/aat/300011031>
        a           owl:NamedIndividual ;
        owl:sameAs  :Platinum .

:ARTWORK_44_Resting  a    owl:NamedIndividual , :Resting ;
        rdfs:comment      "Instance of an activity which is part of the creation process of ARTWORK_44."@en ;
        rdfs:label        "ARTWORK_44_Resting"@en ;
        :Followed-By      <http://www.semanticweb.org/ontologies/Daan/2020/BarbaraNanning#ARTWORK_44_ExaminingQuality(CheckForIrregularitiesInTheGlass)> ;
        :Follows          :ARTWORK_44_Transporting ;
        :Has-Duration     <http://www.semanticweb.org/ontologies/Daan/2020/BarbaraNanning#2018> ;
        :Involves         :AlešZvěřina ;
        :Located-In       :CzechRepublic ;
        :Part-Of          :Creation_Artwork_44 ;
        :Requires-Use-Of  :AnnealingKiln .

<http://vocab.getty.edu/aat/300022850>
        a           owl:NamedIndividual ;
        owl:sameAs  :BlowingPipe .

:ARTWORK_79_Packing_2
        a              owl:NamedIndividual , :Packing ;
        rdfs:comment   "Instance of an activity which is part of the creation process of ARTWORK_79."@en ;
        rdfs:label     "ARTWORK_79_Packing_2"@en ;
        :Followed-By   :ARTWORK_79_Transporting_2 ;
        :Follows       :ARTWORK_79_MeasuringAndBoxesMaking ;
        :Has-Duration  <http://www.semanticweb.org/ontologies/Daan/2020/BarbaraNanning#2018> ;
        :Involves      :BarbaraNanning , :AlešZvěřina ;
        :Located-In    :CzechRepublic ;
        :Part-Of       :Creation_Artwork_79 .

:Coesfeld  a          :City , owl:NamedIndividual ;
        rdfs:comment  "Coesfeld is a city in Germany."@en ;
        rdfs:label    "Coesfeld"@en ;
        owl:sameAs    <http://www.wikidata.org/entity/Q14914> ;
        :Located-In   :Germany ;
        :Location-Of  :GlasmuseumLette , :CollectionGlasmuseumLette , :Artwork_43 .

:Paper  a             owl:NamedIndividual , :Equipment ;
        rdfs:comment  "Paper is a material created from the pulp of wood which can be used for writing and wrapping."@en ;
        rdfs:label    "Paper"@en ;
        owl:sameAs    <http://www.wikidata.org/entity/Q11472> ;
        :Used-For     :ARTWORK_79_ApplyingExtraColour , :ARTWORK_76_ApplyingClearGlassBell , :ARTWORK_44_ApplyingClearGlassBell , :ARTWORK_44_ExaminingTheQualityOfTheGlass , :ARTWORK_75_ExaminingTheQualityOfTheGlass , :ARTWORK_77_ApplyingClearGlassBell , :ARTWORK_79_ApplyingClearGlassBell , :ARTWORK_78_Glassblowing , :ARTWORK_43_Glassblowing , :ARTWORK_78_ApplyingExtraColour , :ARTWORK_76_ExaminingTheQualityOfTheGlass , :ARTWORK_75_ApplyingClearGlassBell , :ARTWORK_77_ExaminingTheQualityOfTheGlass , :ARTWORK_74_ApplyingExtraColour_2 , :ARTWORK_75_ApplyingExtraColour_2 , :ARTWORK_74_ExaminingTheQualityOfTheGlass , :ARTWORK_75_ApplyingExtraColour , :ARTWORK_76_ApplyingExtraColour_2 , :ARTWORK_80_ApplyingClearGlassBell , :ARTWORK_74_ApplyingExtraColour , :ARTWORK_80_ApplyingExtraColour , :ARTWORK_77_ApplyingExtraColour , :ARTWORK_43_ApplyingExtraColour , :ARTWORK_78_ExaminingTheQualityOfTheGlass , :ARTWORK_73_ApplyingClearGlassBell , :ARTWORK_80_Glassblowing , :ARTWORK_74_Glassblowing , :ARTWORK_43_ApplyingClearGlassBell , :ARTWORK_77_Glassblowing , :ARTWORK_43_ExaminingTheQualityOfTheGlass , :ARTWORK_44_ApplyingExtraColour_2 , :ARTWORK_44_ApplyingExtraColour , :ARTWORK_78_ApplyingClearGlassBell , :ARTWORK_79_ApplyingExtraColour_2 , :ARTWORK_44_Glassblowing , :ARTWORK_79_ExaminingTheQualityOfTheGlass , :ARTWORK_73_ExaminingTheQualityOfTheGlass , :ARTWORK_74_ApplyingClearGlassBell , :ARTWORK_76_Glassblowing , :ARTWORK_80_ExaminingTheQualityOfTheGlass , :ARTWORK_79_Glassblowing , :ARTWORK_73_Glassblowing , :ARTWORK_75_Glassblowing , :ARTWORK_76_ApplyingExtraColour .

[ a            owl:AllDisjointClasses ;
  owl:members  ( :Artwork :Collection :Equipment :Material )
] .

:ARTWORK_75_Translocating
        a                 owl:NamedIndividual , :Translocating ;
        rdfs:comment      "Instance of an activity which is part of the creation process of ARTWORK_75."@en ;
        rdfs:label        "ARTWORK_75_Translocating"@en ;
        :Followed-By      :ARTWORK_75_Cooling ;
        :Follows          <http://www.semanticweb.org/ontologies/Daan/2020/BarbaraNanning#ARTWORK_75_ExaminingQuality(Shape/Form)> ;
        :Has-Duration     <http://www.semanticweb.org/ontologies/Daan/2020/BarbaraNanning#2018> ;
        :Involves         :BarbaraNanning ;
        :Located-In       :CzechRepublic ;
        :Part-Of          :Creation_Artwork_75 ;
        :Requires-Use-Of  :Fork .

:ARTWORK_44_Transporting
        a              owl:NamedIndividual , :Transporting ;
        rdfs:comment   "Instance of an activity which is part of the creation process of ARTWORK_44."@en ;
        rdfs:label     "ARTWORK_44_Transporting"@en ;
        :Followed-By   :ARTWORK_44_Resting ;
        :Follows       :ARTWORK_44_Packing ;
        :Has-Duration  <http://www.semanticweb.org/ontologies/Daan/2020/BarbaraNanning#2018> ;
        :Involves      :BarbaraNanning , :AlešZvěřina ;
        :Located-In    :CzechRepublic ;
        :Part-Of       :Creation_Artwork_44 .

:ARTWORK_73_Sawing  a     :Sawing , owl:NamedIndividual ;
        rdfs:comment      "Instance of an activity which is part of the creation process of ARTWORK_73."@en ;
        rdfs:label        "ARTWORK_73_Sawing"@en ;
        :Followed-By      :ARTWORK_73_Grinding ;
        :Follows          <http://www.semanticweb.org/ontologies/Daan/2020/BarbaraNanning#ARTWORK_73_ExaminingQuality(CheckForIrregularitiesInTheGlass)> ;
        :Has-Duration     <http://www.semanticweb.org/ontologies/Daan/2020/BarbaraNanning#2018> ;
        :Involves         :BarbaraNanning , :AlešZvěřina ;
        :Located-In       :CzechRepublic ;
        :Part-Of          :Creation_Artwork_73 ;
        :Requires-Use-Of  :DiamondSaw .

:Pontis  a            :Tool , owl:NamedIndividual ;
        rdfs:comment  "Pontis are used to take glass piece from the blowing pipe."@en ;
        rdfs:label    "Pontis"@en ;
        :Used-For     <http://www.semanticweb.org/ontologies/Daan/2020/BarbaraNanning#ARTWORK_79_ExaminingQuality(Shape/Form)> , :ARTWORK_44_ApplyingExtraColour , :ARTWORK_76_Glassblowing , :ARTWORK_80_ExaminingTheQualityOfTheGlass , :ARTWORK_74_ApplyingExtraColour_2 , :ARTWORK_75_ExaminingTheQualityOfTheGlass , :ARTWORK_43_ApplyingExtraColour , :ARTWORK_78_ExaminingTheQualityOfTheGlass , <http://www.semanticweb.org/ontologies/Daan/2020/BarbaraNanning#ARTWORK_73_ExaminingQuality(Shape/Form)> , :ARTWORK_75_ApplyingExtraColour , :ARTWORK_76_PreparingGlass , :ARTWORK_75_Glassblowing , :ARTWORK_79_ApplyingExtraColour , :ARTWORK_76_ApplyingExtraColour_2 , :ARTWORK_44_ApplyingExtraColour_2 , :ARTWORK_73_PreparingGlass , :ARTWORK_75_ApplyingExtraColour_2 , :ARTWORK_74_ExaminingTheQualityOfTheGlass , <http://www.semanticweb.org/ontologies/Daan/2020/BarbaraNanning#ARTWORK_80_ExaminingQuality(Shape/Form)> , <http://www.semanticweb.org/ontologies/Daan/2020/BarbaraNanning#ARTWORK_43_ExaminingQuality(Shape/Form)> , <http://www.semanticweb.org/ontologies/Daan/2020/BarbaraNanning#ARTWORK_74_ExaminingQuality(Shape/Form)> , :ARTWORK_77_PreparingGlass , :ARTWORK_73_Glassblowing , :ARTWORK_75_PreparingGlass , :ARTWORK_44_Glassblowing , :ARTWORK_74_Glassblowing , :ARTWORK_73_ExaminingTheQualityOfTheGlass , :ARTWORK_80_PreparingGlass , <http://www.semanticweb.org/ontologies/Daan/2020/BarbaraNanning#ARTWORK_76_ExaminingQuality(Shape/Form)> , :ARTWORK_76_ExaminingTheQualityOfTheGlass , <http://www.semanticweb.org/ontologies/Daan/2020/BarbaraNanning#ARTWORK_75_ExaminingQuality(Shape/Form)> , :ARTWORK_76_ApplyingExtraColour , :ARTWORK_79_ApplyingExtraColour_2 , :ARTWORK_79_Glassblowing , <http://www.semanticweb.org/ontologies/Daan/2020/BarbaraNanning#ARTWORK_44_ExaminingQuality(Shape/Form)> , :ARTWORK_74_ApplyingExtraColour , :ARTWORK_78_ApplyingExtraColour , :ARTWORK_78_PreparingGlass , :ARTWORK_77_ApplyingExtraColour , <http://www.semanticweb.org/ontologies/Daan/2020/BarbaraNanning#ARTWORK_78_ExaminingQuality(Shape/Form)> , :ARTWORK_44_PreparingGlass , :ARTWORK_77_ExaminingTheQualityOfTheGlass , :ARTWORK_79_ExaminingTheQualityOfTheGlass , <http://www.semanticweb.org/ontologies/Daan/2020/BarbaraNanning#ARTWORK_77_ExaminingQuality(Shape/Form)> , :ARTWORK_74_PreparingGlass , :ARTWORK_80_ApplyingExtraColour , :ARTWORK_44_ExaminingTheQualityOfTheGlass , :ARTWORK_43_PreparingGlass , :ARTWORK_43_ExaminingTheQualityOfTheGlass , :ARTWORK_43_Glassblowing , :ARTWORK_80_Glassblowing , :ARTWORK_78_Glassblowing , :ARTWORK_77_Glassblowing , :ARTWORK_79_PreparingGlass .

:ARTWORK_39_Packing_3
        a              :Packing , owl:NamedIndividual ;
        rdfs:comment   "Instance of an activity which is part of the creation process of ARTWORK_39."@en ;
        rdfs:label     "ARTWORK_39_Packing_3"@en ;
        :Followed-By   :ARTWORK_39_Documenting ;
        :Follows       :ARTWORK_39_Photographing ;
        :Has-Duration  <http://www.semanticweb.org/ontologies/Daan/2020/BarbaraNanning#2015> ;
        :Involves      :BarbaraNanning ;
        :Located-In    :Amsterdam ;
        :Part-Of       :Creation_Artwork_39 .

:ARTWORK_73_ApplyingClearGlassBell
        a                 :Applying_Clear_Glass_Bell , owl:NamedIndividual ;
        rdfs:comment      "Instance of an activity which is part of the creation process of ARTWORK_73."@en ;
        rdfs:label        "ARTWORK_73_Applying Clear Glass Bell"@en ;
        :Followed-By      :ARTWORK_73_HeatingMetalMold ;
        :Follows          :ARTWORK_73_SetupAndTestingOfTheMetalMold_2 ;
        :Has-Duration     <http://www.semanticweb.org/ontologies/Daan/2020/BarbaraNanning#2018> ;
        :Involves         <http://www.semanticweb.org/ontologies/Daan/2020/BarbaraNanning#LukasHavlas(CZ)> , :BarbaraNanning , <http://www.semanticweb.org/ontologies/Daan/2020/BarbaraNanning#RadekKoten(CZ)> ;
        :Located-In       :CzechRepublic ;
        :Part-Of          :Creation_Artwork_73 ;
        :Processes        :AJETOClearGlass ;
        :Requires-Use-Of  :CeramicPotFilledWithGlass , :YokeOfSupport , :Marver , :Beeswax , :Blocks , :Paper , :Water , :StraightShears , :DiamondShears , :Furnace , :BlowingPipe , :AirCompressor , :Jacks , :Pincet , :IcePick , :Hook .

<http://www.semanticweb.org/ontologies/Daan/2020/BarbaraNanning#ARTWORK_74_ExaminingQuality(Result)>
        a              j.0: , owl:NamedIndividual ;
        rdfs:comment   "Instance of an activity which is part of the creation process of ARTWORK_74."@en ;
        rdfs:label     "ARTWORK_74_Examining Quality (Result)"@en ;
        :Followed-By   :ARTWORK_74_Packing_2 ;
        :Follows       :ARTWORK_74_Polishing ;
        :Has-Duration  <http://www.semanticweb.org/ontologies/Daan/2020/BarbaraNanning#2008> ;
        :Involves      :AlešZvěřina , :BarbaraNanning ;
        :Located-In    :CzechRepublic ;
        :Part-Of       :Creation_Artwork_74 .

:ARTWORK_78_Packing_5
        a              owl:NamedIndividual , :Packing ;
        rdfs:comment   "Instance of an activity which is part of the creation process of ARTWORK_78."@en ;
        rdfs:label     "ARTWORK_78_Packing_5"@en ;
        :Finishes      :Creation_Artwork_78 ;
        :Follows       :ARTWORK_78_Documenting ;
        :Has-Duration  <http://www.semanticweb.org/ontologies/Daan/2020/BarbaraNanning#2008> ;
        :Involves      :BarbaraNanning ;
        :Located-In    :CzechRepublic ;
        :Part-Of       :Creation_Artwork_78 .

:ARTWORK_73_Signing  a    owl:NamedIndividual , :Signing ;
        rdfs:comment      "Instance of an activity which is part of the creation process of ARTWORK_73."@en ;
        rdfs:label        "ARTWORK_73_Signing"@en ;
        :Followed-By      :ARTWORK_73_Packing_3 ;
        :Follows          :ARTWORK_73_Sandblasting ;
        :Has-Duration     <http://www.semanticweb.org/ontologies/Daan/2020/BarbaraNanning#2018> ;
        :Involves         :AlešZvěřina , :BarbaraNanning ;
        :Located-In       :CzechRepublic ;
        :Part-Of          :Creation_Artwork_73 ;
        :Requires-Use-Of  :AirCompressor .

:ARTWORK_73_Gilding  a    owl:NamedIndividual , :Gilding ;
        rdfs:comment      "Instance of an activity which is part of the creation process of ARTWORK_73."@en ;
        rdfs:label        "ARTWORK_73_Gilding"@en ;
        :Followed-By      <http://www.semanticweb.org/ontologies/Daan/2020/BarbaraNanning#ARTWORK_73_ExaminingQuality(FinalResult)> ;
        :Follows          :ARTWORK_73_Transporting_3 ;
        :Has-Duration     <http://www.semanticweb.org/ontologies/Daan/2020/BarbaraNanning#2018> ;
        :Involves         :BarbaraNanning , :VáçlavNovák_Doksy_CzechRepublic ;
        :Located-In       :CzechRepublic ;
        :Part-Of          :Creation_Artwork_73 ;
        :Requires-Use-Of  :GildersKnife , :GildingCushion , :INSTACOLLTool , :GildersTip .

:ARTWORK_80_Signing  a    owl:NamedIndividual , :Signing ;
        rdfs:comment      "Instance of an activity which is part of the creation process of ARTWORK_80."@en ;
        rdfs:label        "ARTWORK_80_Signing"@en ;
        :Followed-By      :ARTWORK_80_Packing_3 ;
        :Follows          :ARTWORK_80_Sandblasting ;
        :Has-Duration     <http://www.semanticweb.org/ontologies/Daan/2020/BarbaraNanning#2018> ;
        :Involves         :AlešZvěřina , :BarbaraNanning ;
        :Located-In       :CzechRepublic ;
        :Part-Of          :Creation_Artwork_80 ;
        :Requires-Use-Of  :AirCompressor .

:ARTWORK_80_Gilding  a    :Gilding , owl:NamedIndividual ;
        rdfs:comment      "Instance of an activity which is part of the creation process of ARTWORK_80."@en ;
        rdfs:label        "ARTWORK_80_Gilding"@en ;
        :Followed-By      <http://www.semanticweb.org/ontologies/Daan/2020/BarbaraNanning#ARTWORK_80_ExaminingQuality(FinalResult)> ;
        :Follows          :ARTWORK_80_Transporting_3 ;
        :Has-Duration     <http://www.semanticweb.org/ontologies/Daan/2020/BarbaraNanning#2018> ;
        :Involves         :BarbaraNanning , :VáçlavNovák_Doksy_CzechRepublic ;
        :Located-In       :CzechRepublic ;
        :Part-Of          :Creation_Artwork_80 ;
        :Requires-Use-Of  :INSTACOLLTool , :GildingCushion , :GildersKnife , :GildersTip .

:ARTWORK_18_64_ExaminingTheQualityOfTheGlass
        a                 :Examining_the_Quality_of_the_Glass , owl:NamedIndividual ;
        rdfs:comment      "Instance of an activity which is part of the creation process of ARTWORK_18_64."@en ;
        rdfs:label        "ARTWORK_18_64_Examining the Quality of the Glass"@en ;
        :Followed-By      :ARTWORK_18_64_ApplyingClearGlassBell ;
        :Follows          :ARTWORK_18_64_PreparingForBlowing ;
        :Has-Duration     <http://www.semanticweb.org/ontologies/Daan/2020/BarbaraNanning#2015> ;
        :Involves         <http://www.semanticweb.org/ontologies/Daan/2020/BarbaraNanning#JiriPacinek(CZ)> , :BarbaraNanning ;
        :Located-In       :Lindava ;
        :Part-Of          :Creation_Artwork_18_64 ;
        :Requires-Use-Of  :BlowingPipe , :Water , :GloryHole , :StraightShears , :Blocks , :Pontis , :Furnace , :Jacks , :CeramicPotFilledWithGlass , :YokeOfSupport , :DiamondShears , :AnnealingKiln , :Paper .

<http://www.wikidata.org/entity/Q1021090>
        a       owl:NamedIndividual .

<http://www.semanticweb.org/ontologies/Daan/2020/BarbaraNanning#StudioVogl(CZ)>
        a             owl:NamedIndividual , :Metal_Worker_3 ;
        rdfs:comment  "Studio Vogl (CZ) is a Metal Worker 3."@en ;
        rdfs:label    "Studio Vogl (CZ)"@en .

:Maintains  a         owl:ObjectProperty ;
        rdfs:comment  "Maintains is a property which connects a thing with an actor who Maintains the thing in question."@en ;
        rdfs:domain   :Actor ;
        rdfs:label    "Maintains"@en ;
        rdfs:range    :Thing .

:ARTWORK_36_Cooling  a    owl:NamedIndividual , :Cooling ;
        rdfs:comment      "Instance of an activity which is part of the creation process of ARTWORK_36."@en ;
        rdfs:label        "ARTWORK_36_Cooling"@en ;
        :Followed-By      :ARTWORK_36_Packing ;
        :Follows          <http://www.semanticweb.org/ontologies/Daan/2020/BarbaraNanning#ARTWORK_36_ExaminingQuality(Shape/Form)> ;
        :Has-Duration     <http://www.semanticweb.org/ontologies/Daan/2020/BarbaraNanning#2015> ;
        :Involves         <http://www.semanticweb.org/ontologies/Daan/2020/BarbaraNanning#JessicaHomich(USA)> , :DurkValkema , <http://www.semanticweb.org/ontologies/Daan/2020/BarbaraNanning#MiaLerssi(DN)> ;
        :Located-In       :Zaandam ;
        :Part-Of          :Creation_Artwork_36 ;
        :Requires-Use-Of  :AnnealingKiln .

:ARTWORK_44_ApplyingExtraColour_2
        a                 owl:NamedIndividual , :Applying_Extra_Colour ;
        rdfs:comment      "Instance of an activity which is part of the creation process of ARTWORK_44."@en ;
        rdfs:label        "ARTWORK_44_Applying Extra Colour_2"@en ;
        :Followed-By      :ARTWORK_44_HeatingMetalMold ;
        :Follows          :ARTWORK_44_ApplyingExtraColour ;
        :Has-Duration     <http://www.semanticweb.org/ontologies/Daan/2020/BarbaraNanning#2018> ;
        :Involves         <http://www.semanticweb.org/ontologies/Daan/2020/BarbaraNanning#RadekKoten(CZ)> , <http://www.semanticweb.org/ontologies/Daan/2020/BarbaraNanning#LukasHavlas(CZ)> , :BarbaraNanning ;
        :Located-In       :CzechRepublic ;
        :Part-Of          :Creation_Artwork_44 ;
        :Processes        :AJETOAlexandriteGlass ;
        :Requires-Use-Of  :DiamondShears , :Hook , :AnnealingKiln , :Jacks , :Blocks , :Paper , :Marver , :Fork , :Tagliol , :CeramicPotFilledWithGlass , :Pontis , :Furnace , :GloryHole , :Pincet , :Water , :Garage , :StraightShears , :Beeswax , :YokeOfSupport , :AirCompressor , :BlowingPipe , :IcePick .

:ARTWORK_43_Cooling  a    owl:NamedIndividual , :Cooling ;
        rdfs:comment      "Instance of an activity which is part of the creation process of ARTWORK_43."@en ;
        rdfs:label        "ARTWORK_43_Cooling"@en ;
        :Followed-By      :ARTWORK_43_Packing ;
        :Follows          :ARTWORK_43_Translocating ;
        :Has-Duration     <http://www.semanticweb.org/ontologies/Daan/2020/BarbaraNanning#2008> ;
        :Involves         :AssistantOfBarbara , :LuděkKout ;
        :Located-In       :CzechRepublic ;
        :Part-Of          :Creation_Artwork_43 ;
        :Requires-Use-Of  :AnnealingKiln .

<http://www.wikidata.org/entity/Q978234>
        a       owl:NamedIndividual .

:ARTWORK_39_ApplyingClearGlassBell
        a                 owl:NamedIndividual , :Applying_Clear_Glass_Bell ;
        rdfs:comment      "Instance of an activity which is part of the creation process of ARTWORK_39."@en ;
        rdfs:label        "ARTWORK_39_Applying Clear Glass Bell"@en ;
        :Followed-By      :ARTWORK_39_PickingUpColouredPanel ;
        :Follows          :ARTWORK_39_ExaminingTheQualityOfTheGlass ;
        :Has-Duration     <http://www.semanticweb.org/ontologies/Daan/2020/BarbaraNanning#2015> ;
        :Involves         :BarbaraNanning , :GertBullée , <http://www.semanticweb.org/ontologies/Daan/2020/BarbaraNanning#MarekBrathko(CZ)> ;
        :Located-In       :Zaandam ;
        :Part-Of          :Creation_Artwork_39 ;
        :Requires-Use-Of  :Pincet , :Marver , :Beeswax , :CeramicPotFilledWithGlass , :AirCompressor , :BlowingPipe , :StraightShears , :Jacks , :IcePick , :Blocks , :DiamondShears , :Water , :Hook , :Furnace , :Paper , :YokeOfSupport .

:BoneMeal  a              :Man-Made_Material , owl:NamedIndividual ;
        rdfs:comment      "Bone meal is a material created by grinding animal bones."@en ;
        rdfs:label        "Bone Meal"@en ;
        owl:sameAs        <http://www.wikidata.org/entity/Q72451031> ;
        :Is-Processed-In  :AJETOWhiteGlass .

<http://www.semanticweb.org/ontologies/Daan/2020/BarbaraNanning#ARTWORK_76_ExaminingQuality(Shape/Form)>
        a                 j.2: , owl:NamedIndividual ;
        rdfs:comment      "Instance of an activity which is part of the creation process of ARTWORK_76."@en ;
        rdfs:label        "ARTWORK_76_Examining Quality (Shape/Form)"@en ;
        :Followed-By      :ARTWORK_76_Translocating ;
        :Follows          :ARTWORK_76_Modeling ;
        :Has-Duration     <http://www.semanticweb.org/ontologies/Daan/2020/BarbaraNanning#2018> ;
        :Involves         <http://www.semanticweb.org/ontologies/Daan/2020/BarbaraNanning#RadekKoten(CZ)> , :BarbaraNanning , :LuděkKout ;
        :Located-In       :CzechRepublic ;
        :Part-Of          :Creation_Artwork_76 ;
        :Requires-Use-Of  :BlowingPipe , :Pontis , :GloryHole .

:ARTWORK_39_Slumping  a   :Slumping , owl:NamedIndividual ;
        rdfs:comment      "Instance of an activity which is part of the creation process of ARTWORK_39."@en ;
        rdfs:label        "ARTWORK_39_Slumping"@en ;
        :Followed-By      :ARTWORK_39_TransportingMetalBowlWithPanel ;
        :Follows          :ARTWORK_39_FusingSheetsAndStrings ;
        :Has-Duration     <http://www.semanticweb.org/ontologies/Daan/2020/BarbaraNanning#2015> ;
        :Involves         :BarbaraNanning ;
        :Located-In       :Amsterdam ;
        :Part-Of          :Creation_Artwork_39 ;
        :Requires-Use-Of  :FusingKiln .

:ARTWORK_74_Translocating
        a                 owl:NamedIndividual , :Translocating ;
        rdfs:comment      "Instance of an activity which is part of the creation process of ARTWORK_74."@en ;
        rdfs:label        "ARTWORK_74_Translocating"@en ;
        :Followed-By      :ARTWORK_74_Cooling ;
        :Follows          <http://www.semanticweb.org/ontologies/Daan/2020/BarbaraNanning#ARTWORK_74_ExaminingQuality(Shape/Form)> ;
        :Has-Duration     <http://www.semanticweb.org/ontologies/Daan/2020/BarbaraNanning#2008> ;
        :Involves         :BarbaraNanning ;
        :Located-In       :CzechRepublic ;
        :Part-Of          :Creation_Artwork_74 ;
        :Requires-Use-Of  :Fork .

:ARTWORK_17_33_Sawing
        a                 :Sawing , owl:NamedIndividual ;
        rdfs:comment      "Instance of an activity which is part of the creation process of ARTWORK_17_33."@en ;
        rdfs:label        "ARTWORK_17_33_Sawing"@en ;
        :Followed-By      :ARTWORK_17_33_Sensing_2 ;
        :Follows          <http://www.semanticweb.org/ontologies/Daan/2020/BarbaraNanning#ARTWORK_17_33_ExaminingQuality(CheckForIrregularitiesInTheGlass)> ;
        :Has-Duration     <http://www.semanticweb.org/ontologies/Daan/2020/BarbaraNanning#2017> ;
        :Involves         :BarbaraNanning , :AlešZvěřina ;
        :Located-In       :NovyBor ;
        :Part-Of          :Creation_Artwork_17_33 ;
        :Requires-Use-Of  :DiamondSaw .

:ARTWORK_79_Transporting_4
        a              :Transporting , owl:NamedIndividual ;
        rdfs:comment   "Instance of an activity which is part of the creation process of ARTWORK_79."@en ;
        rdfs:label     "ARTWORK_79_Transporting_4"@en ;
        :Followed-By   :ARTWORK_79_Photographing ;
        :Follows       :ARTWORK_79_Packing_4 ;
        :Has-Duration  <http://www.semanticweb.org/ontologies/Daan/2020/BarbaraNanning#2018> ;
        :Involves      :BarbaraNanning , :AlešZvěřina ;
        :Located-In    :CzechRepublic ;
        :Part-Of       :Creation_Artwork_79 .

:ARTWORK_79_ExaminingTheQualityOfTheGlass
        a                 :Examining_the_Quality_of_the_Glass , owl:NamedIndividual ;
        rdfs:comment      "Instance of an activity which is part of the creation process of ARTWORK_79."@en ;
        rdfs:label        "ARTWORK_79_Examining the Quality of the Glass"@en ;
        :Followed-By      :ARTWORK_79_Cooling ;
        :Follows          :ARTWORK_79_Modeling ;
        :Has-Duration     <http://www.semanticweb.org/ontologies/Daan/2020/BarbaraNanning#2018> ;
        :Involves         <http://www.semanticweb.org/ontologies/Daan/2020/BarbaraNanning#RadekKoten(CZ)> , :LuděkKout , :BarbaraNanning ;
        :Located-In       :CzechRepublic ;
        :Part-Of          :Creation_Artwork_79 ;
        :Requires-Use-Of  :Blocks , :CeramicPotFilledWithGlass , :YokeOfSupport , :Paper , :Water , :AnnealingKiln , :GloryHole , :DiamondShears , :Furnace , :StraightShears , :BlowingPipe , :Jacks , :Pontis .

:Transporting_Metal_Bowl_with_Panel
        a                owl:Class ;
        rdfs:comment     "Moving said objects from one place to another"@en ;
        rdfs:label       "Transporting Metal Bowl with Panel"@en ;
        rdfs:subClassOf  :Transporting .

:Location-Of  a       owl:ObjectProperty ;
        rdfs:comment  "Location-Of is a property of a location, thing, organisation or event connecting it to a specific location."@en ;
        rdfs:domain   :Place ;
        rdfs:label    "Location-Of"@en ;
        rdfs:range    :Thing , :Place , :Organisation , :Event .

:ARTWORK_36_Grinding_2
        a                 :Grinding , owl:NamedIndividual ;
        rdfs:comment      "Instance of an activity which is part of the creation process of ARTWORK_36."@en ;
        rdfs:label        "ARTWORK_36_Grinding_2"@en ;
        :Followed-By      :ARTWORK_36_Polishing_2 ;
        :Follows          :ARTWORK_36_Sensing_4 ;
        :Has-Duration     <http://www.semanticweb.org/ontologies/Daan/2020/BarbaraNanning#2019> ;
        :Involves         :RobertFlorian , :BarbaraNanning , :AlešZvěřina ;
        :Located-In       :NovyBor ;
        :Part-Of          :Creation_Artwork_36 ;
        :Requires-Use-Of  :GrindingWheel , :SharpeningStone .

:ARTWORK_18_64_TransportingColouredCanes
        a              owl:NamedIndividual , :Transporting_Coloured_Canes ;
        rdfs:comment   "Instance of an activity which is part of the creation process of ARTWORK_18_64."@en ;
        rdfs:label     "ARTWORK_18_64_Transporting Coloured Canes"@en ;
        :Followed-By   :ARTWORK_18_64_CuttingAndPolishingColouredCanes ;
        :Follows       :ARTWORK_18_64_ProducingColouredCanes ;
        :Has-Duration  <http://www.semanticweb.org/ontologies/Daan/2020/BarbaraNanning#2015> ;
        :Involves      :BarbaraNanning ;
        :Located-In    :Zaandam ;
        :Part-Of       :Creation_Artwork_18_64 .

:ARTWORK_73_HeatingMetalMold
        a                 owl:NamedIndividual , :Heating_Metal_Mold ;
        rdfs:comment      "Instance of an activity which is part of the creation process of ARTWORK_73."@en ;
        rdfs:label        "ARTWORK_73_Heating Metal Mold"@en ;
        :Followed-By      :ARTWORK_73_Glassblowing ;
        :Follows          :ARTWORK_73_ApplyingClearGlassBell ;
        :Has-Duration     <http://www.semanticweb.org/ontologies/Daan/2020/BarbaraNanning#2018> ;
        :Involves         :BarbaraNanning ;
        :Located-In       :CzechRepublic ;
        :Part-Of          :Creation_Artwork_73 ;
        :Requires-Use-Of  :PropaneTorch , :Gloves , :InterchangeableMetalMoldSetup .

:ARTWORK_43_Resting  a    :Resting , owl:NamedIndividual ;
        rdfs:comment      "Instance of an activity which is part of the creation process of ARTWORK_43."@en ;
        rdfs:label        "ARTWORK_43_Resting"@en ;
        :Followed-By      <http://www.semanticweb.org/ontologies/Daan/2020/BarbaraNanning#ARTWORK_43_ExaminingQuality(CheckForIrregularitiesInTheGlass)> ;
        :Follows          :ARTWORK_43_Transporting ;
        :Has-Duration     <http://www.semanticweb.org/ontologies/Daan/2020/BarbaraNanning#2008> ;
        :Involves         :AlešZvěřina ;
        :Located-In       :CzechRepublic ;
        :Part-Of          :Creation_Artwork_43 ;
        :Requires-Use-Of  :AnnealingKiln .

:Tackfusing_Coloured_Canes
        a                owl:Class ;
        rdfs:comment     "After a patern of canes has been placed in a metal form it will be placed in the kiln to be fused together before use by the glassblower for the final object."@en ;
        rdfs:label       "Tackfusing Coloured Canes"@en ;
        rdfs:subClassOf  :Activity .

:ARTWORK_76_MeasuringAndBoxesMaking
        a              owl:NamedIndividual , :Measuring_and_Boxes_Making ;
        rdfs:comment   "Instance of an activity which is part of the creation process of ARTWORK_76."@en ;
        rdfs:label     "ARTWORK_76_Measuring and Boxes Making"@en ;
        :Followed-By   :ARTWORK_76_Packing_2 ;
        :Follows       <http://www.semanticweb.org/ontologies/Daan/2020/BarbaraNanning#ARTWORK_76_ExaminingQuality(CheckForIrregularitiesInTheGlass)_2> ;
        :Has-Duration  <http://www.semanticweb.org/ontologies/Daan/2020/BarbaraNanning#2018> ;
        :Involves      :BarbaraNanning , :AlešZvěřina ;
        :Located-In    :CzechRepublic ;
        :Part-Of       :Creation_Artwork_76 .

<http://vocab.getty.edu/aat/300189326>
        a                    owl:Class ;
        owl:equivalentClass  :Signing .

:ARTWORK_79_Documenting
        a              owl:NamedIndividual , :Documenting ;
        rdfs:comment   "Instance of an activity which is part of the creation process of ARTWORK_79."@en ;
        rdfs:label     "ARTWORK_79_Documenting"@en ;
        :Followed-By   :ARTWORK_79_Packing_5 ;
        :Follows       :ARTWORK_79_Photographing ;
        :Has-Duration  <http://www.semanticweb.org/ontologies/Daan/2020/BarbaraNanning#2018> ;
        :Involves      :BarbaraNanning ;
        :Located-In    :CzechRepublic ;
        :Part-Of       :Creation_Artwork_79 .

<http://www.semanticweb.org/ontologies/Daan/2020/BarbaraNanning#ARTWORK_75_ExaminingQuality(Result)>
        a              owl:NamedIndividual , j.0: ;
        rdfs:comment   "Instance of an activity which is part of the creation process of ARTWORK_75."@en ;
        rdfs:label     "ARTWORK_75_Examining Quality (Result)"@en ;
        :Followed-By   :ARTWORK_75_Packing_2 ;
        :Follows       :ARTWORK_75_Polishing ;
        :Has-Duration  <http://www.semanticweb.org/ontologies/Daan/2020/BarbaraNanning#2017> ;
        :Involves      :BarbaraNanning , :AlešZvěřina ;
        :Located-In    :CzechRepublic ;
        :Part-Of       :Creation_Artwork_75 .

:ARTWORK_74_Packing_2
        a              owl:NamedIndividual , :Packing ;
        rdfs:comment   "Instance of an activity which is part of the creation process of ARTWORK_74."@en ;
        rdfs:label     "ARTWORK_74_Packing_2"@en ;
        :Followed-By   :ARTWORK_74_Transporting_2 ;
        :Follows       <http://www.semanticweb.org/ontologies/Daan/2020/BarbaraNanning#ARTWORK_74_ExaminingQuality(Result)> ;
        :Has-Duration  <http://www.semanticweb.org/ontologies/Daan/2020/BarbaraNanning#2008> ;
        :Involves      :BarbaraNanning , :AlešZvěřina ;
        :Located-In    :CzechRepublic ;
        :Part-Of       :Creation_Artwork_74 .

:ARTWORK_17_33_FillingHolesWithClearGlass
        a              owl:NamedIndividual , :Filling_Holes_with_Clear_Glass ;
        rdfs:comment   "Instance of an activity which is part of the creation process of ARTWORK_17_33."@en ;
        rdfs:label     "ARTWORK_17_33_Filling Holes with Clear Glass"@en ;
        :Followed-By   :ARTWORK_17_33_ApplyingClearOverlay ;
        :Follows       :ARTWORK_17_33_ModelingWithTeflonStick ;
        :Has-Duration  <http://www.semanticweb.org/ontologies/Daan/2020/BarbaraNanning#2017> ;
        :Involves      <http://www.semanticweb.org/ontologies/Daan/2020/BarbaraNanning#RadekKoten(CZ)> , <http://www.semanticweb.org/ontologies/Daan/2020/BarbaraNanning#JiriMoravec(CZ)> , <http://www.semanticweb.org/ontologies/Daan/2020/BarbaraNanning#LukasHavlas(CZ)> , :AssistantOfBarbara , <http://www.semanticweb.org/ontologies/Daan/2020/BarbaraNanning#Tom%C3%A1%C5%A1Moravec(CZ)> , :BarbaraNanning , <http://www.semanticweb.org/ontologies/Daan/2020/BarbaraNanning#JessicaHomich(USA)> ;
        :Located-In    :Lindava ;
        :Part-Of       :Creation_Artwork_17_33 .

:Making_Patterns_with_Coloured_Canes_in_the_Metal_Bowl
        a                owl:Class ;
        rdfs:comment     "With the canes and strings I build up the colour patterns in releasing, stainless steel bowls. A colour pattern emerges by stacking hundreds of shortened glass threads against the inner wall of the bowl, and then to smoothly melt them. Using canes and strings of various length they are placed meticulously inside a  bowl creating a design that is later used by the glassblower to create the finished object."@en ;
        rdfs:label       "Making Patterns with Coloured Canes in the Metal Bowl"@en ;
        rdfs:subClassOf  :Activity .

:ARTWORK_75_Transporting_2
        a              owl:NamedIndividual , :Transporting ;
        rdfs:comment   "Instance of an activity which is part of the creation process of ARTWORK_75."@en ;
        rdfs:label     "ARTWORK_75_Transporting_2"@en ;
        :Followed-By   :ARTWORK_75_Sandblasting ;
        :Follows       :ARTWORK_75_Packing_2 ;
        :Has-Duration  <http://www.semanticweb.org/ontologies/Daan/2020/BarbaraNanning#2018> ;
        :Involves      :BarbaraNanning , :AlešZvěřina ;
        :Located-In    :CzechRepublic ;
        :Part-Of       :Creation_Artwork_75 .

<http://www.semanticweb.org/ontologies/Daan/2020/BarbaraNanning#JaroslavSvacha(CZ)>
        a             owl:NamedIndividual , :Grinder_1 ;
        rdfs:comment  "Jaroslav Svacha (CZ) is a Grinder 1."@en ;
        rdfs:label    "Jaroslav Svacha (CZ)"@en ;
        :Involved-In  :ARTWORK_46_TransportingMonochromeRods , :ARTWORK_36_TransportingMonochromeRods , :ARTWORK_18_64_TransportingMonochromeRods ;
        :Works-For    <http://www.semanticweb.org/ontologies/Daan/2020/BarbaraNanning#BullseyeGlassTGKJaroslavSvacha(CZ)> .

:ARTWORK_36_ExaminingTheQualityOfTheGlass_2
        a                 owl:NamedIndividual , :Examining_the_Quality_of_the_Glass ;
        rdfs:comment      "Instance of an activity which is part of the creation process of ARTWORK_36."@en ;
        rdfs:label        "ARTWORK_36_Examining the Quality of the Glass_2"@en ;
        :Followed-By      :ARTWORK_36_ApplyingMassivePieceOfClearGlass ;
        :Follows          :ARTWORK_36_PreparingGlass_2 ;
        :Has-Duration     <http://www.semanticweb.org/ontologies/Daan/2020/BarbaraNanning#2019> ;
        :Involves         :BarbaraNanning , <http://www.semanticweb.org/ontologies/Daan/2020/BarbaraNanning#JiriPacinek(CZ)> ;
        :Located-In       :Lindava ;
        :Part-Of          :Creation_Artwork_36 ;
        :Requires-Use-Of  :Furnace , :Pontis , :GloryHole , :Jacks , :Blocks , :DiamondShears , :StraightShears , :AnnealingKiln , :CeramicPotFilledWithGlass , :YokeOfSupport , :Paper , :Water , :BlowingPipe .

:ARTWORK_73_Packing_5
        a              owl:NamedIndividual , :Packing ;
        rdfs:comment   "Instance of an activity which is part of the creation process of ARTWORK_73."@en ;
        rdfs:label     "ARTWORK_73_Packing_5"@en ;
        :Finishes      :Creation_Artwork_73 ;
        :Follows       :ARTWORK_73_Documenting ;
        :Has-Duration  <http://www.semanticweb.org/ontologies/Daan/2020/BarbaraNanning#2018> ;
        :Involves      :BarbaraNanning ;
        :Located-In    :CzechRepublic ;
        :Part-Of       :Creation_Artwork_73 .

:ARTWORK_44_Packing_3
        a              owl:NamedIndividual , :Packing ;
        rdfs:comment   "Instance of an activity which is part of the creation process of ARTWORK_44."@en ;
        rdfs:label     "ARTWORK_44_Packing_3"@en ;
        :Followed-By   :ARTWORK_44_Transporting_3 ;
        :Follows       :ARTWORK_44_Signing ;
        :Has-Duration  <http://www.semanticweb.org/ontologies/Daan/2020/BarbaraNanning#2018> ;
        :Involves      :BarbaraNanning , :AlešZvěřina ;
        :Located-In    :CzechRepublic ;
        :Part-Of       :Creation_Artwork_44 .

<http://www.semanticweb.org/ontologies/Daan/2020/BarbaraNanning#JessicaHomich(USA)>
        a             :Fourth_Glass_Blower , owl:NamedIndividual ;
        rdfs:comment  "Jessica Homich (USA) is a Fourth Glass Blower."@en ;
        rdfs:label    "Jessica Homich (USA)"@en ;
        :Involved-In  :ARTWORK_46_Glassblowing , :ARTWORK_17_33_PickingUpColouredCanesPattern , <http://www.semanticweb.org/ontologies/Daan/2020/BarbaraNanning#ARTWORK_36_ExaminingQuality(Shape/Form)_2> , :ARTWORK_36_Cooling , :ARTWORK_18_64_Cooling , :ARTWORK_17_33_FillingHolesWithClearGlass , :ARTWORK_46_PreparingForBlowing , :ARTWORK_46_ApplyingClearOverlay , :ARTWORK_39_SetupAndTestingOfTheMetalMold , :ARTWORK_18_64_PickingUpColouredCanesPattern , :ARTWORK_36_Cooling_2 , :ARTWORK_18_64_Glassblowing , :ARTWORK_17_33_ProducingColouredCanes , :ARTWORK_46_Cooling , :ARTWORK_36_ApplyingMassivePieceOfClearGlass , :ARTWORK_36_PickingUpColouredCanesPattern , :ARTWORK_36_ProducingColouredCanes , :ARTWORK_17_33_ModelingWithTeflonStick , :ARTWORK_39_PickingUpColouredPanel , :ARTWORK_18_64_PreparingForBlowing , :ARTWORK_18_64_ProducingColouredCanes , :ARTWORK_36_Glassblowing , <http://www.semanticweb.org/ontologies/Daan/2020/BarbaraNanning#ARTWORK_46_ExaminingQuality(Shape/Form)> , :ARTWORK_46_ProducingColouredCanes , :ARTWORK_36_HeatingMetalMold , :ARTWORK_18_64_Modeling , :ARTWORK_46_PreparingGlass , :ARTWORK_39_Cooling , :ARTWORK_36_SetupAndTestingOfTheMetalMold , :ARTWORK_36_PickingUpColouredPanel , :ARTWORK_39_Glassblowing , :ARTWORK_17_33_ApplyingClearOverlay , :ARTWORK_18_64_PreparingForBlowing_2 , :ARTWORK_46_PickingUpColouredCanesPattern , :ARTWORK_39_Modeling , :ARTWORK_36_Modeling ;
        :Works-For    :GlassStudioVanTetterode , :VRIJGLASZaandam .

:GlassVerreÉglomisé  a    :Period , owl:NamedIndividual ;
        rdfs:comment      "Glass Verre Églomisé is a period from 2002 up to Present Day. Motivated by the desire to take on new challenges, Barbara has journeyed every year since 2001 to Novy Bor in the Czech Republic. The possibilities as regards finishing, such as grinding, polishing and gilding offer a great challenge in Novy Bor, a bulwark of glass decoration. She also brings vigorously the gilding of glass into play, a totally forgotten decorative technique that literally and figuratively enriches the sensual inner surfaces of her dishes."@en ;
        rdfs:label        "Glass Verre Églomisé"@en ;
        :Has-Duration     <http://www.semanticweb.org/ontologies/Daan/2020/BarbaraNanning#2002UpToPresentDay> ;
        :Period-Contains  :Creation_Artwork_74 , :Creation_Artwork_44 , :Creation_Artwork_79 , :Creation_Artwork_78 , :Creation_Artwork_77 , :Creation_Artwork_80 , :Creation_Artwork_75 , :Creation_Artwork_76 , :Creation_Artwork_73 , :Creation_Artwork_43 .

:Transporting_Coloured_Canes
        a                owl:Class ;
        rdfs:comment     "Moving said objects from one place to another"@en ;
        rdfs:label       "Transporting Coloured Canes"@en ;
        rdfs:subClassOf  :Transporting .

:ARTWORK_46_Transporting_2
        a              :Transporting , owl:NamedIndividual ;
        rdfs:comment   "Instance of an activity which is part of the creation process of ARTWORK_46."@en ;
        rdfs:label     "ARTWORK_46_Transporting_2"@en ;
        :Followed-By   :ARTWORK_46_Photographing ;
        :Follows       :ARTWORK_46_Packing_2 ;
        :Has-Duration  <http://www.semanticweb.org/ontologies/Daan/2020/BarbaraNanning#2018> ;
        :Involves      :BarbaraNanning , :AlešZvěřina ;
        :Located-In    :Amsterdam ;
        :Part-Of       :Creation_Artwork_46 .

:Is-Processed-During  a  owl:ObjectProperty ;
        rdfs:comment   "Is-Processed-During connects a material with an activity in which the material is (being) processed."@en ;
        rdfs:domain    :Material ;
        rdfs:label     "Is-Processed-During"@en ;
        rdfs:range     :Activity ;
        owl:inverseOf  :Processes .

:ARTWORK_76_SetupAndTestingOfTheMetalMold
        a                 owl:NamedIndividual , :Setup_and_Testing_of_the_Metal_Mold ;
        rdfs:comment      "Instance of an activity which is part of the creation process of ARTWORK_76."@en ;
        rdfs:label        "ARTWORK_76_Setup and Testing of the Metal Mold"@en ;
        :Followed-By      :ARTWORK_76_ExaminingTheQualityOfTheGlass ;
        :Follows          :ARTWORK_76_PreparingGlass ;
        :Has-Duration     <http://www.semanticweb.org/ontologies/Daan/2020/BarbaraNanning#2018> ;
        :Involves         <http://www.semanticweb.org/ontologies/Daan/2020/BarbaraNanning#JiriMoravec(CZ)> , :AssistantOfBarbara , <http://www.semanticweb.org/ontologies/Daan/2020/BarbaraNanning#RadekKoten(CZ)> , <http://www.semanticweb.org/ontologies/Daan/2020/BarbaraNanning#LukasHavlas(CZ)> , :BarbaraNanning , <http://www.semanticweb.org/ontologies/Daan/2020/BarbaraNanning#Tom%C3%A1%C5%A1Moravec(CZ)> ;
        :Located-In       :CzechRepublic ;
        :Part-Of          :Creation_Artwork_76 ;
        :Requires-Use-Of  :InterchangeableMetalMoldSetup .

<http://vocab.getty.edu/aat/300024743>
        a           owl:NamedIndividual ;
        owl:sameAs  :Pincet .

:ARTWORK_36_Sensing_4
        a              :Sensing , owl:NamedIndividual ;
        rdfs:comment   "Instance of an activity which is part of the creation process of ARTWORK_36."@en ;
        rdfs:label     "ARTWORK_36_Sensing_4"@en ;
        :Followed-By   :ARTWORK_36_Grinding_2 ;
        :Follows       :ARTWORK_36_Sawing_2 ;
        :Has-Duration  <http://www.semanticweb.org/ontologies/Daan/2020/BarbaraNanning#2019> ;
        :Involves      :BarbaraNanning , :AlešZvěřina , :LukášSvoboda ;
        :Located-In    :NovyBor ;
        :Part-Of       :Creation_Artwork_36 .

:ARTWORK_43_Polishing
        a                 :Polishing , owl:NamedIndividual ;
        rdfs:comment      "Instance of an activity which is part of the creation process of ARTWORK_43."@en ;
        rdfs:label        "ARTWORK_43_Polishing"@en ;
        :Followed-By      <http://www.semanticweb.org/ontologies/Daan/2020/BarbaraNanning#ARTWORK_43_ExaminingQuality(Result)> ;
        :Follows          :ARTWORK_43_Grinding ;
        :Has-Duration     <http://www.semanticweb.org/ontologies/Daan/2020/BarbaraNanning#2008> ;
        :Involves         :BarbaraNanning , :AlešZvěřina , :LukášSvoboda ;
        :Located-In       :CzechRepublic ;
        :Part-Of          :Creation_Artwork_43 ;
        :Requires-Use-Of  :PolishingStone .

:ARTWORK_77_Signing  a    owl:NamedIndividual , :Signing ;
        rdfs:comment      "Instance of an activity which is part of the creation process of ARTWORK_77."@en ;
        rdfs:label        "ARTWORK_77_Signing"@en ;
        :Followed-By      :ARTWORK_77_MeasuringAndBoxesMaking ;
        :Follows          :ARTWORK_77_Transporting_2 ;
        :Has-Duration     <http://www.semanticweb.org/ontologies/Daan/2020/BarbaraNanning#2018> ;
        :Involves         :AlešZvěřina , :BarbaraNanning ;
        :Located-In       :CzechRepublic ;
        :Part-Of          :Creation_Artwork_77 ;
        :Requires-Use-Of  :AirCompressor .

:ARTWORK_77_Gilding  a    :Gilding , owl:NamedIndividual ;
        rdfs:comment      "Instance of an activity which is part of the creation process of ARTWORK_77."@en ;
        rdfs:label        "ARTWORK_77_Gilding"@en ;
        :Followed-By      <http://www.semanticweb.org/ontologies/Daan/2020/BarbaraNanning#ARTWORK_77_ExaminingQuality(FinalResult)> ;
        :Follows          :ARTWORK_77_Transporting_3 ;
        :Has-Duration     <http://www.semanticweb.org/ontologies/Daan/2020/BarbaraNanning#2018> ;
        :Involves         :VáçlavNovák_Doksy_CzechRepublic , :BarbaraNanning ;
        :Located-In       :CzechRepublic ;
        :Part-Of          :Creation_Artwork_77 ;
        :Requires-Use-Of  :GildersKnife , :GildersTip , :INSTACOLLTool , :GildingCushion .

<http://www.cidoc-crm.org/cidoc-crm/P109_has_current_or_former_curator>
        a                       owl:ObjectProperty ;
        owl:equivalentProperty  :Maintains .

:ARTWORK_36_MeasuringAndBoxesMaking_2
        a              :Measuring_and_Boxes_Making , owl:NamedIndividual ;
        rdfs:comment   "Instance of an activity which is part of the creation process of ARTWORK_36."@en ;
        rdfs:label     "ARTWORK_36_Measuring and Boxes Making_2"@en ;
        :Followed-By   :ARTWORK_36_Packing_6 ;
        :Follows       <http://www.semanticweb.org/ontologies/Daan/2020/BarbaraNanning#ARTWORK_36_ExaminingQuality(Result)_2> ;
        :Has-Duration  <http://www.semanticweb.org/ontologies/Daan/2020/BarbaraNanning#2019> ;
        :Involves      :AlešZvěřina , :BarbaraNanning ;
        :Located-In    :NovyBor ;
        :Part-Of       :Creation_Artwork_36 .

:Requires-Use-Of  a    owl:ObjectProperty ;
        rdfs:comment   "Requires-Use-Of is a property which connects a tool or equipment of which an activity requires usage."@en ;
        rdfs:domain    :Activity ;
        rdfs:label     "Requires-Use-Of"@en ;
        rdfs:range     :Equipment ;
        owl:inverseOf  :Used-For .

<http://www.semanticweb.org/ontologies/Daan/2020/BarbaraNanning#ARTWORK_80_ExaminingQuality(CheckForIrregularitiesInTheGlass)>
        a              j.3: , owl:NamedIndividual ;
        rdfs:comment   "Instance of an activity which is part of the creation process of ARTWORK_80."@en ;
        rdfs:label     "ARTWORK_80_Examining Quality (Check for Irregularities in the Glass)"@en ;
        :Followed-By   :ARTWORK_80_Sawing ;
        :Follows       :ARTWORK_80_Resting ;
        :Has-Duration  <http://www.semanticweb.org/ontologies/Daan/2020/BarbaraNanning#2018> ;
        :Involves      :AlešZvěřina , :BarbaraNanning ;
        :Located-In    :CzechRepublic ;
        :Part-Of       :Creation_Artwork_80 .

<http://vocab.getty.edu/aat/300053885>
        a                    owl:Class ;
        owl:equivalentClass  :Heating .

:ARTWORK_39_TransportingMetalBowlWithPanel
        a              owl:NamedIndividual , :Transporting_Metal_Bowl_with_Panel ;
        rdfs:comment   "Instance of an activity which is part of the creation process of ARTWORK_39."@en ;
        rdfs:label     "ARTWORK_39_Transporting Metal Bowl with Panel"@en ;
        :Followed-By   :ARTWORK_39_PreparingForBlowing ;
        :Follows       :ARTWORK_39_Slumping ;
        :Has-Duration  <http://www.semanticweb.org/ontologies/Daan/2020/BarbaraNanning#2015> ;
        :Involves      :BarbaraNanning ;
        :Located-In    :Zaandam ;
        :Part-Of       :Creation_Artwork_39 .

<http://www.wikidata.org/entity/Q34679>
        a       owl:NamedIndividual .

<http://www.wikidata.org/entity/Q703>
        a       owl:NamedIndividual .

:Artwork_36_Peacock  a  :Man-Made_Material , owl:NamedIndividual ;
        rdfs:label  "Artwork 36 Peacock" .

<http://www.wikidata.org/entity/Q283>
        a       owl:NamedIndividual .

:ARTWORK_18_64_Cooling
        a                 owl:NamedIndividual , :Cooling ;
        rdfs:comment      "Instance of an activity which is part of the creation process of ARTWORK_18_64."@en ;
        rdfs:label        "ARTWORK_18_64_Cooling"@en ;
        :Followed-By      :ARTWORK_18_64_Packing ;
        :Follows          <http://www.semanticweb.org/ontologies/Daan/2020/BarbaraNanning#ARTWORK_18_64_ExaminingQuality(Shape/Form)> ;
        :Has-Duration     <http://www.semanticweb.org/ontologies/Daan/2020/BarbaraNanning#2015> ;
        :Involves         <http://www.semanticweb.org/ontologies/Daan/2020/BarbaraNanning#JessicaHomich(USA)> , <http://www.semanticweb.org/ontologies/Daan/2020/BarbaraNanning#MiaLerssi(DN)> , :DurkValkema ;
        :Located-In       :Zaandam ;
        :Part-Of          :Creation_Artwork_18_64 ;
        :Requires-Use-Of  :AnnealingKiln .

<http://www.wikidata.org/entity/Q14914>
        a       owl:NamedIndividual .

:ARTWORK_36_Ordening  a   owl:NamedIndividual , :Ordening ;
        rdfs:comment      "Instance of an activity which is part of the creation process of ARTWORK_36."@en ;
        rdfs:label        "ARTWORK_36_Ordening"@en ;
        :Followed-By      :ARTWORK_36_Casting ;
        :Follows          :ARTWORK_36_CuttingMonochromeSheets ;
        :Has-Duration     <http://www.semanticweb.org/ontologies/Daan/2020/BarbaraNanning#2015> ;
        :Involves         :BarbaraNanning ;
        :Located-In       :Langweer ;
        :Part-Of          :Creation_Artwork_36 ;
        :Requires-Use-Of  :Pincet , :Glassscissors , :Computer .

:ARTWORK_18_64_Documenting
        a              :Documenting , owl:NamedIndividual ;
        rdfs:comment   "Instance of an activity which is part of the creation process of ARTWORK_18_64."@en ;
        rdfs:label     "ARTWORK_18_64_Documenting"@en ;
        :Finishes      :Creation_Artwork_18_64 ;
        :Follows       :ARTWORK_18_64_Packing_3 ;
        :Has-Duration  <http://www.semanticweb.org/ontologies/Daan/2020/BarbaraNanning#2015> ;
        :Involves      :BarbaraNanning ;
        :Located-In    :Amsterdam ;
        :Part-Of       :Creation_Artwork_18_64 .

:ARTWORK_46_Modeling  a   owl:NamedIndividual , :Modeling ;
        rdfs:comment      "Instance of an activity which is part of the creation process of ARTWORK_46."@en ;
        rdfs:label        "ARTWORK_46_Modeling"@en ;
        :Followed-By      <http://www.semanticweb.org/ontologies/Daan/2020/BarbaraNanning#ARTWORK_46_ExaminingQuality(Shape/Form)> ;
        :Follows          :ARTWORK_46_Sensing ;
        :Has-Duration     <http://www.semanticweb.org/ontologies/Daan/2020/BarbaraNanning#2018> ;
        :Involves         :JaroslavKubásek , :JiříPačinekJunior , <http://www.semanticweb.org/ontologies/Daan/2020/BarbaraNanning#JiriPacinek(CZ)> , :BarbaraNanning , :JanBaštýř , :DavidČerný ;
        :Located-In       :Lindava ;
        :Part-Of          :Creation_Artwork_46 ;
        :Requires-Use-Of  :Gloves , :BlowingPipe , :InterchangeableMetalMoldSetup , :AirCompressor , :PropaneTorch .

:Transporting_Metal_Bowl_with_Sheet
        a                owl:Class ;
        rdfs:comment     "Moving said objects from one place to another"@en ;
        rdfs:label       "Transporting Metal Bowl with Sheet"@en ;
        rdfs:subClassOf  :Transporting .

<http://www.wikidata.org/entity/Q1000086>
        a       owl:NamedIndividual .

:Employed  a           owl:ObjectProperty ;
        rdfs:comment   "Employed is a property which connects an organisation with a person."@en ;
        rdfs:domain    :Organisation ;
        rdfs:label     "Employed"@en ;
        rdfs:range     :Person ;
        owl:inverseOf  :Works-For .

:ARTWORK_18_64_Grinding
        a                 :Grinding , owl:NamedIndividual ;
        rdfs:comment      "Instance of an activity which is part of the creation process of ARTWORK_18_64."@en ;
        rdfs:label        "ARTWORK_18_64_Grinding_2"@en ;
        :Follows          :ARTWORK_18_64_Sensing_2 ;
        :Has-Duration     <http://www.semanticweb.org/ontologies/Daan/2020/BarbaraNanning#2015> ;
        :Involves         :RobertFlorian , :BarbaraNanning , :AlešZvěřina ;
        :Located-In       :NovyBor ;
        :Part-Of          :Creation_Artwork_18_64 ;
        :Requires-Use-Of  :SharpeningStone , :GrindingWheel .

:ARTWORK_80_MeasuringAndBoxesMaking
        a              owl:NamedIndividual , :Measuring_and_Boxes_Making ;
        rdfs:comment   "Instance of an activity which is part of the creation process of ARTWORK_80."@en ;
        rdfs:label     "ARTWORK_80_Measuring and Boxes Making"@en ;
        :Followed-By   :ARTWORK_80_Packing_2 ;
        :Follows       <http://www.semanticweb.org/ontologies/Daan/2020/BarbaraNanning#ARTWORK_80_ExaminingQuality(Result)> ;
        :Has-Duration  <http://www.semanticweb.org/ontologies/Daan/2020/BarbaraNanning#2018> ;
        :Involves      :BarbaraNanning , :AlešZvěřina ;
        :Located-In    :CzechRepublic ;
        :Part-Of       :Creation_Artwork_80 .

:ARTWORK_76_Sandblasting
        a                 :Sandblasting , owl:NamedIndividual ;
        rdfs:comment      "Instance of an activity which is part of the creation process of ARTWORK_76."@en ;
        rdfs:label        "ARTWORK_76_Sandblasting"@en ;
        :Followed-By      :ARTWORK_76_Signing ;
        :Follows          :ARTWORK_76_Transporting_2 ;
        :Has-Duration     <http://www.semanticweb.org/ontologies/Daan/2020/BarbaraNanning#2018> ;
        :Involves         :AlešZvěřina , :BarbaraNanning ;
        :Located-In       :CzechRepublic ;
        :Part-Of          :Creation_Artwork_76 ;
        :Requires-Use-Of  :AirCompressor .

:Image_Artwork_78  a            :Digital_Image , owl:NamedIndividual ;
        rdfs:comment            "Image of an artwork by Barbara Nanning displayed in \"Barbara Nanning Eeuwige Beweging\" by Eliens (2019)."@en ;
        rdfs:label              "Image_Artwork_78"@en ;
        :Representation-Source  "Tom Haartsen_Ouderkerk a/d Amstel (NL)"@en ;
        :Shows                  :Artwork_78 .

:Examining_the_Quality_of_the_Glass
        a                owl:Class ;
        rdfs:comment     "Examining the Quality of the Glass is an activity conducted by a creator in which the quality of a the glass is assured."@en ;
        rdfs:label       "Examining the Quality of the Glass"@en ;
        rdfs:subClassOf  :Activity .

:ARTWORK_76_ApplyingExtraColour_2
        a                 owl:NamedIndividual , :Applying_Extra_Colour ;
        rdfs:comment      "Instance of an activity which is part of the creation process of ARTWORK_76."@en ;
        rdfs:label        "ARTWORK_76_Applying Extra Colour_2"@en ;
        :Followed-By      :ARTWORK_76_HeatingMetalMold ;
        :Follows          :ARTWORK_76_ApplyingExtraColour ;
        :Has-Duration     <http://www.semanticweb.org/ontologies/Daan/2020/BarbaraNanning#2018> ;
        :Involves         <http://www.semanticweb.org/ontologies/Daan/2020/BarbaraNanning#LukasHavlas(CZ)> , :BarbaraNanning , <http://www.semanticweb.org/ontologies/Daan/2020/BarbaraNanning#RadekKoten(CZ)> ;
        :Located-In       :CzechRepublic ;
        :Part-Of          :Creation_Artwork_76 ;
        :Processes        :AJETOAlexandriteGlass ;
        :Requires-Use-Of  :Tagliol , :Beeswax , :Garage , :Blocks , :Fork , :Pontis , :IcePick , :StraightShears , :Jacks , :BlowingPipe , :Water , :AirCompressor , :Pincet , :DiamondShears , :Marver , :AnnealingKiln , :GloryHole , :Paper , :Hook , :Furnace , :CeramicPotFilledWithGlass , :YokeOfSupport .

:ARTWORK_18_64_Resting
        a                 owl:NamedIndividual , :Resting ;
        rdfs:comment      "Instance of an activity which is part of the creation process of ARTWORK_18_64."@en ;
        rdfs:label        "ARTWORK_18_64_Resting"@en ;
        :Followed-By      <http://www.semanticweb.org/ontologies/Daan/2020/BarbaraNanning#ARTWORK_18_64_ExaminingQuality(CheckForIrregularitiesInTheGlass)> ;
        :Follows          :ARTWORK_18_64_Transporting ;
        :Has-Duration     <http://www.semanticweb.org/ontologies/Daan/2020/BarbaraNanning#2015> ;
        :Involves         :AlešZvěřina ;
        :Located-In       :NovyBor ;
        :Part-Of          :Creation_Artwork_18_64 ;
        :Requires-Use-Of  :AnnealingKiln .

:ARTWORK_17_33_Sensing
        a              owl:NamedIndividual , :Sensing ;
        rdfs:comment   "Instance of an activity which is part of the creation process of ARTWORK_17_33."@en ;
        rdfs:label     "ARTWORK_17_33_Sensing"@en ;
        :Followed-By   :ARTWORK_17_33_Modeling ;
        :Follows       :ARTWORK_17_33_ApplyingClearOverlay ;
        :Has-Duration  <http://www.semanticweb.org/ontologies/Daan/2020/BarbaraNanning#2017> ;
        :Involves      :BarbaraNanning , :LukášSvoboda , :AlešZvěřina ;
        :Located-In    :Lindava ;
        :Part-Of       :Creation_Artwork_17_33 .

:Image_Artwork_46  a            :Digital_Image , owl:NamedIndividual ;
        rdfs:comment            "Image of Artwork_46 by Barbara Nanning."@en ;
        rdfs:label              "Image_Artwork_46"@en ;
        :Representation-Source  "Tom Haartsen_Ouderkerk A/d Amstel (NL)"@en ;
        :Shows                  :Artwork_46 .

:Glassscissors  a     :Tool , owl:NamedIndividual ;
        rdfs:comment  "Glassscissors are a type of scissors used to cut glass materials."@en ;
        rdfs:label    "Glassscissors"@en .

<http://www.cidoc-crm.org/cidoc-crm/P14_carried_out_by>
        a                       owl:ObjectProperty ;
        owl:equivalentProperty  :Involves .

:ARTWORK_18_64_CuttingMonochromeSheets
        a              :Cutting_Monochrome_Sheets , owl:NamedIndividual ;
        rdfs:comment   "Instance of an activity which is part of the creation process of ARTWORK_18_64."@en ;
        rdfs:label     "ARTWORK_18_64_Cutting Monochrome Sheets"@en ;
        :Followed-By   :ARTWORK_18_64_Ordening ;
        :Follows       :ARTWORK_18_64_DecidingColourPaletteAndPatterns ;
        :Has-Duration  <http://www.semanticweb.org/ontologies/Daan/2020/BarbaraNanning#2015> ;
        :Involves      :BarbaraNanning , :SteefHendriks ;
        :Located-In    :Langweer ;
        :Part-Of       :Creation_Artwork_18_64 .

:ARTWORK_78_Transporting_4
        a              :Transporting , owl:NamedIndividual ;
        rdfs:comment   "Instance of an activity which is part of the creation process of ARTWORK_78."@en ;
        rdfs:label     "ARTWORK_78_Transporting_4"@en ;
        :Followed-By   :ARTWORK_78_Photographing ;
        :Follows       :ARTWORK_78_Packing_4 ;
        :Has-Duration  <http://www.semanticweb.org/ontologies/Daan/2020/BarbaraNanning#2008> ;
        :Involves      :AlešZvěřina , :BarbaraNanning ;
        :Located-In    :CzechRepublic ;
        :Part-Of       :Creation_Artwork_78 .

:Followed-By  a        owl:ObjectProperty ;
        rdfs:comment   "Followed-By is a property which connects an event to the event which occurs next."@en ;
        rdfs:domain    :Event ;
        rdfs:label     "Followed-By"@en ;
        rdfs:range     :Event ;
        owl:inverseOf  :Follows .

:GildersTip  a        owl:NamedIndividual , :Tool ;
        rdfs:comment  "A gilders tip is a brush made out of Kölner squirl hair (30 mm or 80 mm) used in gilding to pick up pieces of gold leaf."@en ;
        rdfs:label    "Gilders Tip"@en ;
        :Used-For     :ARTWORK_44_Gilding , :ARTWORK_80_Gilding , :ARTWORK_73_Gilding , :ARTWORK_77_Gilding , :ARTWORK_74_Gilding , :ARTWORK_43_Gilding , :ARTWORK_75_Gilding , :ARTWORK_79_Gilding , :ARTWORK_78_Gilding , :ARTWORK_76_Gilding .

:Creation_Artwork_76  a  :Creation_Event , owl:NamedIndividual ;
        rdfs:comment    "Creation event for an artwork by Barbara Nanning displayed in \"Barbara Nanning Eeuwige Beweging\" by Eliens (2019)."@en ;
        rdfs:label      "Creation_Artwork_76"@en ;
        :Consists-Of    :ARTWORK_76_Transporting_2 , :ARTWORK_76_ApplyingExtraColour_2 , :ARTWORK_76_Gilding , :ARTWORK_76_ExaminingTheQualityOfTheGlass , :ARTWORK_76_Packing_3 , :ARTWORK_76_ApplyingClearGlassBell , :ARTWORK_76_Resting , <http://www.semanticweb.org/ontologies/Daan/2020/BarbaraNanning#ARTWORK_76_ExaminingQuality(CheckForIrregularitiesInTheGlass)_2> , :ARTWORK_76_Sensing , <http://www.semanticweb.org/ontologies/Daan/2020/BarbaraNanning#ARTWORK_76_ExaminingQuality(Shape/Form)> , :ARTWORK_76_HeatingMetalMold , :ARTWORK_76_MeasuringAndBoxesMaking , :ARTWORK_76_Transporting_4 , :ARTWORK_76_Photographing , :ARTWORK_76_SetupAndTestingOfTheMetalMold , :ARTWORK_76_Sandblasting , :ARTWORK_76_Packing_4 , :ARTWORK_76_Documenting , :ARTWORK_76_Cooling , :ARTWORK_76_SetupAndTestingOfTheMetalMold_2 , :ARTWORK_76_Modeling , :ARTWORK_76_PreparingGlass , :ARTWORK_76_Signing , <http://www.semanticweb.org/ontologies/Daan/2020/BarbaraNanning#ARTWORK_76_ExaminingQuality(FinalResult)> , <http://www.semanticweb.org/ontologies/Daan/2020/BarbaraNanning#ARTWORK_76_ExaminingQuality(CheckForIrregularitiesInTheGlass)> , :ARTWORK_76_Packing , :ARTWORK_76_Polishing , :ARTWORK_76_Translocating , :ARTWORK_76_Sawing , :ARTWORK_76_Transporting , :ARTWORK_76_Packing_5 , :ARTWORK_76_Glassblowing , :ARTWORK_76_Grinding , :ARTWORK_76_Transporting_3 , :ARTWORK_76_ApplyingExtraColour , :ARTWORK_76_Packing_2 ;
        :Created        :Artwork_76 ;
        :Finishes-With  :ARTWORK_76_Packing_5 ;
        :Has-Duration   <http://www.semanticweb.org/ontologies/Daan/2020/BarbaraNanning#2018> ;
        :Located-In     :CzechRepublic ;
        :Starts-With    :ARTWORK_76_PreparingGlass ;
        :Within-Period  :GlassVerreÉglomisé .

:ARTWORK_76_Signing  a    owl:NamedIndividual , :Signing ;
        rdfs:comment      "Instance of an activity which is part of the creation process of ARTWORK_76."@en ;
        rdfs:label        "ARTWORK_76_Signing"@en ;
        :Followed-By      :ARTWORK_76_Packing_3 ;
        :Follows          :ARTWORK_76_Sandblasting ;
        :Has-Duration     <http://www.semanticweb.org/ontologies/Daan/2020/BarbaraNanning#2018> ;
        :Involves         :AlešZvěřina , :BarbaraNanning ;
        :Located-In       :CzechRepublic ;
        :Part-Of          :Creation_Artwork_76 ;
        :Requires-Use-Of  :AirCompressor .

:ARTWORK_76_Gilding  a    owl:NamedIndividual , :Gilding ;
        rdfs:comment      "Instance of an activity which is part of the creation process of ARTWORK_76."@en ;
        rdfs:label        "ARTWORK_76_Gilding"@en ;
        :Followed-By      <http://www.semanticweb.org/ontologies/Daan/2020/BarbaraNanning#ARTWORK_76_ExaminingQuality(FinalResult)> ;
        :Follows          :ARTWORK_76_Transporting_3 ;
        :Has-Duration     <http://www.semanticweb.org/ontologies/Daan/2020/BarbaraNanning#2018> ;
        :Involves         :BarbaraNanning , :VáçlavNovák_Doksy_CzechRepublic ;
        :Located-In       :CzechRepublic ;
        :Part-Of          :Creation_Artwork_76 ;
        :Requires-Use-Of  :GildingCushion , :INSTACOLLTool , :GildersTip , :GildersKnife .

:ARTWORK_77_Packing_4
        a              owl:NamedIndividual , :Packing ;
        rdfs:comment   "Instance of an activity which is part of the creation process of ARTWORK_77."@en ;
        rdfs:label     "ARTWORK_77_Packing_4"@en ;
        :Followed-By   :ARTWORK_77_Transporting_4 ;
        :Follows       <http://www.semanticweb.org/ontologies/Daan/2020/BarbaraNanning#ARTWORK_77_ExaminingQuality(FinalResult)> ;
        :Has-Duration  <http://www.semanticweb.org/ontologies/Daan/2020/BarbaraNanning#2018> ;
        :Involves      :BarbaraNanning , :AlešZvěřina , :VáçlavNovák_Doksy_CzechRepublic ;
        :Located-In    :CzechRepublic ;
        :Part-Of       :Creation_Artwork_77 .

:ARTWORK_17_33_Packing_2
        a              owl:NamedIndividual , :Packing ;
        rdfs:comment   "Instance of an activity which is part of the creation process of ARTWORK_17_33."@en ;
        rdfs:label     "ARTWORK_17_33_Packing_2"@en ;
        :Followed-By   :ARTWORK_17_33_Transporting_2 ;
        :Follows       :ARTWORK_17_33_MeasuringAndBoxesMaking ;
        :Has-Duration  <http://www.semanticweb.org/ontologies/Daan/2020/BarbaraNanning#2017> ;
        :Involves      :BarbaraNanning ;
        :Located-In    :NovyBor ;
        :Part-Of       :Creation_Artwork_17_33 .

:Gloves  a            :Equipment , owl:NamedIndividual ;
        rdfs:comment  "Gloves are a piece of clothing used for protecting the hands by covering them."@en ;
        rdfs:label    "Gloves"@en ;
        owl:sameAs    <http://www.wikidata.org/entity/Q169031> ;
        :Used-For     :ARTWORK_79_Modeling , :ARTWORK_74_Modeling , :ARTWORK_73_Modeling , :ARTWORK_77_HeatingMetalMold , :ARTWORK_75_HeatingMetalMold , :ARTWORK_76_Glassblowing , :ARTWORK_77_Modeling , :ARTWORK_75_Glassblowing , :ARTWORK_43_Modeling , :ARTWORK_74_HeatingMetalMold , :ARTWORK_78_Glassblowing , :ARTWORK_43_HeatingMetalMold , :ARTWORK_43_Glassblowing , :ARTWORK_77_Glassblowing , :ARTWORK_80_Modeling , :ARTWORK_78_HeatingMetalMold , :ARTWORK_44_Modeling , :ARTWORK_76_Modeling , :ARTWORK_73_HeatingMetalMold , :ARTWORK_44_HeatingMetalMold , :ARTWORK_80_Glassblowing , :ARTWORK_78_Modeling , :ARTWORK_73_Glassblowing , :ARTWORK_75_Modeling , :ARTWORK_79_HeatingMetalMold , :ARTWORK_79_Glassblowing , :ARTWORK_80_HeatingMetalMold , :ARTWORK_44_Glassblowing , :ARTWORK_74_Glassblowing , :ARTWORK_76_HeatingMetalMold .

<http://vocab.getty.edu/aat/300025297>
        a                    owl:Class ;
        owl:equivalentClass  :Metal_Worker .

:ARTWORK_74_Transporting_2
        a              owl:NamedIndividual , :Transporting ;
        rdfs:comment   "Instance of an activity which is part of the creation process of ARTWORK_74."@en ;
        rdfs:label     "ARTWORK_74_Transporting_2"@en ;
        :Followed-By   :ARTWORK_74_Signing ;
        :Follows       :ARTWORK_74_Packing_2 ;
        :Has-Duration  <http://www.semanticweb.org/ontologies/Daan/2020/BarbaraNanning#2008> ;
        :Involves      :AlešZvěřina , :BarbaraNanning ;
        :Located-In    :CzechRepublic ;
        :Part-Of       :Creation_Artwork_74 .

<http://www.semanticweb.org/ontologies/Daan/2020/BarbaraNanning#ARTWORK_77_ExaminingQuality(Result)>
        a              j.0: , owl:NamedIndividual ;
        rdfs:comment   "Instance of an activity which is part of the creation process of ARTWORK_77."@en ;
        rdfs:label     "ARTWORK_77_Examining Quality (Result)"@en ;
        :Followed-By   :ARTWORK_77_MeasuringAndBoxesMaking ;
        :Follows       :ARTWORK_77_Polishing ;
        :Has-Duration  <http://www.semanticweb.org/ontologies/Daan/2020/BarbaraNanning#2018> ;
        :Involves      :BarbaraNanning , :AlešZvěřina ;
        :Located-In    :CzechRepublic ;
        :Part-Of       :Creation_Artwork_77 .

:Creation_Artwork_44  a  :Creation_Event , owl:NamedIndividual ;
        rdfs:comment    "Creation event for an artwork by Barbara Nanning displayed in \"Barbara Nanning Eeuwige Beweging\" by Eliens (2019)."@en ;
        rdfs:label      "Creation_Artwork_44"@en ;
        :Consists-Of    :ARTWORK_44_Sensing , <http://www.semanticweb.org/ontologies/Daan/2020/BarbaraNanning#ARTWORK_44_ExaminingQuality(CheckForIrregularitiesInTheGlass)> , :ARTWORK_44_ApplyingExtraColour , :ARTWORK_44_Glassblowing , :ARTWORK_44_Packing_5 , :ARTWORK_44_Signing , :ARTWORK_44_Documenting , :ARTWORK_44_SetupAndTestingOfTheMetalMold_2 , :ARTWORK_44_Translocating , :ARTWORK_44_Transporting_4 , :ARTWORK_44_Sawing , :ARTWORK_44_ApplyingClearGlassBell , :ARTWORK_44_Transporting_3 , :ARTWORK_44_PreparingGlass , :ARTWORK_44_Packing_3 , <http://www.semanticweb.org/ontologies/Daan/2020/BarbaraNanning#ARTWORK_44_ExaminingQuality(Shape/Form)> , :ARTWORK_44_Polishing , :ARTWORK_44_Packing , :ARTWORK_44_HeatingMetalMold , :ARTWORK_44_Transporting , :ARTWORK_44_Resting , :ARTWORK_44_Modeling , :ARTWORK_44_Grinding , :ARTWORK_44_MeasuringAndBoxesMaking , :ARTWORK_44_Cooling , :ARTWORK_44_Photographing , :ARTWORK_44_Gilding , :ARTWORK_44_SetupAndTestingOfTheMetalMold , :ARTWORK_44_Packing_4 , :ARTWORK_44_ExaminingTheQualityOfTheGlass , :ARTWORK_44_Packing_2 , :ARTWORK_44_ApplyingExtraColour_2 , <http://www.semanticweb.org/ontologies/Daan/2020/BarbaraNanning#ARTWORK_44_ExaminingQuality(FinalResult)> , :ARTWORK_44_Transporting_2 ;
        :Created        :Artwork_44 ;
        :Finishes-With  :ARTWORK_44_Packing_5 ;
        :Has-Duration   <http://www.semanticweb.org/ontologies/Daan/2020/BarbaraNanning#2018> ;
        :Located-In     :CzechRepublic ;
        :Starts-With    :ARTWORK_44_PreparingGlass ;
        :Within-Period  :GlassVerreÉglomisé .

:ARTWORK_17_33_Glassblowing
        a                 owl:NamedIndividual , :Glassblowing ;
        rdfs:comment      "Instance of an activity which is part of the creation process of ARTWORK_17_33."@en ;
        rdfs:label        "ARTWORK_17_33_Glassblowing"@en ;
        :Followed-By      :ARTWORK_17_33_ModelingWithTeflonStick ;
        :Follows          :ARTWORK_17_33_PickingUpColouredCanesPattern ;
        :Has-Duration     <http://www.semanticweb.org/ontologies/Daan/2020/BarbaraNanning#2017> ;
        :Involves         :AssistantOfBarbara , :BarbaraNanning , <http://www.semanticweb.org/ontologies/Daan/2020/BarbaraNanning#LukasHavlas(CZ)> , <http://www.semanticweb.org/ontologies/Daan/2020/BarbaraNanning#Tom%C3%A1%C5%A1Moravec(CZ)> , <http://www.semanticweb.org/ontologies/Daan/2020/BarbaraNanning#RadekKoten(CZ)> , <http://www.semanticweb.org/ontologies/Daan/2020/BarbaraNanning#JiriMoravec(CZ)> ;
        :Located-In       :Lindava ;
        :Part-Of          :Creation_Artwork_17_33 ;
        :Requires-Use-Of  :InterchangeableMetalMoldSetup , :Paper , :Gloves , :IcePick , :DiamondShears , :Blocks , :Fork , :GloryHole , :Furnace , :YokeOfSupport , :AirCompressor , :BlowingPipe , :Hook , :Water , :Pontis , :AnnealingKiln , :Tagliol , :CeramicPotFilledWithGlass , :Jacks , :Marver , :PropaneTorch , :Pincet , :BitIron , :StraightShears , :Beeswax .

<http://vocab.getty.edu/aat/300054638>
        a                    owl:Class ;
        owl:equivalentClass  :Documenting .

:AlešZvěřina  a       :Grinder_1 , owl:NamedIndividual ;
        rdfs:comment  "Aleš Zvěřina is a Grinder 1."@en ;
        rdfs:label    "Aleš Zvěřina"@en ;
        :Involved-In  :ARTWORK_79_Transporting_3 , :ARTWORK_75_Packing_3 , :ARTWORK_80_Resting , :ARTWORK_75_Sawing , :ARTWORK_74_Grinding , :ARTWORK_77_Packing , :ARTWORK_73_Packing_3 , :ARTWORK_79_Grinding , <http://www.semanticweb.org/ontologies/Daan/2020/BarbaraNanning#ARTWORK_79_ExaminingQuality(FinalResult)> , :ARTWORK_74_Resting , :ARTWORK_79_Packing_4 , :ARTWORK_73_Transporting_2 , <http://www.semanticweb.org/ontologies/Daan/2020/BarbaraNanning#ARTWORK_77_ExaminingQuality(CheckForIrregularitiesInTheGlass)> , :ARTWORK_43_Sandblasting , :ARTWORK_44_Resting , :ARTWORK_78_Packing_4 , :ARTWORK_73_Sensing , :ARTWORK_76_Packing_4 , :ARTWORK_76_Sawing , <http://www.semanticweb.org/ontologies/Daan/2020/BarbaraNanning#ARTWORK_43_ExaminingQuality(CheckForIrregularitiesInTheGlass)> , :ARTWORK_78_Transporting_4 , :ARTWORK_44_Transporting_3 , :ARTWORK_44_MeasuringAndBoxesMaking , :ARTWORK_74_Packing_3 , <http://www.semanticweb.org/ontologies/Daan/2020/BarbaraNanning#ARTWORK_75_ExaminingQuality(FinalResult)> , :ARTWORK_75_Sensing , <http://www.semanticweb.org/ontologies/Daan/2020/BarbaraNanning#ARTWORK_74_ExaminingQuality(CheckForIrregularitiesInTheGlass)> , :ARTWORK_75_Grinding , :ARTWORK_44_Packing_3 , :ARTWORK_79_Polishing , :ARTWORK_79_Resting , :ARTWORK_78_MeasuringAndBoxesMaking , <http://www.semanticweb.org/ontologies/Daan/2020/BarbaraNanning#ARTWORK_73_ExaminingQuality(Result)> , :ARTWORK_43_Packing_4 , :ARTWORK_78_Transporting_2 , <http://www.semanticweb.org/ontologies/Daan/2020/BarbaraNanning#ARTWORK_74_ExaminingQuality(FinalResult)> , :ARTWORK_43_Sawing , :ARTWORK_74_Transporting , :ARTWORK_76_Sensing , <http://www.semanticweb.org/ontologies/Daan/2020/BarbaraNanning#ARTWORK_80_ExaminingQuality(FinalResult)> , :ARTWORK_74_Packing_2 , <http://www.semanticweb.org/ontologies/Daan/2020/BarbaraNanning#ARTWORK_78_ExaminingQuality(CheckForIrregularitiesInTheGlass)> , <http://www.semanticweb.org/ontologies/Daan/2020/BarbaraNanning#ARTWORK_78_ExaminingQuality(FinalResult)> , :ARTWORK_73_MeasuringAndBoxesMaking , :ARTWORK_76_MeasuringAndBoxesMaking , :ARTWORK_43_Transporting_4 , <http://www.semanticweb.org/ontologies/Daan/2020/BarbaraNanning#ARTWORK_76_ExaminingQuality(FinalResult)> , <http://www.semanticweb.org/ontologies/Daan/2020/BarbaraNanning#ARTWORK_75_ExaminingQuality(CheckForIrregularitiesInTheGlass)> , :ARTWORK_75_Packing , :ARTWORK_76_Packing_2 , :ARTWORK_73_Transporting_4 , :ARTWORK_74_Polishing , :ARTWORK_80_Grinding , :ARTWORK_74_Sawing , :ARTWORK_43_Packing_3 , :ARTWORK_75_Polishing , :ARTWORK_75_Resting , :ARTWORK_75_Transporting_2 , <http://www.semanticweb.org/ontologies/Daan/2020/BarbaraNanning#ARTWORK_80_ExaminingQuality(Result)> , :ARTWORK_73_Transporting_3 , :ARTWORK_43_Transporting_3 , :ARTWORK_76_Transporting_2 , :ARTWORK_80_Sawing , :ARTWORK_43_MeasuringAndBoxesMaking , :ARTWORK_78_Grinding , :ARTWORK_43_Packing_2 , :ARTWORK_77_Packing_2 , :ARTWORK_44_Transporting_4 , <http://www.semanticweb.org/ontologies/Daan/2020/BarbaraNanning#ARTWORK_44_ExaminingQuality(FinalResult)> , :ARTWORK_78_Sawing , <http://www.semanticweb.org/ontologies/Daan/2020/BarbaraNanning#ARTWORK_74_ExaminingQuality(Result)> , :ARTWORK_79_Transporting , :ARTWORK_74_Transporting_3 , :ARTWORK_75_Packing_2 , :ARTWORK_43_Transporting_2 , :ARTWORK_80_Packing_2 , :ARTWORK_74_Sensing , :ARTWORK_76_Resting , :ARTWORK_79_Packing_3 , :ARTWORK_79_Packing , :ARTWORK_73_Packing_2 , :ARTWORK_44_Sensing , :ARTWORK_44_Transporting , :ARTWORK_77_Signing , :ARTWORK_77_Transporting , :ARTWORK_80_Transporting_2 , :ARTWORK_74_Transporting_2 , :ARTWORK_44_Grinding , :ARTWORK_76_Packing , <http://www.semanticweb.org/ontologies/Daan/2020/BarbaraNanning#ARTWORK_80_ExaminingQuality(CheckForIrregularitiesInTheGlass)> , :ARTWORK_80_MeasuringAndBoxesMaking , :ARTWORK_80_Sensing , :ARTWORK_76_Transporting , :ARTWORK_78_Sensing , :ARTWORK_77_Sensing , :ARTWORK_78_Packing_3 , :ARTWORK_76_Packing_3 , :ARTWORK_76_Sandblasting , :ARTWORK_77_Transporting_2 , :ARTWORK_78_Transporting_3 , :ARTWORK_44_Transporting_2 , <http://www.semanticweb.org/ontologies/Daan/2020/BarbaraNanning#ARTWORK_77_ExaminingQuality(Result)> , :ARTWORK_73_Sandblasting , :ARTWORK_79_MeasuringAndBoxesMaking , :ARTWORK_73_Packing_4 , :ARTWORK_76_Transporting_4 , :ARTWORK_73_Transporting , <http://www.semanticweb.org/ontologies/Daan/2020/BarbaraNanning#ARTWORK_79_ExaminingQuality(Result)> , :ARTWORK_79_Sensing , :ARTWORK_77_Polishing , :ARTWORK_75_Signing , :ARTWORK_80_Transporting , :ARTWORK_75_Transporting , :ARTWORK_75_Transporting_3 , :ARTWORK_77_Sawing , :ARTWORK_44_Sawing , :ARTWORK_79_Transporting_4 , <http://www.semanticweb.org/ontologies/Daan/2020/BarbaraNanning#ARTWORK_76_ExaminingQuality(CheckForIrregularitiesInTheGlass)> , :ARTWORK_78_Resting , :ARTWORK_78_Polishing , :ARTWORK_44_Polishing , :ARTWORK_44_Packing_2 , <http://www.semanticweb.org/ontologies/Daan/2020/BarbaraNanning#ARTWORK_79_ExaminingQuality(CheckForIrregularitiesInTheGlass)> , <http://www.semanticweb.org/ontologies/Daan/2020/BarbaraNanning#ARTWORK_73_ExaminingQuality(CheckForIrregularitiesInTheGlass)> , :ARTWORK_78_Packing , :ARTWORK_73_Sawing , :ARTWORK_80_Packing_3 , :ARTWORK_79_Transporting_2 , :ARTWORK_77_Resting , :ARTWORK_80_Sandblasting , :ARTWORK_74_Packing_4 , :ARTWORK_43_Transporting , :ARTWORK_73_Packing , :ARTWORK_43_Resting , :ARTWORK_76_Grinding , :ARTWORK_77_Transporting_4 , <http://www.semanticweb.org/ontologies/Daan/2020/BarbaraNanning#ARTWORK_78_ExaminingQuality(Result)> , :ARTWORK_43_Signing , <http://www.semanticweb.org/ontologies/Daan/2020/BarbaraNanning#ARTWORK_76_ExaminingQuality(CheckForIrregularitiesInTheGlass)_2> , :ARTWORK_80_Transporting_3 , <http://www.semanticweb.org/ontologies/Daan/2020/BarbaraNanning#ARTWORK_73_ExaminingQuality(FinalResult)> , :ARTWORK_79_Signing , :ARTWORK_43_Grinding , :ARTWORK_80_Packing , :ARTWORK_44_Packing , :ARTWORK_77_Transporting_3 , :ARTWORK_44_Packing_4 , :ARTWORK_76_Polishing , :ARTWORK_75_Sandblasting , <http://www.semanticweb.org/ontologies/Daan/2020/BarbaraNanning#ARTWORK_43_ExaminingQuality(FinalResult)> , :ARTWORK_43_Sensing , :ARTWORK_79_Sawing , :ARTWORK_79_Packing_2 , :ARTWORK_75_Transporting_4 , :ARTWORK_75_Packing_4 , :ARTWORK_43_Packing , <http://www.semanticweb.org/ontologies/Daan/2020/BarbaraNanning#ARTWORK_43_ExaminingQuality(Result)> , <http://www.semanticweb.org/ontologies/Daan/2020/BarbaraNanning#ARTWORK_75_ExaminingQuality(Result)> , <http://www.semanticweb.org/ontologies/Daan/2020/BarbaraNanning#ARTWORK_77_ExaminingQuality(FinalResult)> , :ARTWORK_77_Packing_4 , :ARTWORK_78_Transporting , :ARTWORK_80_Polishing , :ARTWORK_77_Grinding , :ARTWORK_43_Polishing , <http://www.semanticweb.org/ontologies/Daan/2020/BarbaraNanning#ARTWORK_44_ExaminingQuality(CheckForIrregularitiesInTheGlass)> , :ARTWORK_78_Signing , :ARTWORK_76_Signing , :ARTWORK_73_Grinding , :ARTWORK_78_Packing_2 , :ARTWORK_73_Signing , :ARTWORK_73_Polishing , :ARTWORK_77_Packing_3 , :ARTWORK_74_Packing , :ARTWORK_73_Resting , :ARTWORK_80_Signing , :ARTWORK_74_Signing , :ARTWORK_77_MeasuringAndBoxesMaking , :ARTWORK_44_Signing , :ARTWORK_76_Transporting_3 , :ARTWORK_74_Transporting_4 ;
        :Works-For    <http://www.semanticweb.org/ontologies/Daan/2020/BarbaraNanning#Ale%C5%A1Zv%C4%9B%C5%99ina&AZ-Design> .

:Lausanne  a          :City , owl:NamedIndividual ;
        rdfs:comment  "Lausanne is a city in Switzerland."@en ;
        rdfs:label    "Lausanne"@en ;
        :Located-In   :Switzerland ;
        :Location-Of  <http://www.semanticweb.org/ontologies/Daan/2020/BarbaraNanning#MuseeDeDesignEtd'artsAppliquesContemporains> , <http://www.semanticweb.org/ontologies/Daan/2020/BarbaraNanning#CollectionMuseeDeDesignEtd'artsAppliquesContemporains> , :Artwork_74 .

:ARTWORK_46_Cooling  a    :Cooling , owl:NamedIndividual ;
        rdfs:comment      "Instance of an activity which is part of the creation process of ARTWORK_46."@en ;
        rdfs:label        "ARTWORK_46_Cooling"@en ;
        :Followed-By      :ARTWORK_46_Packing ;
        :Follows          <http://www.semanticweb.org/ontologies/Daan/2020/BarbaraNanning#ARTWORK_46_ExaminingQuality(Shape/Form)> ;
        :Has-Duration     <http://www.semanticweb.org/ontologies/Daan/2020/BarbaraNanning#2018> ;
        :Involves         <http://www.semanticweb.org/ontologies/Daan/2020/BarbaraNanning#JiriPacinek(CZ)> , <http://www.semanticweb.org/ontologies/Daan/2020/BarbaraNanning#JessicaHomich(USA)> ;
        :Located-In       :Lindava ;
        :Part-Of          :Creation_Artwork_46 ;
        :Requires-Use-Of  :AnnealingKiln .

:Leather  a               :Man-Made_Material , owl:NamedIndividual ;
        rdfs:comment      "Leather is a material made from the skin of an animal (e.g. cows)."@en ;
        rdfs:label        "Leather"@en ;
        :Is-Processed-In  :GildingCushion , :GildersKnife .

:ARTWORK_75_Sandblasting
        a                 :Sandblasting , owl:NamedIndividual ;
        rdfs:comment      "Instance of an activity which is part of the creation process of ARTWORK_75."@en ;
        rdfs:label        "ARTWORK_75_Sandblasting"@en ;
        :Followed-By      :ARTWORK_75_Signing ;
        :Follows          :ARTWORK_75_Transporting_2 ;
        :Has-Duration     <http://www.semanticweb.org/ontologies/Daan/2020/BarbaraNanning#2018> ;
        :Involves         :BarbaraNanning , :AlešZvěřina ;
        :Located-In       :CzechRepublic ;
        :Part-Of          :Creation_Artwork_75 ;
        :Requires-Use-Of  :AirCompressor .

:ARTWORK_36_Packing_8
        a              :Packing , owl:NamedIndividual ;
        rdfs:comment   "Instance of an activity which is part of the creation process of ARTWORK_36."@en ;
        rdfs:label     "ARTWORK_36_Packing_8"@en ;
        :Followed-By   :ARTWORK_36_Documenting_2 ;
        :Follows       :ARTWORK_36_Photographing_2 ;
        :Has-Duration  <http://www.semanticweb.org/ontologies/Daan/2020/BarbaraNanning#2019> ;
        :Involves      :BarbaraNanning ;
        :Located-In    <http://www.semanticweb.org/ontologies/Daan/2020/BarbaraNanning#Ouderkerka/dAmstel> ;
        :Part-Of       :Creation_Artwork_36 .

<http://vocab.getty.edu/aat/300025408>
        a                    owl:Class ;
        owl:equivalentClass  :Glass_Blower .

:Heating  a              owl:Class ;
        rdfs:comment     "Heating is an activity in which the temperature of a thing is increased."@en ;
        rdfs:label       "Heating"@en ;
        rdfs:subClassOf  :Activity .

:Place  a                owl:Class ;
        rdfs:comment     "A place is a particular location."@en ;
        rdfs:label       "Place"@en ;
        rdfs:subClassOf  :Entity .

:ARTWORK_36_Resting_2
        a                 owl:NamedIndividual , :Resting ;
        rdfs:comment      "Instance of an activity which is part of the creation process of ARTWORK_36."@en ;
        rdfs:label        "ARTWORK_36_Resting_2"@en ;
        :Followed-By      <http://www.semanticweb.org/ontologies/Daan/2020/BarbaraNanning#ARTWORK_36_ExaminingQuality(CheckForIrregularitiesInTheGlass)_2> ;
        :Follows          :ARTWORK_36_Transporting_4 ;
        :Has-Duration     <http://www.semanticweb.org/ontologies/Daan/2020/BarbaraNanning#2019> ;
        :Involves         :AlešZvěřina ;
        :Located-In       :NovyBor ;
        :Part-Of          :Creation_Artwork_36 ;
        :Requires-Use-Of  :AnnealingKiln .

<http://www.wikidata.org/entity/Q1072404>
        a       owl:DatatypeProperty .

<http://www.wikidata.org/entity/Q929186>
        a       owl:Class .

:Artwork_78  a        :Glass_Artwork , owl:NamedIndividual ;
        rdfs:comment  "Artwork by Barbara Nanning displayed in \"Barbara Nanning Eeuwige Beweging\" by Eliens (2019)."@en ;
        rdfs:label    "Verre églomisé"@en ;
        :Created-By   :Creation_Artwork_78 ;
        :Has-Depth    "23"^^xsd:decimal ;
        :Has-Height   "19"^^xsd:decimal ;
        :Has-Width    "24"^^xsd:decimal ;
        :Is-Unica     "Yes"@en ;
        :Made-By      <http://www.semanticweb.org/ontologies/Daan/2020/BarbaraNanning#Ale%C5%A1Zv%C4%9B%C5%99ina&AZ-Design> , :VáçlavNovák_Doksy_CzechRepublic , :BarbaraNanning , :LASVITAJETO ;
        :Part-Of      :CollectionWithUnknownOwner ;
        :Shown-By     :Image_Artwork_78 .

[ a            owl:AllDisjointClasses ;
  owl:members  ( :First_Glass_Blower :Fourth_Glass_Blower :Master_Glass_Blower :Second_Glass_Blower :Third_Glass_Blower )
] .

j.3:    a                owl:Class ;
        rdfs:comment     "Examining Quality (Check for Irregularities in the Glass) is an activity conducted by the creator in which the iregularities in the glass are examined."@en ;
        rdfs:label       "Examining Quality (Check for Irregularities in the Glass)"@en ;
        rdfs:subClassOf  :Activity .

:City   a                    owl:Class ;
        rdfs:comment         "A city is a large town."@en ;
        rdfs:label           "City"@en ;
        rdfs:subClassOf      :Place ;
        owl:disjointWith     :Country ;
        owl:equivalentClass  <http://www.wikidata.org/entity/Q515> .

:ARTWORK_79_Transporting
        a              :Transporting , owl:NamedIndividual ;
        rdfs:comment   "Instance of an activity which is part of the creation process of ARTWORK_79."@en ;
        rdfs:label     "ARTWORK_79_Transporting"@en ;
        :Followed-By   :ARTWORK_79_Resting ;
        :Follows       :ARTWORK_79_Packing ;
        :Has-Duration  <http://www.semanticweb.org/ontologies/Daan/2020/BarbaraNanning#2018> ;
        :Involves      :AlešZvěřina , :BarbaraNanning ;
        :Located-In    :CzechRepublic ;
        :Part-Of       :Creation_Artwork_79 .

:Artwork_46  a        owl:NamedIndividual , :Glass_Artwork ;
        rdfs:comment  "Artwork_46 is a glass artwork made by Barbara Nanning."@en ;
        rdfs:label    "Coloured Shadows Yellow River"@en ;
        :Created-By   :Creation_Artwork_46 ;
        :Has-Depth    "27"^^xsd:decimal ;
        :Has-Height   "27"^^xsd:decimal , "20"^^xsd:decimal ;
        :Is-Unica     "Yes"@en ;
        :Made-By      :VRIJGLASZaandam , <http://www.semanticweb.org/ontologies/Daan/2020/BarbaraNanning#Ji%C5%99%C3%ADPa%C4%8DinekLindava(CZ)> , :BullseyeGlassSplinterEnDeVosch , <http://www.semanticweb.org/ontologies/Daan/2020/BarbaraNanning#Ale%C5%A1Zv%C4%9B%C5%99ina&AZ-Design> , :BarbaraNanning ;
        :Made-Out-Of  :BullseyeGlass ;
        :Shown-By     :Image_Artwork_46 .

:ARTWORK_77_MeasuringAndBoxesMaking
        a              owl:NamedIndividual , :Measuring_and_Boxes_Making ;
        rdfs:comment   "Instance of an activity which is part of the creation process of ARTWORK_77."@en ;
        rdfs:label     "ARTWORK_77_Measuring and Boxes Making"@en ;
        :Followed-By   :ARTWORK_77_Packing_2 ;
        :Follows       <http://www.semanticweb.org/ontologies/Daan/2020/BarbaraNanning#ARTWORK_77_ExaminingQuality(Result)> ;
        :Has-Duration  <http://www.semanticweb.org/ontologies/Daan/2020/BarbaraNanning#2018> ;
        :Involves      :BarbaraNanning , :AlešZvěřina ;
        :Located-In    :CzechRepublic ;
        :Part-Of       :Creation_Artwork_77 .

<BarbaraNanning/Vladim%C3%ADr%C5%BD%C3%ADlajr.>
        a             :Grinder_2 , owl:NamedIndividual ;
        rdfs:comment  "Vladimír Žíla Jr. is a Grinder 2."@en ;
        rdfs:label    "Vladimír Žíla Jr."@en .

:Metal_Worker_2  a       owl:Class ;
        rdfs:comment     "A Metal Worker 2 is an actor who is the second member of a team responsible for creating metal objects or dealing with metal material."@en ;
        rdfs:label       "Metal Worker 2"@en ;
        rdfs:subClassOf  :Metal_Worker .

<http://www.europeana.eu/schemas/edm/isShownAt>
        a                       owl:ObjectProperty ;
        owl:equivalentProperty  :Shown-By .

:ARTWORK_74_Photographing
        a              owl:NamedIndividual , :Photographing ;
        rdfs:comment   "Instance of an activity which is part of the creation process of ARTWORK_74."@en ;
        rdfs:label     "ARTWORK_74_Photographing"@en ;
        :Followed-By   :ARTWORK_74_Documenting ;
        :Follows       :ARTWORK_74_Transporting_4 ;
        :Has-Duration  <http://www.semanticweb.org/ontologies/Daan/2020/BarbaraNanning#2008> ;
        :Involves      <http://www.semanticweb.org/ontologies/Daan/2020/BarbaraNanning#TomHaartsen_Ouderkerka/dAmstel(NL)> , :BarbaraNanning ;
        :Located-In    :CzechRepublic ;
        :Part-Of       :Creation_Artwork_74 .

<http://vocab.getty.edu/aat/300012941>
        a           owl:NamedIndividual ;
        owl:sameAs  :Rubber .

:DiamondSaw  a        :Tool , owl:NamedIndividual ;
        rdfs:comment  "A diamond saw is a saw created with diamonds used to cut hard materials (e.g. glass)."@en ;
        rdfs:label    "Diamond Saw"@en ;
        :Used-For     :ARTWORK_43_Sawing , :ARTWORK_44_Sawing , :ARTWORK_77_Sawing , :ARTWORK_76_Sawing , :ARTWORK_78_Sawing , :ARTWORK_79_Sawing , :ARTWORK_73_Sawing , :ARTWORK_74_Sawing , :ARTWORK_75_Sawing , :ARTWORK_80_Sawing .

:LASVITAJETO  a       owl:NamedIndividual , :Glass_Studio ;
        rdfs:comment  "LASVIT AJETO is a glass blowing studio in Czech Republic."@en ;
        rdfs:label    "LASVIT AJETO"@en ;
        :Employed     <http://www.semanticweb.org/ontologies/Daan/2020/BarbaraNanning#LukasHavlas(CZ)> , <http://www.semanticweb.org/ontologies/Daan/2020/BarbaraNanning#JiriMoravec(CZ)> , <http://www.semanticweb.org/ontologies/Daan/2020/BarbaraNanning#RostislavMaterka(CZ)> , <http://www.semanticweb.org/ontologies/Daan/2020/BarbaraNanning#RomanTomis(CZ)> , <http://www.semanticweb.org/ontologies/Daan/2020/BarbaraNanning#RadekKoten(CZ)> , <http://www.semanticweb.org/ontologies/Daan/2020/BarbaraNanning#AlesVacek(CZ)> , <http://www.semanticweb.org/ontologies/Daan/2020/BarbaraNanning#Tom%C3%A1%C5%A1Moravec(CZ)> , <http://www.semanticweb.org/ontologies/Daan/2020/BarbaraNanning#RobertHlavacek(CZ)> , :LuděkKout ;
        :Located-In   :Lindava ;
        :Maker-Of     :AJETORedGlass , :AJETOWhiteGlass , :AJETOClearGlass , :AJETOBlackGlass , :AJETOAmberGlass , :Artwork_73 , :Artwork_75 , :AJETOUraniumGlass , :Artwork_79 , :Artwork_74 , :Artwork_78 , :AJETOGreenGlass , :AJETOSmokeGlass , :Artwork_77 , :Artwork_44 , :Artwork_76 , :AJETOAlexandriteGlass , :Artwork_43 , :AJETOBlueGlass , :Artwork_80 .

<http://www.semanticweb.org/ontologies/Daan/2020/BarbaraNanning#ARTWORK_78_ExaminingQuality(Result)>
        a              owl:NamedIndividual , j.0: ;
        rdfs:comment   "Instance of an activity which is part of the creation process of ARTWORK_78."@en ;
        rdfs:label     "ARTWORK_78_Examining Quality (Result)"@en ;
        :Followed-By   :ARTWORK_78_MeasuringAndBoxesMaking ;
        :Follows       :ARTWORK_78_Polishing ;
        :Has-Duration  <http://www.semanticweb.org/ontologies/Daan/2020/BarbaraNanning#2016> ;
        :Involves      :BarbaraNanning , :AlešZvěřina ;
        :Located-In    :CzechRepublic ;
        :Part-Of       :Creation_Artwork_78 .

:ARTWORK_80_SetupAndTestingOfTheMetalMold_2
        a                 :Setup_and_Testing_of_the_Metal_Mold , owl:NamedIndividual ;
        rdfs:comment      "Instance of an activity which is part of the creation process of ARTWORK_80."@en ;
        rdfs:label        "ARTWORK_80_Setup and Testing of the Metal Mold_2"@en ;
        :Followed-By      :ARTWORK_80_ApplyingClearGlassBell ;
        :Follows          :ARTWORK_80_ExaminingTheQualityOfTheGlass ;
        :Has-Duration     <http://www.semanticweb.org/ontologies/Daan/2020/BarbaraNanning#2018> ;
        :Involves         <http://www.semanticweb.org/ontologies/Daan/2020/BarbaraNanning#JiriMoravec(CZ)> , <http://www.semanticweb.org/ontologies/Daan/2020/BarbaraNanning#RadekKoten(CZ)> , :AssistantOfBarbara , <http://www.semanticweb.org/ontologies/Daan/2020/BarbaraNanning#Tom%C3%A1%C5%A1Moravec(CZ)> , :BarbaraNanning , <http://www.semanticweb.org/ontologies/Daan/2020/BarbaraNanning#LukasHavlas(CZ)> ;
        :Located-In       :CzechRepublic ;
        :Part-Of          :Creation_Artwork_80 ;
        :Requires-Use-Of  :InterchangeableMetalMoldSetup .

<http://www.wikidata.org/entity/Q12033551>
        a       owl:NamedIndividual .

<http://www.semanticweb.org/ontologies/Daan/2020/BarbaraNanning#ARTWORK_79_ExaminingQuality(Shape/Form)>
        a                 j.2: , owl:NamedIndividual ;
        rdfs:comment      "Instance of an activity which is part of the creation process of ARTWORK_79."@en ;
        rdfs:label        "ARTWORK_79_Examining Quality (Shape/Form)"@en ;
        :Followed-By      :ARTWORK_79_Translocating ;
        :Follows          :ARTWORK_79_Modeling ;
        :Has-Duration     <http://www.semanticweb.org/ontologies/Daan/2020/BarbaraNanning#2018> ;
        :Involves         <http://www.semanticweb.org/ontologies/Daan/2020/BarbaraNanning#RadekKoten(CZ)> , :BarbaraNanning , :LuděkKout ;
        :Located-In       :CzechRepublic ;
        :Part-Of          :Creation_Artwork_79 ;
        :Requires-Use-Of  :BlowingPipe , :GloryHole , :Pontis .

<http://www.semanticweb.org/ontologies/Daan/2020/BarbaraNanning#RostislavMaterka(CZ)>
        a             owl:NamedIndividual , :First_Glass_Blower ;
        rdfs:comment  "Rostislav Materka (CZ) is a First Glass Blower."@en ;
        rdfs:label    "Rostislav Materka (CZ)"@en ;
        :Involved-In  :ARTWORK_74_Modeling , :ARTWORK_43_ApplyingClearGlassBell , :ARTWORK_43_ApplyingExtraColour , :ARTWORK_78_Modeling , :ARTWORK_78_ApplyingExtraColour , :ARTWORK_74_ApplyingExtraColour_2 , :ARTWORK_78_ApplyingClearGlassBell , :ARTWORK_74_ApplyingExtraColour , :ARTWORK_78_SetupAndTestingOfTheMetalMold_2 , :ARTWORK_43_SetupAndTestingOfTheMetalMold_2 , :ARTWORK_74_SetupAndTestingOfTheMetalMold_2 , :ARTWORK_78_SetupAndTestingOfTheMetalMold , :ARTWORK_74_ApplyingClearGlassBell , :ARTWORK_43_Glassblowing , :ARTWORK_74_SetupAndTestingOfTheMetalMold , :ARTWORK_74_Glassblowing , :ARTWORK_43_SetupAndTestingOfTheMetalMold , :ARTWORK_78_Glassblowing , :ARTWORK_43_Modeling ;
        :Works-For    :LASVITAJETO .

<http://www.semanticweb.org/ontologies/Daan/2020/BarbaraNanning#2018>
        a             owl:NamedIndividual , :Timespan ;
        rdfs:comment  "2018 is a Timespan."@en ;
        rdfs:label    "2018"@en ;
        owl:sameAs    <http://www.wikidata.org/entity/Q25291> ;
        :Duration-Of  :Creation_Artwork_80 , :Creation_Artwork_73 , :Creation_Artwork_44 , :Creation_Artwork_76 , :Creation_Artwork_77 , :Creation_Artwork_79 .

:Sensing  a              owl:Class ;
        rdfs:comment     "Sensing is an activity in which an actor stops to take a breath and reevaluates. It requires creative problem solving."@en ;
        rdfs:label       "Sensing"@en ;
        rdfs:subClassOf  :Activity .

:ARTWORK_36_PickingUpColouredCanesPattern
        a                 :Picking_up_Coloured_Canes_Pattern , owl:NamedIndividual ;
        rdfs:comment      "Instance of an activity which is part of the creation process of ARTWORK_36."@en ;
        rdfs:label        "ARTWORK_36_Picking up Coloured Canes Pattern"@en ;
        :Followed-By      :ARTWORK_36_HeatingMetalMold ;
        :Follows          :ARTWORK_36_ApplyingClearGlassBell ;
        :Has-Duration     <http://www.semanticweb.org/ontologies/Daan/2020/BarbaraNanning#2015> ;
        :Involves         :BarbaraNanning , :GertBullée , <http://www.semanticweb.org/ontologies/Daan/2020/BarbaraNanning#RobertLenner(CZ)> , <http://www.semanticweb.org/ontologies/Daan/2020/BarbaraNanning#MarekEffmert(CZ)> , <http://www.semanticweb.org/ontologies/Daan/2020/BarbaraNanning#MiaLerssi(DN)> , <http://www.semanticweb.org/ontologies/Daan/2020/BarbaraNanning#MarekBrathko(CZ)> , <http://www.semanticweb.org/ontologies/Daan/2020/BarbaraNanning#JessicaHomich(USA)> ;
        :Located-In       :Zaandam ;
        :Part-Of          :Creation_Artwork_36 ;
        :Requires-Use-Of  :Gloves , :Jacks , :GloryHole , :Garage , :Beeswax , :Blocks , :BlowingPipe , :Furnace , :GrindingWheel , :DiamondShears , :Water , :Fork , :Paper , :PropaneTorch , :Hook , :AirCompressor , :StraightShears , :Tagliol , :AnnealingKiln , :Pontis , :Marver , :YokeOfSupport , :FusingKiln .

:ARTWORK_39_PreparingForBlowing
        a                 owl:NamedIndividual , :Preparing_for_Blowing ;
        rdfs:comment      "Instance of an activity which is part of the creation process of ARTWORK_39."@en ;
        rdfs:label        "ARTWORK_39_Preparing for Blowing"@en ;
        :Followed-By      :ARTWORK_39_FillingKilnsWithMetalBowl ;
        :Follows          :ARTWORK_39_TransportingMetalBowlWithPanel ;
        :Has-Duration     <http://www.semanticweb.org/ontologies/Daan/2020/BarbaraNanning#2015> ;
        :Involves         :BarbaraNanning , :DurkValkema , <http://www.semanticweb.org/ontologies/Daan/2020/BarbaraNanning#MiaLerssi(DN)> ;
        :Located-In       :Zaandam ;
        :Part-Of          :Creation_Artwork_39 ;
        :Requires-Use-Of  :Garage , :BlowingPipe , :FusingKiln , :Water , :Paper , :AnnealingKiln , :Furnace .

:PureDucat  a                 :Gold_Leaf , owl:NamedIndividual ;
        rdfs:comment          "Pure ducat is gold leaf which is ideal for gilding outdoors."@en ;
        rdfs:label            "Pure Ducat"@en ;
        :Carat                23.5 ;
        :Is-Processed-During  :ARTWORK_73_Gilding , :ARTWORK_79_Gilding , :ARTWORK_78_Gilding , :ARTWORK_75_Gilding , :ARTWORK_76_Gilding ;
        :Is-Processed-In      :Artwork_75 , :Artwork_78 , :Artwork_73 , :Artwork_76 , :Artwork_79 .

:Iron   a                 :Natural_Material , owl:NamedIndividual ;
        rdfs:comment      "Iron is a solid and metal material and the chemical element of atomic number 26."@en ;
        rdfs:label        "Iron"@en ;
        :Is-Processed-In  :InterchangeableMetalMoldSetup , :BitIron .

:CollectionJ.LohmannGallery
        a               :Collection , owl:NamedIndividual ;
        rdfs:comment    "Collection maintained by the J. Lohmann Gallery."@en ;
        rdfs:label      "Collection J. Lohmann Gallery"@en ;
        :Consists-Of    :Artwork_44 ;
        :Located-In     :NewYork ;
        :Maintained-By  :J.LohmannGallery .

:GrindingWheel  a     owl:NamedIndividual , :Tool ;
        rdfs:comment  "A grinding wheel is a wheel used for grinding objects."@en ;
        rdfs:label    "Grinding Wheel"@en ;
        :Used-For     :ARTWORK_80_Grinding , :ARTWORK_74_Grinding , :ARTWORK_76_Grinding , :ARTWORK_44_Grinding , :ARTWORK_78_Grinding , :ARTWORK_77_Grinding , :ARTWORK_79_Grinding , :ARTWORK_43_Grinding , :ARTWORK_73_Grinding , :ARTWORK_75_Grinding .

:Image_Artwork_73  a            :Digital_Image , owl:NamedIndividual ;
        rdfs:comment            "Image of an artwork by Barbara Nanning displayed in \"Barbara Nanning Eeuwige Beweging\" by Eliens (2019)."@en ;
        rdfs:label              "Image_Artwork_73"@en ;
        :Representation-Source  "Tom Haartsen_Ouderkerk a/d Amstel (NL)"@en ;
        :Shows                  :Artwork_73 .

<http://www.semanticweb.org/ontologies/Daan/2020/BarbaraNanning#ARTWORK_36_ExaminingQuality(FinalResult)_2>
        a              j.1: , owl:NamedIndividual ;
        rdfs:comment   "Instance of an activity which is part of the creation process of ARTWORK_36."@en ;
        rdfs:label     "ARTWORK_36_Examining Quality (Final Result)_2"@en ;
        :Followed-By   :ARTWORK_36_Packing_7 ;
        :Follows       :ARTWORK_36_Signing_2 ;
        :Has-Duration  <http://www.semanticweb.org/ontologies/Daan/2020/BarbaraNanning#2019> ;
        :Involves      :BarbaraNanning , :AlešZvěřina ;
        :Located-In    :NovyBor ;
        :Part-Of       :Creation_Artwork_36 .

:ARTWORK_77_Transporting_4
        a              owl:NamedIndividual , :Transporting ;
        rdfs:comment   "Instance of an activity which is part of the creation process of ARTWORK_77."@en ;
        rdfs:label     "ARTWORK_77_Transporting_4"@en ;
        :Followed-By   :ARTWORK_77_Photographing ;
        :Follows       :ARTWORK_77_Packing_4 ;
        :Has-Duration  <http://www.semanticweb.org/ontologies/Daan/2020/BarbaraNanning#2018> ;
        :Involves      :BarbaraNanning , :AlešZvěřina ;
        :Located-In    :CzechRepublic ;
        :Part-Of       :Creation_Artwork_77 .

:Applying_Extra_Colour
        a                owl:Class ;
        rdfs:comment     "Applying extra colour is an activity in which glass of a different colour is added to (a bell of) molten glass or pipe. The colour is either put directly on the pipe or placed as an overlay on a small clear bubble."@en ;
        rdfs:label       "Applying Extra Colour"@en ;
        rdfs:subClassOf  :Activity .

:ARTWORK_77_ApplyingExtraColour
        a                 owl:NamedIndividual , :Applying_Extra_Colour ;
        rdfs:comment      "Instance of an activity which is part of the creation process of ARTWORK_77."@en ;
        rdfs:label        "ARTWORK_77_Applying Extra Colour"@en ;
        :Followed-By      :ARTWORK_77_HeatingMetalMold ;
        :Follows          :ARTWORK_77_ApplyingClearGlassBell ;
        :Has-Duration     <http://www.semanticweb.org/ontologies/Daan/2020/BarbaraNanning#2018> ;
        :Involves         :BarbaraNanning , <http://www.semanticweb.org/ontologies/Daan/2020/BarbaraNanning#RadekKoten(CZ)> , <http://www.semanticweb.org/ontologies/Daan/2020/BarbaraNanning#LukasHavlas(CZ)> ;
        :Located-In       :CzechRepublic ;
        :Part-Of          :Creation_Artwork_77 ;
        :Processes        :AJETOSmokeGlass ;
        :Requires-Use-Of  :YokeOfSupport , :AirCompressor , :Tagliol , :Fork , :GloryHole , :Hook , :CeramicPotFilledWithGlass , :Garage , :BlowingPipe , :StraightShears , :Jacks , :IcePick , :Furnace , :Marver , :AnnealingKiln , :Paper , :Water , :DiamondShears , :Pincet , :Beeswax , :Blocks , :Pontis .

:ARTWORK_36_DecidingColourPalette
        a                 owl:NamedIndividual , :Deciding_Colour_Palette ;
        rdfs:comment      "Instance of an activity which is part of the creation process of ARTWORK_36."@en ;
        rdfs:label        "ARTWORK_36_Deciding Colour Palette"@en ;
        :Followed-By      :ARTWORK_36_MakingPatternsWithColouredCanesInTheMetalBowl ;
        :Follows          :ARTWORK_36_TransportingColouredCanes_2 ;
        :Has-Duration     <http://www.semanticweb.org/ontologies/Daan/2020/BarbaraNanning#2015> ;
        :Involves         :BarbaraNanning ;
        :Located-In       :Amsterdam ;
        :Part-Of          :Creation_Artwork_36 ;
        :Requires-Use-Of  :Computer .

:ARTWORK_78_Transporting
        a              owl:NamedIndividual , :Transporting ;
        rdfs:comment   "Instance of an activity which is part of the creation process of ARTWORK_78."@en ;
        rdfs:label     "ARTWORK_78_Transporting"@en ;
        :Followed-By   :ARTWORK_78_Resting ;
        :Follows       :ARTWORK_78_Packing ;
        :Has-Duration  <http://www.semanticweb.org/ontologies/Daan/2020/BarbaraNanning#2008> ;
        :Involves      :BarbaraNanning , :AlešZvěřina ;
        :Located-In    :CzechRepublic ;
        :Part-Of       :Creation_Artwork_78 .

:ARTWORK_39_Documenting
        a              :Documenting , owl:NamedIndividual ;
        rdfs:comment   "Instance of an activity which is part of the creation process of ARTWORK_39."@en ;
        rdfs:label     "ARTWORK_39_Documenting"@en ;
        :Finishes      :Creation_Artwork_39 ;
        :Follows       :ARTWORK_39_Packing_3 ;
        :Has-Duration  <http://www.semanticweb.org/ontologies/Daan/2020/BarbaraNanning#2015> ;
        :Involves      :BarbaraNanning ;
        :Located-In    :Amsterdam ;
        :Part-Of       :Creation_Artwork_39 .

:AnnealingKiln  a     :Equipment , owl:NamedIndividual ;
        rdfs:comment  "An annealing kiln is a structure with process controllers in which things can be cooled."@en ;
        rdfs:label    "Annealing Kiln"@en ;
        :Used-For     :ARTWORK_74_ExaminingTheQualityOfTheGlass , :ARTWORK_75_Resting , :ARTWORK_77_Resting , :ARTWORK_78_ApplyingExtraColour , :ARTWORK_76_Glassblowing , :ARTWORK_75_ApplyingExtraColour , :ARTWORK_79_ApplyingExtraColour_2 , :ARTWORK_80_ExaminingTheQualityOfTheGlass , :ARTWORK_77_Cooling , :ARTWORK_75_ExaminingTheQualityOfTheGlass , :ARTWORK_44_Cooling , :ARTWORK_43_Cooling , :ARTWORK_78_Glassblowing , :ARTWORK_74_Glassblowing , :ARTWORK_74_ApplyingExtraColour_2 , :ARTWORK_43_ApplyingExtraColour , :ARTWORK_43_Glassblowing , :ARTWORK_76_ApplyingExtraColour , :ARTWORK_79_Cooling , :ARTWORK_73_Cooling , :ARTWORK_74_Cooling , :ARTWORK_73_ExaminingTheQualityOfTheGlass , :ARTWORK_77_ApplyingExtraColour , :ARTWORK_79_Glassblowing , :ARTWORK_77_ExaminingTheQualityOfTheGlass , :ARTWORK_43_Resting , :ARTWORK_76_Resting , :ARTWORK_44_Glassblowing , :ARTWORK_44_ApplyingExtraColour , :ARTWORK_78_Resting , :ARTWORK_79_ApplyingExtraColour , :ARTWORK_78_ExaminingTheQualityOfTheGlass , :ARTWORK_44_ExaminingTheQualityOfTheGlass , :ARTWORK_79_ExaminingTheQualityOfTheGlass , :ARTWORK_73_Glassblowing , :ARTWORK_80_Cooling , :ARTWORK_74_Resting , :ARTWORK_75_ApplyingExtraColour_2 , :ARTWORK_73_Resting , :ARTWORK_75_Cooling , :ARTWORK_77_Glassblowing , :ARTWORK_80_ApplyingExtraColour , :ARTWORK_76_Cooling , :ARTWORK_79_Resting , :ARTWORK_44_Resting , :ARTWORK_43_ExaminingTheQualityOfTheGlass , :ARTWORK_76_ApplyingExtraColour_2 , :ARTWORK_75_Glassblowing , :ARTWORK_74_ApplyingExtraColour , :ARTWORK_80_Resting , :ARTWORK_44_ApplyingExtraColour_2 , :ARTWORK_80_Glassblowing , :ARTWORK_78_Cooling , :ARTWORK_76_ExaminingTheQualityOfTheGlass .

:Slumping  a             owl:Class ;
        rdfs:comment     "Flat glass when placed in a kiln and heated can be molded to different shapes and forms."@en ;
        rdfs:label       "Slumping"@en ;
        rdfs:subClassOf  :Activity .

:Transporting  a         owl:Class ;
        rdfs:comment     "Transporting is an activity in which a thing is transported to a different location."@en ;
        rdfs:label       "Transporting"@en ;
        rdfs:subClassOf  :Activity .

:ARTWORK_74_Sensing  a  :Sensing , owl:NamedIndividual ;
        rdfs:comment   "Instance of an activity which is part of the creation process of ARTWORK_74."@en ;
        rdfs:label     "ARTWORK_74_Sensing"@en ;
        :Followed-By   :ARTWORK_74_Modeling ;
        :Follows       :ARTWORK_74_Glassblowing ;
        :Has-Duration  <http://www.semanticweb.org/ontologies/Daan/2020/BarbaraNanning#2008> ;
        :Involves      :BarbaraNanning , :AlešZvěřina , :LukášSvoboda ;
        :Located-In    :CzechRepublic ;
        :Part-Of       :Creation_Artwork_74 .

:Platinum  a                  owl:NamedIndividual , :Gold_Leaf ;
        rdfs:comment          "Platinum is a form of gold leaf which is alloyed with platinum."@en ;
        rdfs:label            "Platinum"@en ;
        :Carat                "24"^^xsd:decimal ;
        :Is-Processed-During  :ARTWORK_44_Gilding , :ARTWORK_43_Gilding , :ARTWORK_80_Gilding ;
        :Is-Processed-In      :Artwork_43 , :Artwork_80 , :Artwork_44 .

:ARTWORK_73_Transporting_2
        a              owl:NamedIndividual , :Transporting ;
        rdfs:comment   "Instance of an activity which is part of the creation process of ARTWORK_73."@en ;
        rdfs:label     "ARTWORK_73_Transporting_2"@en ;
        :Followed-By   :ARTWORK_73_Sandblasting ;
        :Follows       :ARTWORK_73_Packing_2 ;
        :Has-Duration  <http://www.semanticweb.org/ontologies/Daan/2020/BarbaraNanning#2018> ;
        :Involves      :BarbaraNanning , :AlešZvěřina ;
        :Located-In    :CzechRepublic ;
        :Part-Of       :Creation_Artwork_73 .

:ARTWORK_17_33_ProducingColouredCanes
        a                 :Producing_Coloured_Canes , owl:NamedIndividual ;
        rdfs:comment      "Instance of an activity which is part of the creation process of ARTWORK_17_33."@en ;
        rdfs:label        "ARTWORK_17_33_Producing Coloured Canes"@en ;
        :Followed-By      :ARTWORK_17_33_TransportingColouredCanes ;
        :Follows          :ARTWORK_17_33_DecidingColourPaletteAndPatterns ;
        :Has-Duration     <http://www.semanticweb.org/ontologies/Daan/2020/BarbaraNanning#2017> ;
        :Involves         <http://www.semanticweb.org/ontologies/Daan/2020/BarbaraNanning#RobertHlavacek(CZ)> , <http://www.semanticweb.org/ontologies/Daan/2020/BarbaraNanning#MiaLerssi(DN)> , :LuděkKout , :BarbaraNanning , <http://www.semanticweb.org/ontologies/Daan/2020/BarbaraNanning#RostislavMaterka(CZ)> , <http://www.semanticweb.org/ontologies/Daan/2020/BarbaraNanning#JessicaHomich(USA)> , <http://www.semanticweb.org/ontologies/Daan/2020/BarbaraNanning#AlesVacek(CZ)> , <http://www.semanticweb.org/ontologies/Daan/2020/BarbaraNanning#RomanTomis(CZ)> ;
        :Located-In       :Lindava ;
        :Part-Of          :Creation_Artwork_17_33 ;
        :Requires-Use-Of  :SharpeningStone , :Beeswax , :PropaneTorch , :Gloves , :StraightShears , :GloryHole , :Water , :Computer , :Marver , :DiamondShears , :Pontis , :FusingKiln , :Paper , :Furnace , :AnnealingKiln , :Tagliol , :YokeOfSupport , :AirCompressor , :Blocks , :BitIrons , :Garage , :Jacks , :GrindingWheel , :Hook .

:ARTWORK_36_SetupAndTestingOfTheMetalMold
        a                 owl:NamedIndividual , :Setup_and_Testing_of_the_Metal_Mold ;
        rdfs:comment      "Instance of an activity which is part of the creation process of ARTWORK_36."@en ;
        rdfs:label        "ARTWORK_36_Setup and Testing of the Metal Mold"@en ;
        :Followed-By      :ARTWORK_36_PreparingGlass ;
        :Follows          :ARTWORK_36_ExaminingTheQualityOfTheGlass ;
        :Has-Duration     <http://www.semanticweb.org/ontologies/Daan/2020/BarbaraNanning#2015> ;
        :Involves         :BarbaraNanning , <http://www.semanticweb.org/ontologies/Daan/2020/BarbaraNanning#JessicaHomich(USA)> , <http://www.semanticweb.org/ontologies/Daan/2020/BarbaraNanning#MarekEffmert(CZ)> , <http://www.semanticweb.org/ontologies/Daan/2020/BarbaraNanning#MarekBrathko(CZ)> , <http://www.semanticweb.org/ontologies/Daan/2020/BarbaraNanning#RobertLenner(CZ)> , :GertBullée ;
        :Located-In       :Zaandam ;
        :Part-Of          :Creation_Artwork_36 ;
        :Requires-Use-Of  :InterchangeableMetalMoldSetup .

<http://www.semanticweb.org/ontologies/Daan/2020/BarbaraNanning#ARTWORK_79_ExaminingQuality(Result)>
        a              owl:NamedIndividual , j.0: ;
        rdfs:comment   "Instance of an activity which is part of the creation process of ARTWORK_79."@en ;
        rdfs:label     "ARTWORK_79_Examining Quality (Result)"@en ;
        :Followed-By   :ARTWORK_79_MeasuringAndBoxesMaking ;
        :Follows       :ARTWORK_79_Polishing ;
        :Has-Duration  <http://www.semanticweb.org/ontologies/Daan/2020/BarbaraNanning#2018> ;
        :Involves      :BarbaraNanning , :AlešZvěřina ;
        :Located-In    :CzechRepublic ;
        :Part-Of       :Creation_Artwork_79 .

:JaroslavKubásek  a   owl:NamedIndividual , :Fourth_Glass_Blower ;
        rdfs:comment  "Jaroslav Kubásek is a Fourth Glass Blower."@en ;
        rdfs:label    "Jaroslav Kubásek"@en ;
        :Involved-In  :ARTWORK_46_Glassblowing , :ARTWORK_36_ApplyingMassivePieceOfClearGlass , :ARTWORK_36_Modeling_2 , :ARTWORK_46_Modeling , :ARTWORK_36_Cooling_2 , :ARTWORK_46_PickingUpColouredCanesPattern , :ARTWORK_46_ApplyingClearOverlay , :ARTWORK_46_SetupAndTestingOfTheMetalMold ;
        :Works-For    <http://www.semanticweb.org/ontologies/Daan/2020/BarbaraNanning#Ji%C5%99%C3%ADPa%C4%8DinekLindava(CZ)> .

:Transparency  a      owl:DatatypeProperty ;
        rdfs:comment  "Tranparency is a property of glass materials which indicates the degree the glass lets light through. This is either Opaque or Transparent."@en ;
        rdfs:domain   :Glass ;
        rdfs:label    "Transparency"@en ;
        rdfs:range    xsd:string .

:ARTWORK_78_ApplyingClearGlassBell
        a                 owl:NamedIndividual , :Applying_Clear_Glass_Bell ;
        rdfs:comment      "Instance of an activity which is part of the creation process of ARTWORK_78."@en ;
        rdfs:label        "ARTWORK_78_Applying Clear Glass Bell"@en ;
        :Followed-By      :ARTWORK_78_ApplyingExtraColour ;
        :Follows          :ARTWORK_78_SetupAndTestingOfTheMetalMold_2 ;
        :Has-Duration     <http://www.semanticweb.org/ontologies/Daan/2020/BarbaraNanning#2016> ;
        :Involves         <http://www.semanticweb.org/ontologies/Daan/2020/BarbaraNanning#RostislavMaterka(CZ)> , <http://www.semanticweb.org/ontologies/Daan/2020/BarbaraNanning#AlesVacek(CZ)> , :BarbaraNanning ;
        :Located-In       :CzechRepublic ;
        :Part-Of          :Creation_Artwork_78 ;
        :Processes        :AJETOClearGlass ;
        :Requires-Use-Of  :CeramicPotFilledWithGlass , :Blocks , :IcePick , :Hook , :Jacks , :Pincet , :DiamondShears , :StraightShears , :Water , :YokeOfSupport , :Furnace , :Marver , :Paper , :AirCompressor , :BlowingPipe , :Beeswax .

:ARTWORK_73_Sandblasting
        a                 :Sandblasting , owl:NamedIndividual ;
        rdfs:comment      "Instance of an activity which is part of the creation process of ARTWORK_73."@en ;
        rdfs:label        "ARTWORK_73_Sandblasting"@en ;
        :Followed-By      :ARTWORK_73_Signing ;
        :Follows          :ARTWORK_73_Transporting_2 ;
        :Has-Duration     <http://www.semanticweb.org/ontologies/Daan/2020/BarbaraNanning#2018> ;
        :Involves         :AlešZvěřina , :BarbaraNanning ;
        :Located-In       :CzechRepublic ;
        :Part-Of          :Creation_Artwork_73 ;
        :Requires-Use-Of  :AirCompressor .

<http://www.semanticweb.org/ontologies/Daan/2020/BarbaraNanning#JiriMoravec(CZ)>
        a             :Second_Glass_Blower , owl:NamedIndividual ;
        rdfs:comment  "Jiri Moravec (CZ) is a Second Glass Blower."@en ;
        rdfs:label    "Jiri Moravec (CZ)"@en ;
        :Involved-In  :ARTWORK_44_SetupAndTestingOfTheMetalMold , :ARTWORK_79_SetupAndTestingOfTheMetalMold , :ARTWORK_77_SetupAndTestingOfTheMetalMold_2 , :ARTWORK_73_Modeling , :ARTWORK_76_Glassblowing , :ARTWORK_77_SetupAndTestingOfTheMetalMold , :ARTWORK_80_Glassblowing , :ARTWORK_75_Modeling , :ARTWORK_75_Glassblowing , :ARTWORK_76_SetupAndTestingOfTheMetalMold_2 , :ARTWORK_80_Modeling , :ARTWORK_44_Glassblowing , :ARTWORK_80_SetupAndTestingOfTheMetalMold_2 , :ARTWORK_80_SetupAndTestingOfTheMetalMold , :ARTWORK_76_Modeling , :ARTWORK_79_Modeling , :ARTWORK_44_SetupAndTestingOfTheMetalMold_2 , :ARTWORK_76_SetupAndTestingOfTheMetalMold , :ARTWORK_79_SetupAndTestingOfTheMetalMold_2 , :ARTWORK_73_SetupAndTestingOfTheMetalMold , :ARTWORK_75_SetupAndTestingOfTheMetalMold_2 , :ARTWORK_79_Glassblowing , :ARTWORK_73_SetupAndTestingOfTheMetalMold_2 , :ARTWORK_77_Glassblowing , :ARTWORK_44_Modeling , :ARTWORK_75_SetupAndTestingOfTheMetalMold , :ARTWORK_73_Glassblowing , :ARTWORK_77_Modeling ;
        :Works-For    :LASVITAJETO .

:Germany  a           :Country , owl:NamedIndividual ;
        rdfs:comment  "Germany is a country in central Europe."@en ;
        rdfs:label    "Germany"@en ;
        owl:sameAs    <http://www.wikidata.org/entity/Q183> ;
        :Location-Of  :Coesfeld .

:ARTWORK_76_Packing_2
        a              owl:NamedIndividual , :Packing ;
        rdfs:comment   "Instance of an activity which is part of the creation process of ARTWORK_76."@en ;
        rdfs:label     "ARTWORK_76_Packing_2"@en ;
        :Followed-By   :ARTWORK_76_Transporting_2 ;
        :Follows       :ARTWORK_76_MeasuringAndBoxesMaking ;
        :Has-Duration  <http://www.semanticweb.org/ontologies/Daan/2020/BarbaraNanning#2018> ;
        :Involves      :AlešZvěřina , :BarbaraNanning ;
        :Located-In    :CzechRepublic ;
        :Part-Of       :Creation_Artwork_76 .

:ARTWORK_36_Packing_3
        a              owl:NamedIndividual , :Packing ;
        rdfs:comment   "Instance of an activity which is part of the creation process of ARTWORK_36."@en ;
        rdfs:label     "ARTWORK_36_Packing_3"@en ;
        :Followed-By   :ARTWORK_36_Transporting_3 ;
        :Follows       <http://www.semanticweb.org/ontologies/Daan/2020/BarbaraNanning#ARTWORK_36_ExaminingQuality(FinalResult)> ;
        :Has-Duration  <http://www.semanticweb.org/ontologies/Daan/2020/BarbaraNanning#2019> ;
        :Involves      :BarbaraNanning ;
        :Located-In    :Amsterdam ;
        :Part-Of       :Creation_Artwork_36 .

:ARTWORK_75_Packing_5
        a              owl:NamedIndividual , :Packing ;
        rdfs:comment   "Instance of an activity which is part of the creation process of ARTWORK_75."@en ;
        rdfs:label     "ARTWORK_75_Packing_5"@en ;
        :Finishes      :Creation_Artwork_75 ;
        :Follows       :ARTWORK_75_Documenting ;
        :Has-Duration  <http://www.semanticweb.org/ontologies/Daan/2020/BarbaraNanning#2018> ;
        :Involves      :BarbaraNanning ;
        :Located-In    :CzechRepublic ;
        :Part-Of       :Creation_Artwork_75 .

:ARTWORK_46_Packing_3
        a              owl:NamedIndividual , :Packing ;
        rdfs:comment   "Instance of an activity which is part of the creation process of ARTWORK_46."@en ;
        rdfs:label     "ARTWORK_46_Packing_3"@en ;
        :Followed-By   :ARTWORK_46_Documenting ;
        :Follows       :ARTWORK_46_Photographing ;
        :Has-Duration  <http://www.semanticweb.org/ontologies/Daan/2020/BarbaraNanning#2018> ;
        :Involves      :BarbaraNanning ;
        :Located-In    :Amsterdam ;
        :Part-Of       :Creation_Artwork_46 .

:ARTWORK_73_Modeling  a   :Modeling , owl:NamedIndividual ;
        rdfs:comment      "Instance of an activity which is part of the creation process of ARTWORK_73."@en ;
        rdfs:label        "ARTWORK_73_Modeling"@en ;
        :Followed-By      <http://www.semanticweb.org/ontologies/Daan/2020/BarbaraNanning#ARTWORK_73_ExaminingQuality(Shape/Form)> ;
        :Follows          :ARTWORK_73_Sensing ;
        :Has-Duration     <http://www.semanticweb.org/ontologies/Daan/2020/BarbaraNanning#2018> ;
        :Involves         <http://www.semanticweb.org/ontologies/Daan/2020/BarbaraNanning#JiriMoravec(CZ)> , <http://www.semanticweb.org/ontologies/Daan/2020/BarbaraNanning#LukasHavlas(CZ)> , <http://www.semanticweb.org/ontologies/Daan/2020/BarbaraNanning#Tom%C3%A1%C5%A1Moravec(CZ)> , <http://www.semanticweb.org/ontologies/Daan/2020/BarbaraNanning#RadekKoten(CZ)> , :AssistantOfBarbara , :BarbaraNanning ;
        :Located-In       :CzechRepublic ;
        :Part-Of          :Creation_Artwork_73 ;
        :Requires-Use-Of  :PropaneTorch , :Gloves , :BlowingPipe , :InterchangeableMetalMoldSetup , :AirCompressor .

:ARTWORK_18_64_ProducingColouredCanes
        a                 owl:NamedIndividual , :Producing_Coloured_Canes ;
        rdfs:comment      "Instance of an activity which is part of the creation process of ARTWORK_18_64."@en ;
        rdfs:label        "ARTWORK_18_64_Producing Coloured Canes"@en ;
        :Followed-By      :ARTWORK_18_64_TransportingColouredCanes ;
        :Follows          :ARTWORK_18_64_TransportingMonochromeRods ;
        :Has-Duration     <http://www.semanticweb.org/ontologies/Daan/2020/BarbaraNanning#2015> ;
        :Involves         :BarbaraNanning , :GertBullée , <http://www.semanticweb.org/ontologies/Daan/2020/BarbaraNanning#JessicaHomich(USA)> , <http://www.semanticweb.org/ontologies/Daan/2020/BarbaraNanning#RobertLenner(CZ)> , <http://www.semanticweb.org/ontologies/Daan/2020/BarbaraNanning#MiaLerssi(DN)> , :DurkValkema , <http://www.semanticweb.org/ontologies/Daan/2020/BarbaraNanning#MarekBrathko(CZ)> , <http://www.semanticweb.org/ontologies/Daan/2020/BarbaraNanning#MarekEffmert(CZ)> ;
        :Located-In       :Zaandam ;
        :Part-Of          :Creation_Artwork_18_64 ;
        :Requires-Use-Of  :Gloves , :GloryHole , :Beeswax , :AirCompressor , :PropaneTorch , :Tagliol , :StraightShears , :Water , :GrindingWheel , :DiamondShears , :SharpeningStone , :AnnealingKiln , :Blocks , :Garage , :Furnace , :Hook , :Computer , :Jacks , :BitIrons , :FusingKiln , :Paper , :Marver , :YokeOfSupport , :Pontis .

:ARTWORK_77_Transporting
        a              owl:NamedIndividual , :Transporting ;
        rdfs:comment   "Instance of an activity which is part of the creation process of ARTWORK_77."@en ;
        rdfs:label     "ARTWORK_77_Transporting"@en ;
        :Followed-By   :ARTWORK_77_Resting ;
        :Follows       :ARTWORK_77_Packing ;
        :Has-Duration  <http://www.semanticweb.org/ontologies/Daan/2020/BarbaraNanning#2018> ;
        :Involves      :BarbaraNanning , :AlešZvěřina ;
        :Located-In    :CzechRepublic ;
        :Part-Of       :Creation_Artwork_77 .

:ARTWORK_79_Signing  a    owl:NamedIndividual , :Signing ;
        rdfs:comment      "Instance of an activity which is part of the creation process of ARTWORK_79."@en ;
        rdfs:label        "ARTWORK_79_Signing"@en ;
        :Followed-By      :ARTWORK_79_Packing_3 ;
        :Follows          :ARTWORK_79_Transporting_2 ;
        :Has-Duration     <http://www.semanticweb.org/ontologies/Daan/2020/BarbaraNanning#2018> ;
        :Involves         :AlešZvěřina , :BarbaraNanning ;
        :Located-In       :CzechRepublic ;
        :Part-Of          :Creation_Artwork_79 ;
        :Requires-Use-Of  :AirCompressor .

:ARTWORK_79_Gilding  a    owl:NamedIndividual , :Gilding ;
        rdfs:comment      "Instance of an activity which is part of the creation process of ARTWORK_79."@en ;
        rdfs:label        "ARTWORK_79_Gilding"@en ;
        :Followed-By      <http://www.semanticweb.org/ontologies/Daan/2020/BarbaraNanning#ARTWORK_79_ExaminingQuality(FinalResult)> ;
        :Follows          :ARTWORK_79_Transporting_3 ;
        :Has-Duration     <http://www.semanticweb.org/ontologies/Daan/2020/BarbaraNanning#2018> ;
        :Involves         :VáçlavNovák_Doksy_CzechRepublic , :BarbaraNanning ;
        :Located-In       :CzechRepublic ;
        :Part-Of          :Creation_Artwork_79 ;
        :Requires-Use-Of  :GildersTip , :INSTACOLLTool , :GildingCushion , :GildersKnife .

<http://www.semanticweb.org/ontologies/Daan/2020/BarbaraNanning#JiriPacinek(CZ)>
        a             owl:NamedIndividual , :Master_Glass_Blower ;
        rdfs:comment  "Jiri Pacinek (CZ) is a Master Glass Blower who also supervises the works."@en ;
        rdfs:label    "Jiri Pacinek (CZ)"@en ;
        owl:sameAs    <http://www.wikidata.org/entity/Q28789947> ;
        :Involved-In  :ARTWORK_46_Sensing , :ARTWORK_36_ApplyingMassivePieceOfClearGlass , :ARTWORK_46_Cooling , :ARTWORK_46_ApplyingClearGlassBell , :ARTWORK_46_PreparingForBlowing , <http://www.semanticweb.org/ontologies/Daan/2020/BarbaraNanning#ARTWORK_36_ExaminingQuality(Shape/Form)_2> , :ARTWORK_46_ApplyingClearOverlay , :ARTWORK_18_64_FillingKilnsWithMetalBowl , <http://www.semanticweb.org/ontologies/Daan/2020/BarbaraNanning#ARTWORK_46_ExaminingQuality(Shape/Form)> , :ARTWORK_46_ExaminingTheQualityOfTheGlass , :ARTWORK_36_Cooling_2 , :ARTWORK_46_FillingKilnsWithMetalBowl , :ARTWORK_46_Glassblowing , :ARTWORK_46_SetupAndTestingOfTheMetalMold , :ARTWORK_18_64_ExaminingTheQualityOfTheGlass , :ARTWORK_36_ExaminingTheQualityOfTheGlass_2 , :ARTWORK_18_64_PreparingForBlowing , :ARTWORK_46_Modeling , :ARTWORK_46_PreparingGlass , :ARTWORK_36_FillingKilnsWithMetalBowl_2 , :ARTWORK_18_64_PreparingForBlowing_2 , :ARTWORK_46_PickingUpColouredCanesPattern , :ARTWORK_36_Modeling_2 ;
        :Works-For    <http://www.semanticweb.org/ontologies/Daan/2020/BarbaraNanning#Ji%C5%99%C3%ADPa%C4%8DinekLindava(CZ)> .

:Equipment  a                owl:Class ;
        rdfs:comment         "A device with a specific function."@en ;
        rdfs:label           "Equipment"@en ;
        rdfs:subClassOf      :Thing ;
        owl:equivalentClass  <http://www.wikidata.org/entity/Q16798631> .

:Follows  a           owl:ObjectProperty ;
        rdfs:comment  "Follows is a property which connects an event to the event which occurs next."@en ;
        rdfs:domain   :Event ;
        rdfs:label    "Follows"@en ;
        rdfs:range    :Event .

:Artwork_73  a        owl:NamedIndividual , :Glass_Artwork ;
        rdfs:comment  "Artwork by Barbara Nanning displayed in \"Barbara Nanning Eeuwige Beweging\" by Eliens (2019)."@en ;
        rdfs:label    "Verre églomisé"@en ;
        :Created-By   :Creation_Artwork_73 ;
        :Has-Depth    "28"^^xsd:decimal ;
        :Has-Height   "19"^^xsd:decimal ;
        :Has-Width    "30"^^xsd:decimal ;
        :Is-Unica     "Yes"@en ;
        :Made-By      <http://www.semanticweb.org/ontologies/Daan/2020/BarbaraNanning#Ale%C5%A1Zv%C4%9B%C5%99ina&AZ-Design> , :LASVITAJETO , :BarbaraNanning , :VáçlavNovák_Doksy_CzechRepublic ;
        :Made-Out-Of  :PureDucat , :AJETOClearGlass ;
        :Part-Of      :CollectionWithUnknownOwner ;
        :Shown-By     :Image_Artwork_73 .

:ARTWORK_46_DecidingColourPaletteAndPatterns_2
        a              owl:NamedIndividual , :Deciding_Colour_Palette_and_Patterns ;
        rdfs:comment   "Instance of an activity which is part of the creation process of ARTWORK_46."@en ;
        rdfs:label     "ARTWORK_46_Deciding Colour Palette and Patterns_2"@en ;
        :Followed-By   :ARTWORK_46_TransportingMonochromeRods ;
        :Follows       :ARTWORK_46_CuttingAndPolishingCastedMonochromeSheetsToSmallRods ;
        :Has-Duration  <http://www.semanticweb.org/ontologies/Daan/2020/BarbaraNanning#2015> ;
        :Involves      :BarbaraNanning ;
        :Located-In    :Amsterdam ;
        :Part-Of       :Creation_Artwork_46 .

:Casting  a              owl:Class ;
        rdfs:comment     "Using sand or other materials to create a mold, hot glass is poured in to create the final form."@en ;
        rdfs:label       "Casting"@en ;
        rdfs:subClassOf  :Activity .

<http://www.semanticweb.org/ontologies/Daan/2020/BarbaraNanning#ARTWORK_80_ExaminingQuality(FinalResult)>
        a              owl:NamedIndividual , j.1: ;
        rdfs:comment   "Instance of an activity which is part of the creation process of ARTWORK_80."@en ;
        rdfs:label     "ARTWORK_80_Examining Quality (Final Result)"@en ;
        :Followed-By   :ARTWORK_80_Photographing ;
        :Follows       :ARTWORK_80_Gilding ;
        :Has-Duration  <http://www.semanticweb.org/ontologies/Daan/2020/BarbaraNanning#2018> ;
        :Involves      :AlešZvěřina , :BarbaraNanning ;
        :Located-In    :CzechRepublic ;
        :Part-Of       :Creation_Artwork_80 .

:Cutting_and_Polishing_Coloured_Canes
        a                owl:Class ;
        rdfs:comment     "A glassblower creates the coloured canes which can then be cut to different lengths and polished by a cutter."@en ;
        rdfs:label       "Cutting and Polishing Coloured Canes"@en ;
        rdfs:subClassOf  :Activity .

<http://www.wikidata.org/entity/Q213>
        a       owl:NamedIndividual .

:ARTWORK_74_SetupAndTestingOfTheMetalMold_2
        a                 owl:NamedIndividual , :Setup_and_Testing_of_the_Metal_Mold ;
        rdfs:comment      "Instance of an activity which is part of the creation process of ARTWORK_74."@en ;
        rdfs:label        "ARTWORK_74_Setup and Testing of the Metal Mold_2"@en ;
        :Followed-By      :ARTWORK_74_ApplyingClearGlassBell ;
        :Follows          :ARTWORK_74_ExaminingTheQualityOfTheGlass ;
        :Has-Duration     <http://www.semanticweb.org/ontologies/Daan/2020/BarbaraNanning#2008> ;
        :Involves         :AssistantOfBarbara , <http://www.semanticweb.org/ontologies/Daan/2020/BarbaraNanning#RomanTomis(CZ)> , <http://www.semanticweb.org/ontologies/Daan/2020/BarbaraNanning#RostislavMaterka(CZ)> , :BarbaraNanning , <http://www.semanticweb.org/ontologies/Daan/2020/BarbaraNanning#AlesVacek(CZ)> , <http://www.semanticweb.org/ontologies/Daan/2020/BarbaraNanning#RobertHlavacek(CZ)> ;
        :Located-In       :CzechRepublic ;
        :Part-Of          :Creation_Artwork_74 ;
        :Requires-Use-Of  :InterchangeableMetalMoldSetup .

:Translocating  a        owl:Class ;
        rdfs:comment     "Translocating is an activity in which an artwork is put in the kiln."@en ;
        rdfs:label       "Translocating"@en ;
        rdfs:subClassOf  :Transporting .

:Calcium  a               :Natural_Material , owl:NamedIndividual ;
        rdfs:comment      "Calcium is a soft grey metal material with the chemical element of atomic number 20."@en ;
        rdfs:label        "Calcium"@en ;
        owl:sameAs        <http://www.wikidata.org/entity/Q706> ;
        :Is-Processed-In  :AJETOWhiteGlass , :AJETOBlueGlass , :AJETOGreenGlass , :AJETOSmokeGlass , :AJETOAmberGlass , :AJETOBlackGlass , :AJETOClearGlass , :AJETORedGlass .

:Entity  a            owl:Class ;
        rdfs:comment  "An entity is something that exists distinctly."@en ;
        rdfs:label    "Entity"@en .

:ARTWORK_73_Sensing  a  owl:NamedIndividual , :Sensing ;
        rdfs:comment   "Instance of an activity which is part of the creation process of ARTWORK_73."@en ;
        rdfs:label     "ARTWORK_73_Sensing"@en ;
        :Followed-By   :ARTWORK_73_Modeling ;
        :Follows       :ARTWORK_73_Glassblowing ;
        :Has-Duration  <http://www.semanticweb.org/ontologies/Daan/2020/BarbaraNanning#2018> ;
        :Involves      :LukášSvoboda , :AlešZvěřina , :BarbaraNanning ;
        :Located-In    :CzechRepublic ;
        :Part-Of       :Creation_Artwork_73 .

:ARTWORK_80_Sensing  a  owl:NamedIndividual , :Sensing ;
        rdfs:comment   "Instance of an activity which is part of the creation process of ARTWORK_80."@en ;
        rdfs:label     "ARTWORK_80_Sensing"@en ;
        :Followed-By   :ARTWORK_80_Modeling ;
        :Follows       :ARTWORK_80_Glassblowing ;
        :Has-Duration  <http://www.semanticweb.org/ontologies/Daan/2020/BarbaraNanning#2018> ;
        :Involves      :AlešZvěřina , :LukášSvoboda , :BarbaraNanning ;
        :Located-In    :CzechRepublic ;
        :Part-Of       :Creation_Artwork_80 .

[ a            owl:AllDisjointClasses ;
  owl:members  ( :Actor :Period :Place :Representation :Thing :Timespan )
] .

<http://www.cidoc-crm.org/cidoc-crm/E4_Period>
        a                    owl:Class ;
        owl:equivalentClass  :Period .

:ARTWORK_18_64_CuttingStrings
        a                 owl:NamedIndividual , :Cutting_Strings ;
        rdfs:comment      "Instance of an activity which is part of the creation process of ARTWORK_18_64."@en ;
        rdfs:label        "ARTWORK_18_64_Cutting Strings"@en ;
        :Followed-By      :ARTWORK_18_64_DecoratingTheSheetWithColouredCanes ;
        :Follows          :ARTWORK_18_64_FusingSheets ;
        :Has-Duration     <http://www.semanticweb.org/ontologies/Daan/2020/BarbaraNanning#2015> ;
        :Involves         :BarbaraNanning ;
        :Located-In       :Amsterdam ;
        :Part-Of          :Creation_Artwork_18_64 ;
        :Requires-Use-Of  :Glassscissors .

:ARTWORK_44_Translocating
        a                 owl:NamedIndividual , :Translocating ;
        rdfs:comment      "Instance of an activity which is part of the creation process of ARTWORK_44."@en ;
        rdfs:label        "ARTWORK_44_Translocating"@en ;
        :Followed-By      :ARTWORK_44_Cooling ;
        :Follows          <http://www.semanticweb.org/ontologies/Daan/2020/BarbaraNanning#ARTWORK_44_ExaminingQuality(Shape/Form)> ;
        :Has-Duration     <http://www.semanticweb.org/ontologies/Daan/2020/BarbaraNanning#2018> ;
        :Involves         :BarbaraNanning ;
        :Located-In       :CzechRepublic ;
        :Part-Of          :Creation_Artwork_44 ;
        :Requires-Use-Of  :Fork .

:ARTWORK_77_Grinding  a   :Grinding , owl:NamedIndividual ;
        rdfs:comment      "Instance of an activity which is part of the creation process of ARTWORK_77."@en ;
        rdfs:label        "ARTWORK_77_Grinding"@en ;
        :Followed-By      :ARTWORK_77_Polishing ;
        :Follows          :ARTWORK_77_Sawing ;
        :Has-Duration     <http://www.semanticweb.org/ontologies/Daan/2020/BarbaraNanning#2018> ;
        :Involves         :BarbaraNanning , :AlešZvěřina , :RobertFlorian ;
        :Located-In       :CzechRepublic ;
        :Part-Of          :Creation_Artwork_77 ;
        :Requires-Use-Of  :GrindingWheel , :SharpeningStone .

<http://www.semanticweb.org/ontologies/Daan/2020/BarbaraNanning#ARTWORK_39_ExaminingQuality(CheckForIrregularitiesInTheGlass)>
        a              j.3: , owl:NamedIndividual ;
        rdfs:comment   "Instance of an activity which is part of the creation process of ARTWORK_39."@en ;
        rdfs:label     "ARTWORK_39_Examining Quality (Check for Irregularities in the Glass)"@en ;
        :Followed-By   :ARTWORK_39_Sawing ;
        :Follows       :ARTWORK_39_Resting ;
        :Has-Duration  <http://www.semanticweb.org/ontologies/Daan/2020/BarbaraNanning#2015> ;
        :Involves      :AlešZvěřina , :BarbaraNanning ;
        :Located-In    :NovyBor ;
        :Part-Of       :Creation_Artwork_39 .

:ARTWORK_18_64_SlumpingSheetsAndStrings
        a                 owl:NamedIndividual , :Slumping_Sheets_and_Strings ;
        rdfs:comment      "Instance of an activity which is part of the creation process of ARTWORK_36."@en ;
        rdfs:label        "ARTWORK_36_Grinding"@en ;
        :Followed-By      :ARTWORK_36_Polishing ;
        :Follows          :ARTWORK_36_Sensing_2 ;
        :Has-Duration     <http://www.semanticweb.org/ontologies/Daan/2020/BarbaraNanning#2015> ;
        :Involves         :AlešZvěřina , :BarbaraNanning , :RobertFlorian ;
        :Located-In       :NovyBor ;
        :Part-Of          :Creation_Artwork_36 ;
        :Requires-Use-Of  :SharpeningStone , :GrindingWheel .

:ARTWORK_36_ProducingColouredCanes
        a                 :Producing_Coloured_Canes , owl:NamedIndividual ;
        rdfs:comment      "Instance of an activity which is part of the creation process of ARTWORK_36."@en ;
        rdfs:label        "ARTWORK_36_Producing Coloured Canes"@en ;
        :Followed-By      :ARTWORK_36_TransportingColouredCanes ;
        :Follows          :ARTWORK_36_TransportingMonochromeRods ;
        :Has-Duration     <http://www.semanticweb.org/ontologies/Daan/2020/BarbaraNanning#2015> ;
        :Involves         <http://www.semanticweb.org/ontologies/Daan/2020/BarbaraNanning#RobertLenner(CZ)> , :BarbaraNanning , :GertBullée , :DurkValkema , <http://www.semanticweb.org/ontologies/Daan/2020/BarbaraNanning#MarekBrathko(CZ)> , <http://www.semanticweb.org/ontologies/Daan/2020/BarbaraNanning#MiaLerssi(DN)> , <http://www.semanticweb.org/ontologies/Daan/2020/BarbaraNanning#MarekEffmert(CZ)> , <http://www.semanticweb.org/ontologies/Daan/2020/BarbaraNanning#JessicaHomich(USA)> ;
        :Located-In       :Zaandam ;
        :Part-Of          :Creation_Artwork_36 ;
        :Requires-Use-Of  :Furnace , :Water , :StraightShears , :YokeOfSupport , :Pontis , :Beeswax , :FusingKiln , :Marver , :Garage , :Blocks , :DiamondShears , :Tagliol , :GloryHole , :SharpeningStone , :Hook , :Gloves , :BitIrons , :PropaneTorch , :Computer , :Paper , :GrindingWheel , :AirCompressor , :Jacks , :AnnealingKiln .

:Belgium  a           :Country , owl:NamedIndividual ;
        rdfs:comment  "Belgium is a country in western Europe."@en ;
        rdfs:label    "Belgium"@en ;
        owl:sameAs    <https://erfgeo.nl/thesaurus/pit/?id=malc/176> ;
        :Location-Of  :Brussels .

:ARTWORK_74_Glassblowing
        a                 :Glassblowing , owl:NamedIndividual ;
        rdfs:comment      "Instance of an activity which is part of the creation process of ARTWORK_74."@en ;
        rdfs:label        "ARTWORK_74_Glassblowing"@en ;
        :Followed-By      :ARTWORK_74_Sensing ;
        :Follows          :ARTWORK_74_HeatingMetalMold ;
        :Has-Duration     <http://www.semanticweb.org/ontologies/Daan/2020/BarbaraNanning#2008> ;
        :Involves         <http://www.semanticweb.org/ontologies/Daan/2020/BarbaraNanning#RostislavMaterka(CZ)> , :BarbaraNanning , <http://www.semanticweb.org/ontologies/Daan/2020/BarbaraNanning#RomanTomis(CZ)> , :AssistantOfBarbara , <http://www.semanticweb.org/ontologies/Daan/2020/BarbaraNanning#AlesVacek(CZ)> , <http://www.semanticweb.org/ontologies/Daan/2020/BarbaraNanning#RobertHlavacek(CZ)> ;
        :Located-In       :CzechRepublic ;
        :Part-Of          :Creation_Artwork_74 ;
        :Requires-Use-Of  :BlowingPipe , :Fork , :StraightShears , :Blocks , :AnnealingKiln , :Hook , :IcePick , :BitIron , :PropaneTorch , :Marver , :YokeOfSupport , :InterchangeableMetalMoldSetup , :Paper , :AirCompressor , :CeramicPotFilledWithGlass , :Tagliol , :Water , :Furnace , :Beeswax , :GloryHole , :Gloves , :Jacks , :DiamondShears , :Pincet , :Pontis .

:ARTWORK_76_Transporting_4
        a              :Transporting , owl:NamedIndividual ;
        rdfs:comment   "Instance of an activity which is part of the creation process of ARTWORK_76."@en ;
        rdfs:label     "ARTWORK_76_Transporting_4"@en ;
        :Followed-By   :ARTWORK_76_Photographing ;
        :Follows       :ARTWORK_76_Packing_4 ;
        :Has-Duration  <http://www.semanticweb.org/ontologies/Daan/2020/BarbaraNanning#2018> ;
        :Involves      :AlešZvěřina , :BarbaraNanning ;
        :Located-In    :CzechRepublic ;
        :Part-Of       :Creation_Artwork_76 .

<http://vocab.getty.edu/aat/300262866>
        a           owl:NamedIndividual ;
        owl:sameAs  :GildingCushion .

:ARTWORK_78_MeasuringAndBoxesMaking
        a              :Measuring_and_Boxes_Making , owl:NamedIndividual ;
        rdfs:comment   "Instance of an activity which is part of the creation process of ARTWORK_78."@en ;
        rdfs:label     "ARTWORK_78_Measuring and Boxes Making"@en ;
        :Followed-By   :ARTWORK_78_Packing_2 ;
        :Follows       <http://www.semanticweb.org/ontologies/Daan/2020/BarbaraNanning#ARTWORK_78_ExaminingQuality(Result)> ;
        :Has-Duration  <http://www.semanticweb.org/ontologies/Daan/2020/BarbaraNanning#2008> ;
        :Involves      :AlešZvěřina , :BarbaraNanning ;
        :Located-In    :CzechRepublic ;
        :Part-Of       :Creation_Artwork_78 .

<http://www.semanticweb.org/ontologies/Daan/2020/BarbaraNanning#ARTWORK_75_ExaminingQuality(FinalResult)>
        a              j.1: , owl:NamedIndividual ;
        rdfs:comment   "Instance of an activity which is part of the creation process of ARTWORK_75."@en ;
        rdfs:label     "ARTWORK_75_Examining Quality (Final Result)"@en ;
        :Followed-By   :ARTWORK_75_Packing_5 ;
        :Follows       :ARTWORK_75_Gilding ;
        :Has-Duration  <http://www.semanticweb.org/ontologies/Daan/2020/BarbaraNanning#2017> ;
        :Involves      :BarbaraNanning , :AlešZvěřina ;
        :Located-In    :CzechRepublic ;
        :Part-Of       :Creation_Artwork_75 .

<http://vocab.getty.edu/aat/300008389>
        a                    owl:Class ;
        owl:equivalentClass  :City .

:ARTWORK_46_CuttingAndPolishingCastedMonochromeSheetsToSmallRods
        a                 :Cutting_and_Polishing_Casted_Monochrome_Sheets_to_Small_Rods , owl:NamedIndividual ;
        rdfs:comment      "Instance of an activity which is part of the creation process of ARTWORK_46."@en ;
        rdfs:label        "ARTWORK_46_Cutting and Polishing Casted Monochrome Sheets to Small Rods"@en ;
        :Followed-By      :ARTWORK_46_DecidingColourPaletteAndPatterns_2 ;
        :Follows          :ARTWORK_46_Casting ;
        :Has-Duration     <http://www.semanticweb.org/ontologies/Daan/2020/BarbaraNanning#2015> ;
        :Involves         :BarbaraNanning ;
        :Located-In       :Amsterdam ;
        :Part-Of          :Creation_Artwork_46 ;
        :Requires-Use-Of  :Water , :SharpeningStone , :DiamondSaw .

:ARTWORK_36_CuttingSheets
        a                 owl:NamedIndividual , :Cutting_Sheets ;
        rdfs:comment      "Instance of an activity which is part of the creation process of ARTWORK_36."@en ;
        rdfs:label        "ARTWORK_36_Cutting Sheets"@en ;
        :Followed-By      :ARTWORK_36_OrdeningFlatSheets ;
        :Follows          :ARTWORK_36_DecidingColourPalette_2 ;
        :Has-Duration     <http://www.semanticweb.org/ontologies/Daan/2020/BarbaraNanning#2019> ;
        :Involves         :BarbaraNanning ;
        :Located-In       :Zaandam ;
        :Part-Of          :Creation_Artwork_36 ;
        :Requires-Use-Of  :DiamondSaw , :Water , :SharpeningStone .

<http://www.wikidata.org/entity/Q1007870>
        a       owl:Class .

:ARTWORK_43_MeasuringAndBoxesMaking
        a              :Measuring_and_Boxes_Making , owl:NamedIndividual ;
        rdfs:comment   "Instance of an activity which is part of the creation process of ARTWORK_43."@en ;
        rdfs:label     "ARTWORK_43_Measuring and Boxes Making"@en ;
        :Followed-By   :ARTWORK_43_Packing_2 ;
        :Follows       <http://www.semanticweb.org/ontologies/Daan/2020/BarbaraNanning#ARTWORK_43_ExaminingQuality(Result)> ;
        :Has-Duration  <http://www.semanticweb.org/ontologies/Daan/2020/BarbaraNanning#2008> ;
        :Involves      :BarbaraNanning , :AlešZvěřina ;
        :Located-In    :CzechRepublic ;
        :Part-Of       :Creation_Artwork_43 .

:ARTWORK_43_SetupAndTestingOfTheMetalMold_2
        a                 owl:NamedIndividual , :Setup_and_Testing_of_the_Metal_Mold ;
        rdfs:comment      "Instance of an activity which is part of the creation process of ARTWORK_43."@en ;
        rdfs:label        "ARTWORK_43_Setup and Testing of the Metal Mold_2"@en ;
        :Followed-By      :ARTWORK_43_ExaminingTheQualityOfTheGlass ;
        :Follows          :ARTWORK_43_ApplyingClearGlassBell ;
        :Has-Duration     <http://www.semanticweb.org/ontologies/Daan/2020/BarbaraNanning#2008> ;
        :Involves         :AssistantOfBarbara , <http://www.semanticweb.org/ontologies/Daan/2020/BarbaraNanning#AlesVacek(CZ)> , <http://www.semanticweb.org/ontologies/Daan/2020/BarbaraNanning#RobertHlavacek(CZ)> , <http://www.semanticweb.org/ontologies/Daan/2020/BarbaraNanning#RostislavMaterka(CZ)> , <http://www.semanticweb.org/ontologies/Daan/2020/BarbaraNanning#RomanTomis(CZ)> , :BarbaraNanning ;
        :Located-In       :CzechRepublic ;
        :Part-Of          :Creation_Artwork_43 ;
        :Requires-Use-Of  :InterchangeableMetalMoldSetup .

:ARTWORK_78_SetupAndTestingOfTheMetalMold
        a                 :Setup_and_Testing_of_the_Metal_Mold , owl:NamedIndividual ;
        rdfs:comment      "Instance of an activity which is part of the creation process of ARTWORK_78."@en ;
        rdfs:label        "ARTWORK_78_Setup and Testing of the Metal Mold"@en ;
        :Followed-By      :ARTWORK_78_ExaminingTheQualityOfTheGlass ;
        :Follows          :ARTWORK_78_PreparingGlass ;
        :Has-Duration     <http://www.semanticweb.org/ontologies/Daan/2020/BarbaraNanning#2008> ;
        :Involves         <http://www.semanticweb.org/ontologies/Daan/2020/BarbaraNanning#AlesVacek(CZ)> , :AssistantOfBarbara , <http://www.semanticweb.org/ontologies/Daan/2020/BarbaraNanning#RomanTomis(CZ)> , <http://www.semanticweb.org/ontologies/Daan/2020/BarbaraNanning#RostislavMaterka(CZ)> , :BarbaraNanning , <http://www.semanticweb.org/ontologies/Daan/2020/BarbaraNanning#RobertHlavacek(CZ)> ;
        :Located-In       :CzechRepublic ;
        :Part-Of          :Creation_Artwork_78 ;
        :Requires-Use-Of  :InterchangeableMetalMoldSetup .

:ARTWORK_17_33_DecidingColourPalette
        a                 owl:NamedIndividual , :Deciding_Colour_Palette ;
        rdfs:comment      "Instance of an activity which is part of the creation process of ARTWORK_17_33."@en ;
        rdfs:label        "ARTWORK_17_33_Deciding Colour Palette"@en ;
        :Followed-By      :ARTWORK_17_33_MakingPatternsWithColouredCanesInTheMetalBowl ;
        :Follows          :ARTWORK_17_33_TransportingColouredCanes_2 ;
        :Has-Duration     <http://www.semanticweb.org/ontologies/Daan/2020/BarbaraNanning#2017> ;
        :Involves         :BarbaraNanning ;
        :Located-In       :Amsterdam ;
        :Part-Of          :Creation_Artwork_17_33 ;
        :Requires-Use-Of  :Computer .

<http://vocab.getty.edu/aat/300024718>
        a           owl:NamedIndividual ;
        owl:sameAs  :GrindingWheel .

:FusingKiln  a        :Equipment , owl:NamedIndividual ;
        rdfs:comment  "A Fusing Kiln is a thermally insulated chamber used for fusing."@en ;
        rdfs:label    "Fusing Kiln"@en .

:Decorating_the_Sheet_with_Coloured_Canes
        a                owl:Class ;
        rdfs:comment     "Merging strips of colored flat glass plates on a stack of multiple colored bottom plates with a top layer of canes."@en ;
        rdfs:label       "Decorating the Sheet with Coloured Canes"@en ;
        rdfs:subClassOf  :Activity .

:Image_Artwork_18_64  a         :Digital_Image , owl:NamedIndividual ;
        rdfs:comment            "Image of Artwork_18_64 by Barbara Nanning."@en ;
        rdfs:label              "Image_Artwork_18_64"@en ;
        :Representation-Source  "Tom Haartsen_Ouderkerk A/d Amstel (NL)"@en ;
        :Shows                  :Artwork_18_64 .

<http://www.semanticweb.org/ontologies/Daan/2020/BarbaraNanning#MiaLerssi(DN)>
        a             owl:NamedIndividual , :Assisting_Team_Member ;
        rdfs:comment  "Mia Lerssi (DN) is an Assisting Team Member."@en ;
        rdfs:label    "Mia Lerssi (DN)"@en ;
        :Involved-In  :ARTWORK_36_PreparingGlass , :ARTWORK_39_PreparingGlass , :ARTWORK_39_Glassblowing , :ARTWORK_36_PickingUpColouredPanel , :ARTWORK_39_PickingUpColouredPanel , :ARTWORK_46_ProducingColouredCanes , :ARTWORK_36_Cooling , :ARTWORK_36_PickingUpColouredCanesPattern , :ARTWORK_18_64_Glassblowing , :ARTWORK_18_64_PreparingGlass , :ARTWORK_36_PreparingForBlowing , :ARTWORK_18_64_ProducingColouredCanes , :ARTWORK_17_33_ProducingColouredCanes , :ARTWORK_18_64_PickingUpColouredCanesPattern , :ARTWORK_36_Glassblowing , :ARTWORK_18_64_Cooling , <http://www.semanticweb.org/ontologies/Daan/2020/BarbaraNanning#ARTWORK_36_ExaminingQuality(Shape/Form)> , <http://www.semanticweb.org/ontologies/Daan/2020/BarbaraNanning#ARTWORK_18_64_ExaminingQuality(Shape/Form)> , :ARTWORK_36_ProducingColouredCanes , :ARTWORK_39_Cooling , <http://www.semanticweb.org/ontologies/Daan/2020/BarbaraNanning#ARTWORK_39_ExaminingQuality(Shape/Form)> , :ARTWORK_39_PreparingForBlowing .

:ARTWORK_79_Packing_4
        a              owl:NamedIndividual , :Packing ;
        rdfs:comment   "Instance of an activity which is part of the creation process of ARTWORK_79."@en ;
        rdfs:label     "ARTWORK_79_Packing_4"@en ;
        :Followed-By   :ARTWORK_79_Transporting_4 ;
        :Follows       <http://www.semanticweb.org/ontologies/Daan/2020/BarbaraNanning#ARTWORK_79_ExaminingQuality(FinalResult)> ;
        :Has-Duration  <http://www.semanticweb.org/ontologies/Daan/2020/BarbaraNanning#2018> ;
        :Involves      :BarbaraNanning , :VáçlavNovák_Doksy_CzechRepublic , :AlešZvěřina ;
        :Located-In    :CzechRepublic ;
        :Part-Of       :Creation_Artwork_79 .

:ARTWORK_17_33_MakingPatternsWithColouredCanesInTheMetalBowl
        a                 :Making_Patterns_with_Coloured_Canes_in_the_Metal_Bowl , owl:NamedIndividual ;
        rdfs:comment      "Instance of an activity which is part of the creation process of ARTWORK_17_33."@en ;
        rdfs:label        "ARTWORK_17_33_Making Patterns with Coloured Canes in the Metal Bowl"@en ;
        :Followed-By      :ARTWORK_17_33_TackfusingColouredCanes ;
        :Follows          :ARTWORK_17_33_DecidingColourPalette ;
        :Has-Duration     <http://www.semanticweb.org/ontologies/Daan/2020/BarbaraNanning#2017> ;
        :Involves         :BarbaraNanning ;
        :Located-In       :Amsterdam ;
        :Part-Of          :Creation_Artwork_17_33 ;
        :Requires-Use-Of  :FusingKiln , :Glassscissors , :Pincet .

:ARTWORK_80_Sandblasting
        a                 owl:NamedIndividual , :Sandblasting ;
        rdfs:comment      "Instance of an activity which is part of the creation process of ARTWORK_80."@en ;
        rdfs:label        "ARTWORK_80_Sandblasting"@en ;
        :Followed-By      :ARTWORK_80_Signing ;
        :Follows          :ARTWORK_80_Transporting_2 ;
        :Has-Duration     <http://www.semanticweb.org/ontologies/Daan/2020/BarbaraNanning#2018> ;
        :Involves         :AlešZvěřina , :BarbaraNanning ;
        :Located-In       :CzechRepublic ;
        :Part-Of          :Creation_Artwork_80 ;
        :Requires-Use-Of  :AirCompressor .

:ARTWORK_36_FlatFusingSheetsWithARTWORK36PeacockToOnePanel
        a                 :Flat_Fusing_Glass_Sheets_with_ARTWORK_36_Peacock_to_One_Glass_Panel , owl:NamedIndividual ;
        rdfs:comment      "Instance of an activity which is part of the creation process of ARTWORK_36."@en ;
        rdfs:label        "ARTWORK_36_Flat Fusing Sheets with ARTWORK 36 Peacock to One Panel"@en ;
        :Followed-By      :ARTWORK_36_SlumpingPanel ;
        :Follows          :ARTWORK_36_FusingSheets ;
        :Has-Duration     <http://www.semanticweb.org/ontologies/Daan/2020/BarbaraNanning#2019> ;
        :Involves         :BarbaraNanning ;
        :Located-In       :Amsterdam ;
        :Part-Of          :Creation_Artwork_36 ;
        :Requires-Use-Of  :FusingKiln .

<http://www.semanticweb.org/ontologies/Daan/2020/BarbaraNanning#ARTWORK_74_ExaminingQuality(FinalResult)>
        a              j.1: , owl:NamedIndividual ;
        rdfs:comment   "Instance of an activity which is part of the creation process of ARTWORK_74."@en ;
        rdfs:label     "ARTWORK_74_Examining Quality (Final Result)"@en ;
        :Followed-By   :ARTWORK_74_Packing_5 ;
        :Follows       :ARTWORK_74_Gilding ;
        :Has-Duration  <http://www.semanticweb.org/ontologies/Daan/2020/BarbaraNanning#2008> ;
        :Involves      :AlešZvěřina , :BarbaraNanning ;
        :Located-In    :CzechRepublic ;
        :Part-Of       :Creation_Artwork_74 .

<http://www.semanticweb.org/ontologies/Daan/2020/BarbaraNanning#ARTWORK_17_33_ExaminingQuality(Shape/Form)>
        a                 owl:NamedIndividual , j.2: ;
        rdfs:comment      "Instance of an activity which is part of the creation process of ARTWORK_17_33."@en ;
        rdfs:label        "ARTWORK_17_33_Examining Quality (Shape/Form)"@en ;
        :Followed-By      :ARTWORK_17_33_Cooling ;
        :Follows          :ARTWORK_17_33_Modeling ;
        :Has-Duration     <http://www.semanticweb.org/ontologies/Daan/2020/BarbaraNanning#2017> ;
        :Involves         :LuděkKout , :BarbaraNanning , <http://www.semanticweb.org/ontologies/Daan/2020/BarbaraNanning#RadekKoten(CZ)> ;
        :Located-In       :Lindava ;
        :Part-Of          :Creation_Artwork_17_33 ;
        :Requires-Use-Of  :GloryHole , :BlowingPipe , :Pontis .

<http://www.semanticweb.org/ontologies/Daan/2020/BarbaraNanning#ARTWORK_75_ExaminingQuality(Shape/Form)>
        a                 owl:NamedIndividual , j.2: ;
        rdfs:comment      "Instance of an activity which is part of the creation process of ARTWORK_75."@en ;
        rdfs:label        "ARTWORK_75_Examining Quality (Shape/Form)"@en ;
        :Followed-By      :ARTWORK_75_Translocating ;
        :Follows          :ARTWORK_75_Modeling ;
        :Has-Duration     <http://www.semanticweb.org/ontologies/Daan/2020/BarbaraNanning#2017> ;
        :Involves         <http://www.semanticweb.org/ontologies/Daan/2020/BarbaraNanning#RadekKoten(CZ)> , :BarbaraNanning , :LuděkKout ;
        :Located-In       :CzechRepublic ;
        :Part-Of          :Creation_Artwork_75 ;
        :Requires-Use-Of  :BlowingPipe , :GloryHole , :Pontis .

:ARTWORK_18_64_PreparingForBlowing_2
        a                 owl:NamedIndividual , :Preparing_for_Blowing ;
        rdfs:comment      "Instance of an activity which is part of the creation process of ARTWORK_18_64."@en ;
        rdfs:label        "ARTWORK_18_64_Preparing for Blowing_2"@en ;
        :Followed-By      :ARTWORK_18_64_ExaminingTheQualityOfTheGlass ;
        :Follows          :ARTWORK_18_64_PreparingGlass ;
        :Has-Duration     <http://www.semanticweb.org/ontologies/Daan/2020/BarbaraNanning#2015> ;
        :Involves         <http://www.semanticweb.org/ontologies/Daan/2020/BarbaraNanning#JiriPacinek(CZ)> , <http://www.semanticweb.org/ontologies/Daan/2020/BarbaraNanning#JessicaHomich(USA)> , :BarbaraNanning ;
        :Located-In       :Lindava ;
        :Part-Of          :Creation_Artwork_18_64 ;
        :Requires-Use-Of  :FusingKiln , :Paper , :Water , :BlowingPipe , :Furnace , :Garage , :AnnealingKiln .

:ARTWORK_36_DecidingColourPalette_2
        a                 owl:NamedIndividual , :Deciding_Colour_Palette ;
        rdfs:comment      "Instance of an activity which is part of the creation process of ARTWORK_36."@en ;
        rdfs:label        "ARTWORK_36_Deciding Colour Palette_2"@en ;
        :Followed-By      :ARTWORK_36_CuttingSheets ;
        :Follows          :ARTWORK_36_FlatFusingFinishedArtwork ;
        :Has-Duration     <http://www.semanticweb.org/ontologies/Daan/2020/BarbaraNanning#2019> ;
        :Involves         :BarbaraNanning ;
        :Located-In       :Amsterdam ;
        :Part-Of          :Creation_Artwork_36 ;
        :Requires-Use-Of  :Computer .

:ARTWORK_75_Packing  a  owl:NamedIndividual , :Packing ;
        rdfs:comment   "Instance of an activity which is part of the creation process of ARTWORK_75."@en ;
        rdfs:label     "ARTWORK_75_Packing"@en ;
        :Followed-By   :ARTWORK_75_Transporting ;
        :Follows       :ARTWORK_75_Cooling ;
        :Has-Duration  <http://www.semanticweb.org/ontologies/Daan/2020/BarbaraNanning#2018> ;
        :Involves      :AlešZvěřina , :BarbaraNanning ;
        :Located-In    :CzechRepublic ;
        :Part-Of       :Creation_Artwork_75 .

:ARTWORK_73_Glassblowing
        a                 :Glassblowing , owl:NamedIndividual ;
        rdfs:comment      "Instance of an activity which is part of the creation process of ARTWORK_73."@en ;
        rdfs:label        "ARTWORK_73_Glassblowing"@en ;
        :Followed-By      :ARTWORK_73_Sensing ;
        :Follows          :ARTWORK_73_HeatingMetalMold ;
        :Has-Duration     <http://www.semanticweb.org/ontologies/Daan/2020/BarbaraNanning#2018> ;
        :Involves         :BarbaraNanning , :AssistantOfBarbara , <http://www.semanticweb.org/ontologies/Daan/2020/BarbaraNanning#RadekKoten(CZ)> , <http://www.semanticweb.org/ontologies/Daan/2020/BarbaraNanning#Tom%C3%A1%C5%A1Moravec(CZ)> , <http://www.semanticweb.org/ontologies/Daan/2020/BarbaraNanning#LukasHavlas(CZ)> , <http://www.semanticweb.org/ontologies/Daan/2020/BarbaraNanning#JiriMoravec(CZ)> ;
        :Located-In       :CzechRepublic ;
        :Part-Of          :Creation_Artwork_73 ;
        :Requires-Use-Of  :Gloves , :CeramicPotFilledWithGlass , :PropaneTorch , :Fork , :Pontis , :IcePick , :AirCompressor , :Marver , :DiamondShears , :Water , :StraightShears , :Blocks , :Pincet , :YokeOfSupport , :Furnace , :Jacks , :GloryHole , :InterchangeableMetalMoldSetup , :BitIron , :Paper , :Beeswax , :Tagliol , :AnnealingKiln , :Hook , :BlowingPipe .

:ARTWORK_44_HeatingMetalMold
        a                 :Heating_Metal_Mold , owl:NamedIndividual ;
        rdfs:comment      "Instance of an activity which is part of the creation process of ARTWORK_44."@en ;
        rdfs:label        "ARTWORK_44_Heating Metal Mold"@en ;
        :Followed-By      :ARTWORK_44_Glassblowing ;
        :Follows          :ARTWORK_44_ApplyingExtraColour_2 ;
        :Has-Duration     <http://www.semanticweb.org/ontologies/Daan/2020/BarbaraNanning#2018> ;
        :Involves         :BarbaraNanning ;
        :Located-In       :CzechRepublic ;
        :Part-Of          :Creation_Artwork_44 ;
        :Requires-Use-Of  :PropaneTorch , :InterchangeableMetalMoldSetup , :Gloves .

:Starts-With  a       owl:ObjectProperty ;
        rdfs:comment  "Starts-With is a property which indicates the sub-event which Starts an event."@en ;
        rdfs:domain   :Event ;
        rdfs:label    "Starts-With"@en ;
        rdfs:range    :Event .

:ARTWORK_77_Sensing  a  owl:NamedIndividual , :Sensing ;
        rdfs:comment   "Instance of an activity which is part of the creation process of ARTWORK_77."@en ;
        rdfs:label     "ARTWORK_77_Sensing"@en ;
        :Followed-By   :ARTWORK_77_Modeling ;
        :Follows       :ARTWORK_77_Glassblowing ;
        :Has-Duration  <http://www.semanticweb.org/ontologies/Daan/2020/BarbaraNanning#2018> ;
        :Involves      :LukášSvoboda , :BarbaraNanning , :AlešZvěřina ;
        :Located-In    :CzechRepublic ;
        :Part-Of       :Creation_Artwork_77 .

<http://vocab.getty.edu/aat/300022796>
        a           owl:NamedIndividual ;
        owl:sameAs  :Fork .

:Grinding  a             owl:Class ;
        rdfs:comment     "Grinding is an activity in which a thing is sharpened by using friction or crushing."@en ;
        rdfs:label       "Grinding"@en ;
        rdfs:subClassOf  :Activity .

<http://www.semanticweb.org/ontologies/Daan/2020/BarbaraNanning#ARTWORK_79_ExaminingQuality(CheckForIrregularitiesInTheGlass)>
        a              j.3: , owl:NamedIndividual ;
        rdfs:comment   "Instance of an activity which is part of the creation process of ARTWORK_79."@en ;
        rdfs:label     "ARTWORK_79_Examining Quality (Check for Irregularities in the Glass)"@en ;
        :Followed-By   :ARTWORK_79_Sawing ;
        :Follows       :ARTWORK_79_Resting ;
        :Has-Duration  <http://www.semanticweb.org/ontologies/Daan/2020/BarbaraNanning#2018> ;
        :Involves      :AlešZvěřina , :BarbaraNanning ;
        :Located-In    :CzechRepublic ;
        :Part-Of       :Creation_Artwork_79 .

:AirCompressor  a     :Equipment , owl:NamedIndividual ;
        rdfs:comment  "An air compressor is a device which uses electricity to create compressed air."@en ;
        rdfs:label    "Air Compressor"@en ;
        owl:sameAs    <http://www.wikidata.org/entity/Q978234> ;
        :Used-For     :ARTWORK_75_Sandblasting , :ARTWORK_79_ApplyingExtraColour , :ARTWORK_75_Modeling , :ARTWORK_77_ApplyingExtraColour , :ARTWORK_44_ApplyingExtraColour , :ARTWORK_77_Glassblowing , :ARTWORK_77_ApplyingClearGlassBell , :ARTWORK_79_Signing , :ARTWORK_79_Glassblowing , :ARTWORK_76_Glassblowing , :ARTWORK_80_Sandblasting , :ARTWORK_44_ApplyingClearGlassBell , :ARTWORK_79_Modeling , :ARTWORK_43_Signing , :ARTWORK_44_Glassblowing , :ARTWORK_78_Modeling , :ARTWORK_78_ApplyingExtraColour , :ARTWORK_80_ApplyingExtraColour , :ARTWORK_77_Signing , :ARTWORK_76_Sandblasting , :ARTWORK_74_ApplyingClearGlassBell , :ARTWORK_73_Modeling , :ARTWORK_73_Glassblowing , :ARTWORK_80_Glassblowing , :ARTWORK_74_ApplyingExtraColour , :ARTWORK_76_Modeling , :ARTWORK_80_Modeling , :ARTWORK_76_ApplyingClearGlassBell , :ARTWORK_76_ApplyingExtraColour_2 , :ARTWORK_80_ApplyingClearGlassBell , :ARTWORK_77_Modeling , :ARTWORK_75_ApplyingClearGlassBell , :ARTWORK_80_Signing , :ARTWORK_74_ApplyingExtraColour_2 , :ARTWORK_73_Sandblasting , :ARTWORK_78_Glassblowing , :ARTWORK_73_Signing , :ARTWORK_73_ApplyingClearGlassBell , :ARTWORK_43_ApplyingClearGlassBell , :ARTWORK_79_ApplyingClearGlassBell , :ARTWORK_75_Glassblowing , :ARTWORK_74_Modeling , :ARTWORK_74_Signing , :ARTWORK_43_Modeling , :ARTWORK_78_ApplyingClearGlassBell , :ARTWORK_76_ApplyingExtraColour , :ARTWORK_44_Signing , :ARTWORK_75_ApplyingExtraColour , :ARTWORK_43_Sandblasting , :ARTWORK_43_Glassblowing , :ARTWORK_43_ApplyingExtraColour , :ARTWORK_44_ApplyingExtraColour_2 , :ARTWORK_75_Signing , :ARTWORK_75_ApplyingExtraColour_2 , :ARTWORK_76_Signing , :ARTWORK_78_Signing , :ARTWORK_44_Modeling , :ARTWORK_79_ApplyingExtraColour_2 , :ARTWORK_74_Glassblowing .

:Applying_Clear_Overlay
        a                owl:Class ;
        rdfs:comment     "Also known as Gathering Glass. While turning a pipe and inserting it into the pot of molten glass the glassblower adds a additional layer of clear glass."@en ;
        rdfs:label       "Applying Clear Overlay"@en ;
        rdfs:subClassOf  :Activity .

<http://www.semanticweb.org/ontologies/Daan/2020/BarbaraNanning#ARTWORK_43_ExaminingQuality(Result)>
        a              j.0: , owl:NamedIndividual ;
        rdfs:comment   "Instance of an activity which is part of the creation process of ARTWORK_43."@en ;
        rdfs:label     "ARTWORK_43_Examining Quality (Result)"@en ;
        :Followed-By   :ARTWORK_43_MeasuringAndBoxesMaking ;
        :Follows       :ARTWORK_43_Polishing ;
        :Has-Duration  <http://www.semanticweb.org/ontologies/Daan/2020/BarbaraNanning#2008> ;
        :Involves      :AlešZvěřina , :BarbaraNanning ;
        :Located-In    :CzechRepublic ;
        :Part-Of       :Creation_Artwork_43 .

:ARTWORK_36_CuttingMonochromeSheets
        a              :Cutting_Monochrome_Sheets , owl:NamedIndividual ;
        rdfs:comment   "Instance of an activity which is part of the creation process of ARTWORK_36."@en ;
        rdfs:label     "ARTWORK_36_Cutting Monochrome Sheets"@en ;
        :Followed-By   :ARTWORK_36_Ordening ;
        :Follows       :ARTWORK_36_DecidingColourPaletteAndPatterns ;
        :Has-Duration  <http://www.semanticweb.org/ontologies/Daan/2020/BarbaraNanning#2015> ;
        :Involves      :SteefHendriks , :BarbaraNanning ;
        :Located-In    :Langweer ;
        :Part-Of       :Creation_Artwork_36 .

:NewYork  a           :City , owl:NamedIndividual ;
        rdfs:comment  "New York is a city in the United States of America."@en ;
        rdfs:label    "New York"@en ;
        owl:sameAs    <http://www.wikidata.org/entity/Q60> ;
        :Located-In   :UnitedStatesOfAmerica ;
        :Location-Of  :J.LohmannGallery , :CollectionJ.LohmannGallery , :Artwork_44 .

:ARTWORK_17_33_DecidingColourPaletteAndPatterns
        a              :Deciding_Colour_Palette_and_Patterns , owl:NamedIndividual ;
        rdfs:comment   "Instance of an activity which is part of the creation process of ARTWORK_17_33."@en ;
        rdfs:label     "ARTWORK_17_33_Deciding Colour Palette and Patterns"@en ;
        :Followed-By   :ARTWORK_17_33_ProducingColouredCanes ;
        :Has-Duration  <http://www.semanticweb.org/ontologies/Daan/2020/BarbaraNanning#2017> ;
        :Involves      :BarbaraNanning ;
        :Located-In    :Amsterdam ;
        :Part-Of       :Creation_Artwork_17_33 ;
        :Processes     :AJETOClearGlass , :AJETORedGlass , :AJETOWhiteGlass ;
        :Starts        :Creation_Artwork_17_33 .

<http://www.semanticweb.org/ontologies/Daan/2020/BarbaraNanning#Ren%C3%A9VanDonselaar(NL)>
        a             owl:NamedIndividual , :Metal_Worker_2 ;
        rdfs:comment  "René van Donselaar (NL) is a Metal Worker 2."@en ;
        rdfs:label    "René van Donselaar (NL)"@en ;
        :Maker-Of     :InterchangeableMetalMoldSetup .

:GertBullée  a        :Master_Glass_Blower , owl:NamedIndividual ;
        rdfs:comment  "Gert Bullée (NL) is a Master Glass Blower."@en ;
        rdfs:label    "Gert Bullée"@en ;
        :Involved-In  :ARTWORK_36_ExaminingTheQualityOfTheGlass , :ARTWORK_36_PickingUpColouredPanel , :ARTWORK_36_ProducingColouredCanes , :ARTWORK_18_64_Modeling , :ARTWORK_36_Glassblowing , :ARTWORK_18_64_PickingUpColouredCanesPattern , :ARTWORK_36_PreparingGlass , :ARTWORK_46_ProducingColouredCanes , :ARTWORK_39_Glassblowing , :ARTWORK_18_64_ApplyingClearGlassBell , :ARTWORK_18_64_Glassblowing , <http://www.semanticweb.org/ontologies/Daan/2020/BarbaraNanning#ARTWORK_36_ExaminingQuality(Shape/Form)> , :ARTWORK_36_ApplyingClearGlassBell , :ARTWORK_39_ApplyingClearGlassBell , :ARTWORK_18_64_ProducingColouredCanes , :ARTWORK_39_ExaminingTheQualityOfTheGlass , :ARTWORK_36_PickingUpColouredCanesPattern , :ARTWORK_18_64_PreparingGlass , :ARTWORK_36_Modeling , <http://www.semanticweb.org/ontologies/Daan/2020/BarbaraNanning#ARTWORK_18_64_ExaminingQuality(Shape/Form)> , :ARTWORK_39_Modeling , :ARTWORK_39_SetupAndTestingOfTheMetalMold , :ARTWORK_36_SetupAndTestingOfTheMetalMold , :ARTWORK_39_PickingUpColouredPanel , <http://www.semanticweb.org/ontologies/Daan/2020/BarbaraNanning#ARTWORK_39_ExaminingQuality(Shape/Form)> , :ARTWORK_39_PreparingGlass ;
        :Works-For    :VRIJGLASZaandam , :GlassStudioVanTetterode .

:ARTWORK_73_ExaminingTheQualityOfTheGlass
        a                 owl:NamedIndividual , :Examining_the_Quality_of_the_Glass ;
        rdfs:comment      "Instance of an activity which is part of the creation process of ARTWORK_73."@en ;
        rdfs:label        "ARTWORK_73_Examining the Quality of the Glass"@en ;
        :Followed-By      :ARTWORK_73_Cooling ;
        :Follows          :ARTWORK_73_Modeling ;
        :Has-Duration     <http://www.semanticweb.org/ontologies/Daan/2020/BarbaraNanning#2018> ;
        :Involves         :BarbaraNanning , :LuděkKout , <http://www.semanticweb.org/ontologies/Daan/2020/BarbaraNanning#RadekKoten(CZ)> ;
        :Located-In       :CzechRepublic ;
        :Part-Of          :Creation_Artwork_73 ;
        :Requires-Use-Of  :StraightShears , :YokeOfSupport , :Water , :Blocks , :CeramicPotFilledWithGlass , :BlowingPipe , :Paper , :Furnace , :DiamondShears , :Pontis , :GloryHole , :Jacks , :AnnealingKiln .

:ARTWORK_74_Packing_4
        a              owl:NamedIndividual , :Packing ;
        rdfs:comment   "Instance of an activity which is part of the creation process of ARTWORK_74."@en ;
        rdfs:label     "ARTWORK_74_Packing_4"@en ;
        :Followed-By   :ARTWORK_74_Transporting_4 ;
        :Follows       <http://www.semanticweb.org/ontologies/Daan/2020/BarbaraNanning#ARTWORK_74_ExaminingQuality(FinalResult)> ;
        :Has-Duration  <http://www.semanticweb.org/ontologies/Daan/2020/BarbaraNanning#2008> ;
        :Involves      :AlešZvěřina , :BarbaraNanning , :VáçlavNovák_Doksy_CzechRepublic ;
        :Located-In    :CzechRepublic ;
        :Part-Of       :Creation_Artwork_74 .

:ARTWORK_77_Documenting
        a              :Documenting , owl:NamedIndividual ;
        rdfs:comment   "Instance of an activity which is part of the creation process of ARTWORK_77."@en ;
        rdfs:label     "ARTWORK_77_Documenting"@en ;
        :Followed-By   :ARTWORK_77_Packing_5 ;
        :Follows       :ARTWORK_77_Photographing ;
        :Has-Duration  <http://www.semanticweb.org/ontologies/Daan/2020/BarbaraNanning#2018> ;
        :Involves      :BarbaraNanning ;
        :Located-In    :CzechRepublic ;
        :Part-Of       :Creation_Artwork_77 .

:ARTWORK_78_Translocating
        a                 :Translocating , owl:NamedIndividual ;
        rdfs:comment      "Instance of an activity which is part of the creation process of ARTWORK_78."@en ;
        rdfs:label        "ARTWORK_78_Translocating"@en ;
        :Followed-By      :ARTWORK_78_Cooling ;
        :Follows          <http://www.semanticweb.org/ontologies/Daan/2020/BarbaraNanning#ARTWORK_78_ExaminingQuality(Shape/Form)> ;
        :Has-Duration     <http://www.semanticweb.org/ontologies/Daan/2020/BarbaraNanning#2008> ;
        :Involves         :BarbaraNanning ;
        :Located-In       :CzechRepublic ;
        :Part-Of          :Creation_Artwork_78 ;
        :Requires-Use-Of  :Fork .

:ARTWORK_75_Transporting_4
        a              owl:NamedIndividual , :Transporting ;
        rdfs:comment   "Instance of an activity which is part of the creation process of ARTWORK_75."@en ;
        rdfs:label     "ARTWORK_75_Transporting_4"@en ;
        :Followed-By   :ARTWORK_75_Photographing ;
        :Follows       :ARTWORK_75_Packing_4 ;
        :Has-Duration  <http://www.semanticweb.org/ontologies/Daan/2020/BarbaraNanning#2018> ;
        :Involves      :BarbaraNanning , :AlešZvěřina ;
        :Located-In    :CzechRepublic ;
        :Part-Of       :Creation_Artwork_75 .

<http://www.semanticweb.org/ontologies/Daan/2020/BarbaraNanning#Ji%C5%99%C3%ADPa%C4%8DinekLindava(CZ)>
        a             :Glass_Studio , owl:NamedIndividual ;
        rdfs:comment  "Jiří Pačinek Lindava (CZ) is a glass studio in Lindava."@en ;
        rdfs:label    "Jiří Pačinek Lindava (CZ)"@en ;
        owl:sameAs    <http://www.wikidata.org/entity/Q60337044> ;
        :Employed     :JanBaštýř , :JaroslavKubásek , <http://www.semanticweb.org/ontologies/Daan/2020/BarbaraNanning#JiriPacinek(CZ)> , :JiříPačinekJunior , :DavidČerný ;
        :Located-In   :Lindava ;
        :Maker-Of     :Artwork_18_64 , :Artwork_36 , :Artwork_46 .

:ARTWORK_44_Packing_5
        a              owl:NamedIndividual , :Packing ;
        rdfs:comment   "Instance of an activity which is part of the creation process of ARTWORK_44."@en ;
        rdfs:label     "ARTWORK_44_Packing_5"@en ;
        :Finishes      :Creation_Artwork_44 ;
        :Follows       :ARTWORK_44_Documenting ;
        :Has-Duration  <http://www.semanticweb.org/ontologies/Daan/2020/BarbaraNanning#2018> ;
        :Involves      :BarbaraNanning ;
        :Located-In    :CzechRepublic ;
        :Part-Of       :Creation_Artwork_44 .

:ARTWORK_43_Documenting
        a              :Documenting , owl:NamedIndividual ;
        rdfs:comment   "Instance of an activity which is part of the creation process of ARTWORK_43."@en ;
        rdfs:label     "ARTWORK_43_Documenting"@en ;
        :Followed-By   :ARTWORK_43_Packing_5 ;
        :Follows       :ARTWORK_43_Photographing ;
        :Has-Duration  <http://www.semanticweb.org/ontologies/Daan/2020/BarbaraNanning#2008> ;
        :Involves      :BarbaraNanning ;
        :Located-In    :CzechRepublic ;
        :Part-Of       :Creation_Artwork_43 .

:ARTWORK_74_Packing  a  :Packing , owl:NamedIndividual ;
        rdfs:comment   "Instance of an activity which is part of the creation process of ARTWORK_74."@en ;
        rdfs:label     "ARTWORK_74_Packing"@en ;
        :Followed-By   :ARTWORK_74_Transporting ;
        :Follows       :ARTWORK_74_Cooling ;
        :Has-Duration  <http://www.semanticweb.org/ontologies/Daan/2020/BarbaraNanning#2008> ;
        :Involves      :AlešZvěřina , :BarbaraNanning ;
        :Located-In    :CzechRepublic ;
        :Part-Of       :Creation_Artwork_74 .

:ARTWORK_36_Signing  a    owl:NamedIndividual , :Signing ;
        rdfs:comment      "Instance of an activity which is part of the creation process of ARTWORK_36."@en ;
        rdfs:label        "ARTWORK_36_Signing"@en ;
        :Followed-By      <http://www.semanticweb.org/ontologies/Daan/2020/BarbaraNanning#ARTWORK_36_ExaminingQuality(FinalResult)> ;
        :Follows          :ARTWORK_36_Sandblasting ;
        :Has-Duration     <http://www.semanticweb.org/ontologies/Daan/2020/BarbaraNanning#2019> ;
        :Involves         :AlešZvěřina , :BarbaraNanning ;
        :Located-In       :NovyBor ;
        :Part-Of          :Creation_Artwork_36 ;
        :Requires-Use-Of  :AirCompressor .

:ARTWORK_76_Sensing  a  owl:NamedIndividual , :Sensing ;
        rdfs:comment   "Instance of an activity which is part of the creation process of ARTWORK_76."@en ;
        rdfs:label     "ARTWORK_76_Sensing"@en ;
        :Followed-By   :ARTWORK_76_Modeling ;
        :Follows       :ARTWORK_76_Glassblowing ;
        :Has-Duration  <http://www.semanticweb.org/ontologies/Daan/2020/BarbaraNanning#2018> ;
        :Involves      :BarbaraNanning , :AlešZvěřina , :LukášSvoboda ;
        :Located-In    :CzechRepublic ;
        :Part-Of       :Creation_Artwork_76 .

:ARTWORK_36_Photographing_2
        a              :Photographing , owl:NamedIndividual ;
        rdfs:comment   "Instance of an activity which is part of the creation process of ARTWORK_36."@en ;
        rdfs:label     "ARTWORK_36_Photographing_2"@en ;
        :Followed-By   :ARTWORK_36_Packing_8 ;
        :Follows       :ARTWORK_36_Transporting_6 ;
        :Has-Duration  <http://www.semanticweb.org/ontologies/Daan/2020/BarbaraNanning#2019> ;
        :Involves      :BarbaraNanning , <http://www.semanticweb.org/ontologies/Daan/2020/BarbaraNanning#TomHaartsen_Ouderkerka/dAmstel(NL)> ;
        :Located-In    <http://www.semanticweb.org/ontologies/Daan/2020/BarbaraNanning#Ouderkerka/dAmstel> ;
        :Part-Of       :Creation_Artwork_36 .

:ARTWORK_43_ApplyingClearGlassBell
        a                 :Applying_Clear_Glass_Bell , owl:NamedIndividual ;
        rdfs:comment      "Instance of an activity which is part of the creation process of ARTWORK_43."@en ;
        rdfs:label        "ARTWORK_43_Applying Clear Glass Bell"@en ;
        :Followed-By      :ARTWORK_43_ApplyingExtraColour ;
        :Follows          :ARTWORK_43_SetupAndTestingOfTheMetalMold_2 ;
        :Has-Duration     <http://www.semanticweb.org/ontologies/Daan/2020/BarbaraNanning#2008> ;
        :Involves         :BarbaraNanning , <http://www.semanticweb.org/ontologies/Daan/2020/BarbaraNanning#RostislavMaterka(CZ)> , <http://www.semanticweb.org/ontologies/Daan/2020/BarbaraNanning#AlesVacek(CZ)> ;
        :Located-In       :CzechRepublic ;
        :Part-Of          :Creation_Artwork_43 ;
        :Processes        :AJETOClearGlass ;
        :Requires-Use-Of  :Pincet , :YokeOfSupport , :BlowingPipe , :Water , :Paper , :Beeswax , :Furnace , :Marver , :Jacks , :AirCompressor , :StraightShears , :Hook , :CeramicPotFilledWithGlass , :IcePick , :Blocks , :DiamondShears .

:ARTWORK_43_Signing  a    :Signing , owl:NamedIndividual ;
        rdfs:comment      "Instance of an activity which is part of the creation process of ARTWORK_43."@en ;
        rdfs:label        "ARTWORK_43_Signing"@en ;
        :Followed-By      :ARTWORK_43_Packing_3 ;
        :Follows          :ARTWORK_44_Transporting_2 ;
        :Has-Duration     <http://www.semanticweb.org/ontologies/Daan/2020/BarbaraNanning#2008> ;
        :Involves         :BarbaraNanning , :AlešZvěřina ;
        :Located-In       :CzechRepublic ;
        :Part-Of          :Creation_Artwork_43 ;
        :Requires-Use-Of  :AirCompressor .

:ARTWORK_43_Gilding  a    :Gilding , owl:NamedIndividual ;
        rdfs:comment      "Instance of an activity which is part of the creation process of ARTWORK_43."@en ;
        rdfs:label        "ARTWORK_43_Gilding"@en ;
        :Followed-By      <http://www.semanticweb.org/ontologies/Daan/2020/BarbaraNanning#ARTWORK_43_ExaminingQuality(FinalResult)> ;
        :Follows          :ARTWORK_43_Transporting_3 ;
        :Has-Duration     <http://www.semanticweb.org/ontologies/Daan/2020/BarbaraNanning#2008> ;
        :Involves         :BarbaraNanning , :VáçlavNovák_Doksy_CzechRepublic ;
        :Located-In       :CzechRepublic ;
        :Part-Of          :Creation_Artwork_43 ;
        :Requires-Use-Of  :GildingCushion , :INSTACOLLTool , :GildersKnife , :GildersTip .

:ARTWORK_46_CuttingMonochromeSheets
        a              owl:NamedIndividual , :Cutting_Monochrome_Sheets ;
        rdfs:comment   "Instance of an activity which is part of the creation process of ARTWORK_46."@en ;
        rdfs:label     "ARTWORK_46_Cutting Monochrome Sheets"@en ;
        :Followed-By   :ARTWORK_46_Ordening ;
        :Follows       :ARTWORK_46_DecidingColourPaletteAndPatterns ;
        :Has-Duration  <http://www.semanticweb.org/ontologies/Daan/2020/BarbaraNanning#2015> ;
        :Involves      :BarbaraNanning , :SteefHendriks ;
        :Located-In    :Langweer ;
        :Part-Of       :Creation_Artwork_46 .

:ARTWORK_44_SetupAndTestingOfTheMetalMold
        a                 :Setup_and_Testing_of_the_Metal_Mold , owl:NamedIndividual ;
        rdfs:comment      "Instance of an activity which is part of the creation process of ARTWORK_44."@en ;
        rdfs:label        "ARTWORK_44_Setup and Testing of the Metal Mold"@en ;
        :Followed-By      :ARTWORK_44_ExaminingTheQualityOfTheGlass ;
        :Follows          :ARTWORK_44_PreparingGlass ;
        :Has-Duration     <http://www.semanticweb.org/ontologies/Daan/2020/BarbaraNanning#2018> ;
        :Involves         :BarbaraNanning , <http://www.semanticweb.org/ontologies/Daan/2020/BarbaraNanning#Tom%C3%A1%C5%A1Moravec(CZ)> , <http://www.semanticweb.org/ontologies/Daan/2020/BarbaraNanning#RadekKoten(CZ)> , <http://www.semanticweb.org/ontologies/Daan/2020/BarbaraNanning#JiriMoravec(CZ)> , <http://www.semanticweb.org/ontologies/Daan/2020/BarbaraNanning#LukasHavlas(CZ)> , :AssistantOfBarbara ;
        :Located-In       :CzechRepublic ;
        :Part-Of          :Creation_Artwork_44 ;
        :Requires-Use-Of  :InterchangeableMetalMoldSetup .

:UnitedStatesOfAmerica
        a             :Country , owl:NamedIndividual ;
        rdfs:comment  "The United States of America is a federation of states and the district of Columbia located in North-America."@en ;
        rdfs:label    "United States of America"@en ;
        owl:sameAs    <http://www.wikidata.org/entity/Q30> ;
        :Location-Of  :NewYork .

:ARTWORK_39_Sandblasting
        a                 :Sandblasting , owl:NamedIndividual ;
        rdfs:comment      "Instance of an activity which is part of the creation process of ARTWORK_39."@en ;
        rdfs:label        "ARTWORK_39_Sandblasting"@en ;
        :Followed-By      :ARTWORK_39_Signing ;
        :Follows          :ARTWORK_39_Polishing ;
        :Has-Duration     <http://www.semanticweb.org/ontologies/Daan/2020/BarbaraNanning#2015> ;
        :Involves         :BarbaraNanning , :AlešZvěřina ;
        :Located-In       :NovyBor ;
        :Part-Of          :Creation_Artwork_39 ;
        :Requires-Use-Of  :AirCompressor .

:Thing  a                owl:Class ;
        rdfs:comment     "A thing is a inanimate, material object or entity."@en ;
        rdfs:label       "Thing"@en ;
        rdfs:subClassOf  :Entity .

:ARTWORK_36_Transporting_3
        a              owl:NamedIndividual , :Transporting ;
        rdfs:comment   "Instance of an activity which is part of the creation process of ARTWORK_36."@en ;
        rdfs:label     "ARTWORK_36_Transporting_3"@en ;
        :Followed-By   :ARTWORK_36_Photographing ;
        :Follows       :ARTWORK_36_Packing_3 ;
        :Has-Duration  <http://www.semanticweb.org/ontologies/Daan/2020/BarbaraNanning#2019> ;
        :Involves      :AlešZvěřina , :BarbaraNanning ;
        :Located-In    :Amsterdam ;
        :Part-Of       :Creation_Artwork_36 .

:ARTWORK_78_Grinding  a   :Grinding , owl:NamedIndividual ;
        rdfs:comment      "Instance of an activity which is part of the creation process of ARTWORK_78."@en ;
        rdfs:label        "ARTWORK_78_Grinding"@en ;
        :Followed-By      :ARTWORK_78_Polishing ;
        :Follows          :ARTWORK_78_Sawing ;
        :Has-Duration     <http://www.semanticweb.org/ontologies/Daan/2020/BarbaraNanning#2008> ;
        :Involves         :AlešZvěřina , :RobertFlorian , :BarbaraNanning ;
        :Located-In       :CzechRepublic ;
        :Part-Of          :Creation_Artwork_78 ;
        :Requires-Use-Of  :GrindingWheel , :SharpeningStone .

<http://www.semanticweb.org/ontologies/Daan/2020/BarbaraNanning#ARTWORK_77_ExaminingQuality(CheckForIrregularitiesInTheGlass)>
        a              j.3: , owl:NamedIndividual ;
        rdfs:comment   "Instance of an activity which is part of the creation process of ARTWORK_77."@en ;
        rdfs:label     "ARTWORK_77_Examining Quality (Check for Irregularities in the Glass)"@en ;
        :Followed-By   :ARTWORK_77_Sawing ;
        :Follows       :ARTWORK_77_Resting ;
        :Has-Duration  <http://www.semanticweb.org/ontologies/Daan/2020/BarbaraNanning#2018> ;
        :Involves      :AlešZvěřina , :BarbaraNanning ;
        :Located-In    :CzechRepublic ;
        :Part-Of       :Creation_Artwork_77 .

:Deciding_Colour_Palette_and_Patterns
        a                owl:Class ;
        rdfs:comment     "The glass threads are about the pattern and the variety. Whimsicalness and dimensions evoke an image of cell division in nature. Color patterns, visible only at the cut ends of a glass thread, and a wide variety of cross sections (ranging between 0.5 - 5 cm) are essential. The details in particular make it either a dull or lively image, and largely determine the end result."@en ;
        rdfs:label       "Deciding Colour Palette and Patterns"@en ;
        rdfs:subClassOf  :Activity .

:Photographing  a        owl:Class ;
        rdfs:comment     "Photographing is an activity in which a photograph is taken of a thing."@en ;
        rdfs:label       "Photographing"@en ;
        rdfs:subClassOf  :Activity .

:BarbaraNanning  a    owl:NamedIndividual , :Creator ;
        rdfs:comment  "Barbara Nanning is a Dutch Ceramic-Glass artist."@en ;
        rdfs:label    "Barbara Nanning"@en ;
        owl:sameAs    <http://www.wikidata.org/entity/Q12013202> ;
        :Involved-In  :ARTWORK_79_Signing , :ARTWORK_44_Packing , :ARTWORK_80_SetupAndTestingOfTheMetalMold , :ARTWORK_75_Glassblowing , <http://www.semanticweb.org/ontologies/Daan/2020/BarbaraNanning#ARTWORK_74_ExaminingQuality(CheckForIrregularitiesInTheGlass)> , :ARTWORK_76_PreparingGlass , :ARTWORK_73_PreparingGlass , <http://www.semanticweb.org/ontologies/Daan/2020/BarbaraNanning#ARTWORK_79_ExaminingQuality(Shape/Form)> , :ARTWORK_73_ExaminingTheQualityOfTheGlass , <http://www.semanticweb.org/ontologies/Daan/2020/BarbaraNanning#ARTWORK_74_ExaminingQuality(Shape/Form)> , :ARTWORK_78_Signing , <http://www.semanticweb.org/ontologies/Daan/2020/BarbaraNanning#ARTWORK_44_ExaminingQuality(Shape/Form)> , :ARTWORK_80_Packing , :ARTWORK_76_Packing , :ARTWORK_77_ApplyingClearGlassBell , <http://www.semanticweb.org/ontologies/Daan/2020/BarbaraNanning#ARTWORK_44_ExaminingQuality(FinalResult)> , :ARTWORK_78_Documenting , :ARTWORK_78_HeatingMetalMold , :ARTWORK_78_Polishing , :ARTWORK_76_Translocating , :ARTWORK_77_ApplyingExtraColour , :ARTWORK_44_ApplyingExtraColour , :ARTWORK_44_Polishing , <http://www.semanticweb.org/ontologies/Daan/2020/BarbaraNanning#ARTWORK_78_ExaminingQuality(FinalResult)> , :ARTWORK_43_Gilding , :ARTWORK_80_MeasuringAndBoxesMaking , :ARTWORK_43_Photographing , :ARTWORK_78_PreparingGlass , :ARTWORK_44_HeatingMetalMold , :ARTWORK_73_SetupAndTestingOfTheMetalMold , :ARTWORK_79_Sawing , :ARTWORK_80_ExaminingTheQualityOfTheGlass , :ARTWORK_75_ApplyingExtraColour , :ARTWORK_74_Documenting , :ARTWORK_77_Documenting , :ARTWORK_79_Photographing , <http://www.semanticweb.org/ontologies/Daan/2020/BarbaraNanning#ARTWORK_80_ExaminingQuality(FinalResult)> , :ARTWORK_80_Sawing , :ARTWORK_80_Gilding , :ARTWORK_43_Sensing , :ARTWORK_79_ExaminingTheQualityOfTheGlass , :ARTWORK_79_Polishing , :ARTWORK_80_Polishing , :ARTWORK_43_Packing , :ARTWORK_74_ApplyingClearGlassBell , <http://www.semanticweb.org/ontologies/Daan/2020/BarbaraNanning#ARTWORK_76_ExaminingQuality(Shape/Form)> , :ARTWORK_78_SetupAndTestingOfTheMetalMold_2 , :ARTWORK_75_Signing , :ARTWORK_78_Packing_3 , :ARTWORK_43_SetupAndTestingOfTheMetalMold_2 , :ARTWORK_43_Grinding , :ARTWORK_74_Gilding , :ARTWORK_43_Glassblowing , :ARTWORK_76_Packing_2 , :ARTWORK_77_Packing_4 , :ARTWORK_74_Signing , :ARTWORK_79_Grinding , :ARTWORK_76_Packing_5 , :ARTWORK_43_Modeling , :ARTWORK_77_Sawing , :ARTWORK_77_Packing , :ARTWORK_77_SetupAndTestingOfTheMetalMold_2 , :ARTWORK_78_ExaminingTheQualityOfTheGlass , :ARTWORK_74_Packing , :ARTWORK_77_Packing_2 , :ARTWORK_43_Sawing , :ARTWORK_80_Glassblowing , :ARTWORK_78_Glassblowing , :ARTWORK_73_Packing_3 , :ARTWORK_76_Packing_3 , :ARTWORK_80_PreparingGlass , <http://www.semanticweb.org/ontologies/Daan/2020/BarbaraNanning#ARTWORK_76_ExaminingQuality(CheckForIrregularitiesInTheGlass)> , :ARTWORK_80_Signing , <http://www.semanticweb.org/ontologies/Daan/2020/BarbaraNanning#ARTWORK_77_ExaminingQuality(FinalResult)> , <http://www.semanticweb.org/ontologies/Daan/2020/BarbaraNanning#ARTWORK_43_ExaminingQuality(Result)> , :ARTWORK_78_Packing , <http://www.semanticweb.org/ontologies/Daan/2020/BarbaraNanning#ARTWORK_73_ExaminingQuality(CheckForIrregularitiesInTheGlass)> , :ARTWORK_80_Sensing , :ARTWORK_73_ApplyingClearGlassBell , :ARTWORK_75_Gilding , :ARTWORK_75_Documenting , :ARTWORK_73_Translocating , :ARTWORK_73_Gilding , :ARTWORK_78_ApplyingExtraColour , :ARTWORK_75_ApplyingClearGlassBell , :ARTWORK_74_HeatingMetalMold , :ARTWORK_76_Signing , :ARTWORK_77_Signing , :ARTWORK_80_Photographing , <http://www.semanticweb.org/ontologies/Daan/2020/BarbaraNanning#ARTWORK_43_ExaminingQuality(FinalResult)> , :ARTWORK_74_Grinding , :ARTWORK_74_PreparingGlass , :ARTWORK_75_Modeling , :ARTWORK_78_MeasuringAndBoxesMaking , :ARTWORK_76_ApplyingExtraColour_2 , :ARTWORK_75_PreparingGlass , :ARTWORK_73_SetupAndTestingOfTheMetalMold_2 , <http://www.semanticweb.org/ontologies/Daan/2020/BarbaraNanning#ARTWORK_80_ExaminingQuality(CheckForIrregularitiesInTheGlass)> , :ARTWORK_76_ApplyingExtraColour , :ARTWORK_75_Packing_5 , :ARTWORK_74_Packing_2 , :ARTWORK_77_PreparingGlass , :ARTWORK_73_Packing_5 , :ARTWORK_75_SetupAndTestingOfTheMetalMold , :ARTWORK_76_MeasuringAndBoxesMaking , :ARTWORK_43_ExaminingTheQualityOfTheGlass , :ARTWORK_44_Packing_4 , :ARTWORK_43_Packing_5 , :ARTWORK_75_Polishing , :ARTWORK_79_HeatingMetalMold , :ARTWORK_73_MeasuringAndBoxesMaking , :ARTWORK_76_Modeling , :ARTWORK_78_Sawing , :ARTWORK_79_ApplyingClearGlassBell , :ARTWORK_43_MeasuringAndBoxesMaking , :ARTWORK_44_Packing_2 , :ARTWORK_43_Packing_3 , :ARTWORK_73_Signing , :ARTWORK_76_Documenting , :ARTWORK_76_ExaminingTheQualityOfTheGlass , :ARTWORK_44_Translocating , <http://www.semanticweb.org/ontologies/Daan/2020/BarbaraNanning#ARTWORK_79_ExaminingQuality(CheckForIrregularitiesInTheGlass)> , :ARTWORK_44_Packing_5 , <http://www.semanticweb.org/ontologies/Daan/2020/BarbaraNanning#ARTWORK_75_ExaminingQuality(Result)> , :ARTWORK_77_HeatingMetalMold , :ARTWORK_79_SetupAndTestingOfTheMetalMold_2 , :ARTWORK_79_Packing_5 , :ARTWORK_73_Packing_2 , :ARTWORK_74_Packing_4 , :ARTWORK_43_Sandblasting , :ARTWORK_74_Sensing , :ARTWORK_74_Glassblowing , :ARTWORK_76_Sawing , <http://www.semanticweb.org/ontologies/Daan/2020/BarbaraNanning#ARTWORK_77_ExaminingQuality(Result)> , :ARTWORK_74_Photographing , <http://www.semanticweb.org/ontologies/Daan/2020/BarbaraNanning#ARTWORK_75_ExaminingQuality(FinalResult)> , :ARTWORK_76_Glassblowing , :ARTWORK_74_SetupAndTestingOfTheMetalMold , :ARTWORK_76_Photographing , :ARTWORK_77_Glassblowing , <http://www.semanticweb.org/ontologies/Daan/2020/BarbaraNanning#ARTWORK_77_ExaminingQuality(CheckForIrregularitiesInTheGlass)> , :ARTWORK_44_Glassblowing , :ARTWORK_44_Packing_3 , :ARTWORK_43_Packing_4 , <http://www.semanticweb.org/ontologies/Daan/2020/BarbaraNanning#ARTWORK_44_ExaminingQuality(CheckForIrregularitiesInTheGlass)> , :ARTWORK_75_Packing_3 , :ARTWORK_74_Polishing , :ARTWORK_76_Polishing , :ARTWORK_79_Translocating , :ARTWORK_80_Documenting , :ARTWORK_79_Sensing , :ARTWORK_78_SetupAndTestingOfTheMetalMold , :ARTWORK_74_Packing_5 , <http://www.semanticweb.org/ontologies/Daan/2020/BarbaraNanning#ARTWORK_80_ExaminingQuality(Shape/Form)> , :ARTWORK_78_Grinding , :ARTWORK_79_MeasuringAndBoxesMaking , :ARTWORK_73_Sandblasting , :ARTWORK_74_Translocating , :ARTWORK_79_ApplyingExtraColour , :ARTWORK_80_ApplyingClearGlassBell , :ARTWORK_77_Photographing , :ARTWORK_73_Polishing , <http://www.semanticweb.org/ontologies/Daan/2020/BarbaraNanning#ARTWORK_43_ExaminingQuality(Shape/Form)> , :ARTWORK_77_SetupAndTestingOfTheMetalMold , :ARTWORK_75_Packing_4 , :ARTWORK_79_PreparingGlass , <http://www.semanticweb.org/ontologies/Daan/2020/BarbaraNanning#ARTWORK_75_ExaminingQuality(CheckForIrregularitiesInTheGlass)> , :ARTWORK_43_Translocating , :ARTWORK_73_Packing_4 , :ARTWORK_78_ApplyingClearGlassBell , :ARTWORK_75_Photographing , :ARTWORK_80_Sandblasting , :ARTWORK_77_Grinding , :ARTWORK_43_HeatingMetalMold , :ARTWORK_79_Packing_3 , :ARTWORK_78_Translocating , :ARTWORK_80_Modeling , :ARTWORK_44_Sawing , :ARTWORK_73_Packing , <http://www.semanticweb.org/ontologies/Daan/2020/BarbaraNanning#ARTWORK_80_ExaminingQuality(Result)> , :ARTWORK_43_Documenting , :ARTWORK_76_SetupAndTestingOfTheMetalMold_2 , :ARTWORK_43_PreparingGlass , :ARTWORK_44_ApplyingClearGlassBell , :ARTWORK_75_Translocating , <http://www.semanticweb.org/ontologies/Daan/2020/BarbaraNanning#ARTWORK_78_ExaminingQuality(Result)> , <http://www.semanticweb.org/ontologies/Daan/2020/BarbaraNanning#ARTWORK_76_ExaminingQuality(CheckForIrregularitiesInTheGlass)_2> , :ARTWORK_75_Packing , :ARTWORK_43_Packing_2 , :ARTWORK_76_HeatingMetalMold , :ARTWORK_74_SetupAndTestingOfTheMetalMold_2 , <http://www.semanticweb.org/ontologies/Daan/2020/BarbaraNanning#ARTWORK_73_ExaminingQuality(Result)> , :ARTWORK_73_Modeling , :ARTWORK_77_Sensing , :ARTWORK_80_ApplyingExtraColour , :ARTWORK_78_Photographing , :ARTWORK_79_Packing_4 , :ARTWORK_43_SetupAndTestingOfTheMetalMold , :ARTWORK_74_Packing_3 , :ARTWORK_79_Modeling , :ARTWORK_44_Grinding , :ARTWORK_74_Modeling , :ARTWORK_44_MeasuringAndBoxesMaking , <http://www.semanticweb.org/ontologies/Daan/2020/BarbaraNanning#ARTWORK_79_ExaminingQuality(FinalResult)> , :ARTWORK_73_HeatingMetalMold , :ARTWORK_76_Gilding , <http://www.semanticweb.org/ontologies/Daan/2020/BarbaraNanning#ARTWORK_75_ExaminingQuality(Shape/Form)> , :ARTWORK_77_Polishing , :ARTWORK_76_SetupAndTestingOfTheMetalMold , :ARTWORK_79_Documenting , :ARTWORK_76_Grinding , :ARTWORK_44_Documenting , :ARTWORK_43_Polishing , :ARTWORK_44_Signing , :ARTWORK_75_Packing_2 , :ARTWORK_44_Modeling , :ARTWORK_73_Sawing , :ARTWORK_44_ApplyingExtraColour_2 , :ARTWORK_73_Photographing , :ARTWORK_80_SetupAndTestingOfTheMetalMold_2 , :ARTWORK_44_Gilding , :ARTWORK_75_Grinding , :ARTWORK_80_HeatingMetalMold , <http://www.semanticweb.org/ontologies/Daan/2020/BarbaraNanning#ARTWORK_78_ExaminingQuality(Shape/Form)> , :ARTWORK_76_Sensing , :ARTWORK_73_Documenting , :ARTWORK_43_ApplyingExtraColour , :ARTWORK_80_Packing_2 , :ARTWORK_79_ApplyingExtraColour_2 , :ARTWORK_76_ApplyingClearGlassBell , <http://www.semanticweb.org/ontologies/Daan/2020/BarbaraNanning#ARTWORK_73_ExaminingQuality(Shape/Form)> , :ARTWORK_74_ApplyingExtraColour , :ARTWORK_43_Signing , :ARTWORK_75_HeatingMetalMold , :ARTWORK_79_Gilding , :ARTWORK_78_Gilding , :ARTWORK_78_Sensing , :ARTWORK_80_Translocating , :ARTWORK_79_Glassblowing , <http://www.semanticweb.org/ontologies/Daan/2020/BarbaraNanning#ARTWORK_43_ExaminingQuality(CheckForIrregularitiesInTheGlass)> , :ARTWORK_80_Packing_3 , :ARTWORK_44_PreparingGlass , :ARTWORK_79_SetupAndTestingOfTheMetalMold , :ARTWORK_77_Modeling , :ARTWORK_79_Packing_2 , :ARTWORK_74_ExaminingTheQualityOfTheGlass , :ARTWORK_44_Sensing , :ARTWORK_75_ExaminingTheQualityOfTheGlass , :ARTWORK_80_Grinding , <http://www.semanticweb.org/ontologies/Daan/2020/BarbaraNanning#ARTWORK_78_ExaminingQuality(CheckForIrregularitiesInTheGlass)> , :ARTWORK_73_Glassblowing , :ARTWORK_75_Sensing , :ARTWORK_80_Packing_4 , :ARTWORK_78_Packing_4 , <http://www.semanticweb.org/ontologies/Daan/2020/BarbaraNanning#ARTWORK_73_ExaminingQuality(FinalResult)> , :ARTWORK_44_Photographing , :ARTWORK_79_Packing , :ARTWORK_78_Modeling , :ARTWORK_44_SetupAndTestingOfTheMetalMold , :ARTWORK_73_Grinding , :ARTWORK_77_Packing_5 , :ARTWORK_77_Translocating , :ARTWORK_75_Sandblasting , <http://www.semanticweb.org/ontologies/Daan/2020/BarbaraNanning#ARTWORK_74_ExaminingQuality(FinalResult)> , :ARTWORK_77_Gilding , :ARTWORK_75_Sawing , :ARTWORK_75_ApplyingExtraColour_2 , :ARTWORK_73_Sensing , :ARTWORK_77_ExaminingTheQualityOfTheGlass , :ARTWORK_44_SetupAndTestingOfTheMetalMold_2 , :ARTWORK_75_SetupAndTestingOfTheMetalMold_2 , :ARTWORK_77_MeasuringAndBoxesMaking , :ARTWORK_78_Packing_2 , <http://www.semanticweb.org/ontologies/Daan/2020/BarbaraNanning#ARTWORK_74_ExaminingQuality(Result)> , <http://www.semanticweb.org/ontologies/Daan/2020/BarbaraNanning#ARTWORK_77_ExaminingQuality(Shape/Form)> , :ARTWORK_44_ExaminingTheQualityOfTheGlass , :ARTWORK_74_Sawing , :ARTWORK_76_Sandblasting , :ARTWORK_78_Packing_5 , :ARTWORK_77_Packing_3 , <http://www.semanticweb.org/ontologies/Daan/2020/BarbaraNanning#ARTWORK_79_ExaminingQuality(Result)> , :ARTWORK_43_ApplyingClearGlassBell , :ARTWORK_74_ApplyingExtraColour_2 , <http://www.semanticweb.org/ontologies/Daan/2020/BarbaraNanning#ARTWORK_76_ExaminingQuality(FinalResult)> , :ARTWORK_76_Packing_4 ;
        :Maintains    :CollectionOfBarbaraNanning ;
        :Maker-Of     :Artwork_74 , :Artwork_76 , :Artwork_79 , :Artwork_75 , :Artwork_43 , :Artwork_77 , :Artwork_44 , :Artwork_80 , :Artwork_73 , :Artwork_78 .

:ARTWORK_18_64_Ordening
        a                 :Ordening , owl:NamedIndividual ;
        rdfs:comment      "Instance of an activity which is part of the creation process of ARTWORK_18_64."@en ;
        rdfs:label        "ARTWORK_18_64_Ordening"@en ;
        :Followed-By      :ARTWORK_18_64_Casting ;
        :Follows          :ARTWORK_18_64_CuttingMonochromeSheets ;
        :Has-Duration     <http://www.semanticweb.org/ontologies/Daan/2020/BarbaraNanning#2015> ;
        :Involves         :BarbaraNanning ;
        :Located-In       :Langweer ;
        :Part-Of          :Creation_Artwork_18_64 ;
        :Requires-Use-Of  :Glassscissors , :Pincet , :Computer .

:ARTWORK_73_Resting  a    :Resting , owl:NamedIndividual ;
        rdfs:comment      "Instance of an activity which is part of the creation process of ARTWORK_73."@en ;
        rdfs:label        "ARTWORK_73_Resting"@en ;
        :Followed-By      <http://www.semanticweb.org/ontologies/Daan/2020/BarbaraNanning#ARTWORK_73_ExaminingQuality(CheckForIrregularitiesInTheGlass)> ;
        :Follows          :ARTWORK_73_Transporting ;
        :Has-Duration     <http://www.semanticweb.org/ontologies/Daan/2020/BarbaraNanning#2018> ;
        :Involves         :AlešZvěřina ;
        :Located-In       :CzechRepublic ;
        :Part-Of          :Creation_Artwork_73 ;
        :Requires-Use-Of  :AnnealingKiln .

:JosefUjka  a         :Grinder_3 , owl:NamedIndividual ;
        rdfs:comment  "Josef Ujka is a Grinder 3."@en ;
        rdfs:label    "Josef Ujka"@en .

:ARTWORK_78_Packing_2
        a              owl:NamedIndividual , :Packing ;
        rdfs:comment   "Instance of an activity which is part of the creation process of ARTWORK_78."@en ;
        rdfs:label     "ARTWORK_78_Packing_2"@en ;
        :Followed-By   :ARTWORK_78_Transporting_2 ;
        :Follows       :ARTWORK_78_MeasuringAndBoxesMaking ;
        :Has-Duration  <http://www.semanticweb.org/ontologies/Daan/2020/BarbaraNanning#2008> ;
        :Involves      :AlešZvěřina , :BarbaraNanning ;
        :Located-In    :CzechRepublic ;
        :Part-Of       :Creation_Artwork_78 .

<http://vocab.getty.edu/aat/300157460>
        a                    owl:Class ;
        owl:equivalentClass  :Studio .

:ARTWORK_74_ApplyingExtraColour_2
        a                 owl:NamedIndividual , :Applying_Extra_Colour ;
        rdfs:comment      "Instance of an activity which is part of the creation process of ARTWORK_74."@en ;
        rdfs:label        "ARTWORK_74_Applying Extra Colour_2"@en ;
        :Followed-By      :ARTWORK_74_HeatingMetalMold ;
        :Follows          :ARTWORK_74_ApplyingExtraColour ;
        :Has-Duration     <http://www.semanticweb.org/ontologies/Daan/2020/BarbaraNanning#2008> ;
        :Involves         <http://www.semanticweb.org/ontologies/Daan/2020/BarbaraNanning#RostislavMaterka(CZ)> , :BarbaraNanning , <http://www.semanticweb.org/ontologies/Daan/2020/BarbaraNanning#AlesVacek(CZ)> ;
        :Located-In       :CzechRepublic ;
        :Part-Of          :Creation_Artwork_74 ;
        :Processes        :AJETOAmberGlass ;
        :Requires-Use-Of  :DiamondShears , :BlowingPipe , :Jacks , :CeramicPotFilledWithGlass , :Fork , :GloryHole , :IcePick , :Hook , :Paper , :Pontis , :Beeswax , :YokeOfSupport , :Garage , :AnnealingKiln , :Blocks , :Pincet , :Tagliol , :Furnace , :StraightShears , :Water , :Marver , :AirCompressor .

:ARTWORK_44_MeasuringAndBoxesMaking
        a              owl:NamedIndividual , :Measuring_and_Boxes_Making ;
        rdfs:comment   "Instance of an activity which is part of the creation process of ARTWORK_44."@en ;
        rdfs:label     "ARTWORK_44_Measuring and Boxes Making"@en ;
        :Followed-By   :ARTWORK_44_Packing_2 ;
        :Follows       :ARTWORK_44_Polishing ;
        :Has-Duration  <http://www.semanticweb.org/ontologies/Daan/2020/BarbaraNanning#2018> ;
        :Involves      :BarbaraNanning , :AlešZvěřina ;
        :Located-In    :CzechRepublic ;
        :Part-Of       :Creation_Artwork_44 .

:ARTWORK_44_Photographing
        a              owl:NamedIndividual , :Photographing ;
        rdfs:comment   "Instance of an activity which is part of the creation process of ARTWORK_44."@en ;
        rdfs:label     "ARTWORK_44_Photographing"@en ;
        :Followed-By   :ARTWORK_44_Documenting ;
        :Follows       :ARTWORK_44_Transporting_4 ;
        :Has-Duration  <http://www.semanticweb.org/ontologies/Daan/2020/BarbaraNanning#2018> ;
        :Involves      :BarbaraNanning , <http://www.semanticweb.org/ontologies/Daan/2020/BarbaraNanning#TomHaartsen_Ouderkerka/dAmstel(NL)> ;
        :Located-In    :CzechRepublic ;
        :Part-Of       :Creation_Artwork_44 .

<http://www.semanticweb.org/ontologies/Daan/2020/BarbaraNanning#PaulGroot(NL)>
        a             owl:NamedIndividual , :Grinder_1 ;
        rdfs:comment  "Paul Groot (NL) is a Grinder 1."@en ;
        rdfs:label    "Paul Groot (NL)"@en ;
        :Involved-In  :ARTWORK_39_CuttingSheets , :ARTWORK_18_64_CuttingSheets ;
        :Works-For    :GlassStudioVanTetterode .

:Filling_Kilns_with_Metal_Bowl
        a                owl:Class ;
        rdfs:comment     "The evening before blowing, the (stainless steel) metal bowls with canes are placed in the glassworks in a warming oven and brought to a temperature of 650 degrees overnight."@en ;
        rdfs:label       "Filling Kilns with Metal Bowl"@en ;
        rdfs:subClassOf  :Activity .

:ARTWORK_17_33_Photographing
        a              :Photographing , owl:NamedIndividual ;
        rdfs:comment   "Instance of an activity which is part of the creation process of ARTWORK_17_33."@en ;
        rdfs:label     "ARTWORK_17_33_Photographing"@en ;
        :Followed-By   :ARTWORK_17_33_Packing_3 ;
        :Follows       :ARTWORK_17_33_Transporting_2 ;
        :Has-Duration  <http://www.semanticweb.org/ontologies/Daan/2020/BarbaraNanning#2017> ;
        :Involves      <http://www.semanticweb.org/ontologies/Daan/2020/BarbaraNanning#TomHaartsen_Ouderkerka/dAmstel(NL)> , :BarbaraNanning ;
        :Located-In    <http://www.semanticweb.org/ontologies/Daan/2020/BarbaraNanning#Ouderkerka/dAmstel> ;
        :Part-Of       :Creation_Artwork_17_33 .

:ARTWORK_39_SetupAndTestingOfTheMetalMold
        a                 :Setup_and_Testing_of_the_Metal_Mold , owl:NamedIndividual ;
        rdfs:comment      "Instance of an activity which is part of the creation process of ARTWORK_39."@en ;
        rdfs:label        "ARTWORK_39_Setup and Testing of the Metal Mold"@en ;
        :Followed-By      :ARTWORK_39_PreparingGlass ;
        :Follows          :ARTWORK_39_ExaminingTheQualityOfTheGlass ;
        :Has-Duration     <http://www.semanticweb.org/ontologies/Daan/2020/BarbaraNanning#2015> ;
        :Involves         :GertBullée , <http://www.semanticweb.org/ontologies/Daan/2020/BarbaraNanning#MarekBrathko(CZ)> , <http://www.semanticweb.org/ontologies/Daan/2020/BarbaraNanning#RobertLenner(CZ)> , <http://www.semanticweb.org/ontologies/Daan/2020/BarbaraNanning#JessicaHomich(USA)> , <http://www.semanticweb.org/ontologies/Daan/2020/BarbaraNanning#MarekEffmert(CZ)> , :BarbaraNanning ;
        :Located-In       :Zaandam ;
        :Part-Of          :Creation_Artwork_39 ;
        :Requires-Use-Of  :InterchangeableMetalMoldSetup .

<http://vocab.getty.edu/aat/300133025>
        a                    owl:Class ;
        owl:equivalentClass  :Artwork .

:ARTWORK_39_ComposingColouredPatternsWithSheetsAndStrings
        a                 owl:NamedIndividual , :Composing_Coloured_Patterns_with_Sheets_and_Strings ;
        rdfs:comment      "Instance of an activity which is part of the creation process of ARTWORK_39."@en ;
        rdfs:label        "ARTWORK_39_Composing Coloured Patterns with Sheets and Strings"@en ;
        :Followed-By      :ARTWORK_39_FusingSheetsAndStrings ;
        :Follows          :ARTWORK_39_CuttingStrings ;
        :Has-Duration     <http://www.semanticweb.org/ontologies/Daan/2020/BarbaraNanning#2015> ;
        :Involves         :BarbaraNanning ;
        :Located-In       :Amsterdam ;
        :Part-Of          :Creation_Artwork_39 ;
        :Requires-Use-Of  :Glassscissors , :Pincet , :Water , :FusingKiln .

<http://www.semanticweb.org/ontologies/Daan/2020/BarbaraNanning#MuseeDeDesignEtd'artsAppliquesContemporains>
        a             owl:NamedIndividual , :Museum ;
        rdfs:comment  "The Musee de design et d'arts appliques contemporains is a museum located in Lausanne (Switzerland)."@en ;
        rdfs:label    "Musee de design et d'arts appliques contemporains"@en ;
        owl:sameAs    <http://www.wikidata.org/entity/Q3329765> ;
        :Located-In   :Lausanne ;
        :Maintains    <http://www.semanticweb.org/ontologies/Daan/2020/BarbaraNanning#CollectionMuseeDeDesignEtd'artsAppliquesContemporains> .

:Creation_Artwork_78  a  :Creation_Event , owl:NamedIndividual ;
        rdfs:comment    "Creation event for an artwork by Barbara Nanning displayed in \"Barbara Nanning Eeuwige Beweging\" by Eliens (2019)."@en ;
        rdfs:label      "Creation_Artwork_78"@en ;
        :Consists-Of    <http://www.semanticweb.org/ontologies/Daan/2020/BarbaraNanning#ARTWORK_78_ExaminingQuality(Shape/Form)> , :ARTWORK_78_Polishing , :ARTWORK_78_Sawing , :ARTWORK_78_PreparingGlass , :ARTWORK_78_Transporting_4 , :ARTWORK_78_MeasuringAndBoxesMaking , :ARTWORK_78_Modeling , :ARTWORK_78_Packing_3 , :ARTWORK_78_Packing , :ARTWORK_78_Documenting , <http://www.semanticweb.org/ontologies/Daan/2020/BarbaraNanning#ARTWORK_78_ExaminingQuality(FinalResult)> , :ARTWORK_78_Photographing , :ARTWORK_78_Glassblowing , :ARTWORK_78_Transporting_3 , :ARTWORK_78_Transporting , :ARTWORK_78_Gilding , :ARTWORK_78_Translocating , :ARTWORK_78_ApplyingExtraColour , :ARTWORK_78_Packing_5 , :ARTWORK_78_ApplyingClearGlassBell , :ARTWORK_78_Packing_2 , :ARTWORK_78_Resting , <http://www.semanticweb.org/ontologies/Daan/2020/BarbaraNanning#ARTWORK_78_ExaminingQuality(CheckForIrregularitiesInTheGlass)> , <http://www.semanticweb.org/ontologies/Daan/2020/BarbaraNanning#ARTWORK_78_ExaminingQuality(Result)> , :ARTWORK_78_HeatingMetalMold , :ARTWORK_78_Grinding , :ARTWORK_78_Packing_4 , :ARTWORK_78_SetupAndTestingOfTheMetalMold_2 , :ARTWORK_78_ExaminingTheQualityOfTheGlass , :ARTWORK_78_Transporting_2 , :ARTWORK_78_Sensing , :ARTWORK_78_SetupAndTestingOfTheMetalMold , :ARTWORK_78_Cooling , :ARTWORK_78_Signing ;
        :Created        :Artwork_78 ;
        :Finishes-With  :ARTWORK_78_Packing_5 ;
        :Has-Duration   <http://www.semanticweb.org/ontologies/Daan/2020/BarbaraNanning#2016> ;
        :Located-In     :CzechRepublic ;
        :Starts-With    :ARTWORK_78_PreparingGlass ;
        :Within-Period  :GlassVerreÉglomisé .

:ARTWORK_78_Packing  a  :Packing , owl:NamedIndividual ;
        rdfs:comment   "Instance of an activity which is part of the creation process of ARTWORK_78."@en ;
        rdfs:label     "ARTWORK_78_Packing"@en ;
        :Followed-By   :ARTWORK_78_Transporting ;
        :Follows       :ARTWORK_78_Cooling ;
        :Has-Duration  <http://www.semanticweb.org/ontologies/Daan/2020/BarbaraNanning#2008> ;
        :Involves      :AlešZvěřina , :BarbaraNanning ;
        :Located-In    :CzechRepublic ;
        :Part-Of       :Creation_Artwork_78 .

:Rubber  a                :Man-Made_Material , owl:NamedIndividual ;
        rdfs:comment      "Rubber is a tough, elastic polymeric material made from the latex of a tropical plant or synthetically."@en ;
        rdfs:label        "Rubber"@en ;
        :Is-Processed-In  :INSTACOLLTool .

:ARTWORK_74_Transporting_4
        a              owl:NamedIndividual , :Transporting ;
        rdfs:comment   "Instance of an activity which is part of the creation process of ARTWORK_74."@en ;
        rdfs:label     "ARTWORK_74_Transporting_4"@en ;
        :Followed-By   :ARTWORK_74_Photographing ;
        :Follows       :ARTWORK_74_Packing_4 ;
        :Has-Duration  <http://www.semanticweb.org/ontologies/Daan/2020/BarbaraNanning#2008> ;
        :Involves      :AlešZvěřina , :BarbaraNanning ;
        :Located-In    :CzechRepublic ;
        :Part-Of       :Creation_Artwork_74 .

:Creation_Artwork_46  a  :Creation_Event , owl:NamedIndividual ;
        rdfs:comment    "Creation event for Artwork_46 by Barbara Nanning."@en ;
        rdfs:label      "Creation_Artwork_46"@en ;
        :Consists-Of    :ARTWORK_46_Packing_3 , <http://www.semanticweb.org/ontologies/Daan/2020/BarbaraNanning#ARTWORK_46_ExaminingQuality(Shape/Form)> , :ARTWORK_46_TransportingMonochromeRods , :ARTWORK_46_Ordening , :ARTWORK_46_MeasuringAndBoxesMaking , :ARTWORK_46_Transporting , :ARTWORK_46_ApplyingClearOverlay , :ARTWORK_46_HeatingMetalMold , :ARTWORK_46_Sensing , :ARTWORK_46_Packing , <http://www.semanticweb.org/ontologies/Daan/2020/BarbaraNanning#ARTWORK_46_ExaminingQuality(CheckForIrregularitiesInTheGlass)> , :ARTWORK_46_PreparingGlass , :ARTWORK_46_PickingUpColouredCanesPattern , :ARTWORK_46_Cooling , :ARTWORK_46_TackfusingColouredCanesAndStrings , :ARTWORK_46_TransportingColouredCanes , :ARTWORK_46_ApplyingClearGlassBell , :ARTWORK_46_TransportingColouredCanes_2 , :ARTWORK_46_Photographing , :ARTWORK_46_Resting , :ARTWORK_46_Packing_2 , :ARTWORK_46_CuttingAndPolishingColouredCanes , :ARTWORK_46_MakingPatternsWithColouredCanesAndStringsInTheMetalBowl , :ARTWORK_46_Transporting_2 , :ARTWORK_46_Grinding , :ARTWORK_46_SetupAndTestingOfTheMetalMold , :ARTWORK_46_Documenting , :ARTWORK_46_PreparingForBlowing , :ARTWORK_46_Polishing , :ARTWORK_46_CuttingStrings , :ARTWORK_46_CuttingAndPolishingCastedMonochromeSheetsToSmallRods , :ARTWORK_46_ProducingColouredCanes , :ARTWORK_46_CuttingMonochromeSheets , :ARTWORK_46_Glassblowing , :ARTWORK_46_FillingKilnsWithMetalBowl , :ARTWORK_46_TransportingMetalBowlWithCanesAndStrings , :ARTWORK_46_DecidingColourPaletteAndPatterns_2 , <http://www.semanticweb.org/ontologies/Daan/2020/BarbaraNanning#ARTWORK_46_ExaminingQuality(Result)> , :ARTWORK_46_Sawing , :ARTWORK_46_Casting , :ARTWORK_46_Modeling , :ARTWORK_46_ExaminingTheQualityOfTheGlass , :ARTWORK_46_Sensing_2 , :ARTWORK_46_DecidingColourPaletteAndPatterns , :ARTWORK_46_Signing ;
        :Created        :Artwork_46 ;
        :Finishes-With  :ARTWORK_46_Documenting ;
        :Starts-With    :ARTWORK_46_DecidingColourPaletteAndPatterns .

:ARTWORK_18_64_Signing
        a                 owl:NamedIndividual , :Signing ;
        rdfs:comment      "Instance of an activity which is part of the creation process of ARTWORK_18_64."@en ;
        rdfs:label        "ARTWORK_18_64_Signing"@en ;
        :Followed-By      <http://www.semanticweb.org/ontologies/Daan/2020/BarbaraNanning#ARTWORK_18_64_ExaminingQuality(Result)> ;
        :Follows          :ARTWORK_18_64_Sandblasting ;
        :Has-Duration     <http://www.semanticweb.org/ontologies/Daan/2020/BarbaraNanning#2019> ;
        :Involves         :BarbaraNanning , :AlešZvěřina ;
        :Located-In       :NovyBor ;
        :Part-Of          :Creation_Artwork_18_64 ;
        :Requires-Use-Of  :AirCompressor .

[ a            owl:AllDisjointClasses ;
  owl:members  ( :Applying_Clear_Glass_Bell :Applying_Extra_Colour :Cooling :Documenting :Examining_the_Quality_of_the_Glass :Gilding :Glassblowing :Grinding :Heating :Measuring_and_Boxes_Making :Modeling :Packing :Photographing :Polishing :Preparing_Glass :Resting :Sandblasting :Sawing :Sensing :Setup_and_Testing_of_the_Metal_Mold :Transporting j.3: j.1: j.0: j.2: )
] .

<http://www.semanticweb.org/ontologies/Daan/2020/BarbaraNanning#JaapDeVries(NL)>
        a             owl:NamedIndividual , :Metal_Worker_4 ;
        rdfs:comment  "Jaap de Vries (NL) is a Metal Worker 4."@en ;
        rdfs:label    "Jaap de Vries (NL)"@en .

:Shown-By  a           owl:ObjectProperty ;
        rdfs:comment   "Shown-By is a property which connects an entity with a representation of the entity. This connection is made in the form of a Hyperlink."@en ;
        rdfs:domain    :Entity ;
        rdfs:label     "Shown-By"@en ;
        rdfs:range     :Representation ;
        owl:inverseOf  :Shows .

<http://www.semanticweb.org/ontologies/Daan/2020/BarbaraNanning#AbHylkema(NL)>
        a             owl:NamedIndividual , :Grinder_3 ;
        rdfs:comment  "Ab Hylkema (NL) is a Grinder 3."@en ;
        rdfs:label    "Ab Hylkema (NL)"@en ;
        :Involved-In  :ARTWORK_39_CuttingSheets , :ARTWORK_18_64_RoundingByGrindingTheSheet , :ARTWORK_18_64_CuttingSheets ;
        :Works-For    :GlassStudioVanTetterode .

<http://www.semanticweb.org/ontologies/Daan/2020/BarbaraNanning#ARTWORK_75_ExaminingQuality(CheckForIrregularitiesInTheGlass)>
        a              j.3: , owl:NamedIndividual ;
        rdfs:comment   "Instance of an activity which is part of the creation process of ARTWORK_75."@en ;
        rdfs:label     "ARTWORK_75_Examining Quality (Check for Irregularities in the Glass)"@en ;
        :Followed-By   :ARTWORK_75_Sawing ;
        :Follows       :ARTWORK_75_Resting ;
        :Has-Duration  <http://www.semanticweb.org/ontologies/Daan/2020/BarbaraNanning#2017> ;
        :Involves      :BarbaraNanning , :AlešZvěřina ;
        :Located-In    :CzechRepublic ;
        :Part-Of       :Creation_Artwork_75 .

:Ordering_Flat_Sheets
        a                owl:Class ;
        rdfs:comment     "Flat glass that can be cut into various shapes to create a specific design."@en ;
        rdfs:label       "Ordering Flat Sheets"@en ;
        rdfs:subClassOf  :Activity .

<http://vocab.getty.edu/aat/300024979>
        a                    owl:Class ;
        owl:equivalentClass  :Person .

:AJETOBlueGlass  a            owl:NamedIndividual , :AJETO_Glass ;
        rdfs:comment          "AJETO Blue is a form of AJETO glass with a blue colour."@en ;
        rdfs:label            "AJETO Blue Glass"@en ;
        :Availability         "Available"@en ;
        :Is-Processed-During  :ARTWORK_78_ApplyingExtraColour , :ARTWORK_79_ApplyingExtraColour_2 ;
        :Is-Processed-In      :Artwork_78 , :Artwork_79 ;
        :Made-By              :LASVITAJETO ;
        :Made-Out-Of          :Soda , :Potassium , :Calcium , :Sand ;
        :Transparency         "Transparent"@en .

:ARTWORK_73_Packing_2
        a              owl:NamedIndividual , :Packing ;
        rdfs:comment   "Instance of an activity which is part of the creation process of ARTWORK_73."@en ;
        rdfs:label     "ARTWORK_73_Packing_2"@en ;
        :Followed-By   :ARTWORK_73_Transporting_2 ;
        :Follows       :ARTWORK_73_MeasuringAndBoxesMaking ;
        :Has-Duration  <http://www.semanticweb.org/ontologies/Daan/2020/BarbaraNanning#2018> ;
        :Involves      :AlešZvěřina , :BarbaraNanning ;
        :Located-In    :CzechRepublic ;
        :Part-Of       :Creation_Artwork_73 .

:ARTWORK_17_33_PickingUpColouredCanesPattern
        a                 owl:NamedIndividual , :Picking_up_Coloured_Canes_Pattern ;
        rdfs:comment      "Instance of an activity which is part of the creation process of ARTWORK_17_33."@en ;
        rdfs:label        "ARTWORK_17_33_Picking up Coloured Canes Pattern"@en ;
        :Followed-By      :ARTWORK_17_33_Glassblowing ;
        :Follows          :ARTWORK_17_33_ApplyingClearGlassBell ;
        :Has-Duration     <http://www.semanticweb.org/ontologies/Daan/2020/BarbaraNanning#2017> ;
        :Involves         <http://www.semanticweb.org/ontologies/Daan/2020/BarbaraNanning#JiriMoravec(CZ)> , :AssistantOfBarbara , <http://www.semanticweb.org/ontologies/Daan/2020/BarbaraNanning#Tom%C3%A1%C5%A1Moravec(CZ)> , <http://www.semanticweb.org/ontologies/Daan/2020/BarbaraNanning#JessicaHomich(USA)> , <http://www.semanticweb.org/ontologies/Daan/2020/BarbaraNanning#RadekKoten(CZ)> , <http://www.semanticweb.org/ontologies/Daan/2020/BarbaraNanning#LukasHavlas(CZ)> , :BarbaraNanning ;
        :Located-In       :Lindava ;
        :Part-Of          :Creation_Artwork_17_33 ;
        :Requires-Use-Of  :Gloves , :StraightShears , :Pontis , :Furnace , :Beeswax , :Marver , :FusingKiln , :BlowingPipe , :AnnealingKiln , :PropaneTorch , :Paper , :Water , :DiamondShears , :GloryHole , :Hook , :Blocks , :GrindingWheel , :Jacks , :Garage , :Fork , :YokeOfSupport , :Tagliol , :AirCompressor .

<http://vocab.getty.edu/aat/300022860>
        a           owl:NamedIndividual ;
        owl:sameAs  :Marver .

<http://www.semanticweb.org/ontologies/Daan/2020/BarbaraNanning#ARTWORK_78_ExaminingQuality(Shape/Form)>
        a                 owl:NamedIndividual , j.2: ;
        rdfs:comment      "Instance of an activity which is part of the creation process of ARTWORK_78."@en ;
        rdfs:label        "ARTWORK_78_Examining Quality (Shape/Form)"@en ;
        :Followed-By      :ARTWORK_78_Translocating ;
        :Follows          :ARTWORK_78_Modeling ;
        :Has-Duration     <http://www.semanticweb.org/ontologies/Daan/2020/BarbaraNanning#2016> ;
        :Involves         :BarbaraNanning , <http://www.semanticweb.org/ontologies/Daan/2020/BarbaraNanning#AlesVacek(CZ)> , :LuděkKout ;
        :Located-In       :CzechRepublic ;
        :Part-Of          :Creation_Artwork_78 ;
        :Requires-Use-Of  :GloryHole , :Pontis , :BlowingPipe .

[ a            owl:AllDisjointClasses ;
  owl:members  ( :Grinder_1 :Grinder_2 :Grinder_3 :Grinder_4 )
] .

<http://vocab.getty.edu/aat/300023299>
        a           owl:NamedIndividual ;
        owl:sameAs  :SharpeningStone .

:ARTWORK_43_Modeling  a   :Modeling , owl:NamedIndividual ;
        rdfs:comment      "Instance of an activity which is part of the creation process of ARTWORK_43."@en ;
        rdfs:label        "ARTWORK_43_Modeling"@en ;
        :Followed-By      <http://www.semanticweb.org/ontologies/Daan/2020/BarbaraNanning#ARTWORK_43_ExaminingQuality(Shape/Form)> ;
        :Follows          :ARTWORK_43_Sensing ;
        :Has-Duration     <http://www.semanticweb.org/ontologies/Daan/2020/BarbaraNanning#2008> ;
        :Involves         :BarbaraNanning , <http://www.semanticweb.org/ontologies/Daan/2020/BarbaraNanning#RostislavMaterka(CZ)> , <http://www.semanticweb.org/ontologies/Daan/2020/BarbaraNanning#RobertHlavacek(CZ)> , <http://www.semanticweb.org/ontologies/Daan/2020/BarbaraNanning#RomanTomis(CZ)> , <http://www.semanticweb.org/ontologies/Daan/2020/BarbaraNanning#AlesVacek(CZ)> , :AssistantOfBarbara ;
        :Located-In       :CzechRepublic ;
        :Part-Of          :Creation_Artwork_43 ;
        :Requires-Use-Of  :BlowingPipe , :AirCompressor , :InterchangeableMetalMoldSetup , :Gloves , :PropaneTorch .

:ARTWORK_43_Packing_3
        a              :Packing , owl:NamedIndividual ;
        rdfs:comment   "Instance of an activity which is part of the creation process of ARTWORK_43."@en ;
        rdfs:label     "ARTWORK_43_Packing_3"@en ;
        :Followed-By   :ARTWORK_43_Transporting_3 ;
        :Follows       :ARTWORK_43_Signing ;
        :Has-Duration  <http://www.semanticweb.org/ontologies/Daan/2020/BarbaraNanning#2008> ;
        :Involves      :BarbaraNanning , :AlešZvěřina ;
        :Located-In    :CzechRepublic ;
        :Part-Of       :Creation_Artwork_43 .

:Modeling_with_Teflon_Stick
        a                owl:Class ;
        rdfs:comment     "When glass is hot it can be sculpted by a variety of materials. Teflon is one of them."@en ;
        rdfs:label       "Modeling with Teflon Stick"@en ;
        rdfs:subClassOf  :Modeling .

:ARTWORK_78_Sawing  a     :Sawing , owl:NamedIndividual ;
        rdfs:comment      "Instance of an activity which is part of the creation process of ARTWORK_78."@en ;
        rdfs:label        "ARTWORK_78_Sawing"@en ;
        :Followed-By      :ARTWORK_78_Grinding ;
        :Follows          <http://www.semanticweb.org/ontologies/Daan/2020/BarbaraNanning#ARTWORK_78_ExaminingQuality(CheckForIrregularitiesInTheGlass)> ;
        :Has-Duration     <http://www.semanticweb.org/ontologies/Daan/2020/BarbaraNanning#2008> ;
        :Involves         :BarbaraNanning , :AlešZvěřina ;
        :Located-In       :CzechRepublic ;
        :Part-Of          :Creation_Artwork_78 ;
        :Requires-Use-Of  :DiamondSaw .

:Grinder_2  a            owl:Class ;
        rdfs:comment     "A Grinder 2 is an actor who is the second member of a team responsible for the grinding, polishing and sharpening of objects."@en ;
        rdfs:label       "Grinder 2"@en ;
        rdfs:subClassOf  :Grinder .

:Glass_Studio  a         owl:Class ;
        rdfs:comment     "A glass studio is a studio were glass objects are manufactured."@en ;
        rdfs:label       "Glass Studio"@en ;
        rdfs:subClassOf  :Studio .

:Metal_Worker_4  a       owl:Class ;
        rdfs:comment     "A Metal Worker 4 is an actor who is the fourth member of a team responsible for creating metal objects or dealing with metal material."@en ;
        rdfs:label       "Metal Worker 4"@en ;
        rdfs:subClassOf  :Metal_Worker .

:Image_Artwork_17_33  a         :Digital_Image , owl:NamedIndividual ;
        rdfs:comment            "Image of Artwork_17_33 by Barbara Nanning."@en ;
        rdfs:label              "Image_Artwork_17_33"@en ;
        :Representation-Source  "Tom Haartsen_Ouderkerk A/d Amstel (NL)"@en ;
        :Shows                  :Artwork_17_33 .

:ARTWORK_39_Glassblowing
        a                 owl:NamedIndividual , :Glassblowing ;
        rdfs:comment      "Instance of an activity which is part of the creation process of ARTWORK_39."@en ;
        rdfs:label        "ARTWORK_39_Glassblowing"@en ;
        :Followed-By      :ARTWORK_39_Sensing ;
        :Follows          :ARTWORK_39_HeatingMetalMold ;
        :Has-Duration     <http://www.semanticweb.org/ontologies/Daan/2020/BarbaraNanning#2015> ;
        :Involves         <http://www.semanticweb.org/ontologies/Daan/2020/BarbaraNanning#MarekBrathko(CZ)> , :GertBullée , :BarbaraNanning , <http://www.semanticweb.org/ontologies/Daan/2020/BarbaraNanning#MiaLerssi(DN)> , <http://www.semanticweb.org/ontologies/Daan/2020/BarbaraNanning#RobertLenner(CZ)> , <http://www.semanticweb.org/ontologies/Daan/2020/BarbaraNanning#JessicaHomich(USA)> , <http://www.semanticweb.org/ontologies/Daan/2020/BarbaraNanning#MarekEffmert(CZ)> ;
        :Located-In       :Zaandam ;
        :Part-Of          :Creation_Artwork_39 ;
        :Requires-Use-Of  :YokeOfSupport , :BlowingPipe , :Tagliol , :InterchangeableMetalMoldSetup , :Gloves , :Paper , :DiamondShears , :BitIron , :IcePick , :Water , :AirCompressor , :Pontis , :Furnace , :Jacks , :Pincet , :Beeswax , :AnnealingKiln , :StraightShears , :Fork , :Blocks , :CeramicPotFilledWithGlass , :Hook , :Marver , :GloryHole , :PropaneTorch .

:ARTWORK_80_Grinding  a   owl:NamedIndividual , :Grinding ;
        rdfs:comment      "Instance of an activity which is part of the creation process of ARTWORK_80."@en ;
        rdfs:label        "ARTWORK_80_Grinding"@en ;
        :Followed-By      :ARTWORK_80_Polishing ;
        :Follows          :ARTWORK_80_Sawing ;
        :Has-Duration     <http://www.semanticweb.org/ontologies/Daan/2020/BarbaraNanning#2018> ;
        :Involves         :AlešZvěřina , :BarbaraNanning , :RobertFlorian ;
        :Located-In       :CzechRepublic ;
        :Part-Of          :Creation_Artwork_80 ;
        :Requires-Use-Of  :SharpeningStone , :GrindingWheel .

<http://www.cidoc-crm.org/cidoc-crm/P94_has_created>
        a                       owl:ObjectProperty ;
        owl:equivalentProperty  :Created .

:ARTWORK_17_33_Transporting
        a              :Transporting , owl:NamedIndividual ;
        rdfs:comment   "Instance of an activity which is part of the creation process of ARTWORK_17_33."@en ;
        rdfs:label     "ARTWORK_17_33_Transporting"@en ;
        :Followed-By   :ARTWORK_17_33_Resting ;
        :Follows       :ARTWORK_17_33_Packing ;
        :Has-Duration  <http://www.semanticweb.org/ontologies/Daan/2020/BarbaraNanning#2017> ;
        :Involves      :AlešZvěřina , :BarbaraNanning ;
        :Located-In    :NovyBor ;
        :Part-Of       :Creation_Artwork_17_33 .

:ARTWORK_75_ApplyingExtraColour
        a                 :Applying_Extra_Colour , owl:NamedIndividual ;
        rdfs:comment      "Instance of an activity which is part of the creation process of ARTWORK_75."@en ;
        rdfs:label        "ARTWORK_75_Applying Extra Colour"@en ;
        :Followed-By      :ARTWORK_75_ApplyingExtraColour_2 ;
        :Follows          :ARTWORK_75_ApplyingClearGlassBell ;
        :Has-Duration     <http://www.semanticweb.org/ontologies/Daan/2020/BarbaraNanning#2017> ;
        :Involves         <http://www.semanticweb.org/ontologies/Daan/2020/BarbaraNanning#RadekKoten(CZ)> , :BarbaraNanning , <http://www.semanticweb.org/ontologies/Daan/2020/BarbaraNanning#LukasHavlas(CZ)> ;
        :Located-In       :CzechRepublic ;
        :Part-Of          :Creation_Artwork_75 ;
        :Processes        <http://www.semanticweb.org/ontologies/Daan/2020/BarbaraNanning#ReichenbachColourRodsGlass(DE)> ;
        :Requires-Use-Of  :IcePick , :Water , :Paper , :GloryHole , :Pincet , :Marver , :CeramicPotFilledWithGlass , :Fork , :Blocks , :Garage , :Furnace , :Beeswax , :StraightShears , :Hook , :AnnealingKiln , :Pontis , :Tagliol , :YokeOfSupport , :Jacks , :BlowingPipe , :DiamondShears , :AirCompressor .

:Photographer  a         owl:Class ;
        rdfs:comment     "A Photographer is an actor who is responsible for making photographs."@en ;
        rdfs:label       "Photographer"@en ;
        rdfs:subClassOf  :Person .

:ARTWORK_39_Signing  a    owl:NamedIndividual , :Signing ;
        rdfs:comment      "Instance of an activity which is part of the creation process of ARTWORK_39."@en ;
        rdfs:label        "ARTWORK_39_Signing"@en ;
        :Followed-By      <http://www.semanticweb.org/ontologies/Daan/2020/BarbaraNanning#ARTWORK_39_ExaminingQuality(FinalResult)> ;
        :Follows          :ARTWORK_39_Sandblasting ;
        :Has-Duration     <http://www.semanticweb.org/ontologies/Daan/2020/BarbaraNanning#2015> ;
        :Involves         :BarbaraNanning , :AlešZvěřina ;
        :Located-In       :NovyBor ;
        :Part-Of          :Creation_Artwork_39 ;
        :Requires-Use-Of  :AirCompressor .

:ARTWORK_79_Sensing  a  :Sensing , owl:NamedIndividual ;
        rdfs:comment   "Instance of an activity which is part of the creation process of ARTWORK_79."@en ;
        rdfs:label     "ARTWORK_79_Sensing"@en ;
        :Followed-By   :ARTWORK_79_Modeling ;
        :Follows       :ARTWORK_79_Glassblowing ;
        :Has-Duration  <http://www.semanticweb.org/ontologies/Daan/2020/BarbaraNanning#2018> ;
        :Involves      :LukášSvoboda , :AlešZvěřina , :BarbaraNanning ;
        :Located-In    :CzechRepublic ;
        :Part-Of       :Creation_Artwork_79 .

:Shows  a             owl:ObjectProperty ;
        rdfs:comment  "Shows is a property which connects an entity with a representation of the entity. This connection is made in the form of a Hyperlink."@en ;
        rdfs:domain   :Representation ;
        rdfs:label    "Shows"@en ;
        rdfs:range    :Entity .

:ARTWORK_46_Signing  a    :Signing , owl:NamedIndividual ;
        rdfs:comment      "Instance of an activity which is part of the creation process of ARTWORK_46."@en ;
        rdfs:label        "ARTWORK_46_Signing"@en ;
        :Followed-By      <http://www.semanticweb.org/ontologies/Daan/2020/BarbaraNanning#ARTWORK_46_ExaminingQuality(Result)> ;
        :Follows          :ARTWORK_46_Polishing ;
        :Has-Duration     <http://www.semanticweb.org/ontologies/Daan/2020/BarbaraNanning#2018> ;
        :Involves         :AlešZvěřina , :BarbaraNanning ;
        :Located-In       :NovyBor ;
        :Part-Of          :Creation_Artwork_46 ;
        :Requires-Use-Of  :AirCompressor .

:AssistantOfBarbara  a  owl:NamedIndividual , :Fourth_Glass_Blower ;
        rdfs:comment  "Assistant of Barbara is a Fourth Glass Blower."@en ;
        rdfs:label    "Assistant of Barbara"@en ;
        :Involved-In  :ARTWORK_76_SetupAndTestingOfTheMetalMold , :ARTWORK_74_SetupAndTestingOfTheMetalMold_2 , :ARTWORK_73_Modeling , :ARTWORK_79_Cooling , :ARTWORK_73_SetupAndTestingOfTheMetalMold , :ARTWORK_73_Glassblowing , :ARTWORK_76_Modeling , :ARTWORK_43_Modeling , :ARTWORK_44_Cooling , :ARTWORK_77_SetupAndTestingOfTheMetalMold , :ARTWORK_78_Modeling , :ARTWORK_77_Glassblowing , :ARTWORK_78_Glassblowing , :ARTWORK_77_Cooling , :ARTWORK_76_Cooling , :ARTWORK_43_SetupAndTestingOfTheMetalMold , :ARTWORK_75_SetupAndTestingOfTheMetalMold_2 , :ARTWORK_44_SetupAndTestingOfTheMetalMold , :ARTWORK_75_SetupAndTestingOfTheMetalMold , :ARTWORK_79_Modeling , :ARTWORK_74_Modeling , :ARTWORK_78_SetupAndTestingOfTheMetalMold_2 , :ARTWORK_80_Glassblowing , :ARTWORK_74_SetupAndTestingOfTheMetalMold , :ARTWORK_73_Cooling , :ARTWORK_76_Glassblowing , :ARTWORK_76_SetupAndTestingOfTheMetalMold_2 , :ARTWORK_43_Gilding , :ARTWORK_78_Cooling , :ARTWORK_73_SetupAndTestingOfTheMetalMold_2 , :ARTWORK_43_Cooling , :ARTWORK_75_Glassblowing , :ARTWORK_80_SetupAndTestingOfTheMetalMold_2 , :ARTWORK_74_Cooling , :ARTWORK_75_Cooling , :ARTWORK_75_Modeling , :ARTWORK_79_Glassblowing , :ARTWORK_80_Cooling , :ARTWORK_77_SetupAndTestingOfTheMetalMold_2 , :ARTWORK_44_Glassblowing , :ARTWORK_43_Glassblowing , :ARTWORK_80_SetupAndTestingOfTheMetalMold , :ARTWORK_78_SetupAndTestingOfTheMetalMold , :ARTWORK_77_Modeling , :ARTWORK_80_Modeling , :ARTWORK_44_SetupAndTestingOfTheMetalMold_2 , :ARTWORK_79_SetupAndTestingOfTheMetalMold , :ARTWORK_44_Modeling , :ARTWORK_79_SetupAndTestingOfTheMetalMold_2 , :ARTWORK_74_Glassblowing , :ARTWORK_43_SetupAndTestingOfTheMetalMold_2 .

:ARTWORK_78_Photographing
        a              owl:NamedIndividual , :Photographing ;
        rdfs:comment   "Instance of an activity which is part of the creation process of ARTWORK_78."@en ;
        rdfs:label     "ARTWORK_78_Photographing"@en ;
        :Followed-By   :ARTWORK_78_Documenting ;
        :Follows       :ARTWORK_78_Transporting_4 ;
        :Has-Duration  <http://www.semanticweb.org/ontologies/Daan/2020/BarbaraNanning#2008> ;
        :Involves      <http://www.semanticweb.org/ontologies/Daan/2020/BarbaraNanning#TomHaartsen_Ouderkerka/dAmstel(NL)> , :BarbaraNanning ;
        :Located-In    :CzechRepublic ;
        :Part-Of       :Creation_Artwork_78 .

:ARTWORK_18_64_Sensing_2
        a              :Sensing , owl:NamedIndividual ;
        rdfs:comment   "Instance of an activity which is part of the creation process of ARTWORK_18_64."@en ;
        rdfs:label     "ARTWORK_18_64_Sensing_2"@en ;
        :Followed-By   :ARTWORK_18_64_Grinding ;
        :Follows       :ARTWORK_18_64_Sawing ;
        :Has-Duration  <http://www.semanticweb.org/ontologies/Daan/2020/BarbaraNanning#2015> ;
        :Involves      :BarbaraNanning , :AlešZvěřina , :LukášSvoboda ;
        :Located-In    :NovyBor ;
        :Part-Of       :Creation_Artwork_18_64 .

<http://www.semanticweb.org/ontologies/Daan/2020/BarbaraNanning#ARTWORK_36_ExaminingQuality(CheckForIrregularitiesInTheGlass)>
        a              j.3: , owl:NamedIndividual ;
        rdfs:comment   "Instance of an activity which is part of the creation process of ARTWORK_36."@en ;
        rdfs:label     "ARTWORK_36_Examining Quality (Check for Irregularities in the Glass)"@en ;
        :Followed-By   :ARTWORK_36_Sawing ;
        :Follows       :ARTWORK_36_Resting ;
        :Has-Duration  <http://www.semanticweb.org/ontologies/Daan/2020/BarbaraNanning#2015> ;
        :Involves      :BarbaraNanning , :AlešZvěřina ;
        :Located-In    :NovyBor ;
        :Part-Of       :Creation_Artwork_36 .

:Image_Artwork_75  a            :Digital_Image , owl:NamedIndividual ;
        rdfs:comment            "Image of an artwork by Barbara Nanning displayed in \"Barbara Nanning Eeuwige Beweging\" by Eliens (2019)."@en ;
        rdfs:label              "Image_Artwork_75"@en ;
        :Representation-Source  "Tom Haartsen_Ouderkerk a/d Amstel (NL)"@en ;
        :Shows                  :Artwork_75 .

:ARTWORK_39_CuttingStrings
        a                 :Cutting_Strings , owl:NamedIndividual ;
        rdfs:comment      "Instance of an activity which is part of the creation process of ARTWORK_39."@en ;
        rdfs:label        "ARTWORK_39_Cutting Strings"@en ;
        :Followed-By      :ARTWORK_39_ComposingColouredPatternsWithSheetsAndStrings ;
        :Follows          :ARTWORK_39_CuttingSheets ;
        :Has-Duration     <http://www.semanticweb.org/ontologies/Daan/2020/BarbaraNanning#2015> ;
        :Involves         :BarbaraNanning ;
        :Located-In       :Amsterdam ;
        :Part-Of          :Creation_Artwork_39 ;
        :Requires-Use-Of  :Glassscissors .

:ARTWORK_36_Modeling  a   :Modeling , owl:NamedIndividual ;
        rdfs:comment      "Instance of an activity which is part of the creation process of ARTWORK_36."@en ;
        rdfs:label        "ARTWORK_36_Modeling"@en ;
        :Followed-By      <http://www.semanticweb.org/ontologies/Daan/2020/BarbaraNanning#ARTWORK_36_ExaminingQuality(Shape/Form)> ;
        :Follows          :ARTWORK_36_Sensing ;
        :Has-Duration     <http://www.semanticweb.org/ontologies/Daan/2020/BarbaraNanning#2015> ;
        :Involves         :BarbaraNanning , <http://www.semanticweb.org/ontologies/Daan/2020/BarbaraNanning#MarekEffmert(CZ)> , <http://www.semanticweb.org/ontologies/Daan/2020/BarbaraNanning#JessicaHomich(USA)> , :GertBullée , <http://www.semanticweb.org/ontologies/Daan/2020/BarbaraNanning#RobertLenner(CZ)> , <http://www.semanticweb.org/ontologies/Daan/2020/BarbaraNanning#MarekBrathko(CZ)> ;
        :Located-In       :Zaandam ;
        :Part-Of          :Creation_Artwork_36 ;
        :Requires-Use-Of  :PropaneTorch , :BlowingPipe , :Gloves , :AirCompressor , :InterchangeableMetalMoldSetup .

:ARTWORK_79_Grinding  a   owl:NamedIndividual , :Grinding ;
        rdfs:comment      "Instance of an activity which is part of the creation process of ARTWORK_79."@en ;
        rdfs:label        "ARTWORK_79_Grinding"@en ;
        :Followed-By      :ARTWORK_79_Polishing ;
        :Follows          :ARTWORK_79_Sawing ;
        :Has-Duration     <http://www.semanticweb.org/ontologies/Daan/2020/BarbaraNanning#2018> ;
        :Involves         :BarbaraNanning , :RobertFlorian , :AlešZvěřina ;
        :Located-In       :CzechRepublic ;
        :Part-Of          :Creation_Artwork_79 ;
        :Requires-Use-Of  :SharpeningStone , :GrindingWheel .

<http://www.semanticweb.org/ontologies/Daan/2020/BarbaraNanning#ARTWORK_76_ExaminingQuality(CheckForIrregularitiesInTheGlass)_2>
        a              j.3: , owl:NamedIndividual ;
        rdfs:comment   "Instance of an activity which is part of the creation process of ARTWORK_76."@en ;
        rdfs:label     "ARTWORK_76_Examining Quality (Check for Irregularities in the Glass)_2"@en ;
        :Followed-By   :ARTWORK_76_MeasuringAndBoxesMaking ;
        :Follows       :ARTWORK_76_Polishing ;
        :Has-Duration  <http://www.semanticweb.org/ontologies/Daan/2020/BarbaraNanning#2018> ;
        :Involves      :AlešZvěřina , :BarbaraNanning ;
        :Located-In    :CzechRepublic ;
        :Part-Of       :Creation_Artwork_76 .

<http://www.cidoc-crm.org/cidoc-crm/P4_has_time-span>
        a                       owl:ObjectProperty ;
        owl:equivalentProperty  :Has-Duration .

<http://vocab.getty.edu/aat/300024841>
        a           owl:NamedIndividual ;
        owl:sameAs  :Tool .

:GlassStudioVanTetterode
        a             :Glass_Studio , owl:NamedIndividual ;
        rdfs:comment  "Glass Studio van Tetterode is a glass studio in Amsterdam."@en ;
        rdfs:label    "Glass Studio van Tetterode"@en ;
        :Employed     <http://www.semanticweb.org/ontologies/Daan/2020/BarbaraNanning#AbHylkema(NL)> , :GertBullée , <http://www.semanticweb.org/ontologies/Daan/2020/BarbaraNanning#JessicaHomich(USA)> , <http://www.semanticweb.org/ontologies/Daan/2020/BarbaraNanning#RichardPrice(NL)> , <http://www.semanticweb.org/ontologies/Daan/2020/BarbaraNanning#FredStikvoort(NL)> , <http://www.semanticweb.org/ontologies/Daan/2020/BarbaraNanning#PaulGroot(NL)> , <http://www.semanticweb.org/ontologies/Daan/2020/BarbaraNanning#MarekEffmert(CZ)> , <http://www.semanticweb.org/ontologies/Daan/2020/BarbaraNanning#RobertLenner(CZ)> ;
        :Located-In   :Amsterdam ;
        :Maker-Of     :Artwork_18_64 , :Artwork_39 .

:Image_Artwork_43  a            :Digital_Image , owl:NamedIndividual ;
        rdfs:comment            "Image of an artwork by Barbara Nanning displayed in \"Barbara Nanning Eeuwige Beweging\" by Eliens (2019)."@en ;
        rdfs:label              "Image_Artwork_43"@en ;
        :Representation-Source  "Tom Haartsen_Ouderkerk a/d Amstel (NL)"@en ;
        :Shows                  :Artwork_43 .

<http://www.semanticweb.org/ontologies/Daan/2020/BarbaraNanning#ARTWORK_77_ExaminingQuality(FinalResult)>
        a              owl:NamedIndividual , j.1: ;
        rdfs:comment   "Instance of an activity which is part of the creation process of ARTWORK_77."@en ;
        rdfs:label     "ARTWORK_77_Examining Quality (Final Result)"@en ;
        :Followed-By   :ARTWORK_77_Packing_5 ;
        :Follows       :ARTWORK_77_Gilding ;
        :Has-Duration  <http://www.semanticweb.org/ontologies/Daan/2020/BarbaraNanning#2018> ;
        :Involves      :AlešZvěřina , :BarbaraNanning ;
        :Located-In    :CzechRepublic ;
        :Part-Of       :Creation_Artwork_77 .

:ARTWORK_44_Transporting_3
        a              :Transporting , owl:NamedIndividual ;
        rdfs:comment   "Instance of an activity which is part of the creation process of ARTWORK_44."@en ;
        rdfs:label     "ARTWORK_44_Transporting_3"@en ;
        :Followed-By   :ARTWORK_44_Gilding ;
        :Follows       :ARTWORK_44_Packing_3 ;
        :Has-Duration  <http://www.semanticweb.org/ontologies/Daan/2020/BarbaraNanning#2018> ;
        :Involves      :AlešZvěřina , :BarbaraNanning ;
        :Located-In    :CzechRepublic ;
        :Part-Of       :Creation_Artwork_44 .

<http://www.semanticweb.org/ontologies/Daan/2020/BarbaraNanning#ARTWORK_73_ExaminingQuality(CheckForIrregularitiesInTheGlass)>
        a              j.3: , owl:NamedIndividual ;
        rdfs:comment   "Instance of an activity which is part of the creation process of ARTWORK_73."@en ;
        rdfs:label     "ARTWORK_73_Examining Quality (Check for Irregularities in the Glass)"@en ;
        :Followed-By   :ARTWORK_73_Sawing ;
        :Follows       :ARTWORK_73_Resting ;
        :Has-Duration  <http://www.semanticweb.org/ontologies/Daan/2020/BarbaraNanning#2018> ;
        :Involves      :BarbaraNanning , :AlešZvěřina ;
        :Located-In    :CzechRepublic ;
        :Part-Of       :Creation_Artwork_73 .

:ARTWORK_76_Resting  a    owl:NamedIndividual , :Resting ;
        rdfs:comment      "Instance of an activity which is part of the creation process of ARTWORK_76."@en ;
        rdfs:label        "ARTWORK_76_Resting"@en ;
        :Followed-By      <http://www.semanticweb.org/ontologies/Daan/2020/BarbaraNanning#ARTWORK_76_ExaminingQuality(CheckForIrregularitiesInTheGlass)> ;
        :Follows          :ARTWORK_76_Transporting ;
        :Has-Duration     <http://www.semanticweb.org/ontologies/Daan/2020/BarbaraNanning#2018> ;
        :Involves         :AlešZvěřina ;
        :Located-In       :CzechRepublic ;
        :Part-Of          :Creation_Artwork_76 ;
        :Requires-Use-Of  :AnnealingKiln .

<http://www.wikidata.org/entity/Q39>
        a       owl:NamedIndividual .

:ARTWORK_73_Transporting_4
        a              :Transporting , owl:NamedIndividual ;
        rdfs:comment   "Instance of an activity which is part of the creation process of ARTWORK_73."@en ;
        rdfs:label     "ARTWORK_73_Transporting_4"@en ;
        :Followed-By   :ARTWORK_73_Photographing ;
        :Follows       :ARTWORK_73_Packing_4 ;
        :Has-Duration  <http://www.semanticweb.org/ontologies/Daan/2020/BarbaraNanning#2018> ;
        :Involves      :BarbaraNanning , :AlešZvěřina ;
        :Located-In    :CzechRepublic ;
        :Part-Of       :Creation_Artwork_73 .

:Creation_Artwork_73  a  :Creation_Event , owl:NamedIndividual ;
        rdfs:comment    "Creation event for an artwork by Barbara Nanning displayed in \"Barbara Nanning Eeuwige Beweging\" by Eliens (2019)."@en ;
        rdfs:label      "Creation_Artwork_73"@en ;
        :Consists-Of    :ARTWORK_73_Polishing , :ARTWORK_73_Transporting , :ARTWORK_73_Packing_5 , :ARTWORK_73_Modeling , :ARTWORK_73_MeasuringAndBoxesMaking , :ARTWORK_73_HeatingMetalMold , :ARTWORK_73_Photographing , :ARTWORK_73_Sensing , :ARTWORK_73_Packing , <http://www.semanticweb.org/ontologies/Daan/2020/BarbaraNanning#ARTWORK_73_ExaminingQuality(Shape/Form)> , <http://www.semanticweb.org/ontologies/Daan/2020/BarbaraNanning#ARTWORK_73_ExaminingQuality(CheckForIrregularitiesInTheGlass)> , :ARTWORK_73_Grinding , :ARTWORK_73_Resting , <http://www.semanticweb.org/ontologies/Daan/2020/BarbaraNanning#ARTWORK_73_ExaminingQuality(Result)> , :ARTWORK_73_SetupAndTestingOfTheMetalMold_2 , :ARTWORK_73_Packing_3 , :ARTWORK_73_Packing_4 , :ARTWORK_73_Signing , :ARTWORK_73_SetupAndTestingOfTheMetalMold , :ARTWORK_73_PreparingGlass , :ARTWORK_73_Documenting , :ARTWORK_73_Translocating , :ARTWORK_73_Sawing , :ARTWORK_73_Packing_2 , :ARTWORK_73_Transporting_3 , :ARTWORK_73_Transporting_4 , :ARTWORK_73_Gilding , :ARTWORK_73_Cooling , :ARTWORK_73_ApplyingClearGlassBell , :ARTWORK_73_Sandblasting , <http://www.semanticweb.org/ontologies/Daan/2020/BarbaraNanning#ARTWORK_73_ExaminingQuality(FinalResult)> , :ARTWORK_73_Glassblowing ;
        :Created        :Artwork_73 ;
        :Finishes-With  :ARTWORK_73_Packing_5 ;
        :Has-Duration   <http://www.semanticweb.org/ontologies/Daan/2020/BarbaraNanning#2018> ;
        :Located-In     :CzechRepublic ;
        :Starts-With    :ARTWORK_73_PreparingGlass ;
        :Within-Period  :GlassVerreÉglomisé .

:ARTWORK_18_64_DecidingColourPaletteAndPatterns_3
        a              :Deciding_Colour_Palette_and_Patterns , owl:NamedIndividual ;
        rdfs:comment   "Instance of an activity which is part of the creation process of ARTWORK_18_64."@en ;
        rdfs:label     "ARTWORK_18_64_Deciding Colour Palette and Patterns_3"@en ;
        :Followed-By   :ARTWORK_18_64_CuttingSheets ;
        :Follows       :ARTWORK_18_64_TransportingColouredCanes_2 ;
        :Has-Duration  <http://www.semanticweb.org/ontologies/Daan/2020/BarbaraNanning#2015> ;
        :Involves      :BarbaraNanning ;
        :Located-In    :Amsterdam ;
        :Part-Of       :Creation_Artwork_18_64 .

:ARTWORK_18_64_PreparingForBlowing
        a                 owl:NamedIndividual , :Preparing_for_Blowing ;
        rdfs:comment      "Instance of an activity which is part of the creation process of ARTWORK_18_64."@en ;
        rdfs:label        "ARTWORK_18_64_Preparing for Blowing"@en ;
        :Followed-By      :ARTWORK_18_64_FillingKilnsWithMetalBowl ;
        :Follows          :ARTWORK_18_64_TransportingMetalBowlWithSheet ;
        :Has-Duration     <http://www.semanticweb.org/ontologies/Daan/2020/BarbaraNanning#2015> ;
        :Involves         <http://www.semanticweb.org/ontologies/Daan/2020/BarbaraNanning#JessicaHomich(USA)> , <http://www.semanticweb.org/ontologies/Daan/2020/BarbaraNanning#JiriPacinek(CZ)> , :BarbaraNanning ;
        :Located-In       :Lindava ;
        :Part-Of          :Creation_Artwork_18_64 ;
        :Requires-Use-Of  :Garage , :AnnealingKiln , :Furnace , :BlowingPipe , :Water , :FusingKiln , :Paper .

<http://www.wikidata.org/entity/Q12013202>
        a       owl:NamedIndividual .

:ARTWORK_39_Sensing_2
        a              owl:NamedIndividual , :Sensing ;
        rdfs:comment   "Instance of an activity which is part of the creation process of ARTWORK_39."@en ;
        rdfs:label     "ARTWORK_39_Sensing_2"@en ;
        :Followed-By   :ARTWORK_39_Grinding ;
        :Follows       :ARTWORK_39_Sawing ;
        :Has-Duration  <http://www.semanticweb.org/ontologies/Daan/2020/BarbaraNanning#2015> ;
        :Involves      :BarbaraNanning , :LukášSvoboda , :AlešZvěřina ;
        :Located-In    :NovyBor ;
        :Part-Of       :Creation_Artwork_39 .

:Marver  a            owl:NamedIndividual , :Equipment ;
        rdfs:comment  "A marver is a table used during glassblowing."@en ;
        rdfs:label    "Marver"@en ;
        :Used-For     :ARTWORK_79_Glassblowing , :ARTWORK_78_PreparingGlass , :ARTWORK_77_ApplyingClearGlassBell , :ARTWORK_74_ApplyingExtraColour_2 , :ARTWORK_77_Glassblowing , :ARTWORK_43_Glassblowing , :ARTWORK_80_PreparingGlass , :ARTWORK_79_ApplyingExtraColour , :ARTWORK_74_ApplyingExtraColour , :ARTWORK_76_Glassblowing , :ARTWORK_77_PreparingGlass , :ARTWORK_73_PreparingGlass , :ARTWORK_79_PreparingGlass , :ARTWORK_80_ApplyingClearGlassBell , :ARTWORK_74_ApplyingClearGlassBell , :ARTWORK_73_ApplyingClearGlassBell , :ARTWORK_43_ApplyingClearGlassBell , :ARTWORK_79_ApplyingClearGlassBell , :ARTWORK_76_ApplyingExtraColour_2 , :ARTWORK_76_ApplyingExtraColour , :ARTWORK_43_PreparingGlass , :ARTWORK_75_ApplyingClearGlassBell , :ARTWORK_76_ApplyingClearGlassBell , :ARTWORK_78_Glassblowing , :ARTWORK_73_Glassblowing , :ARTWORK_44_ApplyingExtraColour , :ARTWORK_44_ApplyingExtraColour_2 , :ARTWORK_79_ApplyingExtraColour_2 , :ARTWORK_44_Glassblowing , :ARTWORK_74_PreparingGlass , :ARTWORK_78_ApplyingExtraColour , :ARTWORK_75_Glassblowing , :ARTWORK_80_ApplyingExtraColour , :ARTWORK_77_ApplyingExtraColour , :ARTWORK_44_PreparingGlass , :ARTWORK_75_PreparingGlass , :ARTWORK_80_Glassblowing , :ARTWORK_75_ApplyingExtraColour_2 , :ARTWORK_43_ApplyingExtraColour , :ARTWORK_74_Glassblowing , :ARTWORK_78_ApplyingClearGlassBell , :ARTWORK_76_PreparingGlass , :ARTWORK_75_ApplyingExtraColour , :ARTWORK_44_ApplyingClearGlassBell .

:ARTWORK_75_Sawing  a     owl:NamedIndividual , :Sawing ;
        rdfs:comment      "Instance of an activity which is part of the creation process of ARTWORK_75."@en ;
        rdfs:label        "ARTWORK_75_Sawing"@en ;
        :Followed-By      :ARTWORK_75_Grinding ;
        :Follows          <http://www.semanticweb.org/ontologies/Daan/2020/BarbaraNanning#ARTWORK_75_ExaminingQuality(CheckForIrregularitiesInTheGlass)> ;
        :Has-Duration     <http://www.semanticweb.org/ontologies/Daan/2020/BarbaraNanning#2018> ;
        :Involves         :AlešZvěřina , :BarbaraNanning ;
        :Located-In       :CzechRepublic ;
        :Part-Of          :Creation_Artwork_75 ;
        :Requires-Use-Of  :DiamondSaw .

:ARTWORK_76_Packing_4
        a              owl:NamedIndividual , :Packing ;
        rdfs:comment   "Instance of an activity which is part of the creation process of ARTWORK_76."@en ;
        rdfs:label     "ARTWORK_76_Packing_4"@en ;
        :Followed-By   :ARTWORK_76_Transporting_4 ;
        :Follows       <http://www.semanticweb.org/ontologies/Daan/2020/BarbaraNanning#ARTWORK_76_ExaminingQuality(FinalResult)> ;
        :Has-Duration  <http://www.semanticweb.org/ontologies/Daan/2020/BarbaraNanning#2018> ;
        :Involves      :AlešZvěřina , :VáçlavNovák_Doksy_CzechRepublic , :BarbaraNanning ;
        :Located-In    :CzechRepublic ;
        :Part-Of       :Creation_Artwork_76 .

:ARTWORK_39_Sawing  a     owl:NamedIndividual , :Sawing ;
        rdfs:comment      "Instance of an activity which is part of the creation process of ARTWORK_39."@en ;
        rdfs:label        "ARTWORK_39_Sawing"@en ;
        :Followed-By      :ARTWORK_39_Sensing_2 ;
        :Follows          <http://www.semanticweb.org/ontologies/Daan/2020/BarbaraNanning#ARTWORK_39_ExaminingQuality(CheckForIrregularitiesInTheGlass)> ;
        :Has-Duration     <http://www.semanticweb.org/ontologies/Daan/2020/BarbaraNanning#2015> ;
        :Involves         :AlešZvěřina , :BarbaraNanning ;
        :Located-In       :NovyBor ;
        :Part-Of          :Creation_Artwork_39 ;
        :Requires-Use-Of  :DiamondSaw .

:Located-In  a         owl:ObjectProperty ;
        rdfs:comment   "Located-In is a property of a location, thing, organisation or event connecting it to a specific location."@en ;
        rdfs:domain    :Thing , :Place , :Organisation , :Event ;
        rdfs:label     "Located-In"@en ;
        rdfs:range     :Place ;
        owl:inverseOf  :Location-Of .

:Ceramic  a               :Man-Made_Material , owl:NamedIndividual ;
        rdfs:comment      "Ceramic is a hardened material made of clay."@en ;
        rdfs:label        "Ceramic"@en ;
        owl:sameAs        <http://www.wikidata.org/entity/Q45621> ;
        :Is-Processed-In  :CeramicPotFilledWithGlass .

:ARTWORK_36_Packing_5
        a              :Packing , owl:NamedIndividual ;
        rdfs:comment   "Instance of an activity which is part of the creation process of ARTWORK_36."@en ;
        rdfs:label     "ARTWORK_36_Packing_5"@en ;
        :Followed-By   :ARTWORK_36_Transporting_4 ;
        :Follows       :ARTWORK_36_Cooling_2 ;
        :Has-Duration  <http://www.semanticweb.org/ontologies/Daan/2020/BarbaraNanning#2019> ;
        :Involves      :BarbaraNanning ;
        :Located-In    :Lindava ;
        :Part-Of       :Creation_Artwork_36 .

:ARTWORK_75_Cooling  a    :Cooling , owl:NamedIndividual ;
        rdfs:comment      "Instance of an activity which is part of the creation process of ARTWORK_75."@en ;
        rdfs:label        "ARTWORK_75_Cooling"@en ;
        :Followed-By      :ARTWORK_75_Packing ;
        :Follows          :ARTWORK_75_Translocating ;
        :Has-Duration     <http://www.semanticweb.org/ontologies/Daan/2020/BarbaraNanning#2017> ;
        :Involves         :LuděkKout , :AssistantOfBarbara ;
        :Located-In       :CzechRepublic ;
        :Part-Of          :Creation_Artwork_75 ;
        :Requires-Use-Of  :AnnealingKiln .

<BarbaraNanning/VladimirZilaSr.>
        a             :Grinder_1 , owl:NamedIndividual ;
        rdfs:comment  "Vladimir Zila Sr. is a Grinder 1."@en ;
        rdfs:label    "Vladimir Zila Sr."@en .

<http://www.semanticweb.org/ontologies/Daan/2020/BarbaraNanning#ARTWORK_46_ExaminingQuality(Shape/Form)>
        a                 j.2: , owl:NamedIndividual ;
        rdfs:comment      "Instance of an activity which is part of the creation process of ARTWORK_46."@en ;
        rdfs:label        "ARTWORK_46_ARTWORK_46_Examining Quality (Shape/Form)"@en ;
        :Followed-By      :ARTWORK_46_Cooling ;
        :Follows          :ARTWORK_46_Modeling ;
        :Has-Duration     <http://www.semanticweb.org/ontologies/Daan/2020/BarbaraNanning#2018> ;
        :Involves         :BarbaraNanning , <http://www.semanticweb.org/ontologies/Daan/2020/BarbaraNanning#JiriPacinek(CZ)> , <http://www.semanticweb.org/ontologies/Daan/2020/BarbaraNanning#JessicaHomich(USA)> ;
        :Located-In       :Lindava ;
        :Part-Of          :Creation_Artwork_46 ;
        :Requires-Use-Of  :PropaneTorch , :Gloves , :BlowingPipe , :AirCompressor , :Pontis , :GloryHole , :InterchangeableMetalMoldSetup .

:Artwork_75  a        :Glass_Artwork , owl:NamedIndividual ;
        rdfs:comment  "Artwork by Barbara Nanning displayed in \"Barbara Nanning Eeuwige Beweging\" by Eliens (2019)."@en ;
        rdfs:label    "Verre églomisé (Alexandrite Glass)"@en ;
        :Created-By   :Creation_Artwork_75 ;
        :Has-Depth    "32"^^xsd:decimal ;
        :Has-Height   "22"^^xsd:decimal ;
        :Has-Width    "34"^^xsd:decimal ;
        :Is-Unica     "Yes"@en ;
        :Located-In   :Amsterdam ;
        :Made-By      :LASVITAJETO , :BarbaraNanning , :VáçlavNovák_Doksy_CzechRepublic , <http://www.semanticweb.org/ontologies/Daan/2020/BarbaraNanning#Ale%C5%A1Zv%C4%9B%C5%99ina&AZ-Design> ;
        :Made-Out-Of  :PureDucat , :AJETOAlexandriteGlass , <http://www.semanticweb.org/ontologies/Daan/2020/BarbaraNanning#ReichenbachColourRodsGlass(DE)> , :AJETOClearGlass ;
        :Part-Of      :CollectionOfBarbaraNanning ;
        :Shown-By     :Image_Artwork_75 .

:Glass_Artwork  a        owl:Class ;
        rdfs:comment     "A glass artwork is an artistic work created using (among other things) glass."@en ;
        rdfs:label       "Glass Artwork"@en ;
        rdfs:subClassOf  :Artwork .

:AJETOUraniumGlass  a  :AJETO_Glass , owl:NamedIndividual ;
        rdfs:comment   "AJETO Uranium glass is a material which changes colour under UV-lighting conditions."@en ;
        rdfs:label     "AJETO Uranium Glass"@en ;
        :Availability  "Orderable"@en ;
        :Made-By       :LASVITAJETO ;
        :Transparency  "Transparent"@en .

:ARTWORK_78_ApplyingExtraColour
        a                 owl:NamedIndividual , :Applying_Extra_Colour ;
        rdfs:comment      "Instance of an activity which is part of the creation process of ARTWORK_78."@en ;
        rdfs:label        "ARTWORK_78_Applying Extra Colour"@en ;
        :Followed-By      :ARTWORK_78_HeatingMetalMold ;
        :Follows          :ARTWORK_78_ApplyingClearGlassBell ;
        :Has-Duration     <http://www.semanticweb.org/ontologies/Daan/2020/BarbaraNanning#2016> ;
        :Involves         <http://www.semanticweb.org/ontologies/Daan/2020/BarbaraNanning#AlesVacek(CZ)> , <http://www.semanticweb.org/ontologies/Daan/2020/BarbaraNanning#RostislavMaterka(CZ)> , :BarbaraNanning ;
        :Located-In       :CzechRepublic ;
        :Part-Of          :Creation_Artwork_78 ;
        :Processes        :AJETOBlueGlass ;
        :Requires-Use-Of  :GloryHole , :Pontis , :IcePick , :AnnealingKiln , :Jacks , :Fork , :Furnace , :DiamondShears , :Paper , :YokeOfSupport , :Water , :CeramicPotFilledWithGlass , :Marver , :Garage , :StraightShears , :AirCompressor , :Blocks , :Tagliol , :BlowingPipe , :Hook , :Pincet , :Beeswax .

:ARTWORK_76_ExaminingTheQualityOfTheGlass
        a                 owl:NamedIndividual , :Examining_the_Quality_of_the_Glass ;
        rdfs:comment      "Instance of an activity which is part of the creation process of ARTWORK_76."@en ;
        rdfs:label        "ARTWORK_76_Examining the Quality of the Glass"@en ;
        :Followed-By      :ARTWORK_76_Cooling ;
        :Follows          :ARTWORK_76_Modeling ;
        :Has-Duration     <http://www.semanticweb.org/ontologies/Daan/2020/BarbaraNanning#2018> ;
        :Involves         :BarbaraNanning , :LuděkKout , <http://www.semanticweb.org/ontologies/Daan/2020/BarbaraNanning#RadekKoten(CZ)> ;
        :Located-In       :CzechRepublic ;
        :Part-Of          :Creation_Artwork_76 ;
        :Requires-Use-Of  :BlowingPipe , :Jacks , :Water , :Furnace , :StraightShears , :CeramicPotFilledWithGlass , :Pontis , :AnnealingKiln , :DiamondShears , :YokeOfSupport , :Paper , :Blocks , :GloryHole .

:ARTWORK_36_FillingKilnsWithMetalBowl
        a                 owl:NamedIndividual , :Filling_Kilns_with_Metal_Bowl ;
        rdfs:comment      "Instance of an activity which is part of the creation process of ARTWORK_36."@en ;
        rdfs:label        "ARTWORK_36_Filling Kilns with Metal Bowl"@en ;
        :Followed-By      :ARTWORK_36_PreparingGlass ;
        :Follows          :ARTWORK_36_PreparingForBlowing ;
        :Has-Duration     <http://www.semanticweb.org/ontologies/Daan/2020/BarbaraNanning#2015> ;
        :Involves         :DurkValkema , :BarbaraNanning ;
        :Located-In       :Zaandam ;
        :Part-Of          :Creation_Artwork_36 ;
        :Requires-Use-Of  :FusingKiln , :Gloves , :Garage .

<http://www.semanticweb.org/ontologies/Daan/2020/BarbaraNanning#RadekKoten(CZ)>
        a             owl:NamedIndividual , :Master_Glass_Blower ;
        rdfs:comment  "Radek Koten (CZ) is a Master Glass Blower."@en ;
        rdfs:label    "Radek Koten (CZ)"@en ;
        :Involved-In  :ARTWORK_44_ApplyingExtraColour_2 , :ARTWORK_44_PreparingGlass , :ARTWORK_44_Sensing , <http://www.semanticweb.org/ontologies/Daan/2020/BarbaraNanning#ARTWORK_77_ExaminingQuality(Shape/Form)> , :ARTWORK_79_ApplyingExtraColour_2 , :ARTWORK_73_Sensing , :ARTWORK_79_ExaminingTheQualityOfTheGlass , :ARTWORK_73_Glassblowing , :ARTWORK_44_Glassblowing , :ARTWORK_75_SetupAndTestingOfTheMetalMold_2 , :ARTWORK_77_SetupAndTestingOfTheMetalMold , :ARTWORK_77_Modeling , :ARTWORK_75_ApplyingClearGlassBell , :ARTWORK_73_SetupAndTestingOfTheMetalMold_2 , <http://www.semanticweb.org/ontologies/Daan/2020/BarbaraNanning#ARTWORK_75_ExaminingQuality(Shape/Form)> , :ARTWORK_80_ApplyingExtraColour , :ARTWORK_44_ApplyingClearGlassBell , :ARTWORK_75_ExaminingTheQualityOfTheGlass , :ARTWORK_75_Sensing , :ARTWORK_80_PreparingGlass , :ARTWORK_77_PreparingGlass , :ARTWORK_75_ApplyingExtraColour , :ARTWORK_75_Modeling , :ARTWORK_77_Glassblowing , :ARTWORK_73_PreparingGlass , :ARTWORK_76_ExaminingTheQualityOfTheGlass , :ARTWORK_77_SetupAndTestingOfTheMetalMold_2 , :ARTWORK_79_PreparingGlass , <http://www.semanticweb.org/ontologies/Daan/2020/BarbaraNanning#ARTWORK_73_ExaminingQuality(Shape/Form)> , :ARTWORK_80_ApplyingClearGlassBell , :ARTWORK_80_Sensing , :ARTWORK_76_ApplyingExtraColour_2 , :ARTWORK_44_SetupAndTestingOfTheMetalMold_2 , :ARTWORK_79_Modeling , :ARTWORK_44_ApplyingExtraColour , :ARTWORK_75_PreparingGlass , :ARTWORK_76_ApplyingExtraColour , :ARTWORK_79_Sensing , <http://www.semanticweb.org/ontologies/Daan/2020/BarbaraNanning#ARTWORK_44_ExaminingQuality(Shape/Form)> , :ARTWORK_44_ExaminingTheQualityOfTheGlass , <http://www.semanticweb.org/ontologies/Daan/2020/BarbaraNanning#ARTWORK_79_ExaminingQuality(Shape/Form)> , :ARTWORK_79_ApplyingClearGlassBell , :ARTWORK_76_Glassblowing , :ARTWORK_80_Modeling , :ARTWORK_79_SetupAndTestingOfTheMetalMold , :ARTWORK_76_Sensing , :ARTWORK_80_SetupAndTestingOfTheMetalMold , :ARTWORK_44_SetupAndTestingOfTheMetalMold , :ARTWORK_79_SetupAndTestingOfTheMetalMold_2 , :ARTWORK_79_ApplyingExtraColour , :ARTWORK_80_Glassblowing , :ARTWORK_75_Glassblowing , :ARTWORK_77_ApplyingExtraColour , :ARTWORK_73_Modeling , :ARTWORK_76_SetupAndTestingOfTheMetalMold , :ARTWORK_77_Sensing , :ARTWORK_76_ApplyingClearGlassBell , :ARTWORK_76_Modeling , :ARTWORK_76_SetupAndTestingOfTheMetalMold_2 , :ARTWORK_73_ApplyingClearGlassBell , :ARTWORK_44_Modeling , :ARTWORK_75_ApplyingExtraColour_2 , :ARTWORK_76_PreparingGlass , :ARTWORK_73_SetupAndTestingOfTheMetalMold , :ARTWORK_77_ApplyingClearGlassBell , :ARTWORK_79_Glassblowing , :ARTWORK_80_SetupAndTestingOfTheMetalMold_2 , <http://www.semanticweb.org/ontologies/Daan/2020/BarbaraNanning#ARTWORK_76_ExaminingQuality(Shape/Form)> , :ARTWORK_80_ExaminingTheQualityOfTheGlass , :ARTWORK_75_SetupAndTestingOfTheMetalMold , :ARTWORK_77_ExaminingTheQualityOfTheGlass , <http://www.semanticweb.org/ontologies/Daan/2020/BarbaraNanning#ARTWORK_80_ExaminingQuality(Shape/Form)> ;
        :Works-For    :LASVITAJETO .

:Artwork_43  a        :Glass_Artwork , owl:NamedIndividual ;
        rdfs:comment  "Artwork by Barbara Nanning displayed in \"Barbara Nanning Eeuwige Beweging\" by Eliens (2019)."@en ;
        rdfs:label    "Verre églomisé"@en ;
        :Created-By   :Creation_Artwork_43 ;
        :Has-Depth    "36"^^xsd:decimal ;
        :Has-Height   "31"^^xsd:decimal ;
        :Has-Width    "28"^^xsd:decimal ;
        :Is-Unica     "Yes"@en ;
        :Located-In   :Coesfeld ;
        :Made-By      :BarbaraNanning , <http://www.semanticweb.org/ontologies/Daan/2020/BarbaraNanning#Ale%C5%A1Zv%C4%9B%C5%99ina&AZ-Design> , :VáçlavNovák_Doksy_CzechRepublic , :LASVITAJETO ;
        :Made-Out-Of  :AJETOClearGlass , <http://www.semanticweb.org/ontologies/Daan/2020/BarbaraNanning#ReichenbachColourRodsGlass(DE)> , :Platinum ;
        :Part-Of      :CollectionGlasmuseumLette ;
        :Shown-By     :Image_Artwork_43 .

:ARTWORK_46_Glassblowing
        a                 owl:NamedIndividual , :Glassblowing ;
        rdfs:comment      "Instance of an activity which is part of the creation process of ARTWORK_46."@en ;
        rdfs:label        "ARTWORK_46_Glassblowing"@en ;
        :Followed-By      :ARTWORK_46_Sensing ;
        :Follows          :ARTWORK_46_HeatingMetalMold ;
        :Has-Duration     <http://www.semanticweb.org/ontologies/Daan/2020/BarbaraNanning#2018> ;
        :Involves         <http://www.semanticweb.org/ontologies/Daan/2020/BarbaraNanning#JiriPacinek(CZ)> , :BarbaraNanning , :DavidČerný , <http://www.semanticweb.org/ontologies/Daan/2020/BarbaraNanning#JessicaHomich(USA)> , :JiříPačinekJunior , :JaroslavKubásek , :JanBaštýř ;
        :Located-In       :Lindava ;
        :Part-Of          :Creation_Artwork_46 ;
        :Requires-Use-Of  :YokeOfSupport , :Pontis , :Tagliol , :DiamondShears , :GloryHole , :Marver , :AirCompressor , :Furnace , :AnnealingKiln , :Blocks , :StraightShears , :Beeswax , :Pincet , :BlowingPipe , :Paper , :BitIron , :InterchangeableMetalMoldSetup , :Hook , :Fork , :PropaneTorch , :Water , :CeramicPotFilledWithGlass , :Gloves , :IcePick , :Jacks .

:ARTWORK_75_Resting  a    owl:NamedIndividual , :Resting ;
        rdfs:comment      "Instance of an activity which is part of the creation process of ARTWORK_75."@en ;
        rdfs:label        "ARTWORK_75_Resting"@en ;
        :Followed-By      <http://www.semanticweb.org/ontologies/Daan/2020/BarbaraNanning#ARTWORK_75_ExaminingQuality(CheckForIrregularitiesInTheGlass)> ;
        :Follows          :ARTWORK_75_Transporting ;
        :Has-Duration     <http://www.semanticweb.org/ontologies/Daan/2020/BarbaraNanning#2018> ;
        :Involves         :AlešZvěřina ;
        :Located-In       :CzechRepublic ;
        :Part-Of          :Creation_Artwork_75 ;
        :Requires-Use-Of  :AnnealingKiln .

<http://www.semanticweb.org/ontologies/Daan/2020/BarbaraNanning#ARTWORK_36_ExaminingQuality(Shape/Form)>
        a                 j.2: , owl:NamedIndividual ;
        rdfs:comment      "Instance of an activity which is part of the creation process of ARTWORK_36."@en ;
        rdfs:label        "ARTWORK_36_Examining Quality (Shape/Form)"@en ;
        :Followed-By      :ARTWORK_36_Cooling ;
        :Follows          :ARTWORK_36_Modeling ;
        :Has-Duration     <http://www.semanticweb.org/ontologies/Daan/2020/BarbaraNanning#2015> ;
        :Involves         <http://www.semanticweb.org/ontologies/Daan/2020/BarbaraNanning#MiaLerssi(DN)> , :DurkValkema , :BarbaraNanning , :GertBullée ;
        :Located-In       :Zaandam ;
        :Part-Of          :Creation_Artwork_36 ;
        :Requires-Use-Of  :BlowingPipe , :InterchangeableMetalMoldSetup , :Gloves , :Pontis , :GloryHole , :PropaneTorch , :AirCompressor .

:ARTWORK_46_PickingUpColouredCanesPattern
        a                 owl:NamedIndividual , :Picking_up_Coloured_Canes_Pattern ;
        rdfs:comment      "Instance of an activity which is part of the creation process of ARTWORK_46."@en ;
        rdfs:label        "ARTWORK_46_Picking up Coloured Canes Pattern"@en ;
        :Followed-By      :ARTWORK_46_ApplyingClearOverlay ;
        :Follows          :ARTWORK_46_ApplyingClearGlassBell ;
        :Has-Duration     <http://www.semanticweb.org/ontologies/Daan/2020/BarbaraNanning#2018> ;
        :Involves         :BarbaraNanning , :JiříPačinekJunior , <http://www.semanticweb.org/ontologies/Daan/2020/BarbaraNanning#JessicaHomich(USA)> , <http://www.semanticweb.org/ontologies/Daan/2020/BarbaraNanning#JiriPacinek(CZ)> , :JanBaštýř , :JaroslavKubásek , :DavidČerný ;
        :Located-In       :Lindava ;
        :Part-Of          :Creation_Artwork_46 ;
        :Requires-Use-Of  :Hook , :Water , :Pontis , :Garage , :Gloves , :StraightShears , :FusingKiln , :DiamondShears , :Tagliol , :YokeOfSupport , :Jacks , :GloryHole , :PropaneTorch , :AirCompressor , :Blocks , :BlowingPipe , :Furnace , :Fork , :Paper , :Marver , :Beeswax , :AnnealingKiln , :GrindingWheel .

:ARTWORK_17_33_Documenting
        a              owl:NamedIndividual , :Documenting ;
        rdfs:comment   "Instance of an activity which is part of the creation process of ARTWORK_17_33."@en ;
        rdfs:label     "ARTWORK_17_33_Documenting"@en ;
        :Finishes      :Creation_Artwork_17_33 ;
        :Follows       :ARTWORK_17_33_Packing_3 ;
        :Has-Duration  <http://www.semanticweb.org/ontologies/Daan/2020/BarbaraNanning#2017> ;
        :Involves      :BarbaraNanning ;
        :Located-In    :Amsterdam ;
        :Part-Of       :Creation_Artwork_17_33 .

<http://www.cidoc-crm.org/cidoc-crm/P4_is_time-span_of>
        a                       owl:ObjectProperty ;
        owl:equivalentProperty  :Duration-Of .

:ARTWORK_44_Modeling  a   :Modeling , owl:NamedIndividual ;
        rdfs:comment      "Instance of an activity which is part of the creation process of ARTWORK_44."@en ;
        rdfs:label        "ARTWORK_44_Modeling"@en ;
        :Followed-By      <http://www.semanticweb.org/ontologies/Daan/2020/BarbaraNanning#ARTWORK_44_ExaminingQuality(Shape/Form)> ;
        :Follows          :ARTWORK_44_Sensing ;
        :Has-Duration     <http://www.semanticweb.org/ontologies/Daan/2020/BarbaraNanning#2018> ;
        :Involves         :BarbaraNanning , <http://www.semanticweb.org/ontologies/Daan/2020/BarbaraNanning#Tom%C3%A1%C5%A1Moravec(CZ)> , :AssistantOfBarbara , <http://www.semanticweb.org/ontologies/Daan/2020/BarbaraNanning#JiriMoravec(CZ)> , <http://www.semanticweb.org/ontologies/Daan/2020/BarbaraNanning#LukasHavlas(CZ)> , <http://www.semanticweb.org/ontologies/Daan/2020/BarbaraNanning#RadekKoten(CZ)> ;
        :Located-In       :CzechRepublic ;
        :Part-Of          :Creation_Artwork_44 ;
        :Requires-Use-Of  :PropaneTorch , :Gloves , :AirCompressor , :InterchangeableMetalMoldSetup , :BlowingPipe .

<http://www.semanticweb.org/ontologies/Daan/2020/BarbaraNanning#2015>
        a             :Timespan , owl:NamedIndividual ;
        rdfs:comment  "2015 is a Timespan."@en ;
        rdfs:label    "2015"@en ;
        owl:sameAs    <http://www.wikidata.org/entity/Q2002> ;
        :Duration-Of  :ARTWORK_36_SetupAndTestingOfTheMetalMold , :ARTWORK_36_TransportingColouredCanes_2 , :ARTWORK_36_TransportingMonochromeRods , :ARTWORK_46_ProducingColouredCanes , :ARTWORK_36_Casting , :ARTWORK_36_DecidingColourPaletteAndPatterns_2 , :ARTWORK_36_PreparingForBlowing , :ARTWORK_36_TransportingMetalBowlWithCanes , :ARTWORK_36_TackfusingColouredCanes , :ARTWORK_46_TransportingColouredCanes_2 , :ARTWORK_36_ProducingColouredCanes , :ARTWORK_36_PreparingGlass , :ARTWORK_36_Resting , :ARTWORK_36_HeatingMetalMold , :ARTWORK_36_DecidingColourPaletteAndPatterns , :ARTWORK_36_Ordening , :ARTWORK_46_CuttingAndPolishingColouredCanes , :ARTWORK_36_DecidingColourPalette , :ARTWORK_36_Sensing , :ARTWORK_46_DecidingColourPaletteAndPatterns , :ARTWORK_46_TransportingColouredCanes , :ARTWORK_36_CuttingMonochromeSheets , :ARTWORK_36_TransportingColouredCanes , :ARTWORK_46_TransportingMonochromeRods , :ARTWORK_36_Packing , :ARTWORK_36_MakingPatternsWithColouredCanesInTheMetalBowl , :ARTWORK_36_Modeling , :ARTWORK_36_MeasuringAndBoxesMaking , :ARTWORK_36_CuttingAndPolishingCastedMonochromeSheetsToSmallRods , <http://www.semanticweb.org/ontologies/Daan/2020/BarbaraNanning#ARTWORK_36_ExaminingQuality(Result)> , :ARTWORK_36_Glassblowing , :ARTWORK_36_Polishing , :ARTWORK_36_Sandblasting , :ARTWORK_36_Transporting_2 , :ARTWORK_46_DecidingColourPaletteAndPatterns_2 , :ARTWORK_36_Grinding , <http://www.semanticweb.org/ontologies/Daan/2020/BarbaraNanning#ARTWORK_36_ExaminingQuality(CheckForIrregularitiesInTheGlass)> , :ARTWORK_36_Cooling , :ARTWORK_46_Casting , :ARTWORK_36_CuttingAndPolishingColouredCanes , :ARTWORK_36_Sensing_2 , :ARTWORK_36_Transporting , :ARTWORK_46_Ordening , :ARTWORK_46_CuttingMonochromeSheets , :ARTWORK_36_ExaminingTheQualityOfTheGlass , :ARTWORK_36_FillingKilnsWithMetalBowl , <http://www.semanticweb.org/ontologies/Daan/2020/BarbaraNanning#ARTWORK_36_ExaminingQuality(Shape/Form)> , :ARTWORK_36_PickingUpColouredCanesPattern , :ARTWORK_46_CuttingAndPolishingCastedMonochromeSheetsToSmallRods , :ARTWORK_36_Sawing , :ARTWORK_36_ApplyingClearGlassBell , :ARTWORK_36_Packing_2 .

:ARTWORK_43_HeatingMetalMold
        a                 owl:NamedIndividual , :Heating_Metal_Mold ;
        rdfs:comment      "Instance of an activity which is part of the creation process of ARTWORK_43."@en ;
        rdfs:label        "ARTWORK_43_Heating Metal Mold"@en ;
        :Followed-By      :ARTWORK_43_Glassblowing ;
        :Follows          :ARTWORK_43_ApplyingExtraColour ;
        :Has-Duration     <http://www.semanticweb.org/ontologies/Daan/2020/BarbaraNanning#2008> ;
        :Involves         :BarbaraNanning ;
        :Located-In       :CzechRepublic ;
        :Part-Of          :Creation_Artwork_43 ;
        :Requires-Use-Of  :Gloves , :PropaneTorch , :InterchangeableMetalMoldSetup .

:ARTWORK_43_Sandblasting
        a                 :Sandblasting , owl:NamedIndividual ;
        rdfs:comment      "Instance of an activity which is part of the creation process of ARTWORK_43."@en ;
        rdfs:label        "ARTWORK_43_Sandblasting"@en ;
        :Followed-By      :ARTWORK_43_Signing ;
        :Follows          :ARTWORK_43_Transporting_2 ;
        :Has-Duration     <http://www.semanticweb.org/ontologies/Daan/2020/BarbaraNanning#2008> ;
        :Involves         :BarbaraNanning , :AlešZvěřina ;
        :Located-In       :CzechRepublic ;
        :Part-Of          :Creation_Artwork_43 ;
        :Requires-Use-Of  :AirCompressor .

<http://www.semanticweb.org/ontologies/Daan/2020/BarbaraNanning#ARTWORK_74_ExaminingQuality(Shape/Form)>
        a                 j.2: , owl:NamedIndividual ;
        rdfs:comment      "Instance of an activity which is part of the creation process of ARTWORK_74."@en ;
        rdfs:label        "ARTWORK_74_Examining Quality (Shape/Form)"@en ;
        :Followed-By      :ARTWORK_74_Translocating ;
        :Follows          :ARTWORK_74_Modeling ;
        :Has-Duration     <http://www.semanticweb.org/ontologies/Daan/2020/BarbaraNanning#2008> ;
        :Involves         :BarbaraNanning , :AlešZvěřina ;
        :Located-In       :CzechRepublic ;
        :Part-Of          :Creation_Artwork_74 ;
        :Requires-Use-Of  :BlowingPipe , :GloryHole , :Pontis .

:Involves  a          owl:ObjectProperty ;
        rdfs:comment  "Involves is a property which connects an actor with an activity."@en ;
        rdfs:domain   :Activity ;
        rdfs:label    "Involves"@en ;
        rdfs:range    :Actor .

:Consists-Of  a        owl:ObjectProperty ;
        rdfs:comment   "Consists-Of is a property which connects an entity to the entities which it encompasses."@en ;
        rdfs:domain    :Entity ;
        rdfs:label     "Consists-Of"@en ;
        rdfs:range     :Entity ;
        owl:inverseOf  :Part-Of .

:ARTWORK_43_Transporting_3
        a              :Transporting , owl:NamedIndividual ;
        rdfs:comment   "Instance of an activity which is part of the creation process of ARTWORK_43."@en ;
        rdfs:label     "ARTWORK_43_Transporting_3"@en ;
        :Followed-By   :ARTWORK_43_Gilding ;
        :Follows       :ARTWORK_43_Packing_3 ;
        :Has-Duration  <http://www.semanticweb.org/ontologies/Daan/2020/BarbaraNanning#2008> ;
        :Involves      :BarbaraNanning , :AlešZvěřina ;
        :Located-In    :CzechRepublic ;
        :Part-Of       :Creation_Artwork_43 .

[ a            owl:AllDisjointClasses ;
  owl:members  ( :Gallery :Museum :Studio )
] .

:ARTWORK_36_Sawing  a     owl:NamedIndividual , :Sawing ;
        rdfs:comment      "Instance of an activity which is part of the creation process of ARTWORK_36."@en ;
        rdfs:label        "ARTWORK_36_Sawing"@en ;
        :Followed-By      :ARTWORK_36_Sensing_2 ;
        :Follows          <http://www.semanticweb.org/ontologies/Daan/2020/BarbaraNanning#ARTWORK_36_ExaminingQuality(CheckForIrregularitiesInTheGlass)> ;
        :Has-Duration     <http://www.semanticweb.org/ontologies/Daan/2020/BarbaraNanning#2015> ;
        :Involves         :AlešZvěřina , :BarbaraNanning ;
        :Located-In       :NovyBor ;
        :Part-Of          :Creation_Artwork_36 ;
        :Requires-Use-Of  :DiamondSaw .

<http://www.semanticweb.org/ontologies/Daan/2020/BarbaraNanning#ARTWORK_43_ExaminingQuality(FinalResult)>
        a              owl:NamedIndividual , j.1: ;
        rdfs:comment   "Instance of an activity which is part of the creation process of ARTWORK_43."@en ;
        rdfs:label     "ARTWORK_43_Examining Quality (Final Result)"@en ;
        :Followed-By   :ARTWORK_43_Packing_5 ;
        :Follows       :ARTWORK_43_Gilding ;
        :Has-Duration  <http://www.semanticweb.org/ontologies/Daan/2020/BarbaraNanning#2008> ;
        :Involves      :AlešZvěřina , :BarbaraNanning ;
        :Located-In    :CzechRepublic ;
        :Part-Of       :Creation_Artwork_43 .

:ARTWORK_79_Sawing  a     owl:NamedIndividual , :Sawing ;
        rdfs:comment      "Instance of an activity which is part of the creation process of ARTWORK_79."@en ;
        rdfs:label        "ARTWORK_79_Sawing"@en ;
        :Followed-By      :ARTWORK_79_Grinding ;
        :Follows          <http://www.semanticweb.org/ontologies/Daan/2020/BarbaraNanning#ARTWORK_79_ExaminingQuality(CheckForIrregularitiesInTheGlass)> ;
        :Has-Duration     <http://www.semanticweb.org/ontologies/Daan/2020/BarbaraNanning#2018> ;
        :Involves         :AlešZvěřina , :BarbaraNanning ;
        :Located-In       :CzechRepublic ;
        :Part-Of          :Creation_Artwork_79 ;
        :Requires-Use-Of  :DiamondSaw .

:ARTWORK_18_64_Photographing
        a              :Photographing , owl:NamedIndividual ;
        rdfs:comment   "Instance of an activity which is part of the creation process of ARTWORK_18_64."@en ;
        rdfs:label     "ARTWORK_18_64_Photographing"@en ;
        :Followed-By   :ARTWORK_18_64_Packing_3 ;
        :Follows       :ARTWORK_18_64_Transporting_2 ;
        :Has-Duration  <http://www.semanticweb.org/ontologies/Daan/2020/BarbaraNanning#2015> ;
        :Involves      <http://www.semanticweb.org/ontologies/Daan/2020/BarbaraNanning#TomHaartsen_Ouderkerka/dAmstel(NL)> , :BarbaraNanning ;
        :Located-In    <http://www.semanticweb.org/ontologies/Daan/2020/BarbaraNanning#Ouderkerka/dAmstel> ;
        :Part-Of       :Creation_Artwork_18_64 .

:ARTWORK_18_64_ApplyingClearGlassBell
        a                 owl:NamedIndividual , :Applying_Clear_Glass_Bell ;
        rdfs:comment      "Instance of an activity which is part of the creation process of ARTWORK_18_64."@en ;
        rdfs:label        "ARTWORK_18_64_Applying Clear Glass Bell"@en ;
        :Followed-By      :ARTWORK_18_64_PickingUpColouredCanesPattern ;
        :Follows          :ARTWORK_18_64_ExaminingTheQualityOfTheGlass ;
        :Has-Duration     <http://www.semanticweb.org/ontologies/Daan/2020/BarbaraNanning#2015> ;
        :Involves         :BarbaraNanning , <http://www.semanticweb.org/ontologies/Daan/2020/BarbaraNanning#MarekBrathko(CZ)> , :GertBullée ;
        :Located-In       :Zaandam ;
        :Part-Of          :Creation_Artwork_18_64 ;
        :Requires-Use-Of  :AirCompressor , :Hook , :Jacks , :Pincet , :Beeswax , :Blocks , :Paper , :Water , :Furnace , :Marver , :IcePick , :BlowingPipe , :StraightShears , :DiamondShears , :CeramicPotFilledWithGlass , :YokeOfSupport .

:ARTWORK_46_SetupAndTestingOfTheMetalMold
        a                 owl:NamedIndividual , :Setup_and_Testing_of_the_Metal_Mold ;
        rdfs:comment      "Instance of an activity which is part of the creation process of ARTWORK_46."@en ;
        rdfs:label        "ARTWORK_46_Setup and Testing of the Metal Mold"@en ;
        :Followed-By      :ARTWORK_46_ExaminingTheQualityOfTheGlass ;
        :Follows          :ARTWORK_46_PreparingGlass ;
        :Has-Duration     <http://www.semanticweb.org/ontologies/Daan/2020/BarbaraNanning#2018> ;
        :Involves         :JaroslavKubásek , :DavidČerný , <http://www.semanticweb.org/ontologies/Daan/2020/BarbaraNanning#JiriPacinek(CZ)> , :JiříPačinekJunior , :BarbaraNanning , :JanBaštýř ;
        :Located-In       :Lindava ;
        :Part-Of          :Creation_Artwork_46 ;
        :Requires-Use-Of  :InterchangeableMetalMoldSetup .

<http://vocab.getty.edu/aat/300053932>
        a                    owl:Class ;
        owl:equivalentClass  :Glassblowing .

:ARTWORK_79_Cooling  a    owl:NamedIndividual , :Cooling ;
        rdfs:comment      "Instance of an activity which is part of the creation process of ARTWORK_79."@en ;
        rdfs:label        "ARTWORK_79_Cooling"@en ;
        :Followed-By      :ARTWORK_79_Packing ;
        :Follows          :ARTWORK_79_Translocating ;
        :Has-Duration     <http://www.semanticweb.org/ontologies/Daan/2020/BarbaraNanning#2018> ;
        :Involves         :LuděkKout , :AssistantOfBarbara ;
        :Located-In       :CzechRepublic ;
        :Part-Of          :Creation_Artwork_79 ;
        :Requires-Use-Of  :AnnealingKiln .

:VRIJGLASZaandam  a   :Glass_Studio , owl:NamedIndividual ;
        rdfs:comment  "VRIJGLAS Zaandam is a glass studio in Zaandam."@en ;
        rdfs:label    "VRIJGLAS Zaandam"@en ;
        :Employed     :DurkValkema , <http://www.semanticweb.org/ontologies/Daan/2020/BarbaraNanning#MarekBrathko(CZ)> , :GertBullée , <http://www.semanticweb.org/ontologies/Daan/2020/BarbaraNanning#MarekEffmert(CZ)> , <http://www.semanticweb.org/ontologies/Daan/2020/BarbaraNanning#RobertLenner(CZ)> , <http://www.semanticweb.org/ontologies/Daan/2020/BarbaraNanning#JessicaHomich(USA)> ;
        :Located-In   :Zaandam ;
        :Maker-Of     :Artwork_36 , :Artwork_46 , :Artwork_39 , :Artwork_18_64 .

:ARTWORK_79_Polishing
        a                 owl:NamedIndividual , :Polishing ;
        rdfs:comment      "Instance of an activity which is part of the creation process of ARTWORK_79."@en ;
        rdfs:label        "ARTWORK_79_Polishing"@en ;
        :Followed-By      <http://www.semanticweb.org/ontologies/Daan/2020/BarbaraNanning#ARTWORK_79_ExaminingQuality(Result)> ;
        :Follows          :ARTWORK_79_Grinding ;
        :Has-Duration     <http://www.semanticweb.org/ontologies/Daan/2020/BarbaraNanning#2018> ;
        :Involves         :AlešZvěřina , :BarbaraNanning , :LukášSvoboda ;
        :Located-In       :CzechRepublic ;
        :Part-Of          :Creation_Artwork_79 ;
        :Requires-Use-Of  :PolishingStone .

<http://vocab.getty.edu/aat/300264232>
        a           owl:NamedIndividual ;
        owl:sameAs  :Calcium .

:ARTWORK_80_Translocating
        a                 :Translocating , owl:NamedIndividual ;
        rdfs:comment      "Instance of an activity which is part of the creation process of ARTWORK_80."@en ;
        rdfs:label        "ARTWORK_80_Translocating"@en ;
        :Followed-By      :ARTWORK_80_Cooling ;
        :Follows          <http://www.semanticweb.org/ontologies/Daan/2020/BarbaraNanning#ARTWORK_80_ExaminingQuality(Shape/Form)> ;
        :Has-Duration     <http://www.semanticweb.org/ontologies/Daan/2020/BarbaraNanning#2018> ;
        :Involves         :BarbaraNanning ;
        :Located-In       :CzechRepublic ;
        :Part-Of          :Creation_Artwork_80 ;
        :Requires-Use-Of  :Fork .

:ARTWORK_36_Sensing  a  :Sensing , owl:NamedIndividual ;
        rdfs:comment   "Instance of an activity which is part of the creation process of ARTWORK_36."@en ;
        rdfs:label     "ARTWORK_36_Sensing"@en ;
        :Followed-By   :ARTWORK_36_Modeling ;
        :Follows       :ARTWORK_36_Glassblowing ;
        :Has-Duration  <http://www.semanticweb.org/ontologies/Daan/2020/BarbaraNanning#2015> ;
        :Involves      :BarbaraNanning ;
        :Located-In    :Zaandam ;
        :Part-Of       :Creation_Artwork_36 .

:ARTWORK_43_Sensing  a  :Sensing , owl:NamedIndividual ;
        rdfs:comment   "Instance of an activity which is part of the creation process of ARTWORK_43."@en ;
        rdfs:label     "ARTWORK_43_Sensing"@en ;
        :Followed-By   :ARTWORK_43_Glassblowing ;
        :Follows       :ARTWORK_43_Modeling ;
        :Has-Duration  <http://www.semanticweb.org/ontologies/Daan/2020/BarbaraNanning#2008> ;
        :Involves      :BarbaraNanning , :LukášSvoboda , :AlešZvěřina ;
        :Located-In    :CzechRepublic ;
        :Part-Of       :Creation_Artwork_43 .

:CollectionOfBarbaraNanning
        a               owl:NamedIndividual , :Private_Collection ;
        rdfs:comment    "The collection of Barbara Nanning is a private art collection of Nanning."@en ;
        rdfs:label      "Collection of Barbara Nanning"@en ;
        :Consists-Of    :Artwork_80 , :Artwork_76 , :Artwork_77 , :Artwork_75 ;
        :Located-In     :Amsterdam ;
        :Maintained-By  :BarbaraNanning .

:First_Glass_Blower  a   owl:Class ;
        rdfs:comment     "The first glass blower is the second highest role within a glass blowing team."@en ;
        rdfs:label       "First Glass Blower"@en ;
        rdfs:subClassOf  :Glass_Blower .

<http://www.wikidata.org/entity/Q6256>
        a       owl:Class .

:ARTWORK_46_PreparingForBlowing
        a                 owl:NamedIndividual , :Preparing_for_Blowing ;
        rdfs:comment      "Instance of an activity which is part of the creation process of ARTWORK_46."@en ;
        rdfs:label        "ARTWORK_46_Preparing for Blowing"@en ;
        :Followed-By      :ARTWORK_46_FillingKilnsWithMetalBowl ;
        :Follows          :ARTWORK_46_TransportingMetalBowlWithCanesAndStrings ;
        :Has-Duration     <http://www.semanticweb.org/ontologies/Daan/2020/BarbaraNanning#2018> ;
        :Involves         :BarbaraNanning , <http://www.semanticweb.org/ontologies/Daan/2020/BarbaraNanning#JiriPacinek(CZ)> , <http://www.semanticweb.org/ontologies/Daan/2020/BarbaraNanning#JessicaHomich(USA)> ;
        :Located-In       :Lindava ;
        :Part-Of          :Creation_Artwork_46 ;
        :Requires-Use-Of  :Paper , :AnnealingKiln , :BlowingPipe , :FusingKiln , :Furnace , :Garage , :Water .

:ARTWORK_79_Resting  a    :Resting , owl:NamedIndividual ;
        rdfs:comment      "Instance of an activity which is part of the creation process of ARTWORK_79."@en ;
        rdfs:label        "ARTWORK_79_Resting"@en ;
        :Followed-By      <http://www.semanticweb.org/ontologies/Daan/2020/BarbaraNanning#ARTWORK_79_ExaminingQuality(CheckForIrregularitiesInTheGlass)> ;
        :Follows          :ARTWORK_79_Transporting ;
        :Has-Duration     <http://www.semanticweb.org/ontologies/Daan/2020/BarbaraNanning#2018> ;
        :Involves         :AlešZvěřina ;
        :Located-In       :CzechRepublic ;
        :Part-Of          :Creation_Artwork_79 ;
        :Requires-Use-Of  :AnnealingKiln .

:ARTWORK_75_Packing_2
        a              owl:NamedIndividual , :Packing ;
        rdfs:comment   "Instance of an activity which is part of the creation process of ARTWORK_75."@en ;
        rdfs:label     "ARTWORK_75_Packing_2"@en ;
        :Followed-By   :ARTWORK_75_Transporting_2 ;
        :Follows       <http://www.semanticweb.org/ontologies/Daan/2020/BarbaraNanning#ARTWORK_75_ExaminingQuality(Result)> ;
        :Has-Duration  <http://www.semanticweb.org/ontologies/Daan/2020/BarbaraNanning#2018> ;
        :Involves      :AlešZvěřina , :BarbaraNanning ;
        :Located-In    :CzechRepublic ;
        :Part-Of       :Creation_Artwork_75 .

<http://sws.geonames.org/2659994>
        a           owl:NamedIndividual ;
        owl:sameAs  :Lausanne .

:ARTWORK_36_ApplyingClearGlassBell
        a                 :Applying_Clear_Glass_Bell , owl:NamedIndividual ;
        rdfs:comment      "Instance of an activity which is part of the creation process of ARTWORK_36."@en ;
        rdfs:label        "ARTWORK_36_Applying Clear Glass Bell"@en ;
        :Followed-By      :ARTWORK_36_PickingUpColouredCanesPattern ;
        :Follows          :ARTWORK_36_ExaminingTheQualityOfTheGlass ;
        :Has-Duration     <http://www.semanticweb.org/ontologies/Daan/2020/BarbaraNanning#2015> ;
        :Involves         :GertBullée , <http://www.semanticweb.org/ontologies/Daan/2020/BarbaraNanning#MarekBrathko(CZ)> , :BarbaraNanning ;
        :Located-In       :Zaandam ;
        :Part-Of          :Creation_Artwork_36 ;
        :Requires-Use-Of  :DiamondShears , :CeramicPotFilledWithGlass , :Water , :BlowingPipe , :Hook , :Pincet , :Furnace , :Jacks , :Paper , :AirCompressor , :StraightShears , :Beeswax , :Marver , :IcePick , :Blocks , :YokeOfSupport .

:Works-For  a         owl:ObjectProperty ;
        rdfs:comment  "Works-For is a property which connects a person with an organisation."@en ;
        rdfs:domain   :Person ;
        rdfs:label    "Works-For"@en ;
        rdfs:range    :Organisation .

:ARTWORK_74_Grinding  a   :Grinding , owl:NamedIndividual ;
        rdfs:comment      "Instance of an activity which is part of the creation process of ARTWORK_74."@en ;
        rdfs:label        "ARTWORK_74_Grinding"@en ;
        :Followed-By      :ARTWORK_74_Polishing ;
        :Follows          :ARTWORK_74_Sawing ;
        :Has-Duration     <http://www.semanticweb.org/ontologies/Daan/2020/BarbaraNanning#2008> ;
        :Involves         :RobertFlorian , :AlešZvěřina , :BarbaraNanning ;
        :Located-In       :CzechRepublic ;
        :Part-Of          :Creation_Artwork_74 ;
        :Requires-Use-Of  :SharpeningStone , :GrindingWheel .

:ARTWORK_79_SetupAndTestingOfTheMetalMold_2
        a                 owl:NamedIndividual , :Setup_and_Testing_of_the_Metal_Mold ;
        rdfs:comment      "Instance of an activity which is part of the creation process of ARTWORK_79."@en ;
        rdfs:label        "ARTWORK_79_Setup and Testing of the Metal Mold_2"@en ;
        :Followed-By      :ARTWORK_79_ApplyingClearGlassBell ;
        :Follows          :ARTWORK_79_ExaminingTheQualityOfTheGlass ;
        :Has-Duration     <http://www.semanticweb.org/ontologies/Daan/2020/BarbaraNanning#2018> ;
        :Involves         <http://www.semanticweb.org/ontologies/Daan/2020/BarbaraNanning#JiriMoravec(CZ)> , <http://www.semanticweb.org/ontologies/Daan/2020/BarbaraNanning#RadekKoten(CZ)> , :BarbaraNanning , <http://www.semanticweb.org/ontologies/Daan/2020/BarbaraNanning#LukasHavlas(CZ)> , :AssistantOfBarbara , <http://www.semanticweb.org/ontologies/Daan/2020/BarbaraNanning#Tom%C3%A1%C5%A1Moravec(CZ)> ;
        :Located-In       :CzechRepublic ;
        :Part-Of          :Creation_Artwork_79 ;
        :Requires-Use-Of  :InterchangeableMetalMoldSetup .

<http://www.semanticweb.org/ontologies/Daan/2020/BarbaraNanning#ARTWORK_18_64_ExaminingQuality(CheckForIrregularitiesInTheGlass)>
        a              j.3: , owl:NamedIndividual ;
        rdfs:comment   "Instance of an activity which is part of the creation process of ARTWORK_18_64."@en ;
        rdfs:label     "ARTWORK_18_64_Examining Quality (Check for Irregularities in the Glass)"@en ;
        :Followed-By   :ARTWORK_18_64_Sawing ;
        :Follows       :ARTWORK_18_64_Resting ;
        :Has-Duration  <http://www.semanticweb.org/ontologies/Daan/2020/BarbaraNanning#2015> ;
        :Involves      :BarbaraNanning , :AlešZvěřina ;
        :Located-In    :NovyBor ;
        :Part-Of       :Creation_Artwork_18_64 .

:ARTWORK_44_Glassblowing
        a                 owl:NamedIndividual , :Glassblowing ;
        rdfs:comment      "Instance of an activity which is part of the creation process of ARTWORK_44."@en ;
        rdfs:label        "ARTWORK_44_Glassblowing"@en ;
        :Followed-By      :ARTWORK_44_Sensing ;
        :Follows          :ARTWORK_44_HeatingMetalMold ;
        :Has-Duration     <http://www.semanticweb.org/ontologies/Daan/2020/BarbaraNanning#2018> ;
        :Involves         <http://www.semanticweb.org/ontologies/Daan/2020/BarbaraNanning#RadekKoten(CZ)> , <http://www.semanticweb.org/ontologies/Daan/2020/BarbaraNanning#JiriMoravec(CZ)> , <http://www.semanticweb.org/ontologies/Daan/2020/BarbaraNanning#LukasHavlas(CZ)> , :AssistantOfBarbara , <http://www.semanticweb.org/ontologies/Daan/2020/BarbaraNanning#Tom%C3%A1%C5%A1Moravec(CZ)> , :BarbaraNanning ;
        :Located-In       :CzechRepublic ;
        :Part-Of          :Creation_Artwork_44 ;
        :Requires-Use-Of  :Furnace , :AirCompressor , :PropaneTorch , :YokeOfSupport , :Gloves , :Pontis , :BitIron , :GloryHole , :Hook , :IcePick , :Tagliol , :Paper , :DiamondShears , :InterchangeableMetalMoldSetup , :BlowingPipe , :Pincet , :Water , :Beeswax , :AnnealingKiln , :Marver , :Blocks , :Jacks , :StraightShears , :CeramicPotFilledWithGlass , :Fork .

:Netherlands  a       :Country , owl:NamedIndividual ;
        rdfs:comment  "The Netherlands is a country in western Europe."@en ;
        rdfs:label    "Netherlands"@en ;
        owl:sameAs    <http://www.wikidata.org/entity/Q55> ;
        :Location-Of  :Amsterdam .

:ARTWORK_39_HeatingMetalMold
        a                 owl:NamedIndividual , :Heating_Metal_Mold ;
        rdfs:comment      "Instance of an activity which is part of the creation process of ARTWORK_39."@en ;
        rdfs:label        "ARTWORK_39_Heating Metal Mold"@en ;
        :Followed-By      :ARTWORK_39_Glassblowing ;
        :Follows          :ARTWORK_39_PickingUpColouredPanel ;
        :Has-Duration     <http://www.semanticweb.org/ontologies/Daan/2020/BarbaraNanning#2015> ;
        :Involves         :BarbaraNanning ;
        :Located-In       :Zaandam ;
        :Part-Of          :Creation_Artwork_39 ;
        :Requires-Use-Of  :Gloves , :PropaneTorch , :InterchangeableMetalMoldSetup .

:Cutting_Strings  a      owl:Class ;
        rdfs:comment     "After being pulled between 2 pipes, a glass string, when cooled, can be cut with a variety of tools to various lengths."@en ;
        rdfs:label       "Cutting Strings"@en ;
        rdfs:subClassOf  :Activity .

:ARTWORK_17_33_ModelingWithTeflonStick
        a                 owl:NamedIndividual , :Modeling_with_Teflon_Stick ;
        rdfs:comment      "Instance of an activity which is part of the creation process of ARTWORK_17_33."@en ;
        rdfs:label        "ARTWORK_17_33_Modeling with Teflon Stick"@en ;
        :Followed-By      :ARTWORK_17_33_FillingHolesWithClearGlass ;
        :Follows          :ARTWORK_17_33_Glassblowing ;
        :Has-Duration     <http://www.semanticweb.org/ontologies/Daan/2020/BarbaraNanning#2017> ;
        :Involves         <http://www.semanticweb.org/ontologies/Daan/2020/BarbaraNanning#LukasHavlas(CZ)> , <http://www.semanticweb.org/ontologies/Daan/2020/BarbaraNanning#JiriMoravec(CZ)> , :BarbaraNanning , <http://www.semanticweb.org/ontologies/Daan/2020/BarbaraNanning#RadekKoten(CZ)> , <http://www.semanticweb.org/ontologies/Daan/2020/BarbaraNanning#Tom%C3%A1%C5%A1Moravec(CZ)> , :AssistantOfBarbara , <http://www.semanticweb.org/ontologies/Daan/2020/BarbaraNanning#JessicaHomich(USA)> ;
        :Located-In       :Lindava ;
        :Part-Of          :Creation_Artwork_17_33 ;
        :Requires-Use-Of  :StraightShears , :CeramicPotFilledWithGlass , :GrindingWheel , :Water , :TeflonStick , :Pincet , :DiamondShears , :Pontis , :Gloves , :Jacks , :BitIron , :Marver , :Hook , :PropaneTorch , :Paper , :YokeOfSupport , :GloryHole , :AirCompressor , :Beeswax , :Tagliol , :Furnace , :Blocks , :BlowingPipe .

[ a            owl:AllDisjointClasses ;
  owl:members  ( :Metal_Worker_1 :Metal_Worker_2 :Metal_Worker_3 )
] .

:ARTWORK_78_SetupAndTestingOfTheMetalMold_2
        a                 :Setup_and_Testing_of_the_Metal_Mold , owl:NamedIndividual ;
        rdfs:comment      "Instance of an activity which is part of the creation process of ARTWORK_78."@en ;
        rdfs:label        "ARTWORK_78_Setup and Testing of the Metal Mold_2"@en ;
        :Followed-By      :ARTWORK_78_ApplyingClearGlassBell ;
        :Follows          :ARTWORK_78_ExaminingTheQualityOfTheGlass ;
        :Has-Duration     <http://www.semanticweb.org/ontologies/Daan/2020/BarbaraNanning#2008> ;
        :Involves         <http://www.semanticweb.org/ontologies/Daan/2020/BarbaraNanning#RomanTomis(CZ)> , :BarbaraNanning , <http://www.semanticweb.org/ontologies/Daan/2020/BarbaraNanning#RobertHlavacek(CZ)> , <http://www.semanticweb.org/ontologies/Daan/2020/BarbaraNanning#AlesVacek(CZ)> , <http://www.semanticweb.org/ontologies/Daan/2020/BarbaraNanning#RostislavMaterka(CZ)> , :AssistantOfBarbara ;
        :Located-In       :CzechRepublic ;
        :Part-Of          :Creation_Artwork_78 ;
        :Requires-Use-Of  :InterchangeableMetalMoldSetup .

<http://www.wikidata.org/entity/Q1250322>
        a       owl:Class .

:Gilder  a               owl:Class ;
        rdfs:comment     "A gilder is a person who applies gold leaf on things."@en ;
        rdfs:label       "Gilder"@en ;
        rdfs:subClassOf  :Person .

:Fork   a             :Tool , owl:NamedIndividual ;
        rdfs:comment  "A fork is a tool with multiple prongs used to lift things."@en ;
        rdfs:label    "Fork"@en ;
        :Used-For     :ARTWORK_79_Glassblowing , :ARTWORK_77_Glassblowing , :ARTWORK_75_ApplyingExtraColour_2 , :ARTWORK_75_Glassblowing , :ARTWORK_80_Glassblowing , :ARTWORK_79_ApplyingExtraColour , :ARTWORK_43_ApplyingExtraColour , :ARTWORK_80_ApplyingExtraColour , :ARTWORK_77_Translocating , :ARTWORK_43_Glassblowing , :ARTWORK_74_ApplyingExtraColour , :ARTWORK_76_Glassblowing , :ARTWORK_74_Translocating , :ARTWORK_75_Translocating , :ARTWORK_44_ApplyingExtraColour_2 , :ARTWORK_78_Translocating , :ARTWORK_44_ApplyingExtraColour , :ARTWORK_74_Glassblowing , :ARTWORK_78_ApplyingExtraColour , :ARTWORK_79_ApplyingExtraColour_2 , :ARTWORK_73_Glassblowing , :ARTWORK_78_Glassblowing , :ARTWORK_76_ApplyingExtraColour , :ARTWORK_76_ApplyingExtraColour_2 , :ARTWORK_43_Translocating , :ARTWORK_77_ApplyingExtraColour , :ARTWORK_75_ApplyingExtraColour , :ARTWORK_76_Translocating , :ARTWORK_79_Translocating , :ARTWORK_74_ApplyingExtraColour_2 , :ARTWORK_44_Glassblowing , :ARTWORK_44_Translocating , :ARTWORK_80_Translocating , :ARTWORK_73_Translocating .

<http://www.cidoc-crm.org/cidoc-crm/P115_finishes>
        a                       owl:ObjectProperty ;
        owl:equivalentProperty  :Finishes .

<http://vocab.getty.edu/aat/300264831>
        a                    owl:Class ;
        owl:equivalentClass  :Gold_Leaf .

:ARTWORK_78_Cooling  a    :Cooling , owl:NamedIndividual ;
        rdfs:comment      "Instance of an activity which is part of the creation process of ARTWORK_78."@en ;
        rdfs:label        "ARTWORK_78_Cooling"@en ;
        :Followed-By      :ARTWORK_78_Packing ;
        :Follows          :ARTWORK_78_Translocating ;
        :Has-Duration     <http://www.semanticweb.org/ontologies/Daan/2020/BarbaraNanning#2016> ;
        :Involves         :AssistantOfBarbara , :LuděkKout ;
        :Located-In       :CzechRepublic ;
        :Part-Of          :Creation_Artwork_78 ;
        :Requires-Use-Of  :AnnealingKiln .

:ARTWORK_75_Documenting
        a              :Documenting , owl:NamedIndividual ;
        rdfs:comment   "Instance of an activity which is part of the creation process of ARTWORK_75."@en ;
        rdfs:label     "ARTWORK_75_Documenting"@en ;
        :Followed-By   :ARTWORK_75_Packing_5 ;
        :Follows       :ARTWORK_75_Photographing ;
        :Has-Duration  <http://www.semanticweb.org/ontologies/Daan/2020/BarbaraNanning#2017> ;
        :Involves      :BarbaraNanning ;
        :Located-In    :CzechRepublic ;
        :Part-Of       :Creation_Artwork_75 .

<http://www.semanticweb.org/ontologies/Daan/2020/BarbaraNanning#LukasHavlas(CZ)>
        a             :First_Glass_Blower , owl:NamedIndividual ;
        rdfs:comment  "Lukas Havlas (CZ) is a First Glass Blower."@en ;
        rdfs:label    "Lukas Havlas (CZ)"@en ;
        :Involved-In  :ARTWORK_80_Modeling , :ARTWORK_44_ApplyingExtraColour_2 , :ARTWORK_44_Glassblowing , :ARTWORK_77_Glassblowing , :ARTWORK_77_SetupAndTestingOfTheMetalMold_2 , :ARTWORK_75_ApplyingExtraColour_2 , :ARTWORK_79_Modeling , :ARTWORK_79_Glassblowing , :ARTWORK_80_SetupAndTestingOfTheMetalMold_2 , :ARTWORK_80_SetupAndTestingOfTheMetalMold , :ARTWORK_73_SetupAndTestingOfTheMetalMold , :ARTWORK_75_ApplyingExtraColour , :ARTWORK_79_SetupAndTestingOfTheMetalMold_2 , :ARTWORK_44_Modeling , :ARTWORK_73_SetupAndTestingOfTheMetalMold_2 , :ARTWORK_76_SetupAndTestingOfTheMetalMold_2 , :ARTWORK_80_Glassblowing , :ARTWORK_44_SetupAndTestingOfTheMetalMold_2 , :ARTWORK_75_SetupAndTestingOfTheMetalMold , :ARTWORK_76_Glassblowing , :ARTWORK_77_ApplyingClearGlassBell , :ARTWORK_80_ApplyingExtraColour , :ARTWORK_76_SetupAndTestingOfTheMetalMold , :ARTWORK_73_Modeling , :ARTWORK_75_SetupAndTestingOfTheMetalMold_2 , :ARTWORK_77_SetupAndTestingOfTheMetalMold , :ARTWORK_76_Modeling , :ARTWORK_80_ApplyingClearGlassBell , :ARTWORK_76_ApplyingExtraColour_2 , :ARTWORK_76_ApplyingExtraColour , :ARTWORK_75_ApplyingClearGlassBell , :ARTWORK_76_ApplyingClearGlassBell , :ARTWORK_73_Glassblowing , :ARTWORK_79_ApplyingExtraColour , :ARTWORK_79_ApplyingClearGlassBell , :ARTWORK_77_Modeling , :ARTWORK_79_SetupAndTestingOfTheMetalMold , :ARTWORK_79_ApplyingExtraColour_2 , :ARTWORK_75_Modeling , :ARTWORK_73_ApplyingClearGlassBell , :ARTWORK_75_Glassblowing , :ARTWORK_44_ApplyingClearGlassBell , :ARTWORK_44_SetupAndTestingOfTheMetalMold , :ARTWORK_77_ApplyingExtraColour , :ARTWORK_44_ApplyingExtraColour ;
        :Works-For    :LASVITAJETO .

:ARTWORK_77_ApplyingClearGlassBell
        a                 :Applying_Clear_Glass_Bell , owl:NamedIndividual ;
        rdfs:comment      "Instance of an activity which is part of the creation process of ARTWORK_77."@en ;
        rdfs:label        "ARTWORK_77_Applying Clear Glass Bell"@en ;
        :Followed-By      :ARTWORK_77_ApplyingExtraColour ;
        :Follows          :ARTWORK_77_ExaminingTheQualityOfTheGlass ;
        :Has-Duration     <http://www.semanticweb.org/ontologies/Daan/2020/BarbaraNanning#2018> ;
        :Involves         <http://www.semanticweb.org/ontologies/Daan/2020/BarbaraNanning#LukasHavlas(CZ)> , :BarbaraNanning , <http://www.semanticweb.org/ontologies/Daan/2020/BarbaraNanning#RadekKoten(CZ)> ;
        :Located-In       :CzechRepublic ;
        :Part-Of          :Creation_Artwork_77 ;
        :Processes        :AJETOClearGlass ;
        :Requires-Use-Of  :AirCompressor , :Marver , :Hook , :Blocks , :Beeswax , :DiamondShears , :Paper , :CeramicPotFilledWithGlass , :IcePick , :Jacks , :Water , :Pincet , :Furnace , :StraightShears , :BlowingPipe , :YokeOfSupport .

<http://www.wikidata.org/entity/Q25290>
        a       owl:NamedIndividual .

:Heating_Metal_Mold  a   owl:Class ;
        rdfs:comment     "Heating Metal Mold is an activity in which an actor is using the propane torch to heat the metal mold."@en ;
        rdfs:label       "Heating Metal Mold"@en ;
        rdfs:subClassOf  :Heating .

:ARTWORK_36_Documenting_2
        a              owl:NamedIndividual , :Documenting ;
        rdfs:comment   "Instance of an activity which is part of the creation process of ARTWORK_36."@en ;
        rdfs:label     "ARTWORK_36_Documenting_2"@en ;
        :Finishes      :Creation_Artwork_36 ;
        :Follows       :ARTWORK_36_Packing_8 ;
        :Has-Duration  <http://www.semanticweb.org/ontologies/Daan/2020/BarbaraNanning#2019> ;
        :Involves      :BarbaraNanning ;
        :Located-In    :Amsterdam ;
        :Part-Of       :Creation_Artwork_36 .

:Furnace  a               :Equipment , owl:NamedIndividual ;
        rdfs:comment      "A furnace is an structure in which things can be heated."@en ;
        rdfs:label        "Furnace"@en ;
        :Has-Temperature  "1400"^^xsd:decimal ;
        :Used-For         :ARTWORK_77_ExaminingTheQualityOfTheGlass , :ARTWORK_77_Glassblowing , :ARTWORK_74_Glassblowing , :ARTWORK_77_ApplyingClearGlassBell , :ARTWORK_75_ApplyingExtraColour , :ARTWORK_79_ApplyingExtraColour_2 , :ARTWORK_75_ExaminingTheQualityOfTheGlass , :ARTWORK_74_ApplyingExtraColour_2 , :ARTWORK_44_ExaminingTheQualityOfTheGlass , :ARTWORK_80_ExaminingTheQualityOfTheGlass , :ARTWORK_73_ExaminingTheQualityOfTheGlass , :ARTWORK_78_ApplyingClearGlassBell , :ARTWORK_73_Glassblowing , :ARTWORK_76_ApplyingClearGlassBell , :ARTWORK_76_ApplyingExtraColour_2 , :ARTWORK_75_ApplyingExtraColour_2 , :ARTWORK_79_ExaminingTheQualityOfTheGlass , :ARTWORK_74_ApplyingClearGlassBell , :ARTWORK_73_ApplyingClearGlassBell , :ARTWORK_75_ApplyingClearGlassBell , :ARTWORK_76_Glassblowing , :ARTWORK_78_Glassblowing , :ARTWORK_79_ApplyingExtraColour , :ARTWORK_80_ApplyingExtraColour , :ARTWORK_44_ApplyingClearGlassBell , :ARTWORK_43_Glassblowing , :ARTWORK_44_ApplyingExtraColour , :ARTWORK_74_ApplyingExtraColour , :ARTWORK_77_ApplyingExtraColour , :ARTWORK_80_Glassblowing , :ARTWORK_43_ExaminingTheQualityOfTheGlass , :ARTWORK_43_ApplyingExtraColour , :ARTWORK_76_ApplyingExtraColour , :ARTWORK_80_ApplyingClearGlassBell , :ARTWORK_78_ExaminingTheQualityOfTheGlass , :ARTWORK_78_ApplyingExtraColour , :ARTWORK_75_Glassblowing , :ARTWORK_44_ApplyingExtraColour_2 , :ARTWORK_79_ApplyingClearGlassBell , :ARTWORK_76_ExaminingTheQualityOfTheGlass , :ARTWORK_79_Glassblowing , :ARTWORK_43_ApplyingClearGlassBell , :ARTWORK_74_ExaminingTheQualityOfTheGlass , :ARTWORK_44_Glassblowing .

<http://www.semanticweb.org/ontologies/Daan/2020/BarbaraNanning#ARTWORK_80_ExaminingQuality(Result)>
        a              owl:NamedIndividual , j.0: ;
        rdfs:comment   "Instance of an activity which is part of the creation process of ARTWORK_80."@en ;
        rdfs:label     "ARTWORK_80_Examining Quality (Result)"@en ;
        :Followed-By   :ARTWORK_80_MeasuringAndBoxesMaking ;
        :Follows       :ARTWORK_80_Polishing ;
        :Has-Duration  <http://www.semanticweb.org/ontologies/Daan/2020/BarbaraNanning#2018> ;
        :Involves      :AlešZvěřina , :BarbaraNanning ;
        :Located-In    :CzechRepublic ;
        :Part-Of       :Creation_Artwork_80 .

:ARTWORK_18_64_Packing_2
        a              owl:NamedIndividual , :Packing ;
        rdfs:comment   "Instance of an activity which is part of the creation process of ARTWORK_18_64."@en ;
        rdfs:label     "ARTWORK_18_64_Packing_2"@en ;
        :Followed-By   :ARTWORK_18_64_Transporting_2 ;
        :Follows       :ARTWORK_18_64_MeasuringAndBoxesMaking ;
        :Has-Duration  <http://www.semanticweb.org/ontologies/Daan/2020/BarbaraNanning#2015> ;
        :Involves      :BarbaraNanning ;
        :Located-In    :NovyBor ;
        :Part-Of       :Creation_Artwork_18_64 .

:Computer  a          :Equipment , owl:NamedIndividual ;
        rdfs:comment  "A Computer is an electronic device for storing and processing data."@en ;
        rdfs:label    "Computer"@en ;
        owl:sameAs    <http://vocab.getty.edu/aat/300024521> .

:ARTWORK_43_Glassblowing
        a                 :Glassblowing , owl:NamedIndividual ;
        rdfs:comment      "Instance of an activity which is part of the creation process of ARTWORK_43."@en ;
        rdfs:label        "ARTWORK_43_Glassblowing"@en ;
        :Followed-By      :ARTWORK_43_Sensing ;
        :Follows          :ARTWORK_43_HeatingMetalMold ;
        :Has-Duration     <http://www.semanticweb.org/ontologies/Daan/2020/BarbaraNanning#2008> ;
        :Involves         <http://www.semanticweb.org/ontologies/Daan/2020/BarbaraNanning#AlesVacek(CZ)> , :BarbaraNanning , <http://www.semanticweb.org/ontologies/Daan/2020/BarbaraNanning#RobertHlavacek(CZ)> , <http://www.semanticweb.org/ontologies/Daan/2020/BarbaraNanning#RostislavMaterka(CZ)> , <http://www.semanticweb.org/ontologies/Daan/2020/BarbaraNanning#RomanTomis(CZ)> , :AssistantOfBarbara ;
        :Located-In       :CzechRepublic ;
        :Part-Of          :Creation_Artwork_43 ;
        :Requires-Use-Of  :InterchangeableMetalMoldSetup , :IcePick , :Gloves , :Fork , :GloryHole , :BitIron , :DiamondShears , :PropaneTorch , :Pincet , :AnnealingKiln , :BlowingPipe , :Paper , :StraightShears , :Furnace , :Tagliol , :YokeOfSupport , :Water , :Blocks , :AirCompressor , :CeramicPotFilledWithGlass , :Jacks , :Marver , :Pontis , :Hook , :Beeswax .

:Organisation  a             owl:Class ;
        rdfs:comment         "An organisation is a group of people with a particular purpose or goal."@en ;
        rdfs:label           "Organisation"@en ;
        rdfs:subClassOf      :Actor ;
        owl:disjointWith     :Person ;
        owl:equivalentClass  <http://www.wikidata.org/entity/Q43229> .

:ARTWORK_36_TransportingColouredCanes_2
        a              owl:NamedIndividual , :Transporting_Coloured_Canes ;
        rdfs:comment   "Instance of an activity which is part of the creation process of ARTWORK_36."@en ;
        rdfs:label     "ARTWORK_36_Transporting Coloured Canes_2"@en ;
        :Followed-By   :ARTWORK_36_DecidingColourPalette ;
        :Follows       :ARTWORK_36_CuttingAndPolishingColouredCanes ;
        :Has-Duration  <http://www.semanticweb.org/ontologies/Daan/2020/BarbaraNanning#2015> ;
        :Involves      :BarbaraNanning , :AlešZvěřina ;
        :Located-In    :NovyBor ;
        :Part-Of       :Creation_Artwork_36 .

:ARTWORK_80_Packing_2
        a              owl:NamedIndividual , :Packing ;
        rdfs:comment   "Instance of an activity which is part of the creation process of ARTWORK_80."@en ;
        rdfs:label     "ARTWORK_80_Packing_2"@en ;
        :Followed-By   :ARTWORK_80_Transporting_2 ;
        :Follows       :ARTWORK_80_MeasuringAndBoxesMaking ;
        :Has-Duration  <http://www.semanticweb.org/ontologies/Daan/2020/BarbaraNanning#2018> ;
        :Involves      :AlešZvěřina , :BarbaraNanning ;
        :Located-In    :CzechRepublic ;
        :Part-Of       :Creation_Artwork_80 .

:ARTWORK_76_Translocating
        a                 owl:NamedIndividual , :Translocating ;
        rdfs:comment      "Instance of an activity which is part of the creation process of ARTWORK_76."@en ;
        rdfs:label        "ARTWORK_76_Translocating"@en ;
        :Followed-By      :ARTWORK_76_Cooling ;
        :Follows          <http://www.semanticweb.org/ontologies/Daan/2020/BarbaraNanning#ARTWORK_76_ExaminingQuality(Shape/Form)> ;
        :Has-Duration     <http://www.semanticweb.org/ontologies/Daan/2020/BarbaraNanning#2018> ;
        :Involves         :BarbaraNanning ;
        :Located-In       :CzechRepublic ;
        :Part-Of          :Creation_Artwork_76 ;
        :Requires-Use-Of  :Fork .

:ARTWORK_18_64_Sensing
        a              owl:NamedIndividual , :Sensing ;
        rdfs:comment   "Instance of an activity which is part of the creation process of ARTWORK_18_64."@en ;
        rdfs:label     "ARTWORK_18_64_Sensing"@en ;
        :Followed-By   :ARTWORK_18_64_Modeling ;
        :Follows       :ARTWORK_18_64_Glassblowing ;
        :Has-Duration  <http://www.semanticweb.org/ontologies/Daan/2020/BarbaraNanning#2015> ;
        :Involves      :BarbaraNanning ;
        :Located-In    :Zaandam ;
        :Part-Of       :Creation_Artwork_18_64 .

:Water  a             owl:NamedIndividual , :Equipment ;
        rdfs:comment  "Water is a colourless, transparent, odourless liquid that is the basis of the fluids of living organisms."@en ;
        rdfs:label    "Water"@en ;
        owl:sameAs    <http://www.wikidata.org/entity/Q283> ;
        :Used-For     :ARTWORK_75_ApplyingExtraColour_2 , :ARTWORK_79_Glassblowing , :ARTWORK_43_Glassblowing , :ARTWORK_80_ExaminingTheQualityOfTheGlass , :ARTWORK_78_Glassblowing , :ARTWORK_74_Glassblowing , :ARTWORK_74_ApplyingClearGlassBell , :ARTWORK_77_ExaminingTheQualityOfTheGlass , :ARTWORK_44_Glassblowing , :ARTWORK_80_ApplyingExtraColour , :ARTWORK_73_Glassblowing , :ARTWORK_75_ApplyingExtraColour , :ARTWORK_79_ApplyingExtraColour , :ARTWORK_80_ApplyingClearGlassBell , :ARTWORK_78_ExaminingTheQualityOfTheGlass , :ARTWORK_74_ExaminingTheQualityOfTheGlass , :ARTWORK_44_ApplyingExtraColour , :ARTWORK_74_ApplyingExtraColour_2 , :ARTWORK_44_ExaminingTheQualityOfTheGlass , :ARTWORK_77_ApplyingExtraColour , :ARTWORK_73_ExaminingTheQualityOfTheGlass , :ARTWORK_73_ApplyingClearGlassBell , :ARTWORK_75_Glassblowing , :ARTWORK_78_ApplyingClearGlassBell , :ARTWORK_79_ApplyingExtraColour_2 , :ARTWORK_75_ExaminingTheQualityOfTheGlass , :ARTWORK_79_ApplyingClearGlassBell , :ARTWORK_80_Glassblowing , :ARTWORK_77_ApplyingClearGlassBell , :ARTWORK_44_ApplyingExtraColour_2 , :ARTWORK_76_Glassblowing , :ARTWORK_74_ApplyingExtraColour , :ARTWORK_76_ApplyingExtraColour , :ARTWORK_43_ApplyingClearGlassBell , :ARTWORK_43_ExaminingTheQualityOfTheGlass , :ARTWORK_79_ExaminingTheQualityOfTheGlass , :ARTWORK_44_ApplyingClearGlassBell , :ARTWORK_78_ApplyingExtraColour , :ARTWORK_77_Glassblowing , :ARTWORK_76_ExaminingTheQualityOfTheGlass , :ARTWORK_76_ApplyingClearGlassBell , :ARTWORK_43_ApplyingExtraColour , :ARTWORK_76_ApplyingExtraColour_2 , :ARTWORK_75_ApplyingClearGlassBell .

:ARTWORK_36_Transporting_5
        a              owl:NamedIndividual , :Transporting ;
        rdfs:comment   "Instance of an activity which is part of the creation process of ARTWORK_36."@en ;
        rdfs:label     "ARTWORK_36_Transporting_5"@en ;
        :Followed-By   :ARTWORK_36_Signing_2 ;
        :Follows       :ARTWORK_36_Packing_6 ;
        :Has-Duration  <http://www.semanticweb.org/ontologies/Daan/2020/BarbaraNanning#2019> ;
        :Involves      :BarbaraNanning , :AlešZvěřina ;
        :Located-In    :NovyBor ;
        :Part-Of       :Creation_Artwork_36 .

:State-Of-Matter  a   owl:DatatypeProperty ;
        rdfs:comment  "State-Of-Matter is a property of a material which indicates the form of the substance (e.g. Solid, Liquid, Gas)."@en ;
        rdfs:domain   :Thing ;
        rdfs:label    "State-Of-Matter"@en ;
        rdfs:range    xsd:string .

j.2:    a                owl:Class ;
        rdfs:comment     "Examining Quality (Shape/Form) is an activity conducted by a creator in which the quality of the shape of an object is assured."@en ;
        rdfs:label       "Examining Quality (Shape/Form)"@en ;
        rdfs:subClassOf  :Activity .

<http://www.semanticweb.org/ontologies/Daan/2020/BarbaraNanning#ARTWORK_80_ExaminingQuality(Shape/Form)>
        a                 owl:NamedIndividual , j.2: ;
        rdfs:comment      "Instance of an activity which is part of the creation process of ARTWORK_80."@en ;
        rdfs:label        "ARTWORK_80_Examining Quality (Shape/Form)"@en ;
        :Followed-By      :ARTWORK_80_Translocating ;
        :Follows          :ARTWORK_80_Modeling ;
        :Has-Duration     <http://www.semanticweb.org/ontologies/Daan/2020/BarbaraNanning#2018> ;
        :Involves         :LuděkKout , <http://www.semanticweb.org/ontologies/Daan/2020/BarbaraNanning#RadekKoten(CZ)> , :BarbaraNanning ;
        :Located-In       :CzechRepublic ;
        :Part-Of          :Creation_Artwork_80 ;
        :Requires-Use-Of  :Pontis , :GloryHole , :BlowingPipe .

:ARTWORK_36_ApplyingMassivePieceOfClearGlass
        a                 owl:NamedIndividual , :Applying_Massive_Piece_of_Clear_Glass ;
        rdfs:comment      "Instance of an activity which is part of the creation process of ARTWORK_36."@en ;
        rdfs:label        "ARTWORK_36_Applying Massive Piece of Clear Glass"@en ;
        :Followed-By      :ARTWORK_36_PickingUpColouredPanel ;
        :Follows          :ARTWORK_36_ExaminingTheQualityOfTheGlass_2 ;
        :Has-Duration     <http://www.semanticweb.org/ontologies/Daan/2020/BarbaraNanning#2019> ;
        :Involves         :JiříPačinekJunior , :AlešZvěřina , :DavidČerný , :JaroslavKubásek , :BarbaraNanning , <http://www.semanticweb.org/ontologies/Daan/2020/BarbaraNanning#JessicaHomich(USA)> , :JanBaštýř , <http://www.semanticweb.org/ontologies/Daan/2020/BarbaraNanning#JiriPacinek(CZ)> ;
        :Located-In       :Lindava ;
        :Part-Of          :Creation_Artwork_36 ;
        :Requires-Use-Of  :AirCompressor , :Tagliol , :BlowingPipe , :Pontis , :Jacks , :IcePick , :Furnace , :Paper , :Hook , :Marver , :Blocks , :GloryHole , :Water , :StraightShears , :Beeswax , :YokeOfSupport , :DiamondShears .

:ARTWORK_77_HeatingMetalMold
        a                 :Heating_Metal_Mold , owl:NamedIndividual ;
        rdfs:comment      "Instance of an activity which is part of the creation process of ARTWORK_77."@en ;
        rdfs:label        "ARTWORK_77_Heating Metal Mold"@en ;
        :Followed-By      :ARTWORK_77_Glassblowing ;
        :Follows          :ARTWORK_77_ApplyingExtraColour ;
        :Has-Duration     <http://www.semanticweb.org/ontologies/Daan/2020/BarbaraNanning#2018> ;
        :Involves         :BarbaraNanning ;
        :Located-In       :CzechRepublic ;
        :Part-Of          :Creation_Artwork_77 ;
        :Requires-Use-Of  :PropaneTorch , :Gloves , :InterchangeableMetalMoldSetup .

:ARTWORK_36_ExaminingTheQualityOfTheGlass
        a                 :Examining_the_Quality_of_the_Glass , owl:NamedIndividual ;
        rdfs:comment      "Instance of an activity which is part of the creation process of ARTWORK_36."@en ;
        rdfs:label        "ARTWORK_36_Examining the Quality of the Glass"@en ;
        :Followed-By      :ARTWORK_36_ApplyingClearGlassBell ;
        :Follows          :ARTWORK_36_SetupAndTestingOfTheMetalMold ;
        :Has-Duration     <http://www.semanticweb.org/ontologies/Daan/2020/BarbaraNanning#2015> ;
        :Involves         :GertBullée , :BarbaraNanning , :DurkValkema ;
        :Located-In       :Zaandam ;
        :Part-Of          :Creation_Artwork_36 ;
        :Requires-Use-Of  :BlowingPipe , :StraightShears , :Pontis , :GloryHole , :CeramicPotFilledWithGlass , :DiamondShears , :Blocks , :Paper , :AnnealingKiln , :YokeOfSupport , :Furnace , :Water , :Jacks .

:ARTWORK_80_Transporting_3
        a              owl:NamedIndividual , :Transporting ;
        rdfs:comment   "Instance of an activity which is part of the creation process of ARTWORK_80."@en ;
        rdfs:label     "ARTWORK_80_Transporting_3"@en ;
        :Followed-By   :ARTWORK_80_Gilding ;
        :Follows       :ARTWORK_80_Packing_3 ;
        :Has-Duration  <http://www.semanticweb.org/ontologies/Daan/2020/BarbaraNanning#2018> ;
        :Involves      :BarbaraNanning , :AlešZvěřina ;
        :Located-In    :CzechRepublic ;
        :Part-Of       :Creation_Artwork_80 .

:Polishing  a            owl:Class ;
        rdfs:comment     "Polishing is an activity in which the surface of a thing is made smooth by rubbing."@en ;
        rdfs:label       "Polishing"@en ;
        rdfs:subClassOf  :Activity .

:Setup_and_Testing_of_the_Metal_Mold
        a                owl:Class ;
        rdfs:comment     "Setup and Testing of the Metal Mold Setup is an activity in which the glass blowing team tests the functioning of the Metal Mold Setup."@en ;
        rdfs:label       "Setup and Testing of the Metal Mold"@en ;
        rdfs:subClassOf  :Activity .

:ARTWORK_39_Packing_2
        a              owl:NamedIndividual , :Packing ;
        rdfs:comment   "Instance of an activity which is part of the creation process of ARTWORK_39."@en ;
        rdfs:label     "ARTWORK_39_Packing_2"@en ;
        :Followed-By   :ARTWORK_39_Transporting_2 ;
        :Follows       <http://www.semanticweb.org/ontologies/Daan/2020/BarbaraNanning#ARTWORK_39_ExaminingQuality(FinalResult)> ;
        :Has-Duration  <http://www.semanticweb.org/ontologies/Daan/2020/BarbaraNanning#2015> ;
        :Involves      :BarbaraNanning ;
        :Located-In    :NovyBor ;
        :Part-Of       :Creation_Artwork_39 .

:ARTWORK_78_Packing_4
        a              :Packing , owl:NamedIndividual ;
        rdfs:comment   "Instance of an activity which is part of the creation process of ARTWORK_78."@en ;
        rdfs:label     "ARTWORK_78_Packing_4"@en ;
        :Followed-By   :ARTWORK_78_Transporting_4 ;
        :Follows       <http://www.semanticweb.org/ontologies/Daan/2020/BarbaraNanning#ARTWORK_78_ExaminingQuality(FinalResult)> ;
        :Has-Duration  <http://www.semanticweb.org/ontologies/Daan/2020/BarbaraNanning#2008> ;
        :Involves      :BarbaraNanning , :VáçlavNovák_Doksy_CzechRepublic , :AlešZvěřina ;
        :Located-In    :CzechRepublic ;
        :Part-Of       :Creation_Artwork_78 .

:ARTWORK_46_CuttingStrings
        a                 owl:NamedIndividual , :Cutting_Strings ;
        rdfs:comment      "Instance of an activity which is part of the creation process of ARTWORK_46."@en ;
        rdfs:label        "ARTWORK_46_Cutting Strings"@en ;
        :Followed-By      :ARTWORK_46_MakingPatternsWithColouredCanesAndStringsInTheMetalBowl ;
        :Follows          :ARTWORK_46_TransportingColouredCanes ;
        :Has-Duration     <http://www.semanticweb.org/ontologies/Daan/2020/BarbaraNanning#2018> ;
        :Involves         :BarbaraNanning ;
        :Located-In       :Amsterdam ;
        :Part-Of          :Creation_Artwork_46 ;
        :Requires-Use-Of  :Glassscissors .

:FlatGlassheetWithColouredCanes
        a                     :Man-Made_Material , owl:NamedIndividual ;
        rdfs:comment          "Flat Glassheet with Coloured Canes is a Man-Made Material used by Barbara Nanning."@en ;
        rdfs:label            "Flat Glassheet with Coloured Canes"@en ;
        :Is-Processed-During  :ARTWORK_18_64_RoundingByGrindingTheSheet ;
        :Is-Processed-In      :Artwork_18_64 .

:ARTWORK_17_33_ApplyingClearOverlay
        a                 :Applying_Clear_Overlay , owl:NamedIndividual ;
        rdfs:comment      "Instance of an activity which is part of the creation process of ARTWORK_17_33."@en ;
        rdfs:label        "ARTWORK_17_33_Applying Clear Overlay"@en ;
        :Followed-By      :ARTWORK_17_33_Sensing ;
        :Follows          :ARTWORK_17_33_FillingHolesWithClearGlass ;
        :Has-Duration     <http://www.semanticweb.org/ontologies/Daan/2020/BarbaraNanning#2017> ;
        :Involves         <http://www.semanticweb.org/ontologies/Daan/2020/BarbaraNanning#LukasHavlas(CZ)> , <http://www.semanticweb.org/ontologies/Daan/2020/BarbaraNanning#JessicaHomich(USA)> , <http://www.semanticweb.org/ontologies/Daan/2020/BarbaraNanning#JiriMoravec(CZ)> , <http://www.semanticweb.org/ontologies/Daan/2020/BarbaraNanning#Tom%C3%A1%C5%A1Moravec(CZ)> , :BarbaraNanning , :AssistantOfBarbara , <http://www.semanticweb.org/ontologies/Daan/2020/BarbaraNanning#RadekKoten(CZ)> ;
        :Located-In       :Lindava ;
        :Part-Of          :Creation_Artwork_17_33 ;
        :Requires-Use-Of  :Marver , :Furnace , :Blocks , :BlowingPipe , :GrindingWheel , :Paper , :StraightShears , :Jacks , :YokeOfSupport , :DiamondShears , :AirCompressor , :Beeswax , :GloryHole , :Hook , :Water , :Tagliol .

<http://vocab.getty.edu/aat/300263648>
        a           owl:NamedIndividual ;
        owl:sameAs  :GildersKnife .

:ARTWORK_36_Sawing_2  a   owl:NamedIndividual , :Sawing ;
        rdfs:comment      "Instance of an activity which is part of the creation process of ARTWORK_36."@en ;
        rdfs:label        "ARTWORK_36_Sawing_2"@en ;
        :Followed-By      :ARTWORK_36_Sensing_4 ;
        :Follows          <http://www.semanticweb.org/ontologies/Daan/2020/BarbaraNanning#ARTWORK_36_ExaminingQuality(CheckForIrregularitiesInTheGlass)_2> ;
        :Has-Duration     <http://www.semanticweb.org/ontologies/Daan/2020/BarbaraNanning#2019> ;
        :Involves         :BarbaraNanning , :AlešZvěřina ;
        :Located-In       :NovyBor ;
        :Part-Of          :Creation_Artwork_36 ;
        :Requires-Use-Of  :DiamondSaw .

:ARTWORK_18_64_FusingSheets
        a                 :Fusing_Sheets , owl:NamedIndividual ;
        rdfs:comment      "Instance of an activity which is part of the creation process of ARTWORK_18_64."@en ;
        rdfs:label        "ARTWORK_18_64_Fusing Sheets"@en ;
        :Followed-By      :ARTWORK_18_64_CuttingStrings ;
        :Follows          :ARTWORK_18_64_OrdeningFlatSheets ;
        :Has-Duration     <http://www.semanticweb.org/ontologies/Daan/2020/BarbaraNanning#2015> ;
        :Involves         :BarbaraNanning ;
        :Located-In       :Amsterdam ;
        :Part-Of          :Creation_Artwork_18_64 ;
        :Requires-Use-Of  :FusingKiln .

<http://www.semanticweb.org/ontologies/Daan/2020/BarbaraNanning#RichardPrice(NL)>
        a             :First_Glass_Blower , owl:NamedIndividual ;
        rdfs:comment  "Richard Price (NL) is a First Glass Blower."@en ;
        rdfs:label    "Richard Price (NL)"@en ;
        :Involved-In  :ARTWORK_36_Glassblowing , :ARTWORK_39_Modeling , :ARTWORK_18_64_Modeling , :ARTWORK_39_PickingUpColouredPanel , :ARTWORK_18_64_Glassblowing , :ARTWORK_18_64_PickingUpColouredCanesPattern , :ARTWORK_39_Glassblowing , :ARTWORK_36_SetupAndTestingOfTheMetalMold , :ARTWORK_36_PickingUpColouredCanesPattern , :ARTWORK_39_SetupAndTestingOfTheMetalMold , :ARTWORK_36_ProducingColouredCanes , :ARTWORK_36_PickingUpColouredPanel , :ARTWORK_18_64_ProducingColouredCanes , :ARTWORK_46_ProducingColouredCanes , :ARTWORK_36_Modeling ;
        :Works-For    :GlassStudioVanTetterode .

<http://sws.geonames.org/2800866>
        a           owl:NamedIndividual ;
        owl:sameAs  :Brussels .

:AJETOWhiteGlass  a           owl:NamedIndividual , :AJETO_Glass ;
        rdfs:comment          "AJETO White is a form of AJETO glass with a white colour."@en ;
        rdfs:label            "AJETO White Glass"@en ;
        :Availability         "Available"@en ;
        :Is-Processed-During  :ARTWORK_79_ApplyingExtraColour ;
        :Is-Processed-In      :Artwork_79 ;
        :Made-By              :LASVITAJETO ;
        :Made-Out-Of          :Sand , :Potassium , :Soda , :Calcium , :BoneMeal ;
        :Transparency         "Opaque"@en .

:ARTWORK_36_TransportingMonochromeRods
        a              :Transporting_Monochrome_Rods , owl:NamedIndividual ;
        rdfs:comment   "Instance of an activity which is part of the creation process of ARTWORK_36."@en ;
        rdfs:label     "ARTWORK_36_Transporting Monochrome Rods"@en ;
        :Followed-By   :ARTWORK_36_ProducingColouredCanes ;
        :Follows       :ARTWORK_36_DecidingColourPaletteAndPatterns_2 ;
        :Has-Duration  <http://www.semanticweb.org/ontologies/Daan/2020/BarbaraNanning#2015> ;
        :Involves      <http://www.semanticweb.org/ontologies/Daan/2020/BarbaraNanning#JaroslavSvacha(CZ)> , :BarbaraNanning ;
        :Located-In    :Langweer ;
        :Part-Of       :Creation_Artwork_36 .

:Made-Out-Of  a       owl:ObjectProperty ;
        rdfs:comment  "Made-Out-Of is a property which connects an entity with the material it is created from."@en ;
        rdfs:domain   :Entity ;
        rdfs:label    "Made-Out-Of"@en ;
        rdfs:range    :Material .

<http://www.cidoc-crm.org/cidoc-crm/P109_is_current_or_former_curator_of>
        a                       owl:ObjectProperty ;
        owl:equivalentProperty  :Maintained-By .

<http://www.semanticweb.org/ontologies/Daan/2020/BarbaraNanning#RobertHlavacek(CZ)>
        a             owl:NamedIndividual , :Second_Glass_Blower ;
        rdfs:comment  "Robert Hlavacek (CZ) is a Second Glass Blower."@en ;
        rdfs:label    "Robert Hlavacek (CZ)"@en ;
        :Involved-In  :ARTWORK_74_Glassblowing , :ARTWORK_74_SetupAndTestingOfTheMetalMold_2 , :ARTWORK_43_Modeling , :ARTWORK_43_SetupAndTestingOfTheMetalMold , :ARTWORK_78_Glassblowing , :ARTWORK_78_Modeling , :ARTWORK_78_SetupAndTestingOfTheMetalMold , :ARTWORK_78_SetupAndTestingOfTheMetalMold_2 , :ARTWORK_43_SetupAndTestingOfTheMetalMold_2 , :ARTWORK_43_Glassblowing , :ARTWORK_74_SetupAndTestingOfTheMetalMold , :ARTWORK_74_Modeling ;
        :Works-For    :LASVITAJETO .

:ARTWORK_44_Packing  a  :Packing , owl:NamedIndividual ;
        rdfs:comment   "Instance of an activity which is part of the creation process of ARTWORK_44."@en ;
        rdfs:label     "ARTWORK_44_Packing"@en ;
        :Followed-By   :ARTWORK_44_Transporting ;
        :Follows       :ARTWORK_44_Cooling ;
        :Has-Duration  <http://www.semanticweb.org/ontologies/Daan/2020/BarbaraNanning#2018> ;
        :Involves      :AlešZvěřina , :BarbaraNanning ;
        :Located-In    :CzechRepublic ;
        :Part-Of       :Creation_Artwork_44 .

:Blocks  a            :Equipment , owl:NamedIndividual ;
        rdfs:comment  "A block is a large solid piece made out of hard material."@en ;
        rdfs:label    "Blocks"@en ;
        :Used-For     :ARTWORK_74_ApplyingClearGlassBell , :ARTWORK_44_ApplyingClearGlassBell , :ARTWORK_79_ApplyingClearGlassBell , :ARTWORK_75_ExaminingTheQualityOfTheGlass , :ARTWORK_75_ApplyingExtraColour_2 , :ARTWORK_76_ExaminingTheQualityOfTheGlass , :ARTWORK_75_Glassblowing , :ARTWORK_78_ExaminingTheQualityOfTheGlass , :ARTWORK_77_ApplyingExtraColour , :ARTWORK_73_ExaminingTheQualityOfTheGlass , :ARTWORK_79_ApplyingExtraColour , :ARTWORK_73_Glassblowing , :ARTWORK_77_ExaminingTheQualityOfTheGlass , :ARTWORK_75_ApplyingExtraColour , :ARTWORK_43_ApplyingClearGlassBell , :ARTWORK_76_ApplyingExtraColour , :ARTWORK_78_ApplyingClearGlassBell , :ARTWORK_80_Glassblowing , :ARTWORK_78_ApplyingExtraColour , :ARTWORK_77_ApplyingClearGlassBell , :ARTWORK_43_Glassblowing , :ARTWORK_78_Glassblowing , :ARTWORK_76_ApplyingClearGlassBell , :ARTWORK_79_ApplyingExtraColour_2 , :ARTWORK_44_ApplyingExtraColour_2 , :ARTWORK_77_Glassblowing , :ARTWORK_79_ExaminingTheQualityOfTheGlass , :ARTWORK_73_ApplyingClearGlassBell , :ARTWORK_44_ApplyingExtraColour , :ARTWORK_74_ApplyingExtraColour , :ARTWORK_74_Glassblowing , :ARTWORK_79_Glassblowing , :ARTWORK_76_Glassblowing , :ARTWORK_76_ApplyingExtraColour_2 , :ARTWORK_43_ApplyingExtraColour , :ARTWORK_75_ApplyingClearGlassBell , :ARTWORK_44_ExaminingTheQualityOfTheGlass , :ARTWORK_80_ApplyingExtraColour , :ARTWORK_44_Glassblowing , :ARTWORK_80_ExaminingTheQualityOfTheGlass , :ARTWORK_80_ApplyingClearGlassBell , :ARTWORK_74_ApplyingExtraColour_2 , :ARTWORK_74_ExaminingTheQualityOfTheGlass , :ARTWORK_43_ExaminingTheQualityOfTheGlass .

<http://www.semanticweb.org/ontologies/Daan/2020/BarbaraNanning#ARTWORK_79_ExaminingQuality(FinalResult)>
        a              owl:NamedIndividual , j.1: ;
        rdfs:comment   "Instance of an activity which is part of the creation process of ARTWORK_79."@en ;
        rdfs:label     "ARTWORK_79_Examining Quality (Final Result)"@en ;
        :Followed-By   :ARTWORK_79_Packing_5 ;
        :Follows       :ARTWORK_79_Gilding ;
        :Has-Duration  <http://www.semanticweb.org/ontologies/Daan/2020/BarbaraNanning#2018> ;
        :Involves      :AlešZvěřina , :BarbaraNanning ;
        :Located-In    :CzechRepublic ;
        :Part-Of       :Creation_Artwork_79 .

:ARTWORK_17_33_Polishing
        a                 :Polishing , owl:NamedIndividual ;
        rdfs:comment      "Instance of an activity which is part of the creation process of ARTWORK_17_33."@en ;
        rdfs:label        "ARTWORK_17_33_Polishing"@en ;
        :Followed-By      :ARTWORK_17_33_Signing ;
        :Follows          :ARTWORK_17_33_Grinding ;
        :Has-Duration     <http://www.semanticweb.org/ontologies/Daan/2020/BarbaraNanning#2017> ;
        :Involves         :BarbaraNanning , :AlešZvěřina , :LukášSvoboda ;
        :Located-In       :NovyBor ;
        :Part-Of          :Creation_Artwork_17_33 ;
        :Requires-Use-Of  :PolishingStone .

:ARTWORK_46_Sensing  a  owl:NamedIndividual , :Sensing ;
        rdfs:comment   "Instance of an activity which is part of the creation process of ARTWORK_46."@en ;
        rdfs:label     "ARTWORK_46_Sensing"@en ;
        :Followed-By   :ARTWORK_46_Modeling ;
        :Follows       :ARTWORK_46_Glassblowing ;
        :Has-Duration  <http://www.semanticweb.org/ontologies/Daan/2020/BarbaraNanning#2018> ;
        :Involves      <http://www.semanticweb.org/ontologies/Daan/2020/BarbaraNanning#JiriPacinek(CZ)> , :BarbaraNanning ;
        :Located-In    :Lindava ;
        :Part-Of       :Creation_Artwork_46 .

:ARTWORK_79_Transporting_3
        a              owl:NamedIndividual , :Transporting ;
        rdfs:comment   "Instance of an activity which is part of the creation process of ARTWORK_79."@en ;
        rdfs:label     "ARTWORK_79_Transporting_3"@en ;
        :Followed-By   :ARTWORK_79_Gilding ;
        :Follows       :ARTWORK_79_Packing_3 ;
        :Has-Duration  <http://www.semanticweb.org/ontologies/Daan/2020/BarbaraNanning#2018> ;
        :Involves      :AlešZvěřina , :BarbaraNanning ;
        :Located-In    :CzechRepublic ;
        :Part-Of       :Creation_Artwork_79 .

:DiamondShears  a     owl:NamedIndividual , :Tool ;
        rdfs:comment  "Diamond Shears are shears with a cutting area shaped like a diamond."@en ;
        rdfs:label    "Diamond Shears"@en ;
        :Used-For     :ARTWORK_44_Glassblowing , :ARTWORK_74_Glassblowing , :ARTWORK_79_ApplyingClearGlassBell , :ARTWORK_80_ExaminingTheQualityOfTheGlass , :ARTWORK_73_Glassblowing , :ARTWORK_75_Glassblowing , :ARTWORK_43_ApplyingExtraColour , :ARTWORK_76_Glassblowing , :ARTWORK_80_ApplyingClearGlassBell , :ARTWORK_75_ExaminingTheQualityOfTheGlass , :ARTWORK_73_ApplyingClearGlassBell , :ARTWORK_43_ExaminingTheQualityOfTheGlass , :ARTWORK_43_ApplyingClearGlassBell , :ARTWORK_74_ApplyingExtraColour , :ARTWORK_76_ExaminingTheQualityOfTheGlass , :ARTWORK_79_ApplyingExtraColour_2 , :ARTWORK_74_ExaminingTheQualityOfTheGlass , :ARTWORK_76_ApplyingExtraColour_2 , :ARTWORK_73_ExaminingTheQualityOfTheGlass , :ARTWORK_80_Glassblowing , :ARTWORK_78_Glassblowing , :ARTWORK_77_ExaminingTheQualityOfTheGlass , :ARTWORK_80_ApplyingExtraColour , :ARTWORK_75_ApplyingExtraColour , :ARTWORK_79_Glassblowing , :ARTWORK_78_ApplyingClearGlassBell , :ARTWORK_44_ApplyingExtraColour_2 , :ARTWORK_44_ApplyingClearGlassBell , :ARTWORK_75_ApplyingClearGlassBell , :ARTWORK_77_Glassblowing , :ARTWORK_78_ApplyingExtraColour , :ARTWORK_79_ApplyingExtraColour , :ARTWORK_43_Glassblowing , :ARTWORK_78_ExaminingTheQualityOfTheGlass , :ARTWORK_44_ApplyingExtraColour , :ARTWORK_76_ApplyingClearGlassBell , :ARTWORK_74_ApplyingClearGlassBell , :ARTWORK_77_ApplyingClearGlassBell , :ARTWORK_74_ApplyingExtraColour_2 , :ARTWORK_76_ApplyingExtraColour , :ARTWORK_77_ApplyingExtraColour , :ARTWORK_44_ExaminingTheQualityOfTheGlass , :ARTWORK_79_ExaminingTheQualityOfTheGlass , :ARTWORK_75_ApplyingExtraColour_2 .

:Sandblasting  a         owl:Class ;
        rdfs:comment     "Sandblasting is an activity in which a jet of sand cleans and roughen the surface of a thing."@en ;
        rdfs:label       "Sandblasting"@en ;
        rdfs:subClassOf  :Activity .

:ARTWORK_46_Sensing_2
        a              :Sensing , owl:NamedIndividual ;
        rdfs:comment   "Instance of an activity which is part of the creation process of ARTWORK_46."@en ;
        rdfs:label     "ARTWORK_46_Sensing_2"@en ;
        :Followed-By   :ARTWORK_46_Grinding ;
        :Follows       :ARTWORK_46_Sawing ;
        :Has-Duration  <http://www.semanticweb.org/ontologies/Daan/2020/BarbaraNanning#2018> ;
        :Involves      :LukášSvoboda , :BarbaraNanning , :AlešZvěřina ;
        :Located-In    :NovyBor ;
        :Part-Of       :Creation_Artwork_46 .

:ARTWORK_46_ApplyingClearGlassBell
        a                 owl:NamedIndividual , :Applying_Clear_Glass_Bell ;
        rdfs:comment      "Instance of an activity which is part of the creation process of ARTWORK_46."@en ;
        rdfs:label        "ARTWORK_46_Applying Clear Glass Bell"@en ;
        :Followed-By      :ARTWORK_46_PickingUpColouredCanesPattern ;
        :Follows          :ARTWORK_46_ExaminingTheQualityOfTheGlass ;
        :Has-Duration     <http://www.semanticweb.org/ontologies/Daan/2020/BarbaraNanning#2018> ;
        :Involves         <http://www.semanticweb.org/ontologies/Daan/2020/BarbaraNanning#JiriPacinek(CZ)> , :BarbaraNanning , :DavidČerný ;
        :Located-In       :Lindava ;
        :Part-Of          :Creation_Artwork_46 ;
        :Requires-Use-Of  :Marver , :Jacks , :CeramicPotFilledWithGlass , :BlowingPipe , :Beeswax , :YokeOfSupport , :Pincet , :AirCompressor , :StraightShears , :Paper , :Blocks , :Hook , :IcePick , :DiamondShears , :Water , :Furnace .

:ARTWORK_75_Grinding  a   owl:NamedIndividual , :Grinding ;
        rdfs:comment      "Instance of an activity which is part of the creation process of ARTWORK_75."@en ;
        rdfs:label        "ARTWORK_75_Grinding"@en ;
        :Followed-By      :ARTWORK_75_Polishing ;
        :Follows          :ARTWORK_75_Sawing ;
        :Has-Duration     <http://www.semanticweb.org/ontologies/Daan/2020/BarbaraNanning#2018> ;
        :Involves         :AlešZvěřina , :RobertFlorian , :BarbaraNanning ;
        :Located-In       :CzechRepublic ;
        :Part-Of          :Creation_Artwork_75 ;
        :Requires-Use-Of  :GrindingWheel , :SharpeningStone .

:ARTWORK_18_64_DecoratingTheSheetWithColouredCanes
        a                 :Decorating_the_Sheet_with_Coloured_Canes , owl:NamedIndividual ;
        rdfs:comment      "Instance of an activity which is part of the creation process of ARTWORK_18_64."@en ;
        rdfs:label        "ARTWORK_18_64_Decorating the Sheet with Coloured Canes"@en ;
        :Followed-By      :ARTWORK_18_64_FusingSheetsAndStrings ;
        :Follows          :ARTWORK_18_64_CuttingStrings ;
        :Has-Duration     <http://www.semanticweb.org/ontologies/Daan/2020/BarbaraNanning#2015> ;
        :Involves         :BarbaraNanning ;
        :Located-In       :Amsterdam ;
        :Part-Of          :Creation_Artwork_18_64 ;
        :Requires-Use-Of  :Glassscissors , :FusingKiln , :Pincet .

:Finishes  a           owl:ObjectProperty ;
        rdfs:comment   "Finishes is a property which indicates the sub-event which ends an event."@en ;
        rdfs:domain    :Event ;
        rdfs:label     "Finishes"@en ;
        rdfs:range     :Event ;
        owl:inverseOf  :Finishes-With .

:Preparing_for_Blowing
        a                owl:Class ;
        rdfs:comment     "Ensuring that the Studio and furnaces are prepared, pipes and all the colours are pre-heated for the days production."@en ;
        rdfs:label       "Preparing for Blowing"@en ;
        rdfs:subClassOf  :Activity .

:ARTWORK_46_Documenting
        a              owl:NamedIndividual , :Documenting ;
        rdfs:comment   "Instance of an activity which is part of the creation process of ARTWORK_46."@en ;
        rdfs:label     "ARTWORK_46_Documenting"@en ;
        :Finishes      :Creation_Artwork_46 ;
        :Follows       :ARTWORK_46_Packing_3 ;
        :Has-Duration  <http://www.semanticweb.org/ontologies/Daan/2020/BarbaraNanning#2018> ;
        :Involves      :BarbaraNanning ;
        :Located-In    :Amsterdam ;
        :Part-Of       :Creation_Artwork_46 .

:ARTWORK_73_Packing_4
        a              owl:NamedIndividual , :Packing ;
        rdfs:comment   "Instance of an activity which is part of the creation process of ARTWORK_73."@en ;
        rdfs:label     "ARTWORK_73_Packing_4"@en ;
        :Followed-By   :ARTWORK_73_Transporting_4 ;
        :Follows       <http://www.semanticweb.org/ontologies/Daan/2020/BarbaraNanning#ARTWORK_73_ExaminingQuality(FinalResult)> ;
        :Has-Duration  <http://www.semanticweb.org/ontologies/Daan/2020/BarbaraNanning#2018> ;
        :Involves      :VáçlavNovák_Doksy_CzechRepublic , :BarbaraNanning , :AlešZvěřina ;
        :Located-In    :CzechRepublic ;
        :Part-Of       :Creation_Artwork_73 .

:ARTWORK_44_Packing_2
        a              owl:NamedIndividual , :Packing ;
        rdfs:comment   "Instance of an activity which is part of the creation process of ARTWORK_44."@en ;
        rdfs:label     "ARTWORK_44_Packing_2"@en ;
        :Followed-By   :ARTWORK_44_Transporting_2 ;
        :Follows       :ARTWORK_44_MeasuringAndBoxesMaking ;
        :Has-Duration  <http://www.semanticweb.org/ontologies/Daan/2020/BarbaraNanning#2018> ;
        :Involves      :AlešZvěřina , :BarbaraNanning ;
        :Located-In    :CzechRepublic ;
        :Part-Of       :Creation_Artwork_44 .

:ARTWORK_36_Resting  a    owl:NamedIndividual , :Resting ;
        rdfs:comment      "Instance of an activity which is part of the creation process of ARTWORK_36."@en ;
        rdfs:label        "ARTWORK_36_Resting"@en ;
        :Followed-By      <http://www.semanticweb.org/ontologies/Daan/2020/BarbaraNanning#ARTWORK_36_ExaminingQuality(CheckForIrregularitiesInTheGlass)> ;
        :Follows          :ARTWORK_36_Transporting ;
        :Has-Duration     <http://www.semanticweb.org/ontologies/Daan/2020/BarbaraNanning#2015> ;
        :Involves         :AlešZvěřina ;
        :Located-In       :NovyBor ;
        :Part-Of          :Creation_Artwork_36 ;
        :Requires-Use-Of  :AnnealingKiln .

:ARTWORK_18_64_Transporting
        a              owl:NamedIndividual , :Transporting ;
        rdfs:comment   "Instance of an activity which is part of the creation process of ARTWORK_18_64."@en ;
        rdfs:label     "ARTWORK_18_64_Transporting"@en ;
        :Followed-By   :ARTWORK_18_64_Resting ;
        :Follows       :ARTWORK_18_64_Packing ;
        :Has-Duration  <http://www.semanticweb.org/ontologies/Daan/2020/BarbaraNanning#2015> ;
        :Involves      :AlešZvěřina , :BarbaraNanning ;
        :Located-In    :NovyBor ;
        :Part-Of       :Creation_Artwork_18_64 .

:Metal_Worker  a         owl:Class ;
        rdfs:comment     "A Metal Worker is an actor who is responsible for creating metal objects or dealing with metal material."@en ;
        rdfs:label       "Metal Worker"@en ;
        rdfs:subClassOf  :Person .

<http://www.wikidata.org/entity/Q72451031>
        a       owl:NamedIndividual .

:ARTWORK_36_Sensing_3
        a              :Sensing , owl:NamedIndividual ;
        rdfs:comment   "Instance of an activity which is part of the creation process of ARTWORK_36."@en ;
        rdfs:label     "ARTWORK_36_Sensing_3"@en ;
        :Followed-By   :ARTWORK_36_Modeling_2 ;
        :Follows       :ARTWORK_36_PickingUpColouredPanel ;
        :Has-Duration  <http://www.semanticweb.org/ontologies/Daan/2020/BarbaraNanning#2019> ;
        :Involves      :BarbaraNanning ;
        :Located-In    :Lindava ;
        :Part-Of       :Creation_Artwork_36 .

:ARTWORK_39_PreparingGlass
        a                 :Preparing_Glass , owl:NamedIndividual ;
        rdfs:comment      "Instance of an activity which is part of the creation process of ARTWORK_39."@en ;
        rdfs:label        "ARTWORK_39_Preparing Glass"@en ;
        :Followed-By      :ARTWORK_39_SetupAndTestingOfTheMetalMold ;
        :Follows          :ARTWORK_39_FillingKilnsWithMetalBowl ;
        :Has-Duration     <http://www.semanticweb.org/ontologies/Daan/2020/BarbaraNanning#2015> ;
        :Involves         :BarbaraNanning , <http://www.semanticweb.org/ontologies/Daan/2020/BarbaraNanning#MiaLerssi(DN)> , :GertBullée ;
        :Located-In       :Zaandam ;
        :Part-Of          :Creation_Artwork_39 ;
        :Requires-Use-Of  :Pontis , :BlowingPipe , :Garage , :Marver , :GloryHole .

:ARTWORK_43_Packing_5
        a              :Packing , owl:NamedIndividual ;
        rdfs:comment   "Instance of an activity which is part of the creation process of ARTWORK_43."@en ;
        rdfs:label     "ARTWORK_43_Packing_5"@en ;
        :Finishes      :Creation_Artwork_43 ;
        :Follows       :ARTWORK_43_Documenting ;
        :Has-Duration  <http://www.semanticweb.org/ontologies/Daan/2020/BarbaraNanning#2008> ;
        :Involves      :BarbaraNanning ;
        :Located-In    :CzechRepublic ;
        :Part-Of       :Creation_Artwork_43 .

<http://www.wikidata.org/entity/Q33506>
        a       owl:Class .

:ARTWORK_80_SetupAndTestingOfTheMetalMold
        a                 :Setup_and_Testing_of_the_Metal_Mold , owl:NamedIndividual ;
        rdfs:comment      "Instance of an activity which is part of the creation process of ARTWORK_80."@en ;
        rdfs:label        "ARTWORK_80_Setup and Testing of the Metal Mold"@en ;
        :Followed-By      :ARTWORK_80_ExaminingTheQualityOfTheGlass ;
        :Follows          :ARTWORK_80_PreparingGlass ;
        :Has-Duration     <http://www.semanticweb.org/ontologies/Daan/2020/BarbaraNanning#2018> ;
        :Involves         :BarbaraNanning , <http://www.semanticweb.org/ontologies/Daan/2020/BarbaraNanning#LukasHavlas(CZ)> , <http://www.semanticweb.org/ontologies/Daan/2020/BarbaraNanning#JiriMoravec(CZ)> , <http://www.semanticweb.org/ontologies/Daan/2020/BarbaraNanning#RadekKoten(CZ)> , <http://www.semanticweb.org/ontologies/Daan/2020/BarbaraNanning#Tom%C3%A1%C5%A1Moravec(CZ)> , :AssistantOfBarbara ;
        :Located-In       :CzechRepublic ;
        :Part-Of          :Creation_Artwork_80 ;
        :Requires-Use-Of  :InterchangeableMetalMoldSetup .

:Doksy  a             :City , owl:NamedIndividual ;
        rdfs:comment  "Doksy is a city in Czech Republic"@en ;
        rdfs:label    "Doksy"@en ;
        owl:sameAs    <http://www.wikidata.org/entity/Q1021090> ;
        :Located-In   :CzechRepublic .

<http://www.semanticweb.org/ontologies/Daan/2020/BarbaraNanning#Ale%C5%A1Zv%C4%9B%C5%99ina&AZ-Design>
        a             :Glass_Studio , owl:NamedIndividual ;
        rdfs:comment  "Aleš Zvěřina-AZ.design.cz is a glass studio in Nový Bor (CZ) where Aleš Zvěřina is a glass glass cutter and designer."@en ;
        rdfs:label    "Aleš Zvěřina & AZ-Design"@en ;
        :Employed     :RobertFlorian , :AlešZvěřina , :LenkaUhlířová , :LukášSvoboda ;
        :Located-In   :NovyBor ;
        :Maker-Of     :Artwork_77 , :Artwork_43 , :Artwork_75 , :Artwork_79 , :Artwork_76 , :Artwork_74 , :Artwork_78 , :Artwork_44 , :Artwork_80 , :Artwork_73 .

:Switzerland  a       :Country , owl:NamedIndividual ;
        rdfs:comment  "Switzerland is a country in western Europe."@en ;
        rdfs:label    "Switzerland"@en ;
        owl:sameAs    <http://www.wikidata.org/entity/Q39> ;
        :Location-Of  :Lausanne .

:Tool   a                owl:NamedIndividual , owl:Class ;
        rdfs:comment     "A device to be held in the hand(s) of an actor with a specific function."@en ;
        rdfs:label       "Tool"@en ;
        rdfs:subClassOf  :Equipment .

:Grinder_4  a            owl:Class ;
        rdfs:comment     "A Grinder 4 is an actor who is the third member of a team responsible for the grinding, polishing and sharpening of objects."@en ;
        rdfs:label       "Grinder 4"@en ;
        rdfs:subClassOf  :Grinder .

:ARTWORK_78_ExaminingTheQualityOfTheGlass
        a                 owl:NamedIndividual , :Examining_the_Quality_of_the_Glass ;
        rdfs:comment      "Instance of an activity which is part of the creation process of ARTWORK_78."@en ;
        rdfs:label        "ARTWORK_78_Examining the Quality of the Glass"@en ;
        :Followed-By      :ARTWORK_78_Cooling ;
        :Follows          :ARTWORK_78_Modeling ;
        :Has-Duration     <http://www.semanticweb.org/ontologies/Daan/2020/BarbaraNanning#2016> ;
        :Involves         :LuděkKout , :BarbaraNanning , <http://www.semanticweb.org/ontologies/Daan/2020/BarbaraNanning#AlesVacek(CZ)> ;
        :Located-In       :CzechRepublic ;
        :Part-Of          :Creation_Artwork_78 ;
        :Requires-Use-Of  :YokeOfSupport , :CeramicPotFilledWithGlass , :GloryHole , :AnnealingKiln , :Blocks , :BlowingPipe , :Jacks , :Water , :Furnace , :StraightShears , :Pontis , :DiamondShears , :Paper .

:JanBaštýř  a         :Second_Glass_Blower , owl:NamedIndividual ;
        rdfs:comment  "Jan Baštýř is a Second Glass Blower."@en ;
        rdfs:label    "Jan Baštýř"@en ;
        :Involved-In  :ARTWORK_46_Modeling , :ARTWORK_46_ApplyingClearOverlay , :ARTWORK_46_PickingUpColouredCanesPattern , :ARTWORK_36_Modeling_2 , :ARTWORK_46_SetupAndTestingOfTheMetalMold , :ARTWORK_46_Glassblowing , :ARTWORK_36_ApplyingMassivePieceOfClearGlass ;
        :Works-For    <http://www.semanticweb.org/ontologies/Daan/2020/BarbaraNanning#Ji%C5%99%C3%ADPa%C4%8DinekLindava(CZ)> .

<http://www.semanticweb.org/ontologies/Daan/2020/BarbaraNanning#ARTWORK_43_ExaminingQuality(CheckForIrregularitiesInTheGlass)>
        a              owl:NamedIndividual , j.3: ;
        rdfs:comment   "Instance of an activity which is part of the creation process of ARTWORK_43."@en ;
        rdfs:label     "ARTWORK_43_Examining Quality (Check for Irregularities in the Glass)"@en ;
        :Followed-By   :ARTWORK_43_Sawing ;
        :Follows       :ARTWORK_43_Resting ;
        :Has-Duration  <http://www.semanticweb.org/ontologies/Daan/2020/BarbaraNanning#2008> ;
        :Involves      :BarbaraNanning , :AlešZvěřina ;
        :Located-In    :CzechRepublic ;
        :Part-Of       :Creation_Artwork_43 .

:Sand   a                 :Natural_Material , owl:NamedIndividual ;
        rdfs:comment      "Sand is a granular material consisting of rock and mineral particles."@en ;
        rdfs:label        "Sand"@en ;
        owl:sameAs        <http://www.wikidata.org/entity/Q34679> ;
        :Is-Processed-In  :AJETOSmokeGlass , :AJETOAmberGlass , :AJETOBlackGlass , :AJETOWhiteGlass , :AJETOBlueGlass , :AJETOClearGlass , :AJETORedGlass , :AJETOGreenGlass .

:Actor  a                owl:Class ;
        rdfs:comment     "An actor is a potential participant of an event."@en ;
        rdfs:label       "Actor"@en ;
        rdfs:subClassOf  :Entity .

:ARTWORK_17_33_CuttingAndPolishingColouredCanes
        a                 :Cutting_and_Polishing_Coloured_Canes , owl:NamedIndividual ;
        rdfs:comment      "Instance of an activity which is part of the creation process of ARTWORK_17_33."@en ;
        rdfs:label        "ARTWORK_17_33_Cutting and Polishing Coloured Canes"@en ;
        :Followed-By      :ARTWORK_17_33_TransportingColouredCanes_2 ;
        :Follows          :ARTWORK_17_33_TransportingColouredCanes ;
        :Has-Duration     <http://www.semanticweb.org/ontologies/Daan/2020/BarbaraNanning#2017> ;
        :Involves         :AlešZvěřina , :RobertFlorian , :BarbaraNanning ;
        :Located-In       :NovyBor ;
        :Part-Of          :Creation_Artwork_17_33 ;
        :Requires-Use-Of  :DiamondSaw , :Glassscissors , :Water , :SharpeningStone .

:Fusing_Sheets_and_Strings
        a                owl:Class ;
        rdfs:comment     "Flat glass and thin pulled strings that can be cut into various shapes to create a specific design."@en ;
        rdfs:label       "Fusing Sheets and Strings"@en ;
        rdfs:subClassOf  :Activity .

:Event  a                owl:Class ;
        rdfs:comment     "An event is something that happens at a time and place."@en ;
        rdfs:label       "Event"@en ;
        rdfs:subClassOf  :Period .

:ARTWORK_36_Documenting
        a              :Documenting , owl:NamedIndividual ;
        rdfs:comment   "Instance of an activity which is part of the creation process of ARTWORK_36."@en ;
        rdfs:label     "ARTWORK_36_Documenting"@en ;
        :Followed-By   :ARTWORK_36_FlatFusingFinishedArtwork ;
        :Follows       :ARTWORK_36_Packing_4 ;
        :Has-Duration  <http://www.semanticweb.org/ontologies/Daan/2020/BarbaraNanning#2019> ;
        :Involves      :BarbaraNanning ;
        :Located-In    :Amsterdam ;
        :Part-Of       :Creation_Artwork_36 .

:ARTWORK_79_Glassblowing
        a                 :Glassblowing , owl:NamedIndividual ;
        rdfs:comment      "Instance of an activity which is part of the creation process of ARTWORK_79."@en ;
        rdfs:label        "ARTWORK_79_Glassblowing"@en ;
        :Followed-By      :ARTWORK_79_Sensing ;
        :Follows          :ARTWORK_79_HeatingMetalMold ;
        :Has-Duration     <http://www.semanticweb.org/ontologies/Daan/2020/BarbaraNanning#2018> ;
        :Involves         <http://www.semanticweb.org/ontologies/Daan/2020/BarbaraNanning#LukasHavlas(CZ)> , :BarbaraNanning , :AssistantOfBarbara , <http://www.semanticweb.org/ontologies/Daan/2020/BarbaraNanning#Tom%C3%A1%C5%A1Moravec(CZ)> , <http://www.semanticweb.org/ontologies/Daan/2020/BarbaraNanning#JiriMoravec(CZ)> , <http://www.semanticweb.org/ontologies/Daan/2020/BarbaraNanning#RadekKoten(CZ)> ;
        :Located-In       :CzechRepublic ;
        :Part-Of          :Creation_Artwork_79 ;
        :Requires-Use-Of  :GloryHole , :Gloves , :BlowingPipe , :Hook , :Beeswax , :Fork , :Water , :DiamondShears , :PropaneTorch , :Tagliol , :InterchangeableMetalMoldSetup , :Pontis , :Marver , :Paper , :AirCompressor , :YokeOfSupport , :IcePick , :StraightShears , :Furnace , :AnnealingKiln , :Jacks , :Pincet , :CeramicPotFilledWithGlass , :BitIron , :Blocks .

:ARTWORK_18_64_Grinding_Facets
        a                 owl:NamedIndividual , :Grinding_Facets ;
        rdfs:comment      "Instance of an activity which is part of the creation process of ARTWORK_18_64."@en ;
        rdfs:label        "ARTWORK_18_64_Grinding_Facets"@en ;
        :Followed-By      :ARTWORK_18_64_Polishing ;
        :Follows          :ARTWORK_18_64_Grinding ;
        :Has-Duration     <http://www.semanticweb.org/ontologies/Daan/2020/BarbaraNanning#2015> ;
        :Involves         :AlešZvěřina , :RobertFlorian , :BarbaraNanning ;
        :Located-In       :NovyBor ;
        :Part-Of          :Creation_Artwork_18_64 ;
        :Requires-Use-Of  :SharpeningStone , :GrindingWheel .

:ARTWORK_17_33_TransportingMetalBowlWithCanes
        a              owl:NamedIndividual , :Transporting_Metal_Bowl_with_Canes ;
        rdfs:comment   "Instance of an activity which is part of the creation process of ARTWORK_17_33."@en ;
        rdfs:label     "ARTWORK_17_33_Transporting Metal Bowl with Canes"@en ;
        :Followed-By   :ARTWORK_17_33_PreparingForBlowing ;
        :Follows       :ARTWORK_17_33_TackfusingColouredCanes ;
        :Has-Duration  <http://www.semanticweb.org/ontologies/Daan/2020/BarbaraNanning#2017> ;
        :Involves      :BarbaraNanning ;
        :Located-In    :Lindava ;
        :Part-Of       :Creation_Artwork_17_33 .

:Image_Artwork_77  a            :Digital_Image , owl:NamedIndividual ;
        rdfs:comment            "Image of an artwork by Barbara Nanning displayed in \"Barbara Nanning Eeuwige Beweging\" by Eliens (2019)."@en ;
        rdfs:label              "Image_Artwork_77"@en ;
        :Representation-Source  "Tom Haartsen_Ouderkerk a/d Amstel (NL)"@en ;
        :Shows                  :Artwork_77 .

:ARTWORK_75_SetupAndTestingOfTheMetalMold
        a                 owl:NamedIndividual , :Setup_and_Testing_of_the_Metal_Mold ;
        rdfs:comment      "Instance of an activity which is part of the creation process of ARTWORK_75."@en ;
        rdfs:label        "ARTWORK_75_Setup and Testing of the Metal Mold"@en ;
        :Followed-By      :ARTWORK_75_ExaminingTheQualityOfTheGlass ;
        :Follows          :ARTWORK_75_PreparingGlass ;
        :Has-Duration     <http://www.semanticweb.org/ontologies/Daan/2020/BarbaraNanning#2018> ;
        :Involves         :AssistantOfBarbara , <http://www.semanticweb.org/ontologies/Daan/2020/BarbaraNanning#RadekKoten(CZ)> , <http://www.semanticweb.org/ontologies/Daan/2020/BarbaraNanning#LukasHavlas(CZ)> , :BarbaraNanning , <http://www.semanticweb.org/ontologies/Daan/2020/BarbaraNanning#Tom%C3%A1%C5%A1Moravec(CZ)> , <http://www.semanticweb.org/ontologies/Daan/2020/BarbaraNanning#JiriMoravec(CZ)> ;
        :Located-In       :CzechRepublic ;
        :Part-Of          :Creation_Artwork_75 ;
        :Requires-Use-Of  :InterchangeableMetalMoldSetup .

:ARTWORK_18_64_Modeling
        a                 :Modeling , owl:NamedIndividual ;
        rdfs:comment      "Instance of an activity which is part of the creation process of ARTWORK_18_64."@en ;
        rdfs:label        "ARTWORK_18_64_Modeling"@en ;
        :Followed-By      <http://www.semanticweb.org/ontologies/Daan/2020/BarbaraNanning#ARTWORK_18_64_ExaminingQuality(Shape/Form)> ;
        :Follows          :ARTWORK_18_64_Sensing ;
        :Has-Duration     <http://www.semanticweb.org/ontologies/Daan/2020/BarbaraNanning#2015> ;
        :Involves         <http://www.semanticweb.org/ontologies/Daan/2020/BarbaraNanning#RobertLenner(CZ)> , <http://www.semanticweb.org/ontologies/Daan/2020/BarbaraNanning#MarekBrathko(CZ)> , <http://www.semanticweb.org/ontologies/Daan/2020/BarbaraNanning#MarekEffmert(CZ)> , :GertBullée , :BarbaraNanning , <http://www.semanticweb.org/ontologies/Daan/2020/BarbaraNanning#JessicaHomich(USA)> ;
        :Located-In       :Zaandam ;
        :Part-Of          :Creation_Artwork_18_64 ;
        :Requires-Use-Of  :InterchangeableMetalMoldSetup , :AirCompressor , :BlowingPipe , :PropaneTorch , :Gloves .

<http://www.semanticweb.org/ontologies/Daan/2020/BarbaraNanning#RobertLenner(CZ)>
        a             owl:NamedIndividual , :Third_Glass_Blower ;
        rdfs:comment  "Robert Lenner (CZ) is a Third Glass Blower."@en ;
        rdfs:label    "Robert Lenner (CZ)"@en ;
        :Involved-In  :ARTWORK_46_ProducingColouredCanes , :ARTWORK_18_64_PickingUpColouredCanesPattern , :ARTWORK_36_PickingUpColouredCanesPattern , :ARTWORK_36_PickingUpColouredPanel , :ARTWORK_39_PickingUpColouredPanel , :ARTWORK_18_64_Modeling , :ARTWORK_39_SetupAndTestingOfTheMetalMold , :ARTWORK_36_SetupAndTestingOfTheMetalMold , :ARTWORK_36_Glassblowing , :ARTWORK_36_Modeling , :ARTWORK_39_Modeling , :ARTWORK_39_Glassblowing , :ARTWORK_18_64_Glassblowing , :ARTWORK_18_64_ProducingColouredCanes , :ARTWORK_36_ProducingColouredCanes ;
        :Works-For    :VRIJGLASZaandam , :GlassStudioVanTetterode .

<http://www.semanticweb.org/ontologies/Daan/2020/BarbaraNanning#Ouderkerka/dAmstel>
        a             owl:NamedIndividual , :City ;
        rdfs:comment  "Ouderkerk a/d Amstel is a town in the Netherlands."@en ;
        rdfs:label    "Ouderkerk A/d Amstel"@en ;
        owl:sameAs    <http://www.wikidata.org/entity/Q282729> ;
        :Located-In   :Netherlands ;
        :Location-Of  :ARTWORK_36_Packing_8 , :ARTWORK_46_Photographing , :ARTWORK_36_Photographing_2 , :ARTWORK_18_64_Photographing , :ARTWORK_39_Photographing , :ARTWORK_36_Photographing , :ARTWORK_17_33_Photographing .

:ARTWORK_78_Transporting_3
        a              owl:NamedIndividual , :Transporting ;
        rdfs:comment   "Instance of an activity which is part of the creation process of ARTWORK_78."@en ;
        rdfs:label     "ARTWORK_78_Transporting_3"@en ;
        :Followed-By   :ARTWORK_78_Gilding ;
        :Follows       :ARTWORK_78_Packing_3 ;
        :Has-Duration  <http://www.semanticweb.org/ontologies/Daan/2020/BarbaraNanning#2008> ;
        :Involves      :BarbaraNanning , :AlešZvěřina ;
        :Located-In    :CzechRepublic ;
        :Part-Of       :Creation_Artwork_78 .

:Creation_Artwork_75  a  :Creation_Event , owl:NamedIndividual ;
        rdfs:comment    "Creation event for an artwork by Barbara Nanning displayed in \"Barbara Nanning Eeuwige Beweging\" by Eliens (2019)."@en ;
        rdfs:label      "Creation_Artwork_75"@en ;
        :Consists-Of    :ARTWORK_75_Packing_3 , :ARTWORK_75_ApplyingExtraColour , :ARTWORK_75_Documenting , :ARTWORK_75_Glassblowing , :ARTWORK_75_HeatingMetalMold , :ARTWORK_75_Transporting , :ARTWORK_75_Packing_5 , :ARTWORK_75_Sawing , :ARTWORK_75_Transporting_4 , :ARTWORK_75_Transporting_3 , :ARTWORK_75_Packing , :ARTWORK_75_Sandblasting , :ARTWORK_75_Modeling , :ARTWORK_75_ExaminingTheQualityOfTheGlass , :ARTWORK_75_Translocating , :ARTWORK_75_Resting , <http://www.semanticweb.org/ontologies/Daan/2020/BarbaraNanning#ARTWORK_75_ExaminingQuality(FinalResult)> , <http://www.semanticweb.org/ontologies/Daan/2020/BarbaraNanning#ARTWORK_75_ExaminingQuality(Result)> , :ARTWORK_75_Cooling , :ARTWORK_75_PreparingGlass , :ARTWORK_75_Gilding , <http://www.semanticweb.org/ontologies/Daan/2020/BarbaraNanning#ARTWORK_75_ExaminingQuality(CheckForIrregularitiesInTheGlass)> , :ARTWORK_75_ApplyingClearGlassBell , :ARTWORK_75_Signing , :ARTWORK_75_Sensing , :ARTWORK_75_Packing_2 , :ARTWORK_75_SetupAndTestingOfTheMetalMold , :ARTWORK_75_Polishing , :ARTWORK_75_Photographing , :ARTWORK_75_Grinding , :ARTWORK_75_ApplyingExtraColour_2 , :ARTWORK_75_Packing_4 , <http://www.semanticweb.org/ontologies/Daan/2020/BarbaraNanning#ARTWORK_75_ExaminingQuality(Shape/Form)> , :ARTWORK_75_SetupAndTestingOfTheMetalMold_2 ;
        :Created        :Artwork_75 ;
        :Finishes-With  :ARTWORK_75_Packing_5 ;
        :Has-Duration   <http://www.semanticweb.org/ontologies/Daan/2020/BarbaraNanning#2017> ;
        :Located-In     :CzechRepublic ;
        :Starts-With    :ARTWORK_75_PreparingGlass ;
        :Within-Period  :GlassVerreÉglomisé .

<http://www.semanticweb.org/ontologies/Daan/2020/BarbaraNanning#ARTWORK_36_ExaminingQuality(CheckForIrregularitiesInTheGlass)_2>
        a              owl:NamedIndividual , j.3: ;
        rdfs:comment   "Instance of an activity which is part of the creation process of ARTWORK_36."@en ;
        rdfs:label     "ARTWORK_36_Examining Quality (Check for Irregularities in the Glass)_2"@en ;
        :Followed-By   :ARTWORK_36_Sawing_2 ;
        :Follows       :ARTWORK_36_Resting_2 ;
        :Has-Duration  <http://www.semanticweb.org/ontologies/Daan/2020/BarbaraNanning#2019> ;
        :Involves      :AlešZvěřina , :BarbaraNanning ;
        :Located-In    :NovyBor ;
        :Part-Of       :Creation_Artwork_36 .

:ARTWORK_77_Packing_3
        a              :Packing , owl:NamedIndividual ;
        rdfs:comment   "Instance of an activity which is part of the creation process of ARTWORK_77."@en ;
        rdfs:label     "ARTWORK_77_Packing_3"@en ;
        :Followed-By   :ARTWORK_77_Transporting_3 ;
        :Follows       :ARTWORK_77_Signing ;
        :Has-Duration  <http://www.semanticweb.org/ontologies/Daan/2020/BarbaraNanning#2018> ;
        :Involves      :BarbaraNanning , :AlešZvěřina ;
        :Located-In    :CzechRepublic ;
        :Part-Of       :Creation_Artwork_77 .

:ARTWORK_36_FlatFusingFinishedArtwork
        a                 owl:NamedIndividual , :Flat_Fusing_Finished_Artwork ;
        rdfs:comment      "Instance of an activity which is part of the creation process of ARTWORK_36."@en ;
        rdfs:label        "ARTWORK_36_Flat Fusing Finished Artwork"@en ;
        :Followed-By      :ARTWORK_36_DecidingColourPalette_2 ;
        :Follows          :ARTWORK_36_Documenting ;
        :Has-Duration     <http://www.semanticweb.org/ontologies/Daan/2020/BarbaraNanning#2019> ;
        :Involves         :BarbaraNanning ;
        :Located-In       :Amsterdam ;
        :Part-Of          :Creation_Artwork_36 ;
        :Processes        :Artwork_36_Peacock ;
        :Requires-Use-Of  :Gloves , :FusingKiln .

:ARTWORK_75_ApplyingClearGlassBell
        a                 :Applying_Clear_Glass_Bell , owl:NamedIndividual ;
        rdfs:comment      "Instance of an activity which is part of the creation process of ARTWORK_75."@en ;
        rdfs:label        "ARTWORK_75_Applying Clear Glass Bell"@en ;
        :Followed-By      :ARTWORK_75_ApplyingExtraColour ;
        :Follows          :ARTWORK_75_SetupAndTestingOfTheMetalMold_2 ;
        :Has-Duration     <http://www.semanticweb.org/ontologies/Daan/2020/BarbaraNanning#2017> ;
        :Involves         <http://www.semanticweb.org/ontologies/Daan/2020/BarbaraNanning#RadekKoten(CZ)> , :BarbaraNanning , <http://www.semanticweb.org/ontologies/Daan/2020/BarbaraNanning#LukasHavlas(CZ)> ;
        :Located-In       :CzechRepublic ;
        :Part-Of          :Creation_Artwork_75 ;
        :Processes        :AJETOClearGlass ;
        :Requires-Use-Of  :DiamondShears , :CeramicPotFilledWithGlass , :Water , :Marver , :YokeOfSupport , :StraightShears , :BlowingPipe , :Beeswax , :IcePick , :Blocks , :Paper , :Pincet , :AirCompressor , :Hook , :Furnace , :Jacks .

:Soda   a                 :Man-Made_Material , owl:NamedIndividual ;
        rdfs:comment      "Soda is a white, water-soluble salt material."@en ;
        rdfs:label        "Soda"@en ;
        :Is-Processed-In  :AJETOClearGlass , :AJETORedGlass , :AJETOWhiteGlass , :AJETOBlackGlass , :AJETOSmokeGlass , :AJETOBlueGlass , :AJETOAmberGlass , :AJETOGreenGlass .

:AJETOClearGlass  a           owl:NamedIndividual , :AJETO_Glass ;
        rdfs:comment          "AJETO Clear Glass is a tranparent form of AJETO glass."@en ;
        rdfs:label            "AJETO Clear Glass"@en ;
        :Availability         "Available"@en ;
        :Is-Processed-During  :ARTWORK_75_ApplyingClearGlassBell , :ARTWORK_79_ApplyingClearGlassBell , :ARTWORK_80_ApplyingClearGlassBell , :ARTWORK_76_ApplyingClearGlassBell , :ARTWORK_43_ApplyingClearGlassBell , :ARTWORK_78_ApplyingClearGlassBell , :ARTWORK_73_ApplyingClearGlassBell , :ARTWORK_44_ApplyingClearGlassBell , :ARTWORK_77_ApplyingClearGlassBell , :ARTWORK_74_ApplyingClearGlassBell ;
        :Is-Processed-In      :Artwork_75 , :Artwork_73 , :Artwork_79 , :Artwork_74 , :Artwork_77 , :Artwork_78 , :Artwork_43 , :Artwork_76 , :Artwork_44 , :Artwork_80 ;
        :Made-By              :LASVITAJETO ;
        :Made-Out-Of          :Calcium , :Sand , :Potassium , :Soda ;
        :Transparency         "Transparent"@en .

:ARTWORK_74_SetupAndTestingOfTheMetalMold
        a                 owl:NamedIndividual , :Setup_and_Testing_of_the_Metal_Mold ;
        rdfs:comment      "Instance of an activity which is part of the creation process of ARTWORK_74."@en ;
        rdfs:label        "ARTWORK_74_Setup and Testing of the Metal Mold"@en ;
        :Followed-By      :ARTWORK_74_ExaminingTheQualityOfTheGlass ;
        :Follows          :ARTWORK_74_PreparingGlass ;
        :Has-Duration     <http://www.semanticweb.org/ontologies/Daan/2020/BarbaraNanning#2008> ;
        :Involves         <http://www.semanticweb.org/ontologies/Daan/2020/BarbaraNanning#RomanTomis(CZ)> , <http://www.semanticweb.org/ontologies/Daan/2020/BarbaraNanning#RostislavMaterka(CZ)> , :AssistantOfBarbara , :BarbaraNanning , <http://www.semanticweb.org/ontologies/Daan/2020/BarbaraNanning#RobertHlavacek(CZ)> , <http://www.semanticweb.org/ontologies/Daan/2020/BarbaraNanning#AlesVacek(CZ)> ;
        :Located-In       :CzechRepublic ;
        :Part-Of          :Creation_Artwork_74 ;
        :Requires-Use-Of  :InterchangeableMetalMoldSetup .

:Creation_Artwork_43  a  :Creation_Event , owl:NamedIndividual ;
        rdfs:comment    "Creation event for an artwork by Barbara Nanning displayed in \"Barbara Nanning Eeuwige Beweging\" by Eliens (2019)."@en ;
        rdfs:label      "Creation_Artwork_43"@en ;
        :Consists-Of    :ARTWORK_43_Packing_3 , :ARTWORK_43_Gilding , :ARTWORK_43_Sawing , :ARTWORK_43_Transporting , :ARTWORK_43_HeatingMetalMold , <http://www.semanticweb.org/ontologies/Daan/2020/BarbaraNanning#ARTWORK_43_ExaminingQuality(CheckForIrregularitiesInTheGlass)> , :ARTWORK_43_Packing_4 , <http://www.semanticweb.org/ontologies/Daan/2020/BarbaraNanning#ARTWORK_43_ExaminingQuality(FinalResult)> , :ARTWORK_43_Documenting , :ARTWORK_43_MeasuringAndBoxesMaking , :ARTWORK_43_Modeling , :ARTWORK_43_Grinding , :ARTWORK_43_Signing , :ARTWORK_43_Photographing , :ARTWORK_43_Transporting_2 , :ARTWORK_43_ApplyingClearGlassBell , :ARTWORK_43_Glassblowing , :ARTWORK_43_Transporting_3 , :ARTWORK_43_Packing_5 , :ARTWORK_43_ApplyingExtraColour , :ARTWORK_43_Sandblasting , :ARTWORK_43_Resting , <http://www.semanticweb.org/ontologies/Daan/2020/BarbaraNanning#ARTWORK_43_ExaminingQuality(Result)> , :ARTWORK_43_Transporting_4 , :ARTWORK_43_Sensing , :ARTWORK_43_SetupAndTestingOfTheMetalMold_2 , :ARTWORK_43_Translocating , :ARTWORK_43_Packing , :ARTWORK_43_ExaminingTheQualityOfTheGlass , :ARTWORK_43_SetupAndTestingOfTheMetalMold , :ARTWORK_43_Cooling , :ARTWORK_43_Polishing , <http://www.semanticweb.org/ontologies/Daan/2020/BarbaraNanning#ARTWORK_43_ExaminingQuality(Shape/Form)> , :ARTWORK_43_PreparingGlass , :ARTWORK_43_Packing_2 ;
        :Created        :Artwork_43 ;
        :Finishes-With  :ARTWORK_43_Packing_5 ;
        :Has-Duration   <http://www.semanticweb.org/ontologies/Daan/2020/BarbaraNanning#2008> ;
        :Located-In     :CzechRepublic ;
        :Starts-With    :ARTWORK_43_PreparingGlass ;
        :Within-Period  :GlassVerreÉglomisé .

<http://www.wikidata.org/entity/Q55>
        a       owl:NamedIndividual .

:ARTWORK_36_MakingPatternsWithColouredCanesInTheMetalBowl
        a                 owl:NamedIndividual , :Making_Patterns_with_Coloured_Canes_and_Strings_in_the_Metal_Bowl ;
        rdfs:comment      "Instance of an activity which is part of the creation process of ARTWORK_36."@en ;
        rdfs:label        "ARTWORK_36_Making Patterns with Coloured Canes in the Metal Bowl"@en ;
        :Followed-By      :ARTWORK_36_TackfusingColouredCanes ;
        :Follows          :ARTWORK_36_DecidingColourPalette ;
        :Has-Duration     <http://www.semanticweb.org/ontologies/Daan/2020/BarbaraNanning#2015> ;
        :Involves         :BarbaraNanning ;
        :Located-In       :Amsterdam ;
        :Part-Of          :Creation_Artwork_36 ;
        :Requires-Use-Of  :Pincet , :FusingKiln , :Glassscissors .

:ARTWORK_76_ApplyingExtraColour
        a                 owl:NamedIndividual , :Applying_Extra_Colour ;
        rdfs:comment      "Instance of an activity which is part of the creation process of ARTWORK_76."@en ;
        rdfs:label        "ARTWORK_76_Applying Extra Colour"@en ;
        :Followed-By      :ARTWORK_76_ApplyingExtraColour_2 ;
        :Follows          :ARTWORK_76_ApplyingClearGlassBell ;
        :Has-Duration     <http://www.semanticweb.org/ontologies/Daan/2020/BarbaraNanning#2018> ;
        :Involves         :BarbaraNanning , <http://www.semanticweb.org/ontologies/Daan/2020/BarbaraNanning#LukasHavlas(CZ)> , <http://www.semanticweb.org/ontologies/Daan/2020/BarbaraNanning#RadekKoten(CZ)> ;
        :Located-In       :CzechRepublic ;
        :Part-Of          :Creation_Artwork_76 ;
        :Processes        <http://www.semanticweb.org/ontologies/Daan/2020/BarbaraNanning#ReichenbachColourRodsGlass(DE)> ;
        :Requires-Use-Of  :Paper , :DiamondShears , :Water , :Garage , :YokeOfSupport , :Jacks , :AirCompressor , :BlowingPipe , :IcePick , :AnnealingKiln , :Hook , :Beeswax , :Blocks , :Tagliol , :Marver , :StraightShears , :Fork , :CeramicPotFilledWithGlass , :Pontis , :Furnace , :Pincet , :GloryHole .

:ARTWORK_76_Polishing
        a                 :Polishing , owl:NamedIndividual ;
        rdfs:comment      "Instance of an activity which is part of the creation process of ARTWORK_76."@en ;
        rdfs:label        "ARTWORK_76_Polishing"@en ;
        :Followed-By      <http://www.semanticweb.org/ontologies/Daan/2020/BarbaraNanning#ARTWORK_76_ExaminingQuality(CheckForIrregularitiesInTheGlass)_2> ;
        :Follows          :ARTWORK_76_Grinding ;
        :Has-Duration     <http://www.semanticweb.org/ontologies/Daan/2020/BarbaraNanning#2018> ;
        :Involves         :AlešZvěřina , :LukášSvoboda , :BarbaraNanning ;
        :Located-In       :CzechRepublic ;
        :Part-Of          :Creation_Artwork_76 ;
        :Requires-Use-Of  :PolishingStone .

<http://vocab.getty.edu/aat/300235507>
        a           owl:NamedIndividual ;
        owl:sameAs  :Ceramic .

:ARTWORK_78_Glassblowing
        a                 :Glassblowing , owl:NamedIndividual ;
        rdfs:comment      "Instance of an activity which is part of the creation process of ARTWORK_78."@en ;
        rdfs:label        "ARTWORK_78_Glassblowing"@en ;
        :Followed-By      :ARTWORK_78_Sensing ;
        :Follows          :ARTWORK_78_HeatingMetalMold ;
        :Has-Duration     <http://www.semanticweb.org/ontologies/Daan/2020/BarbaraNanning#2008> ;
        :Involves         <http://www.semanticweb.org/ontologies/Daan/2020/BarbaraNanning#RostislavMaterka(CZ)> , <http://www.semanticweb.org/ontologies/Daan/2020/BarbaraNanning#RomanTomis(CZ)> , :AssistantOfBarbara , <http://www.semanticweb.org/ontologies/Daan/2020/BarbaraNanning#RobertHlavacek(CZ)> , <http://www.semanticweb.org/ontologies/Daan/2020/BarbaraNanning#AlesVacek(CZ)> , :BarbaraNanning ;
        :Located-In       :CzechRepublic ;
        :Part-Of          :Creation_Artwork_78 ;
        :Requires-Use-Of  :Paper , :Furnace , :CeramicPotFilledWithGlass , :Pontis , :Jacks , :InterchangeableMetalMoldSetup , :YokeOfSupport , :Water , :StraightShears , :Fork , :Gloves , :PropaneTorch , :BlowingPipe , :GloryHole , :Tagliol , :BitIron , :DiamondShears , :AirCompressor , :Blocks , :Marver , :AnnealingKiln , :Hook , :Beeswax , :IcePick , :Pincet .

:Glassblowing  a         owl:Class ;
        rdfs:comment     "Glassblowing is an activity which Involves inflating (semi-) molten glass."@en ;
        rdfs:label       "Glassblowing"@en ;
        rdfs:subClassOf  :Activity .

<http://www.semanticweb.org/ontologies/Daan/2020/BarbaraNanning#RomanTomis(CZ)>
        a             :Third_Glass_Blower , owl:NamedIndividual ;
        rdfs:comment  "Roman Tomis (CZ) is a Third Glass Blower."@en ;
        rdfs:label    "Roman Tomis (CZ)"@en ;
        :Involved-In  :ARTWORK_43_SetupAndTestingOfTheMetalMold , :ARTWORK_78_SetupAndTestingOfTheMetalMold , :ARTWORK_74_SetupAndTestingOfTheMetalMold_2 , :ARTWORK_74_SetupAndTestingOfTheMetalMold , :ARTWORK_78_SetupAndTestingOfTheMetalMold_2 , :ARTWORK_43_Modeling , :ARTWORK_78_Glassblowing , :ARTWORK_43_SetupAndTestingOfTheMetalMold_2 , :ARTWORK_78_Modeling , :ARTWORK_74_Glassblowing , :ARTWORK_74_Modeling , :ARTWORK_43_Glassblowing ;
        :Works-For    :LASVITAJETO .

:ARTWORK_36_Packing_7
        a              :Packing , owl:NamedIndividual ;
        rdfs:comment   "Instance of an activity which is part of the creation process of ARTWORK_36."@en ;
        rdfs:label     "ARTWORK_36_Packing_7"@en ;
        :Followed-By   :ARTWORK_36_Transporting_6 ;
        :Follows       <http://www.semanticweb.org/ontologies/Daan/2020/BarbaraNanning#ARTWORK_36_ExaminingQuality(FinalResult)_2> ;
        :Has-Duration  <http://www.semanticweb.org/ontologies/Daan/2020/BarbaraNanning#2019> ;
        :Involves      :BarbaraNanning ;
        :Located-In    :NovyBor ;
        :Part-Of       :Creation_Artwork_36 .

:Fusing_Sheets  a        owl:Class ;
        rdfs:comment     "To combine all available colours in any desired composition and pattern I make my own rods. Multiple monochrome Bullseye Fusing flat glass plates are stacked and fused into a thick monochrome colored package. Then I saw, grind and sandblast it to 3 x 3 x 6 cm."@en ;
        rdfs:label       "Fusing Sheets"@en ;
        rdfs:subClassOf  :Activity .

:AJETORedGlass  a             owl:NamedIndividual , :AJETO_Glass ;
        rdfs:comment          "AJETO Red is a form of AJETO glass with a red colour."@en ;
        rdfs:label            "AJETO Red Glass"@en ;
        :Availability         "Available"@en ;
        :Is-Processed-During  :ARTWORK_74_ApplyingExtraColour ;
        :Is-Processed-In      :Artwork_74 ;
        :Made-By              :LASVITAJETO ;
        :Made-Out-Of          :Sand , :Soda , :Calcium , :Potassium ;
        :Transparency         "Transparent"@en .

<http://www.cidoc-crm.org/cidoc-crm/P115_is_finished_by>
        a                       owl:ObjectProperty ;
        owl:equivalentProperty  :Finishes-With .

:ARTWORK_39_Modeling  a   :Modeling , owl:NamedIndividual ;
        rdfs:comment      "Instance of an activity which is part of the creation process of ARTWORK_39."@en ;
        rdfs:label        "ARTWORK_39_Modeling"@en ;
        :Followed-By      <http://www.semanticweb.org/ontologies/Daan/2020/BarbaraNanning#ARTWORK_39_ExaminingQuality(Shape/Form)> ;
        :Follows          :ARTWORK_39_Sensing ;
        :Has-Duration     <http://www.semanticweb.org/ontologies/Daan/2020/BarbaraNanning#2015> ;
        :Involves         <http://www.semanticweb.org/ontologies/Daan/2020/BarbaraNanning#MarekEffmert(CZ)> , <http://www.semanticweb.org/ontologies/Daan/2020/BarbaraNanning#MarekBrathko(CZ)> , <http://www.semanticweb.org/ontologies/Daan/2020/BarbaraNanning#RobertLenner(CZ)> , :GertBullée , :BarbaraNanning , <http://www.semanticweb.org/ontologies/Daan/2020/BarbaraNanning#JessicaHomich(USA)> ;
        :Located-In       :Zaandam ;
        :Part-Of          :Creation_Artwork_39 ;
        :Requires-Use-Of  :AirCompressor , :PropaneTorch , :Gloves , :InterchangeableMetalMoldSetup , :BlowingPipe .

:Artwork_77  a        owl:NamedIndividual , :Glass_Artwork ;
        rdfs:comment  "Artwork by Barbara Nanning displayed in \"Barbara Nanning Eeuwige Beweging\" by Eliens (2019)."@en ;
        rdfs:label    "Verre églomisé (Go with the Flow)"@en ;
        :Created-By   :Creation_Artwork_77 ;
        :Has-Depth    "33"^^xsd:decimal ;
        :Has-Height   "19"^^xsd:decimal ;
        :Has-Width    "37"^^xsd:decimal ;
        :Is-Unica     "Yes"@en ;
        :Located-In   :Amsterdam ;
        :Made-By      :LASVITAJETO , <http://www.semanticweb.org/ontologies/Daan/2020/BarbaraNanning#Ale%C5%A1Zv%C4%9B%C5%99ina&AZ-Design> , :VáçlavNovák_Doksy_CzechRepublic , :BarbaraNanning ;
        :Made-Out-Of  :AJETOSmokeGlass , :LouvreGoldLeaf , :AJETOClearGlass ;
        :Part-Of      :CollectionOfBarbaraNanning ;
        :Shown-By     :Image_Artwork_77 .

:ARTWORK_39_Cooling  a    :Cooling , owl:NamedIndividual ;
        rdfs:comment      "Instance of an activity which is part of the creation process of ARTWORK_39."@en ;
        rdfs:label        "ARTWORK_39_Cooling"@en ;
        :Followed-By      :ARTWORK_39_Packing ;
        :Follows          <http://www.semanticweb.org/ontologies/Daan/2020/BarbaraNanning#ARTWORK_39_ExaminingQuality(Shape/Form)> ;
        :Has-Duration     <http://www.semanticweb.org/ontologies/Daan/2020/BarbaraNanning#2015> ;
        :Involves         <http://www.semanticweb.org/ontologies/Daan/2020/BarbaraNanning#MiaLerssi(DN)> , <http://www.semanticweb.org/ontologies/Daan/2020/BarbaraNanning#JessicaHomich(USA)> , :DurkValkema ;
        :Located-In       :Zaandam ;
        :Part-Of          :Creation_Artwork_39 ;
        :Requires-Use-Of  :AnnealingKiln .

:ARTWORK_75_Photographing
        a              owl:NamedIndividual , :Photographing ;
        rdfs:comment   "Instance of an activity which is part of the creation process of ARTWORK_75."@en ;
        rdfs:label     "ARTWORK_75_Photographing"@en ;
        :Followed-By   :ARTWORK_75_Documenting ;
        :Follows       :ARTWORK_75_Transporting_4 ;
        :Has-Duration  <http://www.semanticweb.org/ontologies/Daan/2020/BarbaraNanning#2018> ;
        :Involves      :BarbaraNanning , <http://www.semanticweb.org/ontologies/Daan/2020/BarbaraNanning#TomHaartsen_Ouderkerka/dAmstel(NL)> ;
        :Located-In    :CzechRepublic ;
        :Part-Of       :Creation_Artwork_75 .

:ARTWORK_18_64_Sawing
        a                 :Sawing , owl:NamedIndividual ;
        rdfs:comment      "Instance of an activity which is part of the creation process of ARTWORK_18_64."@en ;
        rdfs:label        "ARTWORK_18_64_Sawing"@en ;
        :Followed-By      :ARTWORK_18_64_Sensing_2 ;
        :Follows          <http://www.semanticweb.org/ontologies/Daan/2020/BarbaraNanning#ARTWORK_18_64_ExaminingQuality(CheckForIrregularitiesInTheGlass)> ;
        :Has-Duration     <http://www.semanticweb.org/ontologies/Daan/2020/BarbaraNanning#2015> ;
        :Involves         :AlešZvěřina , :BarbaraNanning ;
        :Located-In       :NovyBor ;
        :Part-Of          :Creation_Artwork_18_64 ;
        :Requires-Use-Of  :DiamondSaw .

:ARTWORK_44_ExaminingTheQualityOfTheGlass
        a                 :Examining_the_Quality_of_the_Glass , owl:NamedIndividual ;
        rdfs:comment      "Instance of an activity which is part of the creation process of ARTWORK_44."@en ;
        rdfs:label        "ARTWORK_44_Examining the Quality of the Glass"@en ;
        :Followed-By      :ARTWORK_44_Cooling ;
        :Follows          :ARTWORK_44_Modeling ;
        :Has-Duration     <http://www.semanticweb.org/ontologies/Daan/2020/BarbaraNanning#2008> ;
        :Involves         :LuděkKout , :BarbaraNanning , <http://www.semanticweb.org/ontologies/Daan/2020/BarbaraNanning#RadekKoten(CZ)> ;
        :Located-In       :CzechRepublic ;
        :Part-Of          :Creation_Artwork_44 ;
        :Requires-Use-Of  :GloryHole , :Blocks , :Jacks , :Paper , :CeramicPotFilledWithGlass , :StraightShears , :DiamondShears , :Furnace , :Pontis , :YokeOfSupport , :AnnealingKiln , :Water , :BlowingPipe .

:Amsterdam  a         :City , owl:NamedIndividual ;
        rdfs:comment  "Amsterdam is the capital of the Netherlands."@en ;
        rdfs:label    "Amsterdam"@en ;
        :Located-In   :Netherlands ;
        :Location-Of  :Artwork_77 , :Artwork_76 , :CollectionOfBarbaraNanning , :Artwork_80 , :Artwork_75 .

:ARTWORK_44_Grinding  a   owl:NamedIndividual , :Grinding ;
        rdfs:comment      "Instance of an activity which is part of the creation process of ARTWORK_44."@en ;
        rdfs:label        "ARTWORK_44_Grinding"@en ;
        :Followed-By      :ARTWORK_44_Polishing ;
        :Follows          :ARTWORK_44_Sawing ;
        :Has-Duration     <http://www.semanticweb.org/ontologies/Daan/2020/BarbaraNanning#2018> ;
        :Involves         :BarbaraNanning , :AlešZvěřina , :RobertFlorian ;
        :Located-In       :CzechRepublic ;
        :Part-Of          :Creation_Artwork_44 ;
        :Requires-Use-Of  :SharpeningStone , :GrindingWheel .

:ARTWORK_18_64_FusingSheetsAndStrings
        a                 owl:NamedIndividual , :Fusing_Sheets_and_Strings ;
        rdfs:comment      "Instance of an activity which is part of the creation process of ARTWORK_18_64."@en ;
        rdfs:label        "ARTWORK_18_64_Fusing Sheets and Strings"@en ;
        :Followed-By      :ARTWORK_18_64_SlumpingSheetsAndStrings ;
        :Follows          :ARTWORK_18_64_DecoratingTheSheetWithColouredCanes ;
        :Has-Duration     <http://www.semanticweb.org/ontologies/Daan/2020/BarbaraNanning#2015> ;
        :Involves         :BarbaraNanning ;
        :Located-In       :Amsterdam ;
        :Part-Of          :Creation_Artwork_18_64 ;
        :Requires-Use-Of  :FusingKiln .

:Metal_Worker_1  a       owl:Class ;
        rdfs:comment     "A Metal Worker 1 is an actor who is the first member of a team responsible for creating metal objects or dealing with metal material."@en ;
        rdfs:label       "Metal Worker 1"@en ;
        rdfs:subClassOf  :Metal_Worker .

:ARTWORK_76_Grinding  a   :Grinding , owl:NamedIndividual ;
        rdfs:comment      "Instance of an activity which is part of the creation process of ARTWORK_76."@en ;
        rdfs:label        "ARTWORK_76_Grinding"@en ;
        :Followed-By      :ARTWORK_76_Polishing ;
        :Follows          :ARTWORK_76_Sawing ;
        :Has-Duration     <http://www.semanticweb.org/ontologies/Daan/2020/BarbaraNanning#2018> ;
        :Involves         :RobertFlorian , :BarbaraNanning , :AlešZvěřina ;
        :Located-In       :CzechRepublic ;
        :Part-Of          :Creation_Artwork_76 ;
        :Requires-Use-Of  :GrindingWheel , :SharpeningStone .

:Period  a                   owl:Class ;
        rdfs:comment         "A period is a portion of time."@en ;
        rdfs:label           "Period"@en ;
        rdfs:subClassOf      :Entity ;
        owl:equivalentClass  <http://www.wikidata.org/entity/Q11514315> .

:CzechRepublic  a     owl:NamedIndividual , :Country ;
        rdfs:comment  "Czech Republic is a country in central Europe."@en ;
        rdfs:label    "Czech Republic"@en ;
        owl:sameAs    <http://www.wikidata.org/entity/Q213> ;
        :Location-Of  :ARTWORK_43_Photographing , :ARTWORK_44_Packing , :ARTWORK_73_Photographing , :ARTWORK_77_Packing_2 , :ARTWORK_73_Packing , :ARTWORK_77_MeasuringAndBoxesMaking , :ARTWORK_74_Packing_2 , :ARTWORK_73_MeasuringAndBoxesMaking , :ARTWORK_76_Glassblowing , :ARTWORK_74_ApplyingClearGlassBell , :ARTWORK_73_SetupAndTestingOfTheMetalMold_2 , :ARTWORK_78_Packing_2 , :ARTWORK_79_MeasuringAndBoxesMaking , :ARTWORK_76_Documenting , :ARTWORK_78_Translocating , :ARTWORK_79_Sensing , :ARTWORK_75_Transporting_3 , <http://www.semanticweb.org/ontologies/Daan/2020/BarbaraNanning#ARTWORK_80_ExaminingQuality(Result)> , :ARTWORK_78_Transporting_3 , :ARTWORK_78_SetupAndTestingOfTheMetalMold_2 , :ARTWORK_73_Packing_3 , :ARTWORK_79_HeatingMetalMold , :ARTWORK_73_HeatingMetalMold , :ARTWORK_74_Modeling , :ARTWORK_44_Packing_4 , <http://www.semanticweb.org/ontologies/Daan/2020/BarbaraNanning#ARTWORK_43_ExaminingQuality(FinalResult)> , <http://www.semanticweb.org/ontologies/Daan/2020/BarbaraNanning#ARTWORK_79_ExaminingQuality(Shape/Form)> , :ARTWORK_73_Modeling , :ARTWORK_78_ApplyingClearGlassBell , :ARTWORK_75_Polishing , :ARTWORK_75_Modeling , :ARTWORK_79_Documenting , <http://www.semanticweb.org/ontologies/Daan/2020/BarbaraNanning#ARTWORK_77_ExaminingQuality(Result)> , :ARTWORK_43_Sawing , <http://www.semanticweb.org/ontologies/Daan/2020/BarbaraNanning#ARTWORK_79_ExaminingQuality(CheckForIrregularitiesInTheGlass)> , <http://www.semanticweb.org/ontologies/Daan/2020/BarbaraNanning#ARTWORK_75_ExaminingQuality(Shape/Form)> , <http://www.semanticweb.org/ontologies/Daan/2020/BarbaraNanning#ARTWORK_79_ExaminingQuality(FinalResult)> , :ARTWORK_79_Packing_5 , :ARTWORK_44_SetupAndTestingOfTheMetalMold , :ARTWORK_77_Polishing , :ARTWORK_75_Packing_3 , :ARTWORK_74_Packing_5 , :ARTWORK_43_Signing , :ARTWORK_77_Packing , :ARTWORK_44_Glassblowing , :ARTWORK_79_Sawing , :ARTWORK_80_Transporting_3 , <http://www.semanticweb.org/ontologies/Daan/2020/BarbaraNanning#ARTWORK_74_ExaminingQuality(FinalResult)> , :ARTWORK_79_Transporting_3 , :ARTWORK_79_ApplyingExtraColour_2 , :ARTWORK_75_Sawing , :ARTWORK_44_Packing_5 , :ARTWORK_74_Translocating , :ARTWORK_76_Transporting_3 , :ARTWORK_80_Sawing , :ARTWORK_80_Packing_3 , :ARTWORK_77_Modeling , :ARTWORK_80_Sandblasting , :ARTWORK_80_MeasuringAndBoxesMaking , :ARTWORK_75_Sensing , :ARTWORK_76_Transporting , :ARTWORK_75_HeatingMetalMold , <http://www.semanticweb.org/ontologies/Daan/2020/BarbaraNanning#ARTWORK_77_ExaminingQuality(CheckForIrregularitiesInTheGlass)> , :ARTWORK_73_Transporting_3 , :ARTWORK_44_Polishing , :ARTWORK_73_ExaminingTheQualityOfTheGlass , :ARTWORK_73_PreparingGlass , :ARTWORK_73_Polishing , :ARTWORK_77_PreparingGlass , :ARTWORK_75_ApplyingExtraColour_2 , :ARTWORK_43_Packing , :ARTWORK_76_Grinding , :ARTWORK_76_Packing_5 , :ARTWORK_75_SetupAndTestingOfTheMetalMold_2 , :ARTWORK_80_SetupAndTestingOfTheMetalMold_2 , :ARTWORK_73_Sawing , :ARTWORK_76_Gilding , :ARTWORK_77_Photographing , :ARTWORK_43_Sandblasting , :ARTWORK_79_Cooling , :ARTWORK_73_Sensing , :ARTWORK_79_Grinding , <http://www.semanticweb.org/ontologies/Daan/2020/BarbaraNanning#ARTWORK_80_ExaminingQuality(FinalResult)> , :ARTWORK_77_Packing_4 , :ARTWORK_44_Grinding , :ARTWORK_74_Packing_4 , :ARTWORK_77_ApplyingClearGlassBell , <http://www.semanticweb.org/ontologies/Daan/2020/BarbaraNanning#ARTWORK_44_ExaminingQuality(CheckForIrregularitiesInTheGlass)> , :ARTWORK_43_Modeling , :ARTWORK_78_Transporting_2 , :ARTWORK_74_ApplyingExtraColour , :ARTWORK_78_Glassblowing , <http://www.semanticweb.org/ontologies/Daan/2020/BarbaraNanning#ARTWORK_77_ExaminingQuality(FinalResult)> , :ARTWORK_73_Grinding , :NovyBor , :ARTWORK_73_Translocating , :ARTWORK_43_PreparingGlass , :ARTWORK_77_ExaminingTheQualityOfTheGlass , :ARTWORK_80_Gilding , :ARTWORK_75_Grinding , :ARTWORK_76_ApplyingClearGlassBell , :ARTWORK_79_Packing , :ARTWORK_79_Translocating , :ARTWORK_44_Cooling , :ARTWORK_76_PreparingGlass , :ARTWORK_44_SetupAndTestingOfTheMetalMold_2 , :ARTWORK_80_Cooling , :ARTWORK_44_Modeling , :ARTWORK_79_Packing_3 , :ARTWORK_79_Glassblowing , :ARTWORK_74_Sawing , :ARTWORK_77_Transporting , :ARTWORK_79_Photographing , :ARTWORK_79_Signing , :ARTWORK_74_Resting , :ARTWORK_80_Polishing , :ARTWORK_77_SetupAndTestingOfTheMetalMold_2 , :ARTWORK_73_Glassblowing , :ARTWORK_44_Transporting , :ARTWORK_44_Packing_2 , :ARTWORK_79_Gilding , :ARTWORK_43_Documenting , :ARTWORK_77_Grinding , :ARTWORK_73_Packing_4 , :ARTWORK_76_SetupAndTestingOfTheMetalMold , :ARTWORK_78_Gilding , :ARTWORK_74_Gilding , :ARTWORK_75_Signing , :ARTWORK_80_Resting , :ARTWORK_76_ApplyingExtraColour , :ARTWORK_78_HeatingMetalMold , :ARTWORK_43_Grinding , :ARTWORK_74_Transporting_3 , :ARTWORK_78_SetupAndTestingOfTheMetalMold , :ARTWORK_75_ExaminingTheQualityOfTheGlass , :ARTWORK_76_Sandblasting , :ARTWORK_73_Transporting_4 , :ARTWORK_78_ApplyingExtraColour , :ARTWORK_80_Glassblowing , <http://www.semanticweb.org/ontologies/Daan/2020/BarbaraNanning#ARTWORK_75_ExaminingQuality(FinalResult)> , <http://www.semanticweb.org/ontologies/Daan/2020/BarbaraNanning#ARTWORK_80_ExaminingQuality(Shape/Form)> , <http://www.semanticweb.org/ontologies/Daan/2020/BarbaraNanning#ARTWORK_74_ExaminingQuality(Result)> , <http://www.semanticweb.org/ontologies/Daan/2020/BarbaraNanning#ARTWORK_78_ExaminingQuality(CheckForIrregularitiesInTheGlass)> , :ARTWORK_78_Sensing , :ARTWORK_77_Sawing , :ARTWORK_77_Packing_3 , :ARTWORK_43_Polishing , :ARTWORK_75_ApplyingExtraColour , :ARTWORK_44_Documenting , :ARTWORK_74_Sensing , :ARTWORK_79_Transporting , :ARTWORK_75_Transporting_2 , :ARTWORK_44_Translocating , :ARTWORK_76_Packing , :ARTWORK_80_Modeling , :ARTWORK_77_Documenting , :ARTWORK_44_Gilding , :ARTWORK_80_ApplyingClearGlassBell , :ARTWORK_78_Transporting_4 , :ARTWORK_73_Signing , :ARTWORK_76_Packing_3 , :ARTWORK_44_Sensing , :ARTWORK_75_Resting , :ARTWORK_74_Glassblowing , :ARTWORK_80_Documenting , :ARTWORK_78_Packing_3 , :ARTWORK_43_SetupAndTestingOfTheMetalMold , :ARTWORK_75_Sandblasting , :ARTWORK_79_ApplyingExtraColour , :ARTWORK_76_Translocating , <http://www.semanticweb.org/ontologies/Daan/2020/BarbaraNanning#ARTWORK_43_ExaminingQuality(CheckForIrregularitiesInTheGlass)> , :ARTWORK_74_Cooling , :ARTWORK_80_Transporting_2 , :ARTWORK_77_Translocating , :ARTWORK_43_Packing_2 , :ARTWORK_79_Transporting_2 , :ARTWORK_78_Polishing , :ARTWORK_74_HeatingMetalMold , :ARTWORK_74_SetupAndTestingOfTheMetalMold , :ARTWORK_80_HeatingMetalMold , <http://www.semanticweb.org/ontologies/Daan/2020/BarbaraNanning#ARTWORK_44_ExaminingQuality(Shape/Form)> , :ARTWORK_77_Cooling , :ARTWORK_80_Packing_2 , <http://www.semanticweb.org/ontologies/Daan/2020/BarbaraNanning#ARTWORK_75_ExaminingQuality(Result)> , :ARTWORK_73_Documenting , :ARTWORK_76_SetupAndTestingOfTheMetalMold_2 , :ARTWORK_80_Translocating , :ARTWORK_74_Transporting_2 , :ARTWORK_74_Signing , :ARTWORK_76_Transporting_4 , :Doksy , :ARTWORK_73_Transporting_2 , :ARTWORK_76_Packing_2 , :ARTWORK_77_Transporting_3 , :ARTWORK_75_SetupAndTestingOfTheMetalMold , :ARTWORK_74_Photographing , :ARTWORK_80_Transporting , :ARTWORK_75_Gilding , :ARTWORK_76_Modeling , :ARTWORK_44_ApplyingClearGlassBell , :ARTWORK_80_Grinding , <http://www.semanticweb.org/ontologies/Daan/2020/BarbaraNanning#ARTWORK_75_ExaminingQuality(CheckForIrregularitiesInTheGlass)> , <http://www.semanticweb.org/ontologies/Daan/2020/BarbaraNanning#ARTWORK_73_ExaminingQuality(FinalResult)> , :ARTWORK_44_ApplyingExtraColour_2 , :ARTWORK_44_Sawing , :ARTWORK_76_Photographing , :ARTWORK_75_Cooling , :ARTWORK_44_PreparingGlass , :ARTWORK_43_SetupAndTestingOfTheMetalMold_2 , <http://www.semanticweb.org/ontologies/Daan/2020/BarbaraNanning#ARTWORK_73_ExaminingQuality(Result)> , :ARTWORK_75_Packing , :ARTWORK_77_Packing_5 , :ARTWORK_79_SetupAndTestingOfTheMetalMold_2 , :ARTWORK_75_Packing_4 , :ARTWORK_80_ExaminingTheQualityOfTheGlass , :ARTWORK_44_Photographing , <http://www.semanticweb.org/ontologies/Daan/2020/BarbaraNanning#ARTWORK_77_ExaminingQuality(Shape/Form)> , :ARTWORK_75_Transporting_4 , :ARTWORK_43_Translocating , :ARTWORK_44_MeasuringAndBoxesMaking , :ARTWORK_43_Transporting , :ARTWORK_80_PreparingGlass , :ARTWORK_78_Cooling , :ARTWORK_44_Transporting_2 , :ARTWORK_77_Sensing , :ARTWORK_77_Resting , :ARTWORK_76_Cooling , :ARTWORK_74_PreparingGlass , :Lindava , :ARTWORK_76_Signing , :ARTWORK_77_SetupAndTestingOfTheMetalMold , <http://www.semanticweb.org/ontologies/Daan/2020/BarbaraNanning#ARTWORK_76_ExaminingQuality(CheckForIrregularitiesInTheGlass)_2> , :ARTWORK_80_Packing , :ARTWORK_43_Packing_3 , :ARTWORK_75_Transporting , :ARTWORK_77_Gilding , :ARTWORK_77_HeatingMetalMold , :ARTWORK_76_Transporting_2 , :ARTWORK_73_Packing_5 , :ARTWORK_79_Transporting_4 , :ARTWORK_75_ApplyingClearGlassBell , :ARTWORK_78_PreparingGlass , <http://www.semanticweb.org/ontologies/Daan/2020/BarbaraNanning#ARTWORK_76_ExaminingQuality(CheckForIrregularitiesInTheGlass)> , <http://www.semanticweb.org/ontologies/Daan/2020/BarbaraNanning#ARTWORK_73_ExaminingQuality(CheckForIrregularitiesInTheGlass)> , :ARTWORK_73_Packing_2 , <http://www.semanticweb.org/ontologies/Daan/2020/BarbaraNanning#ARTWORK_74_ExaminingQuality(Shape/Form)> , :ARTWORK_80_Packing_4 , :ARTWORK_43_Transporting_2 , <http://www.semanticweb.org/ontologies/Daan/2020/BarbaraNanning#ARTWORK_78_ExaminingQuality(Result)> , :ARTWORK_74_Transporting_4 , :ARTWORK_78_Packing_5 , :ARTWORK_79_PreparingGlass , :ARTWORK_77_Transporting_4 , :ARTWORK_74_Documenting , <http://www.semanticweb.org/ontologies/Daan/2020/BarbaraNanning#ARTWORK_80_ExaminingQuality(CheckForIrregularitiesInTheGlass)> , :ARTWORK_43_Sensing , :ARTWORK_43_ApplyingExtraColour , :ARTWORK_78_Grinding , :ARTWORK_78_Modeling , :ARTWORK_79_Packing_4 , :ARTWORK_78_Signing , <http://www.semanticweb.org/ontologies/Daan/2020/BarbaraNanning#ARTWORK_76_ExaminingQuality(Shape/Form)> , :ARTWORK_43_ExaminingTheQualityOfTheGlass , :ARTWORK_78_ExaminingTheQualityOfTheGlass , :ARTWORK_74_Grinding , :ARTWORK_75_Packing_2 , :ARTWORK_43_Gilding , :ARTWORK_73_Cooling , :ARTWORK_75_Photographing , :ARTWORK_43_Glassblowing , :ARTWORK_43_Packing_4 , <http://www.semanticweb.org/ontologies/Daan/2020/BarbaraNanning#ARTWORK_44_ExaminingQuality(FinalResult)> , :ARTWORK_74_Transporting , :ARTWORK_74_ApplyingExtraColour_2 , :ARTWORK_43_MeasuringAndBoxesMaking , :ARTWORK_78_Packing , :ARTWORK_44_Signing , :ARTWORK_76_Packing_4 , :ARTWORK_73_SetupAndTestingOfTheMetalMold , :ARTWORK_43_ApplyingClearGlassBell , :ARTWORK_78_Transporting , :ARTWORK_73_ApplyingClearGlassBell , :ARTWORK_76_ApplyingExtraColour_2 , :ARTWORK_78_Packing_4 , :ARTWORK_73_Transporting , :ARTWORK_79_Resting , :ARTWORK_44_Resting , :ARTWORK_75_Glassblowing , :ARTWORK_79_Polishing , :ARTWORK_78_MeasuringAndBoxesMaking , :ARTWORK_77_ApplyingExtraColour , :ARTWORK_43_Resting , <http://www.semanticweb.org/ontologies/Daan/2020/BarbaraNanning#ARTWORK_73_ExaminingQuality(Shape/Form)> , :ARTWORK_44_ApplyingExtraColour , :ARTWORK_75_Documenting , :ARTWORK_77_Glassblowing , :ARTWORK_79_SetupAndTestingOfTheMetalMold , <http://www.semanticweb.org/ontologies/Daan/2020/BarbaraNanning#ARTWORK_79_ExaminingQuality(Result)> , :ARTWORK_79_ApplyingClearGlassBell , :ARTWORK_74_Packing_3 , :ARTWORK_80_Sensing , :ARTWORK_78_Photographing , :ARTWORK_43_Packing_5 , :ARTWORK_80_Signing , :ARTWORK_77_Transporting_2 , :ARTWORK_76_ExaminingTheQualityOfTheGlass , :ARTWORK_43_Transporting_3 , :ARTWORK_44_Transporting_4 , <http://www.semanticweb.org/ontologies/Daan/2020/BarbaraNanning#ARTWORK_43_ExaminingQuality(Result)> , :ARTWORK_79_Packing_2 , :ARTWORK_80_ApplyingExtraColour , :ARTWORK_74_Polishing , :ARTWORK_78_Documenting , :ARTWORK_80_SetupAndTestingOfTheMetalMold , :ARTWORK_78_Sawing , :ARTWORK_74_ExaminingTheQualityOfTheGlass , :ARTWORK_43_Cooling , <http://www.semanticweb.org/ontologies/Daan/2020/BarbaraNanning#ARTWORK_43_ExaminingQuality(Shape/Form)> , :ARTWORK_75_Translocating , :ARTWORK_76_Polishing , :ARTWORK_44_Packing_3 , <http://www.semanticweb.org/ontologies/Daan/2020/BarbaraNanning#ARTWORK_74_ExaminingQuality(CheckForIrregularitiesInTheGlass)> , <http://www.semanticweb.org/ontologies/Daan/2020/BarbaraNanning#ARTWORK_78_ExaminingQuality(FinalResult)> , :ARTWORK_73_Sandblasting , :ARTWORK_76_HeatingMetalMold , :ARTWORK_76_Sawing , :ARTWORK_75_Packing_5 , :ARTWORK_78_Resting , :ARTWORK_76_MeasuringAndBoxesMaking , :ARTWORK_43_HeatingMetalMold , :ARTWORK_79_ExaminingTheQualityOfTheGlass , :ARTWORK_77_Signing , :ARTWORK_43_Transporting_4 , :ARTWORK_73_Resting , :ARTWORK_44_HeatingMetalMold , :ARTWORK_73_Gilding , :ARTWORK_79_Modeling , <http://www.semanticweb.org/ontologies/Daan/2020/BarbaraNanning#ARTWORK_76_ExaminingQuality(FinalResult)> , <http://www.semanticweb.org/ontologies/Daan/2020/BarbaraNanning#ARTWORK_78_ExaminingQuality(Shape/Form)> , :ARTWORK_44_ExaminingTheQualityOfTheGlass , :ARTWORK_76_Sensing , :ARTWORK_74_Packing , :ARTWORK_44_Transporting_3 , :ARTWORK_80_Photographing , :ARTWORK_75_PreparingGlass , :ARTWORK_74_SetupAndTestingOfTheMetalMold_2 , :ARTWORK_76_Resting .

:Pincet  a            :Tool , owl:NamedIndividual ;
        rdfs:comment  "A pincet is an tool with moveable arms used for picking up and holding things."@en ;
        rdfs:label    "Pincet"@en ;
        :Used-For     :ARTWORK_77_Glassblowing , :ARTWORK_76_Glassblowing , :ARTWORK_76_ApplyingExtraColour , :ARTWORK_73_Glassblowing , :ARTWORK_76_ApplyingExtraColour_2 , :ARTWORK_44_Glassblowing , :ARTWORK_44_ApplyingExtraColour_2 , :ARTWORK_75_Glassblowing , :ARTWORK_77_ApplyingClearGlassBell , :ARTWORK_43_ApplyingExtraColour , :ARTWORK_43_Glassblowing , :ARTWORK_79_Glassblowing , :ARTWORK_77_ApplyingExtraColour , :ARTWORK_78_ApplyingClearGlassBell , :ARTWORK_78_ApplyingExtraColour , :ARTWORK_79_ApplyingExtraColour_2 , :ARTWORK_43_ApplyingClearGlassBell , :ARTWORK_44_ApplyingClearGlassBell , :ARTWORK_79_ApplyingExtraColour , :ARTWORK_80_ApplyingClearGlassBell , :ARTWORK_73_ApplyingClearGlassBell , :ARTWORK_74_ApplyingClearGlassBell , :ARTWORK_74_Glassblowing , :ARTWORK_80_Glassblowing , :ARTWORK_75_ApplyingClearGlassBell , :ARTWORK_75_ApplyingExtraColour , :ARTWORK_76_ApplyingClearGlassBell , :ARTWORK_74_ApplyingExtraColour_2 , :ARTWORK_44_ApplyingExtraColour , :ARTWORK_78_Glassblowing , :ARTWORK_80_ApplyingExtraColour , :ARTWORK_75_ApplyingExtraColour_2 , :ARTWORK_79_ApplyingClearGlassBell , :ARTWORK_74_ApplyingExtraColour .

:ARTWORK_36_CuttingAndPolishingColouredCanes
        a                 owl:NamedIndividual , :Cutting_and_Polishing_Coloured_Canes ;
        rdfs:comment      "Instance of an activity which is part of the creation process of ARTWORK_36."@en ;
        rdfs:label        "ARTWORK_36_Cutting and Polishing Coloured Canes"@en ;
        :Followed-By      :ARTWORK_36_TransportingColouredCanes_2 ;
        :Follows          :ARTWORK_36_TransportingColouredCanes ;
        :Has-Duration     <http://www.semanticweb.org/ontologies/Daan/2020/BarbaraNanning#2015> ;
        :Involves         :RobertFlorian , :BarbaraNanning , :AlešZvěřina ;
        :Located-In       :NovyBor ;
        :Part-Of          :Creation_Artwork_36 ;
        :Requires-Use-Of  :SharpeningStone , :Water , :DiamondSaw , :Glassscissors .

:ARTWORK_77_Glassblowing
        a                 owl:NamedIndividual , :Glassblowing ;
        rdfs:comment      "Instance of an activity which is part of the creation process of ARTWORK_77."@en ;
        rdfs:label        "ARTWORK_77_Glassblowing"@en ;
        :Followed-By      :ARTWORK_77_Sensing ;
        :Follows          :ARTWORK_77_HeatingMetalMold ;
        :Has-Duration     <http://www.semanticweb.org/ontologies/Daan/2020/BarbaraNanning#2018> ;
        :Involves         <http://www.semanticweb.org/ontologies/Daan/2020/BarbaraNanning#Tom%C3%A1%C5%A1Moravec(CZ)> , <http://www.semanticweb.org/ontologies/Daan/2020/BarbaraNanning#LukasHavlas(CZ)> , :BarbaraNanning , <http://www.semanticweb.org/ontologies/Daan/2020/BarbaraNanning#RadekKoten(CZ)> , <http://www.semanticweb.org/ontologies/Daan/2020/BarbaraNanning#JiriMoravec(CZ)> , :AssistantOfBarbara ;
        :Located-In       :CzechRepublic ;
        :Part-Of          :Creation_Artwork_77 ;
        :Requires-Use-Of  :BlowingPipe , :Hook , :Water , :AirCompressor , :StraightShears , :BitIron , :Gloves , :Tagliol , :DiamondShears , :AnnealingKiln , :Pincet , :CeramicPotFilledWithGlass , :Blocks , :Jacks , :YokeOfSupport , :PropaneTorch , :GloryHole , :Marver , :IcePick , :Paper , :Furnace , :Pontis , :Fork , :InterchangeableMetalMoldSetup , :Beeswax .

:ARTWORK_39_Resting  a    :Resting , owl:NamedIndividual ;
        rdfs:comment      "Instance of an activity which is part of the creation process of ARTWORK_39."@en ;
        rdfs:label        "ARTWORK_39_Resting"@en ;
        :Followed-By      <http://www.semanticweb.org/ontologies/Daan/2020/BarbaraNanning#ARTWORK_39_ExaminingQuality(CheckForIrregularitiesInTheGlass)> ;
        :Follows          :ARTWORK_39_Transporting ;
        :Has-Duration     <http://www.semanticweb.org/ontologies/Daan/2020/BarbaraNanning#2015> ;
        :Involves         :AlešZvěřina ;
        :Located-In       :NovyBor ;
        :Part-Of          :Creation_Artwork_39 ;
        :Requires-Use-Of  :AnnealingKiln .

:ARTWORK_46_Resting  a    :Resting , owl:NamedIndividual ;
        rdfs:comment      "Instance of an activity which is part of the creation process of ARTWORK_46."@en ;
        rdfs:label        "ARTWORK_46_Resting"@en ;
        :Followed-By      <http://www.semanticweb.org/ontologies/Daan/2020/BarbaraNanning#ARTWORK_46_ExaminingQuality(CheckForIrregularitiesInTheGlass)> ;
        :Follows          :ARTWORK_46_Transporting ;
        :Has-Duration     <http://www.semanticweb.org/ontologies/Daan/2020/BarbaraNanning#2018> ;
        :Involves         :AlešZvěřina ;
        :Located-In       :NovyBor ;
        :Part-Of          :Creation_Artwork_46 ;
        :Requires-Use-Of  :AnnealingKiln .

:Duration-Of  a        owl:ObjectProperty ;
        rdfs:comment   "Duration-Of is a property which connects an event to a timespan."@en ;
        rdfs:domain    :Timespan ;
        rdfs:label     "Duration-Of"@en ;
        rdfs:range     :Event ;
        owl:inverseOf  :Has-Duration .

:ARTWORK_79_HeatingMetalMold
        a                 :Heating_Metal_Mold , owl:NamedIndividual ;
        rdfs:comment      "Instance of an activity which is part of the creation process of ARTWORK_79."@en ;
        rdfs:label        "ARTWORK_79_Heating Metal Mold"@en ;
        :Followed-By      :ARTWORK_79_Glassblowing ;
        :Follows          :ARTWORK_79_ApplyingExtraColour_2 ;
        :Has-Duration     <http://www.semanticweb.org/ontologies/Daan/2020/BarbaraNanning#2018> ;
        :Involves         :BarbaraNanning ;
        :Located-In       :CzechRepublic ;
        :Part-Of          :Creation_Artwork_79 ;
        :Requires-Use-Of  :InterchangeableMetalMoldSetup , :Gloves , :PropaneTorch .

:Brussels  a          :City , owl:NamedIndividual ;
        rdfs:comment  "Brussels is a city in Belgium."@en ;
        rdfs:label    "Brussels"@en ;
        :Located-In   :Belgium ;
        :Location-Of  :PierreMarieGiraud .

<http://www.semanticweb.org/ontologies/Daan/2020/BarbaraNanning#2017>
        a             owl:NamedIndividual , :Timespan ;
        rdfs:comment  "2017 is a Timespan."@en ;
        rdfs:label    "2017"@en ;
        owl:sameAs    <http://www.wikidata.org/entity/Q25290> ;
        :Duration-Of  :Creation_Artwork_75 .

:Has-Height  a       owl:DatatypeProperty ;
        rdfs:domain  :Thing ;
        rdfs:range   xsd:integer .

<http://vocab.getty.edu/aat/300146236>
        a                    owl:Class ;
        owl:equivalentClass  :Private_Collection .

:ARTWORK_75_Signing  a    :Signing , owl:NamedIndividual ;
        rdfs:comment      "Instance of an activity which is part of the creation process of ARTWORK_75."@en ;
        rdfs:label        "ARTWORK_75_Signing"@en ;
        :Followed-By      :ARTWORK_75_Packing_3 ;
        :Follows          :ARTWORK_75_Sandblasting ;
        :Has-Duration     <http://www.semanticweb.org/ontologies/Daan/2020/BarbaraNanning#2018> ;
        :Involves         :BarbaraNanning , :AlešZvěřina ;
        :Located-In       :CzechRepublic ;
        :Part-Of          :Creation_Artwork_75 ;
        :Requires-Use-Of  :AirCompressor .

:ARTWORK_75_Gilding  a    :Gilding , owl:NamedIndividual ;
        rdfs:comment      "Instance of an activity which is part of the creation process of ARTWORK_75."@en ;
        rdfs:label        "ARTWORK_75_Gilding"@en ;
        :Followed-By      <http://www.semanticweb.org/ontologies/Daan/2020/BarbaraNanning#ARTWORK_75_ExaminingQuality(FinalResult)> ;
        :Follows          :ARTWORK_75_Transporting_3 ;
        :Has-Duration     <http://www.semanticweb.org/ontologies/Daan/2020/BarbaraNanning#2017> ;
        :Involves         :BarbaraNanning , :VáçlavNovák_Doksy_CzechRepublic ;
        :Located-In       :CzechRepublic ;
        :Part-Of          :Creation_Artwork_75 ;
        :Requires-Use-Of  :GildingCushion , :GildersTip , :GildersKnife , :INSTACOLLTool .

:GildersKnife  a      :Tool , owl:NamedIndividual ;
        rdfs:comment  "The gilder knife is a tool used together with a gilding cushion to cut gold leaf. A gold knife has two sharpened edges that are sharpened at an angle. This quality knife has a leather sheath that can be hung under the gold cushion."@en ;
        rdfs:label    "Gilders Knife"@en ;
        :Made-Out-Of  :Leather ;
        :Used-For     :ARTWORK_79_Gilding , :ARTWORK_73_Gilding , :ARTWORK_76_Gilding , :ARTWORK_80_Gilding , :ARTWORK_75_Gilding , :ARTWORK_77_Gilding , :ARTWORK_78_Gilding , :ARTWORK_74_Gilding , :ARTWORK_43_Gilding , :ARTWORK_44_Gilding .

:ARTWORK_36_FusingSheets
        a                 owl:NamedIndividual , :Fusing_Sheets ;
        rdfs:comment      "Instance of an activity which is part of the creation process of ARTWORK_36."@en ;
        rdfs:label        "ARTWORK_36_Fusing Sheets"@en ;
        :Followed-By      :ARTWORK_36_FlatFusingSheetsWithARTWORK36PeacockToOnePanel ;
        :Follows          :ARTWORK_36_OrdeningFlatSheets ;
        :Has-Duration     <http://www.semanticweb.org/ontologies/Daan/2020/BarbaraNanning#2019> ;
        :Involves         :BarbaraNanning ;
        :Located-In       :Amsterdam ;
        :Part-Of          :Creation_Artwork_36 ;
        :Requires-Use-Of  :FusingKiln .

:ARTWORK_77_Transporting_3
        a              :Transporting , owl:NamedIndividual ;
        rdfs:comment   "Instance of an activity which is part of the creation process of ARTWORK_77."@en ;
        rdfs:label     "ARTWORK_77_Transporting_3"@en ;
        :Followed-By   :ARTWORK_77_Gilding ;
        :Follows       :ARTWORK_77_Packing_3 ;
        :Has-Duration  <http://www.semanticweb.org/ontologies/Daan/2020/BarbaraNanning#2018> ;
        :Involves      :BarbaraNanning , :AlešZvěřina ;
        :Located-In    :CzechRepublic ;
        :Part-Of       :Creation_Artwork_77 .

:Beeswax  a           :Equipment , owl:NamedIndividual ;
        rdfs:comment  "Beeswax is the wax secreted by bees to make honeycombs and used to make e.g. candles."@en ;
        rdfs:label    "Beeswax"@en ;
        owl:sameAs    <http://www.wikidata.org/entity/Q143739> ;
        :Used-For     :ARTWORK_74_ApplyingClearGlassBell , :ARTWORK_44_ApplyingClearGlassBell , :ARTWORK_78_ApplyingExtraColour , :ARTWORK_77_ApplyingClearGlassBell , :ARTWORK_75_Glassblowing , :ARTWORK_79_ApplyingExtraColour_2 , :ARTWORK_78_Glassblowing , :ARTWORK_76_Glassblowing , :ARTWORK_74_ApplyingExtraColour_2 , :ARTWORK_78_ApplyingClearGlassBell , :ARTWORK_73_Glassblowing , :ARTWORK_76_ApplyingExtraColour_2 , :ARTWORK_76_ApplyingExtraColour , :ARTWORK_77_Glassblowing , :ARTWORK_79_Glassblowing , :ARTWORK_80_Glassblowing , :ARTWORK_43_ApplyingClearGlassBell , :ARTWORK_80_ApplyingClearGlassBell , :ARTWORK_76_ApplyingClearGlassBell , :ARTWORK_77_ApplyingExtraColour , :ARTWORK_73_ApplyingClearGlassBell , :ARTWORK_74_ApplyingExtraColour , :ARTWORK_43_Glassblowing , :ARTWORK_79_ApplyingExtraColour , :ARTWORK_79_ApplyingClearGlassBell , :ARTWORK_44_ApplyingExtraColour_2 , :ARTWORK_44_Glassblowing , :ARTWORK_74_Glassblowing , :ARTWORK_44_ApplyingExtraColour , :ARTWORK_75_ApplyingExtraColour , :ARTWORK_75_ApplyingClearGlassBell , :ARTWORK_43_ApplyingExtraColour , :ARTWORK_80_ApplyingExtraColour , :ARTWORK_75_ApplyingExtraColour_2 .

<http://vocab.getty.edu/aat/300053072>
        a                    owl:Class ;
        owl:equivalentClass  :Sawing .

:ARTWORK_39_ExaminingTheQualityOfTheGlass
        a                 owl:NamedIndividual , :Examining_the_Quality_of_the_Glass ;
        rdfs:comment      "Instance of an activity which is part of the creation process of ARTWORK_39."@en ;
        rdfs:label        "ARTWORK_39_Deciding Colour Palette_2"@en ;
        :Followed-By      :ARTWORK_39_ApplyingClearGlassBell ;
        :Follows          :ARTWORK_39_SetupAndTestingOfTheMetalMold ;
        :Has-Duration     <http://www.semanticweb.org/ontologies/Daan/2020/BarbaraNanning#2015> ;
        :Involves         :GertBullée , :BarbaraNanning , :DurkValkema ;
        :Located-In       :Zaandam ;
        :Part-Of          :Creation_Artwork_39 ;
        :Requires-Use-Of  :Paper , :StraightShears , :Water , :Furnace , :GloryHole , :Jacks , :Pontis , :Blocks , :BlowingPipe , :CeramicPotFilledWithGlass , :YokeOfSupport , :DiamondShears , :AnnealingKiln .

:ARTWORK_80_HeatingMetalMold
        a                 :Heating_Metal_Mold , owl:NamedIndividual ;
        rdfs:comment      "Instance of an activity which is part of the creation process of ARTWORK_80."@en ;
        rdfs:label        "ARTWORK_80_Heating Metal Mold"@en ;
        :Followed-By      :ARTWORK_80_Glassblowing ;
        :Follows          :ARTWORK_80_ApplyingExtraColour ;
        :Has-Duration     <http://www.semanticweb.org/ontologies/Daan/2020/BarbaraNanning#2018> ;
        :Involves         :BarbaraNanning ;
        :Located-In       :CzechRepublic ;
        :Part-Of          :Creation_Artwork_80 ;
        :Requires-Use-Of  :Gloves , :PropaneTorch , :InterchangeableMetalMoldSetup .

<http://vocab.getty.edu/aat/300011845>
        a           owl:NamedIndividual ;
        owl:sameAs  :Leather .

<http://www.wikidata.org/entity/Q43229>
        a                owl:Class ;
        rdfs:subClassOf  :Actor .

:ARTWORK_79_ApplyingExtraColour
        a                 owl:NamedIndividual , :Applying_Extra_Colour ;
        rdfs:comment      "Instance of an activity which is part of the creation process of ARTWORK_79."@en ;
        rdfs:label        "ARTWORK_79_Applying Extra Colour"@en ;
        :Followed-By      :ARTWORK_79_ApplyingExtraColour_2 ;
        :Follows          :ARTWORK_79_ApplyingClearGlassBell ;
        :Has-Duration     <http://www.semanticweb.org/ontologies/Daan/2020/BarbaraNanning#2018> ;
        :Involves         <http://www.semanticweb.org/ontologies/Daan/2020/BarbaraNanning#RadekKoten(CZ)> , :BarbaraNanning , <http://www.semanticweb.org/ontologies/Daan/2020/BarbaraNanning#LukasHavlas(CZ)> ;
        :Located-In       :CzechRepublic ;
        :Part-Of          :Creation_Artwork_79 ;
        :Processes        :AJETOWhiteGlass ;
        :Requires-Use-Of  :IcePick , :Paper , :Jacks , :Pincet , :StraightShears , :DiamondShears , :AirCompressor , :Marver , :Blocks , :Furnace , :Beeswax , :CeramicPotFilledWithGlass , :GloryHole , :Garage , :BlowingPipe , :Water , :Hook , :AnnealingKiln , :Tagliol , :Fork , :YokeOfSupport , :Pontis .

:EffieHalkidis  a     :Assisting_Team_Member , owl:NamedIndividual ;
        rdfs:comment  "Effie Halkidis (Greece) is an Assisting Team Member."@en ;
        rdfs:label    "Effie Halkidis"@en .

:ARTWORK_39_FillingKilnsWithMetalBowl
        a                 :Filling_Kilns_with_Metal_Bowl , owl:NamedIndividual ;
        rdfs:comment      "Instance of an activity which is part of the creation process of ARTWORK_39."@en ;
        rdfs:label        "ARTWORK_39_Filling Kilns with Metal Bowl"@en ;
        :Followed-By      :ARTWORK_39_PreparingGlass ;
        :Follows          :ARTWORK_39_PreparingForBlowing ;
        :Has-Duration     <http://www.semanticweb.org/ontologies/Daan/2020/BarbaraNanning#2015> ;
        :Involves         :BarbaraNanning , :DurkValkema ;
        :Located-In       :Zaandam ;
        :Part-Of          :Creation_Artwork_39 ;
        :Requires-Use-Of  :Gloves , :FusingKiln , :Garage .

<http://sws.geonames.org/2759794>
        a           owl:NamedIndividual ;
        owl:sameAs  :Amsterdam .

:Sawing  a               owl:Class ;
        rdfs:comment     "Sawing is an activity in which a thing is cut using a saw."@en ;
        rdfs:label       "Sawing"@en ;
        rdfs:subClassOf  :Activity .

:ARTWORK_76_Glassblowing
        a                 owl:NamedIndividual , :Glassblowing ;
        rdfs:comment      "Instance of an activity which is part of the creation process of ARTWORK_76."@en ;
        rdfs:label        "ARTWORK_76_Glassblowing"@en ;
        :Followed-By      :ARTWORK_76_Sensing ;
        :Follows          :ARTWORK_76_HeatingMetalMold ;
        :Has-Duration     <http://www.semanticweb.org/ontologies/Daan/2020/BarbaraNanning#2018> ;
        :Involves         <http://www.semanticweb.org/ontologies/Daan/2020/BarbaraNanning#LukasHavlas(CZ)> , <http://www.semanticweb.org/ontologies/Daan/2020/BarbaraNanning#JiriMoravec(CZ)> , <http://www.semanticweb.org/ontologies/Daan/2020/BarbaraNanning#RadekKoten(CZ)> , :BarbaraNanning , <http://www.semanticweb.org/ontologies/Daan/2020/BarbaraNanning#Tom%C3%A1%C5%A1Moravec(CZ)> , :AssistantOfBarbara ;
        :Located-In       :CzechRepublic ;
        :Part-Of          :Creation_Artwork_76 ;
        :Requires-Use-Of  :Gloves , :Water , :BitIron , :Beeswax , :PropaneTorch , :Furnace , :Jacks , :BlowingPipe , :GloryHole , :Tagliol , :Hook , :Marver , :YokeOfSupport , :StraightShears , :DiamondShears , :Paper , :AirCompressor , :Pincet , :IcePick , :CeramicPotFilledWithGlass , :Pontis , :InterchangeableMetalMoldSetup , :AnnealingKiln , :Fork , :Blocks .

<http://www.wikidata.org/entity/Q45621>
        a       owl:NamedIndividual .

:PolishingStone  a    owl:NamedIndividual , :Tool ;
        rdfs:comment  "A polishing stone is a stone used by an actor for polishing an object or material."@en ;
        rdfs:label    "Polishing Stone"@en ;
        :Used-For     :ARTWORK_80_Polishing , :ARTWORK_74_Polishing , :ARTWORK_78_Polishing , :ARTWORK_73_Polishing , :ARTWORK_44_Polishing , :ARTWORK_79_Polishing , :ARTWORK_75_Polishing , :ARTWORK_77_Polishing , :ARTWORK_76_Polishing , :ARTWORK_43_Polishing .

:Natural_Material  a     owl:Class ;
        rdfs:comment     "Natural Material refers to a material matter created without human intervention."@en ;
        rdfs:label       "Natural Material"@en ;
        rdfs:subClassOf  :Material .

:DurkValkema  a       owl:NamedIndividual , :Supervisor_Works ;
        rdfs:comment  "Durk Valkema is a Supervisor Works"@en ;
        rdfs:label    "Durk Valkema"@en ;
        owl:sameAs    <http://www.wikidata.org/entity/Q29422094> ;
        :Involved-In  :ARTWORK_18_64_ProducingColouredCanes , :ARTWORK_46_ProducingColouredCanes , <http://www.semanticweb.org/ontologies/Daan/2020/BarbaraNanning#ARTWORK_36_ExaminingQuality(Shape/Form)> , :ARTWORK_39_Cooling , :ARTWORK_18_64_Cooling , :ARTWORK_36_ExaminingTheQualityOfTheGlass , <http://www.semanticweb.org/ontologies/Daan/2020/BarbaraNanning#ARTWORK_39_ExaminingQuality(Shape/Form)> , :ARTWORK_36_Cooling , :ARTWORK_39_ExaminingTheQualityOfTheGlass , :ARTWORK_36_PreparingForBlowing , :ARTWORK_36_FillingKilnsWithMetalBowl , :ARTWORK_39_PreparingForBlowing , :ARTWORK_39_FillingKilnsWithMetalBowl , <http://www.semanticweb.org/ontologies/Daan/2020/BarbaraNanning#ARTWORK_18_64_ExaminingQuality(Shape/Form)> , :ARTWORK_36_ProducingColouredCanes ;
        :Works-For    :VRIJGLASZaandam .

<http://vocab.getty.edu/aat/300025687>
        a                    owl:Class ;
        owl:equivalentClass  :Photographer .

<http://www.cidoc-crm.org/cidoc-crm/E53_Place>
        a                    owl:Class ;
        owl:equivalentClass  :Place .

:ARTWORK_36_Packing_2
        a              :Packing , owl:NamedIndividual ;
        rdfs:comment   "Instance of an activity which is part of the creation process of ARTWORK_36."@en ;
        rdfs:label     "ARTWORK_36_Packing_2"@en ;
        :Followed-By   :ARTWORK_36_Transporting_2 ;
        :Follows       :ARTWORK_36_MeasuringAndBoxesMaking ;
        :Has-Duration  <http://www.semanticweb.org/ontologies/Daan/2020/BarbaraNanning#2015> ;
        :Involves      :BarbaraNanning ;
        :Located-In    :NovyBor ;
        :Part-Of       :Creation_Artwork_36 .

:Hook   a             :Tool , owl:NamedIndividual ;
        rdfs:comment  "A hook is a piece of metal material curved at an angle"@en ;
        rdfs:label    "Hook"@en ;
        :Used-For     :ARTWORK_77_Glassblowing , :ARTWORK_80_Glassblowing , :ARTWORK_74_ApplyingExtraColour , :ARTWORK_75_ApplyingClearGlassBell , :ARTWORK_79_ApplyingClearGlassBell , :ARTWORK_44_ApplyingClearGlassBell , :ARTWORK_43_ApplyingExtraColour , :ARTWORK_73_Glassblowing , :ARTWORK_76_ApplyingClearGlassBell , :ARTWORK_80_ApplyingExtraColour , :ARTWORK_73_ApplyingClearGlassBell , :ARTWORK_75_ApplyingExtraColour_2 , :ARTWORK_43_Glassblowing , :ARTWORK_43_ApplyingClearGlassBell , :ARTWORK_78_ApplyingClearGlassBell , :ARTWORK_80_ApplyingClearGlassBell , :ARTWORK_78_Glassblowing , :ARTWORK_44_Glassblowing , :ARTWORK_79_Glassblowing , :ARTWORK_76_ApplyingExtraColour_2 , :ARTWORK_44_ApplyingExtraColour , :ARTWORK_77_ApplyingClearGlassBell , :ARTWORK_44_ApplyingExtraColour_2 , :ARTWORK_79_ApplyingExtraColour_2 , :ARTWORK_74_Glassblowing , :ARTWORK_79_ApplyingExtraColour , :ARTWORK_74_ApplyingClearGlassBell , :ARTWORK_76_Glassblowing , :ARTWORK_77_ApplyingExtraColour , :ARTWORK_74_ApplyingExtraColour_2 , :ARTWORK_75_Glassblowing , :ARTWORK_75_ApplyingExtraColour , :ARTWORK_78_ApplyingExtraColour , :ARTWORK_76_ApplyingExtraColour .

:ARTWORK_75_Packing_4
        a              owl:NamedIndividual , :Packing ;
        rdfs:comment   "Instance of an activity which is part of the creation process of ARTWORK_75."@en ;
        rdfs:label     "ARTWORK_75_Packing_4"@en ;
        :Followed-By   :ARTWORK_75_Transporting_4 ;
        :Follows       <http://www.semanticweb.org/ontologies/Daan/2020/BarbaraNanning#ARTWORK_75_ExaminingQuality(FinalResult)> ;
        :Has-Duration  <http://www.semanticweb.org/ontologies/Daan/2020/BarbaraNanning#2018> ;
        :Involves      :VáçlavNovák_Doksy_CzechRepublic , :AlešZvěřina , :BarbaraNanning ;
        :Located-In    :CzechRepublic ;
        :Part-Of       :Creation_Artwork_75 .

:ARTWORK_46_Packing_2
        a              :Packing , owl:NamedIndividual ;
        rdfs:comment   "Instance of an activity which is part of the creation process of ARTWORK_46."@en ;
        rdfs:label     "ARTWORK_46_Packing_2"@en ;
        :Followed-By   :ARTWORK_46_Transporting_2 ;
        :Follows       :ARTWORK_46_MeasuringAndBoxesMaking ;
        :Has-Duration  <http://www.semanticweb.org/ontologies/Daan/2020/BarbaraNanning#2018> ;
        :Involves      :BarbaraNanning ;
        :Located-In    :NovyBor ;
        :Part-Of       :Creation_Artwork_46 .

:ARTWORK_39_OrdeningMonochromeSheetsAndStrings
        a                 :Ordening_Monochrome_Sheets_and_Strings , owl:NamedIndividual ;
        rdfs:comment      "Instance of an activity which is part of the creation process of ARTWORK_39."@en ;
        rdfs:label        "ARTWORK_39_Ordening Monochrome Sheets and Strings"@en ;
        :Followed-By      :ARTWORK_39_CuttingSheets ;
        :Follows          :ARTWORK_39_DecidingColourPalette ;
        :Has-Duration     <http://www.semanticweb.org/ontologies/Daan/2020/BarbaraNanning#2015> ;
        :Involves         :BarbaraNanning ;
        :Located-In       :Amsterdam ;
        :Part-Of          :Creation_Artwork_39 ;
        :Requires-Use-Of  :Computer .

:ARTWORK_17_33_Modeling
        a                 owl:NamedIndividual , :Modeling ;
        rdfs:comment      "Instance of an activity which is part of the creation process of ARTWORK_17_33."@en ;
        rdfs:label        "ARTWORK_17_33_Modeling"@en ;
        :Followed-By      <http://www.semanticweb.org/ontologies/Daan/2020/BarbaraNanning#ARTWORK_17_33_ExaminingQuality(Shape/Form)> ;
        :Follows          :ARTWORK_17_33_Sensing ;
        :Has-Duration     <http://www.semanticweb.org/ontologies/Daan/2020/BarbaraNanning#2017> ;
        :Involves         :AssistantOfBarbara , :BarbaraNanning , <http://www.semanticweb.org/ontologies/Daan/2020/BarbaraNanning#JiriMoravec(CZ)> , <http://www.semanticweb.org/ontologies/Daan/2020/BarbaraNanning#RadekKoten(CZ)> , <http://www.semanticweb.org/ontologies/Daan/2020/BarbaraNanning#Tom%C3%A1%C5%A1Moravec(CZ)> , <http://www.semanticweb.org/ontologies/Daan/2020/BarbaraNanning#LukasHavlas(CZ)> ;
        :Located-In       :Lindava ;
        :Part-Of          :Creation_Artwork_17_33 ;
        :Requires-Use-Of  :BlowingPipe , :PropaneTorch , :AirCompressor , :InterchangeableMetalMoldSetup , :Gloves .

:ARTWORK_36_Transporting
        a              :Transporting , owl:NamedIndividual ;
        rdfs:comment   "Instance of an activity which is part of the creation process of ARTWORK_36."@en ;
        rdfs:label     "ARTWORK_36_Transporting"@en ;
        :Followed-By   :ARTWORK_36_Resting ;
        :Follows       :ARTWORK_36_Packing ;
        :Has-Duration  <http://www.semanticweb.org/ontologies/Daan/2020/BarbaraNanning#2015> ;
        :Involves      :BarbaraNanning , :AlešZvěřina ;
        :Located-In    :NovyBor ;
        :Part-Of       :Creation_Artwork_36 .

:ARTWORK_74_Signing  a    :Signing , owl:NamedIndividual ;
        rdfs:comment      "Instance of an activity which is part of the creation process of ARTWORK_74."@en ;
        rdfs:label        "ARTWORK_74_Signing"@en ;
        :Followed-By      :ARTWORK_74_Packing_3 ;
        :Follows          :ARTWORK_74_Transporting_2 ;
        :Has-Duration     <http://www.semanticweb.org/ontologies/Daan/2020/BarbaraNanning#2008> ;
        :Involves         :BarbaraNanning , :AlešZvěřina ;
        :Located-In       :CzechRepublic ;
        :Part-Of          :Creation_Artwork_74 ;
        :Requires-Use-Of  :AirCompressor .

:ARTWORK_74_Gilding  a    :Gilding , owl:NamedIndividual ;
        rdfs:comment      "Instance of an activity which is part of the creation process of ARTWORK_74."@en ;
        rdfs:label        "ARTWORK_74_Gilding"@en ;
        :Followed-By      <http://www.semanticweb.org/ontologies/Daan/2020/BarbaraNanning#ARTWORK_74_ExaminingQuality(FinalResult)> ;
        :Follows          :ARTWORK_74_Transporting_3 ;
        :Has-Duration     <http://www.semanticweb.org/ontologies/Daan/2020/BarbaraNanning#2008> ;
        :Involves         :VáçlavNovák_Doksy_CzechRepublic , :BarbaraNanning ;
        :Located-In       :CzechRepublic ;
        :Part-Of          :Creation_Artwork_74 ;
        :Requires-Use-Of  :GildersKnife , :GildingCushion , :GildersTip , :INSTACOLLTool .

:ARTWORK_76_SetupAndTestingOfTheMetalMold_2
        a                 :Setup_and_Testing_of_the_Metal_Mold , owl:NamedIndividual ;
        rdfs:comment      "Instance of an activity which is part of the creation process of ARTWORK_76."@en ;
        rdfs:label        "ARTWORK_76_Setup and Testing of the Metal Mold_2"@en ;
        :Followed-By      :ARTWORK_76_ApplyingClearGlassBell ;
        :Follows          :ARTWORK_76_ExaminingTheQualityOfTheGlass ;
        :Has-Duration     <http://www.semanticweb.org/ontologies/Daan/2020/BarbaraNanning#2018> ;
        :Involves         <http://www.semanticweb.org/ontologies/Daan/2020/BarbaraNanning#Tom%C3%A1%C5%A1Moravec(CZ)> , <http://www.semanticweb.org/ontologies/Daan/2020/BarbaraNanning#RadekKoten(CZ)> , :AssistantOfBarbara , :BarbaraNanning , <http://www.semanticweb.org/ontologies/Daan/2020/BarbaraNanning#JiriMoravec(CZ)> , <http://www.semanticweb.org/ontologies/Daan/2020/BarbaraNanning#LukasHavlas(CZ)> ;
        :Located-In       :CzechRepublic ;
        :Part-Of          :Creation_Artwork_76 ;
        :Requires-Use-Of  :InterchangeableMetalMoldSetup .

<http://vocab.getty.edu/aat/300014588>
        a           owl:NamedIndividual ;
        owl:sameAs  :Beeswax .

:JiříPačinekJunior  a  :Third_Glass_Blower , owl:NamedIndividual ;
        rdfs:comment  "Jiří Pačinek junior is a Third Glass Blower."@en ;
        rdfs:label    "Jiří Pačinek junior"@en ;
        :Involved-In  :ARTWORK_36_ApplyingMassivePieceOfClearGlass , :ARTWORK_46_PickingUpColouredCanesPattern , :ARTWORK_36_Modeling_2 , :ARTWORK_46_SetupAndTestingOfTheMetalMold , :ARTWORK_46_Glassblowing , :ARTWORK_46_Modeling , :ARTWORK_46_ApplyingClearOverlay ;
        :Works-For    <http://www.semanticweb.org/ontologies/Daan/2020/BarbaraNanning#Ji%C5%99%C3%ADPa%C4%8DinekLindava(CZ)> .

:Material  a                 owl:Class ;
        rdfs:comment         "Material is the matter used to create a thing."@en ;
        rdfs:label           "Material"@en ;
        rdfs:subClassOf      :Thing ;
        owl:equivalentClass  <https://data.cultureelerfgoed.nl/term/id/abr/2dcb88e1-e777-4cff-babc-d97485b42b10> .

:ARTWORK_36_DecidingColourPaletteAndPatterns_2
        a              owl:NamedIndividual , :Deciding_Colour_Palette_and_Patterns ;
        rdfs:comment   "Instance of an activity which is part of the creation process of ARTWORK_36."@en ;
        rdfs:label     "ARTWORK_36_Deciding Colour Palette and Patterns_2"@en ;
        :Followed-By   :ARTWORK_36_TransportingMonochromeRods ;
        :Follows       :ARTWORK_36_CuttingAndPolishingCastedMonochromeSheetsToSmallRods ;
        :Has-Duration  <http://www.semanticweb.org/ontologies/Daan/2020/BarbaraNanning#2015> ;
        :Involves      :BarbaraNanning ;
        :Located-In    :Amsterdam ;
        :Part-Of       :Creation_Artwork_36 .

:ARTWORK_75_Glassblowing
        a                 :Glassblowing , owl:NamedIndividual ;
        rdfs:comment      "Instance of an activity which is part of the creation process of ARTWORK_75."@en ;
        rdfs:label        "ARTWORK_75_Glassblowing"@en ;
        :Followed-By      :ARTWORK_75_Sensing ;
        :Follows          :ARTWORK_75_HeatingMetalMold ;
        :Has-Duration     <http://www.semanticweb.org/ontologies/Daan/2020/BarbaraNanning#2018> ;
        :Involves         <http://www.semanticweb.org/ontologies/Daan/2020/BarbaraNanning#LukasHavlas(CZ)> , :BarbaraNanning , <http://www.semanticweb.org/ontologies/Daan/2020/BarbaraNanning#RadekKoten(CZ)> , <http://www.semanticweb.org/ontologies/Daan/2020/BarbaraNanning#Tom%C3%A1%C5%A1Moravec(CZ)> , <http://www.semanticweb.org/ontologies/Daan/2020/BarbaraNanning#JiriMoravec(CZ)> , :AssistantOfBarbara ;
        :Located-In       :CzechRepublic ;
        :Part-Of          :Creation_Artwork_75 ;
        :Requires-Use-Of  :Beeswax , :Blocks , :IcePick , :BitIron , :Pincet , :Jacks , :DiamondShears , :AnnealingKiln , :Furnace , :GloryHole , :YokeOfSupport , :AirCompressor , :Fork , :BlowingPipe , :InterchangeableMetalMoldSetup , :Tagliol , :PropaneTorch , :CeramicPotFilledWithGlass , :Water , :Pontis , :Hook , :Marver , :Paper , :StraightShears , :Gloves .

:ARTWORK_75_SetupAndTestingOfTheMetalMold_2
        a                 :Setup_and_Testing_of_the_Metal_Mold , owl:NamedIndividual ;
        rdfs:comment      "Instance of an activity which is part of the creation process of ARTWORK_75."@en ;
        rdfs:label        "ARTWORK_75_Setup and Testing of the Metal Mold_2"@en ;
        :Followed-By      :ARTWORK_75_ApplyingClearGlassBell ;
        :Follows          :ARTWORK_75_ExaminingTheQualityOfTheGlass ;
        :Has-Duration     <http://www.semanticweb.org/ontologies/Daan/2020/BarbaraNanning#2018> ;
        :Involves         <http://www.semanticweb.org/ontologies/Daan/2020/BarbaraNanning#Tom%C3%A1%C5%A1Moravec(CZ)> , <http://www.semanticweb.org/ontologies/Daan/2020/BarbaraNanning#RadekKoten(CZ)> , <http://www.semanticweb.org/ontologies/Daan/2020/BarbaraNanning#LukasHavlas(CZ)> , <http://www.semanticweb.org/ontologies/Daan/2020/BarbaraNanning#JiriMoravec(CZ)> , :BarbaraNanning , :AssistantOfBarbara ;
        :Located-In       :CzechRepublic ;
        :Part-Of          :Creation_Artwork_75 ;
        :Requires-Use-Of  :InterchangeableMetalMoldSetup .

:ARTWORK_76_HeatingMetalMold
        a                 :Heating_Metal_Mold , owl:NamedIndividual ;
        rdfs:comment      "Instance of an activity which is part of the creation process of ARTWORK_76."@en ;
        rdfs:label        "ARTWORK_76_Heating Metal Mold"@en ;
        :Followed-By      :ARTWORK_76_Glassblowing ;
        :Follows          :ARTWORK_76_ApplyingExtraColour_2 ;
        :Has-Duration     <http://www.semanticweb.org/ontologies/Daan/2020/BarbaraNanning#2018> ;
        :Involves         :BarbaraNanning ;
        :Located-In       :CzechRepublic ;
        :Part-Of          :Creation_Artwork_76 ;
        :Requires-Use-Of  :PropaneTorch , :InterchangeableMetalMoldSetup , :Gloves .

:ARTWORK_44_Cooling  a    owl:NamedIndividual , :Cooling ;
        rdfs:comment      "Instance of an activity which is part of the creation process of ARTWORK_44."@en ;
        rdfs:label        "ARTWORK_44_Cooling"@en ;
        :Followed-By      :ARTWORK_44_Packing ;
        :Follows          :ARTWORK_44_Translocating ;
        :Has-Duration     <http://www.semanticweb.org/ontologies/Daan/2020/BarbaraNanning#2018> ;
        :Involves         :AssistantOfBarbara , :LuděkKout ;
        :Located-In       :CzechRepublic ;
        :Part-Of          :Creation_Artwork_44 ;
        :Requires-Use-Of  :AnnealingKiln .

:Image_Artwork_39  a            :Digital_Image , owl:NamedIndividual ;
        rdfs:comment            "Image of Artwork_39 by Barbara Nanning."@en ;
        rdfs:label              "Image_Artwork_39"@en ;
        :Representation-Source  "Tom Haartsen_Ouderkerk A/d Amstel (NL)"@en ;
        :Shows                  :Artwork_39 .

:Has-Temperature  a   owl:DatatypeProperty ;
        rdfs:comment  "Has-Temperature is a property which connects a thing with a (range in) temperature in ºC."@en ;
        rdfs:domain   :Thing ;
        rdfs:label    "Has-Temperature"@en ;
        rdfs:range    xsd:integer .

:VáçlavNovák_Doksy_CzechRepublic
        a             owl:NamedIndividual , :Gilder ;
        rdfs:comment  "Váçlav Novák_Doksy_Czech Republic is a Gilder."@en ;
        rdfs:label    "Váçlav Novák_Doksy_Czech Republic"@en ;
        :Involved-In  :ARTWORK_80_Gilding , :ARTWORK_78_Packing_4 , :ARTWORK_76_Packing_4 , :ARTWORK_75_Packing_4 , :ARTWORK_44_Packing_4 , :ARTWORK_74_Packing_4 , :ARTWORK_79_Packing_4 , :ARTWORK_79_Gilding , :ARTWORK_77_Gilding , :ARTWORK_76_Gilding , :ARTWORK_74_Gilding , :ARTWORK_75_Gilding , :ARTWORK_77_Packing_4 , :ARTWORK_44_Gilding , :ARTWORK_73_Packing_4 , :ARTWORK_73_Gilding , :ARTWORK_43_Packing_4 , :ARTWORK_78_Gilding ;
        :Maker-Of     :Artwork_74 , :Artwork_78 , :Artwork_75 , :Artwork_73 , :Artwork_79 , :Artwork_76 , :Artwork_80 , :Artwork_77 , :Artwork_44 , :Artwork_43 .

:ARTWORK_17_33_ExaminingTheQualityOfTheGlass
        a                 :Examining_the_Quality_of_the_Glass , owl:NamedIndividual ;
        rdfs:comment      "Instance of an activity which is part of the creation process of ARTWORK_17_33."@en ;
        rdfs:label        "ARTWORK_17_33_Examining the Quality of the Glass"@en ;
        :Followed-By      :ARTWORK_17_33_ApplyingClearGlassBell ;
        :Follows          :ARTWORK_17_33_PreparingGlass ;
        :Has-Duration     <http://www.semanticweb.org/ontologies/Daan/2020/BarbaraNanning#2017> ;
        :Involves         :LuděkKout , :BarbaraNanning , <http://www.semanticweb.org/ontologies/Daan/2020/BarbaraNanning#RadekKoten(CZ)> ;
        :Located-In       :Lindava ;
        :Part-Of          :Creation_Artwork_17_33 ;
        :Requires-Use-Of  :Jacks , :DiamondShears , :YokeOfSupport , :CeramicPotFilledWithGlass , :BlowingPipe , :Blocks , :Paper , :GloryHole , :Furnace , :StraightShears , :Pontis , :Water , :AnnealingKiln .

:ARTWORK_73_Documenting
        a              :Documenting , owl:NamedIndividual ;
        rdfs:comment   "Instance of an activity which is part of the creation process of ARTWORK_73."@en ;
        rdfs:label     "ARTWORK_73_Documenting"@en ;
        :Followed-By   :ARTWORK_73_Packing_5 ;
        :Follows       :ARTWORK_73_Photographing ;
        :Has-Duration  <http://www.semanticweb.org/ontologies/Daan/2020/BarbaraNanning#2018> ;
        :Involves      :BarbaraNanning ;
        :Located-In    :CzechRepublic ;
        :Part-Of       :Creation_Artwork_73 .

:ARTWORK_18_64_RoundingByGrindingTheSheet
        a                 :Rounding_by_Grinding_the_Sheet , owl:NamedIndividual ;
        rdfs:comment      "Instance of an activity which is part of the creation process of ARTWORK_18_64."@en ;
        rdfs:label        "ARTWORK_18_64_Rounding by Grinding the Sheet"@en ;
        :Followed-By      :ARTWORK_18_64_TransportingMetalBowlWithSheet ;
        :Follows          :ARTWORK_18_64_SlumpingSheetsAndStrings ;
        :Has-Duration     <http://www.semanticweb.org/ontologies/Daan/2020/BarbaraNanning#2015> ;
        :Involves         <http://www.semanticweb.org/ontologies/Daan/2020/BarbaraNanning#AbHylkema(NL)> , :BarbaraNanning ;
        :Located-In       :Amsterdam ;
        :Part-Of          :Creation_Artwork_18_64 ;
        :Processes        :FlatGlassheetWithColouredCanes ;
        :Requires-Use-Of  :SharpeningStone , :Water , :DiamondSaw .

:Timespan  a             owl:Class ;
        rdfs:comment     "A timespan is a description of the approximated (beginning, end and) duration of a certain period."@en ;
        rdfs:label       "Timespan"@en ;
        rdfs:subClassOf  :Entity .

:ARTWORK_46_PreparingGlass
        a                 owl:NamedIndividual , :Preparing_Glass ;
        rdfs:comment      "Instance of an activity which is part of the creation process of ARTWORK_46."@en ;
        rdfs:label        "ARTWORK_46_Preparing Glass"@en ;
        :Followed-By      :ARTWORK_46_SetupAndTestingOfTheMetalMold ;
        :Follows          :ARTWORK_46_FillingKilnsWithMetalBowl ;
        :Has-Duration     <http://www.semanticweb.org/ontologies/Daan/2020/BarbaraNanning#2018> ;
        :Involves         <http://www.semanticweb.org/ontologies/Daan/2020/BarbaraNanning#JessicaHomich(USA)> , <http://www.semanticweb.org/ontologies/Daan/2020/BarbaraNanning#JiriPacinek(CZ)> , :BarbaraNanning ;
        :Located-In       :Lindava ;
        :Part-Of          :Creation_Artwork_46 ;
        :Requires-Use-Of  :Pontis , :BlowingPipe , :Garage , :GloryHole , :Marver .

:ARTWORK_76_Transporting_3
        a              owl:NamedIndividual , :Transporting ;
        rdfs:comment   "Instance of an activity which is part of the creation process of ARTWORK_76."@en ;
        rdfs:label     "ARTWORK_76_Transporting_3"@en ;
        :Followed-By   :ARTWORK_76_Gilding ;
        :Follows       :ARTWORK_76_Packing_3 ;
        :Has-Duration  <http://www.semanticweb.org/ontologies/Daan/2020/BarbaraNanning#2018> ;
        :Involves      :AlešZvěřina , :BarbaraNanning ;
        :Located-In    :CzechRepublic ;
        :Part-Of       :Creation_Artwork_76 .

:Picking_up_Coloured_Canes_Pattern
        a                owl:Class ;
        rdfs:comment     "A glassblower prepares glass on the pipe and picks up the preheated designs from the metal bowls."@en ;
        rdfs:label       "Picking up Coloured Canes Pattern"@en ;
        rdfs:subClassOf  :Activity .

:ARTWORK_18_64_DecidingColourPaletteAndPatterns
        a              owl:NamedIndividual , :Deciding_Colour_Palette_and_Patterns ;
        rdfs:comment   "Instance of an activity which is part of the creation process of ARTWORK_18_64."@en ;
        rdfs:label     "ARTWORK_18_64_Deciding Colour Palette and Patterns"@en ;
        :Followed-By   :ARTWORK_18_64_CuttingMonochromeSheets ;
        :Has-Duration  <http://www.semanticweb.org/ontologies/Daan/2020/BarbaraNanning#2015> ;
        :Involves      :BarbaraNanning ;
        :Located-In    :Amsterdam ;
        :Part-Of       :Creation_Artwork_18_64 ;
        :Processes     :BullseyeGlass ;
        :Starts        :Creation_Artwork_18_64 .

:Within-Period  a     owl:ObjectProperty ;
        rdfs:comment  "Within-Period is a property which connects an event to a period in which it occured."@en ;
        rdfs:domain   :Event ;
        rdfs:label    "Within-Period"@en ;
        rdfs:range    :Period .

:Is-Unica  a          owl:DatatypeProperty ;
        rdfs:comment  "Is-Unica is a property which indicates if a thing is an unique example."@en ;
        rdfs:domain   :Thing ;
        rdfs:label    "Is-Unica"@en ;
        rdfs:range    xsd:string .

:ARTWORK_80_Packing_4
        a              owl:NamedIndividual , :Packing ;
        rdfs:comment   "Instance of an activity which is part of the creation process of ARTWORK_80."@en ;
        rdfs:label     "ARTWORK_80_Packing_4"@en ;
        :Finishes      :Creation_Artwork_80 ;
        :Follows       :ARTWORK_80_Documenting ;
        :Has-Duration  <http://www.semanticweb.org/ontologies/Daan/2020/BarbaraNanning#2018> ;
        :Involves      :BarbaraNanning ;
        :Located-In    :CzechRepublic ;
        :Part-Of       :Creation_Artwork_80 .

:AJETOBlackGlass  a    :AJETO_Glass , owl:NamedIndividual ;
        rdfs:comment   "AJETO Black is a form of AJETO glass with a black colour."@en ;
        rdfs:label     "AJETO Black Glass"@en ;
        :Availability  "Available"@en ;
        :Made-By       :LASVITAJETO ;
        :Made-Out-Of   :Soda , :Sand , :Potassium , :Calcium ;
        :Transparency  "Opaque"@en .

<https://erfgeo.nl/thesaurus/pit/?id=malc/176>
        a       owl:NamedIndividual .

:Studio  a               owl:Class ;
        rdfs:comment     "Studio"@en ;
        rdfs:label       "Studio"@en ;
        rdfs:subClassOf  :Organisation .

:ARTWORK_17_33_Packing
        a              :Packing , owl:NamedIndividual ;
        rdfs:comment   "Instance of an activity which is part of the creation process of ARTWORK_17_33."@en ;
        rdfs:label     "ARTWORK_17_33_Packing"@en ;
        :Followed-By   :ARTWORK_17_33_Transporting ;
        :Follows       :ARTWORK_17_33_Cooling ;
        :Has-Duration  <http://www.semanticweb.org/ontologies/Daan/2020/BarbaraNanning#2017> ;
        :Involves      :BarbaraNanning ;
        :Located-In    :Lindava ;
        :Part-Of       :Creation_Artwork_17_33 .

:ARTWORK_44_SetupAndTestingOfTheMetalMold_2
        a                 :Setup_and_Testing_of_the_Metal_Mold , owl:NamedIndividual ;
        rdfs:comment      "Instance of an activity which is part of the creation process of ARTWORK_44."@en ;
        rdfs:label        "ARTWORK_44_Setup and Testing of the Metal Mold_2"@en ;
        :Followed-By      :ARTWORK_44_ApplyingClearGlassBell ;
        :Follows          :ARTWORK_44_ExaminingTheQualityOfTheGlass ;
        :Has-Duration     <http://www.semanticweb.org/ontologies/Daan/2020/BarbaraNanning#2018> ;
        :Involves         :AssistantOfBarbara , :BarbaraNanning , <http://www.semanticweb.org/ontologies/Daan/2020/BarbaraNanning#RadekKoten(CZ)> , <http://www.semanticweb.org/ontologies/Daan/2020/BarbaraNanning#Tom%C3%A1%C5%A1Moravec(CZ)> , <http://www.semanticweb.org/ontologies/Daan/2020/BarbaraNanning#LukasHavlas(CZ)> , <http://www.semanticweb.org/ontologies/Daan/2020/BarbaraNanning#JiriMoravec(CZ)> ;
        :Located-In       :CzechRepublic ;
        :Part-Of          :Creation_Artwork_44 ;
        :Requires-Use-Of  :InterchangeableMetalMoldSetup .

:BlowingPipe  a       :Tool , owl:NamedIndividual ;
        rdfs:comment  "A blowing pipe is a long tube used to blow molten glass. Each glass blower has their own blowpipe."@en ;
        rdfs:label    "Blowing Pipe"@en ;
        :Used-For     :ARTWORK_43_ExaminingTheQualityOfTheGlass , :ARTWORK_74_ApplyingExtraColour_2 , :ARTWORK_44_Modeling , <http://www.semanticweb.org/ontologies/Daan/2020/BarbaraNanning#ARTWORK_43_ExaminingQuality(Shape/Form)> , :ARTWORK_78_PreparingGlass , :ARTWORK_79_Glassblowing , :ARTWORK_79_ExaminingTheQualityOfTheGlass , :ARTWORK_80_Modeling , :ARTWORK_77_PreparingGlass , :ARTWORK_74_Glassblowing , :ARTWORK_75_ApplyingExtraColour_2 , :ARTWORK_74_ExaminingTheQualityOfTheGlass , :ARTWORK_77_Modeling , :ARTWORK_77_ApplyingExtraColour , :ARTWORK_77_ExaminingTheQualityOfTheGlass , :ARTWORK_80_ExaminingTheQualityOfTheGlass , :ARTWORK_44_Glassblowing , :ARTWORK_76_ApplyingExtraColour , <http://www.semanticweb.org/ontologies/Daan/2020/BarbaraNanning#ARTWORK_78_ExaminingQuality(Shape/Form)> , :ARTWORK_80_PreparingGlass , :ARTWORK_74_Modeling , :ARTWORK_75_Modeling , :ARTWORK_78_ApplyingExtraColour , :ARTWORK_73_ApplyingClearGlassBell , :ARTWORK_79_ApplyingExtraColour_2 , :ARTWORK_75_ApplyingExtraColour , :ARTWORK_43_ApplyingClearGlassBell , <http://www.semanticweb.org/ontologies/Daan/2020/BarbaraNanning#ARTWORK_76_ExaminingQuality(Shape/Form)> , :ARTWORK_75_ExaminingTheQualityOfTheGlass , :ARTWORK_79_Modeling , :ARTWORK_79_ApplyingClearGlassBell , :ARTWORK_73_Modeling , :ARTWORK_43_PreparingGlass , <http://www.semanticweb.org/ontologies/Daan/2020/BarbaraNanning#ARTWORK_80_ExaminingQuality(Shape/Form)> , :ARTWORK_75_PreparingGlass , :ARTWORK_78_Modeling , :ARTWORK_74_ApplyingClearGlassBell , <http://www.semanticweb.org/ontologies/Daan/2020/BarbaraNanning#ARTWORK_79_ExaminingQuality(Shape/Form)> , :ARTWORK_44_ExaminingTheQualityOfTheGlass , :ARTWORK_44_ApplyingClearGlassBell , :ARTWORK_43_Modeling , :ARTWORK_78_Glassblowing , :ARTWORK_77_ApplyingClearGlassBell , :ARTWORK_74_PreparingGlass , :ARTWORK_80_ApplyingExtraColour , :ARTWORK_44_ApplyingExtraColour_2 , :ARTWORK_76_ApplyingClearGlassBell , :ARTWORK_78_ExaminingTheQualityOfTheGlass , :ARTWORK_79_ApplyingExtraColour , :ARTWORK_75_ApplyingClearGlassBell , :ARTWORK_75_Glassblowing , :ARTWORK_76_Modeling , :ARTWORK_43_ApplyingExtraColour , :ARTWORK_79_PreparingGlass , :ARTWORK_76_PreparingGlass , :ARTWORK_76_ExaminingTheQualityOfTheGlass , :ARTWORK_74_ApplyingExtraColour , :ARTWORK_44_ApplyingExtraColour , :ARTWORK_80_Glassblowing , :ARTWORK_76_ApplyingExtraColour_2 , :ARTWORK_73_PreparingGlass , <http://www.semanticweb.org/ontologies/Daan/2020/BarbaraNanning#ARTWORK_74_ExaminingQuality(Shape/Form)> , :ARTWORK_78_ApplyingClearGlassBell , <http://www.semanticweb.org/ontologies/Daan/2020/BarbaraNanning#ARTWORK_73_ExaminingQuality(Shape/Form)> , <http://www.semanticweb.org/ontologies/Daan/2020/BarbaraNanning#ARTWORK_44_ExaminingQuality(Shape/Form)> , :ARTWORK_80_ApplyingClearGlassBell , :ARTWORK_76_Glassblowing , <http://www.semanticweb.org/ontologies/Daan/2020/BarbaraNanning#ARTWORK_77_ExaminingQuality(Shape/Form)> , :ARTWORK_77_Glassblowing , :ARTWORK_73_Glassblowing , <http://www.semanticweb.org/ontologies/Daan/2020/BarbaraNanning#ARTWORK_75_ExaminingQuality(Shape/Form)> , :ARTWORK_44_PreparingGlass , :ARTWORK_73_ExaminingTheQualityOfTheGlass , :ARTWORK_43_Glassblowing .

:Period-Contains  a    owl:ObjectProperty ;
        rdfs:comment   "Period-Contains is a property which connects an event to a period in which it occured."@en ;
        rdfs:domain    :Period ;
        rdfs:label     "Period-Contains"@en ;
        rdfs:range     :Event ;
        owl:inverseOf  :Within-Period .

:ARTWORK_79_Packing_3
        a              owl:NamedIndividual , :Packing ;
        rdfs:comment   "Instance of an activity which is part of the creation process of ARTWORK_79."@en ;
        rdfs:label     "ARTWORK_79_Packing_3"@en ;
        :Followed-By   :ARTWORK_79_Transporting_3 ;
        :Follows       :ARTWORK_79_Signing ;
        :Has-Duration  <http://www.semanticweb.org/ontologies/Daan/2020/BarbaraNanning#2018> ;
        :Involves      :AlešZvěřina , :BarbaraNanning ;
        :Located-In    :CzechRepublic ;
        :Part-Of       :Creation_Artwork_79 .

:ARTWORK_80_Sawing  a     owl:NamedIndividual , :Sawing ;
        rdfs:comment      "Instance of an activity which is part of the creation process of ARTWORK_80."@en ;
        rdfs:label        "ARTWORK_80_Sawing"@en ;
        :Followed-By      :ARTWORK_80_Grinding ;
        :Follows          <http://www.semanticweb.org/ontologies/Daan/2020/BarbaraNanning#ARTWORK_80_ExaminingQuality(CheckForIrregularitiesInTheGlass)> ;
        :Has-Duration     <http://www.semanticweb.org/ontologies/Daan/2020/BarbaraNanning#2018> ;
        :Involves         :BarbaraNanning , :AlešZvěřina ;
        :Located-In       :CzechRepublic ;
        :Part-Of          :Creation_Artwork_80 ;
        :Requires-Use-Of  :DiamondSaw .

:Creation_Artwork_18_64
        a               owl:NamedIndividual , :Creation_Event ;
        rdfs:comment    "Creation event for Artwork_18_64 by Barbara Nanning."@en ;
        rdfs:label      "Creation_Artwork_18_64"@en ;
        :Consists-Of    :ARTWORK_18_64_RoundingByGrindingTheSheet , :ARTWORK_18_64_DecidingColourPaletteAndPatterns_2 , :ARTWORK_18_64_CuttingAndPolishingCastedMonochromeSheetsToSmallRods , :ARTWORK_18_64_Grinding , :ARTWORK_18_64_CuttingSheets , :ARTWORK_18_64_Ordening , :ARTWORK_18_64_Transporting , :ARTWORK_18_64_Sensing_2 , :ARTWORK_18_64_Packing , :ARTWORK_18_64_DecidingColourPaletteAndPatterns_3 , :ARTWORK_18_64_DecoratingTheSheetWithColouredCanes , :ARTWORK_18_64_Sawing , :ARTWORK_18_64_FusingSheets , :ARTWORK_18_64_PickingUpColouredCanesPattern , :ARTWORK_18_64_Documenting , :ARTWORK_18_64_CuttingAndPolishingColouredCanes , :ARTWORK_18_64_Photographing , :ARTWORK_18_64_Resting , :ARTWORK_18_64_Packing_2 , :ARTWORK_18_64_Signing , :ARTWORK_18_64_TransportingColouredCanes , :ARTWORK_18_64_DecidingColourPaletteAndPatterns , :ARTWORK_18_64_Transporting_2 , :ARTWORK_18_64_FillingKilnsWithMetalBowl , :ARTWORK_18_64_CuttingMonochromeSheets , :ARTWORK_18_64_PreparingForBlowing , :ARTWORK_18_64_TransportingColouredCanes_2 , <http://www.semanticweb.org/ontologies/Daan/2020/BarbaraNanning#ARTWORK_18_64_ExaminingQuality(CheckForIrregularitiesInTheGlass)> , :ARTWORK_18_64_PreparingGlass , :ARTWORK_18_64_ProducingColouredCanes , :ARTWORK_18_64_Sandblasting , :ARTWORK_18_64_Casting , :ARTWORK_18_64_Modeling , :ARTWORK_18_64_ApplyingClearGlassBell , :ARTWORK_18_64_Cooling , :ARTWORK_18_64_ExaminingTheQualityOfTheGlass , :ARTWORK_18_64_PreparingForBlowing_2 , :ARTWORK_18_64_TransportingMetalBowlWithSheet , :ARTWORK_18_64_Sensing , :ARTWORK_18_64_Packing_3 , :ARTWORK_18_64_Polishing , <http://www.semanticweb.org/ontologies/Daan/2020/BarbaraNanning#ARTWORK_18_64_ExaminingQuality(Shape/Form)> , :ARTWORK_18_64_MeasuringAndBoxesMaking , :ARTWORK_18_64_OrdeningFlatSheets , :ARTWORK_18_64_TransportingMonochromeRods , :ARTWORK_18_64_SlumpingSheetsAndStrings , :ARTWORK_18_64_CuttingStrings , <http://www.semanticweb.org/ontologies/Daan/2020/BarbaraNanning#ARTWORK_18_64_ExaminingQuality(Result)> , :ARTWORK_18_64_Glassblowing , :ARTWORK_18_64_FusingSheetsAndStrings ;
        :Created        :Artwork_18_64 ;
        :Finishes-With  :ARTWORK_18_64_Documenting ;
        :Has-Duration   <http://www.semanticweb.org/ontologies/Daan/2020/BarbaraNanning#2015> ;
        :Starts-With    :ARTWORK_18_64_DecidingColourPaletteAndPatterns .

:ARTWORK_44_Sawing  a     :Sawing , owl:NamedIndividual ;
        rdfs:comment      "Instance of an activity which is part of the creation process of ARTWORK_44."@en ;
        rdfs:label        "ARTWORK_44_Sawing"@en ;
        :Followed-By      :ARTWORK_44_Grinding ;
        :Follows          <http://www.semanticweb.org/ontologies/Daan/2020/BarbaraNanning#ARTWORK_44_ExaminingQuality(CheckForIrregularitiesInTheGlass)> ;
        :Has-Duration     <http://www.semanticweb.org/ontologies/Daan/2020/BarbaraNanning#2018> ;
        :Involves         :AlešZvěřina , :BarbaraNanning ;
        :Located-In       :CzechRepublic ;
        :Part-Of          :Creation_Artwork_44 ;
        :Requires-Use-Of  :DiamondSaw .

:Garage  a            :Equipment , owl:NamedIndividual ;
        rdfs:comment  "A garage is a building for housing of tools and equipment in which work can be done by actors."@en ;
        rdfs:label    "Garage"@en ;
        :Used-For     :ARTWORK_76_ApplyingExtraColour_2 , :ARTWORK_73_PreparingGlass , :ARTWORK_79_ApplyingExtraColour , :ARTWORK_44_PreparingGlass , :ARTWORK_78_PreparingGlass , :ARTWORK_77_PreparingGlass , :ARTWORK_78_ApplyingExtraColour , :ARTWORK_44_ApplyingExtraColour , :ARTWORK_79_PreparingGlass , :ARTWORK_75_ApplyingExtraColour , :ARTWORK_74_PreparingGlass , :ARTWORK_75_ApplyingExtraColour_2 , :ARTWORK_44_ApplyingExtraColour_2 , :ARTWORK_43_PreparingGlass , :ARTWORK_75_PreparingGlass , :ARTWORK_79_ApplyingExtraColour_2 , :ARTWORK_76_PreparingGlass , :ARTWORK_80_ApplyingExtraColour , :ARTWORK_43_ApplyingExtraColour , :ARTWORK_74_ApplyingExtraColour_2 , :ARTWORK_77_ApplyingExtraColour , :ARTWORK_74_ApplyingExtraColour , :ARTWORK_80_PreparingGlass , :ARTWORK_76_ApplyingExtraColour .

:ARTWORK_36_PreparingGlass
        a                 owl:NamedIndividual , :Preparing_Glass ;
        rdfs:comment      "Instance of an activity which is part of the creation process of ARTWORK_36."@en ;
        rdfs:label        "ARTWORK_36_Preparing Glass"@en ;
        :Followed-By      :ARTWORK_36_SetupAndTestingOfTheMetalMold ;
        :Follows          :ARTWORK_36_FillingKilnsWithMetalBowl ;
        :Has-Duration     <http://www.semanticweb.org/ontologies/Daan/2020/BarbaraNanning#2015> ;
        :Involves         :BarbaraNanning , <http://www.semanticweb.org/ontologies/Daan/2020/BarbaraNanning#MiaLerssi(DN)> , :GertBullée ;
        :Located-In       :Zaandam ;
        :Part-Of          :Creation_Artwork_36 ;
        :Requires-Use-Of  :Garage , :BlowingPipe , :Marver , :Pontis , :GloryHole .

:Artwork_39  a        :Glass_Artwork , owl:NamedIndividual ;
        rdfs:comment  "Artwork_39 is a glass artwork made by Barbara Nanning."@en ;
        rdfs:label    "Coloured Shadows"@en ;
        :Created-By   :Creation_Artwork_39 ;
        :Has-Depth    "22"^^xsd:decimal ;
        :Has-Height   "25"^^xsd:decimal , "16"^^xsd:decimal ;
        :Is-Unica     "Yes"@en ;
        :Made-By      :VRIJGLASZaandam , <http://www.semanticweb.org/ontologies/Daan/2020/BarbaraNanning#Ale%C5%A1Zv%C4%9B%C5%99ina&AZ-Design> , :BarbaraNanning , :GlassStudioVanTetterode ;
        :Made-Out-Of  :BullseyeGlass ;
        :Shown-By     :Image_Artwork_39 .

<http://www.cidoc-crm.org/cidoc-crm/P116_starts>
        a                       owl:ObjectProperty ;
        owl:equivalentProperty  :Starts .

:ARTWORK_78_Signing  a    owl:NamedIndividual , :Signing ;
        rdfs:comment      "Instance of an activity which is part of the creation process of ARTWORK_78."@en ;
        rdfs:label        "ARTWORK_78_Signing"@en ;
        :Followed-By      :ARTWORK_78_Packing_3 ;
        :Follows          :ARTWORK_78_Transporting_2 ;
        :Has-Duration     <http://www.semanticweb.org/ontologies/Daan/2020/BarbaraNanning#2008> ;
        :Involves         :AlešZvěřina , :BarbaraNanning ;
        :Located-In       :CzechRepublic ;
        :Part-Of          :Creation_Artwork_78 ;
        :Requires-Use-Of  :AirCompressor .

:ARTWORK_78_Gilding  a    :Gilding , owl:NamedIndividual ;
        rdfs:comment      "Instance of an activity which is part of the creation process of ARTWORK_78."@en ;
        rdfs:label        "ARTWORK_78_Gilding"@en ;
        :Followed-By      <http://www.semanticweb.org/ontologies/Daan/2020/BarbaraNanning#ARTWORK_78_ExaminingQuality(FinalResult)> ;
        :Follows          :ARTWORK_78_Transporting_3 ;
        :Has-Duration     <http://www.semanticweb.org/ontologies/Daan/2020/BarbaraNanning#2016> ;
        :Involves         :BarbaraNanning , :VáçlavNovák_Doksy_CzechRepublic ;
        :Located-In       :CzechRepublic ;
        :Part-Of          :Creation_Artwork_78 ;
        :Requires-Use-Of  :GildersKnife , :GildersTip , :INSTACOLLTool , :GildingCushion .

:Lindava  a           :City , owl:NamedIndividual ;
        rdfs:comment  "Lindava is a city in Czech Republic."@en ;
        rdfs:label    "Lindava"@en ;
        owl:sameAs    <http://www.wikidata.org/entity/Q12033551> ;
        :Located-In   :CzechRepublic ;
        :Location-Of  :LASVITAJETO .

:Second_Glass_Blower  a  owl:Class ;
        rdfs:comment     "The second glass blower is the third highest role within a glass blowing team."@en ;
        rdfs:label       "Second Glass Blower"@en ;
        rdfs:subClassOf  :Glass_Blower .

:ARTWORK_78_Polishing
        a                 :Polishing , owl:NamedIndividual ;
        rdfs:comment      "Instance of an activity which is part of the creation process of ARTWORK_78."@en ;
        rdfs:label        "ARTWORK_78_Polishing"@en ;
        :Followed-By      <http://www.semanticweb.org/ontologies/Daan/2020/BarbaraNanning#ARTWORK_78_ExaminingQuality(Result)> ;
        :Follows          :ARTWORK_78_Grinding ;
        :Has-Duration     <http://www.semanticweb.org/ontologies/Daan/2020/BarbaraNanning#2008> ;
        :Involves         :LukášSvoboda , :BarbaraNanning , :AlešZvěřina ;
        :Located-In       :CzechRepublic ;
        :Part-Of          :Creation_Artwork_78 ;
        :Requires-Use-Of  :PolishingStone .

:TeflonStick  a       :Tool , owl:NamedIndividual ;
        rdfs:comment  "A teflon stick is a stick made out of the material teflon; a tough and insoluble polymer which is often used in making coatings."@en ;
        rdfs:label    "Teflon Stick"@en .

:Finishes-With  a     owl:ObjectProperty ;
        rdfs:comment  "Finishes-With is a property which indicates the sub-event which ends an event."@en ;
        rdfs:domain   :Event ;
        rdfs:label    "Finishes-With"@en ;
        rdfs:range    :Event .

:Tagliol  a           :Tool , owl:NamedIndividual ;
        rdfs:comment  "A tagliol is a flat metal knife."@en ;
        rdfs:label    "Tagliol"@en ;
        :Used-For     :ARTWORK_44_ApplyingExtraColour , :ARTWORK_80_Glassblowing , :ARTWORK_74_ApplyingExtraColour , :ARTWORK_76_Glassblowing , :ARTWORK_44_Glassblowing , :ARTWORK_44_ApplyingExtraColour_2 , :ARTWORK_79_Glassblowing , :ARTWORK_75_ApplyingExtraColour_2 , :ARTWORK_80_ApplyingExtraColour , :ARTWORK_78_ApplyingExtraColour , :ARTWORK_74_ApplyingExtraColour_2 , :ARTWORK_43_Glassblowing , :ARTWORK_43_ApplyingExtraColour , :ARTWORK_77_ApplyingExtraColour , :ARTWORK_75_ApplyingExtraColour , :ARTWORK_79_ApplyingExtraColour_2 , :ARTWORK_73_Glassblowing , :ARTWORK_77_Glassblowing , :ARTWORK_74_Glassblowing , :ARTWORK_75_Glassblowing , :ARTWORK_76_ApplyingExtraColour_2 , :ARTWORK_76_ApplyingExtraColour , :ARTWORK_79_ApplyingExtraColour , :ARTWORK_78_Glassblowing .

:ARTWORK_46_FillingKilnsWithMetalBowl
        a                 owl:NamedIndividual , :Filling_Kilns_with_Metal_Bowl ;
        rdfs:comment      "Instance of an activity which is part of the creation process of ARTWORK_46."@en ;
        rdfs:label        "ARTWORK_46_Filling Kilns with Metal Bowl"@en ;
        :Followed-By      :ARTWORK_46_PreparingGlass ;
        :Follows          :ARTWORK_46_PreparingForBlowing ;
        :Has-Duration     <http://www.semanticweb.org/ontologies/Daan/2020/BarbaraNanning#2018> ;
        :Involves         <http://www.semanticweb.org/ontologies/Daan/2020/BarbaraNanning#JiriPacinek(CZ)> , :BarbaraNanning ;
        :Located-In       :Lindava ;
        :Part-Of          :Creation_Artwork_46 ;
        :Requires-Use-Of  :FusingKiln , :Garage , :Gloves .

:Modeling  a             owl:Class ;
        rdfs:comment     "Modeling is an activity in which a thing is sculpted into a specific model."@en ;
        rdfs:label       "Modeling"@en ;
        rdfs:subClassOf  :Activity .

:ARTWORK_43_Transporting
        a              owl:NamedIndividual , :Transporting ;
        rdfs:comment   "Instance of an activity which is part of the creation process of ARTWORK_43."@en ;
        rdfs:label     "ARTWORK_43_Transporting"@en ;
        :Followed-By   :ARTWORK_43_Resting ;
        :Follows       :ARTWORK_43_Packing ;
        :Has-Duration  <http://www.semanticweb.org/ontologies/Daan/2020/BarbaraNanning#2008> ;
        :Involves      :AlešZvěřina , :BarbaraNanning ;
        :Located-In    :CzechRepublic ;
        :Part-Of       :Creation_Artwork_43 .

:ARTWORK_77_SetupAndTestingOfTheMetalMold
        a                 owl:NamedIndividual , :Setup_and_Testing_of_the_Metal_Mold ;
        rdfs:comment      "Instance of an activity which is part of the creation process of ARTWORK_77."@en ;
        rdfs:label        "ARTWORK_77_Setup and Testing of the Metal Mold"@en ;
        :Followed-By      :ARTWORK_77_SetupAndTestingOfTheMetalMold_2 ;
        :Follows          :ARTWORK_77_PreparingGlass ;
        :Has-Duration     <http://www.semanticweb.org/ontologies/Daan/2020/BarbaraNanning#2018> ;
        :Involves         <http://www.semanticweb.org/ontologies/Daan/2020/BarbaraNanning#JiriMoravec(CZ)> , <http://www.semanticweb.org/ontologies/Daan/2020/BarbaraNanning#LukasHavlas(CZ)> , <http://www.semanticweb.org/ontologies/Daan/2020/BarbaraNanning#RadekKoten(CZ)> , <http://www.semanticweb.org/ontologies/Daan/2020/BarbaraNanning#Tom%C3%A1%C5%A1Moravec(CZ)> , :BarbaraNanning , :AssistantOfBarbara ;
        :Located-In       :CzechRepublic ;
        :Part-Of          :Creation_Artwork_77 ;
        :Requires-Use-Of  :InterchangeableMetalMoldSetup .

:Maker-Of  a          owl:ObjectProperty ;
        rdfs:comment  "Maker-Of is a property which connects a thing with the creator of this thing."@en ;
        rdfs:domain   :Actor ;
        rdfs:label    "Maker-Of"@en ;
        rdfs:range    :Thing .

:BullseyeGlassSplinterEnDeVosch
        a             :Glass_Studio , owl:NamedIndividual ;
        rdfs:comment  "Bullseye glass Splinter en de Vosch is a glass studio in Langweer."@en ;
        rdfs:label    "Bullseye glass Splinter en de Vosch"@en ;
        :Employed     :SteefHendriks ;
        :Located-In   :Langweer ;
        :Maker-Of     :Artwork_46 , :Artwork_36 , :Artwork_18_64 .

:ARTWORK_17_33_FillingKilnsWithMetalBowl
        a                 owl:NamedIndividual , :Filling_Kilns_with_Metal_Bowl ;
        rdfs:comment      "Instance of an activity which is part of the creation process of ARTWORK_17_33."@en ;
        rdfs:label        "ARTWORK_17_33_Filling Kilns with Metal Bowl"@en ;
        :Followed-By      :ARTWORK_17_33_PreparingGlass ;
        :Follows          :ARTWORK_17_33_PreparingForBlowing ;
        :Has-Duration     <http://www.semanticweb.org/ontologies/Daan/2020/BarbaraNanning#2017> ;
        :Involves         :BarbaraNanning , <http://www.semanticweb.org/ontologies/Daan/2020/BarbaraNanning#RadekKoten(CZ)> ;
        :Located-In       :Lindava ;
        :Part-Of          :Creation_Artwork_17_33 ;
        :Requires-Use-Of  :Gloves , :FusingKiln , :Garage .

:Glass_Blower  a         owl:Class ;
        rdfs:comment     "A glass blower is a person who inflates (semi-) molten glass."@en ;
        rdfs:label       "Glass Blower"@en ;
        rdfs:subClassOf  :Person .

:ARTWORK_74_PreparingGlass
        a                 :Preparing_Glass , owl:NamedIndividual ;
        rdfs:comment      "Instance of an activity which is part of the creation process of ARTWORK_74."@en ;
        rdfs:label        "ARTWORK_74_Preparing Glass"@en ;
        :Followed-By      :ARTWORK_74_SetupAndTestingOfTheMetalMold ;
        :Has-Duration     <http://www.semanticweb.org/ontologies/Daan/2020/BarbaraNanning#2008> ;
        :Involves         <http://www.semanticweb.org/ontologies/Daan/2020/BarbaraNanning#AlesVacek(CZ)> , :BarbaraNanning ;
        :Located-In       :CzechRepublic ;
        :Part-Of          :Creation_Artwork_74 ;
        :Requires-Use-Of  :GloryHole , :Marver , :Pontis , :Garage , :BlowingPipe ;
        :Starts           :Creation_Artwork_74 .

:ARTWORK_36_Signing_2
        a                 owl:NamedIndividual , :Signing ;
        rdfs:comment      "Instance of an activity which is part of the creation process of ARTWORK_36."@en ;
        rdfs:label        "ARTWORK_36_Signing_2"@en ;
        :Followed-By      <http://www.semanticweb.org/ontologies/Daan/2020/BarbaraNanning#ARTWORK_36_ExaminingQuality(FinalResult)_2> ;
        :Follows          :ARTWORK_36_Transporting_5 ;
        :Has-Duration     <http://www.semanticweb.org/ontologies/Daan/2020/BarbaraNanning#2019> ;
        :Involves         :BarbaraNanning , :AlešZvěřina ;
        :Located-In       :NovyBor ;
        :Part-Of          :Creation_Artwork_36 ;
        :Requires-Use-Of  :AirCompressor .

<http://www.semanticweb.org/ontologies/Daan/2020/BarbaraNanning#ARTWORK_18_64_ExaminingQuality(Result)>
        a              owl:NamedIndividual , j.0: ;
        rdfs:comment   "Instance of an activity which is part of the creation process of ARTWORK_18_64."@en ;
        rdfs:label     "ARTWORK_18_64_Examining Quality (Result)"@en ;
        :Followed-By   :ARTWORK_18_64_MeasuringAndBoxesMaking ;
        :Follows       :ARTWORK_18_64_Signing ;
        :Has-Duration  <http://www.semanticweb.org/ontologies/Daan/2020/BarbaraNanning#2015> ;
        :Involves      :AlešZvěřina , :BarbaraNanning ;
        :Located-In    :NovyBor ;
        :Part-Of       :Creation_Artwork_18_64 .

:ARTWORK_79_Translocating
        a                 :Translocating , owl:NamedIndividual ;
        rdfs:comment      "Instance of an activity which is part of the creation process of ARTWORK_79."@en ;
        rdfs:label        "ARTWORK_79_Translocating"@en ;
        :Followed-By      :ARTWORK_79_Cooling ;
        :Follows          <http://www.semanticweb.org/ontologies/Daan/2020/BarbaraNanning#ARTWORK_79_ExaminingQuality(Shape/Form)> ;
        :Has-Duration     <http://www.semanticweb.org/ontologies/Daan/2020/BarbaraNanning#2018> ;
        :Involves         :BarbaraNanning ;
        :Located-In       :CzechRepublic ;
        :Part-Of          :Creation_Artwork_79 ;
        :Requires-Use-Of  :Fork .

:Assisting_Team_Member
        a                owl:Class ;
        rdfs:comment     "The assisting team member is a member of a glass blowing team responsible for Transporting the glass objects."@en ;
        rdfs:label       "Assisting Team Member"@en ;
        rdfs:subClassOf  :Person .

:GloryHole  a         owl:NamedIndividual , :Equipment ;
        rdfs:comment  "A glory hole is a hole in a furnace or heated equipment used during glass blowing to heat things (e.g. glass or blowing pipes)."@en ;
        rdfs:label    "Glory Hole"@en ;
        :Used-For     :ARTWORK_79_PreparingGlass , :ARTWORK_73_ExaminingTheQualityOfTheGlass , <http://www.semanticweb.org/ontologies/Daan/2020/BarbaraNanning#ARTWORK_79_ExaminingQuality(Shape/Form)> , <http://www.semanticweb.org/ontologies/Daan/2020/BarbaraNanning#ARTWORK_76_ExaminingQuality(Shape/Form)> , :ARTWORK_44_ExaminingTheQualityOfTheGlass , :ARTWORK_80_PreparingGlass , :ARTWORK_76_ExaminingTheQualityOfTheGlass , :ARTWORK_75_PreparingGlass , :ARTWORK_74_ApplyingExtraColour , :ARTWORK_74_PreparingGlass , :ARTWORK_44_ApplyingExtraColour , :ARTWORK_43_ApplyingExtraColour , :ARTWORK_75_Glassblowing , :ARTWORK_74_ApplyingExtraColour_2 , :ARTWORK_78_ExaminingTheQualityOfTheGlass , :ARTWORK_74_Glassblowing , :ARTWORK_75_ApplyingExtraColour_2 , <http://www.semanticweb.org/ontologies/Daan/2020/BarbaraNanning#ARTWORK_78_ExaminingQuality(Shape/Form)> , <http://www.semanticweb.org/ontologies/Daan/2020/BarbaraNanning#ARTWORK_77_ExaminingQuality(Shape/Form)> , :ARTWORK_44_Glassblowing , :ARTWORK_43_PreparingGlass , :ARTWORK_77_PreparingGlass , <http://www.semanticweb.org/ontologies/Daan/2020/BarbaraNanning#ARTWORK_75_ExaminingQuality(Shape/Form)> , :ARTWORK_77_ApplyingExtraColour , :ARTWORK_75_ApplyingExtraColour , :ARTWORK_75_ExaminingTheQualityOfTheGlass , :ARTWORK_80_Glassblowing , :ARTWORK_74_ExaminingTheQualityOfTheGlass , <http://www.semanticweb.org/ontologies/Daan/2020/BarbaraNanning#ARTWORK_73_ExaminingQuality(Shape/Form)> , <http://www.semanticweb.org/ontologies/Daan/2020/BarbaraNanning#ARTWORK_43_ExaminingQuality(Shape/Form)> , :ARTWORK_73_PreparingGlass , :ARTWORK_79_ApplyingExtraColour , :ARTWORK_78_PreparingGlass , :ARTWORK_77_ExaminingTheQualityOfTheGlass , :ARTWORK_79_ExaminingTheQualityOfTheGlass , <http://www.semanticweb.org/ontologies/Daan/2020/BarbaraNanning#ARTWORK_44_ExaminingQuality(Shape/Form)> , :ARTWORK_78_Glassblowing , :ARTWORK_80_ApplyingExtraColour , <http://www.semanticweb.org/ontologies/Daan/2020/BarbaraNanning#ARTWORK_74_ExaminingQuality(Shape/Form)> , :ARTWORK_76_ApplyingExtraColour , <http://www.semanticweb.org/ontologies/Daan/2020/BarbaraNanning#ARTWORK_80_ExaminingQuality(Shape/Form)> , :ARTWORK_77_Glassblowing , :ARTWORK_76_ApplyingExtraColour_2 , :ARTWORK_78_ApplyingExtraColour , :ARTWORK_73_Glassblowing , :ARTWORK_76_Glassblowing , :ARTWORK_80_ExaminingTheQualityOfTheGlass , :ARTWORK_43_Glassblowing , :ARTWORK_44_ApplyingExtraColour_2 , :ARTWORK_79_Glassblowing , :ARTWORK_44_PreparingGlass , :ARTWORK_76_PreparingGlass , :ARTWORK_43_ExaminingTheQualityOfTheGlass , :ARTWORK_79_ApplyingExtraColour_2 .

<http://www.semanticweb.org/ontologies/Daan/2020/BarbaraNanning#ARTWORK_73_ExaminingQuality(FinalResult)>
        a              owl:NamedIndividual , j.1: ;
        rdfs:comment   "Instance of an activity which is part of the creation process of ARTWORK_73."@en ;
        rdfs:label     "ARTWORK_73_Examining Quality (Final Result)"@en ;
        :Followed-By   :ARTWORK_73_Packing_5 ;
        :Follows       :ARTWORK_73_Gilding ;
        :Has-Duration  <http://www.semanticweb.org/ontologies/Daan/2020/BarbaraNanning#2018> ;
        :Involves      :AlešZvěřina , :BarbaraNanning ;
        :Located-In    :CzechRepublic ;
        :Part-Of       :Creation_Artwork_73 .

:Maintained-By  a      owl:ObjectProperty ;
        rdfs:comment   "Maintained-By is a property which connects a thing with an actor who Maintains the thing in question."@en ;
        rdfs:domain    :Thing ;
        rdfs:label     "Maintained-By"@en ;
        rdfs:range     :Actor ;
        owl:inverseOf  :Maintains .

<http://www.wikidata.org/entity/Q183>
        a       owl:NamedIndividual .

:GlasmuseumLette  a   :Museum , owl:NamedIndividual ;
        rdfs:comment  "Glasmuseum Lette is a museum for glass artifacts located in Coesfeld (Germany)."@en ;
        rdfs:label    "Glasmuseum Lette"@en ;
        :Located-In   :Coesfeld ;
        :Maintains    :CollectionGlasmuseumLette .

:ARTWORK_73_Translocating
        a                 :Translocating , owl:NamedIndividual ;
        rdfs:comment      "Instance of an activity which is part of the creation process of ARTWORK_73."@en ;
        rdfs:label        "ARTWORK_73_Translocating"@en ;
        :Followed-By      :ARTWORK_73_Cooling ;
        :Follows          <http://www.semanticweb.org/ontologies/Daan/2020/BarbaraNanning#ARTWORK_73_ExaminingQuality(Shape/Form)> ;
        :Has-Duration     <http://www.semanticweb.org/ontologies/Daan/2020/BarbaraNanning#2018> ;
        :Involves         :BarbaraNanning ;
        :Located-In       :CzechRepublic ;
        :Part-Of          :Creation_Artwork_73 ;
        :Requires-Use-Of  :Fork .

:ARTWORK_78_Documenting
        a              owl:NamedIndividual , :Documenting ;
        rdfs:comment   "Instance of an activity which is part of the creation process of ARTWORK_78."@en ;
        rdfs:label     "ARTWORK_78_Documenting"@en ;
        :Followed-By   :ARTWORK_78_Packing_5 ;
        :Follows       :ARTWORK_78_Photographing ;
        :Has-Duration  <http://www.semanticweb.org/ontologies/Daan/2020/BarbaraNanning#2016> ;
        :Involves      :BarbaraNanning ;
        :Located-In    :CzechRepublic ;
        :Part-Of       :Creation_Artwork_78 .

:ARTWORK_74_Packing_3
        a              owl:NamedIndividual , :Packing ;
        rdfs:comment   "Instance of an activity which is part of the creation process of ARTWORK_74."@en ;
        rdfs:label     "ARTWORK_74_Packing_3"@en ;
        :Followed-By   :ARTWORK_74_Transporting_3 ;
        :Follows       :ARTWORK_74_Signing ;
        :Has-Duration  <http://www.semanticweb.org/ontologies/Daan/2020/BarbaraNanning#2008> ;
        :Involves      :BarbaraNanning , :AlešZvěřina ;
        :Located-In    :CzechRepublic ;
        :Part-Of       :Creation_Artwork_74 .

:ARTWORK_75_Transporting_3
        a              owl:NamedIndividual , :Transporting ;
        rdfs:comment   "Instance of an activity which is part of the creation process of ARTWORK_75."@en ;
        rdfs:label     "ARTWORK_75_Transporting_3"@en ;
        :Followed-By   :ARTWORK_75_Gilding ;
        :Follows       :ARTWORK_75_Packing_3 ;
        :Has-Duration  <http://www.semanticweb.org/ontologies/Daan/2020/BarbaraNanning#2018> ;
        :Involves      :BarbaraNanning , :AlešZvěřina ;
        :Located-In    :CzechRepublic ;
        :Part-Of       :Creation_Artwork_75 .

:Image_Artwork_80  a            :Digital_Image , owl:NamedIndividual ;
        rdfs:comment            "Image of an artwork by Barbara Nanning displayed in \"Barbara Nanning Eeuwige Beweging\" by Eliens (2019)."@en ;
        rdfs:label              "Image_Artwork_80"@en ;
        :Representation-Source  "Tom Haartsen_Ouderkerk a/d Amstel (NL)"@en ;
        :Shows                  :Artwork_80 .

:AJETO_Glass  a          owl:Class ;
        rdfs:comment     "AJETO glass is a material created using a recipe of sand, soda, calcium and potassium in the AJETO studio."@en ;
        rdfs:label       "AJETO Glass"@en ;
        rdfs:subClassOf  :Glass .

:ARTWORK_77_Sawing  a     :Sawing , owl:NamedIndividual ;
        rdfs:comment      "Instance of an activity which is part of the creation process of ARTWORK_77."@en ;
        rdfs:label        "ARTWORK_77_Sawing"@en ;
        :Followed-By      :ARTWORK_77_Grinding ;
        :Follows          <http://www.semanticweb.org/ontologies/Daan/2020/BarbaraNanning#ARTWORK_77_ExaminingQuality(CheckForIrregularitiesInTheGlass)> ;
        :Has-Duration     <http://www.semanticweb.org/ontologies/Daan/2020/BarbaraNanning#2018> ;
        :Involves         :AlešZvěřina , :BarbaraNanning ;
        :Located-In       :CzechRepublic ;
        :Part-Of          :Creation_Artwork_77 ;
        :Requires-Use-Of  :DiamondSaw .

[ a            owl:AllDisjointClasses ;
  owl:members  ( :Assisting_Team_Member :Creator :Gilder :Glass_Blower :Grinder :Metal_Worker :Photographer :Supervisor_Works )
] .

:ARTWORK_17_33_PreparingForBlowing
        a                 owl:NamedIndividual , :Preparing_for_Blowing ;
        rdfs:comment      "Instance of an activity which is part of the creation process of ARTWORK_17_33."@en ;
        rdfs:label        "ARTWORK_17_33_Preparing for Blowing"@en ;
        :Followed-By      :ARTWORK_17_33_FillingKilnsWithMetalBowl ;
        :Follows          :ARTWORK_17_33_TransportingMetalBowlWithCanes ;
        :Has-Duration     <http://www.semanticweb.org/ontologies/Daan/2020/BarbaraNanning#2017> ;
        :Involves         :AssistantOfBarbara , :LuděkKout , :BarbaraNanning ;
        :Located-In       :Lindava ;
        :Part-Of          :Creation_Artwork_17_33 ;
        :Requires-Use-Of  :Garage , :AnnealingKiln , :BlowingPipe , :FusingKiln , :Paper , :Furnace , :Water .

:ARTWORK_46_Photographing
        a              :Photographing , owl:NamedIndividual ;
        rdfs:comment   "Instance of an activity which is part of the creation process of ARTWORK_46."@en ;
        rdfs:label     "ARTWORK_46_Photographing"@en ;
        :Followed-By   :ARTWORK_46_Packing_3 ;
        :Follows       :ARTWORK_46_Transporting_2 ;
        :Has-Duration  <http://www.semanticweb.org/ontologies/Daan/2020/BarbaraNanning#2018> ;
        :Involves      <http://www.semanticweb.org/ontologies/Daan/2020/BarbaraNanning#TomHaartsen_Ouderkerka/dAmstel(NL)> , :BarbaraNanning ;
        :Located-In    <http://www.semanticweb.org/ontologies/Daan/2020/BarbaraNanning#Ouderkerka/dAmstel> ;
        :Part-Of       :Creation_Artwork_46 .

:ARTWORK_44_Packing_4
        a              owl:NamedIndividual , :Packing ;
        rdfs:comment   "Instance of an activity which is part of the creation process of ARTWORK_44."@en ;
        rdfs:label     "ARTWORK_44_Packing_4"@en ;
        :Followed-By   :ARTWORK_44_Transporting_4 ;
        :Follows       <http://www.semanticweb.org/ontologies/Daan/2020/BarbaraNanning#ARTWORK_44_ExaminingQuality(FinalResult)> ;
        :Has-Duration  <http://www.semanticweb.org/ontologies/Daan/2020/BarbaraNanning#2018> ;
        :Involves      :VáçlavNovák_Doksy_CzechRepublic , :AlešZvěřina , :BarbaraNanning ;
        :Located-In    :CzechRepublic ;
        :Part-Of       :Creation_Artwork_44 .

:ARTWORK_44_Documenting
        a              :Documenting , owl:NamedIndividual ;
        rdfs:comment   "Instance of an activity which is part of the creation process of ARTWORK_44."@en ;
        rdfs:label     "ARTWORK_44_Documenting"@en ;
        :Followed-By   :ARTWORK_44_Packing_5 ;
        :Follows       :ARTWORK_44_Photographing ;
        :Has-Duration  <http://www.semanticweb.org/ontologies/Daan/2020/BarbaraNanning#2018> ;
        :Involves      :BarbaraNanning ;
        :Located-In    :CzechRepublic ;
        :Part-Of       :Creation_Artwork_44 .

:ARTWORK_73_Polishing
        a                 owl:NamedIndividual , :Polishing ;
        rdfs:comment      "Instance of an activity which is part of the creation process of ARTWORK_73."@en ;
        rdfs:label        "ARTWORK_73_Polishing"@en ;
        :Followed-By      <http://www.semanticweb.org/ontologies/Daan/2020/BarbaraNanning#ARTWORK_73_ExaminingQuality(Result)> ;
        :Follows          :ARTWORK_73_Grinding ;
        :Has-Duration     <http://www.semanticweb.org/ontologies/Daan/2020/BarbaraNanning#2018> ;
        :Involves         :BarbaraNanning , :AlešZvěřina , :LukášSvoboda ;
        :Located-In       :CzechRepublic ;
        :Part-Of          :Creation_Artwork_73 ;
        :Requires-Use-Of  :PolishingStone .

:Packing  a              owl:Class ;
        rdfs:comment     "Packing is an activity in which a thing in put in a packaging."@en ;
        rdfs:label       "Packing"@en ;
        rdfs:subClassOf  :Activity .

:Slumping_Sheets_and_Strings
        a                owl:Class ;
        rdfs:comment     "A variety of coloured flat glass and strings that are used to create a design that when reheated will create the final form."@en ;
        rdfs:label       "Slumping Sheets and Strings"@en ;
        rdfs:subClassOf  :Slumping .

<http://www.wikidata.org/entity/Q515>
        a       owl:Class .

:ARTWORK_36_SlumpingPanel
        a                 :Slumping_Panel , owl:NamedIndividual ;
        rdfs:comment      "Instance of an activity which is part of the creation process of ARTWORK_36."@en ;
        rdfs:label        "ARTWORK_36_Slumping Panel"@en ;
        :Followed-By      :ARTWORK_36_TransportingMetalBowlWithPanel ;
        :Follows          :ARTWORK_36_FlatFusingSheetsWithARTWORK36PeacockToOnePanel ;
        :Has-Duration     <http://www.semanticweb.org/ontologies/Daan/2020/BarbaraNanning#2019> ;
        :Involves         :BarbaraNanning ;
        :Located-In       :Amsterdam ;
        :Part-Of          :Creation_Artwork_36 ;
        :Requires-Use-Of  :FusingKiln .

:Master_Glass_Blower  a  owl:Class ;
        rdfs:comment     "The master glass blower is the highest role within a glass blowing team."@en ;
        rdfs:label       "Master Glass Blower"@en ;
        rdfs:subClassOf  :Glass_Blower .

:ARTWORK_36_Transporting_2
        a              :Transporting , owl:NamedIndividual ;
        rdfs:comment   "Instance of an activity which is part of the creation process of ARTWORK_36."@en ;
        rdfs:label     "ARTWORK_36_Transporting_2"@en ;
        :Followed-By   :ARTWORK_36_Sandblasting ;
        :Follows       :ARTWORK_36_Packing_2 ;
        :Has-Duration  <http://www.semanticweb.org/ontologies/Daan/2020/BarbaraNanning#2015> ;
        :Involves      :AlešZvěřina , :BarbaraNanning ;
        :Located-In    :NovyBor ;
        :Part-Of       :Creation_Artwork_36 .

:ARTWORK_46_ExaminingTheQualityOfTheGlass
        a                 :Examining_the_Quality_of_the_Glass , owl:NamedIndividual ;
        rdfs:comment      "Instance of an activity which is part of the creation process of ARTWORK_46."@en ;
        rdfs:label        "ARTWORK_46_Examining the Quality of the Glass"@en ;
        :Followed-By      :ARTWORK_46_ApplyingClearGlassBell ;
        :Follows          :ARTWORK_46_SetupAndTestingOfTheMetalMold ;
        :Has-Duration     <http://www.semanticweb.org/ontologies/Daan/2020/BarbaraNanning#2018> ;
        :Involves         :BarbaraNanning , <http://www.semanticweb.org/ontologies/Daan/2020/BarbaraNanning#JiriPacinek(CZ)> ;
        :Located-In       :Lindava ;
        :Part-Of          :Creation_Artwork_46 ;
        :Requires-Use-Of  :Paper , :Jacks , :Furnace , :Pontis , :DiamondShears , :StraightShears , :Water , :YokeOfSupport , :Blocks , :CeramicPotFilledWithGlass , :GloryHole , :BlowingPipe , :AnnealingKiln .

:ARTWORK_78_Modeling  a   owl:NamedIndividual , :Modeling ;
        rdfs:comment      "Instance of an activity which is part of the creation process of ARTWORK_78."@en ;
        rdfs:label        "ARTWORK_78_Modeling"@en ;
        :Followed-By      <http://www.semanticweb.org/ontologies/Daan/2020/BarbaraNanning#ARTWORK_78_ExaminingQuality(Shape/Form)> ;
        :Follows          :ARTWORK_78_Sensing ;
        :Has-Duration     <http://www.semanticweb.org/ontologies/Daan/2020/BarbaraNanning#2008> ;
        :Involves         <http://www.semanticweb.org/ontologies/Daan/2020/BarbaraNanning#AlesVacek(CZ)> , <http://www.semanticweb.org/ontologies/Daan/2020/BarbaraNanning#RobertHlavacek(CZ)> , :AssistantOfBarbara , <http://www.semanticweb.org/ontologies/Daan/2020/BarbaraNanning#RomanTomis(CZ)> , :BarbaraNanning , <http://www.semanticweb.org/ontologies/Daan/2020/BarbaraNanning#RostislavMaterka(CZ)> ;
        :Located-In       :CzechRepublic ;
        :Part-Of          :Creation_Artwork_78 ;
        :Requires-Use-Of  :BlowingPipe , :AirCompressor , :PropaneTorch , :Gloves , :InterchangeableMetalMoldSetup .

:ARTWORK_46_Grinding  a   :Grinding , owl:NamedIndividual ;
        rdfs:comment      "Instance of an activity which is part of the creation process of ARTWORK_46."@en ;
        rdfs:label        "ARTWORK_46_Grinding_2"@en ;
        :Followed-By      :ARTWORK_46_Polishing ;
        :Follows          :ARTWORK_46_Sensing_2 ;
        :Has-Duration     <http://www.semanticweb.org/ontologies/Daan/2020/BarbaraNanning#2018> ;
        :Involves         :AlešZvěřina , :BarbaraNanning , :RobertFlorian ;
        :Located-In       :NovyBor ;
        :Part-Of          :Creation_Artwork_46 ;
        :Requires-Use-Of  :SharpeningStone , :GrindingWheel .

:ARTWORK_36_Modeling_2
        a                 owl:NamedIndividual , :Modeling ;
        rdfs:comment      "Instance of an activity which is part of the creation process of ARTWORK_36."@en ;
        rdfs:label        "ARTWORK_36_Modeling_2"@en ;
        :Followed-By      <http://www.semanticweb.org/ontologies/Daan/2020/BarbaraNanning#ARTWORK_36_ExaminingQuality(Shape/Form)_2> ;
        :Follows          :ARTWORK_36_Sensing_2 ;
        :Has-Duration     <http://www.semanticweb.org/ontologies/Daan/2020/BarbaraNanning#2019> ;
        :Involves         :BarbaraNanning , :DavidČerný , :JanBaštýř , <http://www.semanticweb.org/ontologies/Daan/2020/BarbaraNanning#JiriPacinek(CZ)> , :JiříPačinekJunior , :JaroslavKubásek ;
        :Located-In       :Lindava ;
        :Part-Of          :Creation_Artwork_36 ;
        :Requires-Use-Of  :BlowingPipe , :AirCompressor , :InterchangeableMetalMoldSetup , :PropaneTorch , :Gloves .

:ARTWORK_46_ApplyingClearOverlay
        a                 owl:NamedIndividual , :Applying_Clear_Overlay ;
        rdfs:comment      "Instance of an activity which is part of the creation process of ARTWORK_46."@en ;
        rdfs:label        "ARTWORK_46_Applying Clear Overlay"@en ;
        :Followed-By      :ARTWORK_46_ApplyingClearOverlay ;
        :Follows          :ARTWORK_46_ApplyingClearGlassBell ;
        :Has-Duration     <http://www.semanticweb.org/ontologies/Daan/2020/BarbaraNanning#2018> ;
        :Involves         <http://www.semanticweb.org/ontologies/Daan/2020/BarbaraNanning#JessicaHomich(USA)> , <http://www.semanticweb.org/ontologies/Daan/2020/BarbaraNanning#JiriPacinek(CZ)> , :JanBaštýř , :JaroslavKubásek , :JiříPačinekJunior , :DavidČerný , :BarbaraNanning ;
        :Located-In       :Lindava ;
        :Part-Of          :Creation_Artwork_46 ;
        :Requires-Use-Of  :Tagliol , :AirCompressor , :Beeswax , :Hook , :YokeOfSupport , :Water , :Jacks , :Furnace , :GrindingWheel , :GloryHole , :BlowingPipe , :Marver , :StraightShears , :Paper , :DiamondShears , :Blocks .

:Transporting_Monochrome_Rods
        a                owl:Class ;
        rdfs:comment     "Moving said objects from one place to another"@en ;
        rdfs:label       "Transporting Monochrome Rods"@en ;
        rdfs:subClassOf  :Transporting .

:Artwork_80  a        owl:NamedIndividual , :Glass_Artwork ;
        rdfs:comment  "Artwork by Barbara Nanning displayed in \"Barbara Nanning Eeuwige Beweging\" by Eliens (2019)."@en ;
        rdfs:label    "Verre églomisé (Alexandrite Glass)"@en ;
        :Created-By   :Creation_Artwork_80 ;
        :Has-Depth    "25"^^xsd:decimal ;
        :Has-Height   "22"^^xsd:decimal ;
        :Has-Width    "26"^^xsd:decimal ;
        :Is-Unica     "Yes"@en ;
        :Made-By      :LASVITAJETO , <http://www.semanticweb.org/ontologies/Daan/2020/BarbaraNanning#Ale%C5%A1Zv%C4%9B%C5%99ina&AZ-Design> , :VáçlavNovák_Doksy_CzechRepublic , :BarbaraNanning ;
        :Made-Out-Of  :AJETOClearGlass , <http://www.semanticweb.org/ontologies/Daan/2020/BarbaraNanning#ReichenbachColourRodsGlass(DE)> , :Platinum ;
        :Part-Of      :CollectionOfBarbaraNanning ;
        :Shown-By     :Image_Artwork_80 .

<http://www.semanticweb.org/ontologies/Daan/2020/BarbaraNanning#ARTWORK_44_ExaminingQuality(Shape/Form)>
        a                 owl:NamedIndividual , j.2: ;
        rdfs:comment      "Instance of an activity which is part of the creation process of ARTWORK_44."@en ;
        rdfs:label        "ARTWORK_44_Examining Quality (Shape/Form)"@en ;
        :Followed-By      :ARTWORK_44_Translocating ;
        :Follows          :ARTWORK_44_Modeling ;
        :Has-Duration     <http://www.semanticweb.org/ontologies/Daan/2020/BarbaraNanning#2008> ;
        :Involves         <http://www.semanticweb.org/ontologies/Daan/2020/BarbaraNanning#RadekKoten(CZ)> , :BarbaraNanning , :LuděkKout ;
        :Located-In       :CzechRepublic ;
        :Part-Of          :Creation_Artwork_44 ;
        :Requires-Use-Of  :BlowingPipe , :Pontis , :GloryHole .

:Activity  a              owl:Class ;
        rdfs:comment      "An activity is an event in which an actor does something."@en ;
        rdfs:label        "Activity"@en ;
        rdfs:subClassOf   :Event ;
        owl:disjointWith  :Creation_Event .

:ARTWORK_76_ApplyingClearGlassBell
        a                 owl:NamedIndividual , :Applying_Clear_Glass_Bell ;
        rdfs:comment      "Instance of an activity which is part of the creation process of ARTWORK_76."@en ;
        rdfs:label        "ARTWORK_76_Applying Clear Glass Bell"@en ;
        :Followed-By      :ARTWORK_76_ApplyingExtraColour ;
        :Follows          :ARTWORK_76_SetupAndTestingOfTheMetalMold_2 ;
        :Has-Duration     <http://www.semanticweb.org/ontologies/Daan/2020/BarbaraNanning#2018> ;
        :Involves         :BarbaraNanning , <http://www.semanticweb.org/ontologies/Daan/2020/BarbaraNanning#RadekKoten(CZ)> , <http://www.semanticweb.org/ontologies/Daan/2020/BarbaraNanning#LukasHavlas(CZ)> ;
        :Located-In       :CzechRepublic ;
        :Part-Of          :Creation_Artwork_76 ;
        :Processes        :AJETOClearGlass ;
        :Requires-Use-Of  :Paper , :IcePick , :BlowingPipe , :Furnace , :Blocks , :Jacks , :YokeOfSupport , :Beeswax , :Pincet , :StraightShears , :DiamondShears , :Marver , :CeramicPotFilledWithGlass , :Hook , :Water , :AirCompressor .

:ARTWORK_36_PreparingForBlowing
        a                 :Preparing_for_Blowing , owl:NamedIndividual ;
        rdfs:comment      "Instance of an activity which is part of the creation process of ARTWORK_36."@en ;
        rdfs:label        "ARTWORK_36_Preparing for Blowing"@en ;
        :Followed-By      :ARTWORK_36_FillingKilnsWithMetalBowl ;
        :Follows          :ARTWORK_36_TransportingMetalBowlWithCanes ;
        :Has-Duration     <http://www.semanticweb.org/ontologies/Daan/2020/BarbaraNanning#2015> ;
        :Involves         :BarbaraNanning , <http://www.semanticweb.org/ontologies/Daan/2020/BarbaraNanning#MiaLerssi(DN)> , :DurkValkema ;
        :Located-In       :Zaandam ;
        :Part-Of          :Creation_Artwork_36 ;
        :Requires-Use-Of  :FusingKiln , :BlowingPipe , :Furnace , :AnnealingKiln , :Garage , :Water , :Paper .

:Image_Artwork_79  a            :Digital_Image , owl:NamedIndividual ;
        rdfs:comment            "Image of an artwork by Barbara Nanning displayed in \"Barbara Nanning Eeuwige Beweging\" by Eliens (2019)."@en ;
        rdfs:label              "Image_Artwork_79"@en ;
        :Representation-Source  "Tom Haartsen_Ouderkerk a/d Amstel (NL)"@en ;
        :Shows                  :Artwork_79 .

:IcePick  a           :Tool , owl:NamedIndividual ;
        rdfs:comment  "an ice pick is a pointed tool used to pierce holes in things."@en ;
        rdfs:label    "Ice Pick"@en ;
        owl:sameAs    <http://www.wikidata.org/entity/Q586319> ;
        :Used-For     :ARTWORK_74_ApplyingExtraColour_2 , :ARTWORK_76_ApplyingClearGlassBell , :ARTWORK_74_ApplyingExtraColour , :ARTWORK_43_Glassblowing , :ARTWORK_80_ApplyingExtraColour , :ARTWORK_79_Glassblowing , :ARTWORK_73_Glassblowing , :ARTWORK_75_Glassblowing , :ARTWORK_78_ApplyingClearGlassBell , :ARTWORK_74_ApplyingClearGlassBell , :ARTWORK_43_ApplyingClearGlassBell , :ARTWORK_44_Glassblowing , :ARTWORK_76_ApplyingExtraColour_2 , :ARTWORK_44_ApplyingClearGlassBell , :ARTWORK_77_ApplyingExtraColour , :ARTWORK_44_ApplyingExtraColour , :ARTWORK_74_Glassblowing , :ARTWORK_80_ApplyingClearGlassBell , :ARTWORK_79_ApplyingExtraColour_2 , :ARTWORK_78_ApplyingExtraColour , :ARTWORK_43_ApplyingExtraColour , :ARTWORK_77_Glassblowing , :ARTWORK_75_ApplyingClearGlassBell , :ARTWORK_79_ApplyingExtraColour , :ARTWORK_75_ApplyingExtraColour_2 , :ARTWORK_76_ApplyingExtraColour , :ARTWORK_73_ApplyingClearGlassBell , :ARTWORK_76_Glassblowing , :ARTWORK_80_Glassblowing , :ARTWORK_78_Glassblowing , :ARTWORK_77_ApplyingClearGlassBell , :ARTWORK_44_ApplyingExtraColour_2 , :ARTWORK_79_ApplyingClearGlassBell , :ARTWORK_75_ApplyingExtraColour .

:ARTWORK_36_TransportingMetalBowlWithCanes
        a              owl:NamedIndividual , :Transporting_Metal_Bowl_with_Canes ;
        rdfs:comment   "Instance of an activity which is part of the creation process of ARTWORK_36."@en ;
        rdfs:label     "ARTWORK_36_Transporting Metal Bowl with Canes"@en ;
        :Followed-By   :ARTWORK_36_PreparingForBlowing ;
        :Follows       :ARTWORK_36_TackfusingColouredCanes ;
        :Has-Duration  <http://www.semanticweb.org/ontologies/Daan/2020/BarbaraNanning#2015> ;
        :Involves      :BarbaraNanning ;
        :Located-In    :Amsterdam ;
        :Part-Of       :Creation_Artwork_36 .

:ARTWORK_43_SetupAndTestingOfTheMetalMold
        a                 :Setup_and_Testing_of_the_Metal_Mold , owl:NamedIndividual ;
        rdfs:comment      "Instance of an activity which is part of the creation process of ARTWORK_43."@en ;
        rdfs:label        "ARTWORK_43_Setup and Testing of the Metal Mold"@en ;
        :Followed-By      :ARTWORK_43_PreparingGlass ;
        :Follows          :ARTWORK_43_ExaminingTheQualityOfTheGlass ;
        :Has-Duration     <http://www.semanticweb.org/ontologies/Daan/2020/BarbaraNanning#2008> ;
        :Involves         :AssistantOfBarbara , <http://www.semanticweb.org/ontologies/Daan/2020/BarbaraNanning#RomanTomis(CZ)> , <http://www.semanticweb.org/ontologies/Daan/2020/BarbaraNanning#RostislavMaterka(CZ)> , <http://www.semanticweb.org/ontologies/Daan/2020/BarbaraNanning#AlesVacek(CZ)> , <http://www.semanticweb.org/ontologies/Daan/2020/BarbaraNanning#RobertHlavacek(CZ)> , :BarbaraNanning ;
        :Located-In       :CzechRepublic ;
        :Part-Of          :Creation_Artwork_43 ;
        :Requires-Use-Of  :InterchangeableMetalMoldSetup .

:ARTWORK_73_PreparingGlass
        a                 owl:NamedIndividual , :Preparing_Glass ;
        rdfs:comment      "Instance of an activity which is part of the creation process of ARTWORK_73."@en ;
        rdfs:label        "ARTWORK_73_Preparing Glass"@en ;
        :Followed-By      :ARTWORK_73_SetupAndTestingOfTheMetalMold ;
        :Has-Duration     <http://www.semanticweb.org/ontologies/Daan/2020/BarbaraNanning#2018> ;
        :Involves         :BarbaraNanning , <http://www.semanticweb.org/ontologies/Daan/2020/BarbaraNanning#RadekKoten(CZ)> ;
        :Located-In       :CzechRepublic ;
        :Part-Of          :Creation_Artwork_73 ;
        :Requires-Use-Of  :GloryHole , :BlowingPipe , :Marver , :Pontis , :Garage ;
        :Starts           :Creation_Artwork_73 .

:ARTWORK_80_Glassblowing
        a                 :Glassblowing , owl:NamedIndividual ;
        rdfs:comment      "Instance of an activity which is part of the creation process of ARTWORK_80."@en ;
        rdfs:label        "ARTWORK_80_Glassblowing"@en ;
        :Followed-By      :ARTWORK_80_Sensing ;
        :Follows          :ARTWORK_80_HeatingMetalMold ;
        :Has-Duration     <http://www.semanticweb.org/ontologies/Daan/2020/BarbaraNanning#2018> ;
        :Involves         :AssistantOfBarbara , <http://www.semanticweb.org/ontologies/Daan/2020/BarbaraNanning#LukasHavlas(CZ)> , <http://www.semanticweb.org/ontologies/Daan/2020/BarbaraNanning#RadekKoten(CZ)> , <http://www.semanticweb.org/ontologies/Daan/2020/BarbaraNanning#Tom%C3%A1%C5%A1Moravec(CZ)> , :BarbaraNanning , <http://www.semanticweb.org/ontologies/Daan/2020/BarbaraNanning#JiriMoravec(CZ)> ;
        :Located-In       :CzechRepublic ;
        :Part-Of          :Creation_Artwork_80 ;
        :Requires-Use-Of  :CeramicPotFilledWithGlass , :Jacks , :Gloves , :Blocks , :StraightShears , :Marver , :BlowingPipe , :GloryHole , :Paper , :Hook , :Beeswax , :Water , :InterchangeableMetalMoldSetup , :Pontis , :IcePick , :BitIron , :DiamondShears , :Furnace , :PropaneTorch , :AnnealingKiln , :Tagliol , :Pincet , :AirCompressor , :YokeOfSupport , :Fork .

:ARTWORK_74_ApplyingExtraColour
        a                 :Applying_Extra_Colour , owl:NamedIndividual ;
        rdfs:comment      "Instance of an activity which is part of the creation process of ARTWORK_74."@en ;
        rdfs:label        "ARTWORK_74_Applying Extra Colour"@en ;
        :Followed-By      :ARTWORK_74_ApplyingExtraColour_2 ;
        :Follows          :ARTWORK_74_ApplyingClearGlassBell ;
        :Has-Duration     <http://www.semanticweb.org/ontologies/Daan/2020/BarbaraNanning#2008> ;
        :Involves         <http://www.semanticweb.org/ontologies/Daan/2020/BarbaraNanning#AlesVacek(CZ)> , :BarbaraNanning , <http://www.semanticweb.org/ontologies/Daan/2020/BarbaraNanning#RostislavMaterka(CZ)> ;
        :Located-In       :CzechRepublic ;
        :Part-Of          :Creation_Artwork_74 ;
        :Processes        :AJETORedGlass ;
        :Requires-Use-Of  :Pontis , :Fork , :Tagliol , :Pincet , :GloryHole , :Water , :Paper , :CeramicPotFilledWithGlass , :Jacks , :AnnealingKiln , :IcePick , :Marver , :Garage , :Beeswax , :YokeOfSupport , :Blocks , :Furnace , :BlowingPipe , :Hook , :DiamondShears , :AirCompressor , :StraightShears .

:ARTWORK_74_Sawing  a     owl:NamedIndividual , :Sawing ;
        rdfs:comment      "Instance of an activity which is part of the creation process of ARTWORK_74."@en ;
        rdfs:label        "ARTWORK_74_Sawing"@en ;
        :Followed-By      :ARTWORK_74_Grinding ;
        :Follows          <http://www.semanticweb.org/ontologies/Daan/2020/BarbaraNanning#ARTWORK_74_ExaminingQuality(CheckForIrregularitiesInTheGlass)> ;
        :Has-Duration     <http://www.semanticweb.org/ontologies/Daan/2020/BarbaraNanning#2008> ;
        :Involves         :AlešZvěřina , :BarbaraNanning ;
        :Located-In       :CzechRepublic ;
        :Part-Of          :Creation_Artwork_74 ;
        :Requires-Use-Of  :DiamondSaw .

:Creation_Artwork_77  a  :Creation_Event , owl:NamedIndividual ;
        rdfs:comment    "Creation event for an artwork by Barbara Nanning displayed in \"Barbara Nanning Eeuwige Beweging\" by Eliens (2019)."@en ;
        rdfs:label      "Creation_Artwork_77"@en ;
        :Consists-Of    :ARTWORK_77_ApplyingExtraColour , :ARTWORK_77_Packing_2 , :ARTWORK_77_SetupAndTestingOfTheMetalMold_2 , <http://www.semanticweb.org/ontologies/Daan/2020/BarbaraNanning#ARTWORK_77_ExaminingQuality(FinalResult)> , :ARTWORK_77_SetupAndTestingOfTheMetalMold , :ARTWORK_77_Glassblowing , :ARTWORK_77_Packing_4 , :ARTWORK_77_Grinding , :ARTWORK_77_Signing , :ARTWORK_77_Modeling , :ARTWORK_77_Resting , :ARTWORK_77_Packing_3 , :ARTWORK_77_Packing , <http://www.semanticweb.org/ontologies/Daan/2020/BarbaraNanning#ARTWORK_77_ExaminingQuality(Result)> , :ARTWORK_77_HeatingMetalMold , :ARTWORK_77_PreparingGlass , :ARTWORK_77_Translocating , :ARTWORK_77_Packing_5 , :ARTWORK_77_Transporting , :ARTWORK_77_Sawing , :ARTWORK_77_ExaminingTheQualityOfTheGlass , :ARTWORK_77_MeasuringAndBoxesMaking , :ARTWORK_77_Photographing , :ARTWORK_77_ApplyingClearGlassBell , <http://www.semanticweb.org/ontologies/Daan/2020/BarbaraNanning#ARTWORK_77_ExaminingQuality(Shape/Form)> , :ARTWORK_77_Transporting_2 , :ARTWORK_77_Gilding , :ARTWORK_77_Sensing , :ARTWORK_77_Cooling , <http://www.semanticweb.org/ontologies/Daan/2020/BarbaraNanning#ARTWORK_77_ExaminingQuality(CheckForIrregularitiesInTheGlass)> , :ARTWORK_77_Polishing , :ARTWORK_77_Documenting , :ARTWORK_77_Transporting_4 , :ARTWORK_77_Transporting_3 ;
        :Created        :Artwork_77 ;
        :Finishes-With  :ARTWORK_77_Packing_5 ;
        :Has-Duration   <http://www.semanticweb.org/ontologies/Daan/2020/BarbaraNanning#2018> ;
        :Located-In     :CzechRepublic ;
        :Starts-With    :ARTWORK_77_PreparingGlass ;
        :Within-Period  :GlassVerreÉglomisé .

:LenkaUhlířová  a     :Grinder_4 , owl:NamedIndividual ;
        rdfs:comment  "Lenka Uhlířová is a Grinder 4."@en ;
        rdfs:label    "Lenka Uhlířová"@en ;
        :Works-For    <http://www.semanticweb.org/ontologies/Daan/2020/BarbaraNanning#Ale%C5%A1Zv%C4%9B%C5%99ina&AZ-Design> .

<http://vocab.getty.edu/aat/300312281>
        a                    owl:Class ;
        owl:equivalentClass  :Museum .

:ARTWORK_77_Packing_5
        a              owl:NamedIndividual , :Packing ;
        rdfs:comment   "Instance of an activity which is part of the creation process of ARTWORK_77."@en ;
        rdfs:label     "ARTWORK_77_Packing_5"@en ;
        :Finishes      :Creation_Artwork_77 ;
        :Follows       :ARTWORK_77_Documenting ;
        :Has-Duration  <http://www.semanticweb.org/ontologies/Daan/2020/BarbaraNanning#2018> ;
        :Involves      :BarbaraNanning ;
        :Located-In    :CzechRepublic ;
        :Part-Of       :Creation_Artwork_77 .

:ARTWORK_17_33_Packing_3
        a              owl:NamedIndividual , :Packing ;
        rdfs:comment   "Instance of an activity which is part of the creation process of ARTWORK_17_33."@en ;
        rdfs:label     "ARTWORK_17_33_Packing_3"@en ;
        :Followed-By   :ARTWORK_17_33_Documenting ;
        :Follows       :ARTWORK_17_33_Photographing ;
        :Has-Duration  <http://www.semanticweb.org/ontologies/Daan/2020/BarbaraNanning#2017> ;
        :Involves      :BarbaraNanning ;
        :Located-In    :Amsterdam ;
        :Part-Of       :Creation_Artwork_17_33 .

:ARTWORK_44_PreparingGlass
        a                 owl:NamedIndividual , :Preparing_Glass ;
        rdfs:comment      "Instance of an activity which is part of the creation process of ARTWORK_44."@en ;
        rdfs:label        "ARTWORK_44_Preparing Glass"@en ;
        :Followed-By      :ARTWORK_44_SetupAndTestingOfTheMetalMold ;
        :Has-Duration     <http://www.semanticweb.org/ontologies/Daan/2020/BarbaraNanning#2018> ;
        :Involves         :BarbaraNanning , <http://www.semanticweb.org/ontologies/Daan/2020/BarbaraNanning#RadekKoten(CZ)> ;
        :Located-In       :CzechRepublic ;
        :Part-Of          :Creation_Artwork_44 ;
        :Requires-Use-Of  :GloryHole , :Garage , :BlowingPipe , :Marver , :Pontis ;
        :Starts           :Creation_Artwork_44 .

:ARTWORK_73_Packing  a  :Packing , owl:NamedIndividual ;
        rdfs:comment   "Instance of an activity which is part of the creation process of ARTWORK_73."@en ;
        rdfs:label     "ARTWORK_73_Packing"@en ;
        :Followed-By   :ARTWORK_73_Transporting ;
        :Follows       :ARTWORK_73_Cooling ;
        :Has-Duration  <http://www.semanticweb.org/ontologies/Daan/2020/BarbaraNanning#2018> ;
        :Involves      :BarbaraNanning , :AlešZvěřina ;
        :Located-In    :CzechRepublic ;
        :Part-Of       :Creation_Artwork_73 .

:ARTWORK_74_Transporting_3
        a              :Transporting , owl:NamedIndividual ;
        rdfs:comment   "Instance of an activity which is part of the creation process of ARTWORK_74."@en ;
        rdfs:label     "ARTWORK_74_Transporting_3"@en ;
        :Followed-By   :ARTWORK_74_Gilding ;
        :Follows       :ARTWORK_74_Packing_3 ;
        :Has-Duration  <http://www.semanticweb.org/ontologies/Daan/2020/BarbaraNanning#2008> ;
        :Involves      :AlešZvěřina , :BarbaraNanning ;
        :Located-In    :CzechRepublic ;
        :Part-Of       :Creation_Artwork_74 .

:ARTWORK_80_Packing  a  :Packing , owl:NamedIndividual ;
        rdfs:comment   "Instance of an activity which is part of the creation process of ARTWORK_80."@en ;
        rdfs:label     "ARTWORK_80_Packing"@en ;
        :Followed-By   :ARTWORK_80_Transporting ;
        :Follows       :ARTWORK_80_Cooling ;
        :Has-Duration  <http://www.semanticweb.org/ontologies/Daan/2020/BarbaraNanning#2018> ;
        :Involves      :BarbaraNanning , :AlešZvěřina ;
        :Located-In    :CzechRepublic ;
        :Part-Of       :Creation_Artwork_80 .

:ARTWORK_39_Grinding  a   owl:NamedIndividual , :Grinding ;
        rdfs:comment      "Instance of an activity which is part of the creation process of ARTWORK_39."@en ;
        rdfs:label        "ARTWORK_39_Grinding"@en ;
        :Followed-By      :ARTWORK_39_Polishing ;
        :Follows          :ARTWORK_39_Sensing_2 ;
        :Has-Duration     <http://www.semanticweb.org/ontologies/Daan/2020/BarbaraNanning#2015> ;
        :Involves         :RobertFlorian , :AlešZvěřina , :BarbaraNanning ;
        :Located-In       :NovyBor ;
        :Part-Of          :Creation_Artwork_39 ;
        :Requires-Use-Of  :SharpeningStone , :GrindingWheel .

:ARTWORK_46_TackfusingColouredCanesAndStrings
        a                 owl:NamedIndividual , :Tackfusing_Coloured_Canes_and_Strings ;
        rdfs:comment      "Instance of an activity which is part of the creation process of ARTWORK_46."@en ;
        rdfs:label        "ARTWORK_46_Tackfusing Coloured Canes and Strings"@en ;
        :Followed-By      :ARTWORK_46_TransportingMetalBowlWithCanesAndStrings ;
        :Follows          :ARTWORK_46_MakingPatternsWithColouredCanesAndStringsInTheMetalBowl ;
        :Has-Duration     <http://www.semanticweb.org/ontologies/Daan/2020/BarbaraNanning#2018> ;
        :Involves         :BarbaraNanning ;
        :Located-In       :Amsterdam ;
        :Part-Of          :Creation_Artwork_46 ;
        :Requires-Use-Of  :FusingKiln .

:Collection  a           owl:Class ;
        rdfs:comment     "A collection is a group of things."@en ;
        rdfs:label       "Collection"@en ;
        rdfs:subClassOf  :Thing .

:ARTWORK_75_Sensing  a  owl:NamedIndividual , :Sensing ;
        rdfs:comment   "Instance of an activity which is part of the creation process of ARTWORK_75."@en ;
        rdfs:label     "ARTWORK_75_Sensing"@en ;
        :Followed-By   :ARTWORK_75_Modeling ;
        :Follows       :ARTWORK_75_Glassblowing ;
        :Has-Duration  <http://www.semanticweb.org/ontologies/Daan/2020/BarbaraNanning#2018> ;
        :Involves      :LukášSvoboda , :BarbaraNanning , :AlešZvěřina ;
        :Located-In    :CzechRepublic ;
        :Part-Of       :Creation_Artwork_75 .

:ARTWORK_36_DecidingColourPaletteAndPatterns
        a              :Deciding_Colour_Palette_and_Patterns , owl:NamedIndividual ;
        rdfs:comment   "Instance of an activity which is part of the creation process of ARTWORK_36."@en ;
        rdfs:label     "ARTWORK_36_Deciding Colour Palette and Patterns"@en ;
        :Followed-By   :ARTWORK_36_CuttingMonochromeSheets ;
        :Has-Duration  <http://www.semanticweb.org/ontologies/Daan/2020/BarbaraNanning#2015> ;
        :Involves      :BarbaraNanning ;
        :Located-In    :Amsterdam ;
        :Part-Of       :Creation_Artwork_36 ;
        :Processes     :BullseyeGlass ;
        :Starts        :Creation_Artwork_36 .

:ARTWORK_36_Photographing
        a              :Photographing , owl:NamedIndividual ;
        rdfs:comment   "Instance of an activity which is part of the creation process of ARTWORK_36."@en ;
        rdfs:label     "ARTWORK_36_Photographing"@en ;
        :Followed-By   :ARTWORK_36_Packing_4 ;
        :Follows       :ARTWORK_36_Transporting_3 ;
        :Has-Duration  <http://www.semanticweb.org/ontologies/Daan/2020/BarbaraNanning#2019> ;
        :Involves      :BarbaraNanning , <http://www.semanticweb.org/ontologies/Daan/2020/BarbaraNanning#TomHaartsen_Ouderkerka/dAmstel(NL)> ;
        :Located-In    <http://www.semanticweb.org/ontologies/Daan/2020/BarbaraNanning#Ouderkerka/dAmstel> ;
        :Part-Of       :Creation_Artwork_36 .

:PropaneTorch  a      :Tool , owl:NamedIndividual ;
        rdfs:comment  "A propane torch is a tool used to heat things with a flame."@en ;
        rdfs:label    "Propane Torch"@en ;
        :Used-For     :ARTWORK_44_Modeling , :ARTWORK_74_Glassblowing , :ARTWORK_43_HeatingMetalMold , :ARTWORK_80_Glassblowing , :ARTWORK_76_Modeling , :ARTWORK_78_Glassblowing , :ARTWORK_77_HeatingMetalMold , :ARTWORK_75_HeatingMetalMold , :ARTWORK_79_Modeling , :ARTWORK_80_Modeling , :ARTWORK_77_Modeling , :ARTWORK_73_HeatingMetalMold , :ARTWORK_43_Glassblowing , :ARTWORK_44_Glassblowing , :ARTWORK_80_HeatingMetalMold , :ARTWORK_78_HeatingMetalMold , :ARTWORK_78_Modeling , :ARTWORK_73_Glassblowing , :ARTWORK_74_HeatingMetalMold , :ARTWORK_73_Modeling , :ARTWORK_76_HeatingMetalMold , :ARTWORK_79_Glassblowing , :ARTWORK_76_Glassblowing , :ARTWORK_74_Modeling , :ARTWORK_43_Modeling , :ARTWORK_75_Glassblowing , :ARTWORK_44_HeatingMetalMold , :ARTWORK_79_HeatingMetalMold , :ARTWORK_75_Modeling , :ARTWORK_77_Glassblowing .

:ARTWORK_18_64_TransportingColouredCanes_2
        a              :Transporting_Coloured_Canes , owl:NamedIndividual ;
        rdfs:comment   "Instance of an activity which is part of the creation process of ARTWORK_18_64."@en ;
        rdfs:label     "ARTWORK_18_64_Transporting Coloured Canes_2"@en ;
        :Followed-By   :ARTWORK_18_64_DecidingColourPaletteAndPatterns_2 ;
        :Follows       :ARTWORK_18_64_CuttingAndPolishingColouredCanes ;
        :Has-Duration  <http://www.semanticweb.org/ontologies/Daan/2020/BarbaraNanning#2015> ;
        :Involves      :AlešZvěřina , :BarbaraNanning ;
        :Located-In    :NovyBor ;
        :Part-Of       :Creation_Artwork_18_64 .

<http://www.semanticweb.org/ontologies/Daan/2020/BarbaraNanning#MarekEffmert(CZ)>
        a             :Second_Glass_Blower , owl:NamedIndividual ;
        rdfs:comment  "Marek Effmert (CZ) is a Second Glass Blower."@en ;
        rdfs:label    "Marek Effmert (CZ)"@en ;
        :Involved-In  :ARTWORK_36_PickingUpColouredCanesPattern , :ARTWORK_39_Modeling , :ARTWORK_39_SetupAndTestingOfTheMetalMold , :ARTWORK_18_64_Modeling , :ARTWORK_39_PickingUpColouredPanel , :ARTWORK_36_Modeling , :ARTWORK_36_SetupAndTestingOfTheMetalMold , :ARTWORK_36_ProducingColouredCanes , :ARTWORK_18_64_PickingUpColouredCanesPattern , :ARTWORK_18_64_Glassblowing , :ARTWORK_46_ProducingColouredCanes , :ARTWORK_36_Glassblowing , :ARTWORK_39_Glassblowing , :ARTWORK_18_64_ProducingColouredCanes , :ARTWORK_36_PickingUpColouredPanel ;
        :Works-For    :GlassStudioVanTetterode , :VRIJGLASZaandam .

:ARTWORK_78_HeatingMetalMold
        a                 :Heating_Metal_Mold , owl:NamedIndividual ;
        rdfs:comment      "Instance of an activity which is part of the creation process of ARTWORK_78."@en ;
        rdfs:label        "ARTWORK_78_Heating Metal Mold"@en ;
        :Followed-By      :ARTWORK_78_Glassblowing ;
        :Follows          :ARTWORK_78_ApplyingExtraColour ;
        :Has-Duration     <http://www.semanticweb.org/ontologies/Daan/2020/BarbaraNanning#2008> ;
        :Involves         :BarbaraNanning ;
        :Located-In       :CzechRepublic ;
        :Part-Of          :Creation_Artwork_78 ;
        :Requires-Use-Of  :Gloves , :InterchangeableMetalMoldSetup , :PropaneTorch .

:J.LohmannGallery  a  :Gallery , owl:NamedIndividual ;
        rdfs:comment  "The J. Lohmann Gallery is a gallery located in New York (United States of America)."@en ;
        rdfs:label    "J. Lohmann Gallery"@en ;
        :Located-In   :NewYork ;
        :Maintains    :CollectionJ.LohmannGallery .

:ARTWORK_79_ApplyingExtraColour_2
        a                 owl:NamedIndividual , :Applying_Extra_Colour ;
        rdfs:comment      "Instance of an activity which is part of the creation process of ARTWORK_79."@en ;
        rdfs:label        "ARTWORK_79_Applying Extra Colour_2"@en ;
        :Followed-By      :ARTWORK_79_HeatingMetalMold ;
        :Follows          :ARTWORK_79_ApplyingExtraColour ;
        :Has-Duration     <http://www.semanticweb.org/ontologies/Daan/2020/BarbaraNanning#2018> ;
        :Involves         <http://www.semanticweb.org/ontologies/Daan/2020/BarbaraNanning#RadekKoten(CZ)> , :BarbaraNanning , <http://www.semanticweb.org/ontologies/Daan/2020/BarbaraNanning#LukasHavlas(CZ)> ;
        :Located-In       :CzechRepublic ;
        :Part-Of          :Creation_Artwork_79 ;
        :Processes        :AJETOBlueGlass ;
        :Requires-Use-Of  :DiamondShears , :Furnace , :AnnealingKiln , :GloryHole , :Pincet , :Beeswax , :Tagliol , :Garage , :Hook , :Blocks , :CeramicPotFilledWithGlass , :Marver , :StraightShears , :Paper , :Water , :IcePick , :Pontis , :Fork , :YokeOfSupport , :Jacks , :AirCompressor , :BlowingPipe .

:ARTWORK_36_PreparingForBlowing_2
        a                 owl:NamedIndividual , :Preparing_for_Blowing ;
        rdfs:comment      "Instance of an activity which is part of the creation process of ARTWORK_17_33."@en ;
        rdfs:label        "ARTWORK_36_Preparing for Blowing_2"@en ;
        :Followed-By      :ARTWORK_17_33_FillingKilnsWithMetalBowl ;
        :Follows          :ARTWORK_17_33_TransportingMetalBowlWithCanes ;
        :Has-Duration     <http://www.semanticweb.org/ontologies/Daan/2020/BarbaraNanning#2019> ;
        :Involves         :BarbaraNanning , :LuděkKout , :AssistantOfBarbara ;
        :Located-In       :Lindava ;
        :Part-Of          :Creation_Artwork_17_33 ;
        :Requires-Use-Of  :Furnace , :Paper , :BlowingPipe , :Garage , :Water , :FusingKiln , :AnnealingKiln .

:Artwork_79  a        owl:NamedIndividual , :Glass_Artwork ;
        rdfs:comment  "Artwork by Barbara Nanning displayed in \"Barbara Nanning Eeuwige Beweging\" by Eliens (2019)."@en ;
        rdfs:label    "Verre églomisé"@en ;
        :Created-By   :Creation_Artwork_79 ;
        :Has-Depth    "22"^^xsd:decimal ;
        :Has-Height   "17"^^xsd:decimal ;
        :Has-Width    "27"^^xsd:decimal ;
        :Is-Unica     "Yes"@en ;
        :Made-By      :LASVITAJETO , <http://www.semanticweb.org/ontologies/Daan/2020/BarbaraNanning#Ale%C5%A1Zv%C4%9B%C5%99ina&AZ-Design> , :BarbaraNanning , :VáçlavNovák_Doksy_CzechRepublic ;
        :Made-Out-Of  :AJETOClearGlass , :PureDucat , :AJETOWhiteGlass , :AJETOBlueGlass ;
        :Part-Of      :CollectionWithUnknownOwner ;
        :Shown-By     :Image_Artwork_79 .

<http://www.wikidata.org/entity/Q507559>
        a       owl:NamedIndividual .

:ARTWORK_43_Packing_2
        a              :Packing , owl:NamedIndividual ;
        rdfs:comment   "Instance of an activity which is part of the creation process of ARTWORK_43."@en ;
        rdfs:label     "ARTWORK_43_Packing_2"@en ;
        :Followed-By   :ARTWORK_43_Transporting_2 ;
        :Follows       :ARTWORK_43_MeasuringAndBoxesMaking ;
        :Has-Duration  <http://www.semanticweb.org/ontologies/Daan/2020/BarbaraNanning#2008> ;
        :Involves      :BarbaraNanning , :AlešZvěřina ;
        :Located-In    :CzechRepublic ;
        :Part-Of       :Creation_Artwork_43 .

<http://vocab.getty.edu/aat/300053867>
        a                    owl:Class ;
        owl:equivalentClass  :Polishing .

:Zaandam  a           :City , owl:NamedIndividual ;
        rdfs:comment  "Zaandam is a city in the Netherlands."@en ;
        rdfs:label    "Zaandam"@en ;
        owl:sameAs    <http://sws.geonames.org/2744118> ;
        :Located-In   :Netherlands ;
        :Location-Of  :ARTWORK_36_TransportingColouredCanes , :ARTWORK_36_PreparingForBlowing , :ARTWORK_39_Cooling , :ARTWORK_36_ApplyingClearGlassBell , :ARTWORK_36_HeatingMetalMold , :ARTWORK_18_64_TransportingColouredCanes , :ARTWORK_18_64_Sensing , :ARTWORK_36_Sensing , :ARTWORK_39_Glassblowing , :ARTWORK_36_Cooling , :ARTWORK_36_SetupAndTestingOfTheMetalMold , :VRIJGLASZaandam , :ARTWORK_46_ProducingColouredCanes , :ARTWORK_39_Packing , :ARTWORK_39_PreparingForBlowing , :ARTWORK_39_Sensing , :ARTWORK_18_64_ProducingColouredCanes , :ARTWORK_36_Packing , :ARTWORK_18_64_Cooling , :ARTWORK_18_64_ApplyingClearGlassBell , :ARTWORK_18_64_Packing , :ARTWORK_39_PickingUpColouredPanel , :ARTWORK_36_CuttingSheets , <http://www.semanticweb.org/ontologies/Daan/2020/BarbaraNanning#ARTWORK_18_64_ExaminingQuality(Shape/Form)> , :ARTWORK_18_64_PickingUpColouredCanesPattern , :ARTWORK_36_FillingKilnsWithMetalBowl , :ARTWORK_18_64_Modeling , :ARTWORK_36_PreparingGlass , :ARTWORK_39_TransportingMetalBowlWithPanel , :ARTWORK_36_Glassblowing , :ARTWORK_36_ProducingColouredCanes , :ARTWORK_39_ApplyingClearGlassBell , :ARTWORK_46_TransportingColouredCanes , <http://www.semanticweb.org/ontologies/Daan/2020/BarbaraNanning#ARTWORK_36_ExaminingQuality(Shape/Form)> , :ARTWORK_36_Modeling , :ARTWORK_39_ExaminingTheQualityOfTheGlass , :ARTWORK_39_PreparingGlass , <http://www.semanticweb.org/ontologies/Daan/2020/BarbaraNanning#ARTWORK_39_ExaminingQuality(Shape/Form)> , :ARTWORK_36_ExaminingTheQualityOfTheGlass , :ARTWORK_39_SetupAndTestingOfTheMetalMold , :ARTWORK_39_HeatingMetalMold , :ARTWORK_18_64_Glassblowing , :ARTWORK_39_FillingKilnsWithMetalBowl , :ARTWORK_36_PickingUpColouredCanesPattern , :ARTWORK_39_Modeling .

<http://vocab.getty.edu/aat/300248479>
        a                    owl:Class ;
        owl:equivalentClass  :Place .

:Grinder_1  a            owl:Class ;
        rdfs:comment     "A Grinder 1 is an actor who is the first member of a team responsible for the grinding, polishing and sharpening of objects."@en ;
        rdfs:label       "Grinder 1"@en ;
        rdfs:subClassOf  :Grinder .

:Metal_Worker_3  a       owl:Class ;
        rdfs:comment     "A Metal Worker 3 is an actor who is the third member of a team responsible for creating metal objects or dealing with metal material."@en ;
        rdfs:label       "Metal Worker 3"@en ;
        rdfs:subClassOf  :Metal_Worker .

:Creation_Artwork_17_33
        a               owl:NamedIndividual , :Creation_Event ;
        rdfs:comment    "Creation event for Artwork_17_33 by Barbara Nanning."@en ;
        rdfs:label      "Creation_Artwork_17_33"@en ;
        :Consists-Of    :ARTWORK_17_33_TransportingColouredCanes , :ARTWORK_17_33_FillingKilnsWithMetalBowl , :ARTWORK_17_33_Modeling , :ARTWORK_17_33_FillingHolesWithClearGlass , <http://www.semanticweb.org/ontologies/Daan/2020/BarbaraNanning#ARTWORK_17_33_ExaminingQuality(CheckForIrregularitiesInTheGlass)> , :ARTWORK_17_33_Packing , :ARTWORK_17_33_MeasuringAndBoxesMaking , :ARTWORK_17_33_Sensing_2 , :ARTWORK_17_33_MakingPatternsWithColouredCanesInTheMetalBowl , :ARTWORK_17_33_ModelingWithTeflonStick , :ARTWORK_17_33_PickingUpColouredCanesPattern , :ARTWORK_17_33_Documenting , :ARTWORK_17_33_Cooling , :ARTWORK_17_33_ApplyingClearGlassBell , :ARTWORK_17_33_Sawing , :ARTWORK_17_33_DecidingColourPalette , :ARTWORK_17_33_PreparingGlass , :ARTWORK_17_33_Transporting , <http://www.semanticweb.org/ontologies/Daan/2020/BarbaraNanning#ARTWORK_17_33_ExaminingQuality(Result)> , :ARTWORK_17_33_CuttingAndPolishingColouredCanes , :ARTWORK_17_33_TransportingMetalBowlWithCanes , :ARTWORK_17_33_Sensing , :ARTWORK_17_33_Grinding , :ARTWORK_17_33_Polishing , :ARTWORK_17_33_DecidingColourPaletteAndPatterns , :ARTWORK_17_33_Packing_2 , :ARTWORK_17_33_Glassblowing , :ARTWORK_17_33_ApplyingClearOverlay , :ARTWORK_17_33_Signing , :ARTWORK_17_33_TransportingColouredCanes_2 , :ARTWORK_17_33_Photographing , :ARTWORK_17_33_TackfusingColouredCanes , :ARTWORK_17_33_ProducingColouredCanes , :ARTWORK_17_33_ExaminingTheQualityOfTheGlass , :ARTWORK_17_33_PreparingForBlowing , :ARTWORK_17_33_Packing_3 , :ARTWORK_17_33_Resting , <http://www.semanticweb.org/ontologies/Daan/2020/BarbaraNanning#ARTWORK_17_33_ExaminingQuality(Shape/Form)> , :ARTWORK_17_33_Transporting_2 ;
        :Created        :Artwork_17_33 ;
        :Finishes-With  :ARTWORK_17_33_Documenting ;
        :Starts-With    :ARTWORK_17_33_DecidingColourPaletteAndPatterns .

:ARTWORK_79_Photographing
        a              :Photographing , owl:NamedIndividual ;
        rdfs:comment   "Instance of an activity which is part of the creation process of ARTWORK_79."@en ;
        rdfs:label     "ARTWORK_79_Photographing"@en ;
        :Followed-By   :ARTWORK_79_Documenting ;
        :Follows       :ARTWORK_79_Transporting_4 ;
        :Has-Duration  <http://www.semanticweb.org/ontologies/Daan/2020/BarbaraNanning#2018> ;
        :Involves      <http://www.semanticweb.org/ontologies/Daan/2020/BarbaraNanning#TomHaartsen_Ouderkerka/dAmstel(NL)> , :BarbaraNanning ;
        :Located-In    :CzechRepublic ;
        :Part-Of       :Creation_Artwork_79 .

:Fourth_Glass_Blower  a  owl:Class ;
        rdfs:comment     "The fourth glass blower is the fifth highest role within a glass blowing team. While normal glass blowing teams consist of 4 people, Nanning required extra workforces."@en ;
        rdfs:label       "Fourth Glass Blower"@en ;
        rdfs:subClassOf  :Glass_Blower .

:ARTWORK_80_Modeling  a   :Modeling , owl:NamedIndividual ;
        rdfs:comment      "Instance of an activity which is part of the creation process of ARTWORK_80."@en ;
        rdfs:label        "ARTWORK_80_Modeling"@en ;
        :Followed-By      <http://www.semanticweb.org/ontologies/Daan/2020/BarbaraNanning#ARTWORK_80_ExaminingQuality(Shape/Form)> ;
        :Follows          :ARTWORK_80_Sensing ;
        :Has-Duration     <http://www.semanticweb.org/ontologies/Daan/2020/BarbaraNanning#2018> ;
        :Involves         <http://www.semanticweb.org/ontologies/Daan/2020/BarbaraNanning#LukasHavlas(CZ)> , <http://www.semanticweb.org/ontologies/Daan/2020/BarbaraNanning#RadekKoten(CZ)> , <http://www.semanticweb.org/ontologies/Daan/2020/BarbaraNanning#JiriMoravec(CZ)> , :AssistantOfBarbara , <http://www.semanticweb.org/ontologies/Daan/2020/BarbaraNanning#Tom%C3%A1%C5%A1Moravec(CZ)> , :BarbaraNanning ;
        :Located-In       :CzechRepublic ;
        :Part-Of          :Creation_Artwork_80 ;
        :Requires-Use-Of  :InterchangeableMetalMoldSetup , :Gloves , :PropaneTorch .

:Has-Depth  a         owl:DatatypeProperty ;
        rdfs:comment  "Has-Depth is a property which connects a thing with a depth in centimeters."@en ;
        rdfs:domain   :Thing ;
        rdfs:label    "Has-Depth"@en ;
        rdfs:range    xsd:integer .

:ARTWORK_73_Photographing
        a              owl:NamedIndividual , :Photographing ;
        rdfs:comment   "Instance of an activity which is part of the creation process of ARTWORK_73."@en ;
        rdfs:label     "ARTWORK_73_Photographing"@en ;
        :Followed-By   :ARTWORK_73_Documenting ;
        :Follows       :ARTWORK_73_Transporting_4 ;
        :Has-Duration  <http://www.semanticweb.org/ontologies/Daan/2020/BarbaraNanning#2018> ;
        :Involves      <http://www.semanticweb.org/ontologies/Daan/2020/BarbaraNanning#TomHaartsen_Ouderkerka/dAmstel(NL)> , :BarbaraNanning ;
        :Located-In    :CzechRepublic ;
        :Part-Of       :Creation_Artwork_73 .

<http://www.semanticweb.org/ontologies/Daan/2020/BarbaraNanning#2019>
        a             :Timespan , owl:NamedIndividual ;
        rdfs:comment  "2019 is a timespan."@en ;
        rdfs:label    "2019"@en ;
        owl:sameAs    <http://www.wikidata.org/entity/Q25274> ;
        :Duration-Of  <http://www.semanticweb.org/ontologies/Daan/2020/BarbaraNanning#ARTWORK_36_ExaminingQuality(FinalResult)_2> , <http://www.semanticweb.org/ontologies/Daan/2020/BarbaraNanning#ARTWORK_36_ExaminingQuality(FinalResult)> , :ARTWORK_36_Sensing_4 , :ARTWORK_36_Documenting_2 , :ARTWORK_36_DecidingColourPalette_2 , :ARTWORK_36_Photographing , :ARTWORK_36_Packing_3 , :ARTWORK_36_CuttingSheets , :ARTWORK_36_ApplyingMassivePieceOfClearGlass , :ARTWORK_36_Resting_2 , :ARTWORK_36_Transporting_6 , :ARTWORK_36_Transporting_4 , :ARTWORK_36_Grinding_2 , :ARTWORK_36_Packing_8 , :ARTWORK_36_Modeling_2 , :ARTWORK_36_Packing_5 , :ARTWORK_36_PickingUpColouredPanel , :ARTWORK_36_Sawing_2 , :ARTWORK_36_FlatFusingFinishedArtwork , :ARTWORK_36_Packing_4 , :ARTWORK_36_Signing_2 , :ARTWORK_36_OrdeningFlatSheets , :ARTWORK_36_FillingKilnsWithMetalBowl_2 , :ARTWORK_36_FlatFusingSheetsWithARTWORK36PeacockToOnePanel , :ARTWORK_36_SlumpingPanel , :ARTWORK_36_Polishing_2 , <http://www.semanticweb.org/ontologies/Daan/2020/BarbaraNanning#ARTWORK_36_ExaminingQuality(Result)_2> , :ARTWORK_36_Signing , :ARTWORK_36_TransportingMetalBowlWithPanel , :ARTWORK_36_Packing_6 , :ARTWORK_18_64_Signing , <http://www.semanticweb.org/ontologies/Daan/2020/BarbaraNanning#ARTWORK_36_ExaminingQuality(CheckForIrregularitiesInTheGlass)_2> , :ARTWORK_36_FusingSheets , :ARTWORK_36_Sensing_3 , :ARTWORK_36_Cooling_2 , :ARTWORK_36_ExaminingTheQualityOfTheGlass_2 , <http://www.semanticweb.org/ontologies/Daan/2020/BarbaraNanning#ARTWORK_36_ExaminingQuality(Shape/Form)_2> , :ARTWORK_36_Documenting , :ARTWORK_36_MeasuringAndBoxesMaking_2 , :ARTWORK_36_Transporting_5 , :ARTWORK_36_Transporting_3 , :ARTWORK_36_Photographing_2 , :ARTWORK_36_Packing_7 , :ARTWORK_36_PreparingForBlowing_2 .

:PierreMarieGiraud  a  :Gallery , owl:NamedIndividual ;
        rdfs:comment  "Pierre Marie Giraud is a gallery located in Brussels (Belgium)."@en ;
        rdfs:label    "Pierre Marie Giraud"@en ;
        :Located-In   :Brussels .

:ARTWORK_77_Packing  a  owl:NamedIndividual , :Packing ;
        rdfs:comment   "Instance of an activity which is part of the creation process of ARTWORK_77."@en ;
        rdfs:label     "ARTWORK_77_Packing"@en ;
        :Followed-By   :ARTWORK_77_Transporting ;
        :Follows       :ARTWORK_77_Cooling ;
        :Has-Duration  <http://www.semanticweb.org/ontologies/Daan/2020/BarbaraNanning#2018> ;
        :Involves      :AlešZvěřina , :BarbaraNanning ;
        :Located-In    :CzechRepublic ;
        :Part-Of       :Creation_Artwork_77 .

:Carat  a                       owl:DatatypeProperty ;
        rdfs:comment            "Carat is a measure of the purity of gold." ;
        rdfs:domain             :Gold_Leaf ;
        rdfs:label              "Carat"@en ;
        rdfs:range              owl:real ;
        owl:equivalentProperty  <http://www.wikidata.org/entity/Q1072404> .

:Image_Artwork_74  a            :Digital_Image , owl:NamedIndividual ;
        rdfs:comment            "Image of an artwork by Barbara Nanning displayed in \"Barbara Nanning Eeuwige Beweging\" by Eliens (2019)."@en ;
        rdfs:label              "Image_Artwork_74"@en ;
        :Representation-Source  "Tom Haartsen_Ouderkerk a/d Amstel (NL)"@en ;
        :Shows                  :Artwork_74 .

:Flat_Fusing_Finished_Artwork
        a                owl:Class ;
        rdfs:comment     "After layering coloured pieces of flat glass, the object is placed in a kiln to be melted together creating the final artwork."@en ;
        rdfs:label       "Flat Fusing Finished Artwork"@en ;
        rdfs:subClassOf  :Activity .

<http://www.cidoc-crm.org/cidoc-crm/E39_Actor>
        a                    owl:Class ;
        owl:equivalentClass  :Actor .

:ARTWORK_80_ApplyingExtraColour
        a                 owl:NamedIndividual , :Applying_Extra_Colour ;
        rdfs:comment      "Instance of an activity which is part of the creation process of ARTWORK_80."@en ;
        rdfs:label        "ARTWORK_80_Applying Extra Colour"@en ;
        :Followed-By      :ARTWORK_80_HeatingMetalMold ;
        :Follows          :ARTWORK_80_ApplyingClearGlassBell ;
        :Has-Duration     <http://www.semanticweb.org/ontologies/Daan/2020/BarbaraNanning#2018> ;
        :Involves         :BarbaraNanning , <http://www.semanticweb.org/ontologies/Daan/2020/BarbaraNanning#RadekKoten(CZ)> , <http://www.semanticweb.org/ontologies/Daan/2020/BarbaraNanning#LukasHavlas(CZ)> ;
        :Located-In       :CzechRepublic ;
        :Part-Of          :Creation_Artwork_80 ;
        :Processes        <http://www.semanticweb.org/ontologies/Daan/2020/BarbaraNanning#ReichenbachColourRodsGlass(DE)> ;
        :Requires-Use-Of  :Water , :StraightShears , :Tagliol , :AnnealingKiln , :BlowingPipe , :Blocks , :Paper , :Fork , :CeramicPotFilledWithGlass , :Pincet , :Furnace , :IcePick , :Beeswax , :GloryHole , :Garage , :YokeOfSupport , :DiamondShears , :AirCompressor , :Marver , :Pontis , :Hook , :Jacks .

<http://www.semanticweb.org/ontologies/Daan/2020/BarbaraNanning#ARTWORK_18_64_ExaminingQuality(Shape/Form)>
        a                 j.2: , owl:NamedIndividual ;
        rdfs:comment      "Instance of an activity which is part of the creation process of ARTWORK_18_64."@en ;
        rdfs:label        "ARTWORK_18_64_Examining Quality (Shape/Form)"@en ;
        :Followed-By      :ARTWORK_18_64_Cooling ;
        :Follows          :ARTWORK_18_64_Modeling ;
        :Has-Duration     <http://www.semanticweb.org/ontologies/Daan/2020/BarbaraNanning#2015> ;
        :Involves         :DurkValkema , :GertBullée , :BarbaraNanning , <http://www.semanticweb.org/ontologies/Daan/2020/BarbaraNanning#MiaLerssi(DN)> ;
        :Located-In       :Zaandam ;
        :Part-Of          :Creation_Artwork_18_64 ;
        :Requires-Use-Of  :Pontis , :GloryHole , :InterchangeableMetalMoldSetup , :AirCompressor , :Gloves , :PropaneTorch , :BlowingPipe .

:ARTWORK_36_PickingUpColouredPanel
        a                 owl:NamedIndividual , :Picking_up_Coloured_Panel ;
        rdfs:comment      "Instance of an activity which is part of the creation process of ARTWORK_36."@en ;
        rdfs:label        "ARTWORK_36_Picking up Coloured Panel"@en ;
        :Followed-By      :ARTWORK_36_Sensing_3 ;
        :Follows          :ARTWORK_36_ApplyingMassivePieceOfClearGlass ;
        :Has-Duration     <http://www.semanticweb.org/ontologies/Daan/2020/BarbaraNanning#2019> ;
        :Involves         <http://www.semanticweb.org/ontologies/Daan/2020/BarbaraNanning#JessicaHomich(USA)> , :GertBullée , :BarbaraNanning , <http://www.semanticweb.org/ontologies/Daan/2020/BarbaraNanning#RobertLenner(CZ)> , <http://www.semanticweb.org/ontologies/Daan/2020/BarbaraNanning#MarekEffmert(CZ)> , <http://www.semanticweb.org/ontologies/Daan/2020/BarbaraNanning#MarekBrathko(CZ)> , <http://www.semanticweb.org/ontologies/Daan/2020/BarbaraNanning#MiaLerssi(DN)> ;
        :Located-In       :Lindava ;
        :Part-Of          :Creation_Artwork_36 ;
        :Requires-Use-Of  :StraightShears , :Hook , :Water , :Furnace , :Beeswax , :YokeOfSupport , :Blocks , :PropaneTorch , :Pontis , :BlowingPipe , :AnnealingKiln , :Tagliol , :Gloves , :Garage , :Jacks , :FusingKiln , :Fork , :Marver , :DiamondShears , :AirCompressor , :GloryHole , :Paper , :GrindingWheel .

:Has-Width  a         owl:DatatypeProperty ;
        rdfs:comment  "Has-Width is a property which connects a thing with its width in centimeters."@en ;
        rdfs:domain   :Thing ;
        rdfs:label    "Has-Width"@en ;
        rdfs:range    xsd:integer .

:ARTWORK_18_64_PickingUpColouredCanesPattern
        a                 :Picking_up_Coloured_Canes_Pattern , owl:NamedIndividual ;
        rdfs:comment      "Instance of an activity which is part of the creation process of ARTWORK_18_64."@en ;
        rdfs:label        "ARTWORK_18_64_Picking up Coloured Canes Pattern"@en ;
        :Followed-By      :ARTWORK_18_64_Glassblowing ;
        :Follows          :ARTWORK_18_64_ApplyingClearGlassBell ;
        :Has-Duration     <http://www.semanticweb.org/ontologies/Daan/2020/BarbaraNanning#2015> ;
        :Involves         <http://www.semanticweb.org/ontologies/Daan/2020/BarbaraNanning#MiaLerssi(DN)> , <http://www.semanticweb.org/ontologies/Daan/2020/BarbaraNanning#RobertLenner(CZ)> , <http://www.semanticweb.org/ontologies/Daan/2020/BarbaraNanning#MarekEffmert(CZ)> , :GertBullée , <http://www.semanticweb.org/ontologies/Daan/2020/BarbaraNanning#MarekBrathko(CZ)> , :BarbaraNanning , <http://www.semanticweb.org/ontologies/Daan/2020/BarbaraNanning#JessicaHomich(USA)> ;
        :Located-In       :Zaandam ;
        :Part-Of          :Creation_Artwork_18_64 ;
        :Requires-Use-Of  :Beeswax , :Hook , :Marver , :DiamondShears , :PropaneTorch , :FusingKiln , :Garage , :Gloves , :Paper , :AirCompressor , :Furnace , :GloryHole , :GrindingWheel , :YokeOfSupport , :AnnealingKiln , :Fork , :Water , :StraightShears , :Pontis , :Blocks , :Jacks , :BlowingPipe , :Tagliol .

:ARTWORK_79_Modeling  a   owl:NamedIndividual , :Modeling ;
        rdfs:comment      "Instance of an activity which is part of the creation process of ARTWORK_79."@en ;
        rdfs:label        "ARTWORK_79_Modeling"@en ;
        :Followed-By      <http://www.semanticweb.org/ontologies/Daan/2020/BarbaraNanning#ARTWORK_79_ExaminingQuality(Shape/Form)> ;
        :Follows          :ARTWORK_79_Sensing ;
        :Has-Duration     <http://www.semanticweb.org/ontologies/Daan/2020/BarbaraNanning#2018> ;
        :Involves         <http://www.semanticweb.org/ontologies/Daan/2020/BarbaraNanning#LukasHavlas(CZ)> , <http://www.semanticweb.org/ontologies/Daan/2020/BarbaraNanning#Tom%C3%A1%C5%A1Moravec(CZ)> , :BarbaraNanning , <http://www.semanticweb.org/ontologies/Daan/2020/BarbaraNanning#JiriMoravec(CZ)> , <http://www.semanticweb.org/ontologies/Daan/2020/BarbaraNanning#RadekKoten(CZ)> , :AssistantOfBarbara ;
        :Located-In       :CzechRepublic ;
        :Part-Of          :Creation_Artwork_79 ;
        :Requires-Use-Of  :Gloves , :PropaneTorch , :InterchangeableMetalMoldSetup , :BlowingPipe , :AirCompressor .

:Man-Made_Material  a     owl:Class ;
        rdfs:comment      "Man-made material is a material matter created by an actor."@en ;
        rdfs:label        "Man-Made Material"@en ;
        rdfs:subClassOf   :Material ;
        owl:disjointWith  :Natural_Material .

<http://www.semanticweb.org/ontologies/Daan/2020/BarbaraNanning#ARTWORK_78_ExaminingQuality(CheckForIrregularitiesInTheGlass)>
        a              j.3: , owl:NamedIndividual ;
        rdfs:comment   "Instance of an activity which is part of the creation process of ARTWORK_78."@en ;
        rdfs:label     "ARTWORK_78_Examining Quality (Check for Irregularities in the Glass)"@en ;
        :Followed-By   :ARTWORK_78_Sawing ;
        :Follows       :ARTWORK_78_Resting ;
        :Has-Duration  <http://www.semanticweb.org/ontologies/Daan/2020/BarbaraNanning#2016> ;
        :Involves      :BarbaraNanning , :AlešZvěřina ;
        :Located-In    :CzechRepublic ;
        :Part-Of       :Creation_Artwork_78 .

<http://www.semanticweb.org/ontologies/Daan/2020/BarbaraNanning#BullseyeGlassTGKJaroslavSvacha(CZ)>
        a             owl:NamedIndividual , :Glass_Studio ;
        rdfs:comment  "Bullseye glass TGK Jaroslav Svacha (CZ) is a glass studio in Czech Republic."@en ;
        rdfs:label    "Bullseye glass TGK Jaroslav Svacha (CZ)"@en ;
        :Employed     <http://www.semanticweb.org/ontologies/Daan/2020/BarbaraNanning#JaroslavSvacha(CZ)> .

:ARTWORK_43_PreparingGlass
        a                 :Preparing_Glass , owl:NamedIndividual ;
        rdfs:comment      "Instance of an activity which is part of the creation process of ARTWORK_43."@en ;
        rdfs:label        "ARTWORK_43_Preparing Glass"@en ;
        :Followed-By      :ARTWORK_43_SetupAndTestingOfTheMetalMold ;
        :Has-Duration     <http://www.semanticweb.org/ontologies/Daan/2020/BarbaraNanning#2008> ;
        :Involves         <http://www.semanticweb.org/ontologies/Daan/2020/BarbaraNanning#AlesVacek(CZ)> , :BarbaraNanning ;
        :Located-In       :CzechRepublic ;
        :Part-Of          :Creation_Artwork_43 ;
        :Requires-Use-Of  :Marver , :GloryHole , :Garage , :BlowingPipe , :Pontis ;
        :Starts           :Creation_Artwork_43 .

<http://www.wikidata.org/entity/Q11469>
        a       owl:Class .

:ARTWORK_44_Transporting_2
        a              owl:NamedIndividual , :Transporting ;
        rdfs:comment   "Instance of an activity which is part of the creation process of ARTWORK_44."@en ;
        rdfs:label     "ARTWORK_44_Transporting_2"@en ;
        :Followed-By   :ARTWORK_44_Signing ;
        :Follows       :ARTWORK_44_Packing_2 ;
        :Has-Duration  <http://www.semanticweb.org/ontologies/Daan/2020/BarbaraNanning#2018> ;
        :Involves      :BarbaraNanning , :AlešZvěřina ;
        :Located-In    :CzechRepublic ;
        :Part-Of       :Creation_Artwork_44 .

:ARTWORK_73_Transporting_3
        a              :Transporting , owl:NamedIndividual ;
        rdfs:comment   "Instance of an activity which is part of the creation process of ARTWORK_73."@en ;
        rdfs:label     "ARTWORK_73_Transporting_3"@en ;
        :Followed-By   :ARTWORK_73_Gilding ;
        :Follows       :ARTWORK_73_Packing_3 ;
        :Has-Duration  <http://www.semanticweb.org/ontologies/Daan/2020/BarbaraNanning#2018> ;
        :Involves      :AlešZvěřina , :BarbaraNanning ;
        :Located-In    :CzechRepublic ;
        :Part-Of       :Creation_Artwork_73 .

:Documenting  a          owl:Class ;
        rdfs:comment     "Documenting is an activity in which an entity is described thereby creating documentation."@en ;
        rdfs:label       "Documenting"@en ;
        rdfs:subClassOf  :Activity .

:ARTWORK_46_TransportingColouredCanes
        a              :Transporting_Coloured_Canes , owl:NamedIndividual ;
        rdfs:comment   "Instance of an activity which is part of the creation process of ARTWORK_46."@en ;
        rdfs:label     "ARTWORK_46_Transporting Coloured Canes"@en ;
        :Followed-By   :ARTWORK_46_CuttingAndPolishingColouredCanes ;
        :Follows       :ARTWORK_46_ProducingColouredCanes ;
        :Has-Duration  <http://www.semanticweb.org/ontologies/Daan/2020/BarbaraNanning#2015> ;
        :Involves      :BarbaraNanning ;
        :Located-In    :Zaandam ;
        :Part-Of       :Creation_Artwork_46 .

:ARTWORK_18_64_DecidingColourPaletteAndPatterns_2
        a              owl:NamedIndividual , :Deciding_Colour_Palette_and_Patterns ;
        rdfs:comment   "Instance of an activity which is part of the creation process of ARTWORK_18_64."@en ;
        rdfs:label     "ARTWORK_18_64_Deciding Colour Palette and Patterns_2"@en ;
        :Followed-By   :ARTWORK_18_64_TransportingMonochromeRods ;
        :Follows       :ARTWORK_18_64_CuttingAndPolishingCastedMonochromeSheetsToSmallRods ;
        :Has-Duration  <http://www.semanticweb.org/ontologies/Daan/2020/BarbaraNanning#2015> ;
        :Involves      :BarbaraNanning ;
        :Located-In    :Amsterdam ;
        :Part-Of       :Creation_Artwork_18_64 .

:ARTWORK_17_33_Grinding
        a                 :Grinding , owl:NamedIndividual ;
        rdfs:comment      "Instance of an activity which is part of the creation process of ARTWORK_17_33."@en ;
        rdfs:label        "ARTWORK_17_33_Grinding_2"@en ;
        :Followed-By      :ARTWORK_17_33_Polishing ;
        :Follows          :ARTWORK_17_33_Sensing_2 ;
        :Has-Duration     <http://www.semanticweb.org/ontologies/Daan/2020/BarbaraNanning#2017> ;
        :Involves         :RobertFlorian , :AlešZvěřina , :BarbaraNanning ;
        :Located-In       :NovyBor ;
        :Part-Of          :Creation_Artwork_17_33 ;
        :Requires-Use-Of  :GrindingWheel , :SharpeningStone .

:ARTWORK_43_ApplyingExtraColour
        a                 :Applying_Extra_Colour , owl:NamedIndividual ;
        rdfs:comment      "Instance of an activity which is part of the creation process of ARTWORK_43."@en ;
        rdfs:label        "ARTWORK_43_Applying Extra Colour"@en ;
        :Followed-By      :ARTWORK_43_HeatingMetalMold ;
        :Follows          :ARTWORK_43_ApplyingClearGlassBell ;
        :Has-Duration     <http://www.semanticweb.org/ontologies/Daan/2020/BarbaraNanning#2008> ;
        :Involves         :BarbaraNanning , <http://www.semanticweb.org/ontologies/Daan/2020/BarbaraNanning#AlesVacek(CZ)> , <http://www.semanticweb.org/ontologies/Daan/2020/BarbaraNanning#RostislavMaterka(CZ)> ;
        :Located-In       :CzechRepublic ;
        :Part-Of          :Creation_Artwork_43 ;
        :Processes        <http://www.semanticweb.org/ontologies/Daan/2020/BarbaraNanning#ReichenbachColourRodsGlass(DE)> ;
        :Requires-Use-Of  :Garage , :Pontis , :Furnace , :Marver , :DiamondShears , :Fork , :YokeOfSupport , :StraightShears , :Blocks , :AnnealingKiln , :Hook , :IcePick , :AirCompressor , :BlowingPipe , :Beeswax , :GloryHole , :Water , :Jacks , :Pincet , :Paper , :Tagliol , :CeramicPotFilledWithGlass .

:ARTWORK_17_33_Cooling
        a                 :Cooling , owl:NamedIndividual ;
        rdfs:comment      "Instance of an activity which is part of the creation process of ARTWORK_17_33."@en ;
        rdfs:label        "ARTWORK_17_33_Cooling"@en ;
        :Followed-By      :ARTWORK_17_33_Packing ;
        :Follows          <http://www.semanticweb.org/ontologies/Daan/2020/BarbaraNanning#ARTWORK_17_33_ExaminingQuality(Shape/Form)> ;
        :Has-Duration     <http://www.semanticweb.org/ontologies/Daan/2020/BarbaraNanning#2017> ;
        :Involves         :AssistantOfBarbara , :LuděkKout ;
        :Located-In       :Lindava ;
        :Part-Of          :Creation_Artwork_17_33 ;
        :Requires-Use-Of  :AnnealingKiln .

:ARTWORK_75_HeatingMetalMold
        a                 :Heating_Metal_Mold , owl:NamedIndividual ;
        rdfs:comment      "Instance of an activity which is part of the creation process of ARTWORK_75."@en ;
        rdfs:label        "ARTWORK_75_Heating Metal Mold"@en ;
        :Followed-By      :ARTWORK_75_Glassblowing ;
        :Follows          :ARTWORK_75_ApplyingExtraColour_2 ;
        :Has-Duration     <http://www.semanticweb.org/ontologies/Daan/2020/BarbaraNanning#2018> ;
        :Involves         :BarbaraNanning ;
        :Located-In       :CzechRepublic ;
        :Part-Of          :Creation_Artwork_75 ;
        :Requires-Use-Of  :InterchangeableMetalMoldSetup , :PropaneTorch , :Gloves .

:ARTWORK_36_FillingKilnsWithMetalBowl_2
        a                 owl:NamedIndividual , :Filling_Kilns_with_Metal_Bowl ;
        rdfs:comment      "Instance of an activity which is part of the creation process of ARTWORK_36."@en ;
        rdfs:label        "ARTWORK_36_Filling Kilns with Metal Bowl_2"@en ;
        :Followed-By      :ARTWORK_36_PreparingGlass_2 ;
        :Follows          :ARTWORK_36_PreparingForBlowing_2 ;
        :Has-Duration     <http://www.semanticweb.org/ontologies/Daan/2020/BarbaraNanning#2019> ;
        :Involves         :BarbaraNanning , <http://www.semanticweb.org/ontologies/Daan/2020/BarbaraNanning#JiriPacinek(CZ)> ;
        :Located-In       :Lindava ;
        :Part-Of          :Creation_Artwork_36 ;
        :Requires-Use-Of  :Garage , :Gloves , :FusingKiln .

:ARTWORK_17_33_TransportingColouredCanes
        a              :Transporting_Coloured_Canes , owl:NamedIndividual ;
        rdfs:comment   "Instance of an activity which is part of the creation process of ARTWORK_17_33."@en ;
        rdfs:label     "ARTWORK_17_33_Transporting Coloured Canes"@en ;
        :Followed-By   :ARTWORK_17_33_CuttingAndPolishingColouredCanes ;
        :Follows       :ARTWORK_17_33_ProducingColouredCanes ;
        :Has-Duration  <http://www.semanticweb.org/ontologies/Daan/2020/BarbaraNanning#2017> ;
        :Involves      :BarbaraNanning ;
        :Located-In    :NovyBor ;
        :Part-Of       :Creation_Artwork_17_33 .

:ARTWORK_76_Packing_3
        a              owl:NamedIndividual , :Packing ;
        rdfs:comment   "Instance of an activity which is part of the creation process of ARTWORK_76."@en ;
        rdfs:label     "ARTWORK_76_Packing_3"@en ;
        :Followed-By   :ARTWORK_76_Transporting_3 ;
        :Follows       :ARTWORK_76_Signing ;
        :Has-Duration  <http://www.semanticweb.org/ontologies/Daan/2020/BarbaraNanning#2018> ;
        :Involves      :AlešZvěřina , :BarbaraNanning ;
        :Located-In    :CzechRepublic ;
        :Part-Of       :Creation_Artwork_76 .

<http://vocab.getty.edu/aat/300025261>
        a                    owl:Class ;
        owl:equivalentClass  :Gilder .

:INSTACOLLTool  a     :Equipment , owl:NamedIndividual ;
        rdfs:comment  "The INSTACOLL tool is a tool with rubber tips used to get the gold leaf neatly in the corners."@en ;
        rdfs:label    "INSTACOLL Tool"@en ;
        :Made-Out-Of  :Rubber ;
        :Used-For     :ARTWORK_76_Gilding , :ARTWORK_73_Gilding , :ARTWORK_74_Gilding , :ARTWORK_75_Gilding , :ARTWORK_80_Gilding , :ARTWORK_44_Gilding , :ARTWORK_78_Gilding , :ARTWORK_43_Gilding , :ARTWORK_79_Gilding , :ARTWORK_77_Gilding .

:ARTWORK_73_Grinding  a   owl:NamedIndividual , :Grinding ;
        rdfs:comment      "Instance of an activity which is part of the creation process of ARTWORK_73."@en ;
        rdfs:label        "ARTWORK_73_Grinding"@en ;
        :Followed-By      :ARTWORK_73_Polishing ;
        :Follows          :ARTWORK_73_Sawing ;
        :Has-Duration     <http://www.semanticweb.org/ontologies/Daan/2020/BarbaraNanning#2018> ;
        :Involves         :AlešZvěřina , :RobertFlorian , :BarbaraNanning ;
        :Located-In       :CzechRepublic ;
        :Part-Of          :Creation_Artwork_73 ;
        :Requires-Use-Of  :SharpeningStone , :GrindingWheel .

<http://vocab.getty.edu/aat/300022549>
        a           owl:NamedIndividual ;
        owl:sameAs  :GildersTip .

:ARTWORK_36_Packing_4
        a              :Packing , owl:NamedIndividual ;
        rdfs:comment   "Instance of an activity which is part of the creation process of ARTWORK_36."@en ;
        rdfs:label     "ARTWORK_36_Packing_4"@en ;
        :Followed-By   :ARTWORK_36_Documenting ;
        :Follows       :ARTWORK_36_Photographing ;
        :Has-Duration  <http://www.semanticweb.org/ontologies/Daan/2020/BarbaraNanning#2019> ;
        :Involves      :BarbaraNanning ;
        :Located-In    :Amsterdam ;
        :Part-Of       :Creation_Artwork_36 .

:ARTWORK_75_Polishing
        a                 owl:NamedIndividual , :Polishing ;
        rdfs:comment      "Instance of an activity which is part of the creation process of ARTWORK_75."@en ;
        rdfs:label        "ARTWORK_75_Polishing"@en ;
        :Followed-By      <http://www.semanticweb.org/ontologies/Daan/2020/BarbaraNanning#ARTWORK_75_ExaminingQuality(Result)> ;
        :Follows          :ARTWORK_75_Grinding ;
        :Has-Duration     <http://www.semanticweb.org/ontologies/Daan/2020/BarbaraNanning#2018> ;
        :Involves         :BarbaraNanning , :AlešZvěřina , :LukášSvoboda ;
        :Located-In       :CzechRepublic ;
        :Part-Of          :Creation_Artwork_75 ;
        :Requires-Use-Of  :PolishingStone .

:ARTWORK_17_33_Resting
        a                 owl:NamedIndividual , :Resting ;
        rdfs:comment      "Instance of an activity which is part of the creation process of ARTWORK_17_33."@en ;
        rdfs:label        "ARTWORK_17_33_Resting"@en ;
        :Followed-By      <http://www.semanticweb.org/ontologies/Daan/2020/BarbaraNanning#ARTWORK_17_33_ExaminingQuality(CheckForIrregularitiesInTheGlass)> ;
        :Follows          :ARTWORK_17_33_Transporting ;
        :Has-Duration     <http://www.semanticweb.org/ontologies/Daan/2020/BarbaraNanning#2017> ;
        :Involves         :AlešZvěřina ;
        :Located-In       :NovyBor ;
        :Part-Of          :Creation_Artwork_17_33 ;
        :Requires-Use-Of  :AnnealingKiln .

:AJETOAlexandriteGlass
        a                     owl:NamedIndividual , :AJETO_Glass ;
        rdfs:comment          "AJETO Alexandrite glass is a chemically created material which changes colour based on various lighting conditions (e.g. Artificial light)."@en ;
        rdfs:label            "AJETO Alexandrite Glass"@en ;
        :Availability         "Orderable"@en ;
        :Is-Processed-During  :ARTWORK_44_ApplyingExtraColour_2 , :ARTWORK_76_ApplyingExtraColour_2 , :ARTWORK_75_ApplyingExtraColour_2 ;
        :Is-Processed-In      :Artwork_76 , :Artwork_75 , :Artwork_44 ;
        :Made-By              :LASVITAJETO ;
        :Transparency         "Transparent"@en .

:Museum  a                   owl:Class ;
        rdfs:comment         "A museum is an organisation which stores and exhibits cultural heritage objects."@en ;
        rdfs:label           "Museum"@en ;
        rdfs:subClassOf      :Organisation ;
        owl:equivalentClass  <http://www.wikidata.org/entity/Q33506> .

:ARTWORK_39_DecidingColourPalette
        a                 owl:NamedIndividual , :Deciding_Colour_Palette ;
        rdfs:comment      "Instance of an activity which is part of the creation process of ARTWORK_39."@en ;
        rdfs:label        "ARTWORK_39_Deciding Colour Palette"@en ;
        :Followed-By      :ARTWORK_39_OrdeningMonochromeSheetsAndStrings ;
        :Has-Duration     <http://www.semanticweb.org/ontologies/Daan/2020/BarbaraNanning#2015> ;
        :Involves         :BarbaraNanning ;
        :Located-In       :Amsterdam ;
        :Part-Of          :Creation_Artwork_39 ;
        :Processes        :BullseyeGlass ;
        :Requires-Use-Of  :Computer ;
        :Starts           :Creation_Artwork_39 .

:ARTWORK_18_64_PreparingGlass
        a                 :Preparing_Glass , owl:NamedIndividual ;
        rdfs:comment      "Instance of an activity which is part of the creation process of ARTWORK_18_64."@en ;
        rdfs:label        "ARTWORK_18_64_Preparing Glass"@en ;
        :Followed-By      :ARTWORK_18_64_PreparingForBlowing ;
        :Follows          :ARTWORK_18_64_FillingKilnsWithMetalBowl ;
        :Has-Duration     <http://www.semanticweb.org/ontologies/Daan/2020/BarbaraNanning#2015> ;
        :Involves         <http://www.semanticweb.org/ontologies/Daan/2020/BarbaraNanning#MiaLerssi(DN)> , :GertBullée , :BarbaraNanning ;
        :Located-In       :Lindava ;
        :Part-Of          :Creation_Artwork_18_64 ;
        :Requires-Use-Of  :Marver , :BlowingPipe , :GloryHole , :Pontis , :Garage .

:ARTWORK_76_Packing  a  owl:NamedIndividual , :Packing ;
        rdfs:comment   "Instance of an activity which is part of the creation process of ARTWORK_76."@en ;
        rdfs:label     "ARTWORK_76_Packing"@en ;
        :Followed-By   :ARTWORK_76_Transporting ;
        :Follows       :ARTWORK_76_Cooling ;
        :Has-Duration  <http://www.semanticweb.org/ontologies/Daan/2020/BarbaraNanning#2018> ;
        :Involves      :BarbaraNanning , :AlešZvěřina ;
        :Located-In    :CzechRepublic ;
        :Part-Of       :Creation_Artwork_76 .

:Artwork_74  a        owl:NamedIndividual , :Glass_Artwork ;
        rdfs:comment  "Artwork by Barbara Nanning displayed in \"Barbara Nanning Eeuwige Beweging\" by Eliens (2019)."@en ;
        rdfs:label    "Verre églomisé"@en ;
        :Created-By   :Creation_Artwork_74 ;
        :Has-Depth    "37"^^xsd:decimal ;
        :Has-Height   "20"^^xsd:decimal ;
        :Has-Width    "18"^^xsd:decimal ;
        :Is-Unica     "Yes"@en ;
        :Located-In   :Lausanne ;
        :Made-By      :VáçlavNovák_Doksy_CzechRepublic , <http://www.semanticweb.org/ontologies/Daan/2020/BarbaraNanning#Ale%C5%A1Zv%C4%9B%C5%99ina&AZ-Design> , :BarbaraNanning , :LASVITAJETO ;
        :Made-Out-Of  :LouvreGoldLeaf , :AJETOAmberGlass , :AJETOClearGlass , :AJETORedGlass ;
        :Part-Of      <http://www.semanticweb.org/ontologies/Daan/2020/BarbaraNanning#CollectionMuseeDeDesignEtd'artsAppliquesContemporains> ;
        :Shown-By     :Image_Artwork_74 .

<http://www.semanticweb.org/ontologies/Daan/2020/BarbaraNanning#ARTWORK_76_ExaminingQuality(FinalResult)>
        a              owl:NamedIndividual , j.1: ;
        rdfs:comment   "Instance of an activity which is part of the creation process of ARTWORK_76."@en ;
        rdfs:label     "ARTWORK_76_Examining Quality (Final Result)"@en ;
        :Followed-By   :ARTWORK_76_Packing_5 ;
        :Follows       :ARTWORK_76_Gilding ;
        :Has-Duration  <http://www.semanticweb.org/ontologies/Daan/2020/BarbaraNanning#2018> ;
        :Involves      :AlešZvěřina , :BarbaraNanning ;
        :Located-In    :CzechRepublic ;
        :Part-Of       :Creation_Artwork_76 .

:ARTWORK_73_SetupAndTestingOfTheMetalMold_2
        a                 owl:NamedIndividual , :Setup_and_Testing_of_the_Metal_Mold ;
        rdfs:comment      "Instance of an activity which is part of the creation process of ARTWORK_73."@en ;
        rdfs:label        "ARTWORK_73_Setup and Testing of the Metal Mold_2"@en ;
        :Followed-By      :ARTWORK_73_ApplyingClearGlassBell ;
        :Follows          :ARTWORK_73_SetupAndTestingOfTheMetalMold ;
        :Has-Duration     <http://www.semanticweb.org/ontologies/Daan/2020/BarbaraNanning#2018> ;
        :Involves         <http://www.semanticweb.org/ontologies/Daan/2020/BarbaraNanning#JiriMoravec(CZ)> , <http://www.semanticweb.org/ontologies/Daan/2020/BarbaraNanning#LukasHavlas(CZ)> , :AssistantOfBarbara , <http://www.semanticweb.org/ontologies/Daan/2020/BarbaraNanning#Tom%C3%A1%C5%A1Moravec(CZ)> , <http://www.semanticweb.org/ontologies/Daan/2020/BarbaraNanning#RadekKoten(CZ)> , :BarbaraNanning ;
        :Located-In       :CzechRepublic ;
        :Part-Of          :Creation_Artwork_73 ;
        :Requires-Use-Of  :InterchangeableMetalMoldSetup .

:ARTWORK_78_Sensing  a  :Sensing , owl:NamedIndividual ;
        rdfs:comment   "Instance of an activity which is part of the creation process of ARTWORK_78."@en ;
        rdfs:label     "ARTWORK_78_Sensing"@en ;
        :Followed-By   :ARTWORK_78_Modeling ;
        :Follows       :ARTWORK_78_Glassblowing ;
        :Has-Duration  <http://www.semanticweb.org/ontologies/Daan/2020/BarbaraNanning#2008> ;
        :Involves      :LukášSvoboda , :BarbaraNanning , :AlešZvěřina ;
        :Located-In    :CzechRepublic ;
        :Part-Of       :Creation_Artwork_78 .

:ARTWORK_80_ExaminingTheQualityOfTheGlass
        a                 :Examining_the_Quality_of_the_Glass , owl:NamedIndividual ;
        rdfs:comment      "Instance of an activity which is part of the creation process of ARTWORK_80."@en ;
        rdfs:label        "ARTWORK_80_Examining the Quality of the Glass"@en ;
        :Followed-By      :ARTWORK_80_Cooling ;
        :Follows          :ARTWORK_80_Modeling ;
        :Has-Duration     <http://www.semanticweb.org/ontologies/Daan/2020/BarbaraNanning#2018> ;
        :Involves         :BarbaraNanning , :LuděkKout , <http://www.semanticweb.org/ontologies/Daan/2020/BarbaraNanning#RadekKoten(CZ)> ;
        :Located-In       :CzechRepublic ;
        :Part-Of          :Creation_Artwork_80 ;
        :Requires-Use-Of  :Water , :Blocks , :Pontis , :AnnealingKiln , :BlowingPipe , :DiamondShears , :CeramicPotFilledWithGlass , :Jacks , :StraightShears , :YokeOfSupport , :GloryHole , :Paper , :Furnace .

:ARTWORK_79_SetupAndTestingOfTheMetalMold
        a                 :Setup_and_Testing_of_the_Metal_Mold , owl:NamedIndividual ;
        rdfs:comment      "Instance of an activity which is part of the creation process of ARTWORK_79."@en ;
        rdfs:label        "ARTWORK_79_Setup and Testing of the Metal Mold"@en ;
        :Followed-By      :ARTWORK_79_ExaminingTheQualityOfTheGlass ;
        :Follows          :ARTWORK_79_PreparingGlass ;
        :Has-Duration     <http://www.semanticweb.org/ontologies/Daan/2020/BarbaraNanning#2018> ;
        :Involves         :BarbaraNanning , <http://www.semanticweb.org/ontologies/Daan/2020/BarbaraNanning#JiriMoravec(CZ)> , <http://www.semanticweb.org/ontologies/Daan/2020/BarbaraNanning#LukasHavlas(CZ)> , :AssistantOfBarbara , <http://www.semanticweb.org/ontologies/Daan/2020/BarbaraNanning#Tom%C3%A1%C5%A1Moravec(CZ)> , <http://www.semanticweb.org/ontologies/Daan/2020/BarbaraNanning#RadekKoten(CZ)> ;
        :Located-In       :CzechRepublic ;
        :Part-Of          :Creation_Artwork_79 ;
        :Requires-Use-Of  :InterchangeableMetalMoldSetup .

:Ordening_Monochrome_Sheets_and_Strings
        a                owl:Class ;
        rdfs:comment     "Flat glass that can be cut into various shapes to create a specific design."@en ;
        rdfs:label       "Ordening Monochrome Sheets and Strings"@en ;
        rdfs:subClassOf  :Ordening .

<http://www.semanticweb.org/ontologies/Daan/2020/BarbaraNanning#Tom%C3%A1%C5%A1Moravec(CZ)>
        a             owl:NamedIndividual , :Third_Glass_Blower ;
        rdfs:comment  "Tomáš Moravec (CZ) is a Third Glass Blower."@en ;
        rdfs:label    "Tomáš Moravec (CZ)"@en ;
        :Involved-In  :ARTWORK_75_SetupAndTestingOfTheMetalMold_2 , :ARTWORK_76_SetupAndTestingOfTheMetalMold , :ARTWORK_75_Modeling , :ARTWORK_76_Modeling , :ARTWORK_76_SetupAndTestingOfTheMetalMold_2 , :ARTWORK_80_Glassblowing , :ARTWORK_77_SetupAndTestingOfTheMetalMold_2 , :ARTWORK_77_SetupAndTestingOfTheMetalMold , :ARTWORK_44_Modeling , :ARTWORK_75_Glassblowing , :ARTWORK_44_Glassblowing , :ARTWORK_44_SetupAndTestingOfTheMetalMold_2 , :ARTWORK_73_Modeling , :ARTWORK_79_Glassblowing , :ARTWORK_73_Glassblowing , :ARTWORK_79_Modeling , :ARTWORK_80_SetupAndTestingOfTheMetalMold_2 , :ARTWORK_79_SetupAndTestingOfTheMetalMold_2 , :ARTWORK_73_SetupAndTestingOfTheMetalMold , :ARTWORK_76_Glassblowing , :ARTWORK_44_SetupAndTestingOfTheMetalMold , :ARTWORK_75_SetupAndTestingOfTheMetalMold , :ARTWORK_77_Glassblowing , :ARTWORK_79_SetupAndTestingOfTheMetalMold , :ARTWORK_77_Modeling , :ARTWORK_80_SetupAndTestingOfTheMetalMold , :ARTWORK_73_SetupAndTestingOfTheMetalMold_2 , :ARTWORK_80_Modeling ;
        :Works-For    :LASVITAJETO .

:Measuring_and_Boxes_Making
        a                owl:Class ;
        rdfs:comment     "Measuring and Boxes Making is an activity in which an object is measured and a box is created for the object."@en ;
        rdfs:label       "Measuring and Boxes Making"@en ;
        rdfs:subClassOf  :Activity .

<http://www.semanticweb.org/ontologies/Daan/2020/BarbaraNanning#ARTWORK_36_ExaminingQuality(Shape/Form)_2>
        a                 j.2: , owl:NamedIndividual ;
        rdfs:comment      "Instance of an activity which is part of the creation process of ARTWORK_36."@en ;
        rdfs:label        "ARTWORK_36_Examining Quality (Shape/Form)_2"@en ;
        :Followed-By      :ARTWORK_36_Cooling_2 ;
        :Follows          :ARTWORK_36_Modeling_2 ;
        :Has-Duration     <http://www.semanticweb.org/ontologies/Daan/2020/BarbaraNanning#2019> ;
        :Involves         <http://www.semanticweb.org/ontologies/Daan/2020/BarbaraNanning#JessicaHomich(USA)> , :BarbaraNanning , <http://www.semanticweb.org/ontologies/Daan/2020/BarbaraNanning#JiriPacinek(CZ)> ;
        :Located-In       :Lindava ;
        :Part-Of          :Creation_Artwork_36 ;
        :Requires-Use-Of  :GloryHole , :Gloves , :BlowingPipe , :Pontis , :InterchangeableMetalMoldSetup , :PropaneTorch , :AirCompressor .

:SteefHendriks  a     :Grinder_1 , owl:NamedIndividual ;
        rdfs:comment  "Steef Hendriks is a Grinder 1."@en ;
        rdfs:label    "Steef Hendriks"@en ;
        :Involved-In  :ARTWORK_36_CuttingMonochromeSheets , :ARTWORK_46_CuttingMonochromeSheets , :ARTWORK_46_Casting , :ARTWORK_36_Casting , :ARTWORK_18_64_Casting , :ARTWORK_18_64_CuttingMonochromeSheets ;
        :Works-For    :BullseyeGlassSplinterEnDeVosch .

:ARTWORK_76_Transporting
        a              :Transporting , owl:NamedIndividual ;
        rdfs:comment   "Instance of an activity which is part of the creation process of ARTWORK_76."@en ;
        rdfs:label     "ARTWORK_76_Transporting"@en ;
        :Followed-By   :ARTWORK_76_Resting ;
        :Follows       :ARTWORK_76_Packing ;
        :Has-Duration  <http://www.semanticweb.org/ontologies/Daan/2020/BarbaraNanning#2018> ;
        :Involves      :AlešZvěřina , :BarbaraNanning ;
        :Located-In    :CzechRepublic ;
        :Part-Of       :Creation_Artwork_76 .

:BitIron  a           :Tool , owl:NamedIndividual ;
        rdfs:comment  "A bit iron is a tool made out of iron used to alter glass."@en ;
        rdfs:label    "Bit Iron"@en ;
        :Made-Out-Of  :Iron ;
        :Used-For     :ARTWORK_78_Glassblowing , :ARTWORK_77_Glassblowing , :ARTWORK_74_Glassblowing , :ARTWORK_75_Glassblowing , :ARTWORK_79_Glassblowing , :ARTWORK_80_Glassblowing , :ARTWORK_43_Glassblowing , :ARTWORK_44_Glassblowing , :ARTWORK_73_Glassblowing , :ARTWORK_76_Glassblowing .

:ARTWORK_74_ApplyingClearGlassBell
        a                 :Applying_Clear_Glass_Bell , owl:NamedIndividual ;
        rdfs:comment      "Instance of an activity which is part of the creation process of ARTWORK_74."@en ;
        rdfs:label        "ARTWORK_74_Applying Clear Glass Bell"@en ;
        :Followed-By      :ARTWORK_74_ApplyingExtraColour ;
        :Follows          :ARTWORK_74_SetupAndTestingOfTheMetalMold_2 ;
        :Has-Duration     <http://www.semanticweb.org/ontologies/Daan/2020/BarbaraNanning#2008> ;
        :Involves         <http://www.semanticweb.org/ontologies/Daan/2020/BarbaraNanning#RostislavMaterka(CZ)> , :BarbaraNanning , <http://www.semanticweb.org/ontologies/Daan/2020/BarbaraNanning#AlesVacek(CZ)> ;
        :Located-In       :CzechRepublic ;
        :Part-Of          :Creation_Artwork_74 ;
        :Processes        :AJETOClearGlass ;
        :Requires-Use-Of  :BlowingPipe , :Beeswax , :Pincet , :YokeOfSupport , :StraightShears , :AirCompressor , :Blocks , :Marver , :Paper , :Jacks , :IcePick , :DiamondShears , :CeramicPotFilledWithGlass , :Water , :Hook , :Furnace .

<http://www.semanticweb.org/ontologies/Daan/2020/BarbaraNanning#ARTWORK_76_ExaminingQuality(CheckForIrregularitiesInTheGlass)>
        a              owl:NamedIndividual , j.3: ;
        rdfs:comment   "Instance of an activity which is part of the creation process of ARTWORK_76."@en ;
        rdfs:label     "ARTWORK_76_Examining Quality (Check for Irregularities in the Glass)"@en ;
        :Followed-By   :ARTWORK_76_Sawing ;
        :Follows       :ARTWORK_76_Resting ;
        :Has-Duration  <http://www.semanticweb.org/ontologies/Daan/2020/BarbaraNanning#2018> ;
        :Involves      :AlešZvěřina , :BarbaraNanning ;
        :Located-In    :CzechRepublic ;
        :Part-Of       :Creation_Artwork_76 .

:Third_Glass_Blower  a   owl:Class ;
        rdfs:comment     "The third glass blower is the fourth highest role within a glass blowing team. While normal glass blowing teams consist of 4 people, Nanning required extra workforces."@en ;
        rdfs:label       "Third Glass Blower"@en ;
        rdfs:subClassOf  :Glass_Blower .

:AJETOAmberGlass  a           :AJETO_Glass , owl:NamedIndividual ;
        rdfs:comment          "AJETO Amber is a form of AJETO glass with a amber colour."@en ;
        rdfs:label            "AJETO Amber Glass"@en ;
        :Availability         "Available"@en ;
        :Is-Processed-During  :ARTWORK_74_ApplyingExtraColour_2 ;
        :Is-Processed-In      :Artwork_74 ;
        :Made-By              :LASVITAJETO ;
        :Made-Out-Of          :Calcium , :Sand , :Potassium , :Soda ;
        :Transparency         "Transparent"@en .

:Transporting_Metal_Bowl_with_Canes_and_Strings
        a                owl:Class ;
        rdfs:comment     "Moving said objects from one place to another"@en ;
        rdfs:label       "Transporting Metal Bowl with Canes and Strings"@en ;
        rdfs:subClassOf  :Transporting .

:ARTWORK_39_FusingSheetsAndStrings
        a                 owl:NamedIndividual , :Fusing_Sheets_and_Strings ;
        rdfs:comment      "Instance of an activity which is part of the creation process of ARTWORK_39."@en ;
        rdfs:label        "ARTWORK_39_Fusing Sheets and Strings"@en ;
        :Followed-By      :ARTWORK_39_Slumping ;
        :Follows          :ARTWORK_39_ComposingColouredPatternsWithSheetsAndStrings ;
        :Has-Duration     <http://www.semanticweb.org/ontologies/Daan/2020/BarbaraNanning#2015> ;
        :Involves         :BarbaraNanning ;
        :Located-In       :Amsterdam ;
        :Part-Of          :Creation_Artwork_39 ;
        :Requires-Use-Of  :FusingKiln .

<http://www.cidoc-crm.org/cidoc-crm/P14_performed>
        a                       owl:ObjectProperty ;
        owl:equivalentProperty  :Involved-In .

:Creation_Artwork_39  a  :Creation_Event , owl:NamedIndividual ;
        rdfs:comment    "Creation event for Artwork_39 by Barbara Nanning."@en ;
        rdfs:label      "Creation_Artwork_39"@en ;
        :Consists-Of    :ARTWORK_39_HeatingMetalMold , :ARTWORK_39_Glassblowing , :ARTWORK_39_ComposingColouredPatternsWithSheetsAndStrings , :ARTWORK_39_DecidingColourPalette , :ARTWORK_39_Transporting_2 , :ARTWORK_39_TransportingMetalBowlWithPanel , :ARTWORK_39_Resting , :ARTWORK_39_FillingKilnsWithMetalBowl , :ARTWORK_39_OrdeningMonochromeSheetsAndStrings , :ARTWORK_39_Packing_2 , :ARTWORK_39_ApplyingClearGlassBell , :ARTWORK_39_Packing , :ARTWORK_39_CuttingStrings , :ARTWORK_39_Documenting , :ARTWORK_39_ExaminingTheQualityOfTheGlass , <http://www.semanticweb.org/ontologies/Daan/2020/BarbaraNanning#ARTWORK_39_ExaminingQuality(CheckForIrregularitiesInTheGlass)> , :ARTWORK_39_SetupAndTestingOfTheMetalMold , :ARTWORK_39_Sensing , :ARTWORK_39_Modeling , <http://www.semanticweb.org/ontologies/Daan/2020/BarbaraNanning#ARTWORK_39_ExaminingQuality(Shape/Form)> , :ARTWORK_39_CuttingSheets , <http://www.semanticweb.org/ontologies/Daan/2020/BarbaraNanning#ARTWORK_39_ExaminingQuality(FinalResult)> , :ARTWORK_39_Sawing , :ARTWORK_39_Grinding , :ARTWORK_39_Slumping , :ARTWORK_39_Sandblasting , :ARTWORK_39_Polishing , :ARTWORK_39_Signing , :ARTWORK_39_Packing_3 , :ARTWORK_39_PreparingGlass , :ARTWORK_39_Sensing_2 , :ARTWORK_39_Cooling , :ARTWORK_39_FusingSheetsAndStrings , :ARTWORK_39_PickingUpColouredPanel , :ARTWORK_39_Photographing , :ARTWORK_39_Transporting , :ARTWORK_39_PreparingForBlowing ;
        :Created        :Artwork_39 ;
        :Finishes-With  :ARTWORK_39_Documenting ;
        :Has-Duration   <http://www.semanticweb.org/ontologies/Daan/2020/BarbaraNanning#2015> .

:ARTWORK_18_64_Polishing
        a                 :Polishing , owl:NamedIndividual ;
        rdfs:comment      "Instance of an activity which is part of the creation process of ARTWORK_18_64."@en ;
        rdfs:label        "ARTWORK_18_64_Polishing"@en ;
        :Followed-By      :ARTWORK_18_64_Sandblasting ;
        :Has-Duration     <http://www.semanticweb.org/ontologies/Daan/2020/BarbaraNanning#2015> ;
        :Involves         :LukášSvoboda , :BarbaraNanning , :AlešZvěřina ;
        :Located-In       :NovyBor ;
        :Part-Of          :Creation_Artwork_18_64 ;
        :Requires-Use-Of  :PolishingStone .

:ARTWORK_46_TransportingMetalBowlWithCanesAndStrings
        a              :Transporting_Metal_Bowl_with_Canes_and_Strings , owl:NamedIndividual ;
        rdfs:comment   "Instance of an activity which is part of the creation process of ARTWORK_46."@en ;
        rdfs:label     "ARTWORK_46_Transporting Metal Bowl with Canes and Strings"@en ;
        :Followed-By   :ARTWORK_46_PreparingForBlowing ;
        :Follows       :ARTWORK_46_TackfusingColouredCanesAndStrings ;
        :Has-Duration  <http://www.semanticweb.org/ontologies/Daan/2020/BarbaraNanning#2018> ;
        :Involves      :BarbaraNanning ;
        :Located-In    :Lindava ;
        :Part-Of       :Creation_Artwork_46 .

:ARTWORK_36_Peacock  a        owl:NamedIndividual ;
        rdfs:comment          "ARTWORK_36_Peacock is a glass artwork used as a Man-Made material by Barbara Nanning."@en ;
        rdfs:label            "ARTWORK_36_Peacock"@en ;
        :Is-Processed-During  :ARTWORK_36_FlatFusingFinishedArtwork ;
        :Is-Processed-In      :Artwork_36 .

:ARTWORK_43_Translocating
        a                 :Translocating , owl:NamedIndividual ;
        rdfs:comment      "Instance of an activity which is part of the creation process of ARTWORK_43."@en ;
        rdfs:label        "ARTWORK_43_Translocating"@en ;
        :Followed-By      :ARTWORK_43_Cooling ;
        :Follows          <http://www.semanticweb.org/ontologies/Daan/2020/BarbaraNanning#ARTWORK_43_ExaminingQuality(Shape/Form)> ;
        :Has-Duration     <http://www.semanticweb.org/ontologies/Daan/2020/BarbaraNanning#2008> ;
        :Involves         :BarbaraNanning ;
        :Located-In       :CzechRepublic ;
        :Part-Of          :Creation_Artwork_43 ;
        :Requires-Use-Of  :Fork .

<http://www.wikidata.org/entity/Q3329765>
        a       owl:NamedIndividual .

:ARTWORK_17_33_ApplyingClearGlassBell
        a                 :Applying_Clear_Glass_Bell , owl:NamedIndividual ;
        rdfs:comment      "Instance of an activity which is part of the creation process of ARTWORK_17_33."@en ;
        rdfs:label        "ARTWORK_17_33_Applying Clear Glass Bell"@en ;
        :Followed-By      :ARTWORK_17_33_PickingUpColouredCanesPattern ;
        :Follows          :ARTWORK_17_33_ExaminingTheQualityOfTheGlass ;
        :Has-Duration     <http://www.semanticweb.org/ontologies/Daan/2020/BarbaraNanning#2017> ;
        :Involves         <http://www.semanticweb.org/ontologies/Daan/2020/BarbaraNanning#LukasHavlas(CZ)> , :BarbaraNanning , <http://www.semanticweb.org/ontologies/Daan/2020/BarbaraNanning#RadekKoten(CZ)> ;
        :Located-In       :Lindava ;
        :Part-Of          :Creation_Artwork_17_33 ;
        :Requires-Use-Of  :Blocks , :Paper , :Hook , :IcePick , :StraightShears , :BlowingPipe , :AirCompressor , :DiamondShears , :Marver , :Water , :Furnace , :YokeOfSupport , :Beeswax , :CeramicPotFilledWithGlass , :Jacks , :Pincet .

:Person  a               owl:Class ;
        rdfs:comment     "A person is an individual human being."@en ;
        rdfs:label       "Person"@en ;
        rdfs:subClassOf  :Actor .

:ARTWORK_43_Transporting_2
        a              owl:NamedIndividual , :Transporting ;
        rdfs:comment   "Instance of an activity which is part of the creation process of ARTWORK_43."@en ;
        rdfs:label     "ARTWORK_43_Transporting_2"@en ;
        :Followed-By   :ARTWORK_43_Sandblasting ;
        :Follows       :ARTWORK_43_Packing_2 ;
        :Has-Duration  <http://www.semanticweb.org/ontologies/Daan/2020/BarbaraNanning#2008> ;
        :Involves      :BarbaraNanning , :AlešZvěřina ;
        :Located-In    :CzechRepublic ;
        :Part-Of       :Creation_Artwork_43 .

:ARTWORK_75_ExaminingTheQualityOfTheGlass
        a                 :Examining_the_Quality_of_the_Glass , owl:NamedIndividual ;
        rdfs:comment      "Instance of an activity which is part of the creation process of ARTWORK_75."@en ;
        rdfs:label        "ARTWORK_75_Examining the Quality of the Glass"@en ;
        :Followed-By      :ARTWORK_75_Cooling ;
        :Follows          :ARTWORK_75_Modeling ;
        :Has-Duration     <http://www.semanticweb.org/ontologies/Daan/2020/BarbaraNanning#2017> ;
        :Involves         :BarbaraNanning , <http://www.semanticweb.org/ontologies/Daan/2020/BarbaraNanning#RadekKoten(CZ)> , :LuděkKout ;
        :Located-In       :CzechRepublic ;
        :Part-Of          :Creation_Artwork_75 ;
        :Requires-Use-Of  :AnnealingKiln , :Water , :StraightShears , :BlowingPipe , :DiamondShears , :CeramicPotFilledWithGlass , :Jacks , :Blocks , :GloryHole , :Pontis , :Paper , :Furnace , :YokeOfSupport .

:Cooling  a              owl:Class ;
        rdfs:comment     "Cooling is an activity is which the temperature of a thing is decreased. The timing of the cooling is crucial."@en ;
        rdfs:label       "Cooling"@en ;
        rdfs:subClassOf  :Activity .

:ARTWORK_80_Polishing
        a                 :Polishing , owl:NamedIndividual ;
        rdfs:comment      "Instance of an activity which is part of the creation process of ARTWORK_80."@en ;
        rdfs:label        "ARTWORK_80_Polishing"@en ;
        :Followed-By      <http://www.semanticweb.org/ontologies/Daan/2020/BarbaraNanning#ARTWORK_80_ExaminingQuality(Result)> ;
        :Follows          :ARTWORK_80_Grinding ;
        :Has-Duration     <http://www.semanticweb.org/ontologies/Daan/2020/BarbaraNanning#2018> ;
        :Involves         :LukášSvoboda , :BarbaraNanning , :AlešZvěřina ;
        :Located-In       :CzechRepublic ;
        :Part-Of          :Creation_Artwork_80 ;
        :Requires-Use-Of  :PolishingStone .

:ARTWORK_75_Transporting
        a              :Transporting , owl:NamedIndividual ;
        rdfs:comment   "Instance of an activity which is part of the creation process of ARTWORK_75."@en ;
        rdfs:label     "ARTWORK_75_Transporting"@en ;
        :Followed-By   :ARTWORK_75_Resting ;
        :Follows       :ARTWORK_75_Packing ;
        :Has-Duration  <http://www.semanticweb.org/ontologies/Daan/2020/BarbaraNanning#2018> ;
        :Involves      :BarbaraNanning , :AlešZvěřina ;
        :Located-In    :CzechRepublic ;
        :Part-Of       :Creation_Artwork_75 .

:BitIrons  a    owl:NamedIndividual .

:ARTWORK_79_Packing_5
        a              owl:NamedIndividual , :Packing ;
        rdfs:comment   "Instance of an activity which is part of the creation process of ARTWORK_79."@en ;
        rdfs:label     "ARTWORK_79_Packing_5"@en ;
        :Finishes      :Creation_Artwork_79 ;
        :Follows       :ARTWORK_79_Documenting ;
        :Has-Duration  <http://www.semanticweb.org/ontologies/Daan/2020/BarbaraNanning#2018> ;
        :Involves      :BarbaraNanning ;
        :Located-In    :CzechRepublic ;
        :Part-Of       :Creation_Artwork_79 .

:ARTWORK_46_CuttingAndPolishingColouredCanes
        a                 owl:NamedIndividual , :Cutting_and_Polishing_Coloured_Canes ;
        rdfs:comment      "Instance of an activity which is part of the creation process of ARTWORK_46."@en ;
        rdfs:label        "ARTWORK_46_Cutting and Polishing Coloured Canes"@en ;
        :Followed-By      :ARTWORK_46_TransportingColouredCanes_2 ;
        :Follows          :ARTWORK_46_TransportingColouredCanes ;
        :Has-Duration     <http://www.semanticweb.org/ontologies/Daan/2020/BarbaraNanning#2015> ;
        :Involves         :RobertFlorian , :BarbaraNanning , :AlešZvěřina ;
        :Located-In       :NovyBor ;
        :Part-Of          :Creation_Artwork_46 ;
        :Requires-Use-Of  :DiamondSaw , :Water , :Glassscissors , :SharpeningStone .

:ARTWORK_18_64_Sandblasting
        a                 owl:NamedIndividual , :Sandblasting ;
        rdfs:comment      "Instance of an activity which is part of the creation process of ARTWORK_18_64."@en ;
        rdfs:label        "ARTWORK_18_64_Sandblasting"@en ;
        :Followed-By      :ARTWORK_18_64_Signing ;
        :Follows          :ARTWORK_18_64_Polishing ;
        :Has-Duration     <http://www.semanticweb.org/ontologies/Daan/2020/BarbaraNanning#2015> ;
        :Involves         :AlešZvěřina , :BarbaraNanning ;
        :Located-In       :NovyBor ;
        :Part-Of          :Creation_Artwork_18_64 ;
        :Requires-Use-Of  :AirCompressor .

:Is-Processed-In  a    owl:ObjectProperty ;
        rdfs:comment   "Is-Processed-In is a property which connects an entity with the material it is created from."@en ;
        rdfs:domain    :Material ;
        rdfs:label     "Is-Processed-In"@en ;
        rdfs:range     :Entity ;
        owl:inverseOf  :Made-Out-Of .

:ARTWORK_44_Signing  a    owl:NamedIndividual , :Signing ;
        rdfs:comment      "Instance of an activity which is part of the creation process of ARTWORK_44."@en ;
        rdfs:label        "ARTWORK_44_Signing"@en ;
        :Followed-By      :ARTWORK_44_Packing_3 ;
        :Follows          :ARTWORK_44_Transporting_2 ;
        :Has-Duration     <http://www.semanticweb.org/ontologies/Daan/2020/BarbaraNanning#2018> ;
        :Involves         :AlešZvěřina , :BarbaraNanning ;
        :Located-In       :CzechRepublic ;
        :Part-Of          :Creation_Artwork_44 ;
        :Requires-Use-Of  :AirCompressor .

:ARTWORK_44_Gilding  a    :Gilding , owl:NamedIndividual ;
        rdfs:comment      "Instance of an activity which is part of the creation process of ARTWORK_44."@en ;
        rdfs:label        "ARTWORK_44_Gilding"@en ;
        :Followed-By      <http://www.semanticweb.org/ontologies/Daan/2020/BarbaraNanning#ARTWORK_44_ExaminingQuality(FinalResult)> ;
        :Follows          :ARTWORK_44_Transporting_3 ;
        :Has-Duration     <http://www.semanticweb.org/ontologies/Daan/2020/BarbaraNanning#2018> ;
        :Involves         :BarbaraNanning , :VáçlavNovák_Doksy_CzechRepublic ;
        :Located-In       :CzechRepublic ;
        :Part-Of          :Creation_Artwork_44 ;
        :Requires-Use-Of  :GildersKnife , :GildersTip , :GildingCushion , :INSTACOLLTool .

:ARTWORK_74_Cooling  a    owl:NamedIndividual , :Cooling ;
        rdfs:comment      "Instance of an activity which is part of the creation process of ARTWORK_74."@en ;
        rdfs:label        "ARTWORK_74_Cooling"@en ;
        :Followed-By      :ARTWORK_74_Packing ;
        :Follows          :ARTWORK_74_Translocating ;
        :Has-Duration     <http://www.semanticweb.org/ontologies/Daan/2020/BarbaraNanning#2008> ;
        :Involves         :AssistantOfBarbara , :LuděkKout ;
        :Located-In       :CzechRepublic ;
        :Part-Of          :Creation_Artwork_74 ;
        :Requires-Use-Of  :AnnealingKiln .

:Composing_Coloured_Patterns_with_Sheets_and_Strings
        a                owl:Class ;
        rdfs:comment     "Designs can be created using coloured flat glass or coloured glass that has been pulled into thin strings."@en ;
        rdfs:label       "Composing Coloured Patterns with Sheets and Strings"@en ;
        rdfs:subClassOf  :Activity .

<http://vocab.getty.edu/aat/300011002>
        a           owl:NamedIndividual ;
        owl:sameAs  :Iron .

:Flat_Fusing_Glass_Sheets_with_ARTWORK_36_Peacock_to_One_Glass_Panel
        a                owl:Class ;
        rdfs:comment     "To reach the patern of curves in the flat sheet can only be achieved by remelting, reshaping the finished ARTWORK 36 Peacock for the next step. Merge flat decorated plate and multiple stacked colored flat glass plates into one thick plate."@en ;
        rdfs:label       "Flat Fusing Glass Sheets with ARTWORK 36 Peacock to One Glass Panel"@en ;
        rdfs:subClassOf  :Activity .

<http://www.semanticweb.org/ontologies/Daan/2020/BarbaraNanning#CollectionMuseeDeDesignEtd'artsAppliquesContemporains>
        a               owl:NamedIndividual , :Collection ;
        rdfs:comment    "Collection maintained by the Musee de design et d'arts appliques contemporains."@en ;
        rdfs:label      "Collection Musee de design et d'arts appliques contemporains"@en ;
        :Consists-Of    :Artwork_74 ;
        :Located-In     :Lausanne ;
        :Maintained-By  <http://www.semanticweb.org/ontologies/Daan/2020/BarbaraNanning#MuseeDeDesignEtd'artsAppliquesContemporains> .

:ARTWORK_74_ExaminingTheQualityOfTheGlass
        a                 :Examining_the_Quality_of_the_Glass , owl:NamedIndividual ;
        rdfs:comment      "Instance of an activity which is part of the creation process of ARTWORK_74."@en ;
        rdfs:label        "ARTWORK_74_Examining the Quality of the Glass"@en ;
        :Followed-By      :ARTWORK_74_Cooling ;
        :Follows          :ARTWORK_74_Modeling ;
        :Has-Duration     <http://www.semanticweb.org/ontologies/Daan/2020/BarbaraNanning#2008> ;
        :Involves         :LuděkKout , <http://www.semanticweb.org/ontologies/Daan/2020/BarbaraNanning#AlesVacek(CZ)> , :BarbaraNanning ;
        :Located-In       :CzechRepublic ;
        :Part-Of          :Creation_Artwork_74 ;
        :Requires-Use-Of  :Pontis , :StraightShears , :Furnace , :DiamondShears , :GloryHole , :CeramicPotFilledWithGlass , :Paper , :BlowingPipe , :Water , :YokeOfSupport , :Blocks , :AnnealingKiln , :Jacks .

<http://vocab.getty.edu/aat/300005232>
        a                    owl:Class ;
        owl:equivalentClass  :Gallery .

:ARTWORK_39_Polishing
        a                 owl:NamedIndividual , :Polishing ;
        rdfs:comment      "Instance of an activity which is part of the creation process of ARTWORK_39."@en ;
        rdfs:label        "ARTWORK_39_Polishing"@en ;
        :Followed-By      :ARTWORK_39_Sandblasting ;
        :Follows          :ARTWORK_39_Grinding ;
        :Has-Duration     <http://www.semanticweb.org/ontologies/Daan/2020/BarbaraNanning#2015> ;
        :Involves         :LukášSvoboda , :AlešZvěřina , :BarbaraNanning ;
        :Located-In       :NovyBor ;
        :Part-Of          :Creation_Artwork_39 ;
        :Requires-Use-Of  :PolishingStone .

:RobertFlorian  a     :Grinder_3 , owl:NamedIndividual ;
        rdfs:comment  "Robert Florian is a Grinder 3."@en ;
        rdfs:label    "Robert Florian"@en ;
        :Involved-In  :ARTWORK_80_Grinding , :ARTWORK_74_Grinding , :ARTWORK_73_Grinding , :ARTWORK_79_Grinding , :ARTWORK_76_Grinding , :ARTWORK_43_Grinding , :ARTWORK_44_Grinding , :ARTWORK_75_Grinding , :ARTWORK_77_Grinding , :ARTWORK_78_Grinding ;
        :Works-For    <http://www.semanticweb.org/ontologies/Daan/2020/BarbaraNanning#Ale%C5%A1Zv%C4%9B%C5%99ina&AZ-Design> .

:Resting  a              owl:Class ;
        rdfs:comment     "Resting is an activity in which all movement of a thing or actor is ceased. The timing of the resting is crucial."@en ;
        rdfs:label       "Resting"@en ;
        rdfs:subClassOf  :Activity .

:ARTWORK_80_PreparingGlass
        a                 owl:NamedIndividual , :Preparing_Glass ;
        rdfs:comment      "Instance of an activity which is part of the creation process of ARTWORK_80."@en ;
        rdfs:label        "ARTWORK_80_Preparing Glass"@en ;
        :Followed-By      :ARTWORK_80_SetupAndTestingOfTheMetalMold ;
        :Has-Duration     <http://www.semanticweb.org/ontologies/Daan/2020/BarbaraNanning#2018> ;
        :Involves         :BarbaraNanning , <http://www.semanticweb.org/ontologies/Daan/2020/BarbaraNanning#RadekKoten(CZ)> ;
        :Located-In       :CzechRepublic ;
        :Part-Of          :Creation_Artwork_80 ;
        :Requires-Use-Of  :Marver , :Pontis , :GloryHole , :BlowingPipe , :Garage ;
        :Starts           :Creation_Artwork_80 .

:YokeOfSupport  a     :Equipment , owl:NamedIndividual ;
        rdfs:comment  "A yoke of support is similar to a workbench and used during glassblowing to provide support."@en ;
        rdfs:label    "Yoke of Support"@en ;
        :Used-For     :ARTWORK_80_ApplyingClearGlassBell , :ARTWORK_78_Glassblowing , :ARTWORK_74_ApplyingExtraColour , :ARTWORK_73_Glassblowing , :ARTWORK_75_Glassblowing , :ARTWORK_79_ExaminingTheQualityOfTheGlass , :ARTWORK_74_ExaminingTheQualityOfTheGlass , :ARTWORK_74_Glassblowing , :ARTWORK_77_Glassblowing , :ARTWORK_74_ApplyingExtraColour_2 , :ARTWORK_44_ApplyingExtraColour , :ARTWORK_79_Glassblowing , :ARTWORK_75_ApplyingClearGlassBell , :ARTWORK_76_Glassblowing , :ARTWORK_44_Glassblowing , :ARTWORK_80_ExaminingTheQualityOfTheGlass , :ARTWORK_76_ExaminingTheQualityOfTheGlass , :ARTWORK_77_ApplyingClearGlassBell , :ARTWORK_76_ApplyingClearGlassBell , :ARTWORK_79_ApplyingExtraColour , :ARTWORK_75_ExaminingTheQualityOfTheGlass , :ARTWORK_79_ApplyingClearGlassBell , :ARTWORK_43_ExaminingTheQualityOfTheGlass , :ARTWORK_43_Glassblowing , :ARTWORK_44_ApplyingClearGlassBell , :ARTWORK_79_ApplyingExtraColour_2 , :ARTWORK_73_ApplyingClearGlassBell , :ARTWORK_43_ApplyingClearGlassBell , :ARTWORK_77_ApplyingExtraColour , :ARTWORK_77_ExaminingTheQualityOfTheGlass , :ARTWORK_76_ApplyingExtraColour_2 , :ARTWORK_43_ApplyingExtraColour , :ARTWORK_80_ApplyingExtraColour , :ARTWORK_75_ApplyingExtraColour_2 , :ARTWORK_78_ApplyingClearGlassBell , :ARTWORK_78_ExaminingTheQualityOfTheGlass , :ARTWORK_44_ApplyingExtraColour_2 , :ARTWORK_74_ApplyingClearGlassBell , :ARTWORK_80_Glassblowing , :ARTWORK_73_ExaminingTheQualityOfTheGlass , :ARTWORK_75_ApplyingExtraColour , :ARTWORK_76_ApplyingExtraColour , :ARTWORK_78_ApplyingExtraColour , :ARTWORK_44_ExaminingTheQualityOfTheGlass .

<http://www.semanticweb.org/ontologies/Daan/2020/BarbaraNanning#ARTWORK_36_ExaminingQuality(Result)>
        a              owl:NamedIndividual , j.0: ;
        rdfs:comment   "Instance of an activity which is part of the creation process of ARTWORK_36."@en ;
        rdfs:label     "ARTWORK_36_Examining Quality (Result)"@en ;
        :Followed-By   :ARTWORK_36_MeasuringAndBoxesMaking ;
        :Follows       :ARTWORK_36_Polishing ;
        :Has-Duration  <http://www.semanticweb.org/ontologies/Daan/2020/BarbaraNanning#2015> ;
        :Involves      :AlešZvěřina , :BarbaraNanning ;
        :Located-In    :NovyBor ;
        :Part-Of       :Creation_Artwork_36 .

<http://www.wikidata.org/entity/Q16798631>
        a       owl:Class .

:Starts  a             owl:ObjectProperty ;
        rdfs:comment   "Starts is a property which indicates the sub-event which Starts an event."@en ;
        rdfs:domain    :Event ;
        rdfs:label     "Starts"@en ;
        rdfs:range     :Event ;
        owl:inverseOf  :Starts-With .

:ARTWORK_18_64_Transporting_2
        a              :Transporting , owl:NamedIndividual ;
        rdfs:comment   "Instance of an activity which is part of the creation process of ARTWORK_18_64."@en ;
        rdfs:label     "ARTWORK_18_64_Transporting_2"@en ;
        :Followed-By   :ARTWORK_18_64_Photographing ;
        :Follows       :ARTWORK_18_64_Packing_2 ;
        :Has-Duration  <http://www.semanticweb.org/ontologies/Daan/2020/BarbaraNanning#2015> ;
        :Involves      :AlešZvěřina , :BarbaraNanning ;
        :Located-In    :Amsterdam ;
        :Part-Of       :Creation_Artwork_18_64 .

:ARTWORK_74_Resting  a    owl:NamedIndividual , :Resting ;
        rdfs:comment      "Instance of an activity which is part of the creation process of ARTWORK_74."@en ;
        rdfs:label        "ARTWORK_74_Resting"@en ;
        :Followed-By      <http://www.semanticweb.org/ontologies/Daan/2020/BarbaraNanning#ARTWORK_74_ExaminingQuality(CheckForIrregularitiesInTheGlass)> ;
        :Follows          :ARTWORK_74_Transporting ;
        :Has-Duration     <http://www.semanticweb.org/ontologies/Daan/2020/BarbaraNanning#2008> ;
        :Involves         :AlešZvěřina ;
        :Located-In       :CzechRepublic ;
        :Part-Of          :Creation_Artwork_74 ;
        :Requires-Use-Of  :AnnealingKiln .

<http://www.semanticweb.org/ontologies/Daan/2020/BarbaraNanning#ARTWORK_74_ExaminingQuality(CheckForIrregularitiesInTheGlass)>
        a              j.3: , owl:NamedIndividual ;
        rdfs:comment   "Instance of an activity which is part of the creation process of ARTWORK_74."@en ;
        rdfs:label     "ARTWORK_74_Examining Quality (Check for Irregularities in the Glass)"@en ;
        :Followed-By   :ARTWORK_74_Sawing ;
        :Follows       :ARTWORK_74_Resting ;
        :Has-Duration  <http://www.semanticweb.org/ontologies/Daan/2020/BarbaraNanning#2008> ;
        :Involves      :AlešZvěřina , :BarbaraNanning ;
        :Located-In    :CzechRepublic ;
        :Part-Of       :Creation_Artwork_74 .

:ARTWORK_36_TransportingMetalBowlWithPanel
        a              owl:NamedIndividual , :Transporting_Metal_Bowl_with_Panel ;
        rdfs:comment   "Instance of an activity which is part of the creation process of ARTWORK_36."@en ;
        rdfs:label     "ARTWORK_36_Transporting Metal Bowl with Panel"@en ;
        :Followed-By   :ARTWORK_36_PreparingForBlowing_2 ;
        :Follows       :ARTWORK_36_SlumpingPanel ;
        :Has-Duration  <http://www.semanticweb.org/ontologies/Daan/2020/BarbaraNanning#2019> ;
        :Involves      :BarbaraNanning ;
        :Located-In    :Amsterdam ;
        :Part-Of       :Creation_Artwork_36 .

:GildingCushion  a    :Tool , owl:NamedIndividual ;
        rdfs:comment  "A gilding cushion is a leather cushion which is used for gilding together with a gilders knife."@en ;
        rdfs:label    "Gilding Cushion"@en ;
        :Made-Out-Of  :Leather ;
        :Used-For     :ARTWORK_74_Gilding , :ARTWORK_79_Gilding , :ARTWORK_76_Gilding , :ARTWORK_75_Gilding , :ARTWORK_73_Gilding , :ARTWORK_44_Gilding , :ARTWORK_78_Gilding , :ARTWORK_43_Gilding , :ARTWORK_80_Gilding , :ARTWORK_77_Gilding .

<http://www.semanticweb.org/ontologies/Daan/2020/BarbaraNanning#deRoo&Sainthill_Haarlem>
        a             owl:NamedIndividual , :Gilder ;
        rdfs:comment  "de Roo & Sainthill_Haarlem is a Gilder."@en ;
        rdfs:label    "de Roo & Sainthill_Haarlem"@en .

:ARTWORK_74_Modeling  a   owl:NamedIndividual , :Modeling ;
        rdfs:comment      "Instance of an activity which is part of the creation process of ARTWORK_74."@en ;
        rdfs:label        "ARTWORK_74_Modeling"@en ;
        :Followed-By      <http://www.semanticweb.org/ontologies/Daan/2020/BarbaraNanning#ARTWORK_74_ExaminingQuality(Shape/Form)> ;
        :Follows          :ARTWORK_74_Sensing ;
        :Has-Duration     <http://www.semanticweb.org/ontologies/Daan/2020/BarbaraNanning#2008> ;
        :Involves         <http://www.semanticweb.org/ontologies/Daan/2020/BarbaraNanning#AlesVacek(CZ)> , :BarbaraNanning , <http://www.semanticweb.org/ontologies/Daan/2020/BarbaraNanning#RobertHlavacek(CZ)> , <http://www.semanticweb.org/ontologies/Daan/2020/BarbaraNanning#RomanTomis(CZ)> , :AssistantOfBarbara , <http://www.semanticweb.org/ontologies/Daan/2020/BarbaraNanning#RostislavMaterka(CZ)> ;
        :Located-In       :CzechRepublic ;
        :Part-Of          :Creation_Artwork_74 ;
        :Requires-Use-Of  :InterchangeableMetalMoldSetup , :Gloves , :BlowingPipe , :AirCompressor , :PropaneTorch .

:Tackfusing_Coloured_Canes_and_Strings
        a                owl:Class ;
        rdfs:comment     "After a patern of canes and strings has been placed in a metal form or in a metal ring it will be placed in the kiln to be fused together before use by the glassblower for the final object."@en ;
        rdfs:label       "Tackfusing Coloured Canes and Strings"@en ;
        rdfs:subClassOf  :Activity .

:ARTWORK_74_Transporting
        a              owl:NamedIndividual , :Transporting ;
        rdfs:comment   "Instance of an activity which is part of the creation process of ARTWORK_74."@en ;
        rdfs:label     "ARTWORK_74_Transporting"@en ;
        :Followed-By   :ARTWORK_74_Resting ;
        :Follows       :ARTWORK_74_Packing ;
        :Has-Duration  <http://www.semanticweb.org/ontologies/Daan/2020/BarbaraNanning#2008> ;
        :Involves      :BarbaraNanning , :AlešZvěřina ;
        :Located-In    :CzechRepublic ;
        :Part-Of       :Creation_Artwork_74 .

:Artwork_18_64  a     :Glass_Artwork , owl:NamedIndividual ;
        rdfs:comment  "Artwork_18_64 is a glass artwork made by Barbara Nanning."@en ;
        rdfs:label    "Coloured Shadows Facets"@en ;
        :Created-By   :Creation_Artwork_18_64 ;
        :Has-Depth    "22"^^xsd:decimal ;
        :Has-Height   "11"^^xsd:decimal , "22"^^xsd:decimal ;
        :Is-Unica     "Yes"@en ;
        :Made-By      :BarbaraNanning , <http://www.semanticweb.org/ontologies/Daan/2020/BarbaraNanning#Ji%C5%99%C3%ADPa%C4%8DinekLindava(CZ)> , :GlassStudioVanTetterode , :BullseyeGlassSplinterEnDeVosch , <http://www.semanticweb.org/ontologies/Daan/2020/BarbaraNanning#Ale%C5%A1Zv%C4%9B%C5%99ina&AZ-Design> , :VRIJGLASZaandam ;
        :Made-Out-Of  :FlatGlassheetWithColouredCanes , :BullseyeGlass ;
        :Shown-By     :Image_Artwork_18_64 .

:Image_Artwork_36  a            :Digital_Image , owl:NamedIndividual ;
        rdfs:comment            "Image of Artwork_36 by Barbara Nanning."@en ;
        rdfs:label              "Image_Artwork_36"@en ;
        :Representation-Source  "Tom Haartsen_Ouderkerk A/d Amstel (NL)"@en ;
        :Shows                  :Artwork_36 .

:ARTWORK_74_Packing_5
        a              :Packing , owl:NamedIndividual ;
        rdfs:comment   "Instance of an activity which is part of the creation process of ARTWORK_74."@en ;
        rdfs:label     "ARTWORK_74_Packing_5"@en ;
        :Finishes      :Creation_Artwork_74 ;
        :Follows       :ARTWORK_74_Documenting ;
        :Has-Duration  <http://www.semanticweb.org/ontologies/Daan/2020/BarbaraNanning#2008> ;
        :Involves      :BarbaraNanning ;
        :Located-In    :CzechRepublic ;
        :Part-Of       :Creation_Artwork_74 .

:ARTWORK_79_PreparingGlass
        a                 :Preparing_Glass , owl:NamedIndividual ;
        rdfs:comment      "Instance of an activity which is part of the creation process of ARTWORK_79."@en ;
        rdfs:label        "ARTWORK_79_Preparing Glass"@en ;
        :Followed-By      :ARTWORK_79_SetupAndTestingOfTheMetalMold ;
        :Has-Duration     <http://www.semanticweb.org/ontologies/Daan/2020/BarbaraNanning#2018> ;
        :Involves         <http://www.semanticweb.org/ontologies/Daan/2020/BarbaraNanning#RadekKoten(CZ)> , :BarbaraNanning ;
        :Located-In       :CzechRepublic ;
        :Part-Of          :Creation_Artwork_79 ;
        :Requires-Use-Of  :GloryHole , :Marver , :BlowingPipe , :Garage , :Pontis ;
        :Starts           :Creation_Artwork_79 .

:ARTWORK_76_Documenting
        a              owl:NamedIndividual , :Documenting ;
        rdfs:comment   "Instance of an activity which is part of the creation process of ARTWORK_76."@en ;
        rdfs:label     "ARTWORK_76_Documenting"@en ;
        :Followed-By   :ARTWORK_76_Packing_5 ;
        :Follows       :ARTWORK_76_Photographing ;
        :Has-Duration  <http://www.semanticweb.org/ontologies/Daan/2020/BarbaraNanning#2018> ;
        :Involves      :BarbaraNanning ;
        :Located-In    :CzechRepublic ;
        :Part-Of       :Creation_Artwork_76 .

:ARTWORK_17_33_PreparingGlass
        a                 :Preparing_Glass , owl:NamedIndividual ;
        rdfs:comment      "Instance of an activity which is part of the creation process of ARTWORK_17_33."@en ;
        rdfs:label        "ARTWORK_17_33_Preparing Glass"@en ;
        :Followed-By      :ARTWORK_17_33_ExaminingTheQualityOfTheGlass ;
        :Follows          :ARTWORK_17_33_FillingKilnsWithMetalBowl ;
        :Has-Duration     <http://www.semanticweb.org/ontologies/Daan/2020/BarbaraNanning#2017> ;
        :Involves         :BarbaraNanning , <http://www.semanticweb.org/ontologies/Daan/2020/BarbaraNanning#RadekKoten(CZ)> ;
        :Located-In       :Lindava ;
        :Part-Of          :Creation_Artwork_17_33 ;
        :Requires-Use-Of  :Marver , :Garage , :GloryHole , :BlowingPipe , :Pontis .

:Has-Duration  a      owl:ObjectProperty ;
        rdfs:comment  "Has-Duration is a property which connects a timespan to a period."@en ;
        rdfs:domain   :Period ;
        rdfs:label    "Has-Duration"@en ;
        rdfs:range    :Timespan .

:ARTWORK_73_Cooling  a    :Cooling , owl:NamedIndividual ;
        rdfs:comment      "Instance of an activity which is part of the creation process of ARTWORK_73."@en ;
        rdfs:label        "ARTWORK_73_Cooling"@en ;
        :Followed-By      :ARTWORK_73_Packing ;
        :Follows          :ARTWORK_73_Translocating ;
        :Has-Duration     <http://www.semanticweb.org/ontologies/Daan/2020/BarbaraNanning#2018> ;
        :Involves         :LuděkKout , :AssistantOfBarbara ;
        :Located-In       :CzechRepublic ;
        :Part-Of          :Creation_Artwork_73 ;
        :Requires-Use-Of  :AnnealingKiln .

:ARTWORK_80_Cooling  a    owl:NamedIndividual , :Cooling ;
        rdfs:comment      "Instance of an activity which is part of the creation process of ARTWORK_80."@en ;
        rdfs:label        "ARTWORK_80_Cooling"@en ;
        :Followed-By      :ARTWORK_80_Packing ;
        :Follows          :ARTWORK_80_Translocating ;
        :Has-Duration     <http://www.semanticweb.org/ontologies/Daan/2020/BarbaraNanning#2018> ;
        :Involves         :AssistantOfBarbara , :LuděkKout ;
        :Located-In       :CzechRepublic ;
        :Part-Of          :Creation_Artwork_80 ;
        :Requires-Use-Of  :AnnealingKiln .

:Creation_Event  a       owl:Class ;
        rdfs:comment     "A creation event is an event in which a thing is brought into existence."@en ;
        rdfs:label       "Creation Event"@en ;
        rdfs:subClassOf  :Event .

:ARTWORK_79_Packing  a  owl:NamedIndividual , :Packing ;
        rdfs:comment   "Instance of an activity which is part of the creation process of ARTWORK_79."@en ;
        rdfs:label     "ARTWORK_79_Packing"@en ;
        :Followed-By   :ARTWORK_79_Transporting ;
        :Follows       :ARTWORK_79_Cooling ;
        :Has-Duration  <http://www.semanticweb.org/ontologies/Daan/2020/BarbaraNanning#2018> ;
        :Involves      :BarbaraNanning , :AlešZvěřina ;
        :Located-In    :CzechRepublic ;
        :Part-Of       :Creation_Artwork_79 .

:ARTWORK_44_Polishing
        a                 :Polishing , owl:NamedIndividual ;
        rdfs:comment      "Instance of an activity which is part of the creation process of ARTWORK_44."@en ;
        rdfs:label        "ARTWORK_44_Polishing"@en ;
        :Followed-By      :ARTWORK_44_MeasuringAndBoxesMaking ;
        :Follows          :ARTWORK_44_Grinding ;
        :Has-Duration     <http://www.semanticweb.org/ontologies/Daan/2020/BarbaraNanning#2018> ;
        :Involves         :LukášSvoboda , :BarbaraNanning , :AlešZvěřina ;
        :Located-In       :CzechRepublic ;
        :Part-Of          :Creation_Artwork_44 ;
        :Requires-Use-Of  :PolishingStone .

:ARTWORK_18_64_MeasuringAndBoxesMaking
        a              :Measuring_and_Boxes_Making , owl:NamedIndividual ;
        rdfs:comment   "Instance of an activity which is part of the creation process of ARTWORK_18_64."@en ;
        rdfs:label     "ARTWORK_18_64_Measuring and Boxes Making"@en ;
        :Followed-By   :ARTWORK_18_64_Packing_2 ;
        :Follows       <http://www.semanticweb.org/ontologies/Daan/2020/BarbaraNanning#ARTWORK_18_64_ExaminingQuality(Result)> ;
        :Has-Duration  <http://www.semanticweb.org/ontologies/Daan/2020/BarbaraNanning#2015> ;
        :Involves      :AlešZvěřina , :BarbaraNanning ;
        :Located-In    :NovyBor ;
        :Part-Of       :Creation_Artwork_18_64 .

:ARTWORK_77_Translocating
        a                 owl:NamedIndividual , :Translocating ;
        rdfs:comment      "Instance of an activity which is part of the creation process of ARTWORK_77."@en ;
        rdfs:label        "ARTWORK_77_Translocating"@en ;
        :Followed-By      :ARTWORK_77_Cooling ;
        :Follows          <http://www.semanticweb.org/ontologies/Daan/2020/BarbaraNanning#ARTWORK_77_ExaminingQuality(Shape/Form)> ;
        :Has-Duration     <http://www.semanticweb.org/ontologies/Daan/2020/BarbaraNanning#2018> ;
        :Involves         :BarbaraNanning ;
        :Located-In       :CzechRepublic ;
        :Part-Of          :Creation_Artwork_77 ;
        :Requires-Use-Of  :Fork .

:Picking_up_Coloured_Panel
        a                owl:Class ;
        rdfs:comment     "This can be done in two ways. A round coloured panel can be stuck onto a hot bubble of glass and sculpted around.  Or a flat coloured panel can be rolled onto a disc of glass creating a cylinder form."@en ;
        rdfs:label       "Picking up Coloured Panel"@en ;
        rdfs:subClassOf  :Activity .

:Private_Collection  a   owl:Class ;
        rdfs:comment     "A private collection is a art collection owned by an actor."@en ;
        rdfs:label       "Private Collection"@en ;
        rdfs:subClassOf  :Collection .

:LouvreGoldLeaf  a            :Gold_Leaf , owl:NamedIndividual ;
        rdfs:comment          "Louvre gold leaf is champagne coloured gold leaf."@en ;
        rdfs:label            "Louvre Gold Leaf"@en ;
        :Carat                "23"^^xsd:decimal ;
        :Is-Processed-During  :ARTWORK_77_Gilding , :ARTWORK_74_Gilding ;
        :Is-Processed-In      :Artwork_77 , :Artwork_74 .

:Made-By  a            owl:ObjectProperty ;
        rdfs:comment   "Made-By is a property which connects a thing with the creator of this thing."@en ;
        rdfs:domain    :Thing ;
        rdfs:label     "Made-By"@en ;
        rdfs:range     :Actor ;
        owl:inverseOf  :Maker-Of .

:Creation_Artwork_80  a  owl:NamedIndividual , :Creation_Event ;
        rdfs:comment    "Creation event for an artwork by Barbara Nanning displayed in \"Barbara Nanning Eeuwige Beweging\" by Eliens (2019)."@en ;
        rdfs:label      "Creation_Artwork_80"@en ;
        :Consists-Of    :ARTWORK_80_Photographing , :ARTWORK_80_SetupAndTestingOfTheMetalMold_2 , :ARTWORK_80_Modeling , <http://www.semanticweb.org/ontologies/Daan/2020/BarbaraNanning#ARTWORK_80_ExaminingQuality(Shape/Form)> , :ARTWORK_80_Packing_2 , :ARTWORK_80_ExaminingTheQualityOfTheGlass , :ARTWORK_80_Documenting , :ARTWORK_80_SetupAndTestingOfTheMetalMold , :ARTWORK_80_ApplyingExtraColour , :ARTWORK_80_Sensing , :ARTWORK_80_MeasuringAndBoxesMaking , :ARTWORK_80_Sawing , :ARTWORK_80_Grinding , :ARTWORK_80_Sandblasting , :ARTWORK_80_Signing , <http://www.semanticweb.org/ontologies/Daan/2020/BarbaraNanning#ARTWORK_80_ExaminingQuality(CheckForIrregularitiesInTheGlass)> , :ARTWORK_80_Packing_3 , :ARTWORK_80_Packing , :ARTWORK_80_PreparingGlass , :ARTWORK_80_Transporting_2 , <http://www.semanticweb.org/ontologies/Daan/2020/BarbaraNanning#ARTWORK_80_ExaminingQuality(FinalResult)> , :ARTWORK_80_Resting , :ARTWORK_80_Translocating , :ARTWORK_80_Packing_4 , :ARTWORK_80_Transporting , :ARTWORK_80_Transporting_3 , :ARTWORK_80_HeatingMetalMold , :ARTWORK_80_Glassblowing , :ARTWORK_80_Gilding , :ARTWORK_80_ApplyingClearGlassBell , :ARTWORK_80_Polishing , :ARTWORK_80_Cooling , <http://www.semanticweb.org/ontologies/Daan/2020/BarbaraNanning#ARTWORK_80_ExaminingQuality(Result)> ;
        :Created        :Artwork_80 ;
        :Finishes-With  :ARTWORK_80_Packing_4 ;
        :Has-Duration   <http://www.semanticweb.org/ontologies/Daan/2020/BarbaraNanning#2018> ;
        :Located-In     :CzechRepublic ;
        :Starts-With    :ARTWORK_80_PreparingGlass ;
        :Within-Period  :GlassVerreÉglomisé .

:ARTWORK_46_ProducingColouredCanes
        a                 owl:NamedIndividual , :Producing_Coloured_Canes ;
        rdfs:comment      "Instance of an activity which is part of the creation process of ARTWORK_46."@en ;
        rdfs:label        "ARTWORK_46_Producing Coloured Canes"@en ;
        :Followed-By      :ARTWORK_46_TransportingColouredCanes ;
        :Follows          :ARTWORK_46_TransportingMonochromeRods ;
        :Has-Duration     <http://www.semanticweb.org/ontologies/Daan/2020/BarbaraNanning#2015> ;
        :Involves         <http://www.semanticweb.org/ontologies/Daan/2020/BarbaraNanning#MarekEffmert(CZ)> , <http://www.semanticweb.org/ontologies/Daan/2020/BarbaraNanning#MarekBrathko(CZ)> , <http://www.semanticweb.org/ontologies/Daan/2020/BarbaraNanning#JessicaHomich(USA)> , <http://www.semanticweb.org/ontologies/Daan/2020/BarbaraNanning#MiaLerssi(DN)> , <http://www.semanticweb.org/ontologies/Daan/2020/BarbaraNanning#RobertLenner(CZ)> , :DurkValkema , :GertBullée , :BarbaraNanning ;
        :Located-In       :Zaandam ;
        :Part-Of          :Creation_Artwork_46 ;
        :Requires-Use-Of  :Hook , :AirCompressor , :Computer , :SharpeningStone , :FusingKiln , :Water , :Furnace , :Tagliol , :BitIrons , :PropaneTorch , :DiamondShears , :AnnealingKiln , :Beeswax , :Pontis , :StraightShears , :Blocks , :Marver , :Paper , :Jacks , :Garage , :GrindingWheel , :GloryHole , :YokeOfSupport , :Gloves .

<http://www.semanticweb.org/ontologies/Daan/2020/BarbaraNanning#FredStikvoort(NL)>
        a             owl:NamedIndividual , :Grinder_2 ;
        rdfs:comment  "Fred Stikvoort (NL) is a Grinder 2."@en ;
        rdfs:label    "Fred Stikvoort (NL)"@en ;
        :Involved-In  :ARTWORK_39_CuttingSheets , :ARTWORK_18_64_CuttingSheets ;
        :Works-For    :GlassStudioVanTetterode .

:Representation-Source
        a             owl:DatatypeProperty ;
        rdfs:comment  "Representation-Source is a property which connects a representation to the source (string)."@en ;
        rdfs:domain   :Representation ;
        rdfs:label    "Representation-Source"@en ;
        rdfs:range    xsd:string .

:ARTWORK_17_33_MeasuringAndBoxesMaking
        a              owl:NamedIndividual , :Measuring_and_Boxes_Making ;
        rdfs:comment   "Instance of an activity which is part of the creation process of ARTWORK_17_33."@en ;
        rdfs:label     "ARTWORK_17_33_Measuring and Boxes Making"@en ;
        :Followed-By   :ARTWORK_17_33_Packing_2 ;
        :Follows       <http://www.semanticweb.org/ontologies/Daan/2020/BarbaraNanning#ARTWORK_17_33_ExaminingQuality(Result)> ;
        :Has-Duration  <http://www.semanticweb.org/ontologies/Daan/2020/BarbaraNanning#2017> ;
        :Involves      :AlešZvěřina , :BarbaraNanning ;
        :Located-In    :NovyBor ;
        :Part-Of       :Creation_Artwork_17_33 .

:ARTWORK_73_Transporting
        a              :Transporting , owl:NamedIndividual ;
        rdfs:comment   "Instance of an activity which is part of the creation process of ARTWORK_73."@en ;
        rdfs:label     "ARTWORK_73_Transporting"@en ;
        :Followed-By   :ARTWORK_73_Resting ;
        :Follows       :ARTWORK_73_Packing ;
        :Has-Duration  <http://www.semanticweb.org/ontologies/Daan/2020/BarbaraNanning#2018> ;
        :Involves      :BarbaraNanning , :AlešZvěřina ;
        :Located-In    :CzechRepublic ;
        :Part-Of       :Creation_Artwork_73 .

<http://www.semanticweb.org/ontologies/Daan/2020/BarbaraNanning#ARTWORK_43_ExaminingQuality(Shape/Form)>
        a                 j.2: , owl:NamedIndividual ;
        rdfs:comment      "Instance of an activity which is part of the creation process of ARTWORK_43."@en ;
        rdfs:label        "ARTWORK_43_Examining Quality (Shape/Form)"@en ;
        :Followed-By      :ARTWORK_43_Translocating ;
        :Follows          :ARTWORK_43_Modeling ;
        :Has-Duration     <http://www.semanticweb.org/ontologies/Daan/2020/BarbaraNanning#2008> ;
        :Involves         :BarbaraNanning , :LuděkKout , <http://www.semanticweb.org/ontologies/Daan/2020/BarbaraNanning#AlesVacek(CZ)> ;
        :Located-In       :CzechRepublic ;
        :Part-Of          :Creation_Artwork_43 ;
        :Requires-Use-Of  :GloryHole , :Pontis , :BlowingPipe .

:ARTWORK_79_MeasuringAndBoxesMaking
        a              owl:NamedIndividual , :Measuring_and_Boxes_Making ;
        rdfs:comment   "Instance of an activity which is part of the creation process of ARTWORK_79."@en ;
        rdfs:label     "ARTWORK_79_Measuring and Boxes Making"@en ;
        :Followed-By   :ARTWORK_79_Packing_2 ;
        :Follows       <http://www.semanticweb.org/ontologies/Daan/2020/BarbaraNanning#ARTWORK_79_ExaminingQuality(Result)> ;
        :Has-Duration  <http://www.semanticweb.org/ontologies/Daan/2020/BarbaraNanning#2018> ;
        :Involves      :AlešZvěřina , :BarbaraNanning ;
        :Located-In    :CzechRepublic ;
        :Part-Of       :Creation_Artwork_79 .

<http://www.wikidata.org/entity/Q60>
        a       owl:NamedIndividual .

:Gold_Leaf  a                owl:Class ;
        rdfs:comment         "Gold leaf is a thin sheet of gold to be used in gilding."@en ;
        rdfs:label           "Gold Leaf"@en ;
        rdfs:subClassOf      :Man-Made_Material ;
        owl:equivalentClass  <http://www.wikidata.org/entity/Q929186> .

:ARTWORK_80_Resting  a    :Resting , owl:NamedIndividual ;
        rdfs:comment      "Instance of an activity which is part of the creation process of ARTWORK_80."@en ;
        rdfs:label        "ARTWORK_80_Resting"@en ;
        :Followed-By      <http://www.semanticweb.org/ontologies/Daan/2020/BarbaraNanning#ARTWORK_80_ExaminingQuality(CheckForIrregularitiesInTheGlass)> ;
        :Follows          :ARTWORK_80_Transporting ;
        :Has-Duration     <http://www.semanticweb.org/ontologies/Daan/2020/BarbaraNanning#2018> ;
        :Involves         :AlešZvěřina ;
        :Located-In       :CzechRepublic ;
        :Part-Of          :Creation_Artwork_80 ;
        :Requires-Use-Of  :AnnealingKiln .

<http://www.semanticweb.org/ontologies/Daan/2020/BarbaraNanning#MarekBrathko(CZ)>
        a             owl:NamedIndividual , :First_Glass_Blower ;
        rdfs:comment  "Marek Brathko is a First Glass Blower."@en ;
        rdfs:label    "Marek Brathko (CZ)"@en ;
        :Involved-In  :ARTWORK_36_PickingUpColouredCanesPattern , :ARTWORK_18_64_Modeling , :ARTWORK_36_SetupAndTestingOfTheMetalMold , :ARTWORK_18_64_ProducingColouredCanes , :ARTWORK_39_Modeling , :ARTWORK_36_Glassblowing , :ARTWORK_39_SetupAndTestingOfTheMetalMold , :ARTWORK_39_PickingUpColouredPanel , :ARTWORK_39_ApplyingClearGlassBell , :ARTWORK_36_ApplyingClearGlassBell , :ARTWORK_36_PickingUpColouredPanel , :ARTWORK_36_Modeling , :ARTWORK_18_64_Glassblowing , :ARTWORK_18_64_PickingUpColouredCanesPattern , :ARTWORK_39_Glassblowing , :ARTWORK_18_64_ApplyingClearGlassBell , :ARTWORK_36_ProducingColouredCanes , :ARTWORK_46_ProducingColouredCanes ;
        :Works-For    :VRIJGLASZaandam .

:ARTWORK_46_TransportingColouredCanes_2
        a              owl:NamedIndividual , :Transporting_Coloured_Canes ;
        rdfs:comment   "Instance of an activity which is part of the creation process of ARTWORK_46."@en ;
        rdfs:label     "ARTWORK_46_Transporting Coloured Canes_2"@en ;
        :Followed-By   :ARTWORK_46_CuttingStrings ;
        :Follows       :ARTWORK_46_CuttingAndPolishingColouredCanes ;
        :Has-Duration  <http://www.semanticweb.org/ontologies/Daan/2020/BarbaraNanning#2015> ;
        :Involves      :BarbaraNanning , :AlešZvěřina ;
        :Located-In    :NovyBor ;
        :Part-Of       :Creation_Artwork_46 .

:ARTWORK_36_Polishing_2
        a                 owl:NamedIndividual , :Polishing ;
        rdfs:comment      "Instance of an activity which is part of the creation process of ARTWORK_36."@en ;
        rdfs:label        "ARTWORK_36_Polishing_2"@en ;
        :Followed-By      <http://www.semanticweb.org/ontologies/Daan/2020/BarbaraNanning#ARTWORK_36_ExaminingQuality(Result)_2> ;
        :Follows          :ARTWORK_36_Grinding_2 ;
        :Has-Duration     <http://www.semanticweb.org/ontologies/Daan/2020/BarbaraNanning#2019> ;
        :Involves         :LukášSvoboda , :BarbaraNanning , :AlešZvěřina ;
        :Located-In       :NovyBor ;
        :Part-Of          :Creation_Artwork_36 ;
        :Requires-Use-Of  :PolishingStone .

:ARTWORK_36_Transporting_4
        a              owl:NamedIndividual , :Transporting ;
        rdfs:comment   "Instance of an activity which is part of the creation process of ARTWORK_36."@en ;
        rdfs:label     "ARTWORK_36_Transporting_4"@en ;
        :Followed-By   :ARTWORK_36_Resting_2 ;
        :Follows       :ARTWORK_36_Packing_5 ;
        :Has-Duration  <http://www.semanticweb.org/ontologies/Daan/2020/BarbaraNanning#2019> ;
        :Involves      :AlešZvěřina , :BarbaraNanning ;
        :Located-In    :NovyBor ;
        :Part-Of       :Creation_Artwork_36 .

:ARTWORK_46_Ordening  a   :Ordening , owl:NamedIndividual ;
        rdfs:comment      "Instance of an activity which is part of the creation process of ARTWORK_46."@en ;
        rdfs:label        "ARTWORK_46_Ordening"@en ;
        :Followed-By      :ARTWORK_46_Casting ;
        :Follows          :ARTWORK_46_CuttingMonochromeSheets ;
        :Has-Duration     <http://www.semanticweb.org/ontologies/Daan/2020/BarbaraNanning#2015> ;
        :Involves         :BarbaraNanning ;
        :Located-In       :Langweer ;
        :Part-Of          :Creation_Artwork_46 ;
        :Requires-Use-Of  :Computer , :Pincet , :Glassscissors .

:Representation  a       owl:Class ;
        rdfs:comment     "A representation is a portrayal of someone or something."@en ;
        rdfs:label       "Representation"@en ;
        rdfs:subClassOf  :Entity .

<http://www.semanticweb.org/ontologies/Daan/2020/BarbaraNanning#ARTWORK_36_ExaminingQuality(FinalResult)>
        a              j.1: , owl:NamedIndividual ;
        rdfs:comment   "Instance of an activity which is part of the creation process of ARTWORK_36."@en ;
        rdfs:label     "ARTWORK_36_Examining Quality (Final Result)"@en ;
        :Followed-By   :ARTWORK_36_Packing_3 ;
        :Follows       :ARTWORK_36_Signing ;
        :Has-Duration  <http://www.semanticweb.org/ontologies/Daan/2020/BarbaraNanning#2019> ;
        :Involves      :BarbaraNanning , :AlešZvěřina ;
        :Located-In    :NovyBor ;
        :Part-Of       :Creation_Artwork_36 .

<http://www.semanticweb.org/ontologies/Daan/2020/BarbaraNanning#ReichenbachColourRodsGlass(DE)>
        a                     owl:NamedIndividual , :Glass ;
        rdfs:comment          "Reichenbach Colour Rods Glass (DE) are rods of glass material."@en ;
        rdfs:label            "Reichenbach Colour Rods Glass (DE)"@en ;
        :Is-Processed-During  :ARTWORK_44_ApplyingExtraColour , :ARTWORK_75_ApplyingExtraColour , :ARTWORK_76_ApplyingExtraColour , :ARTWORK_43_ApplyingExtraColour , :ARTWORK_80_ApplyingExtraColour ;
        :Is-Processed-In      :Artwork_44 , :Artwork_80 , :Artwork_76 , :Artwork_75 , :Artwork_43 .

:ARTWORK_36_Casting  a    :Casting , owl:NamedIndividual ;
        rdfs:comment      "Instance of an activity which is part of the creation process of ARTWORK_36."@en ;
        rdfs:label        "ARTWORK_36_Casting"@en ;
        :Followed-By      :ARTWORK_36_CuttingAndPolishingCastedMonochromeSheetsToSmallRods ;
        :Follows          :ARTWORK_36_Ordening ;
        :Has-Duration     <http://www.semanticweb.org/ontologies/Daan/2020/BarbaraNanning#2015> ;
        :Involves         :BarbaraNanning , :SteefHendriks ;
        :Located-In       :Langweer ;
        :Part-Of          :Creation_Artwork_36 ;
        :Requires-Use-Of  :FusingKiln , :Gloves , :Furnace , :Pincet .

<http://www.wikidata.org/entity/Q706>
        a       owl:NamedIndividual .

:Country  a                  owl:Class ;
        rdfs:comment         "A country is a nation with a government and a particular location."@en ;
        rdfs:label           "Country"@en ;
        rdfs:subClassOf      :Place ;
        owl:equivalentClass  <http://www.wikidata.org/entity/Q6256> .

:ARTWORK_78_Resting  a    owl:NamedIndividual , :Resting ;
        rdfs:comment      "Instance of an activity which is part of the creation process of ARTWORK_78."@en ;
        rdfs:label        "ARTWORK_78_Resting"@en ;
        :Followed-By      <http://www.semanticweb.org/ontologies/Daan/2020/BarbaraNanning#ARTWORK_78_ExaminingQuality(CheckForIrregularitiesInTheGlass)> ;
        :Follows          :ARTWORK_78_Transporting ;
        :Has-Duration     <http://www.semanticweb.org/ontologies/Daan/2020/BarbaraNanning#2008> ;
        :Involves         :AlešZvěřina ;
        :Located-In       :CzechRepublic ;
        :Part-Of          :Creation_Artwork_78 ;
        :Requires-Use-Of  :AnnealingKiln .

:InterchangeableMetalMoldSetup
        a             owl:NamedIndividual , :Equipment ;
        rdfs:comment  "An Interchangeable Metal Mold setup is collection of cleaned iron plates used to model glass."@en ;
        rdfs:label    "Interchangeable Metal Mold Setup"@en ;
        :Made-By      <http://www.semanticweb.org/ontologies/Daan/2020/BarbaraNanning#StudioVogl(CZ)> , <http://www.semanticweb.org/ontologies/Daan/2020/BarbaraNanning#FlorisVanDonselaar(NL)> , <http://www.semanticweb.org/ontologies/Daan/2020/BarbaraNanning#Ren%C3%A9VanDonselaar(NL)> ;
        :Made-Out-Of  :Iron ;
        :Used-For     :ARTWORK_44_SetupAndTestingOfTheMetalMold_2 , :ARTWORK_43_Glassblowing , :ARTWORK_76_SetupAndTestingOfTheMetalMold_2 , :ARTWORK_73_SetupAndTestingOfTheMetalMold_2 , :ARTWORK_79_HeatingMetalMold , :ARTWORK_79_Modeling , :ARTWORK_43_SetupAndTestingOfTheMetalMold , :ARTWORK_77_SetupAndTestingOfTheMetalMold , :ARTWORK_78_Modeling , :ARTWORK_77_HeatingMetalMold , :ARTWORK_77_Glassblowing , :ARTWORK_78_SetupAndTestingOfTheMetalMold_2 , :ARTWORK_78_SetupAndTestingOfTheMetalMold , :ARTWORK_73_HeatingMetalMold , :ARTWORK_79_SetupAndTestingOfTheMetalMold , :ARTWORK_74_SetupAndTestingOfTheMetalMold , :ARTWORK_77_Modeling , :ARTWORK_44_Glassblowing , :ARTWORK_76_SetupAndTestingOfTheMetalMold , :ARTWORK_75_Modeling , :ARTWORK_73_SetupAndTestingOfTheMetalMold , :ARTWORK_77_SetupAndTestingOfTheMetalMold_2 , :ARTWORK_79_SetupAndTestingOfTheMetalMold_2 , :ARTWORK_80_SetupAndTestingOfTheMetalMold_2 , :ARTWORK_78_Glassblowing , :ARTWORK_44_SetupAndTestingOfTheMetalMold , :ARTWORK_79_Glassblowing , :ARTWORK_80_HeatingMetalMold , :ARTWORK_75_SetupAndTestingOfTheMetalMold , :ARTWORK_43_Modeling , :ARTWORK_43_SetupAndTestingOfTheMetalMold_2 , :ARTWORK_80_Modeling , :ARTWORK_76_Glassblowing , :ARTWORK_76_HeatingMetalMold , :ARTWORK_78_HeatingMetalMold , :ARTWORK_44_Modeling , :ARTWORK_44_HeatingMetalMold , :ARTWORK_75_SetupAndTestingOfTheMetalMold_2 , :ARTWORK_43_HeatingMetalMold , :ARTWORK_74_SetupAndTestingOfTheMetalMold_2 , :ARTWORK_75_HeatingMetalMold , :ARTWORK_73_Modeling , :ARTWORK_80_SetupAndTestingOfTheMetalMold , :ARTWORK_75_Glassblowing , :ARTWORK_74_HeatingMetalMold , :ARTWORK_80_Glassblowing , :ARTWORK_74_Modeling , :ARTWORK_73_Glassblowing , :ARTWORK_76_Modeling , :ARTWORK_74_Glassblowing .

<http://www.cidoc-crm.org/cidoc-crm/E52_Time-Span>
        a                    owl:Class ;
        owl:equivalentClass  :Timespan .

:CollectionGlasmuseumLette
        a               :Collection , owl:NamedIndividual ;
        rdfs:comment    "Collection maintained by the Glasmuseum Lette."@en ;
        rdfs:label      "Collection Glasmuseum Lette"@en ;
        :Consists-Of    :Artwork_43 ;
        :Located-In     :Coesfeld ;
        :Maintained-By  :GlasmuseumLette .

:ARTWORK_73_MeasuringAndBoxesMaking
        a              owl:NamedIndividual , :Measuring_and_Boxes_Making ;
        rdfs:comment   "Instance of an activity which is part of the creation process of ARTWORK_73."@en ;
        rdfs:label     "ARTWORK_73_Measuring and Boxes Making"@en ;
        :Followed-By   :ARTWORK_73_Packing_2 ;
        :Follows       <http://www.semanticweb.org/ontologies/Daan/2020/BarbaraNanning#ARTWORK_73_ExaminingQuality(Result)> ;
        :Has-Duration  <http://www.semanticweb.org/ontologies/Daan/2020/BarbaraNanning#2018> ;
        :Involves      :AlešZvěřina , :BarbaraNanning ;
        :Located-In    :CzechRepublic ;
        :Part-Of       :Creation_Artwork_73 .

:ARTWORK_80_Transporting_2
        a              :Transporting , owl:NamedIndividual ;
        rdfs:comment   "Instance of an activity which is part of the creation process of ARTWORK_80."@en ;
        rdfs:label     "ARTWORK_80_Transporting_2"@en ;
        :Followed-By   :ARTWORK_80_Sandblasting ;
        :Follows       :ARTWORK_80_Packing_2 ;
        :Has-Duration  <http://www.semanticweb.org/ontologies/Daan/2020/BarbaraNanning#2018> ;
        :Involves      :AlešZvěřina , :BarbaraNanning ;
        :Located-In    :CzechRepublic ;
        :Part-Of       :Creation_Artwork_80 .

:ARTWORK_18_64_Glassblowing
        a                 owl:NamedIndividual , :Glassblowing ;
        rdfs:comment      "Instance of an activity which is part of the creation process of ARTWORK_18_64."@en ;
        rdfs:label        "ARTWORK_18_64_Glassblowing"@en ;
        :Followed-By      :ARTWORK_18_64_Sensing ;
        :Follows          :ARTWORK_18_64_PickingUpColouredCanesPattern ;
        :Has-Duration     <http://www.semanticweb.org/ontologies/Daan/2020/BarbaraNanning#2015> ;
        :Involves         :BarbaraNanning , <http://www.semanticweb.org/ontologies/Daan/2020/BarbaraNanning#MiaLerssi(DN)> , <http://www.semanticweb.org/ontologies/Daan/2020/BarbaraNanning#JessicaHomich(USA)> , <http://www.semanticweb.org/ontologies/Daan/2020/BarbaraNanning#MarekEffmert(CZ)> , <http://www.semanticweb.org/ontologies/Daan/2020/BarbaraNanning#RobertLenner(CZ)> , :GertBullée , <http://www.semanticweb.org/ontologies/Daan/2020/BarbaraNanning#MarekBrathko(CZ)> ;
        :Located-In       :Zaandam ;
        :Part-Of          :Creation_Artwork_18_64 ;
        :Requires-Use-Of  :Blocks , :Tagliol , :IcePick , :Fork , :PropaneTorch , :YokeOfSupport , :CeramicPotFilledWithGlass , :Pincet , :Beeswax , :StraightShears , :Hook , :Water , :DiamondShears , :Pontis , :BlowingPipe , :Furnace , :AnnealingKiln , :GloryHole , :BitIron , :AirCompressor , :InterchangeableMetalMoldSetup , :Gloves , :Jacks , :Paper , :Marver .

:Artwork_36  a        :Glass_Artwork , owl:NamedIndividual ;
        rdfs:comment  "Artwork_36 is a glass artwork made by Barbara Nanning."@en ;
        rdfs:label    "Coloured Shadows Beneath the Water"@en ;
        :Created-By   :Creation_Artwork_36 ;
        :Has-Depth    "27"^^xsd:decimal ;
        :Has-Height   "27"^^xsd:decimal , "11"^^xsd:decimal ;
        :Is-Unica     "Yes"@en ;
        :Made-By      <http://www.semanticweb.org/ontologies/Daan/2020/BarbaraNanning#Ale%C5%A1Zv%C4%9B%C5%99ina&AZ-Design> , :VRIJGLASZaandam , :BullseyeGlassSplinterEnDeVosch , :BarbaraNanning , <http://www.semanticweb.org/ontologies/Daan/2020/BarbaraNanning#Ji%C5%99%C3%ADPa%C4%8DinekLindava(CZ)> ;
        :Made-Out-Of  :ARTWORK_36_Peacock , :BullseyeGlass ;
        :Shown-By     :Image_Artwork_36 .

:ARTWORK_78_Packing_3
        a              :Packing , owl:NamedIndividual ;
        rdfs:comment   "Instance of an activity which is part of the creation process of ARTWORK_78."@en ;
        rdfs:label     "ARTWORK_78_Packing_3"@en ;
        :Followed-By   :ARTWORK_78_Transporting_3 ;
        :Follows       :ARTWORK_78_Signing ;
        :Has-Duration  <http://www.semanticweb.org/ontologies/Daan/2020/BarbaraNanning#2008> ;
        :Involves      :BarbaraNanning , :AlešZvěřina ;
        :Located-In    :CzechRepublic ;
        :Part-Of       :Creation_Artwork_78 .

:Producing_Coloured_Canes
        a                owl:Class ;
        rdfs:comment     "Coloured glass is picked up by a glassblower, heated and then attached to a second pipe. It can then be pulled into the appropriate length and thickness. With my team of glass blowers I stretch the long glass threads with their own drawing and variety. Irregularity, asymmetry and variation in dimension evoke the image of cell division in nature. Then, the meters long glass threads are cut and sawn into 1-2 cm length."@en ;
        rdfs:label       "Producing Coloured Canes"@en ;
        rdfs:subClassOf  :Activity .

<>      a             owl:Ontology ;
        rdfs:comment  "An ontology related to the works of Barbara Nanning and the corresponding creation Processes."@en .

:ARTWORK_77_Polishing
        a                 owl:NamedIndividual , :Polishing ;
        rdfs:comment      "Instance of an activity which is part of the creation process of ARTWORK_77."@en ;
        rdfs:label        "ARTWORK_77_Polishing"@en ;
        :Followed-By      <http://www.semanticweb.org/ontologies/Daan/2020/BarbaraNanning#ARTWORK_77_ExaminingQuality(Result)> ;
        :Follows          :ARTWORK_77_Grinding ;
        :Has-Duration     <http://www.semanticweb.org/ontologies/Daan/2020/BarbaraNanning#2018> ;
        :Involves         :LukášSvoboda , :AlešZvěřina , :BarbaraNanning ;
        :Located-In       :CzechRepublic ;
        :Part-Of          :Creation_Artwork_77 ;
        :Requires-Use-Of  :PolishingStone .

:LukášSvoboda  a      :Grinder_2 , owl:NamedIndividual ;
        rdfs:comment  "Lukáš Svoboda is a Grinder 2."@en ;
        rdfs:label    "Lukáš Svoboda"@en ;
        :Involved-In  :ARTWORK_44_Polishing , :ARTWORK_80_Polishing , :ARTWORK_76_Polishing , :ARTWORK_75_Polishing , :ARTWORK_79_Sensing , :ARTWORK_76_Sensing , :ARTWORK_78_Polishing , :ARTWORK_74_Polishing , :ARTWORK_75_Sensing , :ARTWORK_43_Polishing , :ARTWORK_74_Sensing , :ARTWORK_77_Polishing , :ARTWORK_73_Polishing , :ARTWORK_44_Sensing , :ARTWORK_73_Sensing , :ARTWORK_80_Sensing , :ARTWORK_43_Sensing , :ARTWORK_79_Polishing , :ARTWORK_78_Sensing , :ARTWORK_77_Sensing ;
        :Works-For    <http://www.semanticweb.org/ontologies/Daan/2020/BarbaraNanning#Ale%C5%A1Zv%C4%9B%C5%99ina&AZ-Design> .

:Applying_Massive_Piece_of_Clear_Glass
        a                owl:Class ;
        rdfs:comment     "Also known as Bringing a Bit. This is an additional piece of glass that is gathered and brought to the glassblower to apply to the existing piece."@en ;
        rdfs:label       "Applying Massive Piece of Clear Glass"@en ;
        rdfs:subClassOf  :Activity .

:ARTWORK_77_Cooling  a    owl:NamedIndividual , :Cooling ;
        rdfs:comment      "Instance of an activity which is part of the creation process of ARTWORK_77."@en ;
        rdfs:label        "ARTWORK_77_Cooling"@en ;
        :Followed-By      :ARTWORK_77_Packing ;
        :Follows          :ARTWORK_77_Translocating ;
        :Has-Duration     <http://www.semanticweb.org/ontologies/Daan/2020/BarbaraNanning#2018> ;
        :Involves         :AssistantOfBarbara , :LuděkKout ;
        :Located-In       :CzechRepublic ;
        :Part-Of          :Creation_Artwork_77 ;
        :Requires-Use-Of  :AnnealingKiln .

:ARTWORK_43_Photographing
        a              owl:NamedIndividual , :Photographing ;
        rdfs:comment   "Instance of an activity which is part of the creation process of ARTWORK_43."@en ;
        rdfs:label     "ARTWORK_43_Photographing"@en ;
        :Followed-By   :ARTWORK_43_Documenting ;
        :Follows       :ARTWORK_43_Transporting_4 ;
        :Has-Duration  <http://www.semanticweb.org/ontologies/Daan/2020/BarbaraNanning#2008> ;
        :Involves      :BarbaraNanning , <http://www.semanticweb.org/ontologies/Daan/2020/BarbaraNanning#TomHaartsen_Ouderkerka/dAmstel(NL)> ;
        :Located-In    :CzechRepublic ;
        :Part-Of       :Creation_Artwork_43 .

<http://vocab.getty.edu/aat/300033537>
        a           owl:NamedIndividual ;
        owl:sameAs  :Hook .

<http://www.semanticweb.org/ontologies/Daan/2020/BarbaraNanning#2008>
        a             owl:NamedIndividual , :Timespan ;
        rdfs:comment  "2008 is a Timespan."@en ;
        rdfs:label    "2008"@en ;
        owl:sameAs    <http://www.wikidata.org/entity/Q2004> ;
        :Duration-Of  :Creation_Artwork_74 , :Creation_Artwork_43 .

:ARTWORK_18_64_CuttingAndPolishingColouredCanes
        a                 owl:NamedIndividual , :Cutting_and_Polishing_Coloured_Canes ;
        rdfs:comment      "Instance of an activity which is part of the creation process of ARTWORK_18_64."@en ;
        rdfs:label        "ARTWORK_18_64_Cutting and Polishing Coloured Canes"@en ;
        :Followed-By      :ARTWORK_18_64_TransportingColouredCanes_2 ;
        :Follows          :ARTWORK_18_64_TransportingColouredCanes ;
        :Has-Duration     <http://www.semanticweb.org/ontologies/Daan/2020/BarbaraNanning#2015> ;
        :Involves         :RobertFlorian , :BarbaraNanning , :AlešZvěřina ;
        :Located-In       :NovyBor ;
        :Part-Of          :Creation_Artwork_18_64 ;
        :Requires-Use-Of  :Glassscissors , :DiamondSaw , :Water , :SharpeningStone .

:Creation_Artwork_79  a  :Creation_Event , owl:NamedIndividual ;
        rdfs:comment    "Creation event for an artwork by Barbara Nanning displayed in \"Barbara Nanning Eeuwige Beweging\" by Eliens (2019)."@en ;
        rdfs:label      "Creation_Artwork_79"@en ;
        :Consists-Of    :ARTWORK_79_Documenting , :ARTWORK_79_Transporting_4 , :ARTWORK_79_Packing_3 , <http://www.semanticweb.org/ontologies/Daan/2020/BarbaraNanning#ARTWORK_79_ExaminingQuality(Result)> , :ARTWORK_79_Gilding , :ARTWORK_79_Transporting_3 , <http://www.semanticweb.org/ontologies/Daan/2020/BarbaraNanning#ARTWORK_79_ExaminingQuality(CheckForIrregularitiesInTheGlass)> , :ARTWORK_79_Grinding , :ARTWORK_79_SetupAndTestingOfTheMetalMold_2 , :ARTWORK_79_Signing , :ARTWORK_79_Sensing , :ARTWORK_79_ExaminingTheQualityOfTheGlass , :ARTWORK_79_Modeling , :ARTWORK_79_SetupAndTestingOfTheMetalMold , :ARTWORK_79_Sawing , :ARTWORK_79_Transporting_2 , :ARTWORK_79_Packing_2 , <http://www.semanticweb.org/ontologies/Daan/2020/BarbaraNanning#ARTWORK_79_ExaminingQuality(FinalResult)> , :ARTWORK_79_Resting , :ARTWORK_79_ApplyingClearGlassBell , :ARTWORK_79_Transporting , :ARTWORK_79_Glassblowing , :ARTWORK_79_ApplyingExtraColour_2 , <http://www.semanticweb.org/ontologies/Daan/2020/BarbaraNanning#ARTWORK_79_ExaminingQuality(Shape/Form)> , :ARTWORK_79_Packing_5 , :ARTWORK_79_MeasuringAndBoxesMaking , :ARTWORK_79_Polishing , :ARTWORK_79_Packing , :ARTWORK_79_Photographing , :ARTWORK_79_Cooling , :ARTWORK_79_Translocating , :ARTWORK_79_Packing_4 , :ARTWORK_79_HeatingMetalMold , :ARTWORK_79_PreparingGlass , :ARTWORK_79_ApplyingExtraColour ;
        :Created        :Artwork_79 ;
        :Finishes-With  :ARTWORK_79_Packing_5 ;
        :Has-Duration   <http://www.semanticweb.org/ontologies/Daan/2020/BarbaraNanning#2018> ;
        :Located-In     :CzechRepublic ;
        :Starts-With    :ARTWORK_79_PreparingGlass ;
        :Within-Period  :GlassVerreÉglomisé .

:ARTWORK_36_HeatingMetalMold
        a                 owl:NamedIndividual , :Heating_Metal_Mold ;
        rdfs:comment      "Instance of an activity which is part of the creation process of ARTWORK_36."@en ;
        rdfs:label        "ARTWORK_36_Heating Metal Mold"@en ;
        :Followed-By      :ARTWORK_36_Glassblowing ;
        :Follows          :ARTWORK_36_PickingUpColouredCanesPattern ;
        :Has-Duration     <http://www.semanticweb.org/ontologies/Daan/2020/BarbaraNanning#2015> ;
        :Involves         :BarbaraNanning ;
        :Located-In       :Zaandam ;
        :Part-Of          :Creation_Artwork_36 ;
        :Requires-Use-Of  :InterchangeableMetalMoldSetup , :PropaneTorch , :Gloves .

<http://www.semanticweb.org/ontologies/Daan/2020/BarbaraNanning#ARTWORK_39_ExaminingQuality(Shape/Form)>
        a                 j.2: , owl:NamedIndividual ;
        rdfs:comment      "Instance of an activity which is part of the creation process of ARTWORK_39."@en ;
        rdfs:label        "ARTWORK_39_Examining Quality (Shape/Form)"@en ;
        :Followed-By      :ARTWORK_39_Cooling ;
        :Follows          :ARTWORK_39_Modeling ;
        :Has-Duration     <http://www.semanticweb.org/ontologies/Daan/2020/BarbaraNanning#2015> ;
        :Involves         :BarbaraNanning , :DurkValkema , <http://www.semanticweb.org/ontologies/Daan/2020/BarbaraNanning#MiaLerssi(DN)> , :GertBullée ;
        :Located-In       :Zaandam ;
        :Part-Of          :Creation_Artwork_39 ;
        :Requires-Use-Of  :Pontis , :BlowingPipe , :GloryHole .

:ARTWORK_78_PreparingGlass
        a                 owl:NamedIndividual , :Preparing_Glass ;
        rdfs:comment      "Instance of an activity which is part of the creation process of ARTWORK_78."@en ;
        rdfs:label        "ARTWORK_78_Preparing Glass"@en ;
        :Followed-By      :ARTWORK_78_SetupAndTestingOfTheMetalMold ;
        :Has-Duration     <http://www.semanticweb.org/ontologies/Daan/2020/BarbaraNanning#2008> ;
        :Involves         <http://www.semanticweb.org/ontologies/Daan/2020/BarbaraNanning#AlesVacek(CZ)> , :BarbaraNanning ;
        :Located-In       :CzechRepublic ;
        :Part-Of          :Creation_Artwork_78 ;
        :Requires-Use-Of  :Garage , :Pontis , :BlowingPipe , :Marver , :GloryHole ;
        :Starts           :Creation_Artwork_78 .

:ARTWORK_18_64_CuttingAndPolishingCastedMonochromeSheetsToSmallRods
        a                 :Cutting_and_Polishing_Casted_Monochrome_Sheets_to_Small_Rods , owl:NamedIndividual ;
        rdfs:comment      "Instance of an activity which is part of the creation process of ARTWORK_18_64."@en ;
        rdfs:label        "ARTWORK_18_64_Cutting and Polishing Casted Monochrome Sheets to Small Rods"@en ;
        :Followed-By      :ARTWORK_18_64_DecidingColourPaletteAndPatterns_2 ;
        :Follows          :ARTWORK_18_64_Casting ;
        :Has-Duration     <http://www.semanticweb.org/ontologies/Daan/2020/BarbaraNanning#2015> ;
        :Involves         :BarbaraNanning ;
        :Located-In       :Amsterdam ;
        :Part-Of          :Creation_Artwork_18_64 ;
        :Requires-Use-Of  :SharpeningStone , :DiamondSaw , :Water .

:ARTWORK_79_Transporting_2
        a              :Transporting , owl:NamedIndividual ;
        rdfs:comment   "Instance of an activity which is part of the creation process of ARTWORK_79."@en ;
        rdfs:label     "ARTWORK_79_Transporting_2"@en ;
        :Followed-By   :ARTWORK_79_Signing ;
        :Follows       :ARTWORK_79_Packing_2 ;
        :Has-Duration  <http://www.semanticweb.org/ontologies/Daan/2020/BarbaraNanning#2018> ;
        :Involves      :AlešZvěřina , :BarbaraNanning ;
        :Located-In    :CzechRepublic ;
        :Part-Of       :Creation_Artwork_79 .

<http://www.wikidata.org/entity/Q169031>
        a       owl:NamedIndividual .

:ARTWORK_17_33_Transporting_2
        a              owl:NamedIndividual , :Transporting ;
        rdfs:comment   "Instance of an activity which is part of the creation process of ARTWORK_17_33."@en ;
        rdfs:label     "ARTWORK_17_33_Transporting_2"@en ;
        :Followed-By   :ARTWORK_17_33_Photographing ;
        :Follows       :ARTWORK_17_33_Packing_2 ;
        :Has-Duration  <http://www.semanticweb.org/ontologies/Daan/2020/BarbaraNanning#2017> ;
        :Involves      :BarbaraNanning , :AlešZvěřina ;
        :Located-In    :Amsterdam ;
        :Part-Of       :Creation_Artwork_17_33 .

:LuděkKout  a         :Supervisor_Works , owl:NamedIndividual ;
        rdfs:comment  "Luděk Kout is a Supervisor Works."@en ;
        rdfs:label    "Luděk Kout"@en ;
        :Involved-In  :ARTWORK_43_Cooling , :ARTWORK_77_Cooling , <http://www.semanticweb.org/ontologies/Daan/2020/BarbaraNanning#ARTWORK_73_ExaminingQuality(Shape/Form)> , :ARTWORK_43_ExaminingTheQualityOfTheGlass , :ARTWORK_75_Cooling , :ARTWORK_44_ExaminingTheQualityOfTheGlass , :ARTWORK_76_Cooling , :ARTWORK_79_ExaminingTheQualityOfTheGlass , <http://www.semanticweb.org/ontologies/Daan/2020/BarbaraNanning#ARTWORK_79_ExaminingQuality(Shape/Form)> , :ARTWORK_74_Cooling , <http://www.semanticweb.org/ontologies/Daan/2020/BarbaraNanning#ARTWORK_76_ExaminingQuality(Shape/Form)> , <http://www.semanticweb.org/ontologies/Daan/2020/BarbaraNanning#ARTWORK_43_ExaminingQuality(Shape/Form)> , :ARTWORK_73_ExaminingTheQualityOfTheGlass , :ARTWORK_77_ExaminingTheQualityOfTheGlass , :ARTWORK_79_Cooling , :ARTWORK_74_ExaminingTheQualityOfTheGlass , <http://www.semanticweb.org/ontologies/Daan/2020/BarbaraNanning#ARTWORK_77_ExaminingQuality(Shape/Form)> , :ARTWORK_75_ExaminingTheQualityOfTheGlass , <http://www.semanticweb.org/ontologies/Daan/2020/BarbaraNanning#ARTWORK_75_ExaminingQuality(Shape/Form)> , :ARTWORK_80_ExaminingTheQualityOfTheGlass , :ARTWORK_73_Cooling , :ARTWORK_44_Cooling , <http://www.semanticweb.org/ontologies/Daan/2020/BarbaraNanning#ARTWORK_44_ExaminingQuality(Shape/Form)> , <http://www.semanticweb.org/ontologies/Daan/2020/BarbaraNanning#ARTWORK_80_ExaminingQuality(Shape/Form)> , :ARTWORK_78_Cooling , <http://www.semanticweb.org/ontologies/Daan/2020/BarbaraNanning#ARTWORK_74_ExaminingQuality(Shape/Form)> , <http://www.semanticweb.org/ontologies/Daan/2020/BarbaraNanning#ARTWORK_78_ExaminingQuality(Shape/Form)> , :ARTWORK_78_ExaminingTheQualityOfTheGlass , :ARTWORK_80_Cooling , :ARTWORK_76_ExaminingTheQualityOfTheGlass ;
        :Works-For    :LASVITAJETO .

<http://www.semanticweb.org/ontologies/Daan/2020/BarbaraNanning#ARTWORK_46_ExaminingQuality(Result)>
        a              j.0: , owl:NamedIndividual ;
        rdfs:comment   "Instance of an activity which is part of the creation process of ARTWORK_46."@en ;
        rdfs:label     "ARTWORK_46_Examining Quality (Result)"@en ;
        :Followed-By   :ARTWORK_46_MeasuringAndBoxesMaking ;
        :Follows       :ARTWORK_46_Signing ;
        :Has-Duration  <http://www.semanticweb.org/ontologies/Daan/2020/BarbaraNanning#2018> ;
        :Involves      :BarbaraNanning , :AlešZvěřina ;
        :Located-In    :NovyBor ;
        :Part-Of       :Creation_Artwork_46 .

:ARTWORK_36_PreparingGlass_2
        a                 owl:NamedIndividual , :Preparing_Glass ;
        rdfs:comment      "Instance of an activity which is part of the creation process of ARTWORK_36." ;
        rdfs:label        "ARTWORK_36 Preparing Glass_2" ;
        :Followed-By      :ARTWORK_36_ExaminingTheQualityOfTheGlass_2 ;
        :Follows          :ARTWORK_36_FillingKilnsWithMetalBowl_2 ;
        :Has-Duration     <http://www.semanticweb.org/ontologies/Daan/2020/BarbaraNanning#2019> ;
        :Involves         <http://www.semanticweb.org/ontologies/Daan/2020/BarbaraNanning#JiriPacinek(CZ)> , :BarbaraNanning ;
        :Located-In       :Lindava ;
        :Part-Of          :Creation_Artwork_36 ;
        :Requires-Use-Of  :Pontis , :BlowingPipe , :GloryHole , :Marver , :Garage .

:ARTWORK_18_64_CuttingSheets
        a                 :Cutting_Sheets , owl:NamedIndividual ;
        rdfs:comment      "Instance of an activity which is part of the creation process of ARTWORK_18_64."@en ;
        rdfs:label        "ARTWORK_18_64_Cutting Sheets"@en ;
        :Followed-By      :ARTWORK_18_64_OrdeningFlatSheets ;
        :Follows          :ARTWORK_18_64_DecidingColourPaletteAndPatterns_3 ;
        :Has-Duration     <http://www.semanticweb.org/ontologies/Daan/2020/BarbaraNanning#2015> ;
        :Involves         <http://www.semanticweb.org/ontologies/Daan/2020/BarbaraNanning#FredStikvoort(NL)> , <http://www.semanticweb.org/ontologies/Daan/2020/BarbaraNanning#AbHylkema(NL)> , :BarbaraNanning ;
        :Located-In       :Amsterdam ;
        :Part-Of          :Creation_Artwork_18_64 ;
        :Requires-Use-Of  :Water , :DiamondSaw , :SharpeningStone .

<http://vocab.getty.edu/aat/300025268>
        a                    owl:Class ;
        owl:equivalentClass  :Grinder .

<http://www.cidoc-crm.org/cidoc-crm/P116_is_started_by>
        a                       owl:ObjectProperty ;
        owl:equivalentProperty  :Starts-With .

<http://vocab.getty.edu/aat/300053031>
        a                    owl:Class ;
        owl:equivalentClass  :Sandblasting .

<http://www.semanticweb.org/ontologies/Daan/2020/BarbaraNanning#ARTWORK_17_33_ExaminingQuality(CheckForIrregularitiesInTheGlass)>
        a              j.3: , owl:NamedIndividual ;
        rdfs:comment   "Instance of an activity which is part of the creation process of ARTWORK_17_33."@en ;
        rdfs:label     "ARTWORK_17_33_Examining Quality (Check for Irregularities in the Glass)"@en ;
        :Followed-By   :ARTWORK_17_33_Sawing ;
        :Follows       :ARTWORK_17_33_Resting ;
        :Has-Duration  <http://www.semanticweb.org/ontologies/Daan/2020/BarbaraNanning#2017> ;
        :Involves      :BarbaraNanning , :AlešZvěřina ;
        :Located-In    :NovyBor ;
        :Part-Of       :Creation_Artwork_17_33 .

:ARTWORK_77_Resting  a    :Resting , owl:NamedIndividual ;
        rdfs:comment      "Instance of an activity which is part of the creation process of ARTWORK_77."@en ;
        rdfs:label        "ARTWORK_77_Resting"@en ;
        :Followed-By      <http://www.semanticweb.org/ontologies/Daan/2020/BarbaraNanning#ARTWORK_77_ExaminingQuality(CheckForIrregularitiesInTheGlass)> ;
        :Follows          :ARTWORK_77_Transporting ;
        :Has-Duration     <http://www.semanticweb.org/ontologies/Daan/2020/BarbaraNanning#2018> ;
        :Involves         :AlešZvěřina ;
        :Located-In       :CzechRepublic ;
        :Part-Of          :Creation_Artwork_77 ;
        :Requires-Use-Of  :AnnealingKiln .

:ARTWORK_80_ApplyingClearGlassBell
        a                 :Applying_Clear_Glass_Bell , owl:NamedIndividual ;
        rdfs:comment      "Instance of an activity which is part of the creation process of ARTWORK_80."@en ;
        rdfs:label        "ARTWORK_80_Applying Clear Glass Bell"@en ;
        :Followed-By      :ARTWORK_80_ApplyingExtraColour ;
        :Follows          :ARTWORK_80_SetupAndTestingOfTheMetalMold_2 ;
        :Has-Duration     <http://www.semanticweb.org/ontologies/Daan/2020/BarbaraNanning#2018> ;
        :Involves         :BarbaraNanning , <http://www.semanticweb.org/ontologies/Daan/2020/BarbaraNanning#RadekKoten(CZ)> , <http://www.semanticweb.org/ontologies/Daan/2020/BarbaraNanning#LukasHavlas(CZ)> ;
        :Located-In       :CzechRepublic ;
        :Part-Of          :Creation_Artwork_80 ;
        :Processes        :AJETOClearGlass ;
        :Requires-Use-Of  :Hook , :Blocks , :Marver , :Pincet , :DiamondShears , :Paper , :StraightShears , :YokeOfSupport , :AirCompressor , :Beeswax , :BlowingPipe , :Jacks , :Furnace , :IcePick , :Water , :CeramicPotFilledWithGlass .

:NovyBor  a           :City , owl:NamedIndividual ;
        rdfs:comment  "Novy Bor is a city in Czech Republic."@en ;
        rdfs:label    "Novy Bor"@en ;
        owl:sameAs    <http://www.wikidata.org/entity/Q1000086> ;
        :Located-In   :CzechRepublic ;
        :Location-Of  <http://www.semanticweb.org/ontologies/Daan/2020/BarbaraNanning#Ale%C5%A1Zv%C4%9B%C5%99ina&AZ-Design> .

:ARTWORK_39_Sensing  a  :Sensing , owl:NamedIndividual ;
        rdfs:comment   "Instance of an activity which is part of the creation process of ARTWORK_39."@en ;
        rdfs:label     "ARTWORK_39_Sensing"@en ;
        :Followed-By   :ARTWORK_39_Modeling ;
        :Follows       :ARTWORK_39_Glassblowing ;
        :Has-Duration  <http://www.semanticweb.org/ontologies/Daan/2020/BarbaraNanning#2015> ;
        :Involves      :BarbaraNanning ;
        :Located-In    :Zaandam ;
        :Part-Of       :Creation_Artwork_39 .

:Processes  a         owl:ObjectProperty ;
        rdfs:comment  "Processes connects a material with an activity in which the material is (being) processed."@en ;
        rdfs:domain   :Activity ;
        rdfs:label    "Processes"@en ;
        rdfs:range    :Material .

<http://www.semanticweb.org/ontologies/Daan/2020/BarbaraNanning#ARTWORK_77_ExaminingQuality(Shape/Form)>
        a                 owl:NamedIndividual , j.2: ;
        rdfs:comment      "Instance of an activity which is part of the creation process of ARTWORK_77."@en ;
        rdfs:label        "ARTWORK_77_Examining Quality (Shape/Form)"@en ;
        :Followed-By      :ARTWORK_77_Translocating ;
        :Follows          :ARTWORK_77_Modeling ;
        :Has-Duration     <http://www.semanticweb.org/ontologies/Daan/2020/BarbaraNanning#2018> ;
        :Involves         :BarbaraNanning , <http://www.semanticweb.org/ontologies/Daan/2020/BarbaraNanning#RadekKoten(CZ)> , :LuděkKout ;
        :Located-In       :CzechRepublic ;
        :Part-Of          :Creation_Artwork_77 ;
        :Requires-Use-Of  :GloryHole , :Pontis , :BlowingPipe .

:Rounding_by_Grinding_the_Sheet
        a                owl:Class ;
        rdfs:comment     "Using a grind- and polishstone the cutter applies a small edge to shape and remove the sharp edges of the glass."@en ;
        rdfs:label       "Rounding by Grinding the Sheet"@en ;
        rdfs:subClassOf  :Activity .

:ARTWORK_73_Packing_3
        a              owl:NamedIndividual , :Packing ;
        rdfs:comment   "Instance of an activity which is part of the creation process of ARTWORK_73."@en ;
        rdfs:label     "ARTWORK_73_Packing_3"@en ;
        :Followed-By   :ARTWORK_73_Transporting_3 ;
        :Follows       :ARTWORK_73_Signing ;
        :Has-Duration  <http://www.semanticweb.org/ontologies/Daan/2020/BarbaraNanning#2018> ;
        :Involves      :BarbaraNanning , :AlešZvěřina ;
        :Located-In    :CzechRepublic ;
        :Part-Of       :Creation_Artwork_73 .

:ARTWORK_75_Modeling  a   :Modeling , owl:NamedIndividual ;
        rdfs:comment      "Instance of an activity which is part of the creation process of ARTWORK_75."@en ;
        rdfs:label        "ARTWORK_75_Modeling"@en ;
        :Followed-By      <http://www.semanticweb.org/ontologies/Daan/2020/BarbaraNanning#ARTWORK_75_ExaminingQuality(Shape/Form)> ;
        :Follows          :ARTWORK_75_Sensing ;
        :Has-Duration     <http://www.semanticweb.org/ontologies/Daan/2020/BarbaraNanning#2018> ;
        :Involves         :AssistantOfBarbara , <http://www.semanticweb.org/ontologies/Daan/2020/BarbaraNanning#Tom%C3%A1%C5%A1Moravec(CZ)> , <http://www.semanticweb.org/ontologies/Daan/2020/BarbaraNanning#LukasHavlas(CZ)> , <http://www.semanticweb.org/ontologies/Daan/2020/BarbaraNanning#JiriMoravec(CZ)> , <http://www.semanticweb.org/ontologies/Daan/2020/BarbaraNanning#RadekKoten(CZ)> , :BarbaraNanning ;
        :Located-In       :CzechRepublic ;
        :Part-Of          :Creation_Artwork_75 ;
        :Requires-Use-Of  :PropaneTorch , :BlowingPipe , :Gloves , :AirCompressor , :InterchangeableMetalMoldSetup .

j.1:    a                owl:Class ;
        rdfs:comment     "Examining Quality (Final Result) is an activity conducted by a creator in which the quality of a finished thing is assured."@en ;
        rdfs:label       "Examining Quality (Final Result)"@en ;
        rdfs:subClassOf  :Activity .

<http://www.wikidata.org/entity/Q11472>
        a       owl:NamedIndividual .

:ARTWORK_18_64_Casting
        a                 :Casting , owl:NamedIndividual ;
        rdfs:comment      "Instance of an activity which is part of the creation process of ARTWORK_18_64."@en ;
        rdfs:label        "ARTWORK_18_64_Casting"@en ;
        :Followed-By      :ARTWORK_18_64_CuttingAndPolishingCastedMonochromeSheetsToSmallRods ;
        :Follows          :ARTWORK_18_64_Ordening ;
        :Has-Duration     <http://www.semanticweb.org/ontologies/Daan/2020/BarbaraNanning#2015> ;
        :Involves         :BarbaraNanning , :SteefHendriks ;
        :Located-In       :Langweer ;
        :Part-Of          :Creation_Artwork_18_64 ;
        :Requires-Use-Of  :FusingKiln , :Pincet , :Gloves , :Furnace .

:ARTWORK_43_Grinding  a   owl:NamedIndividual , :Grinding ;
        rdfs:comment      "Instance of an activity which is part of the creation process of ARTWORK_43."@en ;
        rdfs:label        "ARTWORK_43_Grinding"@en ;
        :Followed-By      :ARTWORK_43_Polishing ;
        :Follows          :ARTWORK_43_Sawing ;
        :Has-Duration     <http://www.semanticweb.org/ontologies/Daan/2020/BarbaraNanning#2008> ;
        :Involves         :RobertFlorian , :BarbaraNanning , :AlešZvěřina ;
        :Located-In       :CzechRepublic ;
        :Part-Of          :Creation_Artwork_43 ;
        :Requires-Use-Of  :GrindingWheel , :SharpeningStone .

:ARTWORK_80_Transporting
        a              owl:NamedIndividual , :Transporting ;
        rdfs:comment   "Instance of an activity which is part of the creation process of ARTWORK_80."@en ;
        rdfs:label     "ARTWORK_80_Transporting"@en ;
        :Followed-By   :ARTWORK_80_Resting ;
        :Follows       :ARTWORK_80_Packing ;
        :Has-Duration  <http://www.semanticweb.org/ontologies/Daan/2020/BarbaraNanning#2018> ;
        :Involves      :AlešZvěřina , :BarbaraNanning ;
        :Located-In    :CzechRepublic ;
        :Part-Of       :Creation_Artwork_80 .

:ARTWORK_36_TransportingColouredCanes
        a              :Transporting_Coloured_Canes , owl:NamedIndividual ;
        rdfs:comment   "Instance of an activity which is part of the creation process of ARTWORK_36."@en ;
        rdfs:label     "ARTWORK_36_Transporting Coloured Canes"@en ;
        :Followed-By   :ARTWORK_36_CuttingAndPolishingColouredCanes ;
        :Follows       :ARTWORK_36_ProducingColouredCanes ;
        :Has-Duration  <http://www.semanticweb.org/ontologies/Daan/2020/BarbaraNanning#2015> ;
        :Involves      :BarbaraNanning ;
        :Located-In    :Zaandam ;
        :Part-Of       :Creation_Artwork_36 .

:ARTWORK_75_ApplyingExtraColour_2
        a                 owl:NamedIndividual , :Applying_Extra_Colour ;
        rdfs:comment      "Instance of an activity which is part of the creation process of ARTWORK_75."@en ;
        rdfs:label        "ARTWORK_75_Applying Extra Colour_2"@en ;
        :Followed-By      :ARTWORK_75_HeatingMetalMold ;
        :Follows          :ARTWORK_75_ApplyingExtraColour ;
        :Has-Duration     <http://www.semanticweb.org/ontologies/Daan/2020/BarbaraNanning#2017> ;
        :Involves         <http://www.semanticweb.org/ontologies/Daan/2020/BarbaraNanning#RadekKoten(CZ)> , <http://www.semanticweb.org/ontologies/Daan/2020/BarbaraNanning#LukasHavlas(CZ)> , :BarbaraNanning ;
        :Located-In       :CzechRepublic ;
        :Part-Of          :Creation_Artwork_75 ;
        :Processes        :AJETOAlexandriteGlass ;
        :Requires-Use-Of  :Tagliol , :Pincet , :Marver , :AnnealingKiln , :Beeswax , :Furnace , :AirCompressor , :BlowingPipe , :CeramicPotFilledWithGlass , :Fork , :DiamondShears , :Garage , :Water , :Jacks , :Blocks , :IcePick , :YokeOfSupport , :Paper , :Pontis , :Hook , :GloryHole , :StraightShears .

:ARTWORK_43_Packing_4
        a              :Packing , owl:NamedIndividual ;
        rdfs:comment   "Instance of an activity which is part of the creation process of ARTWORK_43."@en ;
        rdfs:label     "ARTWORK_43_Packing_4"@en ;
        :Followed-By   :ARTWORK_43_Transporting_4 ;
        :Follows       <http://www.semanticweb.org/ontologies/Daan/2020/BarbaraNanning#ARTWORK_43_ExaminingQuality(FinalResult)> ;
        :Has-Duration  <http://www.semanticweb.org/ontologies/Daan/2020/BarbaraNanning#2008> ;
        :Involves      :BarbaraNanning , :VáçlavNovák_Doksy_CzechRepublic , :AlešZvěřina ;
        :Located-In    :CzechRepublic ;
        :Part-Of       :Creation_Artwork_43 .

:ARTWORK_36_Sensing_2
        a              :Sensing , owl:NamedIndividual ;
        rdfs:comment   "Instance of an activity which is part of the creation process of ARTWORK_36."@en ;
        rdfs:label     "ARTWORK_36_Sensing_2"@en ;
        :Followed-By   :ARTWORK_36_Grinding ;
        :Follows       :ARTWORK_36_Sawing ;
        :Has-Duration  <http://www.semanticweb.org/ontologies/Daan/2020/BarbaraNanning#2015> ;
        :Involves      :AlešZvěřina , :BarbaraNanning , :LukášSvoboda ;
        :Located-In    :NovyBor ;
        :Part-Of       :Creation_Artwork_36 .

:ARTWORK_80_Photographing
        a              owl:NamedIndividual , :Photographing ;
        rdfs:comment   "Instance of an activity which is part of the creation process of ARTWORK_80."@en ;
        rdfs:label     "ARTWORK_80_Photographing"@en ;
        :Followed-By   :ARTWORK_80_Documenting ;
        :Follows       <http://www.semanticweb.org/ontologies/Daan/2020/BarbaraNanning#ARTWORK_80_ExaminingQuality(FinalResult)> ;
        :Has-Duration  <http://www.semanticweb.org/ontologies/Daan/2020/BarbaraNanning#2018> ;
        :Involves      <http://www.semanticweb.org/ontologies/Daan/2020/BarbaraNanning#TomHaartsen_Ouderkerka/dAmstel(NL)> , :BarbaraNanning ;
        :Located-In    :CzechRepublic ;
        :Part-Of       :Creation_Artwork_80 .

:Filling_Holes_with_Clear_Glass
        a                owl:Class ;
        rdfs:comment     "An extra dimension is created by the thick clear glass layer through which one looks between the outside and inside of the object and the inner shape seems to hang in the shape."@en ;
        rdfs:label       "Filling Holes with Clear Glass"@en ;
        rdfs:subClassOf  :Activity .

:ARTWORK_17_33_TackfusingColouredCanes
        a                 :Tackfusing_Coloured_Canes , owl:NamedIndividual ;
        rdfs:comment      "Instance of an activity which is part of the creation process of ARTWORK_17_33."@en ;
        rdfs:label        "ARTWORK_17_33_Tackfusing Coloured Canes"@en ;
        :Followed-By      :ARTWORK_17_33_TransportingMetalBowlWithCanes ;
        :Follows          :ARTWORK_17_33_MakingPatternsWithColouredCanesInTheMetalBowl ;
        :Has-Duration     <http://www.semanticweb.org/ontologies/Daan/2020/BarbaraNanning#2017> ;
        :Involves         :BarbaraNanning ;
        :Located-In       :Amsterdam ;
        :Part-Of          :Creation_Artwork_17_33 ;
        :Requires-Use-Of  :FusingKiln .

<http://www.semanticweb.org/ontologies/Daan/2020/BarbaraNanning#ARTWORK_78_ExaminingQuality(FinalResult)>
        a              owl:NamedIndividual , j.1: ;
        rdfs:comment   "Instance of an activity which is part of the creation process of ARTWORK_78."@en ;
        rdfs:label     "ARTWORK_78_Examining Quality (Final Result)"@en ;
        :Followed-By   :ARTWORK_78_Packing_5 ;
        :Follows       :ARTWORK_78_Gilding ;
        :Has-Duration  <http://www.semanticweb.org/ontologies/Daan/2020/BarbaraNanning#2016> ;
        :Involves      :BarbaraNanning , :AlešZvěřina ;
        :Located-In    :CzechRepublic ;
        :Part-Of       :Creation_Artwork_78 .

:Grinder_3  a            owl:Class ;
        rdfs:comment     "A Grinder 3 is an actor who is the third member of a team responsible for the grinding, polishing and sharpening of objects."@en ;
        rdfs:label       "Grinder 3"@en ;
        rdfs:subClassOf  :Grinder .

:ARTWORK_76_Cooling  a    :Cooling , owl:NamedIndividual ;
        rdfs:comment      "Instance of an activity which is part of the creation process of ARTWORK_76."@en ;
        rdfs:label        "ARTWORK_76_Cooling"@en ;
        :Followed-By      :ARTWORK_76_Packing ;
        :Follows          :ARTWORK_76_Translocating ;
        :Has-Duration     <http://www.semanticweb.org/ontologies/Daan/2020/BarbaraNanning#2018> ;
        :Involves         :AssistantOfBarbara , :LuděkKout ;
        :Located-In       :CzechRepublic ;
        :Part-Of          :Creation_Artwork_76 ;
        :Requires-Use-Of  :AnnealingKiln .

:ARTWORK_17_33_TransportingColouredCanes_2
        a              owl:NamedIndividual , :Transporting_Coloured_Canes ;
        rdfs:comment   "Instance of an activity which is part of the creation process of ARTWORK_17_33."@en ;
        rdfs:label     "ARTWORK_17_33_Transporting Coloured Canes_2"@en ;
        :Followed-By   :ARTWORK_17_33_DecidingColourPalette ;
        :Follows       :ARTWORK_17_33_CuttingAndPolishingColouredCanes ;
        :Has-Duration  <http://www.semanticweb.org/ontologies/Daan/2020/BarbaraNanning#2017> ;
        :Involves      :BarbaraNanning , :AlešZvěřina ;
        :Located-In    :Amsterdam ;
        :Part-Of       :Creation_Artwork_17_33 .

:ARTWORK_79_ApplyingClearGlassBell
        a                 :Applying_Clear_Glass_Bell , owl:NamedIndividual ;
        rdfs:comment      "Instance of an activity which is part of the creation process of ARTWORK_79."@en ;
        rdfs:label        "ARTWORK_79_Applying Clear Glass Bell"@en ;
        :Followed-By      :ARTWORK_79_ApplyingExtraColour ;
        :Follows          :ARTWORK_79_SetupAndTestingOfTheMetalMold_2 ;
        :Has-Duration     <http://www.semanticweb.org/ontologies/Daan/2020/BarbaraNanning#2018> ;
        :Involves         :BarbaraNanning , <http://www.semanticweb.org/ontologies/Daan/2020/BarbaraNanning#LukasHavlas(CZ)> , <http://www.semanticweb.org/ontologies/Daan/2020/BarbaraNanning#RadekKoten(CZ)> ;
        :Located-In       :CzechRepublic ;
        :Part-Of          :Creation_Artwork_79 ;
        :Processes        :AJETOClearGlass ;
        :Requires-Use-Of  :Water , :StraightShears , :AirCompressor , :Pincet , :Marver , :Paper , :Blocks , :Beeswax , :YokeOfSupport , :Hook , :IcePick , :DiamondShears , :Furnace , :BlowingPipe , :CeramicPotFilledWithGlass , :Jacks .

:ARTWORK_36_Sandblasting
        a                 :Sandblasting , owl:NamedIndividual ;
        rdfs:comment      "Instance of an activity which is part of the creation process of ARTWORK_36."@en ;
        rdfs:label        "ARTWORK_36_Sandblasting"@en ;
        :Followed-By      :ARTWORK_36_Signing ;
        :Follows          :ARTWORK_36_Transporting_2 ;
        :Has-Duration     <http://www.semanticweb.org/ontologies/Daan/2020/BarbaraNanning#2015> ;
        :Involves         :AlešZvěřina , :BarbaraNanning ;
        :Located-In       :NovyBor ;
        :Part-Of          :Creation_Artwork_36 ;
        :Requires-Use-Of  :AirCompressor .

:Making_Patterns_with_Coloured_Canes_and_Strings_in_the_Metal_Bowl
        a                owl:Class ;
        rdfs:comment     "With the canes and strings I build up the colour patterns in releasing, stainless steel bowls. A colour pattern emerges by stacking hundreds of shortened glass threads against the inner wall of the bowl, and then to smoothly melt them. Using canes and strings of various length they are placed meticulously inside a  bowl creating a design that is later used by the glassblower to create the finished object."@en ;
        rdfs:label       "Making Patterns with Coloured Canes and Strings in the Metal Bowl"@en ;
        rdfs:subClassOf  :Activity .

:ARTWORK_46_MakingPatternsWithColouredCanesAndStringsInTheMetalBowl
        a                 :Making_Patterns_with_Coloured_Canes_and_Strings_in_the_Metal_Bowl , owl:NamedIndividual ;
        rdfs:comment      "Instance of an activity which is part of the creation process of ARTWORK_46."@en ;
        rdfs:label        "ARTWORK_46_Making Patterns with Coloured Canes and Strings in the Metal Bowl"@en ;
        :Followed-By      :ARTWORK_46_TackfusingColouredCanesAndStrings ;
        :Follows          :ARTWORK_46_CuttingStrings ;
        :Has-Duration     <http://www.semanticweb.org/ontologies/Daan/2020/BarbaraNanning#2018> ;
        :Involves         :BarbaraNanning ;
        :Located-In       :Amsterdam ;
        :Part-Of          :Creation_Artwork_46 ;
        :Requires-Use-Of  :FusingKiln , :Pincet , :Glassscissors .

:ARTWORK_74_HeatingMetalMold
        a                 owl:NamedIndividual , :Heating_Metal_Mold ;
        rdfs:comment      "Instance of an activity which is part of the creation process of ARTWORK_74."@en ;
        rdfs:label        "ARTWORK_74_Heating Metal Mold"@en ;
        :Followed-By      :ARTWORK_74_Glassblowing ;
        :Follows          :ARTWORK_74_ApplyingExtraColour_2 ;
        :Has-Duration     <http://www.semanticweb.org/ontologies/Daan/2020/BarbaraNanning#2008> ;
        :Involves         :BarbaraNanning ;
        :Located-In       :CzechRepublic ;
        :Part-Of          :Creation_Artwork_74 ;
        :Requires-Use-Of  :PropaneTorch , :InterchangeableMetalMoldSetup , :Gloves .

:CollectionWithUnknownOwner
        a             :Private_Collection , owl:NamedIndividual ;
        rdfs:comment  "Collection with Unknown Owner is a collection whose owner are unknown or not published."@en ;
        rdfs:label    "Collection with Unknown Owner"@en ;
        :Consists-Of  :Artwork_79 , :Artwork_78 , :Artwork_73 .

:ARTWORK_46_HeatingMetalMold
        a                 :Heating_Metal_Mold , owl:NamedIndividual ;
        rdfs:comment      "Instance of an activity which is part of the creation process of ARTWORK_46."@en ;
        rdfs:label        "ARTWORK_46_Heating Metal Mold"@en ;
        :Followed-By      :ARTWORK_46_Glassblowing ;
        :Follows          :ARTWORK_46_ApplyingClearOverlay ;
        :Has-Duration     <http://www.semanticweb.org/ontologies/Daan/2020/BarbaraNanning#2018> ;
        :Involves         :BarbaraNanning , <http://www.semanticweb.org/ontologies/Daan/2020/BarbaraNanning#JessicaHomich(USA)> ;
        :Part-Of          :Creation_Artwork_46 ;
        :Requires-Use-Of  :PropaneTorch , :Gloves , :InterchangeableMetalMoldSetup .

:ARTWORK_18_64_TransportingMonochromeRods
        a              :Transporting_Monochrome_Rods , owl:NamedIndividual ;
        rdfs:comment   "Instance of an activity which is part of the creation process of ARTWORK_18_64."@en ;
        rdfs:label     "ARTWORK_18_64_Transporting Monochrome Rods"@en ;
        :Followed-By   :ARTWORK_18_64_ProducingColouredCanes ;
        :Follows       :ARTWORK_18_64_DecidingColourPaletteAndPatterns_2 ;
        :Has-Duration  <http://www.semanticweb.org/ontologies/Daan/2020/BarbaraNanning#2015> ;
        :Involves      :BarbaraNanning , <http://www.semanticweb.org/ontologies/Daan/2020/BarbaraNanning#JaroslavSvacha(CZ)> ;
        :Located-In    :Langweer ;
        :Part-Of       :Creation_Artwork_18_64 .

:ARTWORK_39_Photographing
        a              owl:NamedIndividual , :Photographing ;
        rdfs:comment   "Instance of an activity which is part of the creation process of ARTWORK_39."@en ;
        rdfs:label     "ARTWORK_39_Photographing"@en ;
        :Followed-By   :ARTWORK_39_Packing_3 ;
        :Follows       :ARTWORK_39_Transporting_2 ;
        :Has-Duration  <http://www.semanticweb.org/ontologies/Daan/2020/BarbaraNanning#2015> ;
        :Involves      <http://www.semanticweb.org/ontologies/Daan/2020/BarbaraNanning#TomHaartsen_Ouderkerka/dAmstel(NL)> , :BarbaraNanning ;
        :Located-In    <http://www.semanticweb.org/ontologies/Daan/2020/BarbaraNanning#Ouderkerka/dAmstel> ;
        :Part-Of       :Creation_Artwork_39 .

<https://data.cultureelerfgoed.nl/term/id/abr/2dcb88e1-e777-4cff-babc-d97485b42b10>
        a       owl:Class .

:ARTWORK_36_Packing  a  :Packing , owl:NamedIndividual ;
        rdfs:comment   "Instance of an activity which is part of the creation process of ARTWORK_36."@en ;
        rdfs:label     "ARTWORK_36_Packing"@en ;
        :Followed-By   :ARTWORK_36_Transporting ;
        :Follows       :ARTWORK_36_Cooling ;
        :Has-Duration  <http://www.semanticweb.org/ontologies/Daan/2020/BarbaraNanning#2015> ;
        :Involves      :BarbaraNanning ;
        :Located-In    :Zaandam ;
        :Part-Of       :Creation_Artwork_36 .

:ARTWORK_43_Packing  a  owl:NamedIndividual , :Packing ;
        rdfs:comment   "Instance of an activity which is part of the creation process of ARTWORK_43."@en ;
        rdfs:label     "ARTWORK_43_Packing"@en ;
        :Followed-By   :ARTWORK_43_Transporting ;
        :Follows       :ARTWORK_43_Cooling ;
        :Has-Duration  <http://www.semanticweb.org/ontologies/Daan/2020/BarbaraNanning#2008> ;
        :Involves      :AlešZvěřina , :BarbaraNanning ;
        :Located-In    :CzechRepublic ;
        :Part-Of       :Creation_Artwork_43 .

:ARTWORK_36_Grinding  a   :Grinding , owl:NamedIndividual ;
        rdfs:comment      "Instance of an activity which is part of the creation process of ARTWORK_36."@en ;
        rdfs:label        "ARTWORK_36_Grinding_2"@en ;
        :Followed-By      :ARTWORK_36_Polishing ;
        :Follows          :ARTWORK_36_Sensing_2 ;
        :Has-Duration     <http://www.semanticweb.org/ontologies/Daan/2020/BarbaraNanning#2015> ;
        :Involves         :BarbaraNanning , :RobertFlorian , :AlešZvěřina ;
        :Located-In       :NovyBor ;
        :Part-Of          :Creation_Artwork_36 ;
        :Requires-Use-Of  :GrindingWheel , :SharpeningStone .

:Image_Artwork_76  a            :Digital_Image , owl:NamedIndividual ;
        rdfs:comment            "Image of an artwork by Barbara Nanning displayed in \"Barbara Nanning Eeuwige Beweging\" by Eliens (2019)."@en ;
        rdfs:label              "Image_Artwork_76"@en ;
        :Representation-Source  "Tom Haartsen_Ouderkerk a/d Amstel (NL)"@en ;
        :Shows                  :Artwork_76 .

:Glass  a                    owl:Class ;
        rdfs:comment         "Glass is a solid and brittle material."@en ;
        rdfs:label           "Glass"@en ;
        rdfs:subClassOf      :Man-Made_Material ;
        owl:disjointWith     :Gold_Leaf ;
        owl:equivalentClass  <http://www.wikidata.org/entity/Q11469> .

:ARTWORK_77_Photographing
        a              owl:NamedIndividual , :Photographing ;
        rdfs:comment   "Instance of an activity which is part of the creation process of ARTWORK_77."@en ;
        rdfs:label     "ARTWORK_77_Photographing"@en ;
        :Followed-By   :ARTWORK_77_Documenting ;
        :Follows       :ARTWORK_77_Transporting_4 ;
        :Has-Duration  <http://www.semanticweb.org/ontologies/Daan/2020/BarbaraNanning#2018> ;
        :Involves      <http://www.semanticweb.org/ontologies/Daan/2020/BarbaraNanning#TomHaartsen_Ouderkerka/dAmstel(NL)> , :BarbaraNanning ;
        :Located-In    :CzechRepublic ;
        :Part-Of       :Creation_Artwork_77 .

:Image_Artwork_44  a            :Digital_Image , owl:NamedIndividual ;
        rdfs:comment            "Image of an artwork by Barbara Nanning displayed in \"Barbara Nanning Eeuwige Beweging\" by Eliens (2019)."@en ;
        rdfs:label              "Image_Artwork_44"@en ;
        :Representation-Source  "Tom Haartsen_Ouderkerk a/d Amstel (NL)"@en ;
        :Shows                  :Artwork_44 .

:ARTWORK_46_Casting  a    owl:NamedIndividual , :Casting ;
        rdfs:comment      "Instance of an activity which is part of the creation process of ARTWORK_46."@en ;
        rdfs:label        "ARTWORK_46_Casting"@en ;
        :Followed-By      :ARTWORK_46_CuttingAndPolishingCastedMonochromeSheetsToSmallRods ;
        :Follows          :ARTWORK_46_Ordening ;
        :Has-Duration     <http://www.semanticweb.org/ontologies/Daan/2020/BarbaraNanning#2015> ;
        :Involves         :BarbaraNanning , :SteefHendriks ;
        :Located-In       :Langweer ;
        :Part-Of          :Creation_Artwork_46 ;
        :Requires-Use-Of  :Furnace , :Gloves , :FusingKiln , :Pincet .

:DavidČerný  a        owl:NamedIndividual , :First_Glass_Blower ;
        rdfs:comment  "David Černý is a First Glass Blower."@en ;
        rdfs:label    "David Černý"@en ;
        owl:sameAs    <http://www.wikidata.org/entity/Q378305> ;
        :Involved-In  :ARTWORK_46_SetupAndTestingOfTheMetalMold , :ARTWORK_36_ApplyingMassivePieceOfClearGlass , :ARTWORK_46_Modeling , :ARTWORK_46_Glassblowing , :ARTWORK_46_PickingUpColouredCanesPattern , :ARTWORK_46_ApplyingClearGlassBell , :ARTWORK_36_Modeling_2 , :ARTWORK_46_ApplyingClearOverlay ;
        :Works-For    <http://www.semanticweb.org/ontologies/Daan/2020/BarbaraNanning#Ji%C5%99%C3%ADPa%C4%8DinekLindava(CZ)> .

:ARTWORK_77_PreparingGlass
        a                 :Preparing_Glass , owl:NamedIndividual ;
        rdfs:comment      "Instance of an activity which is part of the creation process of ARTWORK_77."@en ;
        rdfs:label        "ARTWORK_77_Preparing Glass"@en ;
        :Followed-By      :ARTWORK_77_SetupAndTestingOfTheMetalMold ;
        :Has-Duration     <http://www.semanticweb.org/ontologies/Daan/2020/BarbaraNanning#2018> ;
        :Involves         <http://www.semanticweb.org/ontologies/Daan/2020/BarbaraNanning#RadekKoten(CZ)> , :BarbaraNanning ;
        :Located-In       :CzechRepublic ;
        :Part-Of          :Creation_Artwork_77 ;
        :Requires-Use-Of  :Marver , :BlowingPipe , :Pontis , :GloryHole , :Garage ;
        :Starts           :Creation_Artwork_77 .

:Deciding_Colour_Palette
        a                owl:Class ;
        rdfs:comment     "The effect of the primary, secondary, tertiary and complementary colors determine my choice of color. As a guide I use the color theory of Bauhaus and especially Johannes Itten."@en ;
        rdfs:label       "Deciding Colour Palette"@en ;
        rdfs:subClassOf  :Activity .

:ARTWORK_77_ExaminingTheQualityOfTheGlass
        a                 :Examining_the_Quality_of_the_Glass , owl:NamedIndividual ;
        rdfs:comment      "Instance of an activity which is part of the creation process of ARTWORK_77."@en ;
        rdfs:label        "ARTWORK_77_Examining the Quality of the Glass"@en ;
        :Followed-By      :ARTWORK_77_Cooling ;
        :Follows          :ARTWORK_77_Modeling ;
        :Has-Duration     <http://www.semanticweb.org/ontologies/Daan/2020/BarbaraNanning#2018> ;
        :Involves         <http://www.semanticweb.org/ontologies/Daan/2020/BarbaraNanning#RadekKoten(CZ)> , :LuděkKout , :BarbaraNanning ;
        :Located-In       :CzechRepublic ;
        :Part-Of          :Creation_Artwork_77 ;
        :Requires-Use-Of  :StraightShears , :YokeOfSupport , :CeramicPotFilledWithGlass , :Blocks , :Water , :Pontis , :DiamondShears , :Paper , :BlowingPipe , :AnnealingKiln , :GloryHole , :Furnace , :Jacks .

:ARTWORK_44_Transporting_4
        a              owl:NamedIndividual , :Transporting ;
        rdfs:comment   "Instance of an activity which is part of the creation process of ARTWORK_44."@en ;
        rdfs:label     "ARTWORK_44_Transporting_4"@en ;
        :Followed-By   :ARTWORK_44_Photographing ;
        :Follows       :ARTWORK_44_Packing_4 ;
        :Has-Duration  <http://www.semanticweb.org/ontologies/Daan/2020/BarbaraNanning#2018> ;
        :Involves      :BarbaraNanning , :AlešZvěřina ;
        :Located-In    :CzechRepublic ;
        :Part-Of       :Creation_Artwork_44 .

<http://www.cidoc-crm.org/cidoc-crm/P94_was_created_by>
        a                       owl:ObjectProperty ;
        owl:equivalentProperty  :Created-By .

:ARTWORK_78_Transporting_2
        a              :Transporting , owl:NamedIndividual ;
        rdfs:comment   "Instance of an activity which is part of the creation process of ARTWORK_78."@en ;
        rdfs:label     "ARTWORK_78_Transporting_2"@en ;
        :Followed-By   :ARTWORK_78_Signing ;
        :Follows       :ARTWORK_78_Packing_2 ;
        :Has-Duration  <http://www.semanticweb.org/ontologies/Daan/2020/BarbaraNanning#2008> ;
        :Involves      :BarbaraNanning , :AlešZvěřina ;
        :Located-In    :CzechRepublic ;
        :Part-Of       :Creation_Artwork_78 .

:Part-Of  a           owl:ObjectProperty ;
        rdfs:comment  "Part-Of is a property which connects an entity to the entity in which it is a component."@en ;
        rdfs:domain   :Entity ;
        rdfs:label    "Part-Of"@en ;
        rdfs:range    :Entity .

:ARTWORK_80_Documenting
        a              :Documenting , owl:NamedIndividual ;
        rdfs:comment   "Instance of an activity which is part of the creation process of ARTWORK_80."@en ;
        rdfs:label     "ARTWORK_80_Documenting"@en ;
        :Followed-By   :ARTWORK_80_Packing_4 ;
        :Follows       :ARTWORK_80_Photographing ;
        :Has-Duration  <http://www.semanticweb.org/ontologies/Daan/2020/BarbaraNanning#2018> ;
        :Involves      :BarbaraNanning ;
        :Located-In    :CzechRepublic ;
        :Part-Of       :Creation_Artwork_80 .

:Transporting_Metal_Bowl_with_Canes
        a                owl:Class ;
        rdfs:comment     "Moving said objects from one place to another"@en ;
        rdfs:label       "Transporting Metal Bowl with Canes"@en ;
        rdfs:subClassOf  :Transporting .

<http://vocab.getty.edu/aat/300053090>
        a                    owl:Class ;
        owl:equivalentClass  :Grinding .

:Creation_Artwork_74  a  :Creation_Event , owl:NamedIndividual ;
        rdfs:comment    "Creation event for an artwork by Barbara Nanning displayed in \"Barbara Nanning Eeuwige Beweging\" by Eliens (2019)."@en ;
        rdfs:label      "Creation_Artwork_74"@en ;
        :Consists-Of    <http://www.semanticweb.org/ontologies/Daan/2020/BarbaraNanning#ARTWORK_74_ExaminingQuality(FinalResult)> , :ARTWORK_74_Packing_5 , :ARTWORK_74_Transporting_3 , :ARTWORK_74_HeatingMetalMold , :ARTWORK_74_Modeling , :ARTWORK_74_ExaminingTheQualityOfTheGlass , :ARTWORK_74_Transporting_2 , :ARTWORK_74_Sawing , :ARTWORK_74_Translocating , :ARTWORK_74_SetupAndTestingOfTheMetalMold , :ARTWORK_74_Sensing , :ARTWORK_74_Transporting , :ARTWORK_74_Transporting_4 , :ARTWORK_74_Glassblowing , :ARTWORK_74_Photographing , <http://www.semanticweb.org/ontologies/Daan/2020/BarbaraNanning#ARTWORK_74_ExaminingQuality(Result)> , :ARTWORK_74_Grinding , :ARTWORK_74_Resting , :ARTWORK_74_Polishing , :ARTWORK_74_ApplyingExtraColour , :ARTWORK_74_Packing_3 , <http://www.semanticweb.org/ontologies/Daan/2020/BarbaraNanning#ARTWORK_74_ExaminingQuality(CheckForIrregularitiesInTheGlass)> , :ARTWORK_74_Cooling , :ARTWORK_74_ApplyingClearGlassBell , :ARTWORK_74_ApplyingExtraColour_2 , :ARTWORK_74_Packing_2 , :ARTWORK_74_Packing , :ARTWORK_74_Gilding , <http://www.semanticweb.org/ontologies/Daan/2020/BarbaraNanning#ARTWORK_74_ExaminingQuality(Shape/Form)> , :ARTWORK_74_Documenting , :ARTWORK_74_PreparingGlass , :ARTWORK_74_Signing , :ARTWORK_74_SetupAndTestingOfTheMetalMold_2 , :ARTWORK_74_Packing_4 ;
        :Created        :Artwork_74 ;
        :Finishes-With  :ARTWORK_74_Packing_5 ;
        :Has-Duration   <http://www.semanticweb.org/ontologies/Daan/2020/BarbaraNanning#2008> ;
        :Located-In     :CzechRepublic ;
        :Starts-With    :ARTWORK_74_PreparingGlass ;
        :Within-Period  :GlassVerreÉglomisé .

:ARTWORK_77_Packing_2
        a              :Packing , owl:NamedIndividual ;
        rdfs:comment   "Instance of an activity which is part of the creation process of ARTWORK_77."@en ;
        rdfs:label     "ARTWORK_77_Packing_2"@en ;
        :Followed-By   :ARTWORK_77_Transporting_2 ;
        :Follows       :ARTWORK_77_MeasuringAndBoxesMaking ;
        :Has-Duration  <http://www.semanticweb.org/ontologies/Daan/2020/BarbaraNanning#2018> ;
        :Involves      :BarbaraNanning , :AlešZvěřina ;
        :Located-In    :CzechRepublic ;
        :Part-Of       :Creation_Artwork_77 .

:StraightShears  a    :Tool , owl:NamedIndividual ;
        rdfs:comment  "Straight Shears is a tool to cut material (hot glass)."@en ;
        rdfs:label    "Straight Shears"@en ;
        :Used-For     :ARTWORK_73_Glassblowing , :ARTWORK_80_ApplyingExtraColour , :ARTWORK_75_ApplyingClearGlassBell , :ARTWORK_44_ApplyingExtraColour , :ARTWORK_78_Glassblowing , :ARTWORK_73_ExaminingTheQualityOfTheGlass , :ARTWORK_44_ApplyingExtraColour_2 , :ARTWORK_79_ApplyingClearGlassBell , :ARTWORK_76_Glassblowing , :ARTWORK_80_ApplyingClearGlassBell , :ARTWORK_74_ExaminingTheQualityOfTheGlass , :ARTWORK_44_ApplyingClearGlassBell , :ARTWORK_74_ApplyingExtraColour_2 , :ARTWORK_44_ExaminingTheQualityOfTheGlass , :ARTWORK_43_ExaminingTheQualityOfTheGlass , :ARTWORK_73_ApplyingClearGlassBell , :ARTWORK_78_ApplyingExtraColour , :ARTWORK_79_Glassblowing , :ARTWORK_76_ApplyingExtraColour , :ARTWORK_74_Glassblowing , :ARTWORK_43_ApplyingClearGlassBell , :ARTWORK_79_ApplyingExtraColour , :ARTWORK_78_ExaminingTheQualityOfTheGlass , :ARTWORK_77_ExaminingTheQualityOfTheGlass , :ARTWORK_74_ApplyingClearGlassBell , :ARTWORK_43_ApplyingExtraColour , :ARTWORK_77_Glassblowing , :ARTWORK_77_ApplyingClearGlassBell , :ARTWORK_77_ApplyingExtraColour , :ARTWORK_76_ExaminingTheQualityOfTheGlass , :ARTWORK_76_ApplyingExtraColour_2 , :ARTWORK_75_ExaminingTheQualityOfTheGlass , :ARTWORK_75_ApplyingExtraColour , :ARTWORK_76_ApplyingClearGlassBell , :ARTWORK_44_Glassblowing , :ARTWORK_75_ApplyingExtraColour_2 , :ARTWORK_80_Glassblowing , :ARTWORK_74_ApplyingExtraColour , :ARTWORK_78_ApplyingClearGlassBell , :ARTWORK_79_ExaminingTheQualityOfTheGlass , :ARTWORK_79_ApplyingExtraColour_2 , :ARTWORK_75_Glassblowing , :ARTWORK_43_Glassblowing , :ARTWORK_80_ExaminingTheQualityOfTheGlass .

<http://www.semanticweb.org/ontologies/Daan/2020/BarbaraNanning#ARTWORK_17_33_ExaminingQuality(Result)>
        a              j.0: , owl:NamedIndividual ;
        rdfs:comment   "Instance of an activity which is part of the creation process of ARTWORK_17_33."@en ;
        rdfs:label     "ARTWORK_17_33_Examining Quality (Result)"@en ;
        :Followed-By   :ARTWORK_17_33_MeasuringAndBoxesMaking ;
        :Follows       :ARTWORK_17_33_Signing ;
        :Has-Duration  <http://www.semanticweb.org/ontologies/Daan/2020/BarbaraNanning#2017> ;
        :Involves      :BarbaraNanning , :AlešZvěřina ;
        :Located-In    :NovyBor ;
        :Part-Of       :Creation_Artwork_17_33 .

:AJETOGreenGlass  a    :AJETO_Glass , owl:NamedIndividual ;
        rdfs:comment   "AJETO Green is a form of AJETO glass with a Green colour."@en ;
        rdfs:label     "AJETO Green Glass"@en ;
        :Availability  "Available"@en ;
        :Made-By       :LASVITAJETO ;
        :Made-Out-Of   :Sand , :Potassium , :Calcium , :Soda ;
        :Transparency  "Transparent"@en .

<http://vocab.getty.edu/aat/300148821>
        a           owl:NamedIndividual ;
        owl:sameAs  :Gloves .

:ARTWORK_46_Sawing  a     owl:NamedIndividual , :Sawing ;
        rdfs:comment      "Instance of an activity which is part of the creation process of ARTWORK_46."@en ;
        rdfs:label        "ARTWORK_46_Sawing"@en ;
        :Followed-By      :ARTWORK_46_Sensing_2 ;
        :Follows          <http://www.semanticweb.org/ontologies/Daan/2020/BarbaraNanning#ARTWORK_46_ExaminingQuality(CheckForIrregularitiesInTheGlass)> ;
        :Has-Duration     <http://www.semanticweb.org/ontologies/Daan/2020/BarbaraNanning#2018> ;
        :Involves         :AlešZvěřina , :BarbaraNanning ;
        :Located-In       :NovyBor ;
        :Part-Of          :Creation_Artwork_46 ;
        :Requires-Use-Of  :DiamondSaw .

:Artwork_17_33  a     owl:NamedIndividual , :Glass_Artwork ;
        rdfs:comment  "Artwork_17_33 is a glass artwork made by Barbara Nanning."@en ;
        rdfs:label    "Coloured Shadows Coral Reef"@en ;
        :Created-By   :Creation_Artwork_17_33 ;
        :Has-Depth    "21"^^xsd:decimal ;
        :Has-Height   "21"^^xsd:decimal , "30"^^xsd:decimal ;
        :Is-Unica     "Yes"@en ;
        :Made-By      :BarbaraNanning , <http://www.semanticweb.org/ontologies/Daan/2020/BarbaraNanning#Ale%C5%A1Zv%C4%9B%C5%99ina&AZ-Design> , :LASVITAJETO ;
        :Made-Out-Of  :AJETORedGlass , :AJETOClearGlass , :AJETOWhiteGlass ;
        :Shown-By     :Image_Artwork_17_33 .

:ARTWORK_76_Packing_5
        a              :Packing , owl:NamedIndividual ;
        rdfs:comment   "Instance of an activity which is part of the creation process of ARTWORK_76."@en ;
        rdfs:label     "ARTWORK_76_Packing_5"@en ;
        :Finishes      :Creation_Artwork_76 ;
        :Follows       :ARTWORK_76_Documenting ;
        :Has-Duration  <http://www.semanticweb.org/ontologies/Daan/2020/BarbaraNanning#2018> ;
        :Involves      :BarbaraNanning ;
        :Located-In    :CzechRepublic ;
        :Part-Of       :Creation_Artwork_76 .

:CeramicPotFilledWithGlass
        a             owl:NamedIndividual , :Equipment ;
        rdfs:comment  "A Ceramic Pot filled with Glass is a round container filled with Glass material."@en ;
        rdfs:label    "Ceramic Pot filled with Glass"@en ;
        :Made-Out-Of  :Ceramic ;
        :Used-For     :ARTWORK_43_ApplyingClearGlassBell , :ARTWORK_76_ApplyingClearGlassBell , :ARTWORK_36_CuttingAndPolishingCastedMonochromeSheetsToSmallRods , :ARTWORK_77_ApplyingClearGlassBell , :ARTWORK_44_Glassblowing , :ARTWORK_74_ApplyingExtraColour , :ARTWORK_80_ExaminingTheQualityOfTheGlass , :ARTWORK_75_ApplyingExtraColour_2 , :ARTWORK_18_64_CuttingAndPolishingCastedMonochromeSheetsToSmallRods , :ARTWORK_74_ApplyingClearGlassBell , :ARTWORK_79_ExaminingTheQualityOfTheGlass , :ARTWORK_78_Glassblowing , :ARTWORK_74_ApplyingExtraColour_2 , :ARTWORK_79_ApplyingExtraColour , :ARTWORK_80_ApplyingClearGlassBell , :ARTWORK_18_64_ProducingColouredCanes , :ARTWORK_78_ExaminingTheQualityOfTheGlass , :ARTWORK_17_33_PickingUpColouredCanesPattern , :ARTWORK_36_PickingUpColouredCanesPattern , :ARTWORK_80_ApplyingExtraColour , :ARTWORK_17_33_ApplyingClearOverlay , :ARTWORK_76_Glassblowing , :ARTWORK_46_ApplyingClearOverlay , :ARTWORK_43_Glassblowing , :ARTWORK_80_Glassblowing , :ARTWORK_75_ExaminingTheQualityOfTheGlass , :ARTWORK_79_ApplyingClearGlassBell , :ARTWORK_74_ExaminingTheQualityOfTheGlass , :ARTWORK_44_ExaminingTheQualityOfTheGlass , :ARTWORK_76_ApplyingExtraColour , :ARTWORK_77_Glassblowing , :ARTWORK_39_PickingUpColouredPanel , :ARTWORK_76_ApplyingExtraColour_2 , :ARTWORK_75_Glassblowing , :ARTWORK_73_ApplyingClearGlassBell , :ARTWORK_36_ProducingColouredCanes , :ARTWORK_44_ApplyingExtraColour , :ARTWORK_78_ApplyingExtraColour , :ARTWORK_36_PickingUpColouredPanel , :ARTWORK_79_Glassblowing , :ARTWORK_46_PickingUpColouredCanesPattern , :ARTWORK_43_ExaminingTheQualityOfTheGlass , :ARTWORK_75_ApplyingExtraColour , :ARTWORK_46_CuttingAndPolishingCastedMonochromeSheetsToSmallRods , :ARTWORK_79_ApplyingExtraColour_2 , :ARTWORK_73_Glassblowing , :ARTWORK_44_ApplyingExtraColour_2 , :ARTWORK_36_ApplyingMassivePieceOfClearGlass , :ARTWORK_18_64_PickingUpColouredCanesPattern , :ARTWORK_46_ProducingColouredCanes , :ARTWORK_17_33_ProducingColouredCanes , :ARTWORK_43_ApplyingExtraColour , :ARTWORK_75_ApplyingClearGlassBell , :ARTWORK_74_Glassblowing , :ARTWORK_78_ApplyingClearGlassBell , :ARTWORK_73_ExaminingTheQualityOfTheGlass , :ARTWORK_76_ExaminingTheQualityOfTheGlass , :ARTWORK_44_ApplyingClearGlassBell , :ARTWORK_77_ExaminingTheQualityOfTheGlass , :ARTWORK_77_ApplyingExtraColour .

:Supervisor_Works  a     owl:Class ;
        rdfs:comment     "A Supervisor Works is an actor who supervises the location, furnace, workers and works."@en ;
        rdfs:label       "Supervisor Works"@en ;
        rdfs:subClassOf  :Person .

:Gallery  a                  owl:Class ;
        rdfs:comment         "A gallery is an organisation which displays or sells artwork from a certain location."@en ;
        rdfs:label           "Gallery"@en ;
        rdfs:subClassOf      :Organisation ;
        owl:equivalentClass  <http://www.wikidata.org/entity/Q1007870> .

<http://www.semanticweb.org/ontologies/Daan/2020/BarbaraNanning#FlorisVanDonselaar(NL)>
        a             owl:NamedIndividual , :Metal_Worker_1 ;
        rdfs:comment  "Floris van Donselaar (NL) is a Metal Worker 1."@en ;
        rdfs:label    "Floris van Donselaar (NL)"@en ;
        :Maker-Of     :InterchangeableMetalMoldSetup .

:ARTWORK_76_Photographing
        a              :Photographing , owl:NamedIndividual ;
        rdfs:comment   "Instance of an activity which is part of the creation process of ARTWORK_76."@en ;
        rdfs:label     "ARTWORK_76_Photographing"@en ;
        :Followed-By   :ARTWORK_76_Documenting ;
        :Follows       :ARTWORK_76_Transporting_4 ;
        :Has-Duration  <http://www.semanticweb.org/ontologies/Daan/2020/BarbaraNanning#2018> ;
        :Involves      :BarbaraNanning , <http://www.semanticweb.org/ontologies/Daan/2020/BarbaraNanning#TomHaartsen_Ouderkerka/dAmstel(NL)> ;
        :Located-In    :CzechRepublic ;
        :Part-Of       :Creation_Artwork_76 .

:ARTWORK_36_Packing_6
        a              :Packing , owl:NamedIndividual ;
        rdfs:comment   "Instance of an activity which is part of the creation process of ARTWORK_36."@en ;
        rdfs:label     "ARTWORK_36_Packing_6"@en ;
        :Followed-By   :ARTWORK_36_Transporting_5 ;
        :Follows       :ARTWORK_36_MeasuringAndBoxesMaking_2 ;
        :Has-Duration  <http://www.semanticweb.org/ontologies/Daan/2020/BarbaraNanning#2019> ;
        :Involves      :BarbaraNanning ;
        :Located-In    :NovyBor ;
        :Part-Of       :Creation_Artwork_36 .

:ARTWORK_39_Transporting
        a              :Transporting , owl:NamedIndividual ;
        rdfs:comment   "Instance of an activity which is part of the creation process of ARTWORK_39."@en ;
        rdfs:label     "ARTWORK_39_Transporting"@en ;
        :Followed-By   :ARTWORK_39_Resting ;
        :Follows       :ARTWORK_39_Packing ;
        :Has-Duration  <http://www.semanticweb.org/ontologies/Daan/2020/BarbaraNanning#2015> ;
        :Involves      :AlešZvěřina , :BarbaraNanning ;
        :Located-In    :NovyBor ;
        :Part-Of       :Creation_Artwork_39 .

<http://www.semanticweb.org/ontologies/Daan/2020/BarbaraNanning#ARTWORK_46_ExaminingQuality(CheckForIrregularitiesInTheGlass)>
        a              owl:NamedIndividual , j.3: ;
        rdfs:comment   "Instance of an activity which is part of the creation process of ARTWORK_46."@en ;
        rdfs:label     "ARTWORK_46_Examining Quality (Check for Irregularities in the Glass)"@en ;
        :Followed-By   :ARTWORK_46_Sawing ;
        :Follows       :ARTWORK_46_Resting ;
        :Has-Duration  <http://www.semanticweb.org/ontologies/Daan/2020/BarbaraNanning#2018> ;
        :Involves      :BarbaraNanning , :AlešZvěřina ;
        :Located-In    :NovyBor ;
        :Part-Of       :Creation_Artwork_46 .

:ARTWORK_36_Polishing
        a                 :Polishing , owl:NamedIndividual ;
        rdfs:comment      "Instance of an activity which is part of the creation process of ARTWORK_36."@en ;
        rdfs:label        "ARTWORK_36_Polishing"@en ;
        :Followed-By      <http://www.semanticweb.org/ontologies/Daan/2020/BarbaraNanning#ARTWORK_36_ExaminingQuality(Result)> ;
        :Follows          :ARTWORK_36_Grinding ;
        :Has-Duration     <http://www.semanticweb.org/ontologies/Daan/2020/BarbaraNanning#2015> ;
        :Involves         :AlešZvěřina , :LukášSvoboda , :BarbaraNanning ;
        :Located-In       :NovyBor ;
        :Part-Of          :Creation_Artwork_36 ;
        :Requires-Use-Of  :PolishingStone .

<http://vocab.getty.edu/aat/300007806>
        a           owl:NamedIndividual ;
        owl:sameAs  :Garage .

:ARTWORK_46_Polishing
        a                 owl:NamedIndividual , :Polishing ;
        rdfs:comment      "Instance of an activity which is part of the creation process of ARTWORK_46."@en ;
        rdfs:label        "ARTWORK_46_Polishing"@en ;
        :Followed-By      :ARTWORK_46_Signing ;
        :Follows          :ARTWORK_46_Grinding ;
        :Has-Duration     <http://www.semanticweb.org/ontologies/Daan/2020/BarbaraNanning#2018> ;
        :Involves         :AlešZvěřina , :BarbaraNanning , :LukášSvoboda ;
        :Located-In       :NovyBor ;
        :Part-Of          :Creation_Artwork_46 ;
        :Requires-Use-Of  :PolishingStone .

:ARTWORK_46_TransportingMonochromeRods
        a              owl:NamedIndividual , :Transporting_Monochrome_Rods ;
        rdfs:comment   "Instance of an activity which is part of the creation process of ARTWORK_46."@en ;
        rdfs:label     "ARTWORK_46_Transporting Monochrome Rods"@en ;
        :Followed-By   :ARTWORK_46_ProducingColouredCanes ;
        :Follows       :ARTWORK_46_DecidingColourPaletteAndPatterns_2 ;
        :Has-Duration  <http://www.semanticweb.org/ontologies/Daan/2020/BarbaraNanning#2015> ;
        :Involves      :BarbaraNanning , <http://www.semanticweb.org/ontologies/Daan/2020/BarbaraNanning#JaroslavSvacha(CZ)> ;
        :Located-In    :Langweer ;
        :Part-Of       :Creation_Artwork_46 .

:ARTWORK_18_64_FillingKilnsWithMetalBowl
        a                 owl:NamedIndividual , :Filling_Kilns_with_Metal_Bowl ;
        rdfs:comment      "Instance of an activity which is part of the creation process of ARTWORK_18_64."@en ;
        rdfs:label        "ARTWORK_18_64_Filling Kilns with Metal Bowl"@en ;
        :Followed-By      :ARTWORK_18_64_PreparingGlass ;
        :Follows          :ARTWORK_18_64_PreparingForBlowing ;
        :Has-Duration     <http://www.semanticweb.org/ontologies/Daan/2020/BarbaraNanning#2015> ;
        :Involves         <http://www.semanticweb.org/ontologies/Daan/2020/BarbaraNanning#JiriPacinek(CZ)> , :BarbaraNanning ;
        :Located-In       :Lindava ;
        :Part-Of          :Creation_Artwork_18_64 ;
        :Requires-Use-Of  :Garage , :FusingKiln , :Gloves .

:Artwork_76  a        owl:NamedIndividual , :Glass_Artwork ;
        rdfs:comment  "Artwork by Barbara Nanning displayed in \"Barbara Nanning Eeuwige Beweging\" by Eliens (2019)."@en ;
        rdfs:label    "Verre églomisé (Alexandrite Glass)"@en ;
        :Created-By   :Creation_Artwork_76 ;
        :Has-Depth    "30"^^xsd:decimal ;
        :Has-Height   "18"^^xsd:decimal ;
        :Has-Width    "35"^^xsd:decimal ;
        :Is-Unica     "Yes"@en ;
        :Located-In   :Amsterdam ;
        :Made-By      :LASVITAJETO , :BarbaraNanning , <http://www.semanticweb.org/ontologies/Daan/2020/BarbaraNanning#Ale%C5%A1Zv%C4%9B%C5%99ina&AZ-Design> , :VáçlavNovák_Doksy_CzechRepublic ;
        :Made-Out-Of  <http://www.semanticweb.org/ontologies/Daan/2020/BarbaraNanning#ReichenbachColourRodsGlass(DE)> , :PureDucat , :AJETOClearGlass , :AJETOAlexandriteGlass ;
        :Part-Of      :CollectionOfBarbaraNanning ;
        :Shown-By     :Image_Artwork_76 .

:ARTWORK_44_Sensing  a  owl:NamedIndividual , :Sensing ;
        rdfs:comment   "Instance of an activity which is part of the creation process of ARTWORK_44."@en ;
        rdfs:label     "ARTWORK_44_Sensing"@en ;
        :Followed-By   :ARTWORK_44_Modeling ;
        :Follows       :ARTWORK_44_Glassblowing ;
        :Has-Duration  <http://www.semanticweb.org/ontologies/Daan/2020/BarbaraNanning#2018> ;
        :Involves      :BarbaraNanning , :AlešZvěřina , :LukášSvoboda ;
        :Located-In    :CzechRepublic ;
        :Part-Of       :Creation_Artwork_44 .

:Created-By  a        owl:ObjectProperty ;
        rdfs:comment  "Created-By is a property of a thing connecting the thing with a Creation Event."@en ;
        rdfs:domain   :Thing ;
        rdfs:label    "Created-By"@en ;
        rdfs:range    :Creation_Event .

<http://www.semanticweb.org/ontologies/Daan/2020/BarbaraNanning#ARTWORK_44_ExaminingQuality(FinalResult)>
        a              owl:NamedIndividual , j.1: ;
        rdfs:comment   "Instance of an activity which is part of the creation process of ARTWORK_44."@en ;
        rdfs:label     "ARTWORK_44_Examining Quality (Final Result)"@en ;
        :Followed-By   :ARTWORK_44_Packing_5 ;
        :Follows       :ARTWORK_44_Gilding ;
        :Has-Duration  <http://www.semanticweb.org/ontologies/Daan/2020/BarbaraNanning#2018> ;
        :Involves      :AlešZvěřina , :BarbaraNanning ;
        :Located-In    :CzechRepublic ;
        :Part-Of       :Creation_Artwork_44 .

:Cutting_and_Polishing_Casted_Monochrome_Sheets_to_Small_Rods
        a                owl:Class ;
        rdfs:comment     "Also known as Preparing Glass for Canes. Pieces of Coloured sheet glass are cut, layered and melted together. Then they are polished and ready for the glassblower to use."@en ;
        rdfs:label       "Cutting and Polishing Casted Monochrome Sheets to Small Rods"@en ;
        rdfs:subClassOf  :Activity .

<http://www.cidoc-crm.org/cidoc-crm/P3_has_note>
        a       owl:ObjectProperty .

:Acquired-By  a       owl:ObjectProperty ;
        rdfs:comment  "Acquired-By is a property which connects a thing with an (possibly previous) owner of the thing."@en ;
        rdfs:domain   :Thing ;
        rdfs:label    "Acquired-By"@en ;
        rdfs:range    :Actor .

:Artwork_44  a        owl:NamedIndividual , :Glass_Artwork ;
        rdfs:comment  "Artwork by Barbara Nanning displayed in \"Barbara Nanning Eeuwige Beweging\" by Eliens (2019)."@en ;
        rdfs:label    "Verre églomisé (Alexandrite Glass)"@en ;
        :Created-By   :Creation_Artwork_44 ;
        :Has-Depth    "28"^^xsd:decimal ;
        :Has-Height   "24"^^xsd:decimal ;
        :Has-Width    "27"^^xsd:decimal ;
        :Is-Unica     "Yes"@en ;
        :Located-In   :NewYork ;
        :Made-By      <http://www.semanticweb.org/ontologies/Daan/2020/BarbaraNanning#Ale%C5%A1Zv%C4%9B%C5%99ina&AZ-Design> , :VáçlavNovák_Doksy_CzechRepublic , :LASVITAJETO , :BarbaraNanning ;
        :Made-Out-Of  <http://www.semanticweb.org/ontologies/Daan/2020/BarbaraNanning#ReichenbachColourRodsGlass(DE)> , :Platinum , :AJETOClearGlass , :AJETOAlexandriteGlass ;
        :Part-Of      :CollectionJ.LohmannGallery ;
        :Shown-By     :Image_Artwork_44 .

:ARTWORK_18_64_Packing
        a              :Packing , owl:NamedIndividual ;
        rdfs:comment   "Instance of an activity which is part of the creation process of ARTWORK_18_64."@en ;
        rdfs:label     "ARTWORK_18_64_Packing"@en ;
        :Followed-By   :ARTWORK_18_64_Transporting ;
        :Follows       :ARTWORK_18_64_Cooling ;
        :Has-Duration  <http://www.semanticweb.org/ontologies/Daan/2020/BarbaraNanning#2015> ;
        :Involves      :BarbaraNanning ;
        :Located-In    :Zaandam ;
        :Part-Of       :Creation_Artwork_18_64 .

:SharpeningStone  a   :Tool , owl:NamedIndividual ;
        rdfs:comment  "A sharpening stone is a tool used to sharpen things by making use of the grains on the stone."@en ;
        rdfs:label    "Sharpening Stone"@en ;
        owl:sameAs    <http://www.wikidata.org/entity/Q507559> ;
        :Used-For     :ARTWORK_43_Grinding , :ARTWORK_77_Grinding , :ARTWORK_73_Grinding , :ARTWORK_75_Grinding , :ARTWORK_44_Grinding , :ARTWORK_76_Grinding , :ARTWORK_78_Grinding , :ARTWORK_80_Grinding , :ARTWORK_74_Grinding , :ARTWORK_79_Grinding .

:Digital_Image  a            owl:Class ;
        rdfs:comment         "A digital image is a representation of an image stored on a digital computer."@en ;
        rdfs:label           "Digital Image"@en ;
        rdfs:subClassOf      :Representation ;
        owl:equivalentClass  <http://www.wikidata.org/entity/Q1250322> .

:ARTWORK_39_Transporting_2
        a              owl:NamedIndividual , :Transporting ;
        rdfs:comment   "Instance of an activity which is part of the creation process of ARTWORK_39."@en ;
        rdfs:label     "ARTWORK_39_Transporting_2"@en ;
        :Followed-By   :ARTWORK_39_Photographing ;
        :Follows       :ARTWORK_39_Packing_2 ;
        :Has-Duration  <http://www.semanticweb.org/ontologies/Daan/2020/BarbaraNanning#2015> ;
        :Involves      :AlešZvěřina , :BarbaraNanning ;
        :Located-In    :Amsterdam ;
        :Part-Of       :Creation_Artwork_39 .

:ARTWORK_73_SetupAndTestingOfTheMetalMold
        a                 :Setup_and_Testing_of_the_Metal_Mold , owl:NamedIndividual ;
        rdfs:comment      "Instance of an activity which is part of the creation process of ARTWORK_73."@en ;
        rdfs:label        "ARTWORK_73_Setup and Testing of the Metal Mold"@en ;
        :Followed-By      :ARTWORK_73_SetupAndTestingOfTheMetalMold_2 ;
        :Follows          :ARTWORK_73_PreparingGlass ;
        :Has-Duration     <http://www.semanticweb.org/ontologies/Daan/2020/BarbaraNanning#2018> ;
        :Involves         <http://www.semanticweb.org/ontologies/Daan/2020/BarbaraNanning#RadekKoten(CZ)> , <http://www.semanticweb.org/ontologies/Daan/2020/BarbaraNanning#Tom%C3%A1%C5%A1Moravec(CZ)> , :AssistantOfBarbara , :BarbaraNanning , <http://www.semanticweb.org/ontologies/Daan/2020/BarbaraNanning#JiriMoravec(CZ)> , <http://www.semanticweb.org/ontologies/Daan/2020/BarbaraNanning#LukasHavlas(CZ)> ;
        :Located-In       :CzechRepublic ;
        :Part-Of          :Creation_Artwork_73 ;
        :Requires-Use-Of  :InterchangeableMetalMoldSetup .

:ARTWORK_17_33_Signing
        a                 owl:NamedIndividual , :Signing ;
        rdfs:comment      "Instance of an activity which is part of the creation process of ARTWORK_17_33."@en ;
        rdfs:label        "ARTWORK_17_33_Signing"@en ;
        :Followed-By      <http://www.semanticweb.org/ontologies/Daan/2020/BarbaraNanning#ARTWORK_17_33_ExaminingQuality(Result)> ;
        :Follows          :ARTWORK_17_33_Polishing ;
        :Has-Duration     <http://www.semanticweb.org/ontologies/Daan/2020/BarbaraNanning#2017> ;
        :Involves         :AlešZvěřina , :BarbaraNanning ;
        :Located-In       :NovyBor ;
        :Part-Of          :Creation_Artwork_17_33 ;
        :Requires-Use-Of  :AirCompressor .

:Grinding_Facets  a      owl:Class ;
        rdfs:comment     "Using a grindstone the cutter applies a small edge to remove the sharp edges of the glass."@en ;
        rdfs:label       "Grinding Facets"@en ;
        rdfs:subClassOf  :Activity .

:ARTWORK_46_DecidingColourPaletteAndPatterns
        a              :Deciding_Colour_Palette_and_Patterns , owl:NamedIndividual ;
        rdfs:comment   "Instance of an activity which is part of the creation process of ARTWORK_46."@en ;
        rdfs:label     "ARTWORK_46_Deciding Colour Palette and Patterns"@en ;
        :Followed-By   :ARTWORK_46_CuttingMonochromeSheets ;
        :Has-Duration  <http://www.semanticweb.org/ontologies/Daan/2020/BarbaraNanning#2015> ;
        :Involves      :BarbaraNanning ;
        :Located-In    :Amsterdam ;
        :Part-Of       :Creation_Artwork_46 ;
        :Processes     :BullseyeGlass ;
        :Starts        :Creation_Artwork_46 .

:ARTWORK_44_ApplyingExtraColour
        a                 :Applying_Extra_Colour , owl:NamedIndividual ;
        rdfs:comment      "Instance of an activity which is part of the creation process of ARTWORK_44."@en ;
        rdfs:label        "ARTWORK_44_Applying Extra Colour"@en ;
        :Followed-By      :ARTWORK_44_ApplyingExtraColour_2 ;
        :Follows          :ARTWORK_44_ApplyingClearGlassBell ;
        :Has-Duration     <http://www.semanticweb.org/ontologies/Daan/2020/BarbaraNanning#2018> ;
        :Involves         :BarbaraNanning , <http://www.semanticweb.org/ontologies/Daan/2020/BarbaraNanning#LukasHavlas(CZ)> , <http://www.semanticweb.org/ontologies/Daan/2020/BarbaraNanning#RadekKoten(CZ)> ;
        :Located-In       :CzechRepublic ;
        :Part-Of          :Creation_Artwork_44 ;
        :Processes        <http://www.semanticweb.org/ontologies/Daan/2020/BarbaraNanning#ReichenbachColourRodsGlass(DE)> ;
        :Requires-Use-Of  :Tagliol , :AnnealingKiln , :DiamondShears , :Furnace , :BlowingPipe , :AirCompressor , :YokeOfSupport , :Pincet , :Jacks , :Paper , :Blocks , :Beeswax , :IcePick , :Hook , :CeramicPotFilledWithGlass , :Water , :Pontis , :StraightShears , :Garage , :GloryHole , :Fork , :Marver .

:Used-For  a          owl:ObjectProperty ;
        rdfs:comment  "Used-For is a property which connects a tool or equipment of which an activity requires usage."@en ;
        rdfs:domain   :Equipment ;
        rdfs:label    "Used-For"@en ;
        rdfs:range    :Activity .

:ARTWORK_76_Modeling  a   :Modeling , owl:NamedIndividual ;
        rdfs:comment      "Instance of an activity which is part of the creation process of ARTWORK_76."@en ;
        rdfs:label        "ARTWORK_76_Modeling"@en ;
        :Followed-By      <http://www.semanticweb.org/ontologies/Daan/2020/BarbaraNanning#ARTWORK_76_ExaminingQuality(Shape/Form)> ;
        :Follows          :ARTWORK_76_Sensing ;
        :Has-Duration     <http://www.semanticweb.org/ontologies/Daan/2020/BarbaraNanning#2018> ;
        :Involves         :AssistantOfBarbara , <http://www.semanticweb.org/ontologies/Daan/2020/BarbaraNanning#LukasHavlas(CZ)> , :BarbaraNanning , <http://www.semanticweb.org/ontologies/Daan/2020/BarbaraNanning#RadekKoten(CZ)> , <http://www.semanticweb.org/ontologies/Daan/2020/BarbaraNanning#Tom%C3%A1%C5%A1Moravec(CZ)> , <http://www.semanticweb.org/ontologies/Daan/2020/BarbaraNanning#JiriMoravec(CZ)> ;
        :Located-In       :CzechRepublic ;
        :Part-Of          :Creation_Artwork_76 ;
        :Requires-Use-Of  :AirCompressor , :BlowingPipe , :InterchangeableMetalMoldSetup , :Gloves , :PropaneTorch .

:Langweer  a          owl:NamedIndividual , :City ;
        rdfs:comment  "Langweer is a town in the Netherlands."@en ;
        rdfs:label    "Langweer"@en ;
        owl:sameAs    <http://sws.geonames.org/2751888> ;
        :Located-In   :Netherlands ;
        :Location-Of  :ARTWORK_18_64_Casting , :ARTWORK_18_64_TransportingMonochromeRods , :ARTWORK_46_Casting , :ARTWORK_18_64_CuttingMonochromeSheets , :ARTWORK_36_TransportingMonochromeRods , :ARTWORK_46_Ordening , :ARTWORK_46_CuttingMonochromeSheets , :ARTWORK_36_Casting , :BullseyeGlassSplinterEnDeVosch , :ARTWORK_18_64_Ordening , :ARTWORK_36_Ordening , :ARTWORK_46_TransportingMonochromeRods , :ARTWORK_36_CuttingMonochromeSheets .

:Grinder  a              owl:Class ;
        rdfs:comment     "A Grinder is an actor who is responsible for the grinding, polishing and sharpening of objects."@en ;
        rdfs:label       "Grinder"@en ;
        rdfs:subClassOf  :Person .

:Involved-In  a        owl:ObjectProperty ;
        rdfs:comment   "Involved-In is a property which connects an actor with an activity."@en ;
        rdfs:domain    :Actor ;
        rdfs:label     "Involved-In"@en ;
        rdfs:range     :Activity ;
        owl:inverseOf  :Involves .

<http://www.semanticweb.org/ontologies/Daan/2020/BarbaraNanning#AlesVacek(CZ)>
        a             owl:NamedIndividual , :Master_Glass_Blower ;
        rdfs:comment  "Ales Vacek (CZ) is a Master Glass Blower."@en ;
        rdfs:label    "Ales Vacek (CZ)"@en ;
        :Involved-In  <http://www.semanticweb.org/ontologies/Daan/2020/BarbaraNanning#ARTWORK_74_ExaminingQuality(Shape/Form)> , :ARTWORK_43_ExaminingTheQualityOfTheGlass , <http://www.semanticweb.org/ontologies/Daan/2020/BarbaraNanning#ARTWORK_43_ExaminingQuality(Shape/Form)> , :ARTWORK_43_ApplyingClearGlassBell , :ARTWORK_44_Modeling , :ARTWORK_78_ApplyingClearGlassBell , :ARTWORK_78_ApplyingExtraColour , :ARTWORK_78_Modeling , :ARTWORK_44_ApplyingExtraColour , :ARTWORK_74_PreparingGlass , :ARTWORK_74_ApplyingClearGlassBell , :ARTWORK_74_SetupAndTestingOfTheMetalMold , <http://www.semanticweb.org/ontologies/Daan/2020/BarbaraNanning#ARTWORK_44_ExaminingQuality(Shape/Form)> , :ARTWORK_78_Sensing , :ARTWORK_74_Modeling , :ARTWORK_44_PreparingGlass , :ARTWORK_78_SetupAndTestingOfTheMetalMold , :ARTWORK_43_Modeling , :ARTWORK_43_Glassblowing , :ARTWORK_44_ApplyingClearGlassBell , :ARTWORK_74_Sensing , :ARTWORK_44_ApplyingExtraColour_2 , :ARTWORK_43_SetupAndTestingOfTheMetalMold , :ARTWORK_44_ExaminingTheQualityOfTheGlass , :ARTWORK_44_SetupAndTestingOfTheMetalMold_2 , :ARTWORK_44_Glassblowing , :ARTWORK_43_ApplyingExtraColour , :ARTWORK_74_Glassblowing , <http://www.semanticweb.org/ontologies/Daan/2020/BarbaraNanning#ARTWORK_78_ExaminingQuality(Shape/Form)> , :ARTWORK_74_SetupAndTestingOfTheMetalMold_2 , :ARTWORK_78_SetupAndTestingOfTheMetalMold_2 , :ARTWORK_74_ApplyingExtraColour_2 , :ARTWORK_43_SetupAndTestingOfTheMetalMold_2 , :ARTWORK_43_Sensing , :ARTWORK_78_ExaminingTheQualityOfTheGlass , :ARTWORK_44_Sensing , :ARTWORK_74_ExaminingTheQualityOfTheGlass , :ARTWORK_78_PreparingGlass , :ARTWORK_43_PreparingGlass , :ARTWORK_44_SetupAndTestingOfTheMetalMold , :ARTWORK_78_Glassblowing , :ARTWORK_74_ApplyingExtraColour ;
        :Works-For    :LASVITAJETO .

:ARTWORK_36_Glassblowing
        a                 :Glassblowing , owl:NamedIndividual ;
        rdfs:comment      "Instance of an activity which is part of the creation process of ARTWORK_36."@en ;
        rdfs:label        "ARTWORK_36_Glassblowing"@en ;
        :Followed-By      :ARTWORK_36_Sensing ;
        :Follows          :ARTWORK_36_HeatingMetalMold ;
        :Has-Duration     <http://www.semanticweb.org/ontologies/Daan/2020/BarbaraNanning#2015> ;
        :Involves         :BarbaraNanning , <http://www.semanticweb.org/ontologies/Daan/2020/BarbaraNanning#JessicaHomich(USA)> , <http://www.semanticweb.org/ontologies/Daan/2020/BarbaraNanning#MarekBrathko(CZ)> , <http://www.semanticweb.org/ontologies/Daan/2020/BarbaraNanning#MarekEffmert(CZ)> , <http://www.semanticweb.org/ontologies/Daan/2020/BarbaraNanning#RobertLenner(CZ)> , :GertBullée , <http://www.semanticweb.org/ontologies/Daan/2020/BarbaraNanning#MiaLerssi(DN)> ;
        :Located-In       :Zaandam ;
        :Part-Of          :Creation_Artwork_36 ;
        :Requires-Use-Of  :StraightShears , :Pincet , :Marver , :Water , :Beeswax , :PropaneTorch , :Jacks , :Fork , :BlowingPipe , :Paper , :InterchangeableMetalMoldSetup , :Blocks , :Tagliol , :YokeOfSupport , :IcePick , :DiamondShears , :Furnace , :AirCompressor , :AnnealingKiln , :Gloves , :BitIron , :Pontis , :GloryHole , :Hook , :CeramicPotFilledWithGlass .

<http://vocab.getty.edu/aat/300209549>
        a           owl:NamedIndividual ;
        owl:sameAs  :IcePick .

<http://www.semanticweb.org/ontologies/Daan/2020/BarbaraNanning#ARTWORK_73_ExaminingQuality(Shape/Form)>
        a                 owl:NamedIndividual , j.2: ;
        rdfs:comment      "Instance of an activity which is part of the creation process of ARTWORK_73."@en ;
        rdfs:label        "ARTWORK_73_Examining Quality (Shape/Form)"@en ;
        :Followed-By      :ARTWORK_73_Translocating ;
        :Follows          :ARTWORK_73_Modeling ;
        :Has-Duration     <http://www.semanticweb.org/ontologies/Daan/2020/BarbaraNanning#2018> ;
        :Involves         <http://www.semanticweb.org/ontologies/Daan/2020/BarbaraNanning#RadekKoten(CZ)> , :BarbaraNanning , :LuděkKout ;
        :Located-In       :CzechRepublic ;
        :Part-Of          :Creation_Artwork_73 ;
        :Requires-Use-Of  :BlowingPipe , :GloryHole , :Pontis .

<http://www.wikidata.org/entity/Q73411516>
        a       owl:NamedIndividual .

:ARTWORK_36_MeasuringAndBoxesMaking
        a              :Measuring_and_Boxes_Making , owl:NamedIndividual ;
        rdfs:comment   "Instance of an activity which is part of the creation process of ARTWORK_36."@en ;
        rdfs:label     "ARTWORK_36_Measuring and Boxes Making"@en ;
        :Followed-By   :ARTWORK_36_Packing_2 ;
        :Follows       <http://www.semanticweb.org/ontologies/Daan/2020/BarbaraNanning#ARTWORK_36_ExaminingQuality(Result)> ;
        :Has-Duration  <http://www.semanticweb.org/ontologies/Daan/2020/BarbaraNanning#2015> ;
        :Involves      :BarbaraNanning , :AlešZvěřina ;
        :Located-In    :NovyBor ;
        :Part-Of       :Creation_Artwork_36 .

<http://www.semanticweb.org/ontologies/Daan/2020/BarbaraNanning#2016>
        a             owl:NamedIndividual , :Timespan ;
        rdfs:comment  "2016 is a Timespan."@en ;
        rdfs:label    "2016"@en ;
        owl:sameAs    <http://www.wikidata.org/entity/Q25245> ;
        :Duration-Of  :Creation_Artwork_78 .

:ARTWORK_39_PickingUpColouredPanel
        a                 :Picking_up_Coloured_Panel , owl:NamedIndividual ;
        rdfs:comment      "Instance of an activity which is part of the creation process of ARTWORK_39."@en ;
        rdfs:label        "ARTWORK_39_Picking up Coloured Panel"@en ;
        :Followed-By      :ARTWORK_39_HeatingMetalMold ;
        :Follows          :ARTWORK_39_ApplyingClearGlassBell ;
        :Has-Duration     <http://www.semanticweb.org/ontologies/Daan/2020/BarbaraNanning#2015> ;
        :Involves         <http://www.semanticweb.org/ontologies/Daan/2020/BarbaraNanning#MarekBrathko(CZ)> , <http://www.semanticweb.org/ontologies/Daan/2020/BarbaraNanning#RobertLenner(CZ)> , <http://www.semanticweb.org/ontologies/Daan/2020/BarbaraNanning#JessicaHomich(USA)> , :GertBullée , <http://www.semanticweb.org/ontologies/Daan/2020/BarbaraNanning#MarekEffmert(CZ)> , :BarbaraNanning , <http://www.semanticweb.org/ontologies/Daan/2020/BarbaraNanning#MiaLerssi(DN)> ;
        :Located-In       :Zaandam ;
        :Part-Of          :Creation_Artwork_39 ;
        :Requires-Use-Of  :Water , :Tagliol , :Furnace , :Hook , :Marver , :Pontis , :Blocks , :Beeswax , :StraightShears , :AirCompressor , :Fork , :FusingKiln , :Garage , :GrindingWheel , :Jacks , :YokeOfSupport , :Paper , :PropaneTorch , :AnnealingKiln , :Gloves , :DiamondShears , :BlowingPipe , :GloryHole .

<http://www.wikidata.org/entity/Q11514315>
        a       owl:Class .

:ARTWORK_43_Sawing  a     owl:NamedIndividual , :Sawing ;
        rdfs:comment      "Instance of an activity which is part of the creation process of ARTWORK_43."@en ;
        rdfs:label        "ARTWORK_43_Sawing"@en ;
        :Followed-By      <http://www.semanticweb.org/ontologies/Daan/2020/BarbaraNanning#ARTWORK_43_ExaminingQuality(CheckForIrregularitiesInTheGlass)> ;
        :Follows          :ARTWORK_43_Grinding ;
        :Has-Duration     <http://www.semanticweb.org/ontologies/Daan/2020/BarbaraNanning#2008> ;
        :Involves         :AlešZvěřina , :BarbaraNanning ;
        :Located-In       :CzechRepublic ;
        :Part-Of          :Creation_Artwork_43 ;
        :Requires-Use-Of  :DiamondSaw .

:Cutting_Sheets  a       owl:Class ;
        rdfs:comment     "A cutter cuts the galss sheets with the help of Diamond scissor or Diamond saw."@en ;
        rdfs:label       "Cutting Sheets"@en ;
        rdfs:subClassOf  :Activity .

<http://www.wikidata.org/entity/Q143739>
        a       owl:NamedIndividual .

:ARTWORK_43_Transporting_4
        a              owl:NamedIndividual , :Transporting ;
        rdfs:comment   "Instance of an activity which is part of the creation process of ARTWORK_43."@en ;
        rdfs:label     "ARTWORK_43_Transporting_4"@en ;
        :Followed-By   :ARTWORK_43_Photographing ;
        :Follows       :ARTWORK_43_Packing_4 ;
        :Has-Duration  <http://www.semanticweb.org/ontologies/Daan/2020/BarbaraNanning#2008> ;
        :Involves      :BarbaraNanning , :AlešZvěřina ;
        :Located-In    :CzechRepublic ;
        :Part-Of       :Creation_Artwork_43 .

:ARTWORK_76_PreparingGlass
        a                 owl:NamedIndividual , :Preparing_Glass ;
        rdfs:comment      "Instance of an activity which is part of the creation process of ARTWORK_76."@en ;
        rdfs:label        "ARTWORK_76_Preparing Glass"@en ;
        :Followed-By      :ARTWORK_76_SetupAndTestingOfTheMetalMold ;
        :Has-Duration     <http://www.semanticweb.org/ontologies/Daan/2020/BarbaraNanning#2018> ;
        :Involves         <http://www.semanticweb.org/ontologies/Daan/2020/BarbaraNanning#RadekKoten(CZ)> , :BarbaraNanning ;
        :Located-In       :CzechRepublic ;
        :Part-Of          :Creation_Artwork_76 ;
        :Requires-Use-Of  :GloryHole , :Garage , :Pontis , :Marver , :BlowingPipe ;
        :Starts           :Creation_Artwork_76 .

<http://www.semanticweb.org/ontologies/Daan/2020/BarbaraNanning#ARTWORK_39_ExaminingQuality(FinalResult)>
        a              owl:NamedIndividual , j.1: ;
        rdfs:comment   "Instance of an activity which is part of the creation process of ARTWORK_39."@en ;
        rdfs:label     "ARTWORK_39_Examining Quality (Result)"@en ;
        :Followed-By   :ARTWORK_39_Packing_2 ;
        :Follows       :ARTWORK_39_Signing ;
        :Has-Duration  <http://www.semanticweb.org/ontologies/Daan/2020/BarbaraNanning#2015> ;
        :Involves      :AlešZvěřina , :BarbaraNanning ;
        :Located-In    :NovyBor ;
        :Part-Of       :Creation_Artwork_39 .

:ARTWORK_77_Transporting_2
        a              owl:NamedIndividual , :Transporting ;
        rdfs:comment   "Instance of an activity which is part of the creation process of ARTWORK_77."@en ;
        rdfs:label     "ARTWORK_77_Transporting_2"@en ;
        :Followed-By   :ARTWORK_77_Signing ;
        :Follows       :ARTWORK_77_Packing_2 ;
        :Has-Duration  <http://www.semanticweb.org/ontologies/Daan/2020/BarbaraNanning#2018> ;
        :Involves      :AlešZvěřina , :BarbaraNanning ;
        :Located-In    :CzechRepublic ;
        :Part-Of       :Creation_Artwork_77 .

:ARTWORK_18_64_TransportingMetalBowlWithSheet
        a              :Transporting_Metal_Bowl_with_Sheet , owl:NamedIndividual ;
        rdfs:comment   "Instance of an activity which is part of the creation process of ARTWORK_18_64."@en ;
        rdfs:label     "ARTWORK_18_64_Transporting Metal Bowl with Sheet"@en ;
        :Followed-By   :ARTWORK_18_64_PreparingForBlowing ;
        :Follows       :ARTWORK_18_64_RoundingByGrindingTheSheet ;
        :Has-Duration  <http://www.semanticweb.org/ontologies/Daan/2020/BarbaraNanning#2015> ;
        :Involves      :BarbaraNanning ;
        :Located-In    :Lindava ;
        :Part-Of       :Creation_Artwork_18_64 .

:Ordening  a             owl:Class ;
        rdfs:comment     "Orderning is the activity in which objects are placed in a specific order."@en ;
        rdfs:label       "Ordening"@en ;
        rdfs:subClassOf  :Activity .

:ARTWORK_43_ExaminingTheQualityOfTheGlass
        a                 :Examining_the_Quality_of_the_Glass , owl:NamedIndividual ;
        rdfs:comment      "Instance of an activity which is part of the creation process of ARTWORK_43."@en ;
        rdfs:label        "ARTWORK_43_Examining the Quality of the Glass"@en ;
        :Followed-By      :ARTWORK_43_Cooling ;
        :Follows          :ARTWORK_43_Modeling ;
        :Has-Duration     <http://www.semanticweb.org/ontologies/Daan/2020/BarbaraNanning#2008> ;
        :Involves         <http://www.semanticweb.org/ontologies/Daan/2020/BarbaraNanning#AlesVacek(CZ)> , :BarbaraNanning , :LuděkKout ;
        :Located-In       :CzechRepublic ;
        :Part-Of          :Creation_Artwork_43 ;
        :Requires-Use-Of  :Pontis , :GloryHole , :Furnace , :Jacks , :YokeOfSupport , :StraightShears , :CeramicPotFilledWithGlass , :DiamondShears , :AnnealingKiln , :BlowingPipe , :Water , :Blocks , :Paper .

:Potassium  a             owl:NamedIndividual , :Natural_Material ;
        rdfs:comment      "Potassium is a silvery-white metal material with the chemical element of atomic number 19. It is used to add brightness to the glass."@en ;
        rdfs:label        "Potassium"@en ;
        owl:sameAs        <http://www.wikidata.org/entity/Q703> ;
        :Is-Processed-In  :AJETOBlueGlass , :AJETOBlackGlass , :AJETOWhiteGlass , :AJETOGreenGlass , :AJETOAmberGlass , :AJETORedGlass , :AJETOClearGlass , :AJETOSmokeGlass .

<http://www.semanticweb.org/ontologies/Daan/2020/BarbaraNanning#ARTWORK_44_ExaminingQuality(CheckForIrregularitiesInTheGlass)>
        a              j.3: , owl:NamedIndividual ;
        rdfs:comment   "Instance of an activity which is part of the creation process of ARTWORK_44."@en ;
        rdfs:label     "ARTWORK_44_Examining Quality (Check for Irregularities in the Glass)"@en ;
        :Followed-By   :ARTWORK_44_Sawing ;
        :Follows       :ARTWORK_44_Resting ;
        :Has-Duration  <http://www.semanticweb.org/ontologies/Daan/2020/BarbaraNanning#2018> ;
        :Involves      :BarbaraNanning , :AlešZvěřina ;
        :Located-In    :CzechRepublic ;
        :Part-Of       :Creation_Artwork_44 .

:AJETOSmokeGlass  a           :AJETO_Glass , owl:NamedIndividual ;
        rdfs:comment          "AJETO Smoke is a form of AJETO glass with a smoke colour."@en ;
        rdfs:label            "AJETO Smoke Glass"@en ;
        :Availability         "Available"@en ;
        :Is-Processed-During  :ARTWORK_77_ApplyingExtraColour ;
        :Is-Processed-In      :Artwork_77 ;
        :Made-By              :LASVITAJETO ;
        :Made-Out-Of          :Calcium , :Soda , :Sand , :Potassium ;
        :Transparency         "Transparent"@en .

:ARTWORK_18_64_OrdeningFlatSheets
        a                 :Ordering_Flat_Sheets , owl:NamedIndividual ;
        rdfs:comment      "Instance of an activity which is part of the creation process of ARTWORK_18_64."@en ;
        rdfs:label        "ARTWORK_18_64_Ordening Flat Sheets"@en ;
        :Followed-By      :ARTWORK_18_64_FusingSheets ;
        :Follows          :ARTWORK_18_64_CuttingSheets ;
        :Has-Duration     <http://www.semanticweb.org/ontologies/Daan/2020/BarbaraNanning#2015> ;
        :Involves         :BarbaraNanning ;
        :Located-In       :Amsterdam ;
        :Part-Of          :Creation_Artwork_18_64 ;
        :Requires-Use-Of  :FusingKiln .

:ARTWORK_39_Packing  a  owl:NamedIndividual , :Packing ;
        rdfs:comment   "Instance of an activity which is part of the creation process of ARTWORK_39."@en ;
        rdfs:label     "ARTWORK_39_Packing"@en ;
        :Followed-By   :ARTWORK_39_Transporting ;
        :Follows       :ARTWORK_39_Cooling ;
        :Has-Duration  <http://www.semanticweb.org/ontologies/Daan/2020/BarbaraNanning#2015> ;
        :Involves      :BarbaraNanning ;
        :Located-In    :Zaandam ;
        :Part-Of       :Creation_Artwork_39 .

:ARTWORK_46_Packing  a  owl:NamedIndividual , :Packing ;
        rdfs:comment   "Instance of an activity which is part of the creation process of ARTWORK_46."@en ;
        rdfs:label     "ARTWORK_46_Packing"@en ;
        :Followed-By   :ARTWORK_46_Transporting ;
        :Follows       :ARTWORK_46_Cooling ;
        :Has-Duration  <http://www.semanticweb.org/ontologies/Daan/2020/BarbaraNanning#2018> ;
        :Involves      :BarbaraNanning ;
        :Located-In    :Lindava ;
        :Part-Of       :Creation_Artwork_46 .

:ARTWORK_36_Cooling_2
        a                 owl:NamedIndividual , :Cooling ;
        rdfs:comment      "Instance of an activity which is part of the creation process of ARTWORK_36."@en ;
        rdfs:label        "ARTWORK_36_Cooling_2"@en ;
        :Followed-By      :ARTWORK_36_Packing_5 ;
        :Follows          <http://www.semanticweb.org/ontologies/Daan/2020/BarbaraNanning#ARTWORK_36_ExaminingQuality(Shape/Form)_2> ;
        :Has-Duration     <http://www.semanticweb.org/ontologies/Daan/2020/BarbaraNanning#2019> ;
        :Involves         :JaroslavKubásek , <http://www.semanticweb.org/ontologies/Daan/2020/BarbaraNanning#JiriPacinek(CZ)> , <http://www.semanticweb.org/ontologies/Daan/2020/BarbaraNanning#JessicaHomich(USA)> ;
        :Located-In       :Lindava ;
        :Part-Of          :Creation_Artwork_36 ;
        :Requires-Use-Of  :AnnealingKiln .

j.0:    a                owl:Class ;
        rdfs:comment     "Examining Quality (Result) is an activity conducted by a creator in which the quality of a thing is assured after the completion of an activity."@en ;
        rdfs:label       "Examining Quality (Result)"@en ;
        rdfs:subClassOf  :Activity .

<http://vocab.getty.edu/aat/300215302>
        a                    owl:Class ;
        owl:equivalentClass  :Digital_Image .

:ARTWORK_36_OrdeningFlatSheets
        a                 :Ordering_Flat_Sheets , owl:NamedIndividual ;
        rdfs:comment      "Instance of an activity which is part of the creation process of ARTWORK_36."@en ;
        rdfs:label        "ARTWORK_36_Ordening Flat Sheets"@en ;
        :Followed-By      :ARTWORK_36_FusingSheets ;
        :Follows          :ARTWORK_36_CuttingSheets ;
        :Has-Duration     <http://www.semanticweb.org/ontologies/Daan/2020/BarbaraNanning#2019> ;
        :Involves         :BarbaraNanning ;
        :Located-In       :Amsterdam ;
        :Part-Of          :Creation_Artwork_36 ;
        :Requires-Use-Of  :FusingKiln .

:Slumping_Panel  a       owl:Class ;
        rdfs:comment     "The flat glass that is molded and when reheated will create the final form."@en ;
        rdfs:label       "Slumping Panel"@en ;
        rdfs:subClassOf  :Slumping .

:ARTWORK_46_MeasuringAndBoxesMaking
        a              :Measuring_and_Boxes_Making , owl:NamedIndividual ;
        rdfs:comment   "Instance of an activity which is part of the creation process of ARTWORK_46."@en ;
        rdfs:label     "ARTWORK_46_Measuring and Boxes Making"@en ;
        :Followed-By   :ARTWORK_46_Packing_2 ;
        :Follows       <http://www.semanticweb.org/ontologies/Daan/2020/BarbaraNanning#ARTWORK_46_ExaminingQuality(Result)> ;
        :Has-Duration  <http://www.semanticweb.org/ontologies/Daan/2020/BarbaraNanning#2018> ;
        :Involves      :AlešZvěřina , :BarbaraNanning ;
        :Located-In    :NovyBor ;
        :Part-Of       :Creation_Artwork_46 .

:ARTWORK_46_Transporting
        a              :Transporting , owl:NamedIndividual ;
        rdfs:comment   "Instance of an activity which is part of the creation process of ARTWORK_46."@en ;
        rdfs:label     "ARTWORK_46_Transporting"@en ;
        :Followed-By   :ARTWORK_46_Resting ;
        :Follows       :ARTWORK_46_Packing ;
        :Has-Duration  <http://www.semanticweb.org/ontologies/Daan/2020/BarbaraNanning#2018> ;
        :Involves      :AlešZvěřina , :BarbaraNanning ;
        :Located-In    :NovyBor ;
        :Part-Of       :Creation_Artwork_46 .

:ARTWORK_39_CuttingSheets
        a                 owl:NamedIndividual , :Cutting_Sheets ;
        rdfs:comment      "Instance of an activity which is part of the creation process of ARTWORK_39."@en ;
        rdfs:label        "ARTWORK_39_Cutting Sheets"@en ;
        :Followed-By      :ARTWORK_39_CuttingStrings ;
        :Follows          :ARTWORK_39_OrdeningMonochromeSheetsAndStrings ;
        :Has-Duration     <http://www.semanticweb.org/ontologies/Daan/2020/BarbaraNanning#2015> ;
        :Involves         :BarbaraNanning , <http://www.semanticweb.org/ontologies/Daan/2020/BarbaraNanning#FredStikvoort(NL)> , <http://www.semanticweb.org/ontologies/Daan/2020/BarbaraNanning#PaulGroot(NL)> , <http://www.semanticweb.org/ontologies/Daan/2020/BarbaraNanning#AbHylkema(NL)> ;
        :Located-In       :Amsterdam ;
        :Part-Of          :Creation_Artwork_39 ;
        :Requires-Use-Of  :DiamondSaw , :Water , :SharpeningStone .

<http://www.semanticweb.org/ontologies/Daan/2020/BarbaraNanning#ARTWORK_36_ExaminingQuality(Result)_2>
        a              j.0: , owl:NamedIndividual ;
        rdfs:comment   "Instance of an activity which is part of the creation process of ARTWORK_36."@en ;
        rdfs:label     "ARTWORK_36_Examining Quality (Result)_2"@en ;
        :Followed-By   :ARTWORK_36_MeasuringAndBoxesMaking_2 ;
        :Follows       :ARTWORK_36_Polishing_2 ;
        :Has-Duration  <http://www.semanticweb.org/ontologies/Daan/2020/BarbaraNanning#2019> ;
        :Involves      :BarbaraNanning , :AlešZvěřina ;
        :Located-In    :NovyBor ;
        :Part-Of       :Creation_Artwork_36 .

:Creator  a              owl:Class ;
        rdfs:comment     "A creator is an actor who brings an object into existence."@en ;
        rdfs:label       "Creator"@en ;
        rdfs:subClassOf  :Person .

:ARTWORK_75_Packing_3
        a              :Packing , owl:NamedIndividual ;
        rdfs:comment   "Instance of an activity which is part of the creation process of ARTWORK_75."@en ;
        rdfs:label     "ARTWORK_75_Packing_3"@en ;
        :Followed-By   :ARTWORK_75_Transporting_3 ;
        :Follows       :ARTWORK_75_Signing ;
        :Has-Duration  <http://www.semanticweb.org/ontologies/Daan/2020/BarbaraNanning#2018> ;
        :Involves      :AlešZvěřina , :BarbaraNanning ;
        :Located-In    :CzechRepublic ;
        :Part-Of       :Creation_Artwork_75 .

:Acquired  a           owl:ObjectProperty ;
        rdfs:comment   "Acquired is a property which connects a thing with an (possibly previous) owner of the thing."@en ;
        rdfs:domain    :Actor ;
        rdfs:label     "Acquired"@en ;
        rdfs:range     :Thing ;
        owl:inverseOf  :Acquired-By .

:ARTWORK_44_ApplyingClearGlassBell
        a                 owl:NamedIndividual , :Applying_Clear_Glass_Bell ;
        rdfs:comment      "Instance of an activity which is part of the creation process of ARTWORK_44."@en ;
        rdfs:label        "ARTWORK_44_Applying Clear Glass Bell"@en ;
        :Followed-By      :ARTWORK_44_ApplyingExtraColour ;
        :Follows          :ARTWORK_44_SetupAndTestingOfTheMetalMold_2 ;
        :Has-Duration     <http://www.semanticweb.org/ontologies/Daan/2020/BarbaraNanning#2018> ;
        :Involves         :BarbaraNanning , <http://www.semanticweb.org/ontologies/Daan/2020/BarbaraNanning#RadekKoten(CZ)> , <http://www.semanticweb.org/ontologies/Daan/2020/BarbaraNanning#LukasHavlas(CZ)> ;
        :Located-In       :CzechRepublic ;
        :Part-Of          :Creation_Artwork_44 ;
        :Processes        :AJETOClearGlass ;
        :Requires-Use-Of  :StraightShears , :Paper , :Pincet , :YokeOfSupport , :Jacks , :IcePick , :Water , :BlowingPipe , :Furnace , :Blocks , :DiamondShears , :Beeswax , :Marver , :AirCompressor , :Hook , :CeramicPotFilledWithGlass .

:Preparing_Glass  a      owl:Class ;
        rdfs:comment     "Preparing Glass in an activity in which an actor is melting glass or preparing colour."@en ;
        rdfs:label       "Preparing Glass"@en ;
        rdfs:subClassOf  :Activity .

<http://www.semanticweb.org/ontologies/Daan/2020/BarbaraNanning#TomHaartsen_Ouderkerka/dAmstel(NL)>
        a             owl:NamedIndividual , :Photographer ;
        rdfs:comment  "Tom Haartsen_Ouderkerk a/d Amstel (NL) is a Photographer."@en ;
        rdfs:label    "Tom Haartsen_Ouderkerk a/d Amstel (NL)"@en ;
        owl:sameAs    <http://www.wikidata.org/entity/Q73411516> ;
        :Involved-In  :ARTWORK_80_Photographing , :ARTWORK_74_Photographing , :ARTWORK_78_Photographing , :ARTWORK_75_Photographing , :ARTWORK_44_Photographing , :ARTWORK_43_Photographing , :ARTWORK_76_Photographing , :ARTWORK_77_Photographing , :ARTWORK_79_Photographing , :ARTWORK_73_Photographing .

:ARTWORK_36_CuttingAndPolishingCastedMonochromeSheetsToSmallRods
        a                 :Cutting_and_Polishing_Casted_Monochrome_Sheets_to_Small_Rods , owl:NamedIndividual ;
        rdfs:comment      "Instance of an activity which is part of the creation process of ARTWORK_36."@en ;
        rdfs:label        "ARTWORK_36_Cutting and Polishing Casted Monochrome Sheets to Small Rods"@en ;
        :Followed-By      :ARTWORK_36_DecidingColourPaletteAndPatterns_2 ;
        :Follows          :ARTWORK_36_Casting ;
        :Has-Duration     <http://www.semanticweb.org/ontologies/Daan/2020/BarbaraNanning#2015> ;
        :Involves         :BarbaraNanning ;
        :Located-In       :Amsterdam ;
        :Part-Of          :Creation_Artwork_36 ;
        :Requires-Use-Of  :Water , :SharpeningStone , :DiamondSaw .

:Gilding  a              owl:Class ;
        rdfs:comment     "Gilding is an activity in which gold leaf is applied on a thing."@en ;
        rdfs:label       "Gilding"@en ;
        rdfs:subClassOf  :Activity .

:Signing  a              owl:Class ;
        rdfs:comment     "Signing is an activity in which an signature is added to a thing."@en ;
        rdfs:label       "Signing"@en ;
        rdfs:subClassOf  :Sandblasting .

:ARTWORK_76_Sawing  a     :Sawing , owl:NamedIndividual ;
        rdfs:comment      "Instance of an activity which is part of the creation process of ARTWORK_76."@en ;
        rdfs:label        "ARTWORK_76_Sawing"@en ;
        :Followed-By      :ARTWORK_76_Grinding ;
        :Follows          <http://www.semanticweb.org/ontologies/Daan/2020/BarbaraNanning#ARTWORK_76_ExaminingQuality(CheckForIrregularitiesInTheGlass)> ;
        :Has-Duration     <http://www.semanticweb.org/ontologies/Daan/2020/BarbaraNanning#2018> ;
        :Involves         :BarbaraNanning , :AlešZvěřina ;
        :Located-In       :CzechRepublic ;
        :Part-Of          :Creation_Artwork_76 ;
        :Requires-Use-Of  :DiamondSaw .

:ARTWORK_74_Polishing
        a                 owl:NamedIndividual , :Polishing ;
        rdfs:comment      "Instance of an activity which is part of the creation process of ARTWORK_74."@en ;
        rdfs:label        "ARTWORK_74_Polishing"@en ;
        :Followed-By      <http://www.semanticweb.org/ontologies/Daan/2020/BarbaraNanning#ARTWORK_74_ExaminingQuality(Result)> ;
        :Follows          :ARTWORK_74_Grinding ;
        :Has-Duration     <http://www.semanticweb.org/ontologies/Daan/2020/BarbaraNanning#2008> ;
        :Involves         :AlešZvěřina , :LukášSvoboda , :BarbaraNanning ;
        :Located-In       :CzechRepublic ;
        :Part-Of          :Creation_Artwork_74 ;
        :Requires-Use-Of  :PolishingStone .

<http://www.wikidata.org/entity/Q586319>
        a       owl:NamedIndividual .

:ARTWORK_17_33_Sensing_2
        a              :Sensing , owl:NamedIndividual ;
        rdfs:comment   "Instance of an activity which is part of the creation process of ARTWORK_17_33."@en ;
        rdfs:label     "ARTWORK_17_33_Sensing_2"@en ;
        :Followed-By   :ARTWORK_17_33_Grinding ;
        :Follows       :ARTWORK_17_33_Sawing ;
        :Has-Duration  <http://www.semanticweb.org/ontologies/Daan/2020/BarbaraNanning#2017> ;
        :Involves      :LukášSvoboda , :AlešZvěřina , :BarbaraNanning ;
        :Located-In    :NovyBor ;
        :Part-Of       :Creation_Artwork_17_33 .

:ARTWORK_77_SetupAndTestingOfTheMetalMold_2
        a                 owl:NamedIndividual , :Setup_and_Testing_of_the_Metal_Mold ;
        rdfs:comment      "Instance of an activity which is part of the creation process of ARTWORK_77."@en ;
        rdfs:label        "ARTWORK_77_Setup and Testing of the Metal Mold_2"@en ;
        :Followed-By      :ARTWORK_77_ExaminingTheQualityOfTheGlass ;
        :Follows          :ARTWORK_77_SetupAndTestingOfTheMetalMold ;
        :Has-Duration     <http://www.semanticweb.org/ontologies/Daan/2020/BarbaraNanning#2018> ;
        :Involves         :BarbaraNanning , <http://www.semanticweb.org/ontologies/Daan/2020/BarbaraNanning#JiriMoravec(CZ)> , <http://www.semanticweb.org/ontologies/Daan/2020/BarbaraNanning#LukasHavlas(CZ)> , <http://www.semanticweb.org/ontologies/Daan/2020/BarbaraNanning#RadekKoten(CZ)> , <http://www.semanticweb.org/ontologies/Daan/2020/BarbaraNanning#Tom%C3%A1%C5%A1Moravec(CZ)> , :AssistantOfBarbara ;
        :Located-In       :CzechRepublic ;
        :Part-Of          :Creation_Artwork_77 ;
        :Requires-Use-Of  :InterchangeableMetalMoldSetup .

:Jacks  a             :Tool , owl:NamedIndividual ;
        rdfs:comment  "Jacks is a long pair of shears used to cut heated glass."@en ;
        rdfs:label    "Jacks"@en ;
        :Used-For     :ARTWORK_43_ApplyingClearGlassBell , :ARTWORK_75_ApplyingExtraColour_2 , :ARTWORK_78_ApplyingExtraColour , :ARTWORK_79_ApplyingExtraColour_2 , :ARTWORK_44_ApplyingExtraColour_2 , :ARTWORK_76_Glassblowing , :ARTWORK_74_ExaminingTheQualityOfTheGlass , :ARTWORK_76_ApplyingExtraColour , :ARTWORK_80_ApplyingClearGlassBell , :ARTWORK_77_ApplyingExtraColour , :ARTWORK_43_ApplyingExtraColour , :ARTWORK_78_Glassblowing , :ARTWORK_79_ExaminingTheQualityOfTheGlass , :ARTWORK_73_Glassblowing , :ARTWORK_44_ExaminingTheQualityOfTheGlass , :ARTWORK_75_ExaminingTheQualityOfTheGlass , :ARTWORK_78_ApplyingClearGlassBell , :ARTWORK_75_ApplyingClearGlassBell , :ARTWORK_74_ApplyingExtraColour , :ARTWORK_74_ApplyingClearGlassBell , :ARTWORK_76_ExaminingTheQualityOfTheGlass , :ARTWORK_74_Glassblowing , :ARTWORK_43_ExaminingTheQualityOfTheGlass , :ARTWORK_80_Glassblowing , :ARTWORK_44_ApplyingExtraColour , :ARTWORK_44_Glassblowing , :ARTWORK_77_ApplyingClearGlassBell , :ARTWORK_76_ApplyingClearGlassBell , :ARTWORK_75_Glassblowing , :ARTWORK_80_ExaminingTheQualityOfTheGlass , :ARTWORK_74_ApplyingExtraColour_2 , :ARTWORK_73_ApplyingClearGlassBell , :ARTWORK_80_ApplyingExtraColour , :ARTWORK_79_ApplyingClearGlassBell , :ARTWORK_73_ExaminingTheQualityOfTheGlass , :ARTWORK_79_ApplyingExtraColour , :ARTWORK_77_ExaminingTheQualityOfTheGlass , :ARTWORK_77_Glassblowing , :ARTWORK_78_ExaminingTheQualityOfTheGlass , :ARTWORK_79_Glassblowing , :ARTWORK_43_Glassblowing , :ARTWORK_76_ApplyingExtraColour_2 , :ARTWORK_44_ApplyingClearGlassBell , :ARTWORK_75_ApplyingExtraColour .

:Availability  a      owl:DatatypeProperty ;
        rdfs:comment  "Availability is a property of materials with two options; Orderable and Available as Standard." ;
        rdfs:domain   :Material ;
        rdfs:label    "Availability"@en ;
        rdfs:range    xsd:string .

<http://vocab.getty.edu/aat/300053789>
        a                    owl:Class ;
        owl:equivalentClass  :Gilding .

:BullseyeGlass  a             :Glass , owl:NamedIndividual ;
        rdfs:comment          "Bullseye Glass is a type of art glass mainly used for fusing."@en ;
        rdfs:label            "Bullseye Glass"@en ;
        owl:sameAs            <http://vocab.getty.edu/aat/300263720> ;
        :Is-Processed-During  :ARTWORK_18_64_DecidingColourPaletteAndPatterns , :ARTWORK_39_DecidingColourPalette , :ARTWORK_46_DecidingColourPaletteAndPatterns , :ARTWORK_36_DecidingColourPaletteAndPatterns ;
        :Is-Processed-In      :Artwork_36 , :Artwork_18_64 , :Artwork_46 , :Artwork_39 .

<http://www.wikidata.org/entity/Q25245>
        a       owl:NamedIndividual .

<http://www.semanticweb.org/ontologies/Daan/2020/BarbaraNanning#2002UpToPresentDay>
        a             owl:NamedIndividual , :Timespan ;
        rdfs:comment  "2002 up to Present Day is a Timespan."@en ;
        rdfs:label    "2002 up to Present Day"@en ;
        :Duration-Of  :GlassVerreÉglomisé .

:ARTWORK_74_Documenting
        a              owl:NamedIndividual , :Documenting ;
        rdfs:comment   "Instance of an activity which is part of the creation process of ARTWORK_74."@en ;
        rdfs:label     "ARTWORK_74_Documenting"@en ;
        :Followed-By   :ARTWORK_74_Packing_5 ;
        :Follows       :ARTWORK_74_Photographing ;
        :Has-Duration  <http://www.semanticweb.org/ontologies/Daan/2020/BarbaraNanning#2008> ;
        :Involves      :BarbaraNanning ;
        :Located-In    :CzechRepublic ;
        :Part-Of       :Creation_Artwork_74 .

<http://www.wikidata.org/entity/Q25291>
        a       owl:NamedIndividual .

<http://www.semanticweb.org/ontologies/Daan/2020/BarbaraNanning#ARTWORK_73_ExaminingQuality(Result)>
        a              j.0: , owl:NamedIndividual ;
        rdfs:comment   "Instance of an activity which is part of the creation process of ARTWORK_73."@en ;
        rdfs:label     "ARTWORK_73_Examining Quality (Result)"@en ;
        :Followed-By   :ARTWORK_73_MeasuringAndBoxesMaking ;
        :Follows       :ARTWORK_73_Polishing ;
        :Has-Duration  <http://www.semanticweb.org/ontologies/Daan/2020/BarbaraNanning#2018> ;
        :Involves      :BarbaraNanning , :AlešZvěřina ;
        :Located-In    :CzechRepublic ;
        :Part-Of       :Creation_Artwork_73 .

:Cutting_Monochrome_Sheets
        a                owl:Class ;
        rdfs:comment     "A cutter cuts the galss sheets with the help of Diamond scissor or Diamond saw."@en ;
        rdfs:label       "Cutting Monochrome Sheets"@en ;
        rdfs:subClassOf  :Activity .

:Applying_Clear_Glass_Bell
        a                owl:Class ;
        rdfs:comment     "Applying Clear Glass Bell is an activity in which a bell of glass is applied to a thing. The clear glass is always tested beforehand."@en ;
        rdfs:label       "Applying Clear Glass Bell"@en ;
        rdfs:subClassOf  :Activity .
